<rdf:RDF
    xmlns:dct="http://purl.org/dc/terms/"
    xmlns:rdf="http://www.w3.org/1999/02/22-rdf-syntax-ns#"
    xmlns:dc="http://purl.org/dc/elements/1.1/"
    xmlns:owl="http://www.w3.org/2002/07/owl#"
    xmlns:dcmit="http://purl.org/dc/dcmitype/"
    xmlns:skos="http://www.w3.org/2004/02/skos/core#"
    xmlns:voaf="http://purl.org/vocommons/voaf#"
    xmlns:rdfs="http://www.w3.org/2000/01/rdf-schema#"
    xmlns:vann="http://purl.org/vocab/vann/">
  <skos:Concept rdf:about="http://www.ebusiness-unibw.org/ontologies/consumerelectronics/v1#HDTV_720p">
    <rdfs:label xml:lang="de">HDTV 720p</rdfs:label>
    <rdfs:label xml:lang="en">HDTV 720p</rdfs:label>
    <rdfs:comment xml:lang="en">720p is the shorthand name for a category of HDTV video modes. The number 720 stands for the 720 vertical scan lines of display resolution (also known as 720 pixels of vertical resolution), while the letter p stands for progressive scan or non-interlaced.

(This description is partly based on or reuses content from the Wikipedia article "720p" (http://en.wikipedia.org/wiki/720p) and is licensed under the GNU Free Documentation License (http://www.gnu.org/copyleft/fdl.html).)</rdfs:comment>
    <skos:inScheme>
      <skos:ConceptScheme rdf:about="http://www.ebusiness-unibw.org/ontologies/consumerelectronics/v1#TVDisplayResolution"/>
    </skos:inScheme>
  </skos:Concept>
  <skos:Concept rdf:about="http://www.ebusiness-unibw.org/ontologies/consumerelectronics/v1#SDTV_576i">
    <rdfs:label xml:lang="de">SDTV 576i</rdfs:label>
    <rdfs:label xml:lang="en">SDTV 576i</rdfs:label>
    <rdfs:comment xml:lang="en">576i is a standard-definition video mode used in (former) PAL and SECAM countries. In digital applications it's usually referred to as "576i", in analogue contexts it's often quoted as "625 lines". The 576 identifies a vertical resolution of 576 lines (usually with a horizontal resolution of 720 or 704 pixels), and the i identifies it as an interlaced resolution.

(This description is partly based on or reuses content from the Wikipedia article "576ii" (http://en.wikipedia.org/wiki/576i) and is licensed under the GNU Free Documentation License (http://www.gnu.org/copyleft/fdl.html).)</rdfs:comment>
    <skos:inScheme rdf:resource="http://www.ebusiness-unibw.org/ontologies/consumerelectronics/v1#TVDisplayResolution"/>
  </skos:Concept>
  <skos:Concept rdf:about="http://www.ebusiness-unibw.org/ontologies/consumerelectronics/v1#EDTV_480p">
    <rdfs:label xml:lang="en">EDTV 480p</rdfs:label>
    <rdfs:label xml:lang="de">EDTV 480p</rdfs:label>
    <rdfs:comment xml:lang="en">480p is the shorthand name for a video display resolution. The p stands for progressive scan, i.e. non-interlaced. The 480 denotes a vertical resolution of 480 vertically scanning lines, usually with a horizontal resolution of 640 pixels and 4:3 aspect ratio or a horizontal resolution of 854 pixels and 16:9 aspect ratio.

(This description is partly based on or reuses content from the Wikipedia article "480p" (http://en.wikipedia.org/wiki/480p) and is licensed under the GNU Free Documentation License (http://www.gnu.org/copyleft/fdl.html).)</rdfs:comment>
    <skos:inScheme rdf:resource="http://www.ebusiness-unibw.org/ontologies/consumerelectronics/v1#TVDisplayResolution"/>
  </skos:Concept>
  <skos:Concept rdf:about="http://www.ebusiness-unibw.org/ontologies/consumerelectronics/v1#SDTV_480i">
    <rdfs:label xml:lang="en">SDTV 480i</rdfs:label>
    <rdfs:label xml:lang="de">SDTV 480i</rdfs:label>
    <rdfs:comment xml:lang="en">480i is the shorthand name for a video mode, namely the U.S. NTSC television system or digital television systems with the same characteristics. The i, which is sometimes uppercase, stands for interlaced, the 480 for a vertical frame resolution of 480 lines containing picture information; while NTSC has a total of 525 lines, only 480 of these are used to display the image.

(This description is partly based on or reuses content from the Wikipedia article "480i" (http://en.wikipedia.org/wiki/480i) and is licensed under the GNU Free Documentation License (http://www.gnu.org/copyleft/fdl.html).)</rdfs:comment>
    <skos:inScheme rdf:resource="http://www.ebusiness-unibw.org/ontologies/consumerelectronics/v1#TVDisplayResolution"/>
  </skos:Concept>
  <skos:Concept rdf:about="http://www.ebusiness-unibw.org/ontologies/consumerelectronics/v1#HDTV_1080i">
    <rdfs:label xml:lang="en">HDTV 1080i</rdfs:label>
    <rdfs:label xml:lang="de">HDTV 1080i</rdfs:label>
    <rdfs:comment xml:lang="en">1080i is the shorthand name of a format of high-definition video modes. 1080 denotes the number of horizontal scan lines - also known as vertical resolution - and the letter i stands for interlaced.

(This description is partly based on or reuses content from the Wikipedia article "1080i" (http://en.wikipedia.org/wiki/1080i) and is licensed under the GNU Free Documentation License (http://www.gnu.org/copyleft/fdl.html).)</rdfs:comment>
    <skos:inScheme rdf:resource="http://www.ebusiness-unibw.org/ontologies/consumerelectronics/v1#TVDisplayResolution"/>
  </skos:Concept>
  <skos:Concept rdf:about="http://www.ebusiness-unibw.org/ontologies/consumerelectronics/v1#HDTV_1080p">
    <rdfs:label xml:lang="en">HDTV 1080p</rdfs:label>
    <rdfs:label xml:lang="de">HDTV 1080p</rdfs:label>
    <rdfs:comment xml:lang="en">1080p is the shorthand name for a category of HDTV video modes. The number "1080" represents 1,080 lines of vertical resolution (1080 horizontal scan lines), while the letter p stands for progressive scan (meaning the image is not interlaced). 1080p can be referred to as full HD or full high definition to differentiate it from other HDTV video modes.

(This description is partly based on or reuses content from the Wikipedia article "1080p" (http://en.wikipedia.org/wiki/1080p) and is licensed under the GNU Free Documentation License (http://www.gnu.org/copyleft/fdl.html).)</rdfs:comment>
    <skos:inScheme rdf:resource="http://www.ebusiness-unibw.org/ontologies/consumerelectronics/v1#TVDisplayResolution"/>
  </skos:Concept>
</rdf:RDF>
