<rdf:RDF
    xmlns:rdf="http://www.w3.org/1999/02/22-rdf-syntax-ns#"
    xmlns:dcterms="http://purl.org/dc/terms/"
    xmlns:dc="http://purl.org/dc/elements/1.1/"
    xmlns:owl="http://www.w3.org/2002/07/owl#"
    xmlns:dcmit="http://purl.org/dc/dcmitype/"
    xmlns:skos="http://www.w3.org/2004/02/skos/core#"
    xmlns:voaf="http://purl.org/vocommons/voaf#"
    xmlns:rdfs="http://www.w3.org/2000/01/rdf-schema#"
    xmlns:vann="http://purl.org/vocab/vann/">
  <owl:Ontology rdf:about="http://www.ebusiness-unibw.org/ontologies/consumerelectronics/v1"/>
  <owl:ObjectProperty rdf:about="http://www.ebusiness-unibw.org/ontologies/consumerelectronics/v1#hasDataInterfaceType">
    <rdfs:comment xml:lang="en">Defines the type of interfaces used to exchange data.</rdfs:comment>
    <rdfs:label xml:lang="en">data interface type</rdfs:label>
    <rdfs:range>
      <skos:ConceptScheme rdf:about="http://www.ebusiness-unibw.org/ontologies/consumerelectronics/v1#DataInterfaceType">
        <rdfs:isDefinedBy rdf:resource="http://www.ebusiness-unibw.org/ontologies/consumerelectronics/v1"/>
        <rdfs:label xml:lang="en">Data Interface Type</rdfs:label>
        <rdfs:comment xml:lang="en">Interface generally refers to an abstraction that an entity provides of itself to the outside.

(This description is partly based on or reuses content from the Wikipedia article "Interface (computer science)" (http://en.wikipedia.org/wiki/Interface_(computer_science)) and is licensed under the GNU Free Documentation License (http://www.gnu.org/copyleft/fdl.html).)</rdfs:comment>
      </skos:ConceptScheme>
    </rdfs:range>
  </owl:ObjectProperty>
  <skos:Concept rdf:about="http://www.ebusiness-unibw.org/ontologies/consumerelectronics/v1#Infrared">
    <rdfs:isDefinedBy rdf:resource="http://www.ebusiness-unibw.org/ontologies/consumerelectronics/v1"/>
    <rdfs:label xml:lang="en">Infrared</rdfs:label>
    <rdfs:comment xml:lang="en">Infrared (IR) radiation is electromagnetic radiation whose wavelength is longer than that of visible light, but shorter than that of terahertz radiation and microwaves.

(This description is partly based on or reuses content from the Wikipedia article "Infrared" (http://en.wikipedia.org/wiki/Infrared) and is licensed under the GNU Free Documentation License (http://www.gnu.org/copyleft/fdl.html).)</rdfs:comment>
    <skos:inScheme rdf:resource="http://www.ebusiness-unibw.org/ontologies/consumerelectronics/v1#DataInterfaceType"/>
  </skos:Concept>
  <skos:Concept rdf:about="http://www.ebusiness-unibw.org/ontologies/consumerelectronics/v1#IEEE_802.11">
    <rdfs:isDefinedBy rdf:resource="http://www.ebusiness-unibw.org/ontologies/consumerelectronics/v1"/>
    <rdfs:label xml:lang="en">IEEE 802.11</rdfs:label>
    <rdfs:comment xml:lang="en">IEEE 802.11 is a set of standards for wireless local area network (WLAN) computer communication, developed by the IEEE LAN/MAN Standards Committee (IEEE 802) in the 5 GHz and 2.4 GHz public spectrum bands.

(This description is partly based on or reuses content from the Wikipedia article "802.11" (http://en.wikipedia.org/wiki/802.11) and is licensed under the GNU Free Documentation License (http://www.gnu.org/copyleft/fdl.html).)</rdfs:comment>
    <skos:inScheme rdf:resource="http://www.ebusiness-unibw.org/ontologies/consumerelectronics/v1#DataInterfaceType"/>
  </skos:Concept>
  <skos:Concept rdf:about="http://www.ebusiness-unibw.org/ontologies/consumerelectronics/v1#USB2.0">
    <rdfs:isDefinedBy rdf:resource="http://www.ebusiness-unibw.org/ontologies/consumerelectronics/v1"/>
    <rdfs:label xml:lang="en">USB 2.0</rdfs:label>
    <rdfs:comment xml:lang="en">Maximum speed of 480 Mbit/s.</rdfs:comment>
    <skos:inScheme rdf:resource="http://www.ebusiness-unibw.org/ontologies/consumerelectronics/v1#DataInterfaceType"/>
  </skos:Concept>
  <skos:Concept rdf:about="http://www.ebusiness-unibw.org/ontologies/consumerelectronics/v1#USB3.0">
    <rdfs:isDefinedBy rdf:resource="http://www.ebusiness-unibw.org/ontologies/consumerelectronics/v1"/>
    <rdfs:label xml:lang="en">USB 3.0</rdfs:label>
    <rdfs:comment xml:lang="en">Maximum speed of 4,8 Gbit/s.</rdfs:comment>
    <skos:inScheme rdf:resource="http://www.ebusiness-unibw.org/ontologies/consumerelectronics/v1#DataInterfaceType"/>
  </skos:Concept>
  <skos:Concept rdf:about="http://www.ebusiness-unibw.org/ontologies/consumerelectronics/v1#USB1.0">
    <rdfs:isDefinedBy rdf:resource="http://www.ebusiness-unibw.org/ontologies/consumerelectronics/v1"/>
    <rdfs:label xml:lang="en">USB 1.0</rdfs:label>
    <rdfs:comment xml:lang="en">Specified data rates of 1.5 Mbit/s and 12 Mbit/s.</rdfs:comment>
    <skos:inScheme rdf:resource="http://www.ebusiness-unibw.org/ontologies/consumerelectronics/v1#DataInterfaceType"/>
  </skos:Concept>
  <skos:Concept rdf:about="http://www.ebusiness-unibw.org/ontologies/consumerelectronics/v1#IEEE_1394">
    <rdfs:isDefinedBy rdf:resource="http://www.ebusiness-unibw.org/ontologies/consumerelectronics/v1"/>
    <rdfs:label xml:lang="en">IEEE_1394</rdfs:label>
    <rdfs:comment xml:lang="en">The IEEE 1394 interface is a serial bus interface standard for high-speed communications and isochronous real-time data transfer, frequently used by personal computers, as well as in digital audio, digital video, automotive, and aeronautics applications.  

(This description is partly based on or reuses content from the Wikipedia article "firewire" (http://en.wikipedia.org/wiki/FireWire) and is licensed under the GNU Free Documentation License (http://www.gnu.org/copyleft/fdl.html).)</rdfs:comment>
    <skos:inScheme rdf:resource="http://www.ebusiness-unibw.org/ontologies/consumerelectronics/v1#DataInterfaceType"/>
  </skos:Concept>
  <skos:Concept rdf:about="http://www.ebusiness-unibw.org/ontologies/consumerelectronics/v1#DVI_in">
    <rdfs:isDefinedBy rdf:resource="http://www.ebusiness-unibw.org/ontologies/consumerelectronics/v1"/>
    <rdfs:label xml:lang="en">DV in</rdfs:label>
    <rdfs:comment xml:lang="en">A digital video format created by Sony, JVC, Panasonic and other video camera producers.</rdfs:comment>
    <skos:inScheme rdf:resource="http://www.ebusiness-unibw.org/ontologies/consumerelectronics/v1#DataInterfaceType"/>
  </skos:Concept>
  <skos:Concept rdf:about="http://www.ebusiness-unibw.org/ontologies/consumerelectronics/v1#S-Video_in">
    <rdfs:isDefinedBy rdf:resource="http://www.ebusiness-unibw.org/ontologies/consumerelectronics/v1"/>
    <rdfs:label xml:lang="en">S-Video in</rdfs:label>
    <rdfs:comment xml:lang="en">Is an analog video signal that carries the video data as two separate signals, lumen (luminance) and chroma (color).

(This description is partly based on or reuses content from the Wikipedia article "S-Video" (http://en.wikipedia.org/wiki/S-Video) and is licensed under the GNU Free Documentation License (http://www.gnu.org/copyleft/fdl.html).)</rdfs:comment>
    <skos:inScheme rdf:resource="http://www.ebusiness-unibw.org/ontologies/consumerelectronics/v1#DataInterfaceType"/>
  </skos:Concept>
  <skos:Concept rdf:about="http://www.ebusiness-unibw.org/ontologies/consumerelectronics/v1#MiniUSB">
    <rdfs:label rdf:datatype="http://www.w3.org/2001/XMLSchema#string"
    >Mini USB</rdfs:label>
    <rdfs:isDefinedBy rdf:resource="http://www.ebusiness-unibw.org/ontologies/consumerelectronics/v1"/>
    <rdfs:label xml:lang="en">Mini USB</rdfs:label>
    <rdfs:comment xml:lang="en">The non-standard Mini-USB's, official Mini-B, Micro-A, and Micro-B connectors are used for smaller devices such as PDAs, mobile phones or digital cameras. The Standard-A plug is approximately 4 by 12 mm, the Standard-B approximately 7 by 8 mm, and the Mini-A and Mini-B plugs approximately 2 by 7 mm.

(This description is partly based on or reuses content from the Wikipedia article "Universial Serial Bus" (http://en.wikipedia.org/wiki/Universal_Serial_Bus) and is licensed under the GNU Free Documentation License (http://www.gnu.org/copyleft/fdl.html).)</rdfs:comment>
    <skos:inScheme rdf:resource="http://www.ebusiness-unibw.org/ontologies/consumerelectronics/v1#DataInterfaceType"/>
  </skos:Concept>
  <skos:Concept rdf:about="http://www.ebusiness-unibw.org/ontologies/consumerelectronics/v1#S-Video_out">
    <rdfs:isDefinedBy rdf:resource="http://www.ebusiness-unibw.org/ontologies/consumerelectronics/v1"/>
    <rdfs:label xml:lang="en">S-Video out</rdfs:label>
    <rdfs:comment xml:lang="en">Is an analog video signal that carries the video data as two separate signals, lumen (luminance) and chroma (color).

(This description is partly based on or reuses content from the Wikipedia article "S-Video" (http://en.wikipedia.org/wiki/S-Video) and is licensed under the GNU Free Documentation License (http://www.gnu.org/copyleft/fdl.html).)</rdfs:comment>
    <skos:inScheme rdf:resource="http://www.ebusiness-unibw.org/ontologies/consumerelectronics/v1#DataInterfaceType"/>
  </skos:Concept>
  <skos:Concept rdf:about="http://www.ebusiness-unibw.org/ontologies/consumerelectronics/v1#DVI_out">
    <rdfs:isDefinedBy rdf:resource="http://www.ebusiness-unibw.org/ontologies/consumerelectronics/v1"/>
    <rdfs:label xml:lang="en">DVI out</rdfs:label>
    <rdfs:comment xml:lang="en">A digital video format created by Sony, JVC, Panasonic and other video camera producers.</rdfs:comment>
    <skos:inScheme rdf:resource="http://www.ebusiness-unibw.org/ontologies/consumerelectronics/v1#DataInterfaceType"/>
  </skos:Concept>
  <skos:Concept rdf:about="http://www.ebusiness-unibw.org/ontologies/consumerelectronics/v1#Bluetooth">
    <rdfs:isDefinedBy rdf:resource="http://www.ebusiness-unibw.org/ontologies/consumerelectronics/v1"/>
    <rdfs:label xml:lang="en">Bluetooth</rdfs:label>
    <rdfs:comment xml:lang="en">Bluetooth is a wireless protocol utilizing short-range communications technology facilitating data transmission over short distances from fixed and mobile devices, creating wireless personal area networks.</rdfs:comment>
    <skos:inScheme rdf:resource="http://www.ebusiness-unibw.org/ontologies/consumerelectronics/v1#DataInterfaceType"/>
  </skos:Concept>
  <skos:Concept rdf:about="http://www.ebusiness-unibw.org/ontologies/consumerelectronics/v1#PictBridge">
    <rdfs:isDefinedBy rdf:resource="http://www.ebusiness-unibw.org/ontologies/consumerelectronics/v1"/>
    <rdfs:label xml:lang="en">PictBridge</rdfs:label>
    <rdfs:comment xml:lang="en">Is an industry standard from the Camera &amp; Imaging Products Association (CIPA) for direct printing.</rdfs:comment>
    <skos:inScheme rdf:resource="http://www.ebusiness-unibw.org/ontologies/consumerelectronics/v1#DataInterfaceType"/>
  </skos:Concept>
  <skos:Concept rdf:about="http://www.ebusiness-unibw.org/ontologies/consumerelectronics/v1#HDMI_Interface">
    <rdfs:isDefinedBy rdf:resource="http://www.ebusiness-unibw.org/ontologies/consumerelectronics/v1"/>
    <rdfs:label xml:lang="en">HDMI interface</rdfs:label>
    <rdfs:comment xml:lang="en">HDMI (High-Definition Multimedia Interface) is a compact audio/video interface for transmitting uncompressed digital data.

(This description is partly based on or reuses content from the Wikipedia article "HDMI" (http://en.wikipedia.org/wiki/HDMI) and is licensed under the GNU Free Documentation License (http://www.gnu.org/copyleft/fdl.html).)</rdfs:comment>
    <skos:inScheme rdf:resource="http://www.ebusiness-unibw.org/ontologies/consumerelectronics/v1#DataInterfaceType"/>
  </skos:Concept>
</rdf:RDF>
