<rdf:RDF
    xmlns:rdf="http://www.w3.org/1999/02/22-rdf-syntax-ns#"
    xmlns:dcterms="http://purl.org/dc/terms/"
    xmlns:dc="http://purl.org/dc/elements/1.1/"
    xmlns:owl="http://www.w3.org/2002/07/owl#"
    xmlns:dcmit="http://purl.org/dc/dcmitype/"
    xmlns:skos="http://www.w3.org/2004/02/skos/core#"
    xmlns:voaf="http://purl.org/vocommons/voaf#"
    xmlns:rdfs="http://www.w3.org/2000/01/rdf-schema#"
    xmlns:vann="http://purl.org/vocab/vann/">
  <owl:Ontology rdf:about="https://w3id.org/arco/ontology/context-description"/>
  <owl:ObjectProperty rdf:about="https://w3id.org/arco/ontology/context-description/hasUseTypeSpecification">
    <rdfs:comment xml:lang="en">This property relates the use of a cultural property to the specification of the type of use.</rdfs:comment>
    <rdfs:label xml:lang="en">has use type specification</rdfs:label>
    <rdfs:domain rdf:resource="https://w3id.org/arco/ontology/context-description/Use"/>
    <rdfs:range>
      <skos:ConceptScheme rdf:about="https://w3id.org/arco/ontology/context-description/UseTypeSpecification">
        <rdfs:isDefinedBy rdf:resource="https://w3id.org/arco/ontology/context-description"/>
        <rdfs:label xml:lang="en">Use type specification</rdfs:label>
        <rdfs:comment xml:lang="en">This class represents the specification of the type of use of a cultural property (e.g. building, ornamental, structural, instrumental)</rdfs:comment>
      </skos:ConceptScheme>
    </rdfs:range>
  </owl:ObjectProperty>
  <skos:Concept rdf:about="https://w3id.org/arco/ontology/context-description/BuildingUse">
    <rdfs:isDefinedBy rdf:resource="https://w3id.org/arco/ontology/context-description"/>
    <rdfs:label xml:lang="en">Building use</rdfs:label>
    <rdfs:comment xml:lang="en">This individual represents cultural entity  building use specifications.</rdfs:comment>
    <skos:inScheme rdf:resource="https://w3id.org/arco/ontology/context-description/UseTypeSpecification"/>
  </skos:Concept>
  <skos:Concept rdf:about="https://w3id.org/arco/ontology/context-description/OrnamentalUse">
    <rdfs:isDefinedBy rdf:resource="https://w3id.org/arco/ontology/context-description"/>
    <rdfs:label xml:lang="en">Ornamental</rdfs:label>
    <rdfs:comment xml:lang="en">This individual represents cultural entity's ornamental use specifications.</rdfs:comment>
    <skos:inScheme rdf:resource="https://w3id.org/arco/ontology/context-description/UseTypeSpecification"/>
  </skos:Concept>
  <skos:Concept rdf:about="https://w3id.org/arco/ontology/context-description/StructuralUse">
    <rdfs:isDefinedBy rdf:resource="https://w3id.org/arco/ontology/context-description"/>
    <rdfs:label xml:lang="en">Structural use</rdfs:label>
    <rdfs:comment xml:lang="en">This individual represents cultural entity's structural use specifications.</rdfs:comment>
    <skos:inScheme rdf:resource="https://w3id.org/arco/ontology/context-description/UseTypeSpecification"/>
  </skos:Concept>
  <skos:Concept rdf:about="https://w3id.org/arco/ontology/context-description/Reuse">
    <rdfs:comment xml:lang="en">This class represents cultural entity's reuse.</rdfs:comment>
    <rdfs:isDefinedBy rdf:resource="https://w3id.org/arco/ontology/context-description"/>
    <rdfs:label xml:lang="en">Reuse</rdfs:label>
    <rdfs:comment xml:lang="en">This class represents the reuse of a cultural property or of one of its parts.</rdfs:comment>
    <skos:inScheme rdf:resource="https://w3id.org/arco/ontology/context-description/UseTypeSpecification"/>
  </skos:Concept>
  <skos:Concept rdf:about="https://w3id.org/arco/ontology/context-description/EpigraphicUse">
    <rdfs:isDefinedBy rdf:resource="https://w3id.org/arco/ontology/context-description"/>
    <rdfs:label xml:lang="en">Epigraphic</rdfs:label>
    <rdfs:comment xml:lang="en">This individual represents cultural entity's epigraphic use.</rdfs:comment>
    <skos:inScheme rdf:resource="https://w3id.org/arco/ontology/context-description/UseTypeSpecification"/>
  </skos:Concept>
  <skos:Concept rdf:about="https://w3id.org/arco/ontology/context-description/InstrumentalUse">
    <rdfs:isDefinedBy rdf:resource="https://w3id.org/arco/ontology/context-description"/>
    <rdfs:label xml:lang="en">Instrumental</rdfs:label>
    <rdfs:comment xml:lang="en">This individual represents cultural entity instrumental use specifications.</rdfs:comment>
    <skos:inScheme rdf:resource="https://w3id.org/arco/ontology/context-description/UseTypeSpecification"/>
  </skos:Concept>
</rdf:RDF>
