<rdf:RDF
    xmlns:rdf="http://www.w3.org/1999/02/22-rdf-syntax-ns#"
    xmlns:dcterms="http://purl.org/dc/terms/"
    xmlns:dc="http://purl.org/dc/elements/1.1/"
    xmlns:owl="http://www.w3.org/2002/07/owl#"
    xmlns:dcmit="http://purl.org/dc/dcmitype/"
    xmlns:skos="http://www.w3.org/2004/02/skos/core#"
    xmlns:voaf="http://purl.org/vocommons/voaf#"
    xmlns:rdfs="http://www.w3.org/2000/01/rdf-schema#"
    xmlns:vann="http://purl.org/vocab/vann/">
  <owl:Ontology rdf:about="http://vocab.org/transit/terms/"/>
  <rdf:Property rdf:about="http://vocab.org/transit/terms/pickup">
    <rdf:type rdf:resource="http://www.w3.org/2002/07/owl#ObjectProperty"/>
    <rdfs:comment xml:lang="en">The arrangement required for passengers to be picked up at this service stop.</rdfs:comment>
    <rdfs:label xml:lang="en">Pick Up</rdfs:label>
    <rdfs:domain rdf:resource="http://vocab.org/transit/terms/ServiceStop"/>
    <rdfs:range>
      <skos:ConceptScheme rdf:about="http://vocab.org/transit/terms/AccessArrangement">
        <rdfs:isDefinedBy rdf:resource="http://vocab.org/transit/terms/"/>
        <rdfs:label xml:lang="en">Access Arrangement</rdfs:label>
        <rdfs:comment xml:lang="en">A type of arrangement for picking up or dropping off passengers from a service stop.</rdfs:comment>
      </skos:ConceptScheme>
    </rdfs:range>
  </rdf:Property>
  <rdf:Property rdf:about="http://vocab.org/transit/terms/dropoff">
    <rdf:type rdf:resource="http://www.w3.org/2002/07/owl#ObjectProperty"/>
    <rdfs:comment xml:lang="en">The arrangement required for passengers to be dropped off at this service stop.</rdfs:comment>
    <rdfs:label xml:lang="en">Drop Off</rdfs:label>
    <rdfs:domain rdf:resource="http://vocab.org/transit/terms/ServiceStop"/>
    <rdfs:range rdf:resource="http://vocab.org/transit/terms/AccessArrangement"/>
  </rdf:Property>
  <skos:Concept rdf:about="http://vocab.org/transit/terms/prearranged">
    <rdfs:isDefinedBy rdf:resource="http://vocab.org/transit/terms/"/>
    <rdfs:label xml:lang="en">Pre-arranged</rdfs:label>
    <rdfs:comment xml:lang="en">The particular form of access must be pre-arranged with the transit agency.</rdfs:comment>
    <skos:inScheme rdf:resource="http://vocab.org/transit/terms/AccessArrangement"/>
  </skos:Concept>
  <skos:Concept rdf:about="http://vocab.org/transit/terms/standard">
    <rdfs:isDefinedBy rdf:resource="http://vocab.org/transit/terms/"/>
    <rdfs:label xml:lang="en">Standard</rdfs:label>
    <rdfs:comment xml:lang="en">The particular form of access has no special arrangement.</rdfs:comment>
    <skos:inScheme rdf:resource="http://vocab.org/transit/terms/AccessArrangement"/>
  </skos:Concept>
  <skos:Concept rdf:about="http://vocab.org/transit/terms/disallowed">
    <rdfs:isDefinedBy rdf:resource="http://vocab.org/transit/terms/"/>
    <rdfs:label xml:lang="en">Disallowed</rdfs:label>
    <rdfs:comment xml:lang="en">The particular form of access is unavailable.</rdfs:comment>
    <skos:inScheme rdf:resource="http://vocab.org/transit/terms/AccessArrangement"/>
  </skos:Concept>
  <skos:Concept rdf:about="http://vocab.org/transit/terms/coordinated">
    <rdfs:isDefinedBy rdf:resource="http://vocab.org/transit/terms/"/>
    <rdfs:label xml:lang="en">Coordinated</rdfs:label>
    <rdfs:comment xml:lang="en">The particular form of access must be coordinated with the driver.</rdfs:comment>
    <skos:inScheme rdf:resource="http://vocab.org/transit/terms/AccessArrangement"/>
  </skos:Concept>
</rdf:RDF>
