<rdf:RDF
    xmlns:rdf="http://www.w3.org/1999/02/22-rdf-syntax-ns#"
    xmlns:dcterms="http://purl.org/dc/terms/"
    xmlns:dc="http://purl.org/dc/elements/1.1/"
    xmlns:owl="http://www.w3.org/2002/07/owl#"
    xmlns:dcmit="http://purl.org/dc/dcmitype/"
    xmlns:skos="http://www.w3.org/2004/02/skos/core#"
    xmlns:voaf="http://purl.org/vocommons/voaf#"
    xmlns:rdfs="http://www.w3.org/2000/01/rdf-schema#"
    xmlns:vann="http://purl.org/vocab/vann/">
  <owl:Ontology rdf:about="https://saref.etsi.org/saref4agri/"/>
  <skos:Concept rdf:about="https://saref.etsi.org/saref4agri/Precipitation">
    <rdfs:isDefinedBy rdf:resource="https://saref.etsi.org/saref4agri/"/>
    <rdfs:label xml:lang="en">Precipitation</rdfs:label>
    <rdfs:comment xml:lang="en">The amount of water falling in the soil by natural process (e.g. rain).</rdfs:comment>
    <skos:inScheme>
      <skos:ConceptScheme rdf:about="https://saref.etsi.org/core/Property">
        <rdfs:comment xml:lang="en">Anything that can be sensed, measured or controlled in households, common public buildings or offices. We propose here a list of properties that are relevant for the purpose of SAREF, but this list can be extended.</rdfs:comment>
        <rdfs:isDefinedBy rdf:resource="https://saref.etsi.org/saref4agri/"/>
        <rdfs:label xml:lang="en">Property</rdfs:label>
        <rdfs:comment xml:lang="en">An aspect of an entity that can be observable by a sensor.</rdfs:comment>
      </skos:ConceptScheme>
    </skos:inScheme>
  </skos:Concept>
  <skos:Concept rdf:about="https://saref.etsi.org/saref4agri/SoilMoisture">
    <rdfs:isDefinedBy rdf:resource="https://saref.etsi.org/saref4agri/"/>
    <rdfs:label xml:lang="en">Soil moisture</rdfs:label>
    <rdfs:comment xml:lang="en">The amount of water or humidity contained in the soil.</rdfs:comment>
    <skos:inScheme rdf:resource="https://saref.etsi.org/core/Property"/>
  </skos:Concept>
  <skos:Concept rdf:about="https://saref.etsi.org/saref4agri/PlantGrowthStage">
    <rdfs:isDefinedBy rdf:resource="https://saref.etsi.org/saref4agri/"/>
    <rdfs:label xml:lang="en">Plant growth stage</rdfs:label>
    <rdfs:comment xml:lang="en">The level or stage of growth of the plant.</rdfs:comment>
    <skos:inScheme rdf:resource="https://saref.etsi.org/core/Property"/>
  </skos:Concept>
  <skos:Concept rdf:about="https://saref.etsi.org/saref4agri/IrrigationWater">
    <rdfs:isDefinedBy rdf:resource="https://saref.etsi.org/saref4agri/"/>
    <rdfs:label xml:lang="en">Irrigation water</rdfs:label>
    <rdfs:comment xml:lang="en">The amount of water falling in the soil by irrigation methods.</rdfs:comment>
    <skos:inScheme rdf:resource="https://saref.etsi.org/core/Property"/>
  </skos:Concept>
</rdf:RDF>
