<rdf:RDF
    xmlns:rdf="http://www.w3.org/1999/02/22-rdf-syntax-ns#"
    xmlns:dcterms="http://purl.org/dc/terms/"
    xmlns:dc="http://purl.org/dc/elements/1.1/"
    xmlns:owl="http://www.w3.org/2002/07/owl#"
    xmlns:dcmit="http://purl.org/dc/dcmitype/"
    xmlns:skos="http://www.w3.org/2004/02/skos/core#"
    xmlns:voaf="http://purl.org/vocommons/voaf#"
    xmlns:rdfs="http://www.w3.org/2000/01/rdf-schema#"
    xmlns:vann="http://purl.org/vocab/vann/">
  <owl:Ontology rdf:about="https://w3id.org/timebank"/>
  <owl:ObjectProperty rdf:about="https://w3id.org/timebank#hasSkillLevel">
    <rdfs:comment>Describes the proficiency level of a skill.</rdfs:comment>
    <rdfs:label>has skill level</rdfs:label>
    <rdfs:domain rdf:resource="https://w3id.org/timebank#Skill"/>
    <rdfs:range>
      <skos:ConceptScheme rdf:about="https://w3id.org/timebank#Level">
        <rdfs:isDefinedBy rdf:resource="https://w3id.org/timebank"/>
        <rdfs:label>Level</rdfs:label>
        <rdfs:comment>The level can be low, medium, or high.</rdfs:comment>
      </skos:ConceptScheme>
    </rdfs:range>
  </owl:ObjectProperty>
  <owl:ObjectProperty rdf:about="https://w3id.org/timebank#hasSeverity">
    <rdfs:comment>Indicates the severity of a limitation.</rdfs:comment>
    <rdfs:label>has severity</rdfs:label>
    <rdfs:domain rdf:resource="https://w3id.org/timebank#Limitation"/>
    <rdfs:range rdf:resource="https://w3id.org/timebank#Level"/>
  </owl:ObjectProperty>
  <skos:Concept rdf:about="https://w3id.org/timebank#LevelHigh">
    <rdfs:isDefinedBy rdf:resource="https://w3id.org/timebank"/>
    <rdfs:label>Level: High</rdfs:label>
    <rdfs:comment>Used if a Limitation has a high severity or a Skill is on a high level.</rdfs:comment>
    <skos:inScheme rdf:resource="https://w3id.org/timebank#Level"/>
  </skos:Concept>
  <skos:Concept rdf:about="https://w3id.org/timebank#LevelLow">
    <rdfs:isDefinedBy rdf:resource="https://w3id.org/timebank"/>
    <rdfs:label>Level: Low</rdfs:label>
    <rdfs:comment>Used if a Limitation only has a low severity or a Skill is on a low level.</rdfs:comment>
    <skos:inScheme rdf:resource="https://w3id.org/timebank#Level"/>
  </skos:Concept>
  <skos:Concept rdf:about="https://w3id.org/timebank#LevelMedium">
    <rdfs:isDefinedBy rdf:resource="https://w3id.org/timebank"/>
    <rdfs:label>Level: Medium</rdfs:label>
    <rdfs:comment>Used if a Limitation has a medium severity or a Skill is on a medium level</rdfs:comment>
    <skos:inScheme rdf:resource="https://w3id.org/timebank#Level"/>
  </skos:Concept>
</rdf:RDF>
