<rdf:RDF
    xmlns:rdf="http://www.w3.org/1999/02/22-rdf-syntax-ns#"
    xmlns:dcterms="http://purl.org/dc/terms/"
    xmlns:dc="http://purl.org/dc/elements/1.1/"
    xmlns:owl="http://www.w3.org/2002/07/owl#"
    xmlns:dcmit="http://purl.org/dc/dcmitype/"
    xmlns:skos="http://www.w3.org/2004/02/skos/core#"
    xmlns:voaf="http://purl.org/vocommons/voaf#"
    xmlns:rdfs="http://www.w3.org/2000/01/rdf-schema#"
    xmlns:vann="http://purl.org/vocab/vann/">
  <owl:Ontology rdf:about="http://www.ebusiness-unibw.org/ontologies/consumerelectronics/v1"/>
  <skos:Concept rdf:about="http://www.ebusiness-unibw.org/ontologies/consumerelectronics/v1#SVG">
    <rdfs:isDefinedBy rdf:resource="http://www.ebusiness-unibw.org/ontologies/consumerelectronics/v1"/>
    <rdfs:label xml:lang="en">SVG</rdfs:label>
    <rdfs:comment xml:lang="en">SVG (Scalable Vector Graphics) is an open standard created and developed by the World Wide Web Consortium to address the need (and attempts of several corporations) for a versatile, scriptable and all-purpose vector format for the web and otherwise.

(This description is partly based on or reuses content from the Wikipedia article "Vector graphics" (http://en.wikipedia.org/wiki/Vector_graphics) and is licensed under the GNU Free Documentation License (http://www.gnu.org/copyleft/fdl.html).)</rdfs:comment>
    <skos:inScheme>
      <skos:ConceptScheme rdf:about="http://www.ebusiness-unibw.org/ontologies/consumerelectronics/v1#DataFormatImage">
        <rdfs:isDefinedBy rdf:resource="http://www.ebusiness-unibw.org/ontologies/consumerelectronics/v1"/>
        <rdfs:label xml:lang="en">Data Format Image</rdfs:label>
        <rdfs:comment xml:lang="en">A data format is a particular way to encode information for storage in a computer file (refers to image data).

(This description is partly based on or reuses content from the Wikipedia article "File Format" (http://en.wikipedia.org/wiki/File_format) and is licensed under the GNU Free Documentation License (http://www.gnu.org/copyleft/fdl.html).)</rdfs:comment>
      </skos:ConceptScheme>
    </skos:inScheme>
  </skos:Concept>
  <skos:Concept rdf:about="http://www.ebusiness-unibw.org/ontologies/consumerelectronics/v1#PNG">
    <rdfs:isDefinedBy rdf:resource="http://www.ebusiness-unibw.org/ontologies/consumerelectronics/v1"/>
    <rdfs:label xml:lang="en">PNG</rdfs:label>
    <rdfs:comment xml:lang="en">The PNG (Portable Network Graphics) file format was created as the free, open-source successor to the GIF.

(This description is partly based on or reuses content from the Wikipedia article "Graphics file format" (http://en.wikipedia.org/wiki/Graphics_file_format) and is licensed under the GNU Free Documentation License (http://www.gnu.org/copyleft/fdl.html).)</rdfs:comment>
    <skos:inScheme rdf:resource="http://www.ebusiness-unibw.org/ontologies/consumerelectronics/v1#DataFormatImage"/>
  </skos:Concept>
  <skos:Concept rdf:about="http://www.ebusiness-unibw.org/ontologies/consumerelectronics/v1#JPEG">
    <rdfs:isDefinedBy rdf:resource="http://www.ebusiness-unibw.org/ontologies/consumerelectronics/v1"/>
    <rdfs:label xml:lang="en">JPEG</rdfs:label>
    <rdfs:comment xml:lang="en">JPEG compression is used in a number of image file formats. JPEG/Exif is the most common image format used by digital cameras and other photographic image capture devices; along with JPEG/JFIF, it is the most common format for storing and transmitting photographic images on the World Wide Web.

(This description is partly based on or reuses content from the Wikipedia article "JPEG" (http://en.wikipedia.org/wiki/JPEG) and is licensed under the GNU Free Documentation License (http://www.gnu.org/copyleft/fdl.html).)</rdfs:comment>
    <skos:inScheme rdf:resource="http://www.ebusiness-unibw.org/ontologies/consumerelectronics/v1#DataFormatImage"/>
  </skos:Concept>
  <skos:Concept rdf:about="http://www.ebusiness-unibw.org/ontologies/consumerelectronics/v1#CGM">
    <rdfs:isDefinedBy rdf:resource="http://www.ebusiness-unibw.org/ontologies/consumerelectronics/v1"/>
    <rdfs:label xml:lang="en">CGM</rdfs:label>
    <rdfs:comment xml:lang="en">CGM (Computer Graphics Metafile) is a file format for 2D vector graphics, raster graphics, and text, and is defined by ISO/IEC 8632.

(This description is partly based on or reuses content from the Wikipedia article "Computer Graphics Metafile" (http://en.wikipedia.org/wiki/Computer_Graphics_Metafile) and is licensed under the GNU Free Documentation License (http://www.gnu.org/copyleft/fdl.html).)</rdfs:comment>
    <skos:inScheme rdf:resource="http://www.ebusiness-unibw.org/ontologies/consumerelectronics/v1#DataFormatImage"/>
  </skos:Concept>
  <skos:Concept rdf:about="http://www.ebusiness-unibw.org/ontologies/consumerelectronics/v1#DPOF">
    <rdfs:isDefinedBy rdf:resource="http://www.ebusiness-unibw.org/ontologies/consumerelectronics/v1"/>
    <rdfs:label xml:lang="en">DPOF</rdfs:label>
    <rdfs:comment xml:lang="en">DPOF (Digital Print Order format) is a format which allows the user of a digital camera or other device such as a Mobile Phone or PDA to define which captured images on the storage card are to be printed, together with information on the number of copies or other image information such as paper size, image title text, image orientation, contact information and more.

(This description is partly based on or reuses content from the Wikipedia article "DPOF" (http://en.wikipedia.org/wiki/DPOF) and is licensed under the GNU Free Documentation License (http://www.gnu.org/copyleft/fdl.html).)</rdfs:comment>
    <skos:inScheme rdf:resource="http://www.ebusiness-unibw.org/ontologies/consumerelectronics/v1#DataFormatImage"/>
  </skos:Concept>
  <skos:Concept rdf:about="http://www.ebusiness-unibw.org/ontologies/consumerelectronics/v1#TIFF">
    <rdfs:isDefinedBy rdf:resource="http://www.ebusiness-unibw.org/ontologies/consumerelectronics/v1"/>
    <rdfs:label xml:lang="en">TIFF</rdfs:label>
    <rdfs:comment xml:lang="en">The TIFF (Tagged Image File Format) is a flexible format that normally saves 8 bits or 16 bits per color (red, green, blue) for 24-bit and 48-bit totals, respectively, using either the TIFF or the TIF filenames.

(This description is partly based on or reuses content from the Wikipedia article "Graphics file format" (http://en.wikipedia.org/wiki/Graphics_file_format) and is licensed under the GNU Free Documentation License (http://www.gnu.org/copyleft/fdl.html).)</rdfs:comment>
    <skos:inScheme rdf:resource="http://www.ebusiness-unibw.org/ontologies/consumerelectronics/v1#DataFormatImage"/>
  </skos:Concept>
  <skos:Concept rdf:about="http://www.ebusiness-unibw.org/ontologies/consumerelectronics/v1#GIF">
    <rdfs:isDefinedBy rdf:resource="http://www.ebusiness-unibw.org/ontologies/consumerelectronics/v1"/>
    <rdfs:label xml:lang="en">GIF</rdfs:label>
    <rdfs:comment xml:lang="en">The format supports up to 8 bits per pixel, allowing a single image to reference a palette of up to 256 distinct colors chosen from the 24-bit RGB color space.

(This description is partly based on or reuses content from the Wikipedia article "Graphics Interchange Format" (http://en.wikipedia.org/wiki/Graphics_Interchange_Format) and is licensed under the GNU Free Documentation License (http://www.gnu.org/copyleft/fdl.html).)</rdfs:comment>
    <skos:inScheme rdf:resource="http://www.ebusiness-unibw.org/ontologies/consumerelectronics/v1#DataFormatImage"/>
  </skos:Concept>
  <skos:Concept rdf:about="http://www.ebusiness-unibw.org/ontologies/consumerelectronics/v1#PSD">
    <rdfs:isDefinedBy rdf:resource="http://www.ebusiness-unibw.org/ontologies/consumerelectronics/v1"/>
    <rdfs:label xml:lang="en">PSD</rdfs:label>
    <rdfs:comment xml:lang="en">The .PSD (Photoshop Document) format stores an image with support for most imaging options available in Photoshop. These include layers with masks, color spaces, ICC profiles, transparency, text, alpha channels and spot colors, clipping paths, and duotone settings.

(This description is partly based on or reuses content from the Wikipedia article "Adobe Photoshop" (http://en.wikipedia.org/wiki/Adobe_Photoshop) and is licensed under the GNU Free Documentation License (http://www.gnu.org/copyleft/fdl.html).)</rdfs:comment>
    <skos:inScheme rdf:resource="http://www.ebusiness-unibw.org/ontologies/consumerelectronics/v1#DataFormatImage"/>
  </skos:Concept>
  <skos:Concept rdf:about="http://www.ebusiness-unibw.org/ontologies/consumerelectronics/v1#Bitmap">
    <rdfs:isDefinedBy rdf:resource="http://www.ebusiness-unibw.org/ontologies/consumerelectronics/v1"/>
    <rdfs:label xml:lang="en">Bitmap</rdfs:label>
    <rdfs:comment xml:lang="en">In computer graphics, a bitmap or pixmap is a type of memory organization or image file format used to store digital images.

(This description is partly based on or reuses content from the Wikipedia article "Bitmap" (http://en.wikipedia.org/wiki/Bitmap) and is licensed under the GNU Free Documentation License (http://www.gnu.org/copyleft/fdl.html).)</rdfs:comment>
    <skos:inScheme rdf:resource="http://www.ebusiness-unibw.org/ontologies/consumerelectronics/v1#DataFormatImage"/>
  </skos:Concept>
</rdf:RDF>
