<rdf:RDF
    xmlns:rdf="http://www.w3.org/1999/02/22-rdf-syntax-ns#"
    xmlns:dcterms="http://purl.org/dc/terms/"
    xmlns:dc="http://purl.org/dc/elements/1.1/"
    xmlns:owl="http://www.w3.org/2002/07/owl#"
    xmlns:dcmit="http://purl.org/dc/dcmitype/"
    xmlns:skos="http://www.w3.org/2004/02/skos/core#"
    xmlns:voaf="http://purl.org/vocommons/voaf#"
    xmlns:rdfs="http://www.w3.org/2000/01/rdf-schema#"
    xmlns:vann="http://purl.org/vocab/vann/">
  <owl:Ontology rdf:about="http://www.w3.org/2006/03/test-description"/>
  <owl:ObjectProperty rdf:about="http://www.w3.org/2006/03/test-description#reviewStatus">
    <rdfs:label xml:lang="en">status of review</rdfs:label>
    <rdfs:range>
      <skos:ConceptScheme rdf:about="http://www.w3.org/2006/03/test-description#ReviewStatus">
        <rdfs:isDefinedBy rdf:resource="http://www.w3.org/2006/03/test-description"/>
        <rdfs:label xml:lang="en">Status in a review process</rdfs:label>
        <rdfs:comment>A particular stage in a review process</rdfs:comment>
      </skos:ConceptScheme>
    </rdfs:range>
  </owl:ObjectProperty>
  <skos:Concept rdf:about="http://www.w3.org/2006/03/test-description#rejected">
    <rdfs:isDefinedBy rdf:resource="http://www.w3.org/2006/03/test-description"/>
    <rdfs:label xml:lang="en">rejected</rdfs:label>
    <rdfs:comment>the item has gone through the review process and was rejected</rdfs:comment>
    <skos:inScheme rdf:resource="http://www.w3.org/2006/03/test-description#ReviewStatus"/>
  </skos:Concept>
  <skos:Concept rdf:about="http://www.w3.org/2006/03/test-description#unreviewed">
    <rdfs:isDefinedBy rdf:resource="http://www.w3.org/2006/03/test-description"/>
    <rdfs:label xml:lang="en">unreviewed</rdfs:label>
    <rdfs:comment>the item has been proposed, but hasn't been reviewed (e.g. for completeness) yet</rdfs:comment>
    <skos:inScheme rdf:resource="http://www.w3.org/2006/03/test-description#ReviewStatus"/>
  </skos:Concept>
  <skos:Concept rdf:about="http://www.w3.org/2006/03/test-description#accepted">
    <rdfs:isDefinedBy rdf:resource="http://www.w3.org/2006/03/test-description"/>
    <rdfs:label xml:lang="en">accepted</rdfs:label>
    <rdfs:comment>the item has gone through a first review, which shows it as valid for further processing</rdfs:comment>
    <skos:inScheme rdf:resource="http://www.w3.org/2006/03/test-description#ReviewStatus"/>
  </skos:Concept>
  <skos:Concept rdf:about="http://www.w3.org/2006/03/test-description#assigned">
    <rdfs:isDefinedBy rdf:resource="http://www.w3.org/2006/03/test-description"/>
    <rdfs:label xml:lang="en">assigned</rdfs:label>
    <rdfs:comment>a more specific review of the item has been assigned to someone</rdfs:comment>
    <skos:inScheme rdf:resource="http://www.w3.org/2006/03/test-description#ReviewStatus"/>
  </skos:Concept>
  <skos:Concept rdf:about="http://www.w3.org/2006/03/test-description#approved">
    <rdfs:isDefinedBy rdf:resource="http://www.w3.org/2006/03/test-description"/>
    <rdfs:label xml:lang="en">approved</rdfs:label>
    <rdfs:comment>the item has gone through the review process and was approved</rdfs:comment>
    <skos:inScheme rdf:resource="http://www.w3.org/2006/03/test-description#ReviewStatus"/>
  </skos:Concept>
  <skos:Concept rdf:about="http://www.w3.org/2006/03/test-description#onhold">
    <rdfs:isDefinedBy rdf:resource="http://www.w3.org/2006/03/test-description"/>
    <rdfs:label>on hold</rdfs:label>
    <rdfs:comment>the item had already gone through the review process, but the results of the review need to be re-assessed due to new input</rdfs:comment>
    <skos:inScheme rdf:resource="http://www.w3.org/2006/03/test-description#ReviewStatus"/>
  </skos:Concept>
</rdf:RDF>
