<rdf:RDF
    xmlns:rdf="http://www.w3.org/1999/02/22-rdf-syntax-ns#"
    xmlns:dcterms="http://purl.org/dc/terms/"
    xmlns:dc="http://purl.org/dc/elements/1.1/"
    xmlns:owl="http://www.w3.org/2002/07/owl#"
    xmlns:dcmit="http://purl.org/dc/dcmitype/"
    xmlns:skos="http://www.w3.org/2004/02/skos/core#"
    xmlns:voaf="http://purl.org/vocommons/voaf#"
    xmlns:rdfs="http://www.w3.org/2000/01/rdf-schema#"
    xmlns:vann="http://purl.org/vocab/vann/">
  <owl:Ontology rdf:about="http://rdfunit.aksw.org/ns/core#"/>
  <owl:ObjectProperty rdf:about="http://rdfunit.aksw.org/ns/core#appliesTo">
    <rdfs:comment xml:lang="en">applies to describes the ontology used for terms in the Test.</rdfs:comment>
    <rdfs:label xml:lang="en">appliesTo</rdfs:label>
    <rdfs:domain rdf:resource="http://rdfunit.aksw.org/ns/core#TestCase"/>
    <rdfs:range>
      <skos:ConceptScheme rdf:about="http://rdfunit.aksw.org/ns/core#TestAppliesTo">
        <rdfs:isDefinedBy rdf:resource="http://rdfunit.aksw.org/ns/core#"/>
        <rdfs:label xml:lang="en">TestAppliesTo</rdfs:label>
      </skos:ConceptScheme>
    </rdfs:range>
  </owl:ObjectProperty>
  <skos:Concept rdf:about="http://rdfunit.aksw.org/ns/core#Dataset">
    <rdfs:isDefinedBy rdf:resource="http://rdfunit.aksw.org/ns/core#"/>
    <rdfs:label xml:lang="en">Dataset</rdfs:label>
    <rdfs:comment xml:lang="en">Dataset: When the tests applies to a dataset only (i.e. a SPARQL Endpoint)</rdfs:comment>
    <skos:inScheme rdf:resource="http://rdfunit.aksw.org/ns/core#TestAppliesTo"/>
  </skos:Concept>
  <skos:Concept rdf:about="http://rdfunit.aksw.org/ns/core#Schema">
    <rdfs:isDefinedBy rdf:resource="http://rdfunit.aksw.org/ns/core#"/>
    <rdfs:label xml:lang="en">Schema</rdfs:label>
    <skos:inScheme rdf:resource="http://rdfunit.aksw.org/ns/core#TestAppliesTo"/>
  </skos:Concept>
  <skos:Concept rdf:about="http://rdfunit.aksw.org/ns/core#Application">
    <rdfs:isDefinedBy rdf:resource="http://rdfunit.aksw.org/ns/core#"/>
    <rdfs:label xml:lang="en">Application</rdfs:label>
    <rdfs:comment xml:lang="en">Application: When the tests are specific to an application only</rdfs:comment>
    <skos:inScheme rdf:resource="http://rdfunit.aksw.org/ns/core#TestAppliesTo"/>
  </skos:Concept>
  <skos:Concept rdf:about="http://rdfunit.aksw.org/ns/core#EnrichedSchema">
    <rdfs:isDefinedBy rdf:resource="http://rdfunit.aksw.org/ns/core#"/>
    <rdfs:label xml:lang="en">EnrichedSchema</rdfs:label>
    <rdfs:comment xml:lang="en">EnrichedSchema: When the tests applies to an ontology / vocabulary enriched with external (semi-)automatic approaches</rdfs:comment>
    <skos:inScheme rdf:resource="http://rdfunit.aksw.org/ns/core#TestAppliesTo"/>
  </skos:Concept>
</rdf:RDF>
