<rdf:RDF
    xmlns:rdf="http://www.w3.org/1999/02/22-rdf-syntax-ns#"
    xmlns:dcterms="http://purl.org/dc/terms/"
    xmlns:dc="http://purl.org/dc/elements/1.1/"
    xmlns:owl="http://www.w3.org/2002/07/owl#"
    xmlns:dcmit="http://purl.org/dc/dcmitype/"
    xmlns:skos="http://www.w3.org/2004/02/skos/core#"
    xmlns:voaf="http://purl.org/vocommons/voaf#"
    xmlns:rdfs="http://www.w3.org/2000/01/rdf-schema#"
    xmlns:vann="http://purl.org/vocab/vann/">
  <owl:Ontology rdf:about="http://www.ontology-of-units-of-measure.org/resource/om-2/"/>
  <skos:Concept rdf:about="http://www.ontology-of-units-of-measure.org/resource/om-2/metrePerAttosecond-Time">
    <rdfs:isDefinedBy rdf:resource="http://www.ontology-of-units-of-measure.org/resource/om-2/"/>
    <rdfs:label xml:lang="en">metre per attosecond</rdfs:label>
    <rdfs:comment xml:lang="en">Metre per attosecond is a unit of speed defined as metre divided by attosecond.</rdfs:comment>
    <skos:inScheme>
      <skos:ConceptScheme rdf:about="http://www.ontology-of-units-of-measure.org/resource/om-2/MetrePerPrefixedSecond-Time">
        <rdfs:isDefinedBy rdf:resource="http://www.ontology-of-units-of-measure.org/resource/om-2/"/>
        <rdfs:label xml:lang="en">metre per prefixed second (time)</rdfs:label>
      </skos:ConceptScheme>
    </skos:inScheme>
  </skos:Concept>
  <skos:Concept rdf:about="http://www.ontology-of-units-of-measure.org/resource/om-2/metrePerTerasecond-Time">
    <rdfs:isDefinedBy rdf:resource="http://www.ontology-of-units-of-measure.org/resource/om-2/"/>
    <rdfs:label xml:lang="en">metre per terasecond</rdfs:label>
    <rdfs:comment xml:lang="en">Metre per terasecond is a unit of speed defined as metre divided by terasecond.</rdfs:comment>
    <skos:inScheme rdf:resource="http://www.ontology-of-units-of-measure.org/resource/om-2/MetrePerPrefixedSecond-Time"/>
  </skos:Concept>
  <skos:Concept rdf:about="http://www.ontology-of-units-of-measure.org/resource/om-2/metrePerGigasecond-Time">
    <rdfs:isDefinedBy rdf:resource="http://www.ontology-of-units-of-measure.org/resource/om-2/"/>
    <rdfs:label xml:lang="en">metre per gigasecond</rdfs:label>
    <rdfs:comment xml:lang="en">Metre per gigasecond is a unit of speed defined as metre divided by gigasecond.</rdfs:comment>
    <skos:inScheme rdf:resource="http://www.ontology-of-units-of-measure.org/resource/om-2/MetrePerPrefixedSecond-Time"/>
  </skos:Concept>
  <skos:Concept rdf:about="http://www.ontology-of-units-of-measure.org/resource/om-2/metrePerMillisecond-Time">
    <rdfs:isDefinedBy rdf:resource="http://www.ontology-of-units-of-measure.org/resource/om-2/"/>
    <rdfs:label xml:lang="en">metre per millisecond</rdfs:label>
    <rdfs:comment xml:lang="en">Metre per millisecond is a unit of speed defined as metre divided by millisecond.</rdfs:comment>
    <skos:inScheme rdf:resource="http://www.ontology-of-units-of-measure.org/resource/om-2/MetrePerPrefixedSecond-Time"/>
  </skos:Concept>
  <skos:Concept rdf:about="http://www.ontology-of-units-of-measure.org/resource/om-2/metrePerCentisecond-Time">
    <rdfs:isDefinedBy rdf:resource="http://www.ontology-of-units-of-measure.org/resource/om-2/"/>
    <rdfs:label xml:lang="en">metre per centisecond</rdfs:label>
    <rdfs:comment xml:lang="en">Metre per centisecond is a unit of speed defined as metre divided by centisecond.</rdfs:comment>
    <skos:inScheme rdf:resource="http://www.ontology-of-units-of-measure.org/resource/om-2/MetrePerPrefixedSecond-Time"/>
  </skos:Concept>
  <skos:Concept rdf:about="http://www.ontology-of-units-of-measure.org/resource/om-2/metrePerZeptosecond-Time">
    <rdfs:isDefinedBy rdf:resource="http://www.ontology-of-units-of-measure.org/resource/om-2/"/>
    <rdfs:label xml:lang="en">metre per zeptosecond</rdfs:label>
    <rdfs:comment xml:lang="en">Metre per zeptosecond is a unit of speed defined as metre divided by zeptosecond.</rdfs:comment>
    <skos:inScheme rdf:resource="http://www.ontology-of-units-of-measure.org/resource/om-2/MetrePerPrefixedSecond-Time"/>
  </skos:Concept>
  <skos:Concept rdf:about="http://www.ontology-of-units-of-measure.org/resource/om-2/metrePerYottasecond-Time">
    <rdfs:isDefinedBy rdf:resource="http://www.ontology-of-units-of-measure.org/resource/om-2/"/>
    <rdfs:label xml:lang="en">metre per yottasecond</rdfs:label>
    <rdfs:comment xml:lang="en">Metre per yottasecond is a unit of speed defined as metre divided by yottasecond.</rdfs:comment>
    <skos:inScheme rdf:resource="http://www.ontology-of-units-of-measure.org/resource/om-2/MetrePerPrefixedSecond-Time"/>
  </skos:Concept>
  <skos:Concept rdf:about="http://www.ontology-of-units-of-measure.org/resource/om-2/metrePerKilosecond-Time">
    <rdfs:isDefinedBy rdf:resource="http://www.ontology-of-units-of-measure.org/resource/om-2/"/>
    <rdfs:label xml:lang="en">metre per kilosecond</rdfs:label>
    <rdfs:comment xml:lang="en">Metre per kilosecond is a unit of speed defined as metre divided by kilosecond.</rdfs:comment>
    <skos:inScheme rdf:resource="http://www.ontology-of-units-of-measure.org/resource/om-2/MetrePerPrefixedSecond-Time"/>
  </skos:Concept>
  <skos:Concept rdf:about="http://www.ontology-of-units-of-measure.org/resource/om-2/metrePerZettasecond-Time">
    <rdfs:isDefinedBy rdf:resource="http://www.ontology-of-units-of-measure.org/resource/om-2/"/>
    <rdfs:label xml:lang="en">metre per zettasecond</rdfs:label>
    <rdfs:comment xml:lang="en">Metre per zettasecond is a unit of speed defined as metre divided by zettasecond.</rdfs:comment>
    <skos:inScheme rdf:resource="http://www.ontology-of-units-of-measure.org/resource/om-2/MetrePerPrefixedSecond-Time"/>
  </skos:Concept>
  <skos:Concept rdf:about="http://www.ontology-of-units-of-measure.org/resource/om-2/metrePerDecisecond-Time">
    <rdfs:isDefinedBy rdf:resource="http://www.ontology-of-units-of-measure.org/resource/om-2/"/>
    <rdfs:label xml:lang="en">metre per decisecond</rdfs:label>
    <rdfs:comment xml:lang="en">Metre per decisecond is a unit of speed defined as metre divided by decisecond.</rdfs:comment>
    <skos:inScheme rdf:resource="http://www.ontology-of-units-of-measure.org/resource/om-2/MetrePerPrefixedSecond-Time"/>
  </skos:Concept>
  <skos:Concept rdf:about="http://www.ontology-of-units-of-measure.org/resource/om-2/metrePerDecasecond-Time">
    <rdfs:isDefinedBy rdf:resource="http://www.ontology-of-units-of-measure.org/resource/om-2/"/>
    <rdfs:label xml:lang="en">metre per decasecond</rdfs:label>
    <rdfs:comment xml:lang="en">Metre per decasecond is a unit of speed defined as metre divided by decasecond.</rdfs:comment>
    <skos:inScheme rdf:resource="http://www.ontology-of-units-of-measure.org/resource/om-2/MetrePerPrefixedSecond-Time"/>
  </skos:Concept>
  <skos:Concept rdf:about="http://www.ontology-of-units-of-measure.org/resource/om-2/metrePerExasecond-Time">
    <rdfs:isDefinedBy rdf:resource="http://www.ontology-of-units-of-measure.org/resource/om-2/"/>
    <rdfs:label xml:lang="en">metre per exasecond</rdfs:label>
    <rdfs:comment xml:lang="en">Metre per exasecond is a unit of speed defined as metre divided by exasecond.</rdfs:comment>
    <skos:inScheme rdf:resource="http://www.ontology-of-units-of-measure.org/resource/om-2/MetrePerPrefixedSecond-Time"/>
  </skos:Concept>
  <skos:Concept rdf:about="http://www.ontology-of-units-of-measure.org/resource/om-2/metrePerMegasecond-Time">
    <rdfs:isDefinedBy rdf:resource="http://www.ontology-of-units-of-measure.org/resource/om-2/"/>
    <rdfs:label xml:lang="en">metre per megasecond</rdfs:label>
    <rdfs:comment xml:lang="en">Metre per megasecond is a unit of speed defined as metre divided by megasecond.</rdfs:comment>
    <skos:inScheme rdf:resource="http://www.ontology-of-units-of-measure.org/resource/om-2/MetrePerPrefixedSecond-Time"/>
  </skos:Concept>
  <skos:Concept rdf:about="http://www.ontology-of-units-of-measure.org/resource/om-2/metrePerFemtosecond-Time">
    <rdfs:isDefinedBy rdf:resource="http://www.ontology-of-units-of-measure.org/resource/om-2/"/>
    <rdfs:label xml:lang="en">metre per femtosecond</rdfs:label>
    <rdfs:comment xml:lang="en">Metre per femtosecond is a unit of speed defined as metre divided by femtosecond.</rdfs:comment>
    <skos:inScheme rdf:resource="http://www.ontology-of-units-of-measure.org/resource/om-2/MetrePerPrefixedSecond-Time"/>
  </skos:Concept>
  <skos:Concept rdf:about="http://www.ontology-of-units-of-measure.org/resource/om-2/metrePerNanosecond-Time">
    <rdfs:isDefinedBy rdf:resource="http://www.ontology-of-units-of-measure.org/resource/om-2/"/>
    <rdfs:label xml:lang="en">metre per nanosecond</rdfs:label>
    <rdfs:comment xml:lang="en">Metre per nanosecond is a unit of speed defined as metre divided by nanosecond.</rdfs:comment>
    <skos:inScheme rdf:resource="http://www.ontology-of-units-of-measure.org/resource/om-2/MetrePerPrefixedSecond-Time"/>
  </skos:Concept>
  <skos:Concept rdf:about="http://www.ontology-of-units-of-measure.org/resource/om-2/metrePerYoctosecond-Time">
    <rdfs:isDefinedBy rdf:resource="http://www.ontology-of-units-of-measure.org/resource/om-2/"/>
    <rdfs:label xml:lang="en">metre per yoctosecond</rdfs:label>
    <rdfs:comment xml:lang="en">Metre per yoctosecond is a unit of speed defined as metre divided by yoctosecond.</rdfs:comment>
    <skos:inScheme rdf:resource="http://www.ontology-of-units-of-measure.org/resource/om-2/MetrePerPrefixedSecond-Time"/>
  </skos:Concept>
  <skos:Concept rdf:about="http://www.ontology-of-units-of-measure.org/resource/om-2/metrePerPetasecond-Time">
    <rdfs:isDefinedBy rdf:resource="http://www.ontology-of-units-of-measure.org/resource/om-2/"/>
    <rdfs:label xml:lang="en">metre per petasecond</rdfs:label>
    <rdfs:comment xml:lang="en">Metre per petasecond is a unit of speed defined as metre divided by petasecond.</rdfs:comment>
    <skos:inScheme rdf:resource="http://www.ontology-of-units-of-measure.org/resource/om-2/MetrePerPrefixedSecond-Time"/>
  </skos:Concept>
  <skos:Concept rdf:about="http://www.ontology-of-units-of-measure.org/resource/om-2/metrePerPicosecond-Time">
    <rdfs:isDefinedBy rdf:resource="http://www.ontology-of-units-of-measure.org/resource/om-2/"/>
    <rdfs:label xml:lang="en">metre per picosecond</rdfs:label>
    <rdfs:comment xml:lang="en">Metre per picosecond is a unit of speed defined as metre divided by picosecond.</rdfs:comment>
    <skos:inScheme rdf:resource="http://www.ontology-of-units-of-measure.org/resource/om-2/MetrePerPrefixedSecond-Time"/>
  </skos:Concept>
  <skos:Concept rdf:about="http://www.ontology-of-units-of-measure.org/resource/om-2/metrePerHectosecond-Time">
    <rdfs:isDefinedBy rdf:resource="http://www.ontology-of-units-of-measure.org/resource/om-2/"/>
    <rdfs:label xml:lang="en">metre per hectosecond</rdfs:label>
    <rdfs:comment xml:lang="en">Metre per hectosecond is a unit of speed defined as metre divided by hectosecond.</rdfs:comment>
    <skos:inScheme rdf:resource="http://www.ontology-of-units-of-measure.org/resource/om-2/MetrePerPrefixedSecond-Time"/>
  </skos:Concept>
  <skos:Concept rdf:about="http://www.ontology-of-units-of-measure.org/resource/om-2/metrePerMicrosecond-Time">
    <rdfs:isDefinedBy rdf:resource="http://www.ontology-of-units-of-measure.org/resource/om-2/"/>
    <rdfs:label xml:lang="en">metre per microsecond</rdfs:label>
    <rdfs:comment xml:lang="en">Metre per microsecond is a unit of speed defined as metre divided by microsecond.</rdfs:comment>
    <skos:inScheme rdf:resource="http://www.ontology-of-units-of-measure.org/resource/om-2/MetrePerPrefixedSecond-Time"/>
  </skos:Concept>
</rdf:RDF>
