<rdf:RDF
    xmlns:rdf="http://www.w3.org/1999/02/22-rdf-syntax-ns#"
    xmlns:dcterms="http://purl.org/dc/terms/"
    xmlns:dc="http://purl.org/dc/elements/1.1/"
    xmlns:owl="http://www.w3.org/2002/07/owl#"
    xmlns:dcmit="http://purl.org/dc/dcmitype/"
    xmlns:skos="http://www.w3.org/2004/02/skos/core#"
    xmlns:voaf="http://purl.org/vocommons/voaf#"
    xmlns:rdfs="http://www.w3.org/2000/01/rdf-schema#"
    xmlns:vann="http://purl.org/vocab/vann/">
  <owl:Ontology rdf:about="http://www.ontology-of-units-of-measure.org/resource/om-2/"/>
  <skos:Concept rdf:about="http://www.ontology-of-units-of-measure.org/resource/om-2/metrePerGigasecond-TimeSquared">
    <rdfs:isDefinedBy rdf:resource="http://www.ontology-of-units-of-measure.org/resource/om-2/"/>
    <rdfs:label xml:lang="en">metre per gigasecond squared</rdfs:label>
    <rdfs:comment xml:lang="en">Metre per gigasecond squared is a unit of acceleration defined as metre divided by gigasecond squared.</rdfs:comment>
    <skos:inScheme>
      <skos:ConceptScheme rdf:about="http://www.ontology-of-units-of-measure.org/resource/om-2/MetrePerPrefixedSecond-TimeSquared">
        <rdfs:isDefinedBy rdf:resource="http://www.ontology-of-units-of-measure.org/resource/om-2/"/>
        <rdfs:label xml:lang="en">metre per prefixed second (time) squared</rdfs:label>
      </skos:ConceptScheme>
    </skos:inScheme>
  </skos:Concept>
  <skos:Concept rdf:about="http://www.ontology-of-units-of-measure.org/resource/om-2/metrePerPicosecond-TimeSquared">
    <rdfs:isDefinedBy rdf:resource="http://www.ontology-of-units-of-measure.org/resource/om-2/"/>
    <rdfs:label xml:lang="en">metre per picosecond squared</rdfs:label>
    <rdfs:comment xml:lang="en">Metre per picosecond squared is a unit of acceleration defined as metre divided by picosecond squared.</rdfs:comment>
    <skos:inScheme rdf:resource="http://www.ontology-of-units-of-measure.org/resource/om-2/MetrePerPrefixedSecond-TimeSquared"/>
  </skos:Concept>
  <skos:Concept rdf:about="http://www.ontology-of-units-of-measure.org/resource/om-2/metrePerKilosecond-TimeSquared">
    <rdfs:isDefinedBy rdf:resource="http://www.ontology-of-units-of-measure.org/resource/om-2/"/>
    <rdfs:label xml:lang="en">metre per kilosecond squared</rdfs:label>
    <rdfs:comment xml:lang="en">Metre per kilosecond squared is a unit of acceleration defined as metre divided by kilosecond squared.</rdfs:comment>
    <skos:inScheme rdf:resource="http://www.ontology-of-units-of-measure.org/resource/om-2/MetrePerPrefixedSecond-TimeSquared"/>
  </skos:Concept>
  <skos:Concept rdf:about="http://www.ontology-of-units-of-measure.org/resource/om-2/metrePerCentisecond-TimeSquared">
    <rdfs:isDefinedBy rdf:resource="http://www.ontology-of-units-of-measure.org/resource/om-2/"/>
    <rdfs:label xml:lang="en">metre per centisecond squared</rdfs:label>
    <rdfs:comment xml:lang="en">Metre per centisecond squared is a unit of acceleration defined as metre divided by centisecond squared.</rdfs:comment>
    <skos:inScheme rdf:resource="http://www.ontology-of-units-of-measure.org/resource/om-2/MetrePerPrefixedSecond-TimeSquared"/>
  </skos:Concept>
  <skos:Concept rdf:about="http://www.ontology-of-units-of-measure.org/resource/om-2/metrePerFemtosecond-TimeSquared">
    <rdfs:isDefinedBy rdf:resource="http://www.ontology-of-units-of-measure.org/resource/om-2/"/>
    <rdfs:label xml:lang="en">metre per femtosecond squared</rdfs:label>
    <rdfs:comment xml:lang="en">Metre per femtosecond squared is a unit of acceleration defined as metre divided by femtosecond squared.</rdfs:comment>
    <skos:inScheme rdf:resource="http://www.ontology-of-units-of-measure.org/resource/om-2/MetrePerPrefixedSecond-TimeSquared"/>
  </skos:Concept>
  <skos:Concept rdf:about="http://www.ontology-of-units-of-measure.org/resource/om-2/metrePerAttosecond-TimeSquared">
    <rdfs:isDefinedBy rdf:resource="http://www.ontology-of-units-of-measure.org/resource/om-2/"/>
    <rdfs:label xml:lang="en">metre per attosecond squared</rdfs:label>
    <rdfs:comment xml:lang="en">Metre per attosecond squared is a unit of acceleration defined as metre divided by attosecond squared.</rdfs:comment>
    <skos:inScheme rdf:resource="http://www.ontology-of-units-of-measure.org/resource/om-2/MetrePerPrefixedSecond-TimeSquared"/>
  </skos:Concept>
  <skos:Concept rdf:about="http://www.ontology-of-units-of-measure.org/resource/om-2/metrePerZettasecond-TimeSquared">
    <rdfs:isDefinedBy rdf:resource="http://www.ontology-of-units-of-measure.org/resource/om-2/"/>
    <rdfs:label xml:lang="en">metre per zettasecond squared</rdfs:label>
    <rdfs:comment xml:lang="en">Metre per zettasecond squared is a unit of acceleration defined as metre divided by zettasecond squared.</rdfs:comment>
    <skos:inScheme rdf:resource="http://www.ontology-of-units-of-measure.org/resource/om-2/MetrePerPrefixedSecond-TimeSquared"/>
  </skos:Concept>
  <skos:Concept rdf:about="http://www.ontology-of-units-of-measure.org/resource/om-2/metrePerMegasecond-TimeSquared">
    <rdfs:isDefinedBy rdf:resource="http://www.ontology-of-units-of-measure.org/resource/om-2/"/>
    <rdfs:label xml:lang="en">metre per megasecond squared</rdfs:label>
    <rdfs:comment xml:lang="en">Metre per megasecond squared is a unit of acceleration defined as metre divided by megasecond squared.</rdfs:comment>
    <skos:inScheme rdf:resource="http://www.ontology-of-units-of-measure.org/resource/om-2/MetrePerPrefixedSecond-TimeSquared"/>
  </skos:Concept>
  <skos:Concept rdf:about="http://www.ontology-of-units-of-measure.org/resource/om-2/metrePerTerasecond-TimeSquared">
    <rdfs:isDefinedBy rdf:resource="http://www.ontology-of-units-of-measure.org/resource/om-2/"/>
    <rdfs:label xml:lang="en">metre per terasecond squared</rdfs:label>
    <rdfs:comment xml:lang="en">Metre per terasecond squared is a unit of acceleration defined as metre divided by terasecond squared.</rdfs:comment>
    <skos:inScheme rdf:resource="http://www.ontology-of-units-of-measure.org/resource/om-2/MetrePerPrefixedSecond-TimeSquared"/>
  </skos:Concept>
  <skos:Concept rdf:about="http://www.ontology-of-units-of-measure.org/resource/om-2/metrePerNanosecond-TimeSquared">
    <rdfs:isDefinedBy rdf:resource="http://www.ontology-of-units-of-measure.org/resource/om-2/"/>
    <rdfs:label xml:lang="en">metre per nanosecond squared</rdfs:label>
    <rdfs:comment xml:lang="en">Metre per nanosecond squared is a unit of acceleration defined as metre divided by nanosecond squared.</rdfs:comment>
    <skos:inScheme rdf:resource="http://www.ontology-of-units-of-measure.org/resource/om-2/MetrePerPrefixedSecond-TimeSquared"/>
  </skos:Concept>
  <skos:Concept rdf:about="http://www.ontology-of-units-of-measure.org/resource/om-2/metrePerZeptosecond-TimeSquared">
    <rdfs:isDefinedBy rdf:resource="http://www.ontology-of-units-of-measure.org/resource/om-2/"/>
    <rdfs:label xml:lang="en">metre per zeptosecond squared</rdfs:label>
    <rdfs:comment xml:lang="en">Metre per zeptosecond squared is a unit of acceleration defined as metre divided by zeptosecond squared.</rdfs:comment>
    <skos:inScheme rdf:resource="http://www.ontology-of-units-of-measure.org/resource/om-2/MetrePerPrefixedSecond-TimeSquared"/>
  </skos:Concept>
  <skos:Concept rdf:about="http://www.ontology-of-units-of-measure.org/resource/om-2/metrePerDecisecond-TimeSquared">
    <rdfs:isDefinedBy rdf:resource="http://www.ontology-of-units-of-measure.org/resource/om-2/"/>
    <rdfs:label xml:lang="en">metre per decisecond squared</rdfs:label>
    <rdfs:comment xml:lang="en">Metre per decisecond squared is a unit of acceleration defined as metre divided by decisecond squared.</rdfs:comment>
    <skos:inScheme rdf:resource="http://www.ontology-of-units-of-measure.org/resource/om-2/MetrePerPrefixedSecond-TimeSquared"/>
  </skos:Concept>
  <skos:Concept rdf:about="http://www.ontology-of-units-of-measure.org/resource/om-2/metrePerPetasecond-TimeSquared">
    <rdfs:isDefinedBy rdf:resource="http://www.ontology-of-units-of-measure.org/resource/om-2/"/>
    <rdfs:label xml:lang="en">metre per petasecond squared</rdfs:label>
    <rdfs:comment xml:lang="en">Metre per petasecond squared is a unit of acceleration defined as metre divided by petasecond squared.</rdfs:comment>
    <skos:inScheme rdf:resource="http://www.ontology-of-units-of-measure.org/resource/om-2/MetrePerPrefixedSecond-TimeSquared"/>
  </skos:Concept>
  <skos:Concept rdf:about="http://www.ontology-of-units-of-measure.org/resource/om-2/metrePerMicrosecond-TimeSquared">
    <rdfs:isDefinedBy rdf:resource="http://www.ontology-of-units-of-measure.org/resource/om-2/"/>
    <rdfs:label xml:lang="en">metre per microsecond squared</rdfs:label>
    <rdfs:comment xml:lang="en">Metre per microsecond squared is a unit of acceleration defined as metre divided by microsecond squared.</rdfs:comment>
    <skos:inScheme rdf:resource="http://www.ontology-of-units-of-measure.org/resource/om-2/MetrePerPrefixedSecond-TimeSquared"/>
  </skos:Concept>
  <skos:Concept rdf:about="http://www.ontology-of-units-of-measure.org/resource/om-2/metrePerYottasecond-TimeSquared">
    <rdfs:isDefinedBy rdf:resource="http://www.ontology-of-units-of-measure.org/resource/om-2/"/>
    <rdfs:label xml:lang="en">metre per yottasecond squared</rdfs:label>
    <rdfs:comment xml:lang="en">Metre per yottasecond squared is a unit of acceleration defined as metre divided by yottasecond squared.</rdfs:comment>
    <skos:inScheme rdf:resource="http://www.ontology-of-units-of-measure.org/resource/om-2/MetrePerPrefixedSecond-TimeSquared"/>
  </skos:Concept>
  <skos:Concept rdf:about="http://www.ontology-of-units-of-measure.org/resource/om-2/metrePerExasecond-TimeSquared">
    <rdfs:isDefinedBy rdf:resource="http://www.ontology-of-units-of-measure.org/resource/om-2/"/>
    <rdfs:label xml:lang="en">metre per exasecond squared</rdfs:label>
    <rdfs:comment xml:lang="en">Metre per exasecond squared is a unit of acceleration defined as metre divided by exasecond squared.</rdfs:comment>
    <skos:inScheme rdf:resource="http://www.ontology-of-units-of-measure.org/resource/om-2/MetrePerPrefixedSecond-TimeSquared"/>
  </skos:Concept>
  <skos:Concept rdf:about="http://www.ontology-of-units-of-measure.org/resource/om-2/metrePerMillisecond-TimeSquared">
    <rdfs:isDefinedBy rdf:resource="http://www.ontology-of-units-of-measure.org/resource/om-2/"/>
    <rdfs:label xml:lang="en">metre per millisecond squared</rdfs:label>
    <rdfs:comment xml:lang="en">Metre per millisecond squared is a unit of acceleration defined as metre divided by millisecond squared.</rdfs:comment>
    <skos:inScheme rdf:resource="http://www.ontology-of-units-of-measure.org/resource/om-2/MetrePerPrefixedSecond-TimeSquared"/>
  </skos:Concept>
  <skos:Concept rdf:about="http://www.ontology-of-units-of-measure.org/resource/om-2/metrePerHectosecond-TimeSquared">
    <rdfs:isDefinedBy rdf:resource="http://www.ontology-of-units-of-measure.org/resource/om-2/"/>
    <rdfs:label xml:lang="en">metre per hectosecond squared</rdfs:label>
    <rdfs:comment xml:lang="en">Metre per hectosecond squared is a unit of acceleration defined as metre divided by hectosecond squared.</rdfs:comment>
    <skos:inScheme rdf:resource="http://www.ontology-of-units-of-measure.org/resource/om-2/MetrePerPrefixedSecond-TimeSquared"/>
  </skos:Concept>
  <skos:Concept rdf:about="http://www.ontology-of-units-of-measure.org/resource/om-2/metrePerYoctosecond-TimeSquared">
    <rdfs:isDefinedBy rdf:resource="http://www.ontology-of-units-of-measure.org/resource/om-2/"/>
    <rdfs:label xml:lang="en">metre per yoctosecond squared</rdfs:label>
    <rdfs:comment xml:lang="en">Metre per yoctosecond squared is a unit of acceleration defined as metre divided by yoctosecond squared.</rdfs:comment>
    <skos:inScheme rdf:resource="http://www.ontology-of-units-of-measure.org/resource/om-2/MetrePerPrefixedSecond-TimeSquared"/>
  </skos:Concept>
  <skos:Concept rdf:about="http://www.ontology-of-units-of-measure.org/resource/om-2/metrePerDecasecond-TimeSquared">
    <rdfs:isDefinedBy rdf:resource="http://www.ontology-of-units-of-measure.org/resource/om-2/"/>
    <rdfs:label xml:lang="en">metre per decasecond squared</rdfs:label>
    <rdfs:comment xml:lang="en">Metre per decasecond squared is a unit of acceleration defined as metre divided by decasecond squared.</rdfs:comment>
    <skos:inScheme rdf:resource="http://www.ontology-of-units-of-measure.org/resource/om-2/MetrePerPrefixedSecond-TimeSquared"/>
  </skos:Concept>
</rdf:RDF>
