<rdf:RDF
    xmlns:rdf="http://www.w3.org/1999/02/22-rdf-syntax-ns#"
    xmlns:dcterms="http://purl.org/dc/terms/"
    xmlns:dc="http://purl.org/dc/elements/1.1/"
    xmlns:owl="http://www.w3.org/2002/07/owl#"
    xmlns:dcmit="http://purl.org/dc/dcmitype/"
    xmlns:j.0="http://purl.oclc.org/NET/ssnx/qu/qu#"
    xmlns:skos="http://www.w3.org/2004/02/skos/core#"
    xmlns:voaf="http://purl.org/vocommons/voaf#"
    xmlns:rdfs="http://www.w3.org/2000/01/rdf-schema#"
    xmlns:vann="http://purl.org/vocab/vann/">
  <owl:Ontology rdf:about="http://purl.oclc.org/NET/ssnx/cf/cf-property"/>
  <skos:Concept rdf:about="http://purl.oclc.org/NET/ssnx/cf/cf-property#zenith_angle">
    <rdfs:isDefinedBy rdf:resource="http://purl.oclc.org/NET/ssnx/cf/cf-property"/>
    <j.0:generalQuantityKind>
      <skos:Concept rdf:about="http://purl.oclc.org/NET/ssnx/qu/quantity#angle">
        <skos:inScheme>
          <skos:ConceptScheme rdf:about="http://purl.oclc.org/NET/ssnx/qu/dim#Angle">
            <rdfs:isDefinedBy rdf:resource="http://purl.oclc.org/NET/ssnx/cf/cf-property"/>
          </skos:ConceptScheme>
        </skos:inScheme>
        <rdfs:isDefinedBy rdf:resource="http://purl.oclc.org/NET/ssnx/cf/cf-property"/>
      </skos:Concept>
    </j.0:generalQuantityKind>
    <rdfs:label>zenith angle</rdfs:label>
    <rdfs:comment>Zenith angle is the angle to the local vertical; a value of zero is directly overhead.</rdfs:comment>
    <skos:inScheme rdf:resource="http://purl.oclc.org/NET/ssnx/qu/dim#Angle"/>
  </skos:Concept>
  <skos:Concept rdf:about="http://purl.oclc.org/NET/ssnx/cf/cf-property#solar_elevation_angle">
    <rdfs:isDefinedBy rdf:resource="http://purl.oclc.org/NET/ssnx/cf/cf-property"/>
    <j.0:generalQuantityKind rdf:resource="http://purl.oclc.org/NET/ssnx/qu/quantity#angle"/>
    <rdfs:label>solar elevation angle</rdfs:label>
    <rdfs:comment>Solar elevation angle is the angle between the line of sight to the sun and the local horizontal.</rdfs:comment>
    <skos:inScheme rdf:resource="http://purl.oclc.org/NET/ssnx/qu/dim#Angle"/>
  </skos:Concept>
  <skos:Concept rdf:about="http://purl.oclc.org/NET/ssnx/cf/cf-property#platform_roll_angle">
    <rdfs:isDefinedBy rdf:resource="http://purl.oclc.org/NET/ssnx/cf/cf-property"/>
    <j.0:generalQuantityKind rdf:resource="http://purl.oclc.org/NET/ssnx/qu/quantity#angle"/>
    <rdfs:label>platform roll angle</rdfs:label>
    <rdfs:comment>Standard names for platform describe the motion and orientation of the vehicle from which observations are made e.g. aeroplane or ship.</rdfs:comment>
    <skos:inScheme rdf:resource="http://purl.oclc.org/NET/ssnx/qu/dim#Angle"/>
  </skos:Concept>
  <skos:Concept rdf:about="http://purl.oclc.org/NET/ssnx/cf/cf-property#sea_surface_wind_wave_to_direction">
    <rdfs:isDefinedBy rdf:resource="http://purl.oclc.org/NET/ssnx/cf/cf-property"/>
    <j.0:generalQuantityKind rdf:resource="http://purl.oclc.org/NET/ssnx/qu/quantity#angle"/>
    <rdfs:label>sea surface wind wave to direction</rdfs:label>
    <rdfs:comment>Wind waves are waves on the ocean surface. Wind is defined as a two-dimensional (horizontal) air velocity vector, with no vertical component. (Vertical motion in the atmosphere has the standard name upward_air_velocity.) "to_direction" is used in the construction X_to_direction and indicates the direction towards which the velocity vector of X is headed.</rdfs:comment>
    <skos:inScheme rdf:resource="http://purl.oclc.org/NET/ssnx/qu/dim#Angle"/>
  </skos:Concept>
  <skos:Concept rdf:about="http://purl.oclc.org/NET/ssnx/cf/cf-property#platform_pitch_angle">
    <rdfs:isDefinedBy rdf:resource="http://purl.oclc.org/NET/ssnx/cf/cf-property"/>
    <j.0:generalQuantityKind rdf:resource="http://purl.oclc.org/NET/ssnx/qu/quantity#angle"/>
    <rdfs:label>platform pitch angle</rdfs:label>
    <rdfs:comment>Standard names for platform describe the motion and orientation of the vehicle from which observations are made e.g. aeroplane or ship.</rdfs:comment>
    <skos:inScheme rdf:resource="http://purl.oclc.org/NET/ssnx/qu/dim#Angle"/>
  </skos:Concept>
  <skos:Concept rdf:about="http://purl.oclc.org/NET/ssnx/cf/cf-property#sea_surface_wave_from_direction">
    <rdfs:isDefinedBy rdf:resource="http://purl.oclc.org/NET/ssnx/cf/cf-property"/>
    <j.0:generalQuantityKind rdf:resource="http://purl.oclc.org/NET/ssnx/qu/quantity#angle"/>
    <rdfs:label>sea surface wave from direction</rdfs:label>
    <rdfs:comment>"from_direction" is used in the construction X_from_direction and indicates the direction from which the velocity vector of X is coming.</rdfs:comment>
    <skos:inScheme rdf:resource="http://purl.oclc.org/NET/ssnx/qu/dim#Angle"/>
  </skos:Concept>
  <skos:Concept rdf:about="http://purl.oclc.org/NET/ssnx/cf/cf-property#angle_of_emergence">
    <rdfs:isDefinedBy rdf:resource="http://purl.oclc.org/NET/ssnx/cf/cf-property"/>
    <j.0:generalQuantityKind rdf:resource="http://purl.oclc.org/NET/ssnx/qu/quantity#angle"/>
    <rdfs:label>angle of emergence</rdfs:label>
    <rdfs:comment>The angle of emergence is that between the direction of a beam of radiation emerging from the surface of a medium and the normal to that surface.</rdfs:comment>
    <skos:inScheme rdf:resource="http://purl.oclc.org/NET/ssnx/qu/dim#Angle"/>
  </skos:Concept>
  <skos:Concept rdf:about="http://purl.oclc.org/NET/ssnx/cf/cf-property#grid_latitude">
    <rdfs:isDefinedBy rdf:resource="http://purl.oclc.org/NET/ssnx/cf/cf-property"/>
    <j.0:generalQuantityKind rdf:resource="http://purl.oclc.org/NET/ssnx/qu/quantity#angle"/>
    <rdfs:label>grid latitude</rdfs:label>
    <rdfs:comment>Latitude is positive northward; its units of degree_north (or equivalent) indicate this explicitly. In a latitude-longitude system defined with respect to a rotated North Pole, the standard name of grid_latitude should be used instead of latitude. Grid latitude is positive in the grid-northward direction, but its units should be plain degree.</rdfs:comment>
    <skos:inScheme rdf:resource="http://purl.oclc.org/NET/ssnx/qu/dim#Angle"/>
  </skos:Concept>
  <skos:Concept rdf:about="http://purl.oclc.org/NET/ssnx/cf/cf-property#angle_of_rotation_from_east_to_y">
    <rdfs:isDefinedBy rdf:resource="http://purl.oclc.org/NET/ssnx/cf/cf-property"/>
    <j.0:generalQuantityKind rdf:resource="http://purl.oclc.org/NET/ssnx/qu/quantity#angle"/>
    <rdfs:label>angle of rotation from east to y</rdfs:label>
    <rdfs:comment>The quantity with standard name angle_of_rotation_from_east_to_y is the angle, anticlockwise reckoned positive, between due East and (dr/dj)ik, where r(i,j,k) is the vector 3D position of the point with coordinate indices (i,j,k).  It could be used for rotating vector fields between model space and latitude-longitude space.</rdfs:comment>
    <skos:inScheme rdf:resource="http://purl.oclc.org/NET/ssnx/qu/dim#Angle"/>
  </skos:Concept>
  <skos:Concept rdf:about="http://purl.oclc.org/NET/ssnx/cf/cf-property#sea_surface_wave_to_direction">
    <rdfs:isDefinedBy rdf:resource="http://purl.oclc.org/NET/ssnx/cf/cf-property"/>
    <j.0:generalQuantityKind rdf:resource="http://purl.oclc.org/NET/ssnx/qu/quantity#angle"/>
    <rdfs:label>sea surface wave to direction</rdfs:label>
    <rdfs:comment>"to_direction" is used in the construction X_to_direction and indicates the direction towards which the velocity vector of X is headed.</rdfs:comment>
    <skos:inScheme rdf:resource="http://purl.oclc.org/NET/ssnx/qu/dim#Angle"/>
  </skos:Concept>
  <skos:Concept rdf:about="http://purl.oclc.org/NET/ssnx/cf/cf-property#grid_longitude">
    <rdfs:isDefinedBy rdf:resource="http://purl.oclc.org/NET/ssnx/cf/cf-property"/>
    <j.0:generalQuantityKind rdf:resource="http://purl.oclc.org/NET/ssnx/qu/quantity#angle"/>
    <rdfs:label>grid longitude</rdfs:label>
    <rdfs:comment>Longitude is positive eastward; its units of degree_east (or equivalent) indicate this explicitly. In a latitude-longitude system defined with respect to a rotated North Pole, the standard name of grid_longitude should be used instead of longitude. Grid longitude is positive in the grid-eastward direction, but its units should be plain degree.</rdfs:comment>
    <skos:inScheme rdf:resource="http://purl.oclc.org/NET/ssnx/qu/dim#Angle"/>
  </skos:Concept>
  <skos:Concept rdf:about="http://purl.oclc.org/NET/ssnx/cf/cf-property#direction_of_radial_vector_away_from_instrument">
    <rdfs:isDefinedBy rdf:resource="http://purl.oclc.org/NET/ssnx/cf/cf-property"/>
    <j.0:generalQuantityKind rdf:resource="http://purl.oclc.org/NET/ssnx/qu/quantity#angle"/>
    <rdfs:label>direction of radial vector away from instrument</rdfs:label>
    <rdfs:comment>The direction_of_radial_vector_away_from_instrument is the direction in which the instrument itself is pointing. The direction is measured positive clockwise from due north. The "instrument" (examples are radar and lidar) is the device used to make an observation. "direction_of_X" means direction of a  vector, a bearing.</rdfs:comment>
    <skos:inScheme rdf:resource="http://purl.oclc.org/NET/ssnx/qu/dim#Angle"/>
  </skos:Concept>
  <skos:Concept rdf:about="http://purl.oclc.org/NET/ssnx/cf/cf-property#angle_of_incidence">
    <rdfs:isDefinedBy rdf:resource="http://purl.oclc.org/NET/ssnx/cf/cf-property"/>
    <j.0:generalQuantityKind rdf:resource="http://purl.oclc.org/NET/ssnx/qu/quantity#angle"/>
    <rdfs:label>angle of incidence</rdfs:label>
    <rdfs:comment>The angle of incidence is that between the direction of approach of a beam of radiation toward a surface and the normal to that surface.</rdfs:comment>
    <skos:inScheme rdf:resource="http://purl.oclc.org/NET/ssnx/qu/dim#Angle"/>
  </skos:Concept>
  <skos:Concept rdf:about="http://purl.oclc.org/NET/ssnx/cf/cf-property#platform_course">
    <rdfs:isDefinedBy rdf:resource="http://purl.oclc.org/NET/ssnx/cf/cf-property"/>
    <j.0:generalQuantityKind rdf:resource="http://purl.oclc.org/NET/ssnx/qu/quantity#angle"/>
    <rdfs:label>platform course</rdfs:label>
    <rdfs:comment>Standard names for platform describe the motion and orientation of the vehicle from which observations are made e.g. aeroplane or ship. The platform course is the direction in which the platform is travelling (not necessarily the same as the direction in which it is pointing, called platform_orientation).</rdfs:comment>
    <skos:inScheme rdf:resource="http://purl.oclc.org/NET/ssnx/qu/dim#Angle"/>
  </skos:Concept>
  <skos:Concept rdf:about="http://purl.oclc.org/NET/ssnx/cf/cf-property#direction_of_sea_ice_velocity">
    <rdfs:isDefinedBy rdf:resource="http://purl.oclc.org/NET/ssnx/cf/cf-property"/>
    <j.0:generalQuantityKind rdf:resource="http://purl.oclc.org/NET/ssnx/qu/quantity#angle"/>
    <rdfs:label>direction of sea ice velocity</rdfs:label>
    <rdfs:comment>"direction_of_X" means direction of a vector, a bearing. A velocity is a vector quantity. Sea ice velocity is defined as a two-dimensional vector, with no vertical component.</rdfs:comment>
    <skos:inScheme rdf:resource="http://purl.oclc.org/NET/ssnx/qu/dim#Angle"/>
  </skos:Concept>
  <skos:Concept rdf:about="http://purl.oclc.org/NET/ssnx/cf/cf-property#sea_surface_swell_wave_to_direction">
    <rdfs:isDefinedBy rdf:resource="http://purl.oclc.org/NET/ssnx/cf/cf-property"/>
    <j.0:generalQuantityKind rdf:resource="http://purl.oclc.org/NET/ssnx/qu/quantity#angle"/>
    <rdfs:label>sea surface swell wave to direction</rdfs:label>
    <rdfs:comment>Swell waves are waves on the ocean surface. "to_direction" is used in the construction X_to_direction and indicates the direction towards which the velocity vector of X is headed.</rdfs:comment>
    <skos:inScheme rdf:resource="http://purl.oclc.org/NET/ssnx/qu/dim#Angle"/>
  </skos:Concept>
  <skos:Concept rdf:about="http://purl.oclc.org/NET/ssnx/cf/cf-property#scattering_angle">
    <rdfs:isDefinedBy rdf:resource="http://purl.oclc.org/NET/ssnx/cf/cf-property"/>
    <j.0:generalQuantityKind rdf:resource="http://purl.oclc.org/NET/ssnx/qu/quantity#angle"/>
    <rdfs:label>scattering angle</rdfs:label>
    <rdfs:comment>The scattering angle is that between the direction of the beam of incident radiation and the direction into which it is scattered.</rdfs:comment>
    <skos:inScheme rdf:resource="http://purl.oclc.org/NET/ssnx/qu/dim#Angle"/>
  </skos:Concept>
  <skos:Concept rdf:about="http://purl.oclc.org/NET/ssnx/cf/cf-property#solar_azimuth_angle">
    <rdfs:isDefinedBy rdf:resource="http://purl.oclc.org/NET/ssnx/cf/cf-property"/>
    <j.0:generalQuantityKind rdf:resource="http://purl.oclc.org/NET/ssnx/qu/quantity#angle"/>
    <rdfs:label>solar azimuth angle</rdfs:label>
    <rdfs:comment>Solar azimuth angle is the horizontal angle between the line of sight to the sun and a reference direction which is often due north. The angle is measured clockwise.</rdfs:comment>
    <skos:inScheme rdf:resource="http://purl.oclc.org/NET/ssnx/qu/dim#Angle"/>
  </skos:Concept>
  <skos:Concept rdf:about="http://purl.oclc.org/NET/ssnx/cf/cf-property#platform_yaw_angle">
    <rdfs:isDefinedBy rdf:resource="http://purl.oclc.org/NET/ssnx/cf/cf-property"/>
    <j.0:generalQuantityKind rdf:resource="http://purl.oclc.org/NET/ssnx/qu/quantity#angle"/>
    <rdfs:label>platform yaw angle</rdfs:label>
    <rdfs:comment>Standard names for platform describe the motion and orientation of the vehicle from which observations are made e.g. aeroplane or ship.</rdfs:comment>
    <skos:inScheme rdf:resource="http://purl.oclc.org/NET/ssnx/qu/dim#Angle"/>
  </skos:Concept>
  <skos:Concept rdf:about="http://purl.oclc.org/NET/ssnx/cf/cf-property#wind_to_direction">
    <rdfs:isDefinedBy rdf:resource="http://purl.oclc.org/NET/ssnx/cf/cf-property"/>
    <j.0:generalQuantityKind rdf:resource="http://purl.oclc.org/NET/ssnx/qu/quantity#angle"/>
    <rdfs:label>wind to direction</rdfs:label>
    <rdfs:comment>Wind is defined as a two-dimensional (horizontal) air velocity vector, with no vertical component. (Vertical motion in the atmosphere has the standard name upward_air_velocity.) In meteorological reports, the direction of the wind vector is usually (but not always) given as the direction from which it is blowing (wind_from_direction) (westerly, northerly, etc.). In other contexts, such as atmospheric modelling, it is often natural to give the direction in the usual manner of vectors as the heading or the direction to which it is blowing (wind_to_direction) (eastward, southward, etc.) "to_direction" is used in the construction X_to_direction and indicates the direction towards which the velocity vector of X is headed.</rdfs:comment>
    <skos:inScheme rdf:resource="http://purl.oclc.org/NET/ssnx/qu/dim#Angle"/>
  </skos:Concept>
  <skos:Concept rdf:about="http://purl.oclc.org/NET/ssnx/cf/cf-property#angle_of_rotation_from_east_to_x">
    <rdfs:isDefinedBy rdf:resource="http://purl.oclc.org/NET/ssnx/cf/cf-property"/>
    <j.0:generalQuantityKind rdf:resource="http://purl.oclc.org/NET/ssnx/qu/quantity#angle"/>
    <rdfs:label>angle of rotation from east to x</rdfs:label>
    <rdfs:comment>The quantity with standard name angle_of_rotation_from_east_to_x is the angle, anticlockwise reckoned positive, between due East and (dr/di)jk, where r(i,j,k) is the vector 3D position of the point with coordinate indices (i,j,k).  It could be used for rotating vector fields between model space and latitude-longitude space.</rdfs:comment>
    <skos:inScheme rdf:resource="http://purl.oclc.org/NET/ssnx/qu/dim#Angle"/>
  </skos:Concept>
  <skos:Concept rdf:about="http://purl.oclc.org/NET/ssnx/cf/cf-property#platform_orientation">
    <rdfs:isDefinedBy rdf:resource="http://purl.oclc.org/NET/ssnx/cf/cf-property"/>
    <j.0:generalQuantityKind rdf:resource="http://purl.oclc.org/NET/ssnx/qu/quantity#angle"/>
    <rdfs:label>platform orientation</rdfs:label>
    <rdfs:comment>Standard names for platform describe the motion and orientation of the vehicle from which observations are made e.g. aeroplane or ship. The platform orientation is the direction in which the "front" or longitudinal axis of the platform is pointing (not necessarily the same as the direction in which it is travelling, called platform_course).</rdfs:comment>
    <skos:inScheme rdf:resource="http://purl.oclc.org/NET/ssnx/qu/dim#Angle"/>
  </skos:Concept>
  <skos:Concept rdf:about="http://purl.oclc.org/NET/ssnx/cf/cf-property#solar_zenith_angle">
    <rdfs:isDefinedBy rdf:resource="http://purl.oclc.org/NET/ssnx/cf/cf-property"/>
    <j.0:generalQuantityKind rdf:resource="http://purl.oclc.org/NET/ssnx/qu/quantity#angle"/>
    <rdfs:label>solar zenith angle</rdfs:label>
    <rdfs:comment>Solar zenith angle is the the angle between the line of sight to the sun and the local vertical.</rdfs:comment>
    <skos:inScheme rdf:resource="http://purl.oclc.org/NET/ssnx/qu/dim#Angle"/>
  </skos:Concept>
  <skos:Concept rdf:about="http://purl.oclc.org/NET/ssnx/cf/cf-property#direction_of_sea_water_velocity">
    <rdfs:isDefinedBy rdf:resource="http://purl.oclc.org/NET/ssnx/cf/cf-property"/>
    <j.0:generalQuantityKind rdf:resource="http://purl.oclc.org/NET/ssnx/qu/quantity#angle"/>
    <rdfs:label>direction of sea water velocity</rdfs:label>
    <rdfs:comment>"direction_of_X" means direction of a vector, a bearing. A velocity is a vector quantity.</rdfs:comment>
    <skos:inScheme rdf:resource="http://purl.oclc.org/NET/ssnx/qu/dim#Angle"/>
  </skos:Concept>
  <skos:Concept rdf:about="http://purl.oclc.org/NET/ssnx/cf/cf-property#wind_from_direction">
    <rdfs:isDefinedBy rdf:resource="http://purl.oclc.org/NET/ssnx/cf/cf-property"/>
    <j.0:generalQuantityKind rdf:resource="http://purl.oclc.org/NET/ssnx/qu/quantity#angle"/>
    <rdfs:label>wind from direction</rdfs:label>
    <rdfs:comment>Wind is defined as a two-dimensional (horizontal) air velocity vector, with no vertical component. (Vertical motion in the atmosphere has the standard name upward_air_velocity.) In meteorological reports, the direction of the wind vector is usually (but not always) given as the direction from which it is blowing (wind_from_direction) (westerly, northerly, etc.). In other contexts, such as atmospheric modelling, it is often natural to give the direction in the usual manner of vectors as the heading or the direction to which it is blowing (wind_to_direction) (eastward, southward, etc.) "from_direction" is used in the construction X_from_direction and indicates the direction from which the velocity vector of X is coming.</rdfs:comment>
    <skos:inScheme rdf:resource="http://purl.oclc.org/NET/ssnx/qu/dim#Angle"/>
  </skos:Concept>
</rdf:RDF>
