<rdf:RDF
    xmlns:rdf="http://www.w3.org/1999/02/22-rdf-syntax-ns#"
    xmlns:dcterms="http://purl.org/dc/terms/"
    xmlns:dc="http://purl.org/dc/elements/1.1/"
    xmlns:owl="http://www.w3.org/2002/07/owl#"
    xmlns:dcmit="http://purl.org/dc/dcmitype/"
    xmlns:skos="http://www.w3.org/2004/02/skos/core#"
    xmlns:voaf="http://purl.org/vocommons/voaf#"
    xmlns:rdfs="http://www.w3.org/2000/01/rdf-schema#"
    xmlns:vann="http://purl.org/vocab/vann/">
  <owl:Ontology rdf:about="http://www.semanticweb.org/ontologies/2008/11/OntologySecurity.owl"/>
  <skos:Concept rdf:about="http://www.semanticweb.org/ontologies/2008/11/OntologySecurity.owl#ReadUserDataFunctionGroup">
    <rdfs:isDefinedBy rdf:resource="http://www.semanticweb.org/ontologies/2008/11/OntologySecurity.owl"/>
    <rdfs:comment>Read User Data: Set of permissions to read userâ€™s data like phone book or calendar entries</rdfs:comment>
    <skos:inScheme>
      <skos:ConceptScheme rdf:about="http://www.semanticweb.org/ontologies/2008/11/OntologySecurity.owl#FunctionGroups">
        <rdfs:isDefinedBy rdf:resource="http://www.semanticweb.org/ontologies/2008/11/OntologySecurity.owl"/>
        <rdfs:comment rdf:datatype="http://www.w3.org/2001/XMLSchema#string"
        >A set of sensitive functions under a named group that can get authorization.</rdfs:comment>
      </skos:ConceptScheme>
    </skos:inScheme>
  </skos:Concept>
  <skos:Concept rdf:about="http://www.semanticweb.org/ontologies/2008/11/OntologySecurity.owl#MessagingFunctionsGroup">
    <rdfs:isDefinedBy rdf:resource="http://www.semanticweb.org/ontologies/2008/11/OntologySecurity.owl"/>
    <rdfs:comment>Set of permissions related to sending or receiving messages like SMS</rdfs:comment>
    <skos:inScheme rdf:resource="http://www.semanticweb.org/ontologies/2008/11/OntologySecurity.owl#FunctionGroups"/>
  </skos:Concept>
  <skos:Concept rdf:about="http://www.semanticweb.org/ontologies/2008/11/OntologySecurity.owl#AutoInvocationFunctionGroup">
    <rdfs:isDefinedBy rdf:resource="http://www.semanticweb.org/ontologies/2008/11/OntologySecurity.owl"/>
    <rdfs:comment>Permissions related to automatically starting a MIDlet, for example by Push Registration.</rdfs:comment>
    <skos:inScheme rdf:resource="http://www.semanticweb.org/ontologies/2008/11/OntologySecurity.owl#FunctionGroups"/>
  </skos:Concept>
</rdf:RDF>
