<rdf:RDF
    xmlns:rdf="http://www.w3.org/1999/02/22-rdf-syntax-ns#"
    xmlns:dcterms="http://purl.org/dc/terms/"
    xmlns:dc="http://purl.org/dc/elements/1.1/"
    xmlns:owl="http://www.w3.org/2002/07/owl#"
    xmlns:dcmit="http://purl.org/dc/dcmitype/"
    xmlns:skos="http://www.w3.org/2004/02/skos/core#"
    xmlns:voaf="http://purl.org/vocommons/voaf#"
    xmlns:rdfs="http://www.w3.org/2000/01/rdf-schema#"
    xmlns:vann="http://purl.org/vocab/vann/">
  <owl:Ontology rdf:about="http://www.ontology-of-units-of-measure.org/resource/om-2/"/>
  <skos:Concept rdf:about="http://www.ontology-of-units-of-measure.org/resource/om-2/gramPerGigalitre">
    <rdfs:isDefinedBy rdf:resource="http://www.ontology-of-units-of-measure.org/resource/om-2/"/>
    <rdfs:label xml:lang="en">gram per gigalitre</rdfs:label>
    <rdfs:comment xml:lang="en">Gram per gigalitre is a unit of density defined as gram divided by gigalitre.</rdfs:comment>
    <skos:inScheme>
      <skos:ConceptScheme rdf:about="http://www.ontology-of-units-of-measure.org/resource/om-2/GramPerPrefixedLitre">
        <rdfs:isDefinedBy rdf:resource="http://www.ontology-of-units-of-measure.org/resource/om-2/"/>
        <rdfs:label xml:lang="en">gram per prefixed litre</rdfs:label>
      </skos:ConceptScheme>
    </skos:inScheme>
  </skos:Concept>
  <skos:Concept rdf:about="http://www.ontology-of-units-of-measure.org/resource/om-2/gramPerYottalitre">
    <rdfs:isDefinedBy rdf:resource="http://www.ontology-of-units-of-measure.org/resource/om-2/"/>
    <rdfs:label xml:lang="en">gram per yottalitre</rdfs:label>
    <rdfs:comment xml:lang="en">Gram per yottalitre is a unit of density defined as gram divided by yottalitre.</rdfs:comment>
    <skos:inScheme rdf:resource="http://www.ontology-of-units-of-measure.org/resource/om-2/GramPerPrefixedLitre"/>
  </skos:Concept>
  <skos:Concept rdf:about="http://www.ontology-of-units-of-measure.org/resource/om-2/gramPerMicrolitre">
    <rdfs:isDefinedBy rdf:resource="http://www.ontology-of-units-of-measure.org/resource/om-2/"/>
    <rdfs:label xml:lang="en">gram per microlitre</rdfs:label>
    <rdfs:comment xml:lang="en">Gram per microlitre is a unit of density defined as gram divided by microlitre.</rdfs:comment>
    <skos:inScheme rdf:resource="http://www.ontology-of-units-of-measure.org/resource/om-2/GramPerPrefixedLitre"/>
  </skos:Concept>
  <skos:Concept rdf:about="http://www.ontology-of-units-of-measure.org/resource/om-2/gramPerCentilitre">
    <rdfs:isDefinedBy rdf:resource="http://www.ontology-of-units-of-measure.org/resource/om-2/"/>
    <rdfs:label xml:lang="en">gram per centilitre</rdfs:label>
    <rdfs:comment xml:lang="en">Gram per centilitre is a unit of density defined as gram divided by centilitre.</rdfs:comment>
    <skos:inScheme rdf:resource="http://www.ontology-of-units-of-measure.org/resource/om-2/GramPerPrefixedLitre"/>
  </skos:Concept>
  <skos:Concept rdf:about="http://www.ontology-of-units-of-measure.org/resource/om-2/gramPerPicolitre">
    <rdfs:isDefinedBy rdf:resource="http://www.ontology-of-units-of-measure.org/resource/om-2/"/>
    <rdfs:label xml:lang="en">gram per picolitre</rdfs:label>
    <rdfs:comment xml:lang="en">Gram per picolitre is a unit of density defined as gram divided by picolitre.</rdfs:comment>
    <skos:inScheme rdf:resource="http://www.ontology-of-units-of-measure.org/resource/om-2/GramPerPrefixedLitre"/>
  </skos:Concept>
  <skos:Concept rdf:about="http://www.ontology-of-units-of-measure.org/resource/om-2/gramPerZeptolitre">
    <rdfs:isDefinedBy rdf:resource="http://www.ontology-of-units-of-measure.org/resource/om-2/"/>
    <rdfs:label xml:lang="en">gram per zeptolitre</rdfs:label>
    <rdfs:comment xml:lang="en">Gram per zeptolitre is a unit of density defined as gram divided by zeptolitre.</rdfs:comment>
    <skos:inScheme rdf:resource="http://www.ontology-of-units-of-measure.org/resource/om-2/GramPerPrefixedLitre"/>
  </skos:Concept>
  <skos:Concept rdf:about="http://www.ontology-of-units-of-measure.org/resource/om-2/gramPerExalitre">
    <rdfs:isDefinedBy rdf:resource="http://www.ontology-of-units-of-measure.org/resource/om-2/"/>
    <rdfs:label xml:lang="en">gram per exalitre</rdfs:label>
    <rdfs:comment xml:lang="en">Gram per exalitre is a unit of density defined as gram divided by exalitre.</rdfs:comment>
    <skos:inScheme rdf:resource="http://www.ontology-of-units-of-measure.org/resource/om-2/GramPerPrefixedLitre"/>
  </skos:Concept>
  <skos:Concept rdf:about="http://www.ontology-of-units-of-measure.org/resource/om-2/gramPerNanolitre">
    <rdfs:isDefinedBy rdf:resource="http://www.ontology-of-units-of-measure.org/resource/om-2/"/>
    <rdfs:label xml:lang="en">gram per nanolitre</rdfs:label>
    <rdfs:comment xml:lang="en">Gram per nanolitre is a unit of density defined as gram divided by nanolitre.</rdfs:comment>
    <skos:inScheme rdf:resource="http://www.ontology-of-units-of-measure.org/resource/om-2/GramPerPrefixedLitre"/>
  </skos:Concept>
  <skos:Concept rdf:about="http://www.ontology-of-units-of-measure.org/resource/om-2/gramPerFemtolitre">
    <rdfs:isDefinedBy rdf:resource="http://www.ontology-of-units-of-measure.org/resource/om-2/"/>
    <rdfs:label xml:lang="en">gram per femtolitre</rdfs:label>
    <rdfs:comment xml:lang="en">Gram per femtolitre is a unit of density defined as gram divided by femtolitre.</rdfs:comment>
    <skos:inScheme rdf:resource="http://www.ontology-of-units-of-measure.org/resource/om-2/GramPerPrefixedLitre"/>
  </skos:Concept>
  <skos:Concept rdf:about="http://www.ontology-of-units-of-measure.org/resource/om-2/gramPerTeralitre">
    <rdfs:isDefinedBy rdf:resource="http://www.ontology-of-units-of-measure.org/resource/om-2/"/>
    <rdfs:label xml:lang="en">gram per teralitre</rdfs:label>
    <rdfs:comment xml:lang="en">Gram per teralitre is a unit of density defined as gram divided by teralitre.</rdfs:comment>
    <skos:inScheme rdf:resource="http://www.ontology-of-units-of-measure.org/resource/om-2/GramPerPrefixedLitre"/>
  </skos:Concept>
  <skos:Concept rdf:about="http://www.ontology-of-units-of-measure.org/resource/om-2/gramPerPetalitre">
    <rdfs:isDefinedBy rdf:resource="http://www.ontology-of-units-of-measure.org/resource/om-2/"/>
    <rdfs:label xml:lang="en">gram per petalitre</rdfs:label>
    <rdfs:comment xml:lang="en">Gram per petalitre is a unit of density defined as gram divided by petalitre.</rdfs:comment>
    <skos:inScheme rdf:resource="http://www.ontology-of-units-of-measure.org/resource/om-2/GramPerPrefixedLitre"/>
  </skos:Concept>
  <skos:Concept rdf:about="http://www.ontology-of-units-of-measure.org/resource/om-2/gramPerYoctolitre">
    <rdfs:isDefinedBy rdf:resource="http://www.ontology-of-units-of-measure.org/resource/om-2/"/>
    <rdfs:label xml:lang="en">gram per yoctolitre</rdfs:label>
    <rdfs:comment xml:lang="en">Gram per yoctolitre is a unit of density defined as gram divided by yoctolitre.</rdfs:comment>
    <skos:inScheme rdf:resource="http://www.ontology-of-units-of-measure.org/resource/om-2/GramPerPrefixedLitre"/>
  </skos:Concept>
  <skos:Concept rdf:about="http://www.ontology-of-units-of-measure.org/resource/om-2/gramPerMegalitre">
    <rdfs:isDefinedBy rdf:resource="http://www.ontology-of-units-of-measure.org/resource/om-2/"/>
    <rdfs:label xml:lang="en">gram per megalitre</rdfs:label>
    <rdfs:comment xml:lang="en">Gram per megalitre is a unit of density defined as gram divided by megalitre.</rdfs:comment>
    <skos:inScheme rdf:resource="http://www.ontology-of-units-of-measure.org/resource/om-2/GramPerPrefixedLitre"/>
  </skos:Concept>
  <skos:Concept rdf:about="http://www.ontology-of-units-of-measure.org/resource/om-2/gramPerDecalitre">
    <rdfs:isDefinedBy rdf:resource="http://www.ontology-of-units-of-measure.org/resource/om-2/"/>
    <rdfs:label xml:lang="en">gram per decalitre</rdfs:label>
    <rdfs:comment xml:lang="en">Gram per decalitre is a unit of density defined as gram divided by decalitre.</rdfs:comment>
    <skos:inScheme rdf:resource="http://www.ontology-of-units-of-measure.org/resource/om-2/GramPerPrefixedLitre"/>
  </skos:Concept>
  <skos:Concept rdf:about="http://www.ontology-of-units-of-measure.org/resource/om-2/gramPerAttolitre">
    <rdfs:isDefinedBy rdf:resource="http://www.ontology-of-units-of-measure.org/resource/om-2/"/>
    <rdfs:label xml:lang="en">gram per attolitre</rdfs:label>
    <rdfs:comment xml:lang="en">Gram per attolitre is a unit of density defined as gram divided by attolitre.</rdfs:comment>
    <skos:inScheme rdf:resource="http://www.ontology-of-units-of-measure.org/resource/om-2/GramPerPrefixedLitre"/>
  </skos:Concept>
  <skos:Concept rdf:about="http://www.ontology-of-units-of-measure.org/resource/om-2/gramPerMillilitre">
    <rdfs:isDefinedBy rdf:resource="http://www.ontology-of-units-of-measure.org/resource/om-2/"/>
    <rdfs:label xml:lang="en">gram per millilitre</rdfs:label>
    <rdfs:comment xml:lang="en">Gram per millilitre is a unit of density defined as gram divided by millilitre.</rdfs:comment>
    <skos:inScheme rdf:resource="http://www.ontology-of-units-of-measure.org/resource/om-2/GramPerPrefixedLitre"/>
  </skos:Concept>
  <skos:Concept rdf:about="http://www.ontology-of-units-of-measure.org/resource/om-2/gramPerHectolitre">
    <rdfs:isDefinedBy rdf:resource="http://www.ontology-of-units-of-measure.org/resource/om-2/"/>
    <rdfs:label xml:lang="en">gram per hectolitre</rdfs:label>
    <rdfs:comment xml:lang="en">Gram per hectolitre is a unit of density defined as gram divided by hectolitre.</rdfs:comment>
    <skos:inScheme rdf:resource="http://www.ontology-of-units-of-measure.org/resource/om-2/GramPerPrefixedLitre"/>
  </skos:Concept>
  <skos:Concept rdf:about="http://www.ontology-of-units-of-measure.org/resource/om-2/gramPerZettalitre">
    <rdfs:isDefinedBy rdf:resource="http://www.ontology-of-units-of-measure.org/resource/om-2/"/>
    <rdfs:label xml:lang="en">gram per zettalitre</rdfs:label>
    <rdfs:comment xml:lang="en">Gram per zettalitre is a unit of density defined as gram divided by zettalitre.</rdfs:comment>
    <skos:inScheme rdf:resource="http://www.ontology-of-units-of-measure.org/resource/om-2/GramPerPrefixedLitre"/>
  </skos:Concept>
  <skos:Concept rdf:about="http://www.ontology-of-units-of-measure.org/resource/om-2/gramPerDecilitre">
    <rdfs:isDefinedBy rdf:resource="http://www.ontology-of-units-of-measure.org/resource/om-2/"/>
    <rdfs:label xml:lang="en">gram per decilitre</rdfs:label>
    <rdfs:comment xml:lang="en">Gram per decilitre is a unit of density defined as gram divided by decilitre.</rdfs:comment>
    <skos:inScheme rdf:resource="http://www.ontology-of-units-of-measure.org/resource/om-2/GramPerPrefixedLitre"/>
  </skos:Concept>
  <skos:Concept rdf:about="http://www.ontology-of-units-of-measure.org/resource/om-2/gramPerKilolitre">
    <rdfs:isDefinedBy rdf:resource="http://www.ontology-of-units-of-measure.org/resource/om-2/"/>
    <rdfs:label xml:lang="en">gram per kilolitre</rdfs:label>
    <rdfs:comment xml:lang="en">Gram per kilolitre is a unit of density defined as gram divided by kilolitre.</rdfs:comment>
    <skos:inScheme rdf:resource="http://www.ontology-of-units-of-measure.org/resource/om-2/GramPerPrefixedLitre"/>
  </skos:Concept>
</rdf:RDF>
