<rdf:RDF
    xmlns:rdf="http://www.w3.org/1999/02/22-rdf-syntax-ns#"
    xmlns:dcterms="http://purl.org/dc/terms/"
    xmlns:dc="http://purl.org/dc/elements/1.1/"
    xmlns:owl="http://www.w3.org/2002/07/owl#"
    xmlns:dcmit="http://purl.org/dc/dcmitype/"
    xmlns:j.0="http://purl.oclc.org/NET/ssnx/qu/qu#"
    xmlns:skos="http://www.w3.org/2004/02/skos/core#"
    xmlns:voaf="http://purl.org/vocommons/voaf#"
    xmlns:rdfs="http://www.w3.org/2000/01/rdf-schema#"
    xmlns:vann="http://purl.org/vocab/vann/">
  <owl:Ontology rdf:about="http://purl.oclc.org/NET/ssnx/cf/cf-property"/>
  <skos:Concept rdf:about="http://purl.oclc.org/NET/ssnx/cf/cf-property#northward_ocean_freshwater_transport_due_to_diffusion">
    <rdfs:isDefinedBy rdf:resource="http://purl.oclc.org/NET/ssnx/cf/cf-property"/>
    <j.0:generalQuantityKind>
      <skos:Concept rdf:about="http://purl.oclc.org/NET/ssnx/qu/quantity#massFlowRate">
        <skos:inScheme>
          <skos:ConceptScheme rdf:about="http://purl.oclc.org/NET/ssnx/qu/dim#MassFlowRate">
            <rdfs:isDefinedBy rdf:resource="http://purl.oclc.org/NET/ssnx/cf/cf-property"/>
          </skos:ConceptScheme>
        </skos:inScheme>
        <rdfs:isDefinedBy rdf:resource="http://purl.oclc.org/NET/ssnx/cf/cf-property"/>
      </skos:Concept>
    </j.0:generalQuantityKind>
    <rdfs:label>northward ocean freshwater transport due to diffusion</rdfs:label>
    <rdfs:comment>The specification of a physical process by the phrase due_to_process means that the quantity named is a single term in a sum of terms which together compose the general quantity named by omitting the phrase. "Northward" indicates a vector component which is positive when directed northward (negative southward). Northward transport by diffusion means the part due to horizontal or isopyncal diffusion schemes in an ocean model, but not including the "bolus" or Gent-McWilliams velocity.</rdfs:comment>
    <skos:inScheme rdf:resource="http://purl.oclc.org/NET/ssnx/qu/dim#MassFlowRate"/>
  </skos:Concept>
  <skos:Concept rdf:about="http://purl.oclc.org/NET/ssnx/cf/cf-property#ocean_mass_y_transport_due_to_advection_and_bolus_advection">
    <rdfs:isDefinedBy rdf:resource="http://purl.oclc.org/NET/ssnx/cf/cf-property"/>
    <j.0:generalQuantityKind rdf:resource="http://purl.oclc.org/NET/ssnx/qu/quantity#massFlowRate"/>
    <rdfs:label>ocean mass y transport due to advection and bolus advection</rdfs:label>
    <rdfs:comment> "y" indicates a vector component along the grid y-axis, when this is not true latitude, positive with increasing y.  Transport by bolus advection in an ocean model means the part due to a scheme representing eddy-induced effects not included inthe velocity field.  The specification of a physical process by the phrase due_to_process means that the quantity named is a  single term in a sum of terms which together compose the general quantity  named by omitting the phrase. </rdfs:comment>
    <skos:inScheme rdf:resource="http://purl.oclc.org/NET/ssnx/qu/dim#MassFlowRate"/>
  </skos:Concept>
  <skos:Concept rdf:about="http://purl.oclc.org/NET/ssnx/cf/cf-property#ocean_mass_x_transport_due_to_advection">
    <rdfs:isDefinedBy rdf:resource="http://purl.oclc.org/NET/ssnx/cf/cf-property"/>
    <j.0:generalQuantityKind rdf:resource="http://purl.oclc.org/NET/ssnx/qu/quantity#massFlowRate"/>
    <rdfs:label>ocean mass x transport due to advection</rdfs:label>
    <rdfs:comment> "x" indicates a vector component along the grid x-axis, when this is not true longitude, positive with increasing x.  The specification of a physical process by the phrase due_to_process means that the quantity named is a  single term in a sum of terms which together compose the general quantity  named by omitting the phrase.</rdfs:comment>
    <skos:inScheme rdf:resource="http://purl.oclc.org/NET/ssnx/qu/dim#MassFlowRate"/>
  </skos:Concept>
  <skos:Concept rdf:about="http://purl.oclc.org/NET/ssnx/cf/cf-property#northward_ocean_salt_transport_due_to_bolus_advection">
    <rdfs:isDefinedBy rdf:resource="http://purl.oclc.org/NET/ssnx/cf/cf-property"/>
    <j.0:generalQuantityKind rdf:resource="http://purl.oclc.org/NET/ssnx/qu/quantity#massFlowRate"/>
    <rdfs:label>northward ocean salt transport due to bolus advection</rdfs:label>
    <rdfs:comment>The specification of a physical process by the phrase due_to_process means that the quantity named is a single term in a sum of terms which together compose the general quantity named by omitting the phrase. "Northward" indicates a vector component which is positive when directed northward (negative southward). Northward transport by bolus advection in an ocean model means the part due to a scheme representing eddy-induced effects not included in the velocity field.</rdfs:comment>
    <skos:inScheme rdf:resource="http://purl.oclc.org/NET/ssnx/qu/dim#MassFlowRate"/>
  </skos:Concept>
  <skos:Concept rdf:about="http://purl.oclc.org/NET/ssnx/cf/cf-property#northward_ocean_freshwater_transport_due_to_overturning">
    <rdfs:isDefinedBy rdf:resource="http://purl.oclc.org/NET/ssnx/cf/cf-property"/>
    <j.0:generalQuantityKind rdf:resource="http://purl.oclc.org/NET/ssnx/qu/quantity#massFlowRate"/>
    <rdfs:label>northward ocean freshwater transport due to overturning</rdfs:label>
    <rdfs:comment>The specification of a physical process by the phrase due_to_process means that the quantity named is a single term in a sum of terms which together compose the general quantity named by omitting the phrase. "Northward" indicates a vector component which is positive when directed northward (negative southward). Northward transport by (meridional) overturning is geometrically defined as being the part due to the vertical integral of the product of zonal means of velocity and tracer. The velocity does not include "bolus" or Gent-McWilliams velocity.</rdfs:comment>
    <skos:inScheme rdf:resource="http://purl.oclc.org/NET/ssnx/qu/dim#MassFlowRate"/>
  </skos:Concept>
  <skos:Concept rdf:about="http://purl.oclc.org/NET/ssnx/cf/cf-property#northward_ocean_freshwater_transport">
    <rdfs:isDefinedBy rdf:resource="http://purl.oclc.org/NET/ssnx/cf/cf-property"/>
    <j.0:generalQuantityKind rdf:resource="http://purl.oclc.org/NET/ssnx/qu/quantity#massFlowRate"/>
    <rdfs:label>northward ocean freshwater transport</rdfs:label>
    <rdfs:comment>"Northward" indicates a vector component which is positive when directed northward (negative southward). Ocean transport means transport by all processes, both sea water and sea ice.</rdfs:comment>
    <skos:inScheme rdf:resource="http://purl.oclc.org/NET/ssnx/qu/dim#MassFlowRate"/>
  </skos:Concept>
  <skos:Concept rdf:about="http://purl.oclc.org/NET/ssnx/cf/cf-property#ocean_meridional_overturning_mass_streamfunction_due_to_bolus_advection">
    <rdfs:isDefinedBy rdf:resource="http://purl.oclc.org/NET/ssnx/cf/cf-property"/>
    <j.0:generalQuantityKind rdf:resource="http://purl.oclc.org/NET/ssnx/qu/quantity#massFlowRate"/>
    <rdfs:label>ocean meridional overturning mass streamfunction due to bolus advection</rdfs:label>
    <rdfs:comment> The specification of a physical process by the phrase due_to_process means that the quantity named is a  single term in a sum of terms which together compose the general quantity  named by omitting the phrase.</rdfs:comment>
    <skos:inScheme rdf:resource="http://purl.oclc.org/NET/ssnx/qu/dim#MassFlowRate"/>
  </skos:Concept>
  <skos:Concept rdf:about="http://purl.oclc.org/NET/ssnx/cf/cf-property#ocean_mass_x_transport">
    <rdfs:isDefinedBy rdf:resource="http://purl.oclc.org/NET/ssnx/cf/cf-property"/>
    <j.0:generalQuantityKind rdf:resource="http://purl.oclc.org/NET/ssnx/qu/quantity#massFlowRate"/>
    <rdfs:label>ocean mass x transport</rdfs:label>
    <rdfs:comment> "x" indicates a vector component along the grid x-axis, when this is not true longitude, positive with increasing x.</rdfs:comment>
    <skos:inScheme rdf:resource="http://purl.oclc.org/NET/ssnx/qu/dim#MassFlowRate"/>
  </skos:Concept>
  <skos:Concept rdf:about="http://purl.oclc.org/NET/ssnx/cf/cf-property#northward_ocean_salt_transport_due_to_diffusion">
    <rdfs:isDefinedBy rdf:resource="http://purl.oclc.org/NET/ssnx/cf/cf-property"/>
    <j.0:generalQuantityKind rdf:resource="http://purl.oclc.org/NET/ssnx/qu/quantity#massFlowRate"/>
    <rdfs:label>northward ocean salt transport due to diffusion</rdfs:label>
    <rdfs:comment>The specification of a physical process by the phrase due_to_process means that the quantity named is a single term in a sum of terms which together compose the general quantity named by omitting the phrase. "Northward" indicates a vector component which is positive when directed northward (negative southward). Northward transport by diffusion means the part due to horizontal or isopyncal diffusion schemes in an ocean model, but not including the "bolus" or Gent-McWilliams velocity.</rdfs:comment>
    <skos:inScheme rdf:resource="http://purl.oclc.org/NET/ssnx/qu/dim#MassFlowRate"/>
  </skos:Concept>
  <skos:Concept rdf:about="http://purl.oclc.org/NET/ssnx/cf/cf-property#ocean_meridional_overturning_mass_streamfunction">
    <rdfs:isDefinedBy rdf:resource="http://purl.oclc.org/NET/ssnx/cf/cf-property"/>
    <j.0:generalQuantityKind rdf:resource="http://purl.oclc.org/NET/ssnx/qu/quantity#massFlowRate"/>
    <rdfs:label>ocean meridional overturning mass streamfunction</rdfs:label>
    <rdfs:comment> In contrast to the quantity with standard name ocean_meridional_overturning_streamfunction, this quantity includes all physical processes, resolved or parameterized, that impact mass/volume transport.  Thus it includes contributions from the bolus and Gent-McWilliams velocity.</rdfs:comment>
    <skos:inScheme rdf:resource="http://purl.oclc.org/NET/ssnx/qu/dim#MassFlowRate"/>
  </skos:Concept>
  <skos:Concept rdf:about="http://purl.oclc.org/NET/ssnx/cf/cf-property#ocean_barotropic_mass_streamfunction">
    <rdfs:isDefinedBy rdf:resource="http://purl.oclc.org/NET/ssnx/cf/cf-property"/>
    <j.0:generalQuantityKind rdf:resource="http://purl.oclc.org/NET/ssnx/qu/quantity#massFlowRate"/>
    <rdfs:label>ocean barotropic mass streamfunction</rdfs:label>
    <rdfs:comment> The barotropic stream function with the dimensions of volume transport has the standard name ocean_barotropic_streamfunction.</rdfs:comment>
    <skos:inScheme rdf:resource="http://purl.oclc.org/NET/ssnx/qu/dim#MassFlowRate"/>
  </skos:Concept>
  <skos:Concept rdf:about="http://purl.oclc.org/NET/ssnx/cf/cf-property#ocean_y_overturning_mass_streamfunction">
    <rdfs:isDefinedBy rdf:resource="http://purl.oclc.org/NET/ssnx/cf/cf-property"/>
    <j.0:generalQuantityKind rdf:resource="http://purl.oclc.org/NET/ssnx/qu/quantity#massFlowRate"/>
    <rdfs:label>ocean y overturning mass streamfunction</rdfs:label>
    <rdfs:comment> "y" indicates a vector component along the grid y-axis, when this is not true latitude, positive with increasing y.  In contrast to the quantity with standard name ocean_meridional_overturning_streamfunction, this quantity includes all physicalprocesses, resolved or parameterized, that impact mass/volume transport.  Thus it includescontributions from the bolus and Gent-McWilliams velocity.</rdfs:comment>
    <skos:inScheme rdf:resource="http://purl.oclc.org/NET/ssnx/qu/dim#MassFlowRate"/>
  </skos:Concept>
  <skos:Concept rdf:about="http://purl.oclc.org/NET/ssnx/cf/cf-property#northward_ocean_salt_transport_due_to_overturning">
    <rdfs:isDefinedBy rdf:resource="http://purl.oclc.org/NET/ssnx/cf/cf-property"/>
    <j.0:generalQuantityKind rdf:resource="http://purl.oclc.org/NET/ssnx/qu/quantity#massFlowRate"/>
    <rdfs:label>northward ocean salt transport due to overturning</rdfs:label>
    <rdfs:comment>The specification of a physical process by the phrase due_to_process means that the quantity named is a single term in a sum of terms which together compose the general quantity named by omitting the phrase. "Northward" indicates a vector component which is positive when directed northward (negative southward). Northward transport by (meridional) overturning is geometrically defined as being the part due to the vertical integral of the product of zonal means of velocity and tracer. The velocity does not include "bolus" or Gent-McWilliams velocity.</rdfs:comment>
    <skos:inScheme rdf:resource="http://purl.oclc.org/NET/ssnx/qu/dim#MassFlowRate"/>
  </skos:Concept>
  <skos:Concept rdf:about="http://purl.oclc.org/NET/ssnx/cf/cf-property#northward_ocean_freshwater_transport_due_to_gyre">
    <rdfs:isDefinedBy rdf:resource="http://purl.oclc.org/NET/ssnx/cf/cf-property"/>
    <j.0:generalQuantityKind rdf:resource="http://purl.oclc.org/NET/ssnx/qu/quantity#massFlowRate"/>
    <rdfs:label>northward ocean freshwater transport due to gyre</rdfs:label>
    <rdfs:comment>The specification of a physical process by the phrase due_to_process means that the quantity named is a single term in a sum of terms which together compose the general quantity named by omitting the phrase. "Northward" indicates a vector component which is positive when directed northward (negative southward). Northward transport by the ocean gyre is geometrically defined as being the part due to the vertical integral of the product of deviations of velocity and tracer from their zonal means. The velocity does not include "bolus" or Gent-McWilliams velocity.</rdfs:comment>
    <skos:inScheme rdf:resource="http://purl.oclc.org/NET/ssnx/qu/dim#MassFlowRate"/>
  </skos:Concept>
  <skos:Concept rdf:about="http://purl.oclc.org/NET/ssnx/cf/cf-property#northward_ocean_salt_transport">
    <rdfs:isDefinedBy rdf:resource="http://purl.oclc.org/NET/ssnx/cf/cf-property"/>
    <j.0:generalQuantityKind rdf:resource="http://purl.oclc.org/NET/ssnx/qu/quantity#massFlowRate"/>
    <rdfs:label>northward ocean salt transport</rdfs:label>
    <rdfs:comment>"Northward" indicates a vector component which is positive when directed northward (negative southward). Ocean transport means transport by all processes, both sea water and sea ice.</rdfs:comment>
    <skos:inScheme rdf:resource="http://purl.oclc.org/NET/ssnx/qu/dim#MassFlowRate"/>
  </skos:Concept>
  <skos:Concept rdf:about="http://purl.oclc.org/NET/ssnx/cf/cf-property#northward_ocean_freshwater_transport_due_to_bolus_advection">
    <rdfs:isDefinedBy rdf:resource="http://purl.oclc.org/NET/ssnx/cf/cf-property"/>
    <j.0:generalQuantityKind rdf:resource="http://purl.oclc.org/NET/ssnx/qu/quantity#massFlowRate"/>
    <rdfs:label>northward ocean freshwater transport due to bolus advection</rdfs:label>
    <rdfs:comment>The specification of a physical process by the phrase due_to_process means that the quantity named is a single term in a sum of terms which together compose the general quantity named by omitting the phrase. "Northward" indicates a vector component which is positive when directed northward (negative southward). Northward transport by bolus advection in an ocean model means the part due to a scheme representing eddy-induced effects not included in the velocity field.</rdfs:comment>
    <skos:inScheme rdf:resource="http://purl.oclc.org/NET/ssnx/qu/dim#MassFlowRate"/>
  </skos:Concept>
  <skos:Concept rdf:about="http://purl.oclc.org/NET/ssnx/cf/cf-property#upward_ocean_mass_transport">
    <rdfs:isDefinedBy rdf:resource="http://purl.oclc.org/NET/ssnx/cf/cf-property"/>
    <j.0:generalQuantityKind rdf:resource="http://purl.oclc.org/NET/ssnx/qu/quantity#massFlowRate"/>
    <rdfs:label>upward ocean mass transport</rdfs:label>
    <rdfs:comment> "Upward" indicates a vector component which is positive when directed upward (negative downward). </rdfs:comment>
    <skos:inScheme rdf:resource="http://purl.oclc.org/NET/ssnx/qu/dim#MassFlowRate"/>
  </skos:Concept>
  <skos:Concept rdf:about="http://purl.oclc.org/NET/ssnx/cf/cf-property#ocean_mass_y_transport_due_to_advection">
    <rdfs:isDefinedBy rdf:resource="http://purl.oclc.org/NET/ssnx/cf/cf-property"/>
    <j.0:generalQuantityKind rdf:resource="http://purl.oclc.org/NET/ssnx/qu/quantity#massFlowRate"/>
    <rdfs:label>ocean mass y transport due to advection</rdfs:label>
    <rdfs:comment> "y" indicates a vector component along the grid y-axis, when this is not true latitude, positive with increasing y.  The specification of a physical process by the phrase due_to_process means that the quantity named is a  single term in a sum of terms which together compose the general quantity  named by omitting the phrase. </rdfs:comment>
    <skos:inScheme rdf:resource="http://purl.oclc.org/NET/ssnx/qu/dim#MassFlowRate"/>
  </skos:Concept>
  <skos:Concept rdf:about="http://purl.oclc.org/NET/ssnx/cf/cf-property#ocean_mass_y_transport">
    <rdfs:isDefinedBy rdf:resource="http://purl.oclc.org/NET/ssnx/cf/cf-property"/>
    <j.0:generalQuantityKind rdf:resource="http://purl.oclc.org/NET/ssnx/qu/quantity#massFlowRate"/>
    <rdfs:label>ocean mass y transport</rdfs:label>
    <rdfs:comment> "y" indicates a vector component along the grid y-axis, when this is not true latitude, positive with increasing y.</rdfs:comment>
    <skos:inScheme rdf:resource="http://purl.oclc.org/NET/ssnx/qu/dim#MassFlowRate"/>
  </skos:Concept>
  <skos:Concept rdf:about="http://purl.oclc.org/NET/ssnx/cf/cf-property#sea_ice_transport_across_line">
    <rdfs:isDefinedBy rdf:resource="http://purl.oclc.org/NET/ssnx/cf/cf-property"/>
    <j.0:generalQuantityKind rdf:resource="http://purl.oclc.org/NET/ssnx/qu/quantity#massFlowRate"/>
    <rdfs:label>sea ice transport across line</rdfs:label>
    <rdfs:comment>Transport across_line means that which crosses a particular line on the Earth's surface; formally this means the integral along the line of the normal component of the transport.</rdfs:comment>
    <skos:inScheme rdf:resource="http://purl.oclc.org/NET/ssnx/qu/dim#MassFlowRate"/>
  </skos:Concept>
  <skos:Concept rdf:about="http://purl.oclc.org/NET/ssnx/cf/cf-property#northward_ocean_salt_transport_due_to_gyre">
    <rdfs:isDefinedBy rdf:resource="http://purl.oclc.org/NET/ssnx/cf/cf-property"/>
    <j.0:generalQuantityKind rdf:resource="http://purl.oclc.org/NET/ssnx/qu/quantity#massFlowRate"/>
    <rdfs:label>northward ocean salt transport due to gyre</rdfs:label>
    <rdfs:comment>The specification of a physical process by the phrase due_to_process means that the quantity named is a single term in a sum of terms which together compose the general quantity named by omitting the phrase. "Northward" indicates a vector component which is positive when directed northward (negative southward). Northward transport by the ocean gyre is geometrically defined as being the part due to the vertical integral of the product of deviations of velocity and tracer from their zonal means. The velocity does not include "bolus" or Gent-McWilliams velocity.</rdfs:comment>
    <skos:inScheme rdf:resource="http://purl.oclc.org/NET/ssnx/qu/dim#MassFlowRate"/>
  </skos:Concept>
  <skos:Concept rdf:about="http://purl.oclc.org/NET/ssnx/cf/cf-property#ocean_mass_x_transport_due_to_advection_and_bolus_advection">
    <rdfs:isDefinedBy rdf:resource="http://purl.oclc.org/NET/ssnx/cf/cf-property"/>
    <j.0:generalQuantityKind rdf:resource="http://purl.oclc.org/NET/ssnx/qu/quantity#massFlowRate"/>
    <rdfs:label>ocean mass x transport due to advection and bolus advection</rdfs:label>
    <rdfs:comment> "x" indicates a vector component along the grid x-axis, when this is not true longitude, positive with increasing x.  The specification of a physical process by the phrase due_to_process means that the quantity named is a  single term in a sum of terms which together compose the general quantity  named by omitting the phrase.  Transport by bolus advection in an ocean model means the part due to a scheme representing eddy-induced effects not included in the velocity field. </rdfs:comment>
    <skos:inScheme rdf:resource="http://purl.oclc.org/NET/ssnx/qu/dim#MassFlowRate"/>
  </skos:Concept>
  <skos:Concept rdf:about="http://purl.oclc.org/NET/ssnx/cf/cf-property#ocean_y_overturning_mass_streamfunction_due_to_bolus_advection">
    <rdfs:isDefinedBy rdf:resource="http://purl.oclc.org/NET/ssnx/cf/cf-property"/>
    <j.0:generalQuantityKind rdf:resource="http://purl.oclc.org/NET/ssnx/qu/quantity#massFlowRate"/>
    <rdfs:label>ocean y overturning mass streamfunction due to bolus advection</rdfs:label>
    <rdfs:comment> "y" indicates a vector component along the grid y-axis, when this is not true latitude, positive with increasing y.  The specification of a physical process by the phrase due_to_process means that the quantity named is a  single term in a sum of terms which together compose the general quantity  named by omitting the phrase. </rdfs:comment>
    <skos:inScheme rdf:resource="http://purl.oclc.org/NET/ssnx/qu/dim#MassFlowRate"/>
  </skos:Concept>
</rdf:RDF>
