<rdf:RDF
    xmlns:rdf="http://www.w3.org/1999/02/22-rdf-syntax-ns#"
    xmlns:dcterms="http://purl.org/dc/terms/"
    xmlns:dc="http://purl.org/dc/elements/1.1/"
    xmlns:owl="http://www.w3.org/2002/07/owl#"
    xmlns:dcmit="http://purl.org/dc/dcmitype/"
    xmlns:skos="http://www.w3.org/2004/02/skos/core#"
    xmlns:voaf="http://purl.org/vocommons/voaf#"
    xmlns:rdfs="http://www.w3.org/2000/01/rdf-schema#"
    xmlns:vann="http://purl.org/vocab/vann/">
  <owl:Ontology rdf:about="http://purl.org/eem"/>
  <owl:ObjectProperty rdf:about="http://purl.org/eem#action">
    <rdfs:range>
      <skos:ConceptScheme rdf:about="http://purl.org/eem#Action">
        <rdfs:isDefinedBy rdf:resource="http://purl.org/eem"/>
        <rdfs:comment>The Action type says how an event relates to the lifecycle of the entity being described.</rdfs:comment>
      </skos:ConceptScheme>
    </rdfs:range>
  </owl:ObjectProperty>
  <skos:Concept rdf:about="http://purl.org/eem#OBSERVE">
    <rdfs:isDefinedBy rdf:resource="http://purl.org/eem"/>
    <rdfs:comment>The entity in question has not been changed: it has neither been created, added to, destroyed, or removed from.</rdfs:comment>
    <skos:inScheme rdf:resource="http://purl.org/eem#Action"/>
  </skos:Concept>
  <skos:Concept rdf:about="http://purl.org/eem#ADD">
    <rdfs:isDefinedBy rdf:resource="http://purl.org/eem"/>
    <rdfs:comment>The entity in question has been created or added to</rdfs:comment>
    <skos:inScheme rdf:resource="http://purl.org/eem#Action"/>
  </skos:Concept>
  <skos:Concept rdf:about="http://purl.org/eem#DELETE">
    <rdfs:isDefinedBy rdf:resource="http://purl.org/eem"/>
    <rdfs:comment>The entity in question has been removed from or destroyed
altogether. </rdfs:comment>
    <skos:inScheme rdf:resource="http://purl.org/eem#Action"/>
  </skos:Concept>
</rdf:RDF>
