<rdf:RDF
    xmlns:rdf="http://www.w3.org/1999/02/22-rdf-syntax-ns#"
    xmlns:dcterms="http://purl.org/dc/terms/"
    xmlns:dc="http://purl.org/dc/elements/1.1/"
    xmlns:owl="http://www.w3.org/2002/07/owl#"
    xmlns:dcmit="http://purl.org/dc/dcmitype/"
    xmlns:skos="http://www.w3.org/2004/02/skos/core#"
    xmlns:voaf="http://purl.org/vocommons/voaf#"
    xmlns:rdfs="http://www.w3.org/2000/01/rdf-schema#"
    xmlns:vann="http://purl.org/vocab/vann/">
  <owl:Ontology rdf:about="http://purl.org/cwmo/#"/>
  <owl:AsymmetricProperty rdf:about="http://purl.org/cwmo/#progress">
    <rdf:type rdf:resource="http://www.w3.org/2002/07/owl#IrreflexiveProperty"/>
    <rdf:type rdf:resource="http://www.w3.org/2002/07/owl#FunctionalProperty"/>
    <rdf:type rdf:resource="http://www.w3.org/2002/07/owl#ObjectProperty"/>
    <rdfs:domain rdf:resource="http://purl.org/cwmo/#CreativeWorkshop"/>
    <rdfs:range>
      <skos:ConceptScheme rdf:about="http://purl.org/cwmo/#CreativePhase">
        <rdfs:isDefinedBy rdf:resource="http://purl.org/cwmo/#"/>
        <rdfs:label xml:lang="en">Creative Phase</rdfs:label>
        <rdfs:comment xml:lang="en">The creative phase class is the decompastion of the creative process into steps/ phases which implies different nature of activities, goals and interaction.</rdfs:comment>
      </skos:ConceptScheme>
    </rdfs:range>
  </owl:AsymmetricProperty>
  <owl:AsymmetricProperty rdf:about="http://purl.org/cwmo/#hasCreativePhase">
    <rdf:type rdf:resource="http://www.w3.org/2002/07/owl#ObjectProperty"/>
    <rdfs:domain rdf:resource="http://purl.org/cwmo/#CreativeTechnique"/>
    <rdfs:range rdf:resource="http://purl.org/cwmo/#CreativePhase"/>
  </owl:AsymmetricProperty>
  <skos:Concept rdf:about="http://purl.org/cwmo/#Synthesis">
    <rdfs:comment xml:lang="en">The synthesis class represent the phase of the creative process where further information a researched. Classification of the application of creative technic based on the Universal Method of Design (Martin et al., 2008).</rdfs:comment>
    <rdfs:seeAlso>
      <skos:Concept rdf:about="http://purl.org/cwmo/#EvalAndRafinement">
        <owl:sameAs>
          <skos:Concept rdf:about="http://purl.org/cwmo/#Implementation">
            <rdfs:seeAlso>
              <skos:Concept rdf:about="http://purl.org/cwmo/#ProblemAnalysis">
                <rdfs:seeAlso rdf:resource="http://purl.org/cwmo/#Implementation"/>
                <rdfs:seeAlso>
                  <skos:Concept rdf:about="http://purl.org/cwmo/#IdeaEvaluation">
                    <rdfs:seeAlso rdf:resource="http://purl.org/cwmo/#ProblemAnalysis"/>
                    <rdfs:seeAlso rdf:resource="http://purl.org/cwmo/#Implementation"/>
                    <owl:sameAs rdf:resource="http://purl.org/cwmo/#Implementation"/>
                    <rdfs:seeAlso>
                      <skos:Concept rdf:about="http://purl.org/cwmo/#Ideation">
                        <rdfs:seeAlso rdf:resource="http://purl.org/cwmo/#ProblemAnalysis"/>
                        <rdfs:seeAlso rdf:resource="http://purl.org/cwmo/#Implementation"/>
                        <rdfs:isDefinedBy rdf:resource="http://purl.org/cwmo/#"/>
                        <rdfs:seeAlso rdf:resource="http://purl.org/cwmo/#IdeaEvaluation"/>
                        <rdfs:label xml:lang="en">Ideation</rdfs:label>
                        <rdfs:comment xml:lang="en">The ideation class is a phase of the creative process where ideas to respond to the problematic are generated.</rdfs:comment>
                        <skos:inScheme rdf:resource="http://purl.org/cwmo/#CreativePhase"/>
                      </skos:Concept>
                    </rdfs:seeAlso>
                    <rdfs:label xml:lang="en">IdeaEvaluation</rdfs:label>
                    <rdfs:comment xml:lang="en">The idea evaluation class is a phase of the creative process where the idea are evluated, sorted or ranked.</rdfs:comment>
                    <skos:inScheme rdf:resource="http://purl.org/cwmo/#CreativePhase"/>
                    <rdfs:isDefinedBy rdf:resource="http://purl.org/cwmo/#"/>
                  </skos:Concept>
                </rdfs:seeAlso>
                <rdfs:seeAlso rdf:resource="http://purl.org/cwmo/#Ideation"/>
                <rdfs:label xml:lang="en">Problem Analysis</rdfs:label>
                <rdfs:comment xml:lang="en">The problem analysis class is a phase of the creative process where the problem is formalized and the information seeked and organized.</rdfs:comment>
                <skos:inScheme rdf:resource="http://purl.org/cwmo/#CreativePhase"/>
                <rdfs:isDefinedBy rdf:resource="http://purl.org/cwmo/#"/>
              </skos:Concept>
            </rdfs:seeAlso>
            <rdfs:seeAlso rdf:resource="http://purl.org/cwmo/#IdeaEvaluation"/>
            <rdfs:seeAlso rdf:resource="http://purl.org/cwmo/#Ideation"/>
            <rdfs:label xml:lang="en">Implementation</rdfs:label>
            <rdfs:comment xml:lang="en">The implementation class is a phase of the creative process where the most interesting ideas are experimented in real condition.</rdfs:comment>
            <skos:inScheme rdf:resource="http://purl.org/cwmo/#CreativePhase"/>
            <rdfs:isDefinedBy rdf:resource="http://purl.org/cwmo/#"/>
          </skos:Concept>
        </owl:sameAs>
        <owl:sameAs rdf:resource="http://purl.org/cwmo/#IdeaEvaluation"/>
        <rdfs:label xml:lang="en">Evaluation and Rafinement</rdfs:label>
        <rdfs:comment xml:lang="en">The evaluation and rafinement is an iterative phase of testing and feedback about a production. Classification of the application of creative technic based on the Universal Method of Design (Martin et al., 2008).</rdfs:comment>
        <skos:inScheme rdf:resource="http://purl.org/cwmo/#CreativePhase"/>
        <rdfs:isDefinedBy rdf:resource="http://purl.org/cwmo/#"/>
      </skos:Concept>
    </rdfs:seeAlso>
    <rdfs:seeAlso>
      <skos:Concept rdf:about="http://purl.org/cwmo/#Definition">
        <rdfs:label xml:lang="en">planning, scoping and definition</rdfs:label>
        <rdfs:comment xml:lang="en">The defintion class is a phase of the creative process where project parameters are explored and defined. Classification of the application of creative technic based on the Universal Method of Design (Martin et al., 2008).</rdfs:comment>
        <skos:inScheme rdf:resource="http://purl.org/cwmo/#CreativePhase"/>
        <rdfs:isDefinedBy rdf:resource="http://purl.org/cwmo/#"/>
      </skos:Concept>
    </rdfs:seeAlso>
    <rdfs:isDefinedBy rdf:resource="http://purl.org/cwmo/#"/>
    <rdfs:seeAlso>
      <skos:Concept rdf:about="http://purl.org/cwmo/#ImplementAndMonitoring">
        <rdfs:isDefinedBy rdf:resource="http://purl.org/cwmo/#"/>
        <rdfs:label xml:lang="en">Lunch and Monitoring</rdfs:label>
        <rdfs:comment xml:lang="en">The Implementation and monitoring class is a phase of the creative process where the readiness of the idea  is tested. Classification of the application of creative technic based on the Universal Method of Design (Martin et al., 2008).</rdfs:comment>
        <skos:inScheme rdf:resource="http://purl.org/cwmo/#CreativePhase"/>
      </skos:Concept>
    </rdfs:seeAlso>
    <rdfs:comment xml:lang="en">Exploration, synthesis and design implications</rdfs:comment>
    <skos:inScheme rdf:resource="http://purl.org/cwmo/#CreativePhase"/>
  </skos:Concept>
  <skos:Concept rdf:about="http://purl.org/cwmo/#ConceptGeneration">
    <rdfs:isDefinedBy rdf:resource="http://purl.org/cwmo/#"/>
    <owl:sameAs rdf:resource="http://purl.org/cwmo/#Ideation"/>
    <rdfs:label xml:lang="en">Concept generation and early prototyping</rdfs:label>
    <rdfs:comment xml:lang="en">the phase of concept generation and eraly prototyping is an itarative phase that involves participatory and generative design activities. Classification of the application of creative technic based on the Universal Method of Design (Martin et al., 2008).</rdfs:comment>
    <skos:inScheme rdf:resource="http://purl.org/cwmo/#CreativePhase"/>
  </skos:Concept>
</rdf:RDF>
