<rdf:RDF
    xmlns:dct="http://purl.org/dc/terms/"
    xmlns:rdf="http://www.w3.org/1999/02/22-rdf-syntax-ns#"
    xmlns:dc="http://purl.org/dc/elements/1.1/"
    xmlns:owl="http://www.w3.org/2002/07/owl#"
    xmlns:dcmit="http://purl.org/dc/dcmitype/"
    xmlns:skos="http://www.w3.org/2004/02/skos/core#"
    xmlns:voaf="http://purl.org/vocommons/voaf#"
    xmlns:rdfs="http://www.w3.org/2000/01/rdf-schema#"
    xmlns:vann="http://purl.org/vocab/vann/">
  <owl:Ontology rdf:about="http://purl.org/opdm/refrigerator#"/>
  <owl:ObjectProperty rdf:about="http://purl.org/opdm/refrigerator#typeOfBody">
    <rdfs:isDefinedBy rdf:resource="http://purl.org/opdm/refrigerator#"/>
    <rdfs:comment xml:lang="en">The type of body frame that the fridge/freezer is equipped with.</rdfs:comment>
    <rdfs:label xml:lang="en">Type of body</rdfs:label>
    <rdfs:domain>
      <rdf:Description rdf:about="http://purl.org/opdm/refrigerator#FridgeFreezer">
        <rdfs:isDefinedBy rdf:resource="http://purl.org/opdm/refrigerator#"/>
      </rdf:Description>
    </rdfs:domain>
    <rdfs:range>
      <skos:ConceptScheme rdf:about="http://purl.org/opdm/refrigerator#TypeOfBody">
        <rdfs:isDefinedBy rdf:resource="http://purl.org/opdm/refrigerator#"/>
        <rdfs:label xml:lang="en">Class to represent the different types of body frames of a fridge/freezer. Possible values include: built-in, free-standing.</rdfs:label>
        <rdfs:comment xml:lang="en">Class to represent the different types of body frames of a fridge/freezer. Possible values include: built-in, free-standing.</rdfs:comment>
      </skos:ConceptScheme>
    </rdfs:range>
  </owl:ObjectProperty>
  <skos:Concept rdf:about="http://purl.org/opdm/refrigerator#Chest">
    <rdfs:isDefinedBy rdf:resource="http://purl.org/opdm/refrigerator#"/>
    <rdfs:label xml:lang="en">Chest</rdfs:label>
    <rdfs:comment xml:lang="en">It represents a chest type of body frame for a fridge/freezer.</rdfs:comment>
    <skos:inScheme rdf:resource="http://purl.org/opdm/refrigerator#TypeOfBody"/>
  </skos:Concept>
  <skos:Concept rdf:about="http://purl.org/opdm/refrigerator#FreeStanding">
    <rdfs:isDefinedBy rdf:resource="http://purl.org/opdm/refrigerator#"/>
    <rdfs:label xml:lang="en">FreeStanding</rdfs:label>
    <rdfs:comment xml:lang="en">It represents a free-standing type of body frame for a fridge/freezer.</rdfs:comment>
    <skos:inScheme rdf:resource="http://purl.org/opdm/refrigerator#TypeOfBody"/>
  </skos:Concept>
  <skos:Concept rdf:about="http://purl.org/opdm/refrigerator#BuiltIn">
    <rdfs:isDefinedBy rdf:resource="http://purl.org/opdm/refrigerator#"/>
    <rdfs:label xml:lang="en">BuiltIn</rdfs:label>
    <rdfs:comment xml:lang="en">It represents a bult-in type of body frame for a fridge/freezer.</rdfs:comment>
    <skos:inScheme rdf:resource="http://purl.org/opdm/refrigerator#TypeOfBody"/>
  </skos:Concept>
</rdf:RDF>
