<rdf:RDF
    xmlns:rdf="http://www.w3.org/1999/02/22-rdf-syntax-ns#"
    xmlns:dcterms="http://purl.org/dc/terms/"
    xmlns:dc="http://purl.org/dc/elements/1.1/"
    xmlns:owl="http://www.w3.org/2002/07/owl#"
    xmlns:dcmit="http://purl.org/dc/dcmitype/"
    xmlns:skos="http://www.w3.org/2004/02/skos/core#"
    xmlns:voaf="http://purl.org/vocommons/voaf#"
    xmlns:rdfs="http://www.w3.org/2000/01/rdf-schema#"
    xmlns:vann="http://purl.org/vocab/vann/">
  <owl:Ontology rdf:about="https://vocab.eccenca.com/pubsub/"/>
  <owl:ObjectProperty rdf:about="https://vocab.eccenca.com/pubsub/requestState">
    <rdfs:comment xml:lang="en">The state of a subscription request.</rdfs:comment>
    <rdfs:label xml:lang="en">has subscription request state</rdfs:label>
    <rdfs:domain rdf:resource="https://vocab.eccenca.com/pubsub/SubscriptionRequest"/>
    <rdfs:range>
      <skos:ConceptScheme rdf:about="https://vocab.eccenca.com/pubsub/SubscriptionRequestState">
        <rdfs:isDefinedBy rdf:resource="https://vocab.eccenca.com/pubsub/"/>
        <rdfs:label xml:lang="en">subscription request state</rdfs:label>
        <rdfs:comment xml:lang="en">A state of a subscription request.</rdfs:comment>
      </skos:ConceptScheme>
    </rdfs:range>
  </owl:ObjectProperty>
  <skos:Concept rdf:about="https://vocab.eccenca.com/pubsub/SUBSCRIPTION_REQUEST_DENIED">
    <rdfs:isDefinedBy rdf:resource="https://vocab.eccenca.com/pubsub/"/>
    <rdfs:label xml:lang="en">request denied</rdfs:label>
    <rdfs:comment xml:lang="en">Indicates that a subscription request was denied.</rdfs:comment>
    <skos:inScheme rdf:resource="https://vocab.eccenca.com/pubsub/SubscriptionRequestState"/>
  </skos:Concept>
  <skos:Concept rdf:about="https://vocab.eccenca.com/pubsub/SUBSCRIPTION_REQUEST_DELETED">
    <rdfs:isDefinedBy rdf:resource="https://vocab.eccenca.com/pubsub/"/>
    <rdfs:label xml:lang="en">request deleted</rdfs:label>
    <rdfs:comment xml:lang="en">Indicates that a subscription cancellation request was successfully verified.</rdfs:comment>
    <skos:inScheme rdf:resource="https://vocab.eccenca.com/pubsub/SubscriptionRequestState"/>
  </skos:Concept>
  <skos:Concept rdf:about="https://vocab.eccenca.com/pubsub/SUBSCRIPTION_REQUEST_PENDING">
    <rdfs:isDefinedBy rdf:resource="https://vocab.eccenca.com/pubsub/"/>
    <rdfs:label xml:lang="en">request pending</rdfs:label>
    <rdfs:comment xml:lang="en">Indicates that a subscription request was successfully sent to the hub but is not yet verified.</rdfs:comment>
    <skos:inScheme rdf:resource="https://vocab.eccenca.com/pubsub/SubscriptionRequestState"/>
  </skos:Concept>
  <skos:Concept rdf:about="https://vocab.eccenca.com/pubsub/SUBSCRIPTION_REQUEST_VERIFIED">
    <rdfs:isDefinedBy rdf:resource="https://vocab.eccenca.com/pubsub/"/>
    <rdfs:label xml:lang="en">request verified</rdfs:label>
    <rdfs:comment xml:lang="en">Indicates that a subscription request was successfully validated and verified.</rdfs:comment>
    <skos:inScheme rdf:resource="https://vocab.eccenca.com/pubsub/SubscriptionRequestState"/>
  </skos:Concept>
  <skos:Concept rdf:about="https://vocab.eccenca.com/pubsub/SUBSCRIPTION_REQUEST_CANCELED">
    <rdfs:isDefinedBy rdf:resource="https://vocab.eccenca.com/pubsub/"/>
    <rdfs:label xml:lang="en">request canceled</rdfs:label>
    <rdfs:comment xml:lang="en">Indicates that a subscription cancellation request was successfully sent to the hub but is not yet verified.</rdfs:comment>
    <skos:inScheme rdf:resource="https://vocab.eccenca.com/pubsub/SubscriptionRequestState"/>
  </skos:Concept>
</rdf:RDF>
