<rdf:RDF
    xmlns:rdf="http://www.w3.org/1999/02/22-rdf-syntax-ns#"
    xmlns:dcterms="http://purl.org/dc/terms/"
    xmlns:dc="http://purl.org/dc/elements/1.1/"
    xmlns:owl="http://www.w3.org/2002/07/owl#"
    xmlns:dcmit="http://purl.org/dc/dcmitype/"
    xmlns:skos="http://www.w3.org/2004/02/skos/core#"
    xmlns:voaf="http://purl.org/vocommons/voaf#"
    xmlns:rdfs="http://www.w3.org/2000/01/rdf-schema#"
    xmlns:vann="http://purl.org/vocab/vann/">
  <owl:Ontology rdf:about="http://www.ebusiness-unibw.org/ontologies/consumerelectronics/v1"/>
  <skos:Concept rdf:about="http://www.ebusiness-unibw.org/ontologies/consumerelectronics/v1#TXT">
    <rdfs:isDefinedBy rdf:resource="http://www.ebusiness-unibw.org/ontologies/consumerelectronics/v1"/>
    <rdfs:label xml:lang="en">TXT</rdfs:label>
    <rdfs:comment xml:lang="en">Is a filename extension for files consisting of text usually contain very little formatting.</rdfs:comment>
    <skos:inScheme>
      <skos:ConceptScheme rdf:about="http://www.ebusiness-unibw.org/ontologies/consumerelectronics/v1#DataFormatOffice">
        <rdfs:isDefinedBy rdf:resource="http://www.ebusiness-unibw.org/ontologies/consumerelectronics/v1"/>
        <rdfs:label xml:lang="en">Data Format Office</rdfs:label>
        <rdfs:comment xml:lang="en">A data format is a particular way to encode information for storage in a computer file (refers to office data).

(This description is partly based on or reuses content from the Wikipedia article "File Format" (http://en.wikipedia.org/wiki/File_format) and is licensed under the GNU Free Documentation License (http://www.gnu.org/copyleft/fdl.html).)</rdfs:comment>
      </skos:ConceptScheme>
    </skos:inScheme>
  </skos:Concept>
  <skos:Concept rdf:about="http://www.ebusiness-unibw.org/ontologies/consumerelectronics/v1#DOC">
    <rdfs:isDefinedBy rdf:resource="http://www.ebusiness-unibw.org/ontologies/consumerelectronics/v1"/>
    <rdfs:label xml:lang="en">DOC</rdfs:label>
    <rdfs:comment xml:lang="en">A file extension for word processing documents.</rdfs:comment>
    <skos:inScheme rdf:resource="http://www.ebusiness-unibw.org/ontologies/consumerelectronics/v1#DataFormatOffice"/>
  </skos:Concept>
  <skos:Concept rdf:about="http://www.ebusiness-unibw.org/ontologies/consumerelectronics/v1#PDF">
    <rdfs:isDefinedBy rdf:resource="http://www.ebusiness-unibw.org/ontologies/consumerelectronics/v1"/>
    <rdfs:label xml:lang="en">PDF</rdfs:label>
    <rdfs:comment xml:lang="en">Portable Document Format (PDF) is a file format created by Adobe Systems in 1993 for document exchange.

(This description is partly based on or reuses content from the Wikipedia article "Pdf" (http://en.wikipedia.org/wiki/Pdf) and is licensed under the GNU Free Documentation License (http://www.gnu.org/copyleft/fdl.html).)</rdfs:comment>
    <skos:inScheme rdf:resource="http://www.ebusiness-unibw.org/ontologies/consumerelectronics/v1#DataFormatOffice"/>
  </skos:Concept>
</rdf:RDF>
