<rdf:RDF
    xmlns:rdf="http://www.w3.org/1999/02/22-rdf-syntax-ns#"
    xmlns:dcterms="http://purl.org/dc/terms/"
    xmlns:dc="http://purl.org/dc/elements/1.1/"
    xmlns:owl="http://www.w3.org/2002/07/owl#"
    xmlns:dcmit="http://purl.org/dc/dcmitype/"
    xmlns:skos="http://www.w3.org/2004/02/skos/core#"
    xmlns:voaf="http://purl.org/vocommons/voaf#"
    xmlns:rdfs="http://www.w3.org/2000/01/rdf-schema#"
    xmlns:vann="http://purl.org/vocab/vann/">
  <owl:Ontology rdf:about="http://rdf.geospecies.org/ont/geospecies"/>
  <skos:Concept rdf:about="http://rdf.geospecies.org/ont/geospecies#nativeness_managed">
    <rdfs:isDefinedBy rdf:resource="http://rdf.geospecies.org/ont/geospecies"/>
    <rdfs:label>Managed</rdfs:label>
    <rdfs:comment>The organism maintains its presence through intentional cultivation or husbandry</rdfs:comment>
    <skos:inScheme>
      <skos:ConceptScheme rdf:about="http://rdf.geospecies.org/ont/geospecies#Nativeness">
        <rdfs:isDefinedBy rdf:resource="http://rdf.geospecies.org/ont/geospecies"/>
        <rdfs:label>Nativeness</rdfs:label>
      </skos:ConceptScheme>
    </skos:inScheme>
  </skos:Concept>
  <skos:Concept rdf:about="http://rdf.geospecies.org/ont/geospecies#nativeness_native">
    <rdfs:isDefinedBy rdf:resource="http://rdf.geospecies.org/ont/geospecies"/>
    <rdfs:label>Native</rdfs:label>
    <rdfs:comment>The organism either evolved in this region or arrived by non-anthropogenic means</rdfs:comment>
    <skos:inScheme rdf:resource="http://rdf.geospecies.org/ont/geospecies#Nativeness"/>
  </skos:Concept>
  <skos:Concept rdf:about="http://rdf.geospecies.org/ont/geospecies#nativeness_introduced">
    <rdfs:isDefinedBy rdf:resource="http://rdf.geospecies.org/ont/geospecies"/>
    <rdfs:label>Introduced</rdfs:label>
    <rdfs:comment>The organism arrived in the region via an anthropogenic mechanism or mechanisms</rdfs:comment>
    <skos:inScheme rdf:resource="http://rdf.geospecies.org/ont/geospecies#Nativeness"/>
  </skos:Concept>
  <skos:Concept rdf:about="http://rdf.geospecies.org/ont/geospecies#nativeness_invasive">
    <rdfs:isDefinedBy rdf:resource="http://rdf.geospecies.org/ont/geospecies"/>
    <rdfs:label>Invasive</rdfs:label>
    <rdfs:comment>The organism is having a deleterious impact on another organism, multiple organisms or the ecosystem as a whole</rdfs:comment>
    <skos:inScheme rdf:resource="http://rdf.geospecies.org/ont/geospecies#Nativeness"/>
  </skos:Concept>
  <skos:Concept rdf:about="http://rdf.geospecies.org/ont/geospecies#nativeness_naturalised">
    <rdfs:isDefinedBy rdf:resource="http://rdf.geospecies.org/ont/geospecies"/>
    <rdfs:label>Naturalised</rdfs:label>
    <rdfs:comment>The organism reproduces naturally and forms part of the local ecology</rdfs:comment>
    <skos:inScheme rdf:resource="http://rdf.geospecies.org/ont/geospecies#Nativeness"/>
  </skos:Concept>
</rdf:RDF>
