<rdf:RDF
    xmlns:rdf="http://www.w3.org/1999/02/22-rdf-syntax-ns#"
    xmlns:dcterms="http://purl.org/dc/terms/"
    xmlns:dc="http://purl.org/dc/elements/1.1/"
    xmlns:owl="http://www.w3.org/2002/07/owl#"
    xmlns:dcmit="http://purl.org/dc/dcmitype/"
    xmlns:skos="http://www.w3.org/2004/02/skos/core#"
    xmlns:voaf="http://purl.org/vocommons/voaf#"
    xmlns:rdfs="http://www.w3.org/2000/01/rdf-schema#"
    xmlns:vann="http://purl.org/vocab/vann/">
  <owl:Ontology rdf:about="http://www.ontology-of-units-of-measure.org/resource/om-2/"/>
  <skos:Concept rdf:about="http://www.ontology-of-units-of-measure.org/resource/om-2/teragramPerLitre">
    <rdfs:isDefinedBy rdf:resource="http://www.ontology-of-units-of-measure.org/resource/om-2/"/>
    <rdfs:label xml:lang="en">teragram per litre</rdfs:label>
    <rdfs:comment xml:lang="en">Teragram per litre is a unit of density defined as teragram divided by litre.</rdfs:comment>
    <skos:inScheme>
      <skos:ConceptScheme rdf:about="http://www.ontology-of-units-of-measure.org/resource/om-2/PrefixedGramPerLitre">
        <rdfs:isDefinedBy rdf:resource="http://www.ontology-of-units-of-measure.org/resource/om-2/"/>
        <rdfs:label xml:lang="en">prefixed gram per litre</rdfs:label>
      </skos:ConceptScheme>
    </skos:inScheme>
  </skos:Concept>
  <skos:Concept rdf:about="http://www.ontology-of-units-of-measure.org/resource/om-2/megagramPerLitre">
    <rdfs:isDefinedBy rdf:resource="http://www.ontology-of-units-of-measure.org/resource/om-2/"/>
    <rdfs:label xml:lang="en">megagram per litre</rdfs:label>
    <rdfs:comment xml:lang="en">Megagram per litre is a unit of density defined as megagram divided by litre.</rdfs:comment>
    <skos:inScheme rdf:resource="http://www.ontology-of-units-of-measure.org/resource/om-2/PrefixedGramPerLitre"/>
  </skos:Concept>
  <skos:Concept rdf:about="http://www.ontology-of-units-of-measure.org/resource/om-2/centigramPerLitre">
    <rdfs:isDefinedBy rdf:resource="http://www.ontology-of-units-of-measure.org/resource/om-2/"/>
    <rdfs:label xml:lang="en">centigram per litre</rdfs:label>
    <rdfs:comment xml:lang="en">Centigram per litre is a unit of density defined as centigram divided by litre.</rdfs:comment>
    <skos:inScheme rdf:resource="http://www.ontology-of-units-of-measure.org/resource/om-2/PrefixedGramPerLitre"/>
  </skos:Concept>
  <skos:Concept rdf:about="http://www.ontology-of-units-of-measure.org/resource/om-2/yoctogramPerLitre">
    <rdfs:isDefinedBy rdf:resource="http://www.ontology-of-units-of-measure.org/resource/om-2/"/>
    <rdfs:label xml:lang="en">yoctogram per litre</rdfs:label>
    <rdfs:comment xml:lang="en">Yoctogram per litre is a unit of density defined as yoctogram divided by litre.</rdfs:comment>
    <skos:inScheme rdf:resource="http://www.ontology-of-units-of-measure.org/resource/om-2/PrefixedGramPerLitre"/>
  </skos:Concept>
  <skos:Concept rdf:about="http://www.ontology-of-units-of-measure.org/resource/om-2/decagramPerLitre">
    <rdfs:isDefinedBy rdf:resource="http://www.ontology-of-units-of-measure.org/resource/om-2/"/>
    <rdfs:label xml:lang="en">decagram per litre</rdfs:label>
    <rdfs:comment xml:lang="en">Decagram per litre is a unit of density defined as decagram divided by litre.</rdfs:comment>
    <skos:inScheme rdf:resource="http://www.ontology-of-units-of-measure.org/resource/om-2/PrefixedGramPerLitre"/>
  </skos:Concept>
  <skos:Concept rdf:about="http://www.ontology-of-units-of-measure.org/resource/om-2/yottagramPerLitre">
    <rdfs:isDefinedBy rdf:resource="http://www.ontology-of-units-of-measure.org/resource/om-2/"/>
    <rdfs:label xml:lang="en">yottagram per litre</rdfs:label>
    <rdfs:comment xml:lang="en">Yottagram per litre is a unit of density defined as yottagram divided by litre.</rdfs:comment>
    <skos:inScheme rdf:resource="http://www.ontology-of-units-of-measure.org/resource/om-2/PrefixedGramPerLitre"/>
  </skos:Concept>
  <skos:Concept rdf:about="http://www.ontology-of-units-of-measure.org/resource/om-2/decigramPerLitre">
    <rdfs:isDefinedBy rdf:resource="http://www.ontology-of-units-of-measure.org/resource/om-2/"/>
    <rdfs:label xml:lang="en">decigram per litre</rdfs:label>
    <rdfs:comment xml:lang="en">Decigram per litre is a unit of density defined as decigram divided by litre.</rdfs:comment>
    <skos:inScheme rdf:resource="http://www.ontology-of-units-of-measure.org/resource/om-2/PrefixedGramPerLitre"/>
  </skos:Concept>
  <skos:Concept rdf:about="http://www.ontology-of-units-of-measure.org/resource/om-2/petagramPerLitre">
    <rdfs:isDefinedBy rdf:resource="http://www.ontology-of-units-of-measure.org/resource/om-2/"/>
    <rdfs:label xml:lang="en">petagram per litre</rdfs:label>
    <rdfs:comment xml:lang="en">Petagram per litre is a unit of density defined as petagram divided by litre.</rdfs:comment>
    <skos:inScheme rdf:resource="http://www.ontology-of-units-of-measure.org/resource/om-2/PrefixedGramPerLitre"/>
  </skos:Concept>
  <skos:Concept rdf:about="http://www.ontology-of-units-of-measure.org/resource/om-2/zettagramPerLitre">
    <rdfs:isDefinedBy rdf:resource="http://www.ontology-of-units-of-measure.org/resource/om-2/"/>
    <rdfs:label xml:lang="en">zettagram per litre</rdfs:label>
    <rdfs:comment xml:lang="en">Zettagram per litre is a unit of density defined as zettagram divided by litre.</rdfs:comment>
    <skos:inScheme rdf:resource="http://www.ontology-of-units-of-measure.org/resource/om-2/PrefixedGramPerLitre"/>
  </skos:Concept>
  <skos:Concept rdf:about="http://www.ontology-of-units-of-measure.org/resource/om-2/zeptogramPerLitre">
    <rdfs:isDefinedBy rdf:resource="http://www.ontology-of-units-of-measure.org/resource/om-2/"/>
    <rdfs:label xml:lang="en">zeptogram per litre</rdfs:label>
    <rdfs:comment xml:lang="en">Zeptogram per litre is a unit of density defined as zeptogram divided by litre.</rdfs:comment>
    <skos:inScheme rdf:resource="http://www.ontology-of-units-of-measure.org/resource/om-2/PrefixedGramPerLitre"/>
  </skos:Concept>
  <skos:Concept rdf:about="http://www.ontology-of-units-of-measure.org/resource/om-2/exagramPerLitre">
    <rdfs:isDefinedBy rdf:resource="http://www.ontology-of-units-of-measure.org/resource/om-2/"/>
    <rdfs:label xml:lang="en">exagram per litre</rdfs:label>
    <rdfs:comment xml:lang="en">Exagram per litre is a unit of density defined as exagram divided by litre.</rdfs:comment>
    <skos:inScheme rdf:resource="http://www.ontology-of-units-of-measure.org/resource/om-2/PrefixedGramPerLitre"/>
  </skos:Concept>
  <skos:Concept rdf:about="http://www.ontology-of-units-of-measure.org/resource/om-2/kilogramPerLitre">
    <rdfs:isDefinedBy rdf:resource="http://www.ontology-of-units-of-measure.org/resource/om-2/"/>
    <rdfs:label xml:lang="en">kilogram per litre</rdfs:label>
    <rdfs:comment xml:lang="en">Kilogram per litre is a unit of density defined as kilogram divided by litre.</rdfs:comment>
    <skos:inScheme rdf:resource="http://www.ontology-of-units-of-measure.org/resource/om-2/PrefixedGramPerLitre"/>
  </skos:Concept>
  <skos:Concept rdf:about="http://www.ontology-of-units-of-measure.org/resource/om-2/milligramPerLitre">
    <rdfs:isDefinedBy rdf:resource="http://www.ontology-of-units-of-measure.org/resource/om-2/"/>
    <rdfs:label xml:lang="en">milligram per litre</rdfs:label>
    <rdfs:comment xml:lang="en">Milligram per litre is a unit of density defined as milligram divided by litre.</rdfs:comment>
    <skos:inScheme rdf:resource="http://www.ontology-of-units-of-measure.org/resource/om-2/PrefixedGramPerLitre"/>
  </skos:Concept>
  <skos:Concept rdf:about="http://www.ontology-of-units-of-measure.org/resource/om-2/hectogramPerLitre">
    <rdfs:isDefinedBy rdf:resource="http://www.ontology-of-units-of-measure.org/resource/om-2/"/>
    <rdfs:label xml:lang="en">hectogram per litre</rdfs:label>
    <rdfs:comment xml:lang="en">Hectogram per litre is a unit of density defined as hectogram divided by litre.</rdfs:comment>
    <skos:inScheme rdf:resource="http://www.ontology-of-units-of-measure.org/resource/om-2/PrefixedGramPerLitre"/>
  </skos:Concept>
  <skos:Concept rdf:about="http://www.ontology-of-units-of-measure.org/resource/om-2/attogramPerLitre">
    <rdfs:isDefinedBy rdf:resource="http://www.ontology-of-units-of-measure.org/resource/om-2/"/>
    <rdfs:label xml:lang="en">attogram per litre</rdfs:label>
    <rdfs:comment xml:lang="en">Attogram per litre is a unit of density defined as attogram divided by litre.</rdfs:comment>
    <skos:inScheme rdf:resource="http://www.ontology-of-units-of-measure.org/resource/om-2/PrefixedGramPerLitre"/>
  </skos:Concept>
  <skos:Concept rdf:about="http://www.ontology-of-units-of-measure.org/resource/om-2/gigagramPerLitre">
    <rdfs:isDefinedBy rdf:resource="http://www.ontology-of-units-of-measure.org/resource/om-2/"/>
    <rdfs:label xml:lang="en">gigagram per litre</rdfs:label>
    <rdfs:comment xml:lang="en">Gigagram per litre is a unit of density defined as gigagram divided by litre.</rdfs:comment>
    <skos:inScheme rdf:resource="http://www.ontology-of-units-of-measure.org/resource/om-2/PrefixedGramPerLitre"/>
  </skos:Concept>
  <skos:Concept rdf:about="http://www.ontology-of-units-of-measure.org/resource/om-2/nanogramPerLitre">
    <rdfs:isDefinedBy rdf:resource="http://www.ontology-of-units-of-measure.org/resource/om-2/"/>
    <rdfs:label xml:lang="en">nanogram per litre</rdfs:label>
    <rdfs:comment xml:lang="en">Nanogram per litre is a unit of density defined as nanogram divided by litre.</rdfs:comment>
    <skos:inScheme rdf:resource="http://www.ontology-of-units-of-measure.org/resource/om-2/PrefixedGramPerLitre"/>
  </skos:Concept>
  <skos:Concept rdf:about="http://www.ontology-of-units-of-measure.org/resource/om-2/femtogramPerLitre">
    <rdfs:isDefinedBy rdf:resource="http://www.ontology-of-units-of-measure.org/resource/om-2/"/>
    <rdfs:label xml:lang="en">femtogram per litre</rdfs:label>
    <rdfs:comment xml:lang="en">Femtogram per litre is a unit of density defined as femtogram divided by litre.</rdfs:comment>
    <skos:inScheme rdf:resource="http://www.ontology-of-units-of-measure.org/resource/om-2/PrefixedGramPerLitre"/>
  </skos:Concept>
  <skos:Concept rdf:about="http://www.ontology-of-units-of-measure.org/resource/om-2/picogramPerLitre">
    <rdfs:isDefinedBy rdf:resource="http://www.ontology-of-units-of-measure.org/resource/om-2/"/>
    <rdfs:label xml:lang="en">picogram per litre</rdfs:label>
    <rdfs:comment xml:lang="en">Picogram per litre is a unit of density defined as picogram divided by litre.</rdfs:comment>
    <skos:inScheme rdf:resource="http://www.ontology-of-units-of-measure.org/resource/om-2/PrefixedGramPerLitre"/>
  </skos:Concept>
  <skos:Concept rdf:about="http://www.ontology-of-units-of-measure.org/resource/om-2/microgramPerLitre">
    <rdfs:isDefinedBy rdf:resource="http://www.ontology-of-units-of-measure.org/resource/om-2/"/>
    <rdfs:label xml:lang="en">microgram per litre</rdfs:label>
    <rdfs:comment xml:lang="en">Microgram per litre is a unit of density defined as microgram divided by litre.</rdfs:comment>
    <skos:inScheme rdf:resource="http://www.ontology-of-units-of-measure.org/resource/om-2/PrefixedGramPerLitre"/>
  </skos:Concept>
</rdf:RDF>
