<rdf:RDF
    xmlns:rdf="http://www.w3.org/1999/02/22-rdf-syntax-ns#"
    xmlns:dcterms="http://purl.org/dc/terms/"
    xmlns:dc="http://purl.org/dc/elements/1.1/"
    xmlns:owl="http://www.w3.org/2002/07/owl#"
    xmlns:dcmit="http://purl.org/dc/dcmitype/"
    xmlns:skos="http://www.w3.org/2004/02/skos/core#"
    xmlns:voaf="http://purl.org/vocommons/voaf#"
    xmlns:rdfs="http://www.w3.org/2000/01/rdf-schema#"
    xmlns:vann="http://purl.org/vocab/vann/">
  <owl:Ontology rdf:about="http://www.ontology-of-units-of-measure.org/resource/om-2/"/>
  <skos:Concept rdf:about="http://www.ontology-of-units-of-measure.org/resource/om-2/molePerExalitre">
    <rdfs:isDefinedBy rdf:resource="http://www.ontology-of-units-of-measure.org/resource/om-2/"/>
    <rdfs:label xml:lang="en">mole per exalitre</rdfs:label>
    <rdfs:comment xml:lang="en">Mole per exalitre is a unit of amount of substance concentration defined as mole divided by exalitre.</rdfs:comment>
    <skos:inScheme>
      <skos:ConceptScheme rdf:about="http://www.ontology-of-units-of-measure.org/resource/om-2/MolePerPrefixedLitre">
        <rdfs:isDefinedBy rdf:resource="http://www.ontology-of-units-of-measure.org/resource/om-2/"/>
        <rdfs:label xml:lang="en">mole per prefixed litre</rdfs:label>
      </skos:ConceptScheme>
    </skos:inScheme>
  </skos:Concept>
  <skos:Concept rdf:about="http://www.ontology-of-units-of-measure.org/resource/om-2/molePerYoctolitre">
    <rdfs:isDefinedBy rdf:resource="http://www.ontology-of-units-of-measure.org/resource/om-2/"/>
    <rdfs:label xml:lang="en">mole per yoctolitre</rdfs:label>
    <rdfs:comment xml:lang="en">Mole per yoctolitre is a unit of amount of substance concentration defined as mole divided by yoctolitre.</rdfs:comment>
    <skos:inScheme rdf:resource="http://www.ontology-of-units-of-measure.org/resource/om-2/MolePerPrefixedLitre"/>
  </skos:Concept>
  <skos:Concept rdf:about="http://www.ontology-of-units-of-measure.org/resource/om-2/molePerPicolitre">
    <rdfs:isDefinedBy rdf:resource="http://www.ontology-of-units-of-measure.org/resource/om-2/"/>
    <rdfs:label xml:lang="en">mole per picolitre</rdfs:label>
    <rdfs:comment xml:lang="en">Mole per picolitre is a unit of amount of substance concentration defined as mole divided by picolitre.</rdfs:comment>
    <skos:inScheme rdf:resource="http://www.ontology-of-units-of-measure.org/resource/om-2/MolePerPrefixedLitre"/>
  </skos:Concept>
  <skos:Concept rdf:about="http://www.ontology-of-units-of-measure.org/resource/om-2/molePerMegalitre">
    <rdfs:isDefinedBy rdf:resource="http://www.ontology-of-units-of-measure.org/resource/om-2/"/>
    <rdfs:label xml:lang="en">mole per megalitre</rdfs:label>
    <rdfs:comment xml:lang="en">Mole per megalitre is a unit of amount of substance concentration defined as mole divided by megalitre.</rdfs:comment>
    <skos:inScheme rdf:resource="http://www.ontology-of-units-of-measure.org/resource/om-2/MolePerPrefixedLitre"/>
  </skos:Concept>
  <skos:Concept rdf:about="http://www.ontology-of-units-of-measure.org/resource/om-2/molePerFemtolitre">
    <rdfs:isDefinedBy rdf:resource="http://www.ontology-of-units-of-measure.org/resource/om-2/"/>
    <rdfs:label xml:lang="en">mole per femtolitre</rdfs:label>
    <rdfs:comment xml:lang="en">Mole per femtolitre is a unit of amount of substance concentration defined as mole divided by femtolitre.</rdfs:comment>
    <skos:inScheme rdf:resource="http://www.ontology-of-units-of-measure.org/resource/om-2/MolePerPrefixedLitre"/>
  </skos:Concept>
  <skos:Concept rdf:about="http://www.ontology-of-units-of-measure.org/resource/om-2/molePerYottalitre">
    <rdfs:isDefinedBy rdf:resource="http://www.ontology-of-units-of-measure.org/resource/om-2/"/>
    <rdfs:label xml:lang="en">mole per yottalitre</rdfs:label>
    <rdfs:comment xml:lang="en">Mole per yottalitre is a unit of amount of substance concentration defined as mole divided by yottalitre.</rdfs:comment>
    <skos:inScheme rdf:resource="http://www.ontology-of-units-of-measure.org/resource/om-2/MolePerPrefixedLitre"/>
  </skos:Concept>
  <skos:Concept rdf:about="http://www.ontology-of-units-of-measure.org/resource/om-2/molePerTeralitre">
    <rdfs:isDefinedBy rdf:resource="http://www.ontology-of-units-of-measure.org/resource/om-2/"/>
    <rdfs:label xml:lang="en">mole per teralitre</rdfs:label>
    <rdfs:comment xml:lang="en">Mole per teralitre is a unit of amount of substance concentration defined as mole divided by teralitre.</rdfs:comment>
    <skos:inScheme rdf:resource="http://www.ontology-of-units-of-measure.org/resource/om-2/MolePerPrefixedLitre"/>
  </skos:Concept>
  <skos:Concept rdf:about="http://www.ontology-of-units-of-measure.org/resource/om-2/molePerZeptolitre">
    <rdfs:isDefinedBy rdf:resource="http://www.ontology-of-units-of-measure.org/resource/om-2/"/>
    <rdfs:label xml:lang="en">mole per zeptolitre</rdfs:label>
    <rdfs:comment xml:lang="en">Mole per zeptolitre is a unit of amount of substance concentration defined as mole divided by zeptolitre.</rdfs:comment>
    <skos:inScheme rdf:resource="http://www.ontology-of-units-of-measure.org/resource/om-2/MolePerPrefixedLitre"/>
  </skos:Concept>
  <skos:Concept rdf:about="http://www.ontology-of-units-of-measure.org/resource/om-2/molePerPetalitre">
    <rdfs:isDefinedBy rdf:resource="http://www.ontology-of-units-of-measure.org/resource/om-2/"/>
    <rdfs:label xml:lang="en">mole per petalitre</rdfs:label>
    <rdfs:comment xml:lang="en">Mole per petalitre is a unit of amount of substance concentration defined as mole divided by petalitre.</rdfs:comment>
    <skos:inScheme rdf:resource="http://www.ontology-of-units-of-measure.org/resource/om-2/MolePerPrefixedLitre"/>
  </skos:Concept>
  <skos:Concept rdf:about="http://www.ontology-of-units-of-measure.org/resource/om-2/molePerZettalitre">
    <rdfs:isDefinedBy rdf:resource="http://www.ontology-of-units-of-measure.org/resource/om-2/"/>
    <rdfs:label xml:lang="en">mole per zettalitre</rdfs:label>
    <rdfs:comment xml:lang="en">Mole per zettalitre is a unit of amount of substance concentration defined as mole divided by zettalitre.</rdfs:comment>
    <skos:inScheme rdf:resource="http://www.ontology-of-units-of-measure.org/resource/om-2/MolePerPrefixedLitre"/>
  </skos:Concept>
  <skos:Concept rdf:about="http://www.ontology-of-units-of-measure.org/resource/om-2/molePerNanolitre">
    <rdfs:isDefinedBy rdf:resource="http://www.ontology-of-units-of-measure.org/resource/om-2/"/>
    <rdfs:label xml:lang="en">mole per nanolitre</rdfs:label>
    <rdfs:comment xml:lang="en">Mole per nanolitre is a unit of amount of substance concentration defined as mole divided by nanolitre.</rdfs:comment>
    <skos:inScheme rdf:resource="http://www.ontology-of-units-of-measure.org/resource/om-2/MolePerPrefixedLitre"/>
  </skos:Concept>
  <skos:Concept rdf:about="http://www.ontology-of-units-of-measure.org/resource/om-2/molePerCentilitre">
    <rdfs:isDefinedBy rdf:resource="http://www.ontology-of-units-of-measure.org/resource/om-2/"/>
    <rdfs:label xml:lang="en">mole per centilitre</rdfs:label>
    <rdfs:comment xml:lang="en">Mole per centilitre is a unit of amount of substance concentration defined as mole divided by centilitre.</rdfs:comment>
    <skos:inScheme rdf:resource="http://www.ontology-of-units-of-measure.org/resource/om-2/MolePerPrefixedLitre"/>
  </skos:Concept>
  <skos:Concept rdf:about="http://www.ontology-of-units-of-measure.org/resource/om-2/molePerAttolitre">
    <rdfs:isDefinedBy rdf:resource="http://www.ontology-of-units-of-measure.org/resource/om-2/"/>
    <rdfs:label xml:lang="en">mole per attolitre</rdfs:label>
    <rdfs:comment xml:lang="en">Mole per attolitre is a unit of amount of substance concentration defined as mole divided by attolitre.</rdfs:comment>
    <skos:inScheme rdf:resource="http://www.ontology-of-units-of-measure.org/resource/om-2/MolePerPrefixedLitre"/>
  </skos:Concept>
  <skos:Concept rdf:about="http://www.ontology-of-units-of-measure.org/resource/om-2/molePerGigalitre">
    <rdfs:isDefinedBy rdf:resource="http://www.ontology-of-units-of-measure.org/resource/om-2/"/>
    <rdfs:label xml:lang="en">mole per gigalitre</rdfs:label>
    <rdfs:comment xml:lang="en">Mole per gigalitre is a unit of amount of substance concentration defined as mole divided by gigalitre.</rdfs:comment>
    <skos:inScheme rdf:resource="http://www.ontology-of-units-of-measure.org/resource/om-2/MolePerPrefixedLitre"/>
  </skos:Concept>
  <skos:Concept rdf:about="http://www.ontology-of-units-of-measure.org/resource/om-2/molePerDecalitre">
    <rdfs:isDefinedBy rdf:resource="http://www.ontology-of-units-of-measure.org/resource/om-2/"/>
    <rdfs:label xml:lang="en">mole per decalitre</rdfs:label>
    <rdfs:comment xml:lang="en">Mole per decalitre is a unit of amount of substance concentration defined as mole divided by decalitre.</rdfs:comment>
    <skos:inScheme rdf:resource="http://www.ontology-of-units-of-measure.org/resource/om-2/MolePerPrefixedLitre"/>
  </skos:Concept>
  <skos:Concept rdf:about="http://www.ontology-of-units-of-measure.org/resource/om-2/molePerMillilitre">
    <rdfs:isDefinedBy rdf:resource="http://www.ontology-of-units-of-measure.org/resource/om-2/"/>
    <rdfs:label xml:lang="en">mole per millilitre</rdfs:label>
    <rdfs:comment xml:lang="en">Mole per millilitre is a unit of amount of substance concentration defined as mole divided by millilitre.</rdfs:comment>
    <skos:inScheme rdf:resource="http://www.ontology-of-units-of-measure.org/resource/om-2/MolePerPrefixedLitre"/>
  </skos:Concept>
  <skos:Concept rdf:about="http://www.ontology-of-units-of-measure.org/resource/om-2/molePerHectolitre">
    <rdfs:isDefinedBy rdf:resource="http://www.ontology-of-units-of-measure.org/resource/om-2/"/>
    <rdfs:label xml:lang="en">mole per hectolitre</rdfs:label>
    <rdfs:comment xml:lang="en">Mole per hectolitre is a unit of amount of substance concentration defined as mole divided by hectolitre.</rdfs:comment>
    <skos:inScheme rdf:resource="http://www.ontology-of-units-of-measure.org/resource/om-2/MolePerPrefixedLitre"/>
  </skos:Concept>
  <skos:Concept rdf:about="http://www.ontology-of-units-of-measure.org/resource/om-2/molePerDecilitre">
    <rdfs:isDefinedBy rdf:resource="http://www.ontology-of-units-of-measure.org/resource/om-2/"/>
    <rdfs:label xml:lang="en">mole per decilitre</rdfs:label>
    <rdfs:comment xml:lang="en">Mole per decilitre is a unit of amount of substance concentration defined as mole divided by decilitre.</rdfs:comment>
    <skos:inScheme rdf:resource="http://www.ontology-of-units-of-measure.org/resource/om-2/MolePerPrefixedLitre"/>
  </skos:Concept>
  <skos:Concept rdf:about="http://www.ontology-of-units-of-measure.org/resource/om-2/molePerMicrolitre">
    <rdfs:isDefinedBy rdf:resource="http://www.ontology-of-units-of-measure.org/resource/om-2/"/>
    <rdfs:label xml:lang="en">mole per microlitre</rdfs:label>
    <rdfs:comment xml:lang="en">Mole per microlitre is a unit of amount of substance concentration defined as mole divided by microlitre.</rdfs:comment>
    <skos:inScheme rdf:resource="http://www.ontology-of-units-of-measure.org/resource/om-2/MolePerPrefixedLitre"/>
  </skos:Concept>
  <skos:Concept rdf:about="http://www.ontology-of-units-of-measure.org/resource/om-2/molePerKilolitre">
    <rdfs:isDefinedBy rdf:resource="http://www.ontology-of-units-of-measure.org/resource/om-2/"/>
    <rdfs:label xml:lang="en">mole per kilolitre</rdfs:label>
    <rdfs:comment xml:lang="en">Mole per kilolitre is a unit of amount of substance concentration defined as mole divided by kilolitre.</rdfs:comment>
    <skos:inScheme rdf:resource="http://www.ontology-of-units-of-measure.org/resource/om-2/MolePerPrefixedLitre"/>
  </skos:Concept>
</rdf:RDF>
