<rdf:RDF
    xmlns:rdf="http://www.w3.org/1999/02/22-rdf-syntax-ns#"
    xmlns:dcterms="http://purl.org/dc/terms/"
    xmlns:dc="http://purl.org/dc/elements/1.1/"
    xmlns:owl="http://www.w3.org/2002/07/owl#"
    xmlns:dcmit="http://purl.org/dc/dcmitype/"
    xmlns:skos="http://www.w3.org/2004/02/skos/core#"
    xmlns:voaf="http://purl.org/vocommons/voaf#"
    xmlns:rdfs="http://www.w3.org/2000/01/rdf-schema#"
    xmlns:vann="http://purl.org/vocab/vann/">
  <owl:Ontology rdf:about="https://w3id.org/nno/ontology"/>
  <owl:ObjectProperty rdf:about="https://w3id.org/nno/ontology#hasOptimizer">
    <rdfs:comment>Optimization function used by Neural Network (e.g. SGD, Adam or RMSprop).</rdfs:comment>
    <rdfs:label>has optimizer</rdfs:label>
    <rdfs:domain rdf:resource="https://w3id.org/nno/ontology#Model"/>
    <rdfs:range>
      <skos:ConceptScheme rdf:about="https://w3id.org/nno/ontology#Optimizer">
        <rdfs:isDefinedBy rdf:resource="https://w3id.org/nno/ontology"/>
        <rdfs:label>Optimizer</rdfs:label>
        <rdfs:comment>Optimizer used by Neural Network.</rdfs:comment>
      </skos:ConceptScheme>
    </rdfs:range>
  </owl:ObjectProperty>
  <skos:Concept rdf:about="https://w3id.org/nno/ontology#adam">
    <rdfs:isDefinedBy rdf:resource="https://w3id.org/nno/ontology"/>
    <rdfs:label>Adam Optimizer</rdfs:label>
    <skos:inScheme rdf:resource="https://w3id.org/nno/ontology#Optimizer"/>
  </skos:Concept>
  <skos:Concept rdf:about="https://w3id.org/nno/ontology#nadam">
    <rdfs:isDefinedBy rdf:resource="https://w3id.org/nno/ontology"/>
    <rdfs:label>Nesterov Adam Optimizer</rdfs:label>
    <rdfs:comment>Much like Adam is essentially RMSprop with momentum, Nadam is Adam RMSprop with Nesterov momentum.</rdfs:comment>
    <skos:inScheme rdf:resource="https://w3id.org/nno/ontology#Optimizer"/>
  </skos:Concept>
  <skos:Concept rdf:about="https://w3id.org/nno/ontology#customoptimizer">
    <rdfs:isDefinedBy rdf:resource="https://w3id.org/nno/ontology"/>
    <rdfs:label>Custom Optimizer</rdfs:label>
    <rdfs:comment>Custom optimizer defined by user</rdfs:comment>
    <skos:inScheme rdf:resource="https://w3id.org/nno/ontology#Optimizer"/>
  </skos:Concept>
  <skos:Concept rdf:about="https://w3id.org/nno/ontology#adadelta">
    <rdfs:isDefinedBy rdf:resource="https://w3id.org/nno/ontology"/>
    <rdfs:label>Adadelta Optimizer</rdfs:label>
    <rdfs:comment>Adadelta is a more robust extension of Adagrad that adapts learning rates based on a moving window of gradient updates, instead of accumulating all past gradients. This way, Adadelta continues learning even when many updates have been done. Compared to Adagrad, in the original version of Adadelta you don't have to set an initial learning rate. In this version, initial learning rate and decay factor can be set, as in most other Keras optimizers.</rdfs:comment>
    <skos:inScheme rdf:resource="https://w3id.org/nno/ontology#Optimizer"/>
  </skos:Concept>
  <skos:Concept rdf:about="https://w3id.org/nno/ontology#rmsprop">
    <rdfs:isDefinedBy rdf:resource="https://w3id.org/nno/ontology"/>
    <rdfs:label>RMSProp Optimizer</rdfs:label>
    <rdfs:comment>This optimizer is usually a good choice for recurrent neural networks.</rdfs:comment>
    <skos:inScheme rdf:resource="https://w3id.org/nno/ontology#Optimizer"/>
  </skos:Concept>
  <skos:Concept rdf:about="https://w3id.org/nno/ontology#sgd">
    <rdfs:isDefinedBy rdf:resource="https://w3id.org/nno/ontology"/>
    <rdfs:label>Stochastic Gradient Descent Optimizer</rdfs:label>
    <rdfs:comment>Includes support for momentum, learning rate decay, and Nesterov momentum.</rdfs:comment>
    <skos:inScheme rdf:resource="https://w3id.org/nno/ontology#Optimizer"/>
  </skos:Concept>
  <skos:Concept rdf:about="https://w3id.org/nno/ontology#adagrad">
    <rdfs:isDefinedBy rdf:resource="https://w3id.org/nno/ontology"/>
    <rdfs:label>Adagrad Optimizer</rdfs:label>
    <rdfs:comment>Adagrad is an optimizer with parameter-specific learning rates, which are adapted relative to how frequently a parameter gets updated during training. The more updates a parameter receives, the smaller the learning rate.</rdfs:comment>
    <skos:inScheme rdf:resource="https://w3id.org/nno/ontology#Optimizer"/>
  </skos:Concept>
  <skos:Concept rdf:about="https://w3id.org/nno/ontology#adamax">
    <rdfs:isDefinedBy rdf:resource="https://w3id.org/nno/ontology"/>
    <rdfs:label>Adamax Optimizer</rdfs:label>
    <skos:inScheme rdf:resource="https://w3id.org/nno/ontology#Optimizer"/>
  </skos:Concept>
</rdf:RDF>
