<rdf:RDF
    xmlns:rdf="http://www.w3.org/1999/02/22-rdf-syntax-ns#"
    xmlns:dcterms="http://purl.org/dc/terms/"
    xmlns:dc="http://purl.org/dc/elements/1.1/"
    xmlns:owl="http://www.w3.org/2002/07/owl#"
    xmlns:dcmit="http://purl.org/dc/dcmitype/"
    xmlns:skos="http://www.w3.org/2004/02/skos/core#"
    xmlns:voaf="http://purl.org/vocommons/voaf#"
    xmlns:rdfs="http://www.w3.org/2000/01/rdf-schema#"
    xmlns:vann="http://purl.org/vocab/vann/">
  <owl:Ontology rdf:about="https://w3id.org/arco/ontology/context-description"/>
  <owl:ObjectProperty rdf:about="https://w3id.org/arco/ontology/context-description/hasAlternativeDatingType">
    <rdfs:comment xml:lang="en">This property relates an alternative dating to its type.</rdfs:comment>
    <rdfs:label xml:lang="en">has alternative dating type</rdfs:label>
    <rdfs:domain rdf:resource="https://w3id.org/arco/ontology/context-description/AlternativeDating"/>
    <rdfs:range>
      <skos:ConceptScheme rdf:about="https://w3id.org/arco/ontology/context-description/AlternativeDatingType">
        <rdfs:isDefinedBy rdf:resource="https://w3id.org/arco/ontology/context-description"/>
        <rdfs:label xml:lang="en">Alternative dating type</rdfs:label>
        <rdfs:comment xml:lang="en">This class represents the type of alternative dating of a cultural property (different dating, obsolete dating, other method dating)</rdfs:comment>
      </skos:ConceptScheme>
    </rdfs:range>
  </owl:ObjectProperty>
  <skos:Concept rdf:about="https://w3id.org/arco/ontology/context-description/OtherMethodOfDating">
    <rdfs:isDefinedBy rdf:resource="https://w3id.org/arco/ontology/context-description"/>
    <rdfs:label xml:lang="en">Other method of dating</rdfs:label>
    <rdfs:comment xml:lang="en">This individual represents a different type of dating method than the one present in cultural entity's chronological information.</rdfs:comment>
    <skos:inScheme rdf:resource="https://w3id.org/arco/ontology/context-description/AlternativeDatingType"/>
  </skos:Concept>
  <skos:Concept rdf:about="https://w3id.org/arco/ontology/context-description/DifferentDating">
    <rdfs:isDefinedBy rdf:resource="https://w3id.org/arco/ontology/context-description"/>
    <rdfs:label xml:lang="en">Different dating</rdfs:label>
    <rdfs:comment xml:lang="en">This individual represents a different type of dating than the one present in cultural entity's chronological information.</rdfs:comment>
    <skos:inScheme rdf:resource="https://w3id.org/arco/ontology/context-description/AlternativeDatingType"/>
  </skos:Concept>
  <skos:Concept rdf:about="https://w3id.org/arco/ontology/context-description/ObsoleteDating">
    <rdfs:isDefinedBy rdf:resource="https://w3id.org/arco/ontology/context-description"/>
    <rdfs:label xml:lang="en">Obsolete dating</rdfs:label>
    <rdfs:comment xml:lang="en">This individual represents an obsolete dating.</rdfs:comment>
    <skos:inScheme rdf:resource="https://w3id.org/arco/ontology/context-description/AlternativeDatingType"/>
  </skos:Concept>
</rdf:RDF>
