<rdf:RDF
    xmlns:dct="http://purl.org/dc/terms/"
    xmlns:rdf="http://www.w3.org/1999/02/22-rdf-syntax-ns#"
    xmlns:dc="http://purl.org/dc/elements/1.1/"
    xmlns:owl="http://www.w3.org/2002/07/owl#"
    xmlns:dcmit="http://purl.org/dc/dcmitype/"
    xmlns:skos="http://www.w3.org/2004/02/skos/core#"
    xmlns:voaf="http://purl.org/vocommons/voaf#"
    xmlns:rdfs="http://www.w3.org/2000/01/rdf-schema#"
    xmlns:vann="http://purl.org/vocab/vann/">
  <owl:Ontology rdf:about="http://www.ebusiness-unibw.org/ontologies/consumerelectronics/v1"/>
  <skos:Concept rdf:about="http://www.ebusiness-unibw.org/ontologies/consumerelectronics/v1#Lit-Ion">
    <rdfs:isDefinedBy rdf:resource="http://www.ebusiness-unibw.org/ontologies/consumerelectronics/v1"/>
    <rdfs:label xml:lang="en">Lit-Ion</rdfs:label>
    <rdfs:comment xml:lang="en">Type of rechargeable battery in which a lithium ion moves between the anode and cathode.

(This description is partly based on or reuses content from the Wikipedia article "Lithium ion battery" (http://en.wikipedia.org/wiki/Lithium_ion_battery) and is licensed under the GNU Free Documentation License (http://www.gnu.org/copyleft/fdl.html).)</rdfs:comment>
    <skos:inScheme>
      <skos:ConceptScheme rdf:about="http://www.ebusiness-unibw.org/ontologies/consumerelectronics/v1#RechargeableEnergySource">
        <rdfs:isDefinedBy rdf:resource="http://www.ebusiness-unibw.org/ontologies/consumerelectronics/v1"/>
        <rdfs:label xml:lang="en">A rechargeable battery is a kind of energy source that is able to be reused by refilling it with a charger.</rdfs:label>
        <rdfs:comment xml:lang="en">A rechargeable battery is a kind of energy source that is able to be reused by refilling it with a charger.</rdfs:comment>
      </skos:ConceptScheme>
    </skos:inScheme>
  </skos:Concept>
  <skos:Concept rdf:about="http://www.ebusiness-unibw.org/ontologies/consumerelectronics/v1#NiCd">
    <rdfs:isDefinedBy rdf:resource="http://www.ebusiness-unibw.org/ontologies/consumerelectronics/v1"/>
    <rdfs:label xml:lang="en">NiCd</rdfs:label>
    <rdfs:comment xml:lang="en">A type of rechargeable battery using nickel oxide hydroxide and metallic cadmium as electrodes.

(This description is partly based on or reuses content from the Wikipedia article "Nickel-cadmium battery" (http://en.wikipedia.org/wiki/Nickel-cadmium_battery) and is licensed under the GNU Free Documentation License (http://www.gnu.org/copyleft/fdl.html).)</rdfs:comment>
    <skos:inScheme rdf:resource="http://www.ebusiness-unibw.org/ontologies/consumerelectronics/v1#RechargeableEnergySource"/>
  </skos:Concept>
  <skos:Concept rdf:about="http://www.ebusiness-unibw.org/ontologies/consumerelectronics/v1#Li-Ion_Polymer">
    <rdfs:isDefinedBy rdf:resource="http://www.ebusiness-unibw.org/ontologies/consumerelectronics/v1"/>
    <rdfs:label xml:lang="en">Li-ion Polymer</rdfs:label>
    <rdfs:comment xml:lang="en">Lithium polymer batteries (abbreviated Li-poly, Li-Pol, LiPo, LIP, PLI or LiP) are rechargeable batteries which have technologically evolved from lithium-ion batteries.

(This description is partly based on or reuses content from the Wikipedia article "Lithium-polymer" (http://en.wikipedia.org/wiki/Lithium-polymer) and is licensed under the GNU Free Documentation License (http://www.gnu.org/copyleft/fdl.html).)</rdfs:comment>
    <skos:inScheme rdf:resource="http://www.ebusiness-unibw.org/ontologies/consumerelectronics/v1#RechargeableEnergySource"/>
  </skos:Concept>
  <skos:Concept rdf:about="http://www.ebusiness-unibw.org/ontologies/consumerelectronics/v1#Solar">
    <rdfs:isDefinedBy rdf:resource="http://www.ebusiness-unibw.org/ontologies/consumerelectronics/v1"/>
    <rdfs:label xml:lang="en">Solar</rdfs:label>
    <rdfs:comment xml:lang="en">Solar cell or photovoltaic cell is a wide area electronic device that converts solar energy into electricity by the photovoltaic effect.

(This description is partly based on or reuses content from the Wikipedia article "Solar cell" (http://en.wikipedia.org/wiki/Solar_cell) and is licensed under the GNU Free Documentation License (http://www.gnu.org/copyleft/fdl.html).)</rdfs:comment>
    <skos:inScheme rdf:resource="http://www.ebusiness-unibw.org/ontologies/consumerelectronics/v1#RechargeableEnergySource"/>
  </skos:Concept>
  <skos:Concept rdf:about="http://www.ebusiness-unibw.org/ontologies/consumerelectronics/v1#NiMH">
    <rdfs:isDefinedBy rdf:resource="http://www.ebusiness-unibw.org/ontologies/consumerelectronics/v1"/>
    <rdfs:label xml:lang="en">NiMH</rdfs:label>
    <rdfs:comment xml:lang="en">A nickel-metal hydride battery, abbreviated NiMH, is a type of rechargeable battery similar to a nickel-cadmium (NiCd) battery but using a hydrogen-absorbing alloy for the negative electrode instead of cadmium.

(This description is partly based on or reuses content from the Wikipedia article "Nickel metal hydride battery" (http://en.wikipedia.org/wiki/Nickel_metal_hydride_battery) and is licensed under the GNU Free Documentation License (http://www.gnu.org/copyleft/fdl.html).)</rdfs:comment>
    <skos:inScheme rdf:resource="http://www.ebusiness-unibw.org/ontologies/consumerelectronics/v1#RechargeableEnergySource"/>
  </skos:Concept>
  <skos:Concept rdf:about="http://www.ebusiness-unibw.org/ontologies/consumerelectronics/v1#NIH2">
    <rdfs:isDefinedBy rdf:resource="http://www.ebusiness-unibw.org/ontologies/consumerelectronics/v1"/>
    <rdfs:label xml:lang="en">NIH2</rdfs:label>
    <rdfs:comment xml:lang="en">A nickel hydrogen battery (NIH2 or Ni-H2) is a rechargeable electrochemical power source based on nickel and hydrogen.</rdfs:comment>
    <skos:inScheme rdf:resource="http://www.ebusiness-unibw.org/ontologies/consumerelectronics/v1#RechargeableEnergySource"/>
  </skos:Concept>
</rdf:RDF>
