<rdf:RDF
    xmlns:rdf="http://www.w3.org/1999/02/22-rdf-syntax-ns#"
    xmlns:dcterms="http://purl.org/dc/terms/"
    xmlns:dc="http://purl.org/dc/elements/1.1/"
    xmlns:owl="http://www.w3.org/2002/07/owl#"
    xmlns:dcmit="http://purl.org/dc/dcmitype/"
    xmlns:skos="http://www.w3.org/2004/02/skos/core#"
    xmlns:voaf="http://purl.org/vocommons/voaf#"
    xmlns:rdfs="http://www.w3.org/2000/01/rdf-schema#"
    xmlns:vann="http://purl.org/vocab/vann/">
  <owl:Ontology rdf:about="http://rdf.geospecies.org/ont/geospecies"/>
  <owl:ObjectProperty rdf:about="http://rdf.geospecies.org/ont/geospecies#hasOmernik_4_Ecozone">
    <rdfs:label>hasOmernik_4_Ecozone</rdfs:label>
    <rdfs:domain rdf:resource="http://rdf.geospecies.org/ont/geospecies#Location"/>
    <rdfs:range>
      <skos:ConceptScheme rdf:about="http://rdf.geospecies.org/ont/geospecies#Omernik_Level_IV_Ecoregion_Classification">
        <rdfs:isDefinedBy rdf:resource="http://rdf.geospecies.org/ont/geospecies"/>
        <rdfs:label>Omernik_Level_Four_Classification</rdfs:label>
        <rdfs:comment>Ecoregions denote areas of general similarity in ecosystems and in the type, quality, and quantity of environmental resources. The level IV state projects depict revisions and subdivisions of ecoregions, that were compiled at a relatively small scale (Omernik 1987). Compilation of the level IV maps, performed at the larger 1:250,000 scale, has been a part of collaborative projects between United States Environmental Protection Agency, National Health and Environmental Effects Laboratory (NHEERL)--Corvallis, OR, the U.S. Forest Service, Natural Resources Conservation Service, and a variety of other state and federal resource agencies. The ecoregions and subregions are designed to serve as a spatial framework for environmental resource management. The most immediate needs by the states are for developing regional biological criteria and water resource standards, and for setting management goals for nonpoint-source pollution. Explanation of the methods used to delineate the ecoregions are given in Omernik (1995), Griffith et al. (1994), and Gallant et al. (1989). This series of maps has been produced as part of a regional interagency collaborative project aimed at obtaining consensus between the EPA, the NRCS, and the USFS regarding alignments of ecological regions.</rdfs:comment>
      </skos:ConceptScheme>
    </rdfs:range>
  </owl:ObjectProperty>
  <skos:Concept rdf:about="http://rdf.geospecies.org/ont/geospecies#Omernik_3_54_Central_Corn_Belt_Plains">
    <rdfs:isDefinedBy rdf:resource="http://rdf.geospecies.org/ont/geospecies"/>
    <rdfs:label>Omernik_3_Central Corn Belt Plains</rdfs:label>
    <rdfs:comment>Prairie communities were native to the glaciated Central Corn Belt Plains, and they were a stark contrast to the hardwood forests that grew on the drift plains of ecoregions to the east. Beginning in the nineteenth century, the natural vegetation was gradually replaced by agriculture. Farms are now extensive on the dark, fertile soils of the Central Corn Belt Plains 54, producing corn and soybeans, cattle, sheep, poultry, and especially hogs. However, livestock operations are not as dominant as in the drier Western Corn Belt Plains to the west. Agriculture has affected stream chemistry, turbidity, and habitat. The extent of the Central Corn Belt Plains (54) ecoregion in Wisconsin is contained in a small area in the southeastern portion of the state. Land use of the ecoregion continues to change, from exclusively agriculture to a pattern with an increasing amount of urban and industrial land.</rdfs:comment>
    <skos:inScheme rdf:resource="http://rdf.geospecies.org/ont/geospecies#Omernik_Level_IV_Ecoregion_Classification"/>
  </skos:Concept>
  <skos:Concept rdf:about="http://rdf.geospecies.org/ont/geospecies#Omernik_4_51b_Central_Wisconsin_Undulating_Till_Plain">
    <rdfs:isDefinedBy rdf:resource="http://rdf.geospecies.org/ont/geospecies"/>
    <rdfs:label>Omernik_4_Central_Wisconsin_Undulating_Till_Plain</rdfs:label>
    <rdfs:comment>The Central Wisconsin Undulating Till Plain (51b) ecoregion has a greater percentage of agricultural land use than adjacent ecoregion 51a. The land cover mosaic of woodland and agriculture includes large areas of cropland that produce silage corn, oats, barley, and some apples. Ecoregion 51b has fewer lakes, with higher trophic states, than adjacent level IV ecoregions in ecoregion 51. The undulating to rolling irregular plains of sandy loam till and outwash sands also distinguish this ecoregion from the stagnation moraines of ecoregion 51a to the west and the lacustrine sand plains of ecoregion 51c to the south. This ecoregion has areas in the far east that are underlain with igneous metamorphic rock outcrops, and areas in the west and southwest that are underlain by sandstone and shale. Outcrops of sandstone comprise roughly 70% of the total area of the ecoregion. The region supports a transitional PNV mosaic of oak, hemlock/sugar maple/yellow birch, and white pine/red pine forests in the north, and more sugar maple/basswood/ oak forests to the south.</rdfs:comment>
    <skos:inScheme rdf:resource="http://rdf.geospecies.org/ont/geospecies#Omernik_Level_IV_Ecoregion_Classification"/>
  </skos:Concept>
  <skos:Concept rdf:about="http://rdf.geospecies.org/ont/geospecies#Omernik_4_51c_Glacial_Lake_Wisconsin_Sand_Plain">
    <rdfs:isDefinedBy rdf:resource="http://rdf.geospecies.org/ont/geospecies"/>
    <rdfs:label>Omernik_4_Glacial_Lake_Wisconsin_Sand_Plain</rdfs:label>
    <rdfs:comment>Compared to adjacent ecoregions, the Glacial Lake Wisconsin Sand Plain (51c) is an area of low relief. The droughty outwash, lacustrine and slope wash sands, sand buttes, and stream bottom and wetland soils support a PNV of jack pine/scrub-oak forests and barrens, along with sedge meadows and conifer swamps, which characterize this flat sandy lake plain. This PNV is in contrast to the predominantly white and black oak vegetation of ecoregion 51d. The region is also distinguished by its more extensive wetlands and a lack of natural lakes. Most of the existing lakes have been constructed for use in cranberry production. Land use in this region consists of woodland and agriculture, with crops including cranberries, strawberries, and potatoes.</rdfs:comment>
    <skos:inScheme rdf:resource="http://rdf.geospecies.org/ont/geospecies#Omernik_Level_IV_Ecoregion_Classification"/>
  </skos:Concept>
  <skos:Concept rdf:about="http://rdf.geospecies.org/ont/geospecies#Omernik_4_51f_Green_Bay_Till_and_Lacustrine_Plain">
    <rdfs:isDefinedBy rdf:resource="http://rdf.geospecies.org/ont/geospecies"/>
    <rdfs:label>Omernik_4_51f_Green Bay Till and Lacustrine Plain</rdfs:label>
    <rdfs:comment>Green Bay Till and Lacustrine Plain (51f) is a transitional ecoregion characterized by wetlands, a mix of outwash and loamy recessional moraines, with many areas of outwash plains in the northwest, lake plains and ground moraines in the south, and ground moraines throughout the rest of the region. The PNV of the region represents a shift from the predominantly northern hardwoods and conifer swamps along the lake shore to the maple/basswood/oak forests and oak savanna to the south. The red sandy, loamy soils of this ecoregion are similar to some southern areas in the northern Wisconsin/Michigan Pine Barrens (50k); however, due to the generally milder climate (because of proximity to Lake Michigan), the growing season is more favorable and much of the area has been cleared of natural vegetation and replaced by agriculture.</rdfs:comment>
    <skos:inScheme rdf:resource="http://rdf.geospecies.org/ont/geospecies#Omernik_Level_IV_Ecoregion_Classification"/>
  </skos:Concept>
  <skos:Concept rdf:about="http://rdf.geospecies.org/ont/geospecies#Omernik_4_51d_Central_Sand_Ridges">
    <rdfs:isDefinedBy rdf:resource="http://rdf.geospecies.org/ont/geospecies"/>
    <rdfs:label>Omernik_4_Central_Sand_Ridges</rdfs:label>
    <rdfs:comment>The Central Sand Ridges (51d) ecoregion has the highest density of lakes with the lowest trophic states of all level IV ecoregions in the North Central Hardwood Forests (51). Pitted glacial outwash with extensive eskers and drumlins, ice contact deposits, rolling ground moraines, and steep end moraines distinguish this region from the flat lake plain of adjacent ecoregion 51c. The dry, sandy, and loamy till soils of the region support a PNV of oak savanna (white oak, black oak, and bur oak) with areas of sedge meadows, unlike the wetland vegetation and pine or oak barrens of ecoregion 51c and the mosaic of hemlock/beech/maple forests and mixed conifers of ecoregion 51e to the north.</rdfs:comment>
    <skos:inScheme rdf:resource="http://rdf.geospecies.org/ont/geospecies#Omernik_Level_IV_Ecoregion_Classification"/>
  </skos:Concept>
  <skos:Concept rdf:about="http://rdf.geospecies.org/ont/geospecies#Omernik_4_50a_Lake_Superior_Clay_Plain">
    <rdfs:isDefinedBy rdf:resource="http://rdf.geospecies.org/ont/geospecies"/>
    <rdfs:label>Omernik_4_Lake Superior Clay Plain</rdfs:label>
    <rdfs:comment>The Lake Superior Clay Plain (50a) is a flat to undulating lake plain and outwash lowland. The soils of 50a are generally calcareous red clays with organic deposits in swampy areas. A dearth of lakes, along with a somewhat milder climate and longer growing season due to the climate amelioration by Lake Superior, differentiates 50a from surrounding ecoregions. Land use in 50a is predominantly woodland with some limited agriculture of hay, small grains, and apples on Bayfield Peninsula, distinguishing 50a from most other level IV ecoregions in Northern Lakes and Forests (50) where the land use/land cover is predominantly forest and woodland. Ecoregion 50a has a PNV of boreal forest (although somewhat different than boreal forests to the north), unlike the pine barrens and pine forests of 50c, the mosaic of pine and birch in 50b, and the northern mesic forest of 50e.</rdfs:comment>
    <skos:inScheme rdf:resource="http://rdf.geospecies.org/ont/geospecies#Omernik_Level_IV_Ecoregion_Classification"/>
  </skos:Concept>
  <skos:Concept rdf:about="http://rdf.geospecies.org/ont/geospecies#Omernik_4_51e_Upper_Wolf_River_Stagnation_Moraine">
    <rdfs:isDefinedBy rdf:resource="http://rdf.geospecies.org/ont/geospecies"/>
    <rdfs:label>Omernik_4_51e_Upper Wolf River Stagnation Moraine</rdfs:label>
    <rdfs:comment>The Upper Wolf River Stagnation Moraine (51e) ecoregion is characterized by the hummocky ground and end moraines and pitted outwash, in contrast to the level till plains of ecoregion 51f to the east and the irregular till plain of ecoregion 51b to the west. This region supports a PNV mosaic of hemlock/beech/sugar-maple, wetland vegetation, and mixed conifers, as compared to the predominantly oak forests of 51d to the south. Land use in 51e is mixed agriculture/woodland with a larger area of extensive forest than adjacent level IV ecoregions in the North Central Hardwoods Forests (51). This is due to land use practices within the Menominee Indian Reservation; more forest cover is still intact, and agricultural practices are less significant. The lake trophic state in 51e is generally higher than in 51d to the south.</rdfs:comment>
    <skos:inScheme rdf:resource="http://rdf.geospecies.org/ont/geospecies#Omernik_Level_IV_Ecoregion_Classification"/>
  </skos:Concept>
  <skos:Concept rdf:about="http://rdf.geospecies.org/ont/geospecies#Omernik_4_47g_Prairie_Pothole_Region_">
    <rdfs:isDefinedBy rdf:resource="http://rdf.geospecies.org/ont/geospecies"/>
    <rdfs:label>Omernik_4_Prairie Pothole Region</rdfs:label>
    <rdfs:comment>The Prairie Pothole Region (47g) is characterized by smooth to undulating topography, productive prairie soils, and loess- and till-capped dolomite bedrock. The potential natural vegetation (PNV) is predominantly tall grass prairie with a gradual transition eastward to more mixed hardwoods, distinguishing 47g from the greater concentration of mixed hardwoods of both 51a to the north and 51b to the east, and the mixed prairie and oak savanna of 52b to the south.</rdfs:comment>
    <skos:inScheme rdf:resource="http://rdf.geospecies.org/ont/geospecies#Omernik_Level_IV_Ecoregion_Classification"/>
  </skos:Concept>
  <skos:Concept rdf:about="http://rdf.geospecies.org/ont/geospecies#Omernik_4_52b_Coulee_Section">
    <rdfs:isDefinedBy rdf:resource="http://rdf.geospecies.org/ont/geospecies"/>
    <rdfs:label>Omernik_4_Paleozoic_Plateau_Coulee_Section</rdfs:label>
    <rdfs:comment>Dissected slopes and open hills with most of the gentle slope on the lowland characterize the Coulee Section (52b) ecoregion. Soils are well drained silty loess over residuum, limestone, sandstone or shale, with soils over quartzite in the Baraboo Hills area. Land use in the region is predominantly mixed agriculture/woodland, with most of the griculture occurring on the lowlands and more level hilltops. The PNV of ecoregion 52b is a mosaic of oak forests and prairie, with larger areas of sugar maple/basswood/oak forests than in 52a.</rdfs:comment>
    <skos:inScheme rdf:resource="http://rdf.geospecies.org/ont/geospecies#Omernik_Level_IV_Ecoregion_Classification"/>
  </skos:Concept>
  <skos:Concept rdf:about="http://rdf.geospecies.org/ont/geospecies#Omernik_4_53a_Rock_River_Drift_Plain">
    <rdfs:isDefinedBy rdf:resource="http://rdf.geospecies.org/ont/geospecies"/>
    <rdfs:label>Omernik_4_53a_Rock River Drift Plain</rdfs:label>
    <rdfs:comment>The Rock River Drift Plain (53a) ecoregion has a greater stream density and fewer lakes than in ecoregions to the north and east. Glaciation of this region is older, late Pliocene-early Pleistocene, than in surrounding ecoregions. The drift mantle is thin and deeply weathered, with leached soils developed from a silt-loam cap of loess over glacial drift. Steeper topography and broad outwash plains with loamy and sandy soils also characterize this region.</rdfs:comment>
    <skos:inScheme rdf:resource="http://rdf.geospecies.org/ont/geospecies#Omernik_Level_IV_Ecoregion_Classification"/>
  </skos:Concept>
  <skos:Concept rdf:about="http://rdf.geospecies.org/ont/geospecies#Omernik_4_54e_Chiwaukee_Prairie_Region">
    <rdfs:isDefinedBy rdf:resource="http://rdf.geospecies.org/ont/geospecies"/>
    <rdfs:label>Omernik_4_Chiwaukee Prairie Region</rdfs:label>
    <rdfs:comment>The Chiwaukee Prairie Region (54e) is characterized by intensive agriculture, prairie soils, loess capped loamy till, and lacustrine deposits. The soils of ecoregion 54e are fertile and generally more productive than those of ecoregion 53 to the north and west. The PNV of the Chiwaukee Prairie Region is predominantly tall-grass prairie, in contrast to the southern mesic forest and oak savanna of the adjacent region to the north and west. Most of the natural prairie vegetation of ecoregion 54e has been replaced with cropland or urban and industrial land cover.</rdfs:comment>
    <skos:inScheme rdf:resource="http://rdf.geospecies.org/ont/geospecies#Omernik_Level_IV_Ecoregion_Classification"/>
  </skos:Concept>
  <skos:Concept rdf:about="http://rdf.geospecies.org/ont/geospecies#Omernik_4_53c_Southeastern_Wisconsin_Savannah_and_Till_Plain">
    <rdfs:isDefinedBy rdf:resource="http://rdf.geospecies.org/ont/geospecies"/>
    <rdfs:label>Omernik_4_Southeastern_Wisconsin_Savannah_and_Till_Plain</rdfs:label>
    <rdfs:comment>The till plains of the Southeastern Wisconsin Savanna and Till Plain (53c) ecoregion support a mix of agriculture (cropland and dairy operations) and woodland. Crops include forage crops to support the dairy operations and a wide range of truck and specialty crops. Most of the original vegetation has been cleared, with forested areas remaining only on steeper end moraines and poorly drained depressions. Irregular till plains, end moraines, kettles, and drumlins are common, and wetlands are found throughout the region, especially along end morainal ridges. PNV of this region is transitional with a mosaic of sugar maple, basswood, oak to the east, and an increasing amount of white, black, and bur oak, oak savanna, prairie, and sedge meadows toward the west.</rdfs:comment>
    <skos:inScheme rdf:resource="http://rdf.geospecies.org/ont/geospecies#Omernik_Level_IV_Ecoregion_Classification"/>
  </skos:Concept>
  <skos:Concept rdf:about="http://rdf.geospecies.org/ont/geospecies#Omernik_4_53d_Lake_Michigan_Lacustrine_Clay_Plain">
    <rdfs:isDefinedBy rdf:resource="http://rdf.geospecies.org/ont/geospecies"/>
    <rdfs:label>Omernik_4_53d_Lake Michigan Lacustrine Clay Plain</rdfs:label>
    <rdfs:comment>The Lake Michigan Lacustrine Clay Plain (53d) ecoregion is characterized by red calcareous clay soil, lacustrine and till deposits, and a flat plain. The topography is flatter than ecoregions to the south, and there are fewer lakes, but the lakes have generally higher trophic states than in adjacent level IV ecoregions in 50 and 51. Soils are generally silty and loamy over calcareous loamy till, with muck and loamy lacustrine soils in low-lying areas. Ecoregion 53d has prime farmland with a longer growing season and more fertile soils than surrounding ecoregions. Agriculture has a different mix of crops, with more fruits and vegetables, than that of ecoregion 53c. The PNV of this region is beech/sugar maple/basswood/red and white oak forests with a greater concentration of beech than other ecoregions in 53.</rdfs:comment>
    <skos:inScheme rdf:resource="http://rdf.geospecies.org/ont/geospecies#Omernik_Level_IV_Ecoregion_Classification"/>
  </skos:Concept>
  <skos:Concept rdf:about="http://rdf.geospecies.org/ont/geospecies#Omernik_4_51g_Door_Peninsula">
    <rdfs:isDefinedBy rdf:resource="http://rdf.geospecies.org/ont/geospecies"/>
    <rdfs:label>Omernik_4_Door_Peninsula</rdfs:label>
    <rdfs:comment>The Door Peninsula (51g) ecoregion is a lakeshore region with ground moraines. The longer growing season and shallow, fertile, calcareous loamy till soils of this ecoregion support a mixed woodland/agriculture land use. Orchard and fruit crops, such as apples and cherries, are common. The bedrock geology of 51g is shallower than other ecoregions in 51 and consists primarily of Silurian dolomite bedrock. In recent years, this region has become popular for tourism.</rdfs:comment>
    <skos:inScheme rdf:resource="http://rdf.geospecies.org/ont/geospecies#Omernik_Level_IV_Ecoregion_Classification"/>
  </skos:Concept>
  <skos:Concept rdf:about="http://rdf.geospecies.org/ont/geospecies#Omernik_4_51a_St._Croix_Pitted_Stagnation_Moraines">
    <rdfs:isDefinedBy rdf:resource="http://rdf.geospecies.org/ont/geospecies"/>
    <rdfs:label>Omernik_4_51a_St. Croix Pitted Stagnation Moraines</rdfs:label>
    <rdfs:comment>The St. Croix Pitted Stagnation Moraines (51a) is a region of ground and stagnation moraines with broad irregular areas of hummocky topography. Soils are silty and loamy, with sandy loamy till commonly underlain by a substratum of acid sand and gravel glacial outwash. There are more lakes in 51a than in ecoregions to the east and south, and lake trophic states, although generally higher than in the region to the north, are lower than in the bordering ecoregion to the southeast. Land use in this region is a mix of agriculture and woodland, in contrast to the mostly woodland and forest land cover of ecoregions to the north and the greater amounts of agriculture in ecoregions to the southeast. The PNV of 51a includes aspen/birch/pine forests, oak-maple forests, and sugar-maple/birch/pine forests, representing a transition from the pines of 50b to the tall grass prairie and oak forests of 47g.</rdfs:comment>
    <skos:inScheme rdf:resource="http://rdf.geospecies.org/ont/geospecies#Omernik_Level_IV_Ecoregion_Classification"/>
  </skos:Concept>
  <skos:Concept rdf:about="http://rdf.geospecies.org/ont/geospecies#Omernik_4_52a_Savanna_Section">
    <rdfs:isDefinedBy rdf:resource="http://rdf.geospecies.org/ont/geospecies"/>
    <rdfs:label>Omernik_4_Savanna Section</rdfs:label>
    <rdfs:comment>Topography in the Savanna Section (52a) of the Driftless Area is different than the rest of the level III ecoregion because of its characteristic broad, relatively level ridge tops and narrow steep sided valley bottoms. Elsewhere in the dissected Driftless Area, the landform mosaic comprises relatively broad, flat valley bottoms with steep sharper crested ridges or a pattern of nearly equal amounts of flatter areas in the valley bottoms and interfluves. The soils are well drained silty loess over residuum, dolostone, limestone, or sandstone. Land use patterns in the Driftless Area also follow spatial differences in slope; hence, 52a is predominantly agriculture on the uplands and some mixed woodland/agriculture in lowland areas. The PNV of the region is a mosaic of oak forests and savannas, large prairie grassland areas, and some sugar maple/basswood/oak forests. The region is also known for past lead and zinc mining.</rdfs:comment>
    <skos:inScheme rdf:resource="http://rdf.geospecies.org/ont/geospecies#Omernik_Level_IV_Ecoregion_Classification"/>
  </skos:Concept>
  <skos:Concept rdf:about="http://rdf.geospecies.org/ont/geospecies#Omernik_4_53b_Kettle_Moraines">
    <rdfs:isDefinedBy rdf:resource="http://rdf.geospecies.org/ont/geospecies"/>
    <rdfs:label>Omernik_4_Kettle_Moraines</rdfs:label>
    <rdfs:comment>The Kettle Moraines (53b) ecoregion contains a higher concentration of lakes with lower trophic states than in the rest of the Southeastern Wisconsin Till Plains (53). The soils are clayey to the east, especially along the Lake Michigan shore, and more sandy to the west, but generally less clayey than the soils in ecoregion 53d to the north. The region also contains extensive ground and end moraines and pitted outwash with belts of hilly moraines. It generally has greater relief than ecoregion 53d to the northeast.</rdfs:comment>
    <skos:inScheme rdf:resource="http://rdf.geospecies.org/ont/geospecies#Omernik_Level_IV_Ecoregion_Classification"/>
  </skos:Concept>
</rdf:RDF>
