<rdf:RDF
    xmlns:dct="http://purl.org/dc/terms/"
    xmlns:rdf="http://www.w3.org/1999/02/22-rdf-syntax-ns#"
    xmlns:dc="http://purl.org/dc/elements/1.1/"
    xmlns:owl="http://www.w3.org/2002/07/owl#"
    xmlns:dcmit="http://purl.org/dc/dcmitype/"
    xmlns:skos="http://www.w3.org/2004/02/skos/core#"
    xmlns:voaf="http://purl.org/vocommons/voaf#"
    xmlns:rdfs="http://www.w3.org/2000/01/rdf-schema#"
    xmlns:vann="http://purl.org/vocab/vann/">
  <skos:Concept rdf:about="http://www.data-knowledge.org/dk/hasDataLifecycle">
    <rdfs:comment xml:lang="en">Specifies the life cycle of an individual instance of a Business Object, Data Object or Data Asset. This property can be used to override the general type level life cycle definition expressed by definesLifecycleOfInstances. The current life cycle state of the instance is referred to via the property lifecycle:state</rdfs:comment>
    <rdfs:label xml:lang="de">hat Datenlebenszyklus</rdfs:label>
    <rdfs:label xml:lang="en">has data lifecycle</rdfs:label>
    <rdfs:comment xml:lang="de">Spezifiziert den Lebenszyklus einer individuellen Instanz eines Geschäftsobjekts, Datenobjekts oder Datenguts. Diese Relation kann genutzt werden, um die generelle Typebenen-Definition des Lebenszyklus, welche durch definesLifecycleOfInstances ausgedrückt wird, zu überschreiben. Der aktuelle Lebenszyklusstatus der Instanz wird über die Relation lifecycle:state zugewiesen.</rdfs:comment>
    <skos:inScheme>
      <skos:ConceptScheme rdf:about="http://www.w3.org/2000/01/rdf-schema#Property"/>
    </skos:inScheme>
  </skos:Concept>
  <skos:Concept rdf:about="http://www.data-knowledge.org/dk/hasKnowledgeLifecycle">
    <rdfs:comment xml:lang="de">Kann genutzt werden, um einen allgemeinen Lebenszyklus, der auf alle Klassen des Modells oder nur auf spezielle Klassen zutrifft, zu definieren.</rdfs:comment>
    <rdfs:label xml:lang="en">has Knowledge Lifecycle</rdfs:label>
    <rdfs:label xml:lang="de">hat Wissenslebenszyklus</rdfs:label>
    <rdfs:comment xml:lang="en">May be used to define a general life cycle that applies to all classes of the model or certain classes.</rdfs:comment>
    <skos:inScheme rdf:resource="http://www.w3.org/2000/01/rdf-schema#Property"/>
  </skos:Concept>
  <skos:Concept rdf:about="http://www.data-knowledge.org/dk/hasTerms">
    <rdfs:comment xml:lang="de">Ressourcen können spezifische Nutzungsbedingungen haben</rdfs:comment>
    <rdfs:label xml:lang="de">hat Nutzungsbedingungen</rdfs:label>
    <rdfs:label xml:lang="en">has Terms of Use</rdfs:label>
    <rdfs:comment xml:lang="en">Resources can have specific Terms of Use</rdfs:comment>
    <skos:inScheme rdf:resource="http://www.w3.org/2000/01/rdf-schema#Property"/>
  </skos:Concept>
  <skos:Concept rdf:about="http://www.data-knowledge.org/dk/hasApplicationLifecycle">
    <rdfs:comment xml:lang="en">Specifies the life cycle of an individual Application instance. The current life cycle state of the instance is referred to via the property lifecycle:state.</rdfs:comment>
    <rdfs:label xml:lang="de">hat Applikationslebenszyklus</rdfs:label>
    <rdfs:label xml:lang="en">has application lifecycle</rdfs:label>
    <rdfs:comment xml:lang="de">Spezifiziert den Lebenszyklus einer individuellen Applikation. Der aktuelle Lebenszyklusstatus der Instanz wird über die Relation lifecycle:state zugewiesen.</rdfs:comment>
    <skos:inScheme rdf:resource="http://www.w3.org/2000/01/rdf-schema#Property"/>
  </skos:Concept>
</rdf:RDF>
