<rdf:RDF
    xmlns:dct="http://purl.org/dc/terms/"
    xmlns:rdf="http://www.w3.org/1999/02/22-rdf-syntax-ns#"
    xmlns:dc="http://purl.org/dc/elements/1.1/"
    xmlns:owl="http://www.w3.org/2002/07/owl#"
    xmlns:dcmit="http://purl.org/dc/dcmitype/"
    xmlns:skos="http://www.w3.org/2004/02/skos/core#"
    xmlns:voaf="http://purl.org/vocommons/voaf#"
    xmlns:rdfs="http://www.w3.org/2000/01/rdf-schema#"
    xmlns:vann="http://purl.org/vocab/vann/">
  <skos:Concept rdf:about="http://www.data-knowledge.org/dk/BusinessObjectType">
    <rdfs:comment xml:lang="en">Conceptual (data) entity relevant to business that represents a coherent set of information about a group of real or virtual objects</rdfs:comment>
    <rdfs:label xml:lang="de">Geschäftsobjekttyp (BOT)</rdfs:label>
    <dct:isPartOf>
      <skos:Concept rdf:about="http://www.data-knowledge.org/dk/BusinessObjectDomain">
        <rdfs:comment xml:lang="de">Gruppierung kohärenter Geschäftsobjekttypen (BOTs), entweder aus Themen- oder Verwaltungssicht</rdfs:comment>
        <rdfs:label xml:lang="de">Geschäftsobjektdomäne (BOD)</rdfs:label>
        <dct:hasPart rdf:resource="http://www.data-knowledge.org/dk/BusinessObjectType"/>
        <rdfs:label xml:lang="en">Business Object Domain (BOD)</rdfs:label>
        <rdfs:comment xml:lang="en">Clusters of coherent Business Object Types (BOTs), either from a subject matter or management point of view</rdfs:comment>
        <skos:inScheme>
          <skos:ConceptScheme rdf:about="http://www.data-knowledge.org/dk/DataConceptualization"/>
        </skos:inScheme>
      </skos:Concept>
    </dct:isPartOf>
    <dct:hasPart>
      <skos:Concept rdf:about="http://www.data-knowledge.org/dk/BusinessObjectTypeAttribute">
        <rdfs:comment xml:lang="de">Konzeptuell elementare Informationseinheit als Teil eines Geschäftsobjekttyps (BOT)</rdfs:comment>
        <rdfs:label xml:lang="de">Geschäftsobjekttyp-Attribut (BOTA)</rdfs:label>
        <dct:isPartOf rdf:resource="http://www.data-knowledge.org/dk/BusinessObjectType"/>
        <rdfs:label xml:lang="en">Business Object Type Attribute (BOTA)</rdfs:label>
        <rdfs:comment xml:lang="en">Conceptually elementary piece of information as part of a Business Object Type (BOT)</rdfs:comment>
        <skos:inScheme rdf:resource="http://www.data-knowledge.org/dk/DataConceptualization"/>
      </skos:Concept>
    </dct:hasPart>
    <rdfs:label xml:lang="en">Business Object Type (BOT)</rdfs:label>
    <rdfs:comment xml:lang="de">Konzeptuelle, unternehmensrelevante (Daten-) Einheit, welche eine kohärente Menge von Informationen über eine Gruppe realer oder virtueller Objekte darstellt</rdfs:comment>
    <skos:inScheme rdf:resource="http://www.data-knowledge.org/dk/DataConceptualization"/>
  </skos:Concept>
</rdf:RDF>
