<?xml version="1.0" encoding="UTF-8"?>
<rdf:RDF
	xmlns:vann="http://purl.org/vocab/vann/"
	xmlns:voaf="http://purl.org/vocommons/voaf#"
	xmlns:rdfs="http://www.w3.org/2000/01/rdf-schema#"
	xmlns:owl="http://www.w3.org/2002/07/owl#"
	xmlns:skos="http://www.w3.org/2004/02/skos/core#"
	xmlns:rdf="http://www.w3.org/1999/02/22-rdf-syntax-ns#"
	xmlns:dcterms="http://purl.org/dc/terms/"
	xmlns:dc="http://purl.org/dc/elements/1.1/"
	xmlns:dcmit="http://purl.org/dc/dcmitype/"
	xmlns:sesame="http://www.openrdf.org/schema/sesame#"
	xmlns:xsd="http://www.w3.org/2001/XMLSchema#"
	xmlns:fn="http://www.w3.org/2005/xpath-functions#"
	xmlns:foaf="http://xmlns.com/foaf/0.1/"
	xmlns:hint="http://www.bigdata.com/queryHints#"
	xmlns:bd="http://www.bigdata.com/rdf#"
	xmlns:bds="http://www.bigdata.com/rdf/search#">

<rdf:Description rdf:about="https://w3id.org/nno/ontology">
	<rdf:type rdf:resource="http://www.w3.org/2002/07/owl#Ontology"/>
</rdf:Description>

<rdf:Description rdf:about="https://w3id.org/nno/ontology#Optimizer">
	<rdf:type rdf:resource="http://www.w3.org/2004/02/skos/core#ConceptScheme"/>
</rdf:Description>

<rdf:Description rdf:about="https://w3id.org/nno/ontology#adadelta">
	<rdf:type rdf:resource="http://www.w3.org/2004/02/skos/core#Concept"/>
	<skos:inScheme rdf:resource="https://w3id.org/nno/ontology#Optimizer"/>
</rdf:Description>

<rdf:Description rdf:about="https://w3id.org/nno/ontology#Optimizer">
	<rdfs:comment>Optimizer used by Neural Network.</rdfs:comment>
	<rdfs:label>Optimizer</rdfs:label>
</rdf:Description>

<rdf:Description rdf:about="https://w3id.org/nno/ontology#adadelta">
	<rdfs:comment>Adadelta is a more robust extension of Adagrad that adapts learning rates based on a moving window of gradient updates, instead of accumulating all past gradients. This way, Adadelta continues learning even when many updates have been done. Compared to Adagrad, in the original version of Adadelta you don't have to set an initial learning rate. In this version, initial learning rate and decay factor can be set, as in most other Keras optimizers.</rdfs:comment>
	<rdfs:label>Adadelta Optimizer</rdfs:label>
</rdf:Description>

<rdf:Description rdf:about="https://w3id.org/nno/ontology#hasOptimizer">
	<rdfs:range rdf:resource="https://w3id.org/nno/ontology#Optimizer"/>
	<rdfs:domain rdf:resource="https://w3id.org/nno/ontology#Model"/>
	<rdfs:label>has optimizer</rdfs:label>
	<rdfs:comment>Optimization function used by Neural Network (e.g. SGD, Adam or RMSprop).</rdfs:comment>
	<rdf:type rdf:resource="http://www.w3.org/2002/07/owl#ObjectProperty"/>
</rdf:Description>

<rdf:Description rdf:about="https://w3id.org/nno/ontology#Optimizer">
	<rdfs:isDefinedBy rdf:resource="https://w3id.org/nno/ontology"/>
</rdf:Description>

<rdf:Description rdf:about="https://w3id.org/nno/ontology#adadelta">
	<rdfs:isDefinedBy rdf:resource="https://w3id.org/nno/ontology"/>
</rdf:Description>

<rdf:Description rdf:about="https://w3id.org/nno/ontology#adagrad">
	<rdf:type rdf:resource="http://www.w3.org/2004/02/skos/core#Concept"/>
	<skos:inScheme rdf:resource="https://w3id.org/nno/ontology#Optimizer"/>
	<rdfs:comment>Adagrad is an optimizer with parameter-specific learning rates, which are adapted relative to how frequently a parameter gets updated during training. The more updates a parameter receives, the smaller the learning rate.</rdfs:comment>
	<rdfs:label>Adagrad Optimizer</rdfs:label>
	<rdfs:isDefinedBy rdf:resource="https://w3id.org/nno/ontology"/>
</rdf:Description>

<rdf:Description rdf:about="https://w3id.org/nno/ontology#customoptimizer">
	<rdf:type rdf:resource="http://www.w3.org/2004/02/skos/core#Concept"/>
	<skos:inScheme rdf:resource="https://w3id.org/nno/ontology#Optimizer"/>
	<rdfs:comment>Custom optimizer defined by user</rdfs:comment>
	<rdfs:label>Custom Optimizer</rdfs:label>
	<rdfs:isDefinedBy rdf:resource="https://w3id.org/nno/ontology"/>
</rdf:Description>

<rdf:Description rdf:about="https://w3id.org/nno/ontology#nadam">
	<rdf:type rdf:resource="http://www.w3.org/2004/02/skos/core#Concept"/>
	<skos:inScheme rdf:resource="https://w3id.org/nno/ontology#Optimizer"/>
	<rdfs:comment>Much like Adam is essentially RMSprop with momentum, Nadam is Adam RMSprop with Nesterov momentum.</rdfs:comment>
	<rdfs:label>Nesterov Adam Optimizer</rdfs:label>
	<rdfs:isDefinedBy rdf:resource="https://w3id.org/nno/ontology"/>
</rdf:Description>

<rdf:Description rdf:about="https://w3id.org/nno/ontology#rmsprop">
	<rdf:type rdf:resource="http://www.w3.org/2004/02/skos/core#Concept"/>
	<skos:inScheme rdf:resource="https://w3id.org/nno/ontology#Optimizer"/>
	<rdfs:comment>This optimizer is usually a good choice for recurrent neural networks.</rdfs:comment>
	<rdfs:label>RMSProp Optimizer</rdfs:label>
	<rdfs:isDefinedBy rdf:resource="https://w3id.org/nno/ontology"/>
</rdf:Description>

<rdf:Description rdf:about="https://w3id.org/nno/ontology#sgd">
	<rdf:type rdf:resource="http://www.w3.org/2004/02/skos/core#Concept"/>
	<skos:inScheme rdf:resource="https://w3id.org/nno/ontology#Optimizer"/>
	<rdfs:comment>Includes support for momentum, learning rate decay, and Nesterov momentum.</rdfs:comment>
	<rdfs:label>Stochastic Gradient Descent Optimizer</rdfs:label>
	<rdfs:isDefinedBy rdf:resource="https://w3id.org/nno/ontology"/>
</rdf:Description>

<rdf:Description rdf:about="https://w3id.org/nno/ontology#adam">
	<rdf:type rdf:resource="http://www.w3.org/2004/02/skos/core#Concept"/>
	<skos:inScheme rdf:resource="https://w3id.org/nno/ontology#Optimizer"/>
	<rdfs:label>Adam Optimizer</rdfs:label>
	<rdfs:isDefinedBy rdf:resource="https://w3id.org/nno/ontology"/>
</rdf:Description>

<rdf:Description rdf:about="https://w3id.org/nno/ontology#adamax">
	<rdf:type rdf:resource="http://www.w3.org/2004/02/skos/core#Concept"/>
	<skos:inScheme rdf:resource="https://w3id.org/nno/ontology#Optimizer"/>
	<rdfs:label>Adamax Optimizer</rdfs:label>
	<rdfs:isDefinedBy rdf:resource="https://w3id.org/nno/ontology"/>
</rdf:Description>

</rdf:RDF>