<?xml version="1.0" encoding="UTF-8"?>
<rdf:RDF
	xmlns:vann="http://purl.org/vocab/vann/"
	xmlns:voaf="http://purl.org/vocommons/voaf#"
	xmlns:rdfs="http://www.w3.org/2000/01/rdf-schema#"
	xmlns:owl="http://www.w3.org/2002/07/owl#"
	xmlns:skos="http://www.w3.org/2004/02/skos/core#"
	xmlns:rdf="http://www.w3.org/1999/02/22-rdf-syntax-ns#"
	xmlns:dcterms="http://purl.org/dc/terms/"
	xmlns:dc="http://purl.org/dc/elements/1.1/"
	xmlns:dcmit="http://purl.org/dc/dcmitype/"
	xmlns:sesame="http://www.openrdf.org/schema/sesame#"
	xmlns:xsd="http://www.w3.org/2001/XMLSchema#"
	xmlns:fn="http://www.w3.org/2005/xpath-functions#"
	xmlns:foaf="http://xmlns.com/foaf/0.1/"
	xmlns:hint="http://www.bigdata.com/queryHints#"
	xmlns:bd="http://www.bigdata.com/rdf#"
	xmlns:bds="http://www.bigdata.com/rdf/search#">

<rdf:Description rdf:about="http://www.ontology-of-units-of-measure.org/resource/om-2/">
	<rdf:type rdf:resource="http://www.w3.org/2002/07/owl#Ontology"/>
</rdf:Description>

<rdf:Description rdf:about="http://www.ontology-of-units-of-measure.org/resource/om-2/PrefixedMetrePerSecond-Time">
	<rdf:type rdf:resource="http://www.w3.org/2004/02/skos/core#ConceptScheme"/>
</rdf:Description>

<rdf:Description rdf:about="http://www.ontology-of-units-of-measure.org/resource/om-2/attometrePerSecond-Time">
	<rdf:type rdf:resource="http://www.w3.org/2004/02/skos/core#Concept"/>
	<skos:inScheme rdf:resource="http://www.ontology-of-units-of-measure.org/resource/om-2/PrefixedMetrePerSecond-Time"/>
</rdf:Description>

<rdf:Description rdf:about="http://www.ontology-of-units-of-measure.org/resource/om-2/PrefixedMetrePerSecond-Time">
	<rdfs:label xml:lang="en">prefixed metre per second (time)</rdfs:label>
</rdf:Description>

<rdf:Description rdf:about="http://www.ontology-of-units-of-measure.org/resource/om-2/attometrePerSecond-Time">
	<rdfs:comment xml:lang="en">Attometre per second is a unit of speed defined as attometre divided by second.</rdfs:comment>
	<rdfs:label xml:lang="en">attometre per second</rdfs:label>
</rdf:Description>

<rdf:Description rdf:about="http://www.ontology-of-units-of-measure.org/resource/om-2/PrefixedMetrePerSecond-Time">
	<rdfs:isDefinedBy rdf:resource="http://www.ontology-of-units-of-measure.org/resource/om-2/"/>
</rdf:Description>

<rdf:Description rdf:about="http://www.ontology-of-units-of-measure.org/resource/om-2/attometrePerSecond-Time">
	<rdfs:isDefinedBy rdf:resource="http://www.ontology-of-units-of-measure.org/resource/om-2/"/>
</rdf:Description>

<rdf:Description rdf:about="http://www.ontology-of-units-of-measure.org/resource/om-2/centimetrePerSecond-Time">
	<rdf:type rdf:resource="http://www.w3.org/2004/02/skos/core#Concept"/>
	<skos:inScheme rdf:resource="http://www.ontology-of-units-of-measure.org/resource/om-2/PrefixedMetrePerSecond-Time"/>
	<rdfs:comment xml:lang="en">Centimetre per second is a unit of speed defined as centimetre divided by second.</rdfs:comment>
	<rdfs:label xml:lang="en">centimetre per second</rdfs:label>
	<rdfs:isDefinedBy rdf:resource="http://www.ontology-of-units-of-measure.org/resource/om-2/"/>
</rdf:Description>

<rdf:Description rdf:about="http://www.ontology-of-units-of-measure.org/resource/om-2/decametrePerSecond-Time">
	<rdf:type rdf:resource="http://www.w3.org/2004/02/skos/core#Concept"/>
	<skos:inScheme rdf:resource="http://www.ontology-of-units-of-measure.org/resource/om-2/PrefixedMetrePerSecond-Time"/>
	<rdfs:comment xml:lang="en">Decametre per second is a unit of speed defined as decametre divided by second.</rdfs:comment>
	<rdfs:label xml:lang="en">decametre per second</rdfs:label>
	<rdfs:isDefinedBy rdf:resource="http://www.ontology-of-units-of-measure.org/resource/om-2/"/>
</rdf:Description>

<rdf:Description rdf:about="http://www.ontology-of-units-of-measure.org/resource/om-2/decimetrePerSecond-Time">
	<rdf:type rdf:resource="http://www.w3.org/2004/02/skos/core#Concept"/>
	<skos:inScheme rdf:resource="http://www.ontology-of-units-of-measure.org/resource/om-2/PrefixedMetrePerSecond-Time"/>
	<rdfs:comment xml:lang="en">Decimetre per second is a unit of speed defined as decimetre divided by second.</rdfs:comment>
	<rdfs:label xml:lang="en">decimetre per second</rdfs:label>
	<rdfs:isDefinedBy rdf:resource="http://www.ontology-of-units-of-measure.org/resource/om-2/"/>
</rdf:Description>

<rdf:Description rdf:about="http://www.ontology-of-units-of-measure.org/resource/om-2/exametrePerSecond-Time">
	<rdf:type rdf:resource="http://www.w3.org/2004/02/skos/core#Concept"/>
	<skos:inScheme rdf:resource="http://www.ontology-of-units-of-measure.org/resource/om-2/PrefixedMetrePerSecond-Time"/>
	<rdfs:comment xml:lang="en">Exametre per second is a unit of speed defined as exametre divided by second.</rdfs:comment>
	<rdfs:label xml:lang="en">exametre per second</rdfs:label>
	<rdfs:isDefinedBy rdf:resource="http://www.ontology-of-units-of-measure.org/resource/om-2/"/>
</rdf:Description>

<rdf:Description rdf:about="http://www.ontology-of-units-of-measure.org/resource/om-2/femtometrePerSecond-Time">
	<rdf:type rdf:resource="http://www.w3.org/2004/02/skos/core#Concept"/>
	<skos:inScheme rdf:resource="http://www.ontology-of-units-of-measure.org/resource/om-2/PrefixedMetrePerSecond-Time"/>
	<rdfs:comment xml:lang="en">Femtometre per second is a unit of speed defined as femtometre divided by second.</rdfs:comment>
	<rdfs:label xml:lang="en">femtometre per second</rdfs:label>
	<rdfs:isDefinedBy rdf:resource="http://www.ontology-of-units-of-measure.org/resource/om-2/"/>
</rdf:Description>

<rdf:Description rdf:about="http://www.ontology-of-units-of-measure.org/resource/om-2/gigametrePerSecond-Time">
	<rdf:type rdf:resource="http://www.w3.org/2004/02/skos/core#Concept"/>
	<skos:inScheme rdf:resource="http://www.ontology-of-units-of-measure.org/resource/om-2/PrefixedMetrePerSecond-Time"/>
	<rdfs:comment xml:lang="en">Gigametre per second is a unit of speed defined as gigametre divided by second.</rdfs:comment>
	<rdfs:label xml:lang="en">gigametre per second</rdfs:label>
	<rdfs:isDefinedBy rdf:resource="http://www.ontology-of-units-of-measure.org/resource/om-2/"/>
</rdf:Description>

<rdf:Description rdf:about="http://www.ontology-of-units-of-measure.org/resource/om-2/hectometrePerSecond-Time">
	<rdf:type rdf:resource="http://www.w3.org/2004/02/skos/core#Concept"/>
	<skos:inScheme rdf:resource="http://www.ontology-of-units-of-measure.org/resource/om-2/PrefixedMetrePerSecond-Time"/>
	<rdfs:comment xml:lang="en">Hectometre per second is a unit of speed defined as hectometre divided by second.</rdfs:comment>
	<rdfs:label xml:lang="en">hectometre per second</rdfs:label>
	<rdfs:isDefinedBy rdf:resource="http://www.ontology-of-units-of-measure.org/resource/om-2/"/>
</rdf:Description>

<rdf:Description rdf:about="http://www.ontology-of-units-of-measure.org/resource/om-2/kilometrePerSecond-Time">
	<rdf:type rdf:resource="http://www.w3.org/2004/02/skos/core#Concept"/>
	<skos:inScheme rdf:resource="http://www.ontology-of-units-of-measure.org/resource/om-2/PrefixedMetrePerSecond-Time"/>
	<rdfs:comment xml:lang="en">Kilometre per second is a unit of speed defined as kilometre divided by second.</rdfs:comment>
	<rdfs:label xml:lang="en">kilometre per second</rdfs:label>
	<rdfs:isDefinedBy rdf:resource="http://www.ontology-of-units-of-measure.org/resource/om-2/"/>
</rdf:Description>

<rdf:Description rdf:about="http://www.ontology-of-units-of-measure.org/resource/om-2/megametrePerSecond-Time">
	<rdf:type rdf:resource="http://www.w3.org/2004/02/skos/core#Concept"/>
	<skos:inScheme rdf:resource="http://www.ontology-of-units-of-measure.org/resource/om-2/PrefixedMetrePerSecond-Time"/>
	<rdfs:comment xml:lang="en">Megametre per second is a unit of speed defined as megametre divided by second.</rdfs:comment>
	<rdfs:label xml:lang="en">megametre per second</rdfs:label>
	<rdfs:isDefinedBy rdf:resource="http://www.ontology-of-units-of-measure.org/resource/om-2/"/>
</rdf:Description>

<rdf:Description rdf:about="http://www.ontology-of-units-of-measure.org/resource/om-2/micrometrePerSecond-Time">
	<rdf:type rdf:resource="http://www.w3.org/2004/02/skos/core#Concept"/>
	<skos:inScheme rdf:resource="http://www.ontology-of-units-of-measure.org/resource/om-2/PrefixedMetrePerSecond-Time"/>
	<rdfs:comment xml:lang="en">Micrometre per second is a unit of speed defined as micrometre divided by second.</rdfs:comment>
	<rdfs:label xml:lang="en">micrometre per second</rdfs:label>
	<rdfs:isDefinedBy rdf:resource="http://www.ontology-of-units-of-measure.org/resource/om-2/"/>
</rdf:Description>

<rdf:Description rdf:about="http://www.ontology-of-units-of-measure.org/resource/om-2/millimetrePerSecond-Time">
	<rdf:type rdf:resource="http://www.w3.org/2004/02/skos/core#Concept"/>
	<skos:inScheme rdf:resource="http://www.ontology-of-units-of-measure.org/resource/om-2/PrefixedMetrePerSecond-Time"/>
	<rdfs:comment xml:lang="en">Millimetre per second is a unit of speed defined as millimetre divided by second.</rdfs:comment>
	<rdfs:label xml:lang="en">millimetre per second</rdfs:label>
	<rdfs:isDefinedBy rdf:resource="http://www.ontology-of-units-of-measure.org/resource/om-2/"/>
</rdf:Description>

<rdf:Description rdf:about="http://www.ontology-of-units-of-measure.org/resource/om-2/nanometrePerSecond-Time">
	<rdf:type rdf:resource="http://www.w3.org/2004/02/skos/core#Concept"/>
	<skos:inScheme rdf:resource="http://www.ontology-of-units-of-measure.org/resource/om-2/PrefixedMetrePerSecond-Time"/>
	<rdfs:comment xml:lang="en">Nanometre per second is a unit of speed defined as nanometre divided by second.</rdfs:comment>
	<rdfs:label xml:lang="en">nanometre per second</rdfs:label>
	<rdfs:isDefinedBy rdf:resource="http://www.ontology-of-units-of-measure.org/resource/om-2/"/>
</rdf:Description>

<rdf:Description rdf:about="http://www.ontology-of-units-of-measure.org/resource/om-2/petametrePerSecond-Time">
	<rdf:type rdf:resource="http://www.w3.org/2004/02/skos/core#Concept"/>
	<skos:inScheme rdf:resource="http://www.ontology-of-units-of-measure.org/resource/om-2/PrefixedMetrePerSecond-Time"/>
	<rdfs:comment xml:lang="en">Petametre per second is a unit of speed defined as petametre divided by second.</rdfs:comment>
	<rdfs:label xml:lang="en">petametre per second</rdfs:label>
	<rdfs:isDefinedBy rdf:resource="http://www.ontology-of-units-of-measure.org/resource/om-2/"/>
</rdf:Description>

<rdf:Description rdf:about="http://www.ontology-of-units-of-measure.org/resource/om-2/picometrePerSecond-Time">
	<rdf:type rdf:resource="http://www.w3.org/2004/02/skos/core#Concept"/>
	<skos:inScheme rdf:resource="http://www.ontology-of-units-of-measure.org/resource/om-2/PrefixedMetrePerSecond-Time"/>
	<rdfs:comment xml:lang="en">Picometre per second is a unit of speed defined as picometre divided by second.</rdfs:comment>
	<rdfs:label xml:lang="en">picometre per second</rdfs:label>
	<rdfs:isDefinedBy rdf:resource="http://www.ontology-of-units-of-measure.org/resource/om-2/"/>
</rdf:Description>

<rdf:Description rdf:about="http://www.ontology-of-units-of-measure.org/resource/om-2/terametrePerSecond-Time">
	<rdf:type rdf:resource="http://www.w3.org/2004/02/skos/core#Concept"/>
	<skos:inScheme rdf:resource="http://www.ontology-of-units-of-measure.org/resource/om-2/PrefixedMetrePerSecond-Time"/>
	<rdfs:comment xml:lang="en">Terametre per second is a unit of speed defined as terametre divided by second.</rdfs:comment>
	<rdfs:label xml:lang="en">terametre per second</rdfs:label>
	<rdfs:isDefinedBy rdf:resource="http://www.ontology-of-units-of-measure.org/resource/om-2/"/>
</rdf:Description>

<rdf:Description rdf:about="http://www.ontology-of-units-of-measure.org/resource/om-2/yoctometrePerSecond-Time">
	<rdf:type rdf:resource="http://www.w3.org/2004/02/skos/core#Concept"/>
	<skos:inScheme rdf:resource="http://www.ontology-of-units-of-measure.org/resource/om-2/PrefixedMetrePerSecond-Time"/>
	<rdfs:comment xml:lang="en">Yoctometre per second is a unit of speed defined as yoctometre divided by second.</rdfs:comment>
	<rdfs:label xml:lang="en">yoctometre per second</rdfs:label>
	<rdfs:isDefinedBy rdf:resource="http://www.ontology-of-units-of-measure.org/resource/om-2/"/>
</rdf:Description>

<rdf:Description rdf:about="http://www.ontology-of-units-of-measure.org/resource/om-2/yottametrePerSecond-Time">
	<rdf:type rdf:resource="http://www.w3.org/2004/02/skos/core#Concept"/>
	<skos:inScheme rdf:resource="http://www.ontology-of-units-of-measure.org/resource/om-2/PrefixedMetrePerSecond-Time"/>
	<rdfs:comment xml:lang="en">Yottametre per second is a unit of speed defined as yottametre divided by second.</rdfs:comment>
	<rdfs:label xml:lang="en">yottametre per second</rdfs:label>
	<rdfs:isDefinedBy rdf:resource="http://www.ontology-of-units-of-measure.org/resource/om-2/"/>
</rdf:Description>

<rdf:Description rdf:about="http://www.ontology-of-units-of-measure.org/resource/om-2/zeptometrePerSecond-Time">
	<rdf:type rdf:resource="http://www.w3.org/2004/02/skos/core#Concept"/>
	<skos:inScheme rdf:resource="http://www.ontology-of-units-of-measure.org/resource/om-2/PrefixedMetrePerSecond-Time"/>
	<rdfs:comment xml:lang="en">Zeptometre per second is a unit of speed defined as zeptometre divided by second.</rdfs:comment>
	<rdfs:label xml:lang="en">zeptometre per second</rdfs:label>
	<rdfs:isDefinedBy rdf:resource="http://www.ontology-of-units-of-measure.org/resource/om-2/"/>
</rdf:Description>

<rdf:Description rdf:about="http://www.ontology-of-units-of-measure.org/resource/om-2/zettametrePerSecond-Time">
	<rdf:type rdf:resource="http://www.w3.org/2004/02/skos/core#Concept"/>
	<skos:inScheme rdf:resource="http://www.ontology-of-units-of-measure.org/resource/om-2/PrefixedMetrePerSecond-Time"/>
	<rdfs:comment xml:lang="en">Zettametre per second is a unit of speed defined as zettametre divided by second.</rdfs:comment>
	<rdfs:label xml:lang="en">zettametre per second</rdfs:label>
	<rdfs:isDefinedBy rdf:resource="http://www.ontology-of-units-of-measure.org/resource/om-2/"/>
</rdf:Description>

</rdf:RDF>