<?xml version="1.0" encoding="UTF-8"?>
<rdf:RDF
	xmlns:vann="http://purl.org/vocab/vann/"
	xmlns:voaf="http://purl.org/vocommons/voaf#"
	xmlns:rdfs="http://www.w3.org/2000/01/rdf-schema#"
	xmlns:owl="http://www.w3.org/2002/07/owl#"
	xmlns:skos="http://www.w3.org/2004/02/skos/core#"
	xmlns:rdf="http://www.w3.org/1999/02/22-rdf-syntax-ns#"
	xmlns:dcterms="http://purl.org/dc/terms/"
	xmlns:dc="http://purl.org/dc/elements/1.1/"
	xmlns:dcmit="http://purl.org/dc/dcmitype/"
	xmlns:sesame="http://www.openrdf.org/schema/sesame#"
	xmlns:xsd="http://www.w3.org/2001/XMLSchema#"
	xmlns:fn="http://www.w3.org/2005/xpath-functions#"
	xmlns:foaf="http://xmlns.com/foaf/0.1/"
	xmlns:hint="http://www.bigdata.com/queryHints#"
	xmlns:bd="http://www.bigdata.com/rdf#"
	xmlns:bds="http://www.bigdata.com/rdf/search#">

<rdf:Description rdf:about="http://purl.org/opdm/refrigerator#">
	<rdf:type rdf:resource="http://www.w3.org/2002/07/owl#Ontology"/>
</rdf:Description>

<rdf:Description rdf:about="http://purl.org/opdm/refrigerator#ClimateClass">
	<rdf:type rdf:resource="http://www.w3.org/2004/02/skos/core#ConceptScheme"/>
</rdf:Description>

<rdf:Description rdf:about="http://purl.org/opdm/refrigerator#ClimateN">
	<rdf:type rdf:resource="http://www.w3.org/2004/02/skos/core#Concept"/>
	<skos:inScheme rdf:resource="http://purl.org/opdm/refrigerator#ClimateClass"/>
</rdf:Description>

<rdf:Description rdf:about="http://purl.org/opdm/refrigerator#ClimateClass">
	<rdfs:comment xml:lang="en">Class to represent the range of room temperatures that a fridge/freezer can operate. Possible values include: N, SN, ST, T.</rdfs:comment>
	<rdfs:label xml:lang="en">ClimateClass</rdfs:label>
</rdf:Description>

<rdf:Description rdf:about="http://purl.org/opdm/refrigerator#ClimateN">
	<rdfs:comment xml:lang="en">This concept represents the N climate class rating. The fridge/freezer can operate between 16 - 32 degree celsius of room temperature</rdfs:comment>
	<rdfs:label xml:lang="en">N Rating</rdfs:label>
</rdf:Description>

<rdf:Description rdf:about="http://purl.org/opdm/refrigerator#ratingOfClimateClass">
	<rdfs:range rdf:resource="http://purl.org/opdm/refrigerator#ClimateClass"/>
	<rdfs:domain rdf:resource="http://purl.org/opdm/refrigerator#FridgeFreezer"/>
	<rdfs:label xml:lang="en">Rating of climate class</rdfs:label>
	<rdfs:comment xml:lang="en">The climate class rating that the fridge/freezer can operate at.</rdfs:comment>
	<rdf:type rdf:resource="http://www.w3.org/2002/07/owl#ObjectProperty"/>
</rdf:Description>

<rdf:Description rdf:about="http://purl.org/opdm/refrigerator#ClimateClass">
	<rdfs:isDefinedBy rdf:resource="http://purl.org/opdm/refrigerator#"/>
</rdf:Description>

<rdf:Description rdf:about="http://purl.org/opdm/refrigerator#ClimateN">
	<rdfs:isDefinedBy rdf:resource="http://purl.org/opdm/refrigerator#"/>
</rdf:Description>

<rdf:Description rdf:about="http://purl.org/opdm/refrigerator#ClimateSN">
	<rdf:type rdf:resource="http://www.w3.org/2004/02/skos/core#Concept"/>
	<skos:inScheme rdf:resource="http://purl.org/opdm/refrigerator#ClimateClass"/>
	<rdfs:comment xml:lang="en">This concept represents the SN climate class rating. The fridge/freezer can operate between 10 - 32 degree celsius of room temperature</rdfs:comment>
	<rdfs:label xml:lang="en">SN Rating</rdfs:label>
	<rdfs:isDefinedBy rdf:resource="http://purl.org/opdm/refrigerator#"/>
</rdf:Description>

<rdf:Description rdf:about="http://purl.org/opdm/refrigerator#ClimateST">
	<rdf:type rdf:resource="http://www.w3.org/2004/02/skos/core#Concept"/>
	<skos:inScheme rdf:resource="http://purl.org/opdm/refrigerator#ClimateClass"/>
	<rdfs:comment xml:lang="en">This concept represents the ST climate class rating. The fridge/freezer can operate between 18 - 38 degree celsius of room temperature</rdfs:comment>
	<rdfs:label xml:lang="en">ST Rating</rdfs:label>
	<rdfs:isDefinedBy rdf:resource="http://purl.org/opdm/refrigerator#"/>
</rdf:Description>

<rdf:Description rdf:about="http://purl.org/opdm/refrigerator#ClimateT">
	<rdf:type rdf:resource="http://www.w3.org/2004/02/skos/core#Concept"/>
	<skos:inScheme rdf:resource="http://purl.org/opdm/refrigerator#ClimateClass"/>
	<rdfs:comment xml:lang="en">This concept represents the T climate class rating. The fridge/freezer can operate between 18 - 43 degree celsius of room temperature</rdfs:comment>
	<rdfs:label xml:lang="en">T Rating</rdfs:label>
	<rdfs:isDefinedBy rdf:resource="http://purl.org/opdm/refrigerator#"/>
</rdf:Description>

</rdf:RDF>