<?xml version="1.0" encoding="UTF-8"?>
<rdf:RDF
	xmlns:vann="http://purl.org/vocab/vann/"
	xmlns:voaf="http://purl.org/vocommons/voaf#"
	xmlns:rdfs="http://www.w3.org/2000/01/rdf-schema#"
	xmlns:owl="http://www.w3.org/2002/07/owl#"
	xmlns:skos="http://www.w3.org/2004/02/skos/core#"
	xmlns:rdf="http://www.w3.org/1999/02/22-rdf-syntax-ns#"
	xmlns:dcterms="http://purl.org/dc/terms/"
	xmlns:dc="http://purl.org/dc/elements/1.1/"
	xmlns:dcmit="http://purl.org/dc/dcmitype/"
	xmlns:sesame="http://www.openrdf.org/schema/sesame#"
	xmlns:xsd="http://www.w3.org/2001/XMLSchema#"
	xmlns:fn="http://www.w3.org/2005/xpath-functions#"
	xmlns:foaf="http://xmlns.com/foaf/0.1/"
	xmlns:hint="http://www.bigdata.com/queryHints#"
	xmlns:bd="http://www.bigdata.com/rdf#"
	xmlns:bds="http://www.bigdata.com/rdf/search#">

<rdf:Description rdf:about="http://securitytoolbox.appspot.com/securityMain">
	<rdf:type rdf:resource="http://www.w3.org/2002/07/owl#Ontology"/>
</rdf:Description>

<rdf:Description rdf:about="http://securitytoolbox.appspot.com/securityMain#SecurityObjective">
	<rdf:type rdf:resource="http://www.w3.org/2004/02/skos/core#ConceptScheme"/>
</rdf:Description>

<rdf:Description rdf:about="http://securitytoolbox.appspot.com/securityMain#Anonymity">
	<rdf:type rdf:resource="http://www.w3.org/2004/02/skos/core#Concept"/>
	<skos:inScheme rdf:resource="http://securitytoolbox.appspot.com/securityMain#SecurityObjective"/>
</rdf:Description>

<rdf:Description rdf:about="http://securitytoolbox.appspot.com/securityMain#SecurityObjective">
	<rdfs:label xml:lang="en">Security Objective</rdfs:label>
</rdf:Description>

<rdf:Description rdf:about="http://securitytoolbox.appspot.com/securityMain#Anonymity">
	<rdfs:comment>
(Secondary Objective) Provides anonymity
</rdfs:comment>
</rdf:Description>

<rdf:Description rdf:about="http://securitytoolbox.appspot.com/securityMain#supportsSecurityObjectives">
	<rdfs:range rdf:resource="http://securitytoolbox.appspot.com/securityMain#SecurityObjective"/>
	<rdfs:domain rdf:resource="http://securitytoolbox.appspot.com/securityMain#SecurityConcept"/>
	<rdfs:label xml:lang="en">supports Security Objectives</rdfs:label>
	<rdfs:comment>
Any SecurityConcept can support one or more of the Security Objectives defined
in the SecurityObjective class
</rdfs:comment>
	<rdf:type rdf:resource="http://www.w3.org/2002/07/owl#ObjectProperty"/>
</rdf:Description>

<rdf:Description rdf:about="http://securitytoolbox.appspot.com/securityMain#SecurityObjective">
	<rdfs:isDefinedBy rdf:resource="http://securitytoolbox.appspot.com/securityMain"/>
</rdf:Description>

<rdf:Description rdf:about="http://securitytoolbox.appspot.com/securityMain#Anonymity">
	<rdfs:isDefinedBy rdf:resource="http://securitytoolbox.appspot.com/securityMain"/>
</rdf:Description>

<rdf:Description rdf:about="http://securitytoolbox.appspot.com/securityMain#Authorization">
	<rdf:type rdf:resource="http://www.w3.org/2004/02/skos/core#Concept"/>
	<skos:inScheme rdf:resource="http://securitytoolbox.appspot.com/securityMain#SecurityObjective"/>
	<rdfs:comment>
Only authorized entities are allowed to access resources in an authorized
manner.
(Aka Access Control). If desired, user may create instance of AccessControl as
well.
</rdfs:comment>
	<rdfs:isDefinedBy rdf:resource="http://securitytoolbox.appspot.com/securityMain"/>
</rdf:Description>

<rdf:Description rdf:about="http://securitytoolbox.appspot.com/securityMain#Availability">
	<rdf:type rdf:resource="http://www.w3.org/2004/02/skos/core#Concept"/>
	<skos:inScheme rdf:resource="http://securitytoolbox.appspot.com/securityMain#SecurityObjective"/>
	<rdfs:comment>
Provides guarantee that resource is available to authorized users at any
authorized time.
</rdfs:comment>
	<rdfs:isDefinedBy rdf:resource="http://securitytoolbox.appspot.com/securityMain"/>
</rdf:Description>

<rdf:Description rdf:about="http://securitytoolbox.appspot.com/securityMain#Confidentiality">
	<rdf:type rdf:resource="http://www.w3.org/2004/02/skos/core#Concept"/>
	<skos:inScheme rdf:resource="http://securitytoolbox.appspot.com/securityMain#SecurityObjective"/>
	<rdfs:comment>
Protects against information being disclosed or revealed to unauthorized
parties.
</rdfs:comment>
	<rdfs:isDefinedBy rdf:resource="http://securitytoolbox.appspot.com/securityMain"/>
</rdf:Description>

<rdf:Description rdf:about="http://securitytoolbox.appspot.com/securityMain#CovertChannelPrevention">
	<rdf:type rdf:resource="http://www.w3.org/2004/02/skos/core#Concept"/>
	<skos:inScheme rdf:resource="http://securitytoolbox.appspot.com/securityMain#SecurityObjective"/>
	<rdfs:comment>
(Secondary Objective) Prevent or limit the existance of covert channels
</rdfs:comment>
	<rdfs:isDefinedBy rdf:resource="http://securitytoolbox.appspot.com/securityMain"/>
</rdf:Description>

<rdf:Description rdf:about="http://securitytoolbox.appspot.com/securityMain#HostTrust">
	<rdf:type rdf:resource="http://www.w3.org/2004/02/skos/core#Concept"/>
	<skos:inScheme rdf:resource="http://securitytoolbox.appspot.com/securityMain#SecurityObjective"/>
	<rdfs:comment>
(Secondary Objective) How to trust host or platform. Is relevant to Common
criteria, etc.
</rdfs:comment>
	<rdfs:isDefinedBy rdf:resource="http://securitytoolbox.appspot.com/securityMain"/>
</rdf:Description>

<rdf:Description rdf:about="http://securitytoolbox.appspot.com/securityMain#KeyManagement">
	<rdf:type rdf:resource="http://www.w3.org/2004/02/skos/core#Concept"/>
	<skos:inScheme rdf:resource="http://securitytoolbox.appspot.com/securityMain#SecurityObjective"/>
	<rdfs:comment>
(SecondaryObjective) Securely manages keys for legitimate users.
</rdfs:comment>
	<rdfs:isDefinedBy rdf:resource="http://securitytoolbox.appspot.com/securityMain"/>
</rdf:Description>

<rdf:Description rdf:about="http://securitytoolbox.appspot.com/securityMain#MessageAuthentication">
	<rdf:type rdf:resource="http://www.w3.org/2004/02/skos/core#Concept"/>
	<skos:inScheme rdf:resource="http://securitytoolbox.appspot.com/securityMain#SecurityObjective"/>
	<rdfs:comment>
Provides guarantee that message came from whoever claimed to have sent it.
</rdfs:comment>
	<rdfs:isDefinedBy rdf:resource="http://securitytoolbox.appspot.com/securityMain"/>
</rdf:Description>

<rdf:Description rdf:about="http://securitytoolbox.appspot.com/securityMain#MessageIntegrity">
	<rdf:type rdf:resource="http://www.w3.org/2004/02/skos/core#Concept"/>
	<skos:inScheme rdf:resource="http://securitytoolbox.appspot.com/securityMain#SecurityObjective"/>
	<rdfs:comment>
Data integrity or Message integrity; data cannot be changed, deleted,
modified, etc by unauthorized parties.
</rdfs:comment>
	<rdfs:isDefinedBy rdf:resource="http://securitytoolbox.appspot.com/securityMain"/>
</rdf:Description>

<rdf:Description rdf:about="http://securitytoolbox.appspot.com/securityMain#ReplayPrevention">
	<rdf:type rdf:resource="http://www.w3.org/2004/02/skos/core#Concept"/>
	<skos:inScheme rdf:resource="http://securitytoolbox.appspot.com/securityMain#SecurityObjective"/>
	<rdfs:comment>
(Secondary Objective) Protect against replay attacks
</rdfs:comment>
	<rdfs:isDefinedBy rdf:resource="http://securitytoolbox.appspot.com/securityMain"/>
</rdf:Description>

<rdf:Description rdf:about="http://securitytoolbox.appspot.com/securityMain#Separation">
	<rdf:type rdf:resource="http://www.w3.org/2004/02/skos/core#Concept"/>
	<skos:inScheme rdf:resource="http://securitytoolbox.appspot.com/securityMain#SecurityObjective"/>
	<rdfs:comment>
(Secondary Objective)
</rdfs:comment>
	<rdfs:isDefinedBy rdf:resource="http://securitytoolbox.appspot.com/securityMain"/>
</rdf:Description>

<rdf:Description rdf:about="http://securitytoolbox.appspot.com/securityMain#TrafficHiding">
	<rdf:type rdf:resource="http://www.w3.org/2004/02/skos/core#Concept"/>
	<skos:inScheme rdf:resource="http://securitytoolbox.appspot.com/securityMain#SecurityObjective"/>
	<rdfs:comment>
(Secondary Objective) Pad traffic with bogus data to hide traffic patterns
</rdfs:comment>
	<rdfs:isDefinedBy rdf:resource="http://securitytoolbox.appspot.com/securityMain"/>
</rdf:Description>

<rdf:Description rdf:about="http://securitytoolbox.appspot.com/securityMain#Trust">
	<rdf:type rdf:resource="http://www.w3.org/2004/02/skos/core#Concept"/>
	<skos:inScheme rdf:resource="http://securitytoolbox.appspot.com/securityMain#SecurityObjective"/>
	<rdfs:comment>
(Secondary Objective) How to trust entity. Trust not only of identification,
but statements, claims, etc.
</rdfs:comment>
	<rdfs:isDefinedBy rdf:resource="http://securitytoolbox.appspot.com/securityMain"/>
</rdf:Description>

<rdf:Description rdf:about="http://securitytoolbox.appspot.com/securityMain#UserAuthentication">
	<rdf:type rdf:resource="http://www.w3.org/2004/02/skos/core#Concept"/>
	<skos:inScheme rdf:resource="http://securitytoolbox.appspot.com/securityMain#SecurityObjective"/>
	<rdfs:comment>
Provides assurance of the identity of a person or entity.
</rdfs:comment>
	<rdfs:isDefinedBy rdf:resource="http://securitytoolbox.appspot.com/securityMain"/>
</rdf:Description>

</rdf:RDF>