<?xml version="1.0" encoding="UTF-8"?>
<rdf:RDF
	xmlns:vann="http://purl.org/vocab/vann/"
	xmlns:voaf="http://purl.org/vocommons/voaf#"
	xmlns:rdfs="http://www.w3.org/2000/01/rdf-schema#"
	xmlns:owl="http://www.w3.org/2002/07/owl#"
	xmlns:skos="http://www.w3.org/2004/02/skos/core#"
	xmlns:rdf="http://www.w3.org/1999/02/22-rdf-syntax-ns#"
	xmlns:dcterms="http://purl.org/dc/terms/"
	xmlns:dc="http://purl.org/dc/elements/1.1/"
	xmlns:dcmit="http://purl.org/dc/dcmitype/"
	xmlns:sesame="http://www.openrdf.org/schema/sesame#"
	xmlns:xsd="http://www.w3.org/2001/XMLSchema#"
	xmlns:fn="http://www.w3.org/2005/xpath-functions#"
	xmlns:foaf="http://xmlns.com/foaf/0.1/"
	xmlns:hint="http://www.bigdata.com/queryHints#"
	xmlns:bd="http://www.bigdata.com/rdf#"
	xmlns:bds="http://www.bigdata.com/rdf/search#">

<rdf:Description rdf:about="http://purl.org/opdm/refrigerator#">
	<rdf:type rdf:resource="http://www.w3.org/2002/07/owl#Ontology"/>
</rdf:Description>

<rdf:Description rdf:about="http://purl.org/opdm/refrigerator#EnergyRatingEU">
	<rdf:type rdf:resource="http://www.w3.org/2004/02/skos/core#ConceptScheme"/>
</rdf:Description>

<rdf:Description rdf:about="http://purl.org/opdm/refrigerator#EnergyA">
	<rdf:type rdf:resource="http://www.w3.org/2004/02/skos/core#Concept"/>
	<skos:inScheme rdf:resource="http://purl.org/opdm/refrigerator#EnergyRatingEU"/>
</rdf:Description>

<rdf:Description rdf:about="http://purl.org/opdm/refrigerator#EnergyRatingEU">
	<rdfs:comment xml:lang="en">Class to represent the European Union energy label codas of a fridge. Possible values go from A+++ to G.</rdfs:comment>
	<rdfs:label xml:lang="en">EnergyRatingEU</rdfs:label>
</rdf:Description>

<rdf:Description rdf:about="http://purl.org/opdm/refrigerator#EnergyA">
	<rdfs:comment xml:lang="en">This concept represents the A energy efficiency rating in the European Union labelling scheme</rdfs:comment>
	<rdfs:label xml:lang="en">A Rating</rdfs:label>
</rdf:Description>

<rdf:Description rdf:about="http://purl.org/opdm/refrigerator#ratingOfEnergyEU">
	<rdfs:range rdf:resource="http://purl.org/opdm/refrigerator#EnergyRatingEU"/>
	<rdfs:domain rdf:resource="http://purl.org/opdm/refrigerator#FridgeFreezer"/>
	<rdfs:label xml:lang="en">Rating of energy EU</rdfs:label>
	<rdfs:comment xml:lang="en">The rating of energy efficiency in the European Union that the fridge/freezer operates at.</rdfs:comment>
	<rdf:type rdf:resource="http://www.w3.org/2002/07/owl#ObjectProperty"/>
</rdf:Description>

<rdf:Description rdf:about="http://purl.org/opdm/refrigerator#EnergyRatingEU">
	<rdfs:isDefinedBy rdf:resource="http://purl.org/opdm/refrigerator#"/>
</rdf:Description>

<rdf:Description rdf:about="http://purl.org/opdm/refrigerator#EnergyA">
	<rdfs:isDefinedBy rdf:resource="http://purl.org/opdm/refrigerator#"/>
</rdf:Description>

<rdf:Description rdf:about="http://purl.org/opdm/refrigerator#EnergyA1">
	<rdf:type rdf:resource="http://www.w3.org/2004/02/skos/core#Concept"/>
	<skos:inScheme rdf:resource="http://purl.org/opdm/refrigerator#EnergyRatingEU"/>
	<rdfs:comment xml:lang="en">This concept represents the A+ energy efficiency rating in the European Union labelling scheme</rdfs:comment>
	<rdfs:label xml:lang="en">A+ Rating</rdfs:label>
	<rdfs:isDefinedBy rdf:resource="http://purl.org/opdm/refrigerator#"/>
</rdf:Description>

<rdf:Description rdf:about="http://purl.org/opdm/refrigerator#EnergyA2">
	<rdf:type rdf:resource="http://www.w3.org/2004/02/skos/core#Concept"/>
	<skos:inScheme rdf:resource="http://purl.org/opdm/refrigerator#EnergyRatingEU"/>
	<rdfs:comment xml:lang="en">This concept represents the A++ energy efficiency rating in the European Union labelling scheme</rdfs:comment>
	<rdfs:label xml:lang="en">A++ Rating</rdfs:label>
	<rdfs:isDefinedBy rdf:resource="http://purl.org/opdm/refrigerator#"/>
</rdf:Description>

<rdf:Description rdf:about="http://purl.org/opdm/refrigerator#EnergyA3">
	<rdf:type rdf:resource="http://www.w3.org/2004/02/skos/core#Concept"/>
	<skos:inScheme rdf:resource="http://purl.org/opdm/refrigerator#EnergyRatingEU"/>
	<rdfs:comment xml:lang="en">This concept represents the A+++ energy efficiency rating in the European Union labelling scheme</rdfs:comment>
	<rdfs:label xml:lang="en">A+++ Rating</rdfs:label>
	<rdfs:isDefinedBy rdf:resource="http://purl.org/opdm/refrigerator#"/>
</rdf:Description>

<rdf:Description rdf:about="http://purl.org/opdm/refrigerator#EnergyB">
	<rdf:type rdf:resource="http://www.w3.org/2004/02/skos/core#Concept"/>
	<skos:inScheme rdf:resource="http://purl.org/opdm/refrigerator#EnergyRatingEU"/>
	<rdfs:comment xml:lang="en">This concept represents the B energy efficiency rating in the European Union labelling scheme</rdfs:comment>
	<rdfs:label xml:lang="en">B Rating</rdfs:label>
	<rdfs:isDefinedBy rdf:resource="http://purl.org/opdm/refrigerator#"/>
</rdf:Description>

<rdf:Description rdf:about="http://purl.org/opdm/refrigerator#EnergyC">
	<rdf:type rdf:resource="http://www.w3.org/2004/02/skos/core#Concept"/>
	<skos:inScheme rdf:resource="http://purl.org/opdm/refrigerator#EnergyRatingEU"/>
	<rdfs:comment xml:lang="en">This concept represents the C energy efficiency rating in the European Union labelling scheme</rdfs:comment>
	<rdfs:label xml:lang="en">C Rating</rdfs:label>
	<rdfs:isDefinedBy rdf:resource="http://purl.org/opdm/refrigerator#"/>
</rdf:Description>

<rdf:Description rdf:about="http://purl.org/opdm/refrigerator#EnergyD">
	<rdf:type rdf:resource="http://www.w3.org/2004/02/skos/core#Concept"/>
	<skos:inScheme rdf:resource="http://purl.org/opdm/refrigerator#EnergyRatingEU"/>
	<rdfs:comment xml:lang="en">This concept represents the D energy efficiency rating in the European Union labelling scheme</rdfs:comment>
	<rdfs:label xml:lang="en">D Rating</rdfs:label>
	<rdfs:isDefinedBy rdf:resource="http://purl.org/opdm/refrigerator#"/>
</rdf:Description>

<rdf:Description rdf:about="http://purl.org/opdm/refrigerator#EnergyE">
	<rdf:type rdf:resource="http://www.w3.org/2004/02/skos/core#Concept"/>
	<skos:inScheme rdf:resource="http://purl.org/opdm/refrigerator#EnergyRatingEU"/>
	<rdfs:comment xml:lang="en">This concept represents the E energy efficiency rating in the European Union labelling scheme</rdfs:comment>
	<rdfs:label xml:lang="en">E Rating</rdfs:label>
	<rdfs:isDefinedBy rdf:resource="http://purl.org/opdm/refrigerator#"/>
</rdf:Description>

<rdf:Description rdf:about="http://purl.org/opdm/refrigerator#EnergyF">
	<rdf:type rdf:resource="http://www.w3.org/2004/02/skos/core#Concept"/>
	<skos:inScheme rdf:resource="http://purl.org/opdm/refrigerator#EnergyRatingEU"/>
	<rdfs:comment xml:lang="en">This concept represents the F energy efficiency rating in the European Union labelling scheme</rdfs:comment>
	<rdfs:label xml:lang="en">F Rating</rdfs:label>
	<rdfs:isDefinedBy rdf:resource="http://purl.org/opdm/refrigerator#"/>
</rdf:Description>

<rdf:Description rdf:about="http://purl.org/opdm/refrigerator#EnergyG">
	<rdf:type rdf:resource="http://www.w3.org/2004/02/skos/core#Concept"/>
	<skos:inScheme rdf:resource="http://purl.org/opdm/refrigerator#EnergyRatingEU"/>
	<rdfs:comment xml:lang="en">This concept represents the G energy efficiency rating in the European Union labelling scheme</rdfs:comment>
	<rdfs:label xml:lang="en">G Rating</rdfs:label>
	<rdfs:isDefinedBy rdf:resource="http://purl.org/opdm/refrigerator#"/>
</rdf:Description>

</rdf:RDF>