<?xml version="1.0" encoding="UTF-8"?>
<rdf:RDF
	xmlns:vann="http://purl.org/vocab/vann/"
	xmlns:voaf="http://purl.org/vocommons/voaf#"
	xmlns:rdfs="http://www.w3.org/2000/01/rdf-schema#"
	xmlns:owl="http://www.w3.org/2002/07/owl#"
	xmlns:skos="http://www.w3.org/2004/02/skos/core#"
	xmlns:rdf="http://www.w3.org/1999/02/22-rdf-syntax-ns#"
	xmlns:dcterms="http://purl.org/dc/terms/"
	xmlns:dc="http://purl.org/dc/elements/1.1/"
	xmlns:dcmit="http://purl.org/dc/dcmitype/"
	xmlns:sesame="http://www.openrdf.org/schema/sesame#"
	xmlns:xsd="http://www.w3.org/2001/XMLSchema#"
	xmlns:fn="http://www.w3.org/2005/xpath-functions#"
	xmlns:foaf="http://xmlns.com/foaf/0.1/"
	xmlns:hint="http://www.bigdata.com/queryHints#"
	xmlns:bd="http://www.bigdata.com/rdf#"
	xmlns:bds="http://www.bigdata.com/rdf/search#">

<rdf:Description rdf:about="http://www.ontology-of-units-of-measure.org/resource/om-2/">
	<rdf:type rdf:resource="http://www.w3.org/2002/07/owl#Ontology"/>
</rdf:Description>

<rdf:Description rdf:about="http://www.ontology-of-units-of-measure.org/resource/om-2/SingularUnit">
	<rdf:type rdf:resource="http://www.w3.org/2004/02/skos/core#ConceptScheme"/>
</rdf:Description>

<rdf:Description rdf:about="http://www.ontology-of-units-of-measure.org/resource/om-2/statampere">
	<rdf:type rdf:resource="http://www.w3.org/2004/02/skos/core#Concept"/>
	<skos:inScheme rdf:resource="http://www.ontology-of-units-of-measure.org/resource/om-2/SingularUnit"/>
</rdf:Description>

<rdf:Description rdf:about="http://www.ontology-of-units-of-measure.org/resource/om-2/SingularUnit">
	<rdfs:label xml:lang="en">singular unit</rdfs:label>
</rdf:Description>

<rdf:Description rdf:about="http://www.ontology-of-units-of-measure.org/resource/om-2/statampere">
	<rdfs:comment xml:lang="en">The statampere is a unit of electric current defined as 3.335641e-10 ampere.</rdfs:comment>
	<rdfs:label xml:lang="en">statampere</rdfs:label>
	<hasUnit xmlns="http://www.ontology-of-units-of-measure.org/resource/om-2/" rdf:resource="http://www.ontology-of-units-of-measure.org/resource/om-2/ampere"/>
</rdf:Description>

<rdf:Description rdf:about="http://www.ontology-of-units-of-measure.org/resource/om-2/ampere">
	<rdf:type rdf:resource="http://www.w3.org/2004/02/skos/core#Concept"/>
</rdf:Description>

<rdf:Description rdf:about="http://www.ontology-of-units-of-measure.org/resource/om-2/SingularUnit">
	<rdfs:isDefinedBy rdf:resource="http://www.ontology-of-units-of-measure.org/resource/om-2/"/>
</rdf:Description>

<rdf:Description rdf:about="http://www.ontology-of-units-of-measure.org/resource/om-2/statampere">
	<rdfs:isDefinedBy rdf:resource="http://www.ontology-of-units-of-measure.org/resource/om-2/"/>
</rdf:Description>

<rdf:Description rdf:about="http://www.ontology-of-units-of-measure.org/resource/om-2/ampere">
	<rdfs:isDefinedBy rdf:resource="http://www.ontology-of-units-of-measure.org/resource/om-2/"/>
</rdf:Description>

<rdf:Description rdf:about="http://www.ontology-of-units-of-measure.org/resource/om-2/abampere">
	<rdf:type rdf:resource="http://www.w3.org/2004/02/skos/core#Concept"/>
	<skos:inScheme rdf:resource="http://www.ontology-of-units-of-measure.org/resource/om-2/SingularUnit"/>
	<rdfs:comment xml:lang="en">The abampere is a unit of electric current defined as 10 ampere.</rdfs:comment>
	<rdfs:label xml:lang="en">abampere</rdfs:label>
	<hasUnit xmlns="http://www.ontology-of-units-of-measure.org/resource/om-2/" rdf:resource="http://www.ontology-of-units-of-measure.org/resource/om-2/ampere"/>
	<rdfs:isDefinedBy rdf:resource="http://www.ontology-of-units-of-measure.org/resource/om-2/"/>
</rdf:Description>

<rdf:Description rdf:about="http://www.ontology-of-units-of-measure.org/resource/om-2/biot">
	<rdf:type rdf:resource="http://www.w3.org/2004/02/skos/core#Concept"/>
	<skos:inScheme rdf:resource="http://www.ontology-of-units-of-measure.org/resource/om-2/SingularUnit"/>
	<rdfs:comment xml:lang="en">The biot is a unit of electric current defined as 10 ampere.</rdfs:comment>
	<rdfs:label xml:lang="en">biot</rdfs:label>
	<hasUnit xmlns="http://www.ontology-of-units-of-measure.org/resource/om-2/" rdf:resource="http://www.ontology-of-units-of-measure.org/resource/om-2/ampere"/>
	<rdfs:isDefinedBy rdf:resource="http://www.ontology-of-units-of-measure.org/resource/om-2/"/>
</rdf:Description>

<rdf:Description rdf:about="http://www.ontology-of-units-of-measure.org/resource/om-2/gilbert">
	<rdf:type rdf:resource="http://www.w3.org/2004/02/skos/core#Concept"/>
	<skos:inScheme rdf:resource="http://www.ontology-of-units-of-measure.org/resource/om-2/SingularUnit"/>
	<rdfs:comment xml:lang="en">The gilbert is a unit of electric current defined as 7.957747e-1 ampere.</rdfs:comment>
	<rdfs:label xml:lang="en">gilbert</rdfs:label>
	<hasUnit xmlns="http://www.ontology-of-units-of-measure.org/resource/om-2/" rdf:resource="http://www.ontology-of-units-of-measure.org/resource/om-2/ampere"/>
	<rdfs:isDefinedBy rdf:resource="http://www.ontology-of-units-of-measure.org/resource/om-2/"/>
</rdf:Description>

<rdf:Description rdf:about="http://www.ontology-of-units-of-measure.org/resource/om-2/curie">
	<rdf:type rdf:resource="http://www.w3.org/2004/02/skos/core#Concept"/>
	<skos:inScheme rdf:resource="http://www.ontology-of-units-of-measure.org/resource/om-2/SingularUnit"/>
	<rdfs:comment xml:lang="en">The curie is a unit of activity defined as 3.7e10 becquerel.</rdfs:comment>
	<rdfs:label xml:lang="en">curie</rdfs:label>
	<hasUnit xmlns="http://www.ontology-of-units-of-measure.org/resource/om-2/" rdf:resource="http://www.ontology-of-units-of-measure.org/resource/om-2/becquerel"/>
</rdf:Description>

<rdf:Description rdf:about="http://www.ontology-of-units-of-measure.org/resource/om-2/becquerel">
	<rdf:type rdf:resource="http://www.w3.org/2004/02/skos/core#Concept"/>
</rdf:Description>

<rdf:Description rdf:about="http://www.ontology-of-units-of-measure.org/resource/om-2/curie">
	<rdfs:isDefinedBy rdf:resource="http://www.ontology-of-units-of-measure.org/resource/om-2/"/>
</rdf:Description>

<rdf:Description rdf:about="http://www.ontology-of-units-of-measure.org/resource/om-2/becquerel">
	<rdfs:isDefinedBy rdf:resource="http://www.ontology-of-units-of-measure.org/resource/om-2/"/>
</rdf:Description>

<rdf:Description rdf:about="http://www.ontology-of-units-of-measure.org/resource/om-2/byte">
	<rdf:type rdf:resource="http://www.w3.org/2004/02/skos/core#Concept"/>
	<skos:inScheme rdf:resource="http://www.ontology-of-units-of-measure.org/resource/om-2/SingularUnit"/>
	<rdfs:comment xml:lang="en">The byte is a unit of information capacity defined as 8 bit.</rdfs:comment>
	<rdfs:label xml:lang="en">byte</rdfs:label>
	<hasUnit xmlns="http://www.ontology-of-units-of-measure.org/resource/om-2/" rdf:resource="http://www.ontology-of-units-of-measure.org/resource/om-2/bit"/>
</rdf:Description>

<rdf:Description rdf:about="http://www.ontology-of-units-of-measure.org/resource/om-2/bit">
	<rdf:type rdf:resource="http://www.w3.org/2004/02/skos/core#Concept"/>
</rdf:Description>

<rdf:Description rdf:about="http://www.ontology-of-units-of-measure.org/resource/om-2/byte">
	<rdfs:isDefinedBy rdf:resource="http://www.ontology-of-units-of-measure.org/resource/om-2/"/>
</rdf:Description>

<rdf:Description rdf:about="http://www.ontology-of-units-of-measure.org/resource/om-2/bit">
	<rdfs:isDefinedBy rdf:resource="http://www.ontology-of-units-of-measure.org/resource/om-2/"/>
</rdf:Description>

<rdf:Description rdf:about="http://www.ontology-of-units-of-measure.org/resource/om-2/hartley">
	<rdf:type rdf:resource="http://www.w3.org/2004/02/skos/core#Concept"/>
	<skos:inScheme rdf:resource="http://www.ontology-of-units-of-measure.org/resource/om-2/SingularUnit"/>
	<rdfs:comment xml:lang="en">The hartley is a unit of information capacity defined as 3.321928095 bit.</rdfs:comment>
	<rdfs:label xml:lang="en">hartley</rdfs:label>
	<hasUnit xmlns="http://www.ontology-of-units-of-measure.org/resource/om-2/" rdf:resource="http://www.ontology-of-units-of-measure.org/resource/om-2/bit"/>
	<rdfs:isDefinedBy rdf:resource="http://www.ontology-of-units-of-measure.org/resource/om-2/"/>
</rdf:Description>

<rdf:Description rdf:about="http://www.ontology-of-units-of-measure.org/resource/om-2/shannon">
	<rdf:type rdf:resource="http://www.w3.org/2004/02/skos/core#Concept"/>
	<skos:inScheme rdf:resource="http://www.ontology-of-units-of-measure.org/resource/om-2/SingularUnit"/>
	<rdfs:comment xml:lang="en">The shannon is a unit of information capacity defined as 1 bit.</rdfs:comment>
	<rdfs:label xml:lang="en">shannon</rdfs:label>
	<hasUnit xmlns="http://www.ontology-of-units-of-measure.org/resource/om-2/" rdf:resource="http://www.ontology-of-units-of-measure.org/resource/om-2/bit"/>
	<rdfs:isDefinedBy rdf:resource="http://www.ontology-of-units-of-measure.org/resource/om-2/"/>
</rdf:Description>

<rdf:Description rdf:about="http://www.ontology-of-units-of-measure.org/resource/om-2/quad">
	<rdf:type rdf:resource="http://www.w3.org/2004/02/skos/core#Concept"/>
	<skos:inScheme rdf:resource="http://www.ontology-of-units-of-measure.org/resource/om-2/SingularUnit"/>
	<rdfs:comment xml:lang="en">The quad is a unit of energy defined as 1.0e15 British thermal unit (International Table).</rdfs:comment>
	<rdfs:label xml:lang="en">quad</rdfs:label>
	<hasUnit xmlns="http://www.ontology-of-units-of-measure.org/resource/om-2/" rdf:resource="http://www.ontology-of-units-of-measure.org/resource/om-2/BritishThermalUnit-InternationalTable"/>
</rdf:Description>

<rdf:Description rdf:about="http://www.ontology-of-units-of-measure.org/resource/om-2/BritishThermalUnit-InternationalTable">
	<rdf:type rdf:resource="http://www.w3.org/2004/02/skos/core#Concept"/>
</rdf:Description>

<rdf:Description rdf:about="http://www.ontology-of-units-of-measure.org/resource/om-2/quad">
	<rdfs:isDefinedBy rdf:resource="http://www.ontology-of-units-of-measure.org/resource/om-2/"/>
</rdf:Description>

<rdf:Description rdf:about="http://www.ontology-of-units-of-measure.org/resource/om-2/BritishThermalUnit-InternationalTable">
	<rdfs:isDefinedBy rdf:resource="http://www.ontology-of-units-of-measure.org/resource/om-2/"/>
</rdf:Description>

<rdf:Description rdf:about="http://www.ontology-of-units-of-measure.org/resource/om-2/abcoulomb">
	<rdf:type rdf:resource="http://www.w3.org/2004/02/skos/core#Concept"/>
	<skos:inScheme rdf:resource="http://www.ontology-of-units-of-measure.org/resource/om-2/SingularUnit"/>
	<rdfs:comment xml:lang="en">The abcoulomb is a unit of electric charge defined as 10 coulomb.</rdfs:comment>
	<rdfs:label xml:lang="en">abcoulomb</rdfs:label>
	<hasUnit xmlns="http://www.ontology-of-units-of-measure.org/resource/om-2/" rdf:resource="http://www.ontology-of-units-of-measure.org/resource/om-2/coulomb"/>
</rdf:Description>

<rdf:Description rdf:about="http://www.ontology-of-units-of-measure.org/resource/om-2/coulomb">
	<rdf:type rdf:resource="http://www.w3.org/2004/02/skos/core#Concept"/>
</rdf:Description>

<rdf:Description rdf:about="http://www.ontology-of-units-of-measure.org/resource/om-2/abcoulomb">
	<rdfs:isDefinedBy rdf:resource="http://www.ontology-of-units-of-measure.org/resource/om-2/"/>
</rdf:Description>

<rdf:Description rdf:about="http://www.ontology-of-units-of-measure.org/resource/om-2/coulomb">
	<rdfs:isDefinedBy rdf:resource="http://www.ontology-of-units-of-measure.org/resource/om-2/"/>
</rdf:Description>

<rdf:Description rdf:about="http://www.ontology-of-units-of-measure.org/resource/om-2/statcoulomb">
	<rdf:type rdf:resource="http://www.w3.org/2004/02/skos/core#Concept"/>
	<skos:inScheme rdf:resource="http://www.ontology-of-units-of-measure.org/resource/om-2/SingularUnit"/>
	<rdfs:comment xml:lang="en">The statcoulomb is a unit of electric charge defined as 3.335641e-10 coulomb.</rdfs:comment>
	<rdfs:label xml:lang="en">statcoulomb</rdfs:label>
	<hasUnit xmlns="http://www.ontology-of-units-of-measure.org/resource/om-2/" rdf:resource="http://www.ontology-of-units-of-measure.org/resource/om-2/coulomb"/>
	<rdfs:isDefinedBy rdf:resource="http://www.ontology-of-units-of-measure.org/resource/om-2/"/>
</rdf:Description>

<rdf:Description rdf:about="http://www.ontology-of-units-of-measure.org/resource/om-2/faraday">
	<rdf:type rdf:resource="http://www.w3.org/2004/02/skos/core#Concept"/>
	<skos:inScheme rdf:resource="http://www.ontology-of-units-of-measure.org/resource/om-2/SingularUnit"/>
	<rdfs:comment xml:lang="en">The faraday is a unit of electric charge defined as 9.648531e4 coulomb.</rdfs:comment>
	<rdfs:label xml:lang="en">faraday</rdfs:label>
	<hasUnit xmlns="http://www.ontology-of-units-of-measure.org/resource/om-2/" rdf:resource="http://www.ontology-of-units-of-measure.org/resource/om-2/coulomb"/>
	<rdfs:isDefinedBy rdf:resource="http://www.ontology-of-units-of-measure.org/resource/om-2/"/>
</rdf:Description>

<rdf:Description rdf:about="http://www.ontology-of-units-of-measure.org/resource/om-2/franklin">
	<rdf:type rdf:resource="http://www.w3.org/2004/02/skos/core#Concept"/>
	<skos:inScheme rdf:resource="http://www.ontology-of-units-of-measure.org/resource/om-2/SingularUnit"/>
	<rdfs:comment xml:lang="en">The franklin is a unit of electric charge defined as 3.335641e-10 coulomb.</rdfs:comment>
	<rdfs:label xml:lang="en">franklin</rdfs:label>
	<hasUnit xmlns="http://www.ontology-of-units-of-measure.org/resource/om-2/" rdf:resource="http://www.ontology-of-units-of-measure.org/resource/om-2/coulomb"/>
	<rdfs:isDefinedBy rdf:resource="http://www.ontology-of-units-of-measure.org/resource/om-2/"/>
</rdf:Description>

<rdf:Description rdf:about="http://www.ontology-of-units-of-measure.org/resource/om-2/hour-HourAngle">
	<rdf:type rdf:resource="http://www.w3.org/2004/02/skos/core#Concept"/>
	<skos:inScheme rdf:resource="http://www.ontology-of-units-of-measure.org/resource/om-2/SingularUnit"/>
	<rdfs:label xml:lang="en">hour (hour angle)</rdfs:label>
	<hasUnit xmlns="http://www.ontology-of-units-of-measure.org/resource/om-2/" rdf:resource="http://www.ontology-of-units-of-measure.org/resource/om-2/degree"/>
</rdf:Description>

<rdf:Description rdf:about="http://www.ontology-of-units-of-measure.org/resource/om-2/degree">
	<rdf:type rdf:resource="http://www.w3.org/2004/02/skos/core#Concept"/>
</rdf:Description>

<rdf:Description rdf:about="http://www.ontology-of-units-of-measure.org/resource/om-2/hour-HourAngle">
	<rdfs:isDefinedBy rdf:resource="http://www.ontology-of-units-of-measure.org/resource/om-2/"/>
</rdf:Description>

<rdf:Description rdf:about="http://www.ontology-of-units-of-measure.org/resource/om-2/degree">
	<rdfs:isDefinedBy rdf:resource="http://www.ontology-of-units-of-measure.org/resource/om-2/"/>
</rdf:Description>

<rdf:Description rdf:about="http://www.ontology-of-units-of-measure.org/resource/om-2/minute-HourAngle">
	<rdf:type rdf:resource="http://www.w3.org/2004/02/skos/core#Concept"/>
	<skos:inScheme rdf:resource="http://www.ontology-of-units-of-measure.org/resource/om-2/SingularUnit"/>
	<rdfs:label xml:lang="en">minute (hour angle)</rdfs:label>
	<hasUnit xmlns="http://www.ontology-of-units-of-measure.org/resource/om-2/" rdf:resource="http://www.ontology-of-units-of-measure.org/resource/om-2/degree"/>
	<rdfs:isDefinedBy rdf:resource="http://www.ontology-of-units-of-measure.org/resource/om-2/"/>
</rdf:Description>

<rdf:Description rdf:about="http://www.ontology-of-units-of-measure.org/resource/om-2/second-HourAngle">
	<rdf:type rdf:resource="http://www.w3.org/2004/02/skos/core#Concept"/>
	<skos:inScheme rdf:resource="http://www.ontology-of-units-of-measure.org/resource/om-2/SingularUnit"/>
	<rdfs:label xml:lang="en">second (hour angle)</rdfs:label>
	<hasUnit xmlns="http://www.ontology-of-units-of-measure.org/resource/om-2/" rdf:resource="http://www.ontology-of-units-of-measure.org/resource/om-2/degree"/>
	<rdfs:isDefinedBy rdf:resource="http://www.ontology-of-units-of-measure.org/resource/om-2/"/>
</rdf:Description>

<rdf:Description rdf:about="http://www.ontology-of-units-of-measure.org/resource/om-2/point-Postscript">
	<rdf:type rdf:resource="http://www.w3.org/2004/02/skos/core#Concept"/>
	<skos:inScheme rdf:resource="http://www.ontology-of-units-of-measure.org/resource/om-2/SingularUnit"/>
	<rdfs:comment xml:lang="en">The Postscript point is a unit of length defined as 0.013888888888888888888888888888889 inch.</rdfs:comment>
	<rdfs:label xml:lang="en">point (Postscript)</rdfs:label>
	<hasUnit xmlns="http://www.ontology-of-units-of-measure.org/resource/om-2/" rdf:resource="http://www.ontology-of-units-of-measure.org/resource/om-2/inch-International"/>
</rdf:Description>

<rdf:Description rdf:about="http://www.ontology-of-units-of-measure.org/resource/om-2/inch-International">
	<rdf:type rdf:resource="http://www.w3.org/2004/02/skos/core#Concept"/>
</rdf:Description>

<rdf:Description rdf:about="http://www.ontology-of-units-of-measure.org/resource/om-2/point-Postscript">
	<rdfs:isDefinedBy rdf:resource="http://www.ontology-of-units-of-measure.org/resource/om-2/"/>
</rdf:Description>

<rdf:Description rdf:about="http://www.ontology-of-units-of-measure.org/resource/om-2/inch-International">
	<rdfs:isDefinedBy rdf:resource="http://www.ontology-of-units-of-measure.org/resource/om-2/"/>
</rdf:Description>

<rdf:Description rdf:about="http://www.ontology-of-units-of-measure.org/resource/om-2/point-TeX">
	<rdf:type rdf:resource="http://www.w3.org/2004/02/skos/core#Concept"/>
	<skos:inScheme rdf:resource="http://www.ontology-of-units-of-measure.org/resource/om-2/SingularUnit"/>
	<rdfs:comment xml:lang="en">The TeX point is a unit of length defined as 0.01383700013837000138370001383 inch.</rdfs:comment>
	<rdfs:label xml:lang="en">point (TeX)</rdfs:label>
	<hasUnit xmlns="http://www.ontology-of-units-of-measure.org/resource/om-2/" rdf:resource="http://www.ontology-of-units-of-measure.org/resource/om-2/inch-International"/>
	<rdfs:isDefinedBy rdf:resource="http://www.ontology-of-units-of-measure.org/resource/om-2/"/>
</rdf:Description>

<rdf:Description rdf:about="http://www.ontology-of-units-of-measure.org/resource/om-2/therm-EC">
	<rdf:type rdf:resource="http://www.w3.org/2004/02/skos/core#Concept"/>
	<skos:inScheme rdf:resource="http://www.ontology-of-units-of-measure.org/resource/om-2/SingularUnit"/>
	<rdfs:comment xml:lang="en">The EC therm is a unit of energy defined as 1.05506e8 joule.</rdfs:comment>
	<rdfs:label xml:lang="en">therm (EC)</rdfs:label>
	<hasUnit xmlns="http://www.ontology-of-units-of-measure.org/resource/om-2/" rdf:resource="http://www.ontology-of-units-of-measure.org/resource/om-2/joule"/>
</rdf:Description>

<rdf:Description rdf:about="http://www.ontology-of-units-of-measure.org/resource/om-2/joule">
	<rdf:type rdf:resource="http://www.w3.org/2004/02/skos/core#Concept"/>
</rdf:Description>

<rdf:Description rdf:about="http://www.ontology-of-units-of-measure.org/resource/om-2/therm-EC">
	<rdfs:isDefinedBy rdf:resource="http://www.ontology-of-units-of-measure.org/resource/om-2/"/>
</rdf:Description>

<rdf:Description rdf:about="http://www.ontology-of-units-of-measure.org/resource/om-2/joule">
	<rdfs:isDefinedBy rdf:resource="http://www.ontology-of-units-of-measure.org/resource/om-2/"/>
</rdf:Description>

<rdf:Description rdf:about="http://www.ontology-of-units-of-measure.org/resource/om-2/therm-US">
	<rdf:type rdf:resource="http://www.w3.org/2004/02/skos/core#Concept"/>
	<skos:inScheme rdf:resource="http://www.ontology-of-units-of-measure.org/resource/om-2/SingularUnit"/>
	<rdfs:comment xml:lang="en">The US therm is a unit of energy defined as 1.054804e8 joule.</rdfs:comment>
	<rdfs:label xml:lang="en">therm (US)</rdfs:label>
	<hasUnit xmlns="http://www.ontology-of-units-of-measure.org/resource/om-2/" rdf:resource="http://www.ontology-of-units-of-measure.org/resource/om-2/joule"/>
	<rdfs:isDefinedBy rdf:resource="http://www.ontology-of-units-of-measure.org/resource/om-2/"/>
</rdf:Description>

<rdf:Description rdf:about="http://www.ontology-of-units-of-measure.org/resource/om-2/tonOfTNT">
	<rdf:type rdf:resource="http://www.w3.org/2004/02/skos/core#Concept"/>
	<skos:inScheme rdf:resource="http://www.ontology-of-units-of-measure.org/resource/om-2/SingularUnit"/>
	<rdfs:comment xml:lang="en">The ton of TNT is a unit of energy defined as 4.184e9 joule.</rdfs:comment>
	<rdfs:label xml:lang="en">ton of TNT</rdfs:label>
	<hasUnit xmlns="http://www.ontology-of-units-of-measure.org/resource/om-2/" rdf:resource="http://www.ontology-of-units-of-measure.org/resource/om-2/joule"/>
	<rdfs:isDefinedBy rdf:resource="http://www.ontology-of-units-of-measure.org/resource/om-2/"/>
</rdf:Description>

<rdf:Description rdf:about="http://www.ontology-of-units-of-measure.org/resource/om-2/rad">
	<rdf:type rdf:resource="http://www.w3.org/2004/02/skos/core#Concept"/>
	<skos:inScheme rdf:resource="http://www.ontology-of-units-of-measure.org/resource/om-2/SingularUnit"/>
	<rdfs:comment xml:lang="en">The rad is a unit of absorbed dose defined as 1.0e-2 gray.</rdfs:comment>
	<rdfs:label xml:lang="en">rad</rdfs:label>
	<hasUnit xmlns="http://www.ontology-of-units-of-measure.org/resource/om-2/" rdf:resource="http://www.ontology-of-units-of-measure.org/resource/om-2/gray"/>
</rdf:Description>

<rdf:Description rdf:about="http://www.ontology-of-units-of-measure.org/resource/om-2/gray">
	<rdf:type rdf:resource="http://www.w3.org/2004/02/skos/core#Concept"/>
</rdf:Description>

<rdf:Description rdf:about="http://www.ontology-of-units-of-measure.org/resource/om-2/rad">
	<rdfs:isDefinedBy rdf:resource="http://www.ontology-of-units-of-measure.org/resource/om-2/"/>
</rdf:Description>

<rdf:Description rdf:about="http://www.ontology-of-units-of-measure.org/resource/om-2/gray">
	<rdfs:isDefinedBy rdf:resource="http://www.ontology-of-units-of-measure.org/resource/om-2/"/>
</rdf:Description>

<rdf:Description rdf:about="http://www.ontology-of-units-of-measure.org/resource/om-2/abhenry">
	<rdf:type rdf:resource="http://www.w3.org/2004/02/skos/core#Concept"/>
	<skos:inScheme rdf:resource="http://www.ontology-of-units-of-measure.org/resource/om-2/SingularUnit"/>
	<rdfs:comment xml:lang="en">The abhenry is a unit of inductance defined as 1.0e-9 henry.</rdfs:comment>
	<rdfs:label xml:lang="en">abhenry</rdfs:label>
	<hasUnit xmlns="http://www.ontology-of-units-of-measure.org/resource/om-2/" rdf:resource="http://www.ontology-of-units-of-measure.org/resource/om-2/henry"/>
</rdf:Description>

<rdf:Description rdf:about="http://www.ontology-of-units-of-measure.org/resource/om-2/henry">
	<rdf:type rdf:resource="http://www.w3.org/2004/02/skos/core#Concept"/>
</rdf:Description>

<rdf:Description rdf:about="http://www.ontology-of-units-of-measure.org/resource/om-2/abhenry">
	<rdfs:isDefinedBy rdf:resource="http://www.ontology-of-units-of-measure.org/resource/om-2/"/>
</rdf:Description>

<rdf:Description rdf:about="http://www.ontology-of-units-of-measure.org/resource/om-2/henry">
	<rdfs:isDefinedBy rdf:resource="http://www.ontology-of-units-of-measure.org/resource/om-2/"/>
</rdf:Description>

<rdf:Description rdf:about="http://www.ontology-of-units-of-measure.org/resource/om-2/stathenry">
	<rdf:type rdf:resource="http://www.w3.org/2004/02/skos/core#Concept"/>
	<skos:inScheme rdf:resource="http://www.ontology-of-units-of-measure.org/resource/om-2/SingularUnit"/>
	<rdfs:comment xml:lang="en">The stathenry is a unit of inductance defined as 8.987552e11 henry.</rdfs:comment>
	<rdfs:label xml:lang="en">stathenry</rdfs:label>
	<hasUnit xmlns="http://www.ontology-of-units-of-measure.org/resource/om-2/" rdf:resource="http://www.ontology-of-units-of-measure.org/resource/om-2/henry"/>
	<rdfs:isDefinedBy rdf:resource="http://www.ontology-of-units-of-measure.org/resource/om-2/"/>
</rdf:Description>

<rdf:Description rdf:about="http://www.ontology-of-units-of-measure.org/resource/om-2/quart-Imperial">
	<rdf:type rdf:resource="http://www.w3.org/2004/02/skos/core#Concept"/>
	<skos:inScheme rdf:resource="http://www.ontology-of-units-of-measure.org/resource/om-2/SingularUnit"/>
	<rdfs:comment xml:lang="en">The imperial quart is a unit of volume defined as 1.1365 litre.</rdfs:comment>
	<rdfs:label xml:lang="en">quart (imperial)</rdfs:label>
	<hasUnit xmlns="http://www.ontology-of-units-of-measure.org/resource/om-2/" rdf:resource="http://www.ontology-of-units-of-measure.org/resource/om-2/litre"/>
</rdf:Description>

<rdf:Description rdf:about="http://www.ontology-of-units-of-measure.org/resource/om-2/litre">
	<rdf:type rdf:resource="http://www.w3.org/2004/02/skos/core#Concept"/>
</rdf:Description>

<rdf:Description rdf:about="http://www.ontology-of-units-of-measure.org/resource/om-2/quart-Imperial">
	<rdfs:isDefinedBy rdf:resource="http://www.ontology-of-units-of-measure.org/resource/om-2/"/>
</rdf:Description>

<rdf:Description rdf:about="http://www.ontology-of-units-of-measure.org/resource/om-2/litre">
	<rdfs:isDefinedBy rdf:resource="http://www.ontology-of-units-of-measure.org/resource/om-2/"/>
</rdf:Description>

<rdf:Description rdf:about="http://www.ontology-of-units-of-measure.org/resource/om-2/calorie-15C">
	<rdf:type rdf:resource="http://www.w3.org/2004/02/skos/core#Concept"/>
	<skos:inScheme rdf:resource="http://www.ontology-of-units-of-measure.org/resource/om-2/SingularUnit"/>
	<rdfs:comment xml:lang="en">The 15 °C calorie is a unit of energy defined as 4.18580 joule.</rdfs:comment>
	<rdfs:label xml:lang="en">calorie (15 °C)</rdfs:label>
	<hasUnit xmlns="http://www.ontology-of-units-of-measure.org/resource/om-2/" rdf:resource="http://www.ontology-of-units-of-measure.org/resource/om-2/joule"/>
	<rdfs:isDefinedBy rdf:resource="http://www.ontology-of-units-of-measure.org/resource/om-2/"/>
</rdf:Description>

<rdf:Description rdf:about="http://www.ontology-of-units-of-measure.org/resource/om-2/calorie-20C">
	<rdf:type rdf:resource="http://www.w3.org/2004/02/skos/core#Concept"/>
	<skos:inScheme rdf:resource="http://www.ontology-of-units-of-measure.org/resource/om-2/SingularUnit"/>
	<rdfs:comment xml:lang="en">The 20 °C calorie is a unit of energy defined as 4.18190 joule.</rdfs:comment>
	<rdfs:label xml:lang="en">calorie (20 °C)</rdfs:label>
	<hasUnit xmlns="http://www.ontology-of-units-of-measure.org/resource/om-2/" rdf:resource="http://www.ontology-of-units-of-measure.org/resource/om-2/joule"/>
	<rdfs:isDefinedBy rdf:resource="http://www.ontology-of-units-of-measure.org/resource/om-2/"/>
</rdf:Description>

<rdf:Description rdf:about="http://www.ontology-of-units-of-measure.org/resource/om-2/calorie-InternationalTable">
	<rdf:type rdf:resource="http://www.w3.org/2004/02/skos/core#Concept"/>
	<skos:inScheme rdf:resource="http://www.ontology-of-units-of-measure.org/resource/om-2/SingularUnit"/>
	<rdfs:comment xml:lang="en">The International Table calorie is a unit of energy defined as 4.1868 joule.</rdfs:comment>
	<rdfs:label xml:lang="en">calorie (International Table)</rdfs:label>
	<hasUnit xmlns="http://www.ontology-of-units-of-measure.org/resource/om-2/" rdf:resource="http://www.ontology-of-units-of-measure.org/resource/om-2/joule"/>
	<rdfs:isDefinedBy rdf:resource="http://www.ontology-of-units-of-measure.org/resource/om-2/"/>
</rdf:Description>

<rdf:Description rdf:about="http://www.ontology-of-units-of-measure.org/resource/om-2/calorie-Mean">
	<rdf:type rdf:resource="http://www.w3.org/2004/02/skos/core#Concept"/>
	<skos:inScheme rdf:resource="http://www.ontology-of-units-of-measure.org/resource/om-2/SingularUnit"/>
	<rdfs:comment xml:lang="en">The mean calorie is a unit of energy defined as 4.19002 joule.</rdfs:comment>
	<rdfs:label xml:lang="en">calorie (mean)</rdfs:label>
	<hasUnit xmlns="http://www.ontology-of-units-of-measure.org/resource/om-2/" rdf:resource="http://www.ontology-of-units-of-measure.org/resource/om-2/joule"/>
	<rdfs:isDefinedBy rdf:resource="http://www.ontology-of-units-of-measure.org/resource/om-2/"/>
</rdf:Description>

<rdf:Description rdf:about="http://www.ontology-of-units-of-measure.org/resource/om-2/calorie-Thermochemical">
	<rdf:type rdf:resource="http://www.w3.org/2004/02/skos/core#Concept"/>
	<skos:inScheme rdf:resource="http://www.ontology-of-units-of-measure.org/resource/om-2/SingularUnit"/>
	<rdfs:comment xml:lang="en">The thermochemical calorie is a unit of energy defined as 4.184 joule.</rdfs:comment>
	<rdfs:label xml:lang="en">calorie (thermochemical)</rdfs:label>
	<hasUnit xmlns="http://www.ontology-of-units-of-measure.org/resource/om-2/" rdf:resource="http://www.ontology-of-units-of-measure.org/resource/om-2/joule"/>
	<rdfs:isDefinedBy rdf:resource="http://www.ontology-of-units-of-measure.org/resource/om-2/"/>
</rdf:Description>

<rdf:Description rdf:about="http://www.ontology-of-units-of-measure.org/resource/om-2/electronvolt">
	<rdf:type rdf:resource="http://www.w3.org/2004/02/skos/core#Concept"/>
	<skos:inScheme rdf:resource="http://www.ontology-of-units-of-measure.org/resource/om-2/SingularUnit"/>
	<rdfs:comment xml:lang="en">The electronvolt is a unit of energy defined as 1.602177e-19 joule.</rdfs:comment>
	<rdfs:label xml:lang="en">electronvolt</rdfs:label>
	<hasUnit xmlns="http://www.ontology-of-units-of-measure.org/resource/om-2/" rdf:resource="http://www.ontology-of-units-of-measure.org/resource/om-2/joule"/>
	<rdfs:isDefinedBy rdf:resource="http://www.ontology-of-units-of-measure.org/resource/om-2/"/>
</rdf:Description>

<rdf:Description rdf:about="http://www.ontology-of-units-of-measure.org/resource/om-2/erg">
	<rdf:type rdf:resource="http://www.w3.org/2004/02/skos/core#Concept"/>
	<skos:inScheme rdf:resource="http://www.ontology-of-units-of-measure.org/resource/om-2/SingularUnit"/>
	<rdfs:comment xml:lang="en">The erg is a unit of energy defined as 1.0e-7 joule.</rdfs:comment>
	<rdfs:label xml:lang="en">erg</rdfs:label>
	<hasUnit xmlns="http://www.ontology-of-units-of-measure.org/resource/om-2/" rdf:resource="http://www.ontology-of-units-of-measure.org/resource/om-2/joule"/>
	<rdfs:isDefinedBy rdf:resource="http://www.ontology-of-units-of-measure.org/resource/om-2/"/>
</rdf:Description>

<rdf:Description rdf:about="http://www.ontology-of-units-of-measure.org/resource/om-2/footPoundal">
	<rdf:type rdf:resource="http://www.w3.org/2004/02/skos/core#Concept"/>
	<skos:inScheme rdf:resource="http://www.ontology-of-units-of-measure.org/resource/om-2/SingularUnit"/>
	<rdfs:comment xml:lang="en">The foot poundal is a unit of energy defined as 4.214011e-2 joule.</rdfs:comment>
	<rdfs:label xml:lang="en">foot poundal</rdfs:label>
	<hasUnit xmlns="http://www.ontology-of-units-of-measure.org/resource/om-2/" rdf:resource="http://www.ontology-of-units-of-measure.org/resource/om-2/joule"/>
	<rdfs:isDefinedBy rdf:resource="http://www.ontology-of-units-of-measure.org/resource/om-2/"/>
</rdf:Description>

<rdf:Description rdf:about="http://www.ontology-of-units-of-measure.org/resource/om-2/degreeCelsius">
	<rdf:type rdf:resource="http://www.w3.org/2004/02/skos/core#Concept"/>
	<skos:inScheme rdf:resource="http://www.ontology-of-units-of-measure.org/resource/om-2/SingularUnit"/>
	<rdfs:comment xml:lang="en">The degree Celsius is a unit of temperature defined as 1 kelvin.</rdfs:comment>
	<rdfs:label xml:lang="en">degree Celsius</rdfs:label>
	<hasUnit xmlns="http://www.ontology-of-units-of-measure.org/resource/om-2/" rdf:resource="http://www.ontology-of-units-of-measure.org/resource/om-2/kelvin"/>
</rdf:Description>

<rdf:Description rdf:about="http://www.ontology-of-units-of-measure.org/resource/om-2/kelvin">
	<rdf:type rdf:resource="http://www.w3.org/2004/02/skos/core#Concept"/>
</rdf:Description>

<rdf:Description rdf:about="http://www.ontology-of-units-of-measure.org/resource/om-2/degreeCelsius">
	<rdfs:isDefinedBy rdf:resource="http://www.ontology-of-units-of-measure.org/resource/om-2/"/>
</rdf:Description>

<rdf:Description rdf:about="http://www.ontology-of-units-of-measure.org/resource/om-2/kelvin">
	<rdfs:isDefinedBy rdf:resource="http://www.ontology-of-units-of-measure.org/resource/om-2/"/>
</rdf:Description>

<rdf:Description rdf:about="http://www.ontology-of-units-of-measure.org/resource/om-2/degreeFahrenheit">
	<rdf:type rdf:resource="http://www.w3.org/2004/02/skos/core#Concept"/>
	<skos:inScheme rdf:resource="http://www.ontology-of-units-of-measure.org/resource/om-2/SingularUnit"/>
	<rdfs:comment xml:lang="en">The degree Fahrenheit is a unit of temperature defined as 5.555556e-1 kelvin.</rdfs:comment>
	<rdfs:label xml:lang="en">degree Fahrenheit</rdfs:label>
	<hasUnit xmlns="http://www.ontology-of-units-of-measure.org/resource/om-2/" rdf:resource="http://www.ontology-of-units-of-measure.org/resource/om-2/kelvin"/>
	<rdfs:isDefinedBy rdf:resource="http://www.ontology-of-units-of-measure.org/resource/om-2/"/>
</rdf:Description>

<rdf:Description rdf:about="http://www.ontology-of-units-of-measure.org/resource/om-2/degreeRankine">
	<rdf:type rdf:resource="http://www.w3.org/2004/02/skos/core#Concept"/>
	<skos:inScheme rdf:resource="http://www.ontology-of-units-of-measure.org/resource/om-2/SingularUnit"/>
	<rdfs:comment xml:lang="en">The degree Rankine is a unit of temperature defined as 5.555556e-1 kelvin.</rdfs:comment>
	<rdfs:label xml:lang="en">degree Rankine</rdfs:label>
	<hasUnit xmlns="http://www.ontology-of-units-of-measure.org/resource/om-2/" rdf:resource="http://www.ontology-of-units-of-measure.org/resource/om-2/kelvin"/>
	<rdfs:isDefinedBy rdf:resource="http://www.ontology-of-units-of-measure.org/resource/om-2/"/>
</rdf:Description>

<rdf:Description rdf:about="http://www.ontology-of-units-of-measure.org/resource/om-2/degreeReaumur">
	<rdf:type rdf:resource="http://www.w3.org/2004/02/skos/core#Concept"/>
	<skos:inScheme rdf:resource="http://www.ontology-of-units-of-measure.org/resource/om-2/SingularUnit"/>
	<rdfs:comment xml:lang="en">The degree Réaumur is a unit of temperature defined as 1.25 kelvin.</rdfs:comment>
	<rdfs:label xml:lang="en">degree Réaumur</rdfs:label>
	<hasUnit xmlns="http://www.ontology-of-units-of-measure.org/resource/om-2/" rdf:resource="http://www.ontology-of-units-of-measure.org/resource/om-2/kelvin"/>
	<rdfs:isDefinedBy rdf:resource="http://www.ontology-of-units-of-measure.org/resource/om-2/"/>
</rdf:Description>

<rdf:Description rdf:about="http://www.ontology-of-units-of-measure.org/resource/om-2/mil-Angle">
	<rdf:type rdf:resource="http://www.w3.org/2004/02/skos/core#Concept"/>
	<skos:inScheme rdf:resource="http://www.ontology-of-units-of-measure.org/resource/om-2/SingularUnit"/>
	<rdfs:comment xml:lang="en">The mil (angle) is a unit of angle defined as 9.817477e-4 radian.</rdfs:comment>
	<rdfs:label xml:lang="en">mil (angle)</rdfs:label>
	<hasUnit xmlns="http://www.ontology-of-units-of-measure.org/resource/om-2/" rdf:resource="http://www.ontology-of-units-of-measure.org/resource/om-2/radian"/>
</rdf:Description>

<rdf:Description rdf:about="http://www.ontology-of-units-of-measure.org/resource/om-2/radian">
	<rdf:type rdf:resource="http://www.w3.org/2004/02/skos/core#Concept"/>
</rdf:Description>

<rdf:Description rdf:about="http://www.ontology-of-units-of-measure.org/resource/om-2/mil-Angle">
	<rdfs:isDefinedBy rdf:resource="http://www.ontology-of-units-of-measure.org/resource/om-2/"/>
</rdf:Description>

<rdf:Description rdf:about="http://www.ontology-of-units-of-measure.org/resource/om-2/radian">
	<rdfs:isDefinedBy rdf:resource="http://www.ontology-of-units-of-measure.org/resource/om-2/"/>
</rdf:Description>

<rdf:Description rdf:about="http://www.ontology-of-units-of-measure.org/resource/om-2/minute-Angle">
	<rdf:type rdf:resource="http://www.w3.org/2004/02/skos/core#Concept"/>
	<skos:inScheme rdf:resource="http://www.ontology-of-units-of-measure.org/resource/om-2/SingularUnit"/>
	<rdfs:comment xml:lang="en">The minute (angle) is a unit of angle defined as 2.908882e-4 radian.</rdfs:comment>
	<rdfs:label xml:lang="en">minute (angle)</rdfs:label>
	<hasUnit xmlns="http://www.ontology-of-units-of-measure.org/resource/om-2/" rdf:resource="http://www.ontology-of-units-of-measure.org/resource/om-2/radian"/>
	<rdfs:isDefinedBy rdf:resource="http://www.ontology-of-units-of-measure.org/resource/om-2/"/>
</rdf:Description>

<rdf:Description rdf:about="http://www.ontology-of-units-of-measure.org/resource/om-2/revolution">
	<rdf:type rdf:resource="http://www.w3.org/2004/02/skos/core#Concept"/>
	<skos:inScheme rdf:resource="http://www.ontology-of-units-of-measure.org/resource/om-2/SingularUnit"/>
	<rdfs:comment xml:lang="en">The revolution is a unit of angle defined as 6.283185 radian.</rdfs:comment>
	<rdfs:label xml:lang="en">revolution</rdfs:label>
	<hasUnit xmlns="http://www.ontology-of-units-of-measure.org/resource/om-2/" rdf:resource="http://www.ontology-of-units-of-measure.org/resource/om-2/radian"/>
	<rdfs:isDefinedBy rdf:resource="http://www.ontology-of-units-of-measure.org/resource/om-2/"/>
</rdf:Description>

<rdf:Description rdf:about="http://www.ontology-of-units-of-measure.org/resource/om-2/second-Angle">
	<rdf:type rdf:resource="http://www.w3.org/2004/02/skos/core#Concept"/>
	<skos:inScheme rdf:resource="http://www.ontology-of-units-of-measure.org/resource/om-2/SingularUnit"/>
	<rdfs:comment xml:lang="en">The second (angle) is a unit of angle defined as 4.848137e-6 radian.</rdfs:comment>
	<rdfs:label xml:lang="en">second (angle)</rdfs:label>
	<hasUnit xmlns="http://www.ontology-of-units-of-measure.org/resource/om-2/" rdf:resource="http://www.ontology-of-units-of-measure.org/resource/om-2/radian"/>
	<rdfs:isDefinedBy rdf:resource="http://www.ontology-of-units-of-measure.org/resource/om-2/"/>
</rdf:Description>

<rdf:Description rdf:about="http://www.ontology-of-units-of-measure.org/resource/om-2/footcandle">
	<rdf:type rdf:resource="http://www.w3.org/2004/02/skos/core#Concept"/>
	<skos:inScheme rdf:resource="http://www.ontology-of-units-of-measure.org/resource/om-2/SingularUnit"/>
	<rdfs:comment xml:lang="en">The footcandle is a unit of illuminance defined as 1.076391e1 lux.</rdfs:comment>
	<rdfs:label xml:lang="en">footcandle</rdfs:label>
	<hasUnit xmlns="http://www.ontology-of-units-of-measure.org/resource/om-2/" rdf:resource="http://www.ontology-of-units-of-measure.org/resource/om-2/lux"/>
</rdf:Description>

<rdf:Description rdf:about="http://www.ontology-of-units-of-measure.org/resource/om-2/lux">
	<rdf:type rdf:resource="http://www.w3.org/2004/02/skos/core#Concept"/>
</rdf:Description>

<rdf:Description rdf:about="http://www.ontology-of-units-of-measure.org/resource/om-2/footcandle">
	<rdfs:isDefinedBy rdf:resource="http://www.ontology-of-units-of-measure.org/resource/om-2/"/>
</rdf:Description>

<rdf:Description rdf:about="http://www.ontology-of-units-of-measure.org/resource/om-2/lux">
	<rdfs:isDefinedBy rdf:resource="http://www.ontology-of-units-of-measure.org/resource/om-2/"/>
</rdf:Description>

<rdf:Description rdf:about="http://www.ontology-of-units-of-measure.org/resource/om-2/astronomicalUnit">
	<rdf:type rdf:resource="http://www.w3.org/2004/02/skos/core#Concept"/>
	<skos:inScheme rdf:resource="http://www.ontology-of-units-of-measure.org/resource/om-2/SingularUnit"/>
	<rdfs:comment xml:lang="en">The atronomical unit is a unit of length defined as 149 597 870 700 metre (IAU 2012 Resolution).</rdfs:comment>
	<rdfs:label xml:lang="en">astronomical unit</rdfs:label>
	<hasUnit xmlns="http://www.ontology-of-units-of-measure.org/resource/om-2/" rdf:resource="http://www.ontology-of-units-of-measure.org/resource/om-2/metre"/>
</rdf:Description>

<rdf:Description rdf:about="http://www.ontology-of-units-of-measure.org/resource/om-2/metre">
	<rdf:type rdf:resource="http://www.w3.org/2004/02/skos/core#Concept"/>
</rdf:Description>

<rdf:Description rdf:about="http://www.ontology-of-units-of-measure.org/resource/om-2/astronomicalUnit">
	<rdfs:isDefinedBy rdf:resource="http://www.ontology-of-units-of-measure.org/resource/om-2/"/>
</rdf:Description>

<rdf:Description rdf:about="http://www.ontology-of-units-of-measure.org/resource/om-2/metre">
	<rdfs:isDefinedBy rdf:resource="http://www.ontology-of-units-of-measure.org/resource/om-2/"/>
</rdf:Description>

<rdf:Description rdf:about="http://www.ontology-of-units-of-measure.org/resource/om-2/chain">
	<rdf:type rdf:resource="http://www.w3.org/2004/02/skos/core#Concept"/>
	<skos:inScheme rdf:resource="http://www.ontology-of-units-of-measure.org/resource/om-2/SingularUnit"/>
	<rdfs:comment xml:lang="en">The chain is a unit of length defined as 2.011684e1 metre.</rdfs:comment>
	<rdfs:label xml:lang="en">chain</rdfs:label>
	<hasUnit xmlns="http://www.ontology-of-units-of-measure.org/resource/om-2/" rdf:resource="http://www.ontology-of-units-of-measure.org/resource/om-2/metre"/>
	<rdfs:isDefinedBy rdf:resource="http://www.ontology-of-units-of-measure.org/resource/om-2/"/>
</rdf:Description>

<rdf:Description rdf:about="http://www.ontology-of-units-of-measure.org/resource/om-2/fathom-USSurvey">
	<rdf:type rdf:resource="http://www.w3.org/2004/02/skos/core#Concept"/>
	<skos:inScheme rdf:resource="http://www.ontology-of-units-of-measure.org/resource/om-2/SingularUnit"/>
	<rdfs:comment xml:lang="en">The US survey fathom is a unit of length defined as 1.828804 metre.</rdfs:comment>
	<rdfs:label xml:lang="en">fathom (US survey)</rdfs:label>
	<hasUnit xmlns="http://www.ontology-of-units-of-measure.org/resource/om-2/" rdf:resource="http://www.ontology-of-units-of-measure.org/resource/om-2/metre"/>
	<rdfs:isDefinedBy rdf:resource="http://www.ontology-of-units-of-measure.org/resource/om-2/"/>
</rdf:Description>

<rdf:Description rdf:about="http://www.ontology-of-units-of-measure.org/resource/om-2/fermi">
	<rdf:type rdf:resource="http://www.w3.org/2004/02/skos/core#Concept"/>
	<skos:inScheme rdf:resource="http://www.ontology-of-units-of-measure.org/resource/om-2/SingularUnit"/>
	<rdfs:comment xml:lang="en">The fermi is a unit of length defined as 1.0e-15 metre.</rdfs:comment>
	<rdfs:label xml:lang="en">fermi</rdfs:label>
	<hasUnit xmlns="http://www.ontology-of-units-of-measure.org/resource/om-2/" rdf:resource="http://www.ontology-of-units-of-measure.org/resource/om-2/metre"/>
	<rdfs:isDefinedBy rdf:resource="http://www.ontology-of-units-of-measure.org/resource/om-2/"/>
</rdf:Description>

<rdf:Description rdf:about="http://www.ontology-of-units-of-measure.org/resource/om-2/foot-International">
	<rdf:type rdf:resource="http://www.w3.org/2004/02/skos/core#Concept"/>
	<skos:inScheme rdf:resource="http://www.ontology-of-units-of-measure.org/resource/om-2/SingularUnit"/>
	<rdfs:comment xml:lang="en">The international foot is a unit of length defined as 3.048e-1 metre.</rdfs:comment>
	<rdfs:label xml:lang="en">foot (international)</rdfs:label>
	<hasUnit xmlns="http://www.ontology-of-units-of-measure.org/resource/om-2/" rdf:resource="http://www.ontology-of-units-of-measure.org/resource/om-2/metre"/>
	<rdfs:isDefinedBy rdf:resource="http://www.ontology-of-units-of-measure.org/resource/om-2/"/>
</rdf:Description>

<rdf:Description rdf:about="http://www.ontology-of-units-of-measure.org/resource/om-2/foot-USSurvey">
	<rdf:type rdf:resource="http://www.w3.org/2004/02/skos/core#Concept"/>
	<skos:inScheme rdf:resource="http://www.ontology-of-units-of-measure.org/resource/om-2/SingularUnit"/>
	<rdfs:comment xml:lang="en">The US survey foot is a unit of length defined as 3.048006e-1 metre.</rdfs:comment>
	<rdfs:label xml:lang="en">foot (US survey)</rdfs:label>
	<hasUnit xmlns="http://www.ontology-of-units-of-measure.org/resource/om-2/" rdf:resource="http://www.ontology-of-units-of-measure.org/resource/om-2/metre"/>
	<rdfs:isDefinedBy rdf:resource="http://www.ontology-of-units-of-measure.org/resource/om-2/"/>
</rdf:Description>

<rdf:Description rdf:about="http://www.ontology-of-units-of-measure.org/resource/om-2/furlong-International">
	<rdf:type rdf:resource="http://www.w3.org/2004/02/skos/core#Concept"/>
	<skos:inScheme rdf:resource="http://www.ontology-of-units-of-measure.org/resource/om-2/SingularUnit"/>
	<rdfs:comment xml:lang="en">The international furlong is a unit of length defined as 201.168 metre.</rdfs:comment>
	<rdfs:label xml:lang="en">furlong (international)</rdfs:label>
	<hasUnit xmlns="http://www.ontology-of-units-of-measure.org/resource/om-2/" rdf:resource="http://www.ontology-of-units-of-measure.org/resource/om-2/metre"/>
	<rdfs:isDefinedBy rdf:resource="http://www.ontology-of-units-of-measure.org/resource/om-2/"/>
</rdf:Description>

<rdf:Description rdf:about="http://www.ontology-of-units-of-measure.org/resource/om-2/inch-International">
	<skos:inScheme rdf:resource="http://www.ontology-of-units-of-measure.org/resource/om-2/SingularUnit"/>
	<rdfs:comment xml:lang="en">The international inch is a unit of length defined as 2.54e-2 metre.</rdfs:comment>
	<rdfs:label xml:lang="en">inch (international)</rdfs:label>
	<hasUnit xmlns="http://www.ontology-of-units-of-measure.org/resource/om-2/" rdf:resource="http://www.ontology-of-units-of-measure.org/resource/om-2/metre"/>
</rdf:Description>

<rdf:Description rdf:about="http://www.ontology-of-units-of-measure.org/resource/om-2/teaspoon-US">
	<rdf:type rdf:resource="http://www.w3.org/2004/02/skos/core#Concept"/>
	<skos:inScheme rdf:resource="http://www.ontology-of-units-of-measure.org/resource/om-2/SingularUnit"/>
	<rdfs:comment xml:lang="en">The US teaspoon is a unit of volume defined as 4.928922e-6 cubic metre.</rdfs:comment>
	<rdfs:label xml:lang="en">teaspoon (US)</rdfs:label>
	<rdfs:isDefinedBy rdf:resource="http://www.ontology-of-units-of-measure.org/resource/om-2/"/>
</rdf:Description>

<rdf:Description rdf:about="http://www.ontology-of-units-of-measure.org/resource/om-2/tesla">
	<rdf:type rdf:resource="http://www.w3.org/2004/02/skos/core#Concept"/>
	<skos:inScheme rdf:resource="http://www.ontology-of-units-of-measure.org/resource/om-2/SingularUnit"/>
	<rdfs:comment xml:lang="en">The tesla is a unit of magnetic flux density defined as volt times second divided by square metre = newton divided by ampere times metre = weber divided by square metre = kilogram divided by coulomb times second = kilogram divided by ampere times second squared.</rdfs:comment>
	<rdfs:label xml:lang="en">tesla</rdfs:label>
	<rdfs:isDefinedBy rdf:resource="http://www.ontology-of-units-of-measure.org/resource/om-2/"/>
</rdf:Description>

<rdf:Description rdf:about="http://www.ontology-of-units-of-measure.org/resource/om-2/ton-Long">
	<rdf:type rdf:resource="http://www.w3.org/2004/02/skos/core#Concept"/>
	<skos:inScheme rdf:resource="http://www.ontology-of-units-of-measure.org/resource/om-2/SingularUnit"/>
	<rdfs:comment xml:lang="en">The long ton is a unit of mass defined as 1.016047e3 kilogram.</rdfs:comment>
	<rdfs:label xml:lang="en">ton (long)</rdfs:label>
	<rdfs:isDefinedBy rdf:resource="http://www.ontology-of-units-of-measure.org/resource/om-2/"/>
</rdf:Description>

<rdf:Description rdf:about="http://www.ontology-of-units-of-measure.org/resource/om-2/ton-Register">
	<rdf:type rdf:resource="http://www.w3.org/2004/02/skos/core#Concept"/>
	<skos:inScheme rdf:resource="http://www.ontology-of-units-of-measure.org/resource/om-2/SingularUnit"/>
	<rdfs:comment xml:lang="en">The register ton is a unit of volume defined as 2.831658 cubic metre.</rdfs:comment>
	<rdfs:label xml:lang="en">ton (register)</rdfs:label>
	<rdfs:isDefinedBy rdf:resource="http://www.ontology-of-units-of-measure.org/resource/om-2/"/>
</rdf:Description>

<rdf:Description rdf:about="http://www.ontology-of-units-of-measure.org/resource/om-2/ton-Short">
	<rdf:type rdf:resource="http://www.w3.org/2004/02/skos/core#Concept"/>
	<skos:inScheme rdf:resource="http://www.ontology-of-units-of-measure.org/resource/om-2/SingularUnit"/>
	<rdfs:comment xml:lang="en">The short ton is a unit of mass defined as 9.071847e2 kilogram.</rdfs:comment>
	<rdfs:label xml:lang="en">ton (short)</rdfs:label>
	<rdfs:isDefinedBy rdf:resource="http://www.ontology-of-units-of-measure.org/resource/om-2/"/>
</rdf:Description>

<rdf:Description rdf:about="http://www.ontology-of-units-of-measure.org/resource/om-2/ton-ShortAssay">
	<rdf:type rdf:resource="http://www.w3.org/2004/02/skos/core#Concept"/>
	<skos:inScheme rdf:resource="http://www.ontology-of-units-of-measure.org/resource/om-2/SingularUnit"/>
	<rdfs:comment xml:lang="en">The short assay ton is a unit of mass defined as 2.916667e-2 kilogram.</rdfs:comment>
	<rdfs:label xml:lang="en">ton (short assay)</rdfs:label>
	<rdfs:isDefinedBy rdf:resource="http://www.ontology-of-units-of-measure.org/resource/om-2/"/>
</rdf:Description>

<rdf:Description rdf:about="http://www.ontology-of-units-of-measure.org/resource/om-2/tonne">
	<rdf:type rdf:resource="http://www.w3.org/2004/02/skos/core#Concept"/>
	<skos:inScheme rdf:resource="http://www.ontology-of-units-of-measure.org/resource/om-2/SingularUnit"/>
	<rdfs:comment xml:lang="en">The tonne is a unit of mass defined as 1000 kilogram.</rdfs:comment>
	<rdfs:label xml:lang="en">tonne</rdfs:label>
	<rdfs:isDefinedBy rdf:resource="http://www.ontology-of-units-of-measure.org/resource/om-2/"/>
</rdf:Description>

<rdf:Description rdf:about="http://www.ontology-of-units-of-measure.org/resource/om-2/unifiedAtomicMassUnit">
	<rdf:type rdf:resource="http://www.w3.org/2004/02/skos/core#Concept"/>
	<skos:inScheme rdf:resource="http://www.ontology-of-units-of-measure.org/resource/om-2/SingularUnit"/>
	<rdfs:comment xml:lang="en">The unified atomic mass unit is a unit of mass defined as 1.660538782(83)e-27 kilogram.</rdfs:comment>
	<rdfs:label xml:lang="en">unified atomic mass unit</rdfs:label>
	<rdfs:isDefinedBy rdf:resource="http://www.ontology-of-units-of-measure.org/resource/om-2/"/>
</rdf:Description>

<rdf:Description rdf:about="http://www.ontology-of-units-of-measure.org/resource/om-2/volt">
	<rdf:type rdf:resource="http://www.w3.org/2004/02/skos/core#Concept"/>
	<skos:inScheme rdf:resource="http://www.ontology-of-units-of-measure.org/resource/om-2/SingularUnit"/>
	<rdfs:comment xml:lang="en">The volt is a unit of electric potential defined as watt divided by ampere = joule divided by coulomb = newton times metre divided by ampere times second = kilogram times square metre divided by ampere times second to the power 3.</rdfs:comment>
	<rdfs:label xml:lang="en">volt</rdfs:label>
	<rdfs:isDefinedBy rdf:resource="http://www.ontology-of-units-of-measure.org/resource/om-2/"/>
</rdf:Description>

<rdf:Description rdf:about="http://www.ontology-of-units-of-measure.org/resource/om-2/watt">
	<rdf:type rdf:resource="http://www.w3.org/2004/02/skos/core#Concept"/>
	<skos:inScheme rdf:resource="http://www.ontology-of-units-of-measure.org/resource/om-2/SingularUnit"/>
	<rdfs:comment xml:lang="en">The watt is a unit of power defined as joule divided by second = newton times metre divided by second = volt times ampere = kilogram times square metre divided by second to the power 3.</rdfs:comment>
	<rdfs:label xml:lang="en">watt</rdfs:label>
	<rdfs:isDefinedBy rdf:resource="http://www.ontology-of-units-of-measure.org/resource/om-2/"/>
</rdf:Description>

<rdf:Description rdf:about="http://www.ontology-of-units-of-measure.org/resource/om-2/weber">
	<rdf:type rdf:resource="http://www.w3.org/2004/02/skos/core#Concept"/>
	<skos:inScheme rdf:resource="http://www.ontology-of-units-of-measure.org/resource/om-2/SingularUnit"/>
	<rdfs:comment xml:lang="en">The weber is a unit of magnetic flux defined as kilogram times square metre divided by second squared times ampere = volt times second = joule divided by ampere.</rdfs:comment>
	<rdfs:label xml:lang="en">weber</rdfs:label>
	<rdfs:isDefinedBy rdf:resource="http://www.ontology-of-units-of-measure.org/resource/om-2/"/>
</rdf:Description>

<rdf:Description rdf:about="http://www.ontology-of-units-of-measure.org/resource/om-2/acre-International">
	<rdf:type rdf:resource="http://www.w3.org/2004/02/skos/core#Concept"/>
	<skos:inScheme rdf:resource="http://www.ontology-of-units-of-measure.org/resource/om-2/SingularUnit"/>
	<rdfs:comment xml:lang="en">The international acre is a unit of area defined as 4.0468564224e3 square metre.</rdfs:comment>
	<rdfs:label xml:lang="en">acre (international)</rdfs:label>
	<rdfs:isDefinedBy rdf:resource="http://www.ontology-of-units-of-measure.org/resource/om-2/"/>
</rdf:Description>

<rdf:Description rdf:about="http://www.ontology-of-units-of-measure.org/resource/om-2/acre-USSurvey">
	<rdf:type rdf:resource="http://www.w3.org/2004/02/skos/core#Concept"/>
	<skos:inScheme rdf:resource="http://www.ontology-of-units-of-measure.org/resource/om-2/SingularUnit"/>
	<rdfs:comment xml:lang="en">The US survey acre is a unit of area defined as 4.046872609874252e3 square metre.</rdfs:comment>
	<rdfs:label xml:lang="en">acre (US survey)</rdfs:label>
	<rdfs:isDefinedBy rdf:resource="http://www.ontology-of-units-of-measure.org/resource/om-2/"/>
</rdf:Description>

<rdf:Description rdf:about="http://www.ontology-of-units-of-measure.org/resource/om-2/acreFoot">
	<rdf:type rdf:resource="http://www.w3.org/2004/02/skos/core#Concept"/>
	<skos:inScheme rdf:resource="http://www.ontology-of-units-of-measure.org/resource/om-2/SingularUnit"/>
	<rdfs:comment xml:lang="en">The acre foot is a unit of volume defined as 1.233489e3 cubic metre.</rdfs:comment>
	<rdfs:label xml:lang="en">acre foot</rdfs:label>
	<rdfs:isDefinedBy rdf:resource="http://www.ontology-of-units-of-measure.org/resource/om-2/"/>
</rdf:Description>

<rdf:Description rdf:about="http://www.ontology-of-units-of-measure.org/resource/om-2/ampere">
	<skos:inScheme rdf:resource="http://www.ontology-of-units-of-measure.org/resource/om-2/SingularUnit"/>
	<rdfs:comment xml:lang="en">The ampere is a unit of electric current defined as the constant current that produces an attractive force of 2e–7 newton per metre of length between two straight, parallel conductors of infinite length and negligible circular cross section placed one metre apart in a vacuum.</rdfs:comment>
	<rdfs:label xml:lang="en">ampere</rdfs:label>
</rdf:Description>

<rdf:Description rdf:about="http://www.ontology-of-units-of-measure.org/resource/om-2/amylaseUnit">
	<rdf:type rdf:resource="http://www.w3.org/2004/02/skos/core#Concept"/>
	<skos:inScheme rdf:resource="http://www.ontology-of-units-of-measure.org/resource/om-2/SingularUnit"/>
	<rdfs:comment xml:lang="en">The amylase unit is a unit of catalytic activity.</rdfs:comment>
	<rdfs:label xml:lang="en">amylase unit</rdfs:label>
	<rdfs:isDefinedBy rdf:resource="http://www.ontology-of-units-of-measure.org/resource/om-2/"/>
</rdf:Description>

<rdf:Description rdf:about="http://www.ontology-of-units-of-measure.org/resource/om-2/are">
	<rdf:type rdf:resource="http://www.w3.org/2004/02/skos/core#Concept"/>
	<skos:inScheme rdf:resource="http://www.ontology-of-units-of-measure.org/resource/om-2/SingularUnit"/>
	<rdfs:comment xml:lang="en">The are is a unit of area defined as 100 square metre.</rdfs:comment>
	<rdfs:label xml:lang="en">are</rdfs:label>
	<rdfs:isDefinedBy rdf:resource="http://www.ontology-of-units-of-measure.org/resource/om-2/"/>
</rdf:Description>

<rdf:Description rdf:about="http://www.ontology-of-units-of-measure.org/resource/om-2/barn">
	<rdf:type rdf:resource="http://www.w3.org/2004/02/skos/core#Concept"/>
	<skos:inScheme rdf:resource="http://www.ontology-of-units-of-measure.org/resource/om-2/SingularUnit"/>
	<rdfs:comment xml:lang="en">The barn is a unit of area defined as 1.0e-28 square metre.</rdfs:comment>
	<rdfs:label xml:lang="en">barn</rdfs:label>
	<rdfs:isDefinedBy rdf:resource="http://www.ontology-of-units-of-measure.org/resource/om-2/"/>
</rdf:Description>

<rdf:Description rdf:about="http://www.ontology-of-units-of-measure.org/resource/om-2/barrel-US">
	<rdf:type rdf:resource="http://www.w3.org/2004/02/skos/core#Concept"/>
	<skos:inScheme rdf:resource="http://www.ontology-of-units-of-measure.org/resource/om-2/SingularUnit"/>
	<rdfs:comment xml:lang="en">The US barrel is a unit of volume defined as 1.589873e-1 cubic metre.</rdfs:comment>
	<rdfs:label xml:lang="en">barrel (US)</rdfs:label>
	<rdfs:isDefinedBy rdf:resource="http://www.ontology-of-units-of-measure.org/resource/om-2/"/>
</rdf:Description>

<rdf:Description rdf:about="http://www.ontology-of-units-of-measure.org/resource/om-2/baud">
	<rdf:type rdf:resource="http://www.w3.org/2004/02/skos/core#Concept"/>
	<skos:inScheme rdf:resource="http://www.ontology-of-units-of-measure.org/resource/om-2/SingularUnit"/>
	<rdfs:comment xml:lang="en">The baud is a unit of symbol rate defined as one distinct symbol change or signalling event made to the transmission medium per second in a digitally modulated signal or a line code.</rdfs:comment>
	<rdfs:label xml:lang="en">baud</rdfs:label>
	<rdfs:isDefinedBy rdf:resource="http://www.ontology-of-units-of-measure.org/resource/om-2/"/>
</rdf:Description>

<rdf:Description rdf:about="http://www.ontology-of-units-of-measure.org/resource/om-2/becquerel">
	<skos:inScheme rdf:resource="http://www.ontology-of-units-of-measure.org/resource/om-2/SingularUnit"/>
	<rdfs:comment xml:lang="en">The becquerel is a unit of activity defined as the activity of a quantity of radioactive material in which one nucleus decays per second. Algebraically it is defined as 1 divided by second.</rdfs:comment>
	<rdfs:label xml:lang="en">becquerel</rdfs:label>
</rdf:Description>

<rdf:Description rdf:about="http://www.ontology-of-units-of-measure.org/resource/om-2/bit">
	<skos:inScheme rdf:resource="http://www.ontology-of-units-of-measure.org/resource/om-2/SingularUnit"/>
	<rdfs:comment xml:lang="en">The bit is a unit of information capacity defined as the information capacity of one binary digit.</rdfs:comment>
	<rdfs:label xml:lang="en">bit</rdfs:label>
</rdf:Description>

<rdf:Description rdf:about="http://www.ontology-of-units-of-measure.org/resource/om-2/bushel-US">
	<rdf:type rdf:resource="http://www.w3.org/2004/02/skos/core#Concept"/>
	<skos:inScheme rdf:resource="http://www.ontology-of-units-of-measure.org/resource/om-2/SingularUnit"/>
	<rdfs:comment xml:lang="en">The US bushel is a unit of volume defined as 3.523907e-2 cubic metre.</rdfs:comment>
	<rdfs:label xml:lang="en">bushel (US)</rdfs:label>
	<rdfs:isDefinedBy rdf:resource="http://www.ontology-of-units-of-measure.org/resource/om-2/"/>
</rdf:Description>

<rdf:Description rdf:about="http://www.ontology-of-units-of-measure.org/resource/om-2/candela">
	<rdf:type rdf:resource="http://www.w3.org/2004/02/skos/core#Concept"/>
	<skos:inScheme rdf:resource="http://www.ontology-of-units-of-measure.org/resource/om-2/SingularUnit"/>
	<rdfs:comment xml:lang="en">The candela is a unit of luminous intensity defined as the luminous intensity, in a given direction, of a source that emits monochromatic radiation of frequency 540e12 hertz and that has a radiant intensity in that direction of 1/683 watt per steradian.</rdfs:comment>
	<rdfs:label xml:lang="en">candela</rdfs:label>
	<rdfs:isDefinedBy rdf:resource="http://www.ontology-of-units-of-measure.org/resource/om-2/"/>
</rdf:Description>

<rdf:Description rdf:about="http://www.ontology-of-units-of-measure.org/resource/om-2/carat-Mass">
	<rdf:type rdf:resource="http://www.w3.org/2004/02/skos/core#Concept"/>
	<skos:inScheme rdf:resource="http://www.ontology-of-units-of-measure.org/resource/om-2/SingularUnit"/>
	<rdfs:comment xml:lang="en">The carat (mass) is a unit of mass defined as 2.0e-4 kilogram.</rdfs:comment>
	<rdfs:label xml:lang="en">carat (mass)</rdfs:label>
	<rdfs:isDefinedBy rdf:resource="http://www.ontology-of-units-of-measure.org/resource/om-2/"/>
</rdf:Description>

<rdf:Description rdf:about="http://www.ontology-of-units-of-measure.org/resource/om-2/cicero">
	<rdf:type rdf:resource="http://www.w3.org/2004/02/skos/core#Concept"/>
	<skos:inScheme rdf:resource="http://www.ontology-of-units-of-measure.org/resource/om-2/SingularUnit"/>
	<rdfs:comment xml:lang="en">The cicero is a unit of length defined as 12 point (Didot).</rdfs:comment>
	<rdfs:label xml:lang="en">cicero</rdfs:label>
	<hasUnit xmlns="http://www.ontology-of-units-of-measure.org/resource/om-2/" rdf:resource="http://www.ontology-of-units-of-measure.org/resource/om-2/point-Didot"/>
</rdf:Description>

<rdf:Description rdf:about="http://www.ontology-of-units-of-measure.org/resource/om-2/point-Didot">
	<rdf:type rdf:resource="http://www.w3.org/2004/02/skos/core#Concept"/>
</rdf:Description>

<rdf:Description rdf:about="http://www.ontology-of-units-of-measure.org/resource/om-2/cicero">
	<rdfs:isDefinedBy rdf:resource="http://www.ontology-of-units-of-measure.org/resource/om-2/"/>
</rdf:Description>

<rdf:Description rdf:about="http://www.ontology-of-units-of-measure.org/resource/om-2/point-Didot">
	<rdfs:isDefinedBy rdf:resource="http://www.ontology-of-units-of-measure.org/resource/om-2/"/>
</rdf:Description>

<rdf:Description rdf:about="http://www.ontology-of-units-of-measure.org/resource/om-2/degree">
	<skos:inScheme rdf:resource="http://www.ontology-of-units-of-measure.org/resource/om-2/SingularUnit"/>
	<rdfs:comment xml:lang="en">The degree is a unit of angle defined as 1.745329e-2 radian.</rdfs:comment>
	<rdfs:label xml:lang="en">degree</rdfs:label>
	<hasUnit xmlns="http://www.ontology-of-units-of-measure.org/resource/om-2/" rdf:resource="http://www.ontology-of-units-of-measure.org/resource/om-2/radian"/>
</rdf:Description>

<rdf:Description rdf:about="http://www.ontology-of-units-of-measure.org/resource/om-2/gon">
	<rdf:type rdf:resource="http://www.w3.org/2004/02/skos/core#Concept"/>
	<skos:inScheme rdf:resource="http://www.ontology-of-units-of-measure.org/resource/om-2/SingularUnit"/>
	<rdfs:comment xml:lang="en">The gon is a unit of angle defined as 1.570796e-2 radian.</rdfs:comment>
	<rdfs:label xml:lang="en">gon</rdfs:label>
	<hasUnit xmlns="http://www.ontology-of-units-of-measure.org/resource/om-2/" rdf:resource="http://www.ontology-of-units-of-measure.org/resource/om-2/radian"/>
	<rdfs:isDefinedBy rdf:resource="http://www.ontology-of-units-of-measure.org/resource/om-2/"/>
</rdf:Description>

<rdf:Description rdf:about="http://www.ontology-of-units-of-measure.org/resource/om-2/horsepower-Boiler">
	<rdf:type rdf:resource="http://www.w3.org/2004/02/skos/core#Concept"/>
	<skos:inScheme rdf:resource="http://www.ontology-of-units-of-measure.org/resource/om-2/SingularUnit"/>
	<rdfs:comment xml:lang="en">The boiler horsepower is a unit of power defined as 9.80950e3 watt.</rdfs:comment>
	<rdfs:label xml:lang="en">horsepower (boiler)</rdfs:label>
	<hasUnit xmlns="http://www.ontology-of-units-of-measure.org/resource/om-2/" rdf:resource="http://www.ontology-of-units-of-measure.org/resource/om-2/watt"/>
	<rdfs:isDefinedBy rdf:resource="http://www.ontology-of-units-of-measure.org/resource/om-2/"/>
</rdf:Description>

<rdf:Description rdf:about="http://www.ontology-of-units-of-measure.org/resource/om-2/horsepower-British">
	<rdf:type rdf:resource="http://www.w3.org/2004/02/skos/core#Concept"/>
	<skos:inScheme rdf:resource="http://www.ontology-of-units-of-measure.org/resource/om-2/SingularUnit"/>
	<rdfs:comment xml:lang="en">The British horsepower is a unit of power defined as 7.4570e2 watt.</rdfs:comment>
	<rdfs:label xml:lang="en">horsepower (British)</rdfs:label>
	<hasUnit xmlns="http://www.ontology-of-units-of-measure.org/resource/om-2/" rdf:resource="http://www.ontology-of-units-of-measure.org/resource/om-2/watt"/>
	<rdfs:isDefinedBy rdf:resource="http://www.ontology-of-units-of-measure.org/resource/om-2/"/>
</rdf:Description>

<rdf:Description rdf:about="http://www.ontology-of-units-of-measure.org/resource/om-2/horsepower-Electric">
	<rdf:type rdf:resource="http://www.w3.org/2004/02/skos/core#Concept"/>
	<skos:inScheme rdf:resource="http://www.ontology-of-units-of-measure.org/resource/om-2/SingularUnit"/>
	<rdfs:comment xml:lang="en">The electric horsepower is a unit of power defined as 7.46e2 watt.</rdfs:comment>
	<rdfs:label xml:lang="en">horsepower (electric)</rdfs:label>
	<hasUnit xmlns="http://www.ontology-of-units-of-measure.org/resource/om-2/" rdf:resource="http://www.ontology-of-units-of-measure.org/resource/om-2/watt"/>
	<rdfs:isDefinedBy rdf:resource="http://www.ontology-of-units-of-measure.org/resource/om-2/"/>
</rdf:Description>

<rdf:Description rdf:about="http://www.ontology-of-units-of-measure.org/resource/om-2/tonOfRefrigeration">
	<rdf:type rdf:resource="http://www.w3.org/2004/02/skos/core#Concept"/>
	<skos:inScheme rdf:resource="http://www.ontology-of-units-of-measure.org/resource/om-2/SingularUnit"/>
	<rdfs:comment xml:lang="en">The ton of refrigeration is a unit of power defined as 3.516853e3 watt.</rdfs:comment>
	<rdfs:label xml:lang="en">ton of refrigeration</rdfs:label>
	<hasUnit xmlns="http://www.ontology-of-units-of-measure.org/resource/om-2/" rdf:resource="http://www.ontology-of-units-of-measure.org/resource/om-2/watt"/>
	<rdfs:isDefinedBy rdf:resource="http://www.ontology-of-units-of-measure.org/resource/om-2/"/>
</rdf:Description>

<rdf:Description rdf:about="http://www.ontology-of-units-of-measure.org/resource/om-2/stattesla">
	<rdf:type rdf:resource="http://www.w3.org/2004/02/skos/core#Concept"/>
	<skos:inScheme rdf:resource="http://www.ontology-of-units-of-measure.org/resource/om-2/SingularUnit"/>
	<rdfs:comment xml:lang="en">The stattesla is a unit of magnetic flux density defined as 2.9979e6 tesla.</rdfs:comment>
	<rdfs:label xml:lang="en">stattesla</rdfs:label>
	<hasUnit xmlns="http://www.ontology-of-units-of-measure.org/resource/om-2/" rdf:resource="http://www.ontology-of-units-of-measure.org/resource/om-2/tesla"/>
	<rdfs:isDefinedBy rdf:resource="http://www.ontology-of-units-of-measure.org/resource/om-2/"/>
</rdf:Description>

<rdf:Description rdf:about="http://www.ontology-of-units-of-measure.org/resource/om-2/maxwell">
	<rdf:type rdf:resource="http://www.w3.org/2004/02/skos/core#Concept"/>
	<skos:inScheme rdf:resource="http://www.ontology-of-units-of-measure.org/resource/om-2/SingularUnit"/>
	<rdfs:comment xml:lang="en">The maxwell is a unit of magnetic flux defined as 1.0e-8 weber.</rdfs:comment>
	<rdfs:label xml:lang="en">maxwell</rdfs:label>
	<hasUnit xmlns="http://www.ontology-of-units-of-measure.org/resource/om-2/" rdf:resource="http://www.ontology-of-units-of-measure.org/resource/om-2/weber"/>
	<rdfs:isDefinedBy rdf:resource="http://www.ontology-of-units-of-measure.org/resource/om-2/"/>
</rdf:Description>

<rdf:Description rdf:about="http://www.ontology-of-units-of-measure.org/resource/om-2/statweber">
	<rdf:type rdf:resource="http://www.w3.org/2004/02/skos/core#Concept"/>
	<skos:inScheme rdf:resource="http://www.ontology-of-units-of-measure.org/resource/om-2/SingularUnit"/>
	<rdfs:comment xml:lang="en">The statweber is a unit of magnetic flux defined as 2.9979e2 weber.</rdfs:comment>
	<rdfs:label xml:lang="en">statweber</rdfs:label>
	<hasUnit xmlns="http://www.ontology-of-units-of-measure.org/resource/om-2/" rdf:resource="http://www.ontology-of-units-of-measure.org/resource/om-2/weber"/>
	<rdfs:isDefinedBy rdf:resource="http://www.ontology-of-units-of-measure.org/resource/om-2/"/>
</rdf:Description>

<rdf:Description rdf:about="http://www.ontology-of-units-of-measure.org/resource/om-2/unitPole">
	<rdf:type rdf:resource="http://www.w3.org/2004/02/skos/core#Concept"/>
	<skos:inScheme rdf:resource="http://www.ontology-of-units-of-measure.org/resource/om-2/SingularUnit"/>
	<rdfs:comment xml:lang="en">The unit pole is a unit of magnetic flux defined as 1.256637e-7 weber.</rdfs:comment>
	<rdfs:label xml:lang="en">unit pole</rdfs:label>
	<hasUnit xmlns="http://www.ontology-of-units-of-measure.org/resource/om-2/" rdf:resource="http://www.ontology-of-units-of-measure.org/resource/om-2/weber"/>
	<rdfs:isDefinedBy rdf:resource="http://www.ontology-of-units-of-measure.org/resource/om-2/"/>
</rdf:Description>

<rdf:Description rdf:about="http://www.ontology-of-units-of-measure.org/resource/om-2/pica-ATA">
	<rdf:type rdf:resource="http://www.w3.org/2004/02/skos/core#Concept"/>
	<skos:inScheme rdf:resource="http://www.ontology-of-units-of-measure.org/resource/om-2/SingularUnit"/>
	<rdfs:comment xml:lang="en">The ATA pica is a unit of length defined as 12 point (ATA).</rdfs:comment>
	<rdfs:label xml:lang="en">pica (ATA)</rdfs:label>
	<hasUnit xmlns="http://www.ontology-of-units-of-measure.org/resource/om-2/" rdf:resource="http://www.ontology-of-units-of-measure.org/resource/om-2/point-ATA"/>
</rdf:Description>

<rdf:Description rdf:about="http://www.ontology-of-units-of-measure.org/resource/om-2/point-ATA">
	<rdf:type rdf:resource="http://www.w3.org/2004/02/skos/core#Concept"/>
</rdf:Description>

<rdf:Description rdf:about="http://www.ontology-of-units-of-measure.org/resource/om-2/pica-ATA">
	<rdfs:isDefinedBy rdf:resource="http://www.ontology-of-units-of-measure.org/resource/om-2/"/>
</rdf:Description>

<rdf:Description rdf:about="http://www.ontology-of-units-of-measure.org/resource/om-2/point-ATA">
	<rdfs:isDefinedBy rdf:resource="http://www.ontology-of-units-of-measure.org/resource/om-2/"/>
</rdf:Description>

<rdf:Description rdf:about="http://www.ontology-of-units-of-measure.org/resource/om-2/day">
	<rdf:type rdf:resource="http://www.w3.org/2004/02/skos/core#Concept"/>
	<skos:inScheme rdf:resource="http://www.ontology-of-units-of-measure.org/resource/om-2/SingularUnit"/>
	<rdfs:comment xml:lang="en">The day is a unit of time defined as 86400 second.</rdfs:comment>
	<rdfs:label xml:lang="en">day</rdfs:label>
	<hasUnit xmlns="http://www.ontology-of-units-of-measure.org/resource/om-2/" rdf:resource="http://www.ontology-of-units-of-measure.org/resource/om-2/second-Time"/>
</rdf:Description>

<rdf:Description rdf:about="http://www.ontology-of-units-of-measure.org/resource/om-2/second-Time">
	<rdf:type rdf:resource="http://www.w3.org/2004/02/skos/core#Concept"/>
</rdf:Description>

<rdf:Description rdf:about="http://www.ontology-of-units-of-measure.org/resource/om-2/day">
	<rdfs:isDefinedBy rdf:resource="http://www.ontology-of-units-of-measure.org/resource/om-2/"/>
</rdf:Description>

<rdf:Description rdf:about="http://www.ontology-of-units-of-measure.org/resource/om-2/second-Time">
	<rdfs:isDefinedBy rdf:resource="http://www.ontology-of-units-of-measure.org/resource/om-2/"/>
</rdf:Description>

<rdf:Description rdf:about="http://www.ontology-of-units-of-measure.org/resource/om-2/day-Sidereal">
	<rdf:type rdf:resource="http://www.w3.org/2004/02/skos/core#Concept"/>
	<skos:inScheme rdf:resource="http://www.ontology-of-units-of-measure.org/resource/om-2/SingularUnit"/>
	<rdfs:comment xml:lang="en">The sidereal day is a unit of time defined as 8.616409e4 second.</rdfs:comment>
	<rdfs:label xml:lang="en">day (sidereal)</rdfs:label>
	<hasUnit xmlns="http://www.ontology-of-units-of-measure.org/resource/om-2/" rdf:resource="http://www.ontology-of-units-of-measure.org/resource/om-2/second-Time"/>
	<rdfs:isDefinedBy rdf:resource="http://www.ontology-of-units-of-measure.org/resource/om-2/"/>
</rdf:Description>

<rdf:Description rdf:about="http://www.ontology-of-units-of-measure.org/resource/om-2/hour">
	<rdf:type rdf:resource="http://www.w3.org/2004/02/skos/core#Concept"/>
	<skos:inScheme rdf:resource="http://www.ontology-of-units-of-measure.org/resource/om-2/SingularUnit"/>
	<rdfs:comment xml:lang="en">The hour is a unit of time defined as 3600 second.</rdfs:comment>
	<rdfs:label xml:lang="en">hour</rdfs:label>
	<hasUnit xmlns="http://www.ontology-of-units-of-measure.org/resource/om-2/" rdf:resource="http://www.ontology-of-units-of-measure.org/resource/om-2/second-Time"/>
	<rdfs:isDefinedBy rdf:resource="http://www.ontology-of-units-of-measure.org/resource/om-2/"/>
</rdf:Description>

<rdf:Description rdf:about="http://www.ontology-of-units-of-measure.org/resource/om-2/pica-Postscript">
	<rdf:type rdf:resource="http://www.w3.org/2004/02/skos/core#Concept"/>
	<skos:inScheme rdf:resource="http://www.ontology-of-units-of-measure.org/resource/om-2/SingularUnit"/>
	<rdfs:comment xml:lang="en">The Postscript pica is a unit of length defined as 12 point (Postscript).</rdfs:comment>
	<rdfs:label xml:lang="en">pica (Postscript)</rdfs:label>
	<hasUnit xmlns="http://www.ontology-of-units-of-measure.org/resource/om-2/" rdf:resource="http://www.ontology-of-units-of-measure.org/resource/om-2/point-Postscript"/>
	<rdfs:isDefinedBy rdf:resource="http://www.ontology-of-units-of-measure.org/resource/om-2/"/>
</rdf:Description>

<rdf:Description rdf:about="http://www.ontology-of-units-of-measure.org/resource/om-2/pica-TeX">
	<rdf:type rdf:resource="http://www.w3.org/2004/02/skos/core#Concept"/>
	<skos:inScheme rdf:resource="http://www.ontology-of-units-of-measure.org/resource/om-2/SingularUnit"/>
	<rdfs:comment xml:lang="en">The TeX pica is a unit of length defined as 12 point (TeX).</rdfs:comment>
	<rdfs:label xml:lang="en">pica (TeX)</rdfs:label>
	<hasUnit xmlns="http://www.ontology-of-units-of-measure.org/resource/om-2/" rdf:resource="http://www.ontology-of-units-of-measure.org/resource/om-2/point-TeX"/>
	<rdfs:isDefinedBy rdf:resource="http://www.ontology-of-units-of-measure.org/resource/om-2/"/>
</rdf:Description>

<rdf:Description rdf:about="http://www.ontology-of-units-of-measure.org/resource/om-2/abvolt">
	<rdf:type rdf:resource="http://www.w3.org/2004/02/skos/core#Concept"/>
	<skos:inScheme rdf:resource="http://www.ontology-of-units-of-measure.org/resource/om-2/SingularUnit"/>
	<rdfs:comment xml:lang="en">The abvolt is a unit of electric potential defined as 1.0e-8 volt.</rdfs:comment>
	<rdfs:label xml:lang="en">abvolt</rdfs:label>
	<hasUnit xmlns="http://www.ontology-of-units-of-measure.org/resource/om-2/" rdf:resource="http://www.ontology-of-units-of-measure.org/resource/om-2/volt"/>
	<rdfs:isDefinedBy rdf:resource="http://www.ontology-of-units-of-measure.org/resource/om-2/"/>
</rdf:Description>

<rdf:Description rdf:about="http://www.ontology-of-units-of-measure.org/resource/om-2/statvolt">
	<rdf:type rdf:resource="http://www.w3.org/2004/02/skos/core#Concept"/>
	<skos:inScheme rdf:resource="http://www.ontology-of-units-of-measure.org/resource/om-2/SingularUnit"/>
	<rdfs:comment xml:lang="en">The statvolt is a unit of electric potential defined as 2.997925e2 volt.</rdfs:comment>
	<rdfs:label xml:lang="en">statvolt</rdfs:label>
	<hasUnit xmlns="http://www.ontology-of-units-of-measure.org/resource/om-2/" rdf:resource="http://www.ontology-of-units-of-measure.org/resource/om-2/volt"/>
	<rdfs:isDefinedBy rdf:resource="http://www.ontology-of-units-of-measure.org/resource/om-2/"/>
</rdf:Description>

<rdf:Description rdf:about="http://www.ontology-of-units-of-measure.org/resource/om-2/dessertspoon">
	<rdf:type rdf:resource="http://www.w3.org/2004/02/skos/core#Concept"/>
	<skos:inScheme rdf:resource="http://www.ontology-of-units-of-measure.org/resource/om-2/SingularUnit"/>
	<rdfs:comment xml:lang="en">The desserspoon is a unit of volume defined as 2 teaspoon.</rdfs:comment>
	<rdfs:label xml:lang="en">dessertspoon</rdfs:label>
	<hasUnit xmlns="http://www.ontology-of-units-of-measure.org/resource/om-2/" rdf:resource="http://www.ontology-of-units-of-measure.org/resource/om-2/teaspoon-US"/>
	<rdfs:isDefinedBy rdf:resource="http://www.ontology-of-units-of-measure.org/resource/om-2/"/>
</rdf:Description>

<rdf:Description rdf:about="http://www.ontology-of-units-of-measure.org/resource/om-2/gamma">
	<rdf:type rdf:resource="http://www.w3.org/2004/02/skos/core#Concept"/>
	<skos:inScheme rdf:resource="http://www.ontology-of-units-of-measure.org/resource/om-2/SingularUnit"/>
	<rdfs:comment xml:lang="en">The gamma is a unit of magnetic flux density defined as 1.0e-9 tesla.</rdfs:comment>
	<rdfs:label xml:lang="en">gamma</rdfs:label>
	<hasUnit xmlns="http://www.ontology-of-units-of-measure.org/resource/om-2/" rdf:resource="http://www.ontology-of-units-of-measure.org/resource/om-2/tesla"/>
	<rdfs:isDefinedBy rdf:resource="http://www.ontology-of-units-of-measure.org/resource/om-2/"/>
</rdf:Description>

<rdf:Description rdf:about="http://www.ontology-of-units-of-measure.org/resource/om-2/gauss">
	<rdf:type rdf:resource="http://www.w3.org/2004/02/skos/core#Concept"/>
	<skos:inScheme rdf:resource="http://www.ontology-of-units-of-measure.org/resource/om-2/SingularUnit"/>
	<rdfs:comment xml:lang="en">The gauss is a unit of magnetic flux density defined as 1.0e-4 tesla.</rdfs:comment>
	<rdfs:label xml:lang="en">gauss</rdfs:label>
	<hasUnit xmlns="http://www.ontology-of-units-of-measure.org/resource/om-2/" rdf:resource="http://www.ontology-of-units-of-measure.org/resource/om-2/tesla"/>
	<rdfs:isDefinedBy rdf:resource="http://www.ontology-of-units-of-measure.org/resource/om-2/"/>
</rdf:Description>

<rdf:Description rdf:about="http://www.ontology-of-units-of-measure.org/resource/om-2/solarLuminosity">
	<rdf:type rdf:resource="http://www.w3.org/2004/02/skos/core#Concept"/>
	<skos:inScheme rdf:resource="http://www.ontology-of-units-of-measure.org/resource/om-2/SingularUnit"/>
	<rdfs:comment xml:lang="en">Solar luminosity is a unit used in astronomy to denote stellar or galactic radiant fluxes (http://en.wikipedia.org/wiki/SolarLuminosity).</rdfs:comment>
	<rdfs:label xml:lang="en">solar luminosity</rdfs:label>
	<hasUnit xmlns="http://www.ontology-of-units-of-measure.org/resource/om-2/" rdf:resource="http://www.ontology-of-units-of-measure.org/resource/om-2/watt"/>
	<rdfs:isDefinedBy rdf:resource="http://www.ontology-of-units-of-measure.org/resource/om-2/"/>
</rdf:Description>

<rdf:Description rdf:about="http://www.ontology-of-units-of-measure.org/resource/om-2/hour-Sidereal">
	<rdf:type rdf:resource="http://www.w3.org/2004/02/skos/core#Concept"/>
	<skos:inScheme rdf:resource="http://www.ontology-of-units-of-measure.org/resource/om-2/SingularUnit"/>
	<rdfs:label xml:lang="en">hour (sidereal)</rdfs:label>
	<hasUnit xmlns="http://www.ontology-of-units-of-measure.org/resource/om-2/" rdf:resource="http://www.ontology-of-units-of-measure.org/resource/om-2/second-Time"/>
	<rdfs:isDefinedBy rdf:resource="http://www.ontology-of-units-of-measure.org/resource/om-2/"/>
</rdf:Description>

<rdf:Description rdf:about="http://www.ontology-of-units-of-measure.org/resource/om-2/horsepower-Metric">
	<rdf:type rdf:resource="http://www.w3.org/2004/02/skos/core#Concept"/>
	<skos:inScheme rdf:resource="http://www.ontology-of-units-of-measure.org/resource/om-2/SingularUnit"/>
	<rdfs:comment xml:lang="en">The metric horsepower is a unit of power defined as 7.354988e2 watt.</rdfs:comment>
	<rdfs:label xml:lang="en">horsepower (metric)</rdfs:label>
	<hasUnit xmlns="http://www.ontology-of-units-of-measure.org/resource/om-2/" rdf:resource="http://www.ontology-of-units-of-measure.org/resource/om-2/watt"/>
	<rdfs:isDefinedBy rdf:resource="http://www.ontology-of-units-of-measure.org/resource/om-2/"/>
</rdf:Description>

<rdf:Description rdf:about="http://www.ontology-of-units-of-measure.org/resource/om-2/nauticalMile-International">
	<rdf:type rdf:resource="http://www.w3.org/2004/02/skos/core#Concept"/>
	<skos:inScheme rdf:resource="http://www.ontology-of-units-of-measure.org/resource/om-2/SingularUnit"/>
	<rdfs:comment xml:lang="en">The international nautical mile is a unit of length defined as 1852 metre.</rdfs:comment>
	<rdfs:label xml:lang="en">nautical mile (international)</rdfs:label>
	<hasUnit xmlns="http://www.ontology-of-units-of-measure.org/resource/om-2/" rdf:resource="http://www.ontology-of-units-of-measure.org/resource/om-2/metre"/>
	<rdfs:isDefinedBy rdf:resource="http://www.ontology-of-units-of-measure.org/resource/om-2/"/>
</rdf:Description>

<rdf:Description rdf:about="http://www.ontology-of-units-of-measure.org/resource/om-2/parsec">
	<rdf:type rdf:resource="http://www.w3.org/2004/02/skos/core#Concept"/>
	<skos:inScheme rdf:resource="http://www.ontology-of-units-of-measure.org/resource/om-2/SingularUnit"/>
	<rdfs:comment xml:lang="en">The parsec is a unit of length defined as 3.08567758149137e16 metre.</rdfs:comment>
	<rdfs:label xml:lang="en">parsec</rdfs:label>
	<hasUnit xmlns="http://www.ontology-of-units-of-measure.org/resource/om-2/" rdf:resource="http://www.ontology-of-units-of-measure.org/resource/om-2/metre"/>
	<rdfs:isDefinedBy rdf:resource="http://www.ontology-of-units-of-measure.org/resource/om-2/"/>
</rdf:Description>

<rdf:Description rdf:about="http://www.ontology-of-units-of-measure.org/resource/om-2/phot">
	<rdf:type rdf:resource="http://www.w3.org/2004/02/skos/core#Concept"/>
	<skos:inScheme rdf:resource="http://www.ontology-of-units-of-measure.org/resource/om-2/SingularUnit"/>
	<rdfs:comment xml:lang="en">The phot is a unit of illuminance defined as 1.0e4 lux.</rdfs:comment>
	<rdfs:label xml:lang="en">phot</rdfs:label>
	<hasUnit xmlns="http://www.ontology-of-units-of-measure.org/resource/om-2/" rdf:resource="http://www.ontology-of-units-of-measure.org/resource/om-2/lux"/>
	<rdfs:isDefinedBy rdf:resource="http://www.ontology-of-units-of-measure.org/resource/om-2/"/>
</rdf:Description>

<rdf:Description rdf:about="http://www.ontology-of-units-of-measure.org/resource/om-2/point-ATA">
	<skos:inScheme rdf:resource="http://www.ontology-of-units-of-measure.org/resource/om-2/SingularUnit"/>
	<rdfs:comment xml:lang="en">The ATA point is a unit of length defined as 0.3514598e-3 metre.</rdfs:comment>
	<rdfs:label xml:lang="en">point (ATA)</rdfs:label>
	<hasUnit xmlns="http://www.ontology-of-units-of-measure.org/resource/om-2/" rdf:resource="http://www.ontology-of-units-of-measure.org/resource/om-2/metre"/>
</rdf:Description>

<rdf:Description rdf:about="http://www.ontology-of-units-of-measure.org/resource/om-2/solarRadius">
	<rdf:type rdf:resource="http://www.w3.org/2004/02/skos/core#Concept"/>
	<skos:inScheme rdf:resource="http://www.ontology-of-units-of-measure.org/resource/om-2/SingularUnit"/>
	<rdfs:comment xml:lang="en">Solar radius is a unit used in astronomy to denote stellar or stellar system radii (http://en.wikipedia.org/wiki/solarRadius).</rdfs:comment>
	<rdfs:label xml:lang="en">solar radius</rdfs:label>
	<hasUnit xmlns="http://www.ontology-of-units-of-measure.org/resource/om-2/" rdf:resource="http://www.ontology-of-units-of-measure.org/resource/om-2/metre"/>
	<rdfs:isDefinedBy rdf:resource="http://www.ontology-of-units-of-measure.org/resource/om-2/"/>
</rdf:Description>

<rdf:Description rdf:about="http://www.ontology-of-units-of-measure.org/resource/om-2/minute-Sidereal">
	<rdf:type rdf:resource="http://www.w3.org/2004/02/skos/core#Concept"/>
	<skos:inScheme rdf:resource="http://www.ontology-of-units-of-measure.org/resource/om-2/SingularUnit"/>
	<rdfs:comment xml:lang="en">The sidereal minute is a unit of time defined as 5.983617e1 second.</rdfs:comment>
	<rdfs:label xml:lang="en">minute (sidereal)</rdfs:label>
	<hasUnit xmlns="http://www.ontology-of-units-of-measure.org/resource/om-2/" rdf:resource="http://www.ontology-of-units-of-measure.org/resource/om-2/second-Time"/>
	<rdfs:isDefinedBy rdf:resource="http://www.ontology-of-units-of-measure.org/resource/om-2/"/>
</rdf:Description>

<rdf:Description rdf:about="http://www.ontology-of-units-of-measure.org/resource/om-2/minute-Time">
	<rdf:type rdf:resource="http://www.w3.org/2004/02/skos/core#Concept"/>
	<skos:inScheme rdf:resource="http://www.ontology-of-units-of-measure.org/resource/om-2/SingularUnit"/>
	<rdfs:comment xml:lang="en">The minute (time) is a unit of time defined as 60 second.</rdfs:comment>
	<rdfs:label xml:lang="en">minute</rdfs:label>
	<hasUnit xmlns="http://www.ontology-of-units-of-measure.org/resource/om-2/" rdf:resource="http://www.ontology-of-units-of-measure.org/resource/om-2/second-Time"/>
	<rdfs:isDefinedBy rdf:resource="http://www.ontology-of-units-of-measure.org/resource/om-2/"/>
</rdf:Description>

<rdf:Description rdf:about="http://www.ontology-of-units-of-measure.org/resource/om-2/second-Sidereal">
	<rdf:type rdf:resource="http://www.w3.org/2004/02/skos/core#Concept"/>
	<skos:inScheme rdf:resource="http://www.ontology-of-units-of-measure.org/resource/om-2/SingularUnit"/>
	<rdfs:comment xml:lang="en">The sidereal second is a unit of time defined as 9.972696e-1 second.</rdfs:comment>
	<rdfs:label xml:lang="en">second (sidereal)</rdfs:label>
	<hasUnit xmlns="http://www.ontology-of-units-of-measure.org/resource/om-2/" rdf:resource="http://www.ontology-of-units-of-measure.org/resource/om-2/second-Time"/>
	<rdfs:isDefinedBy rdf:resource="http://www.ontology-of-units-of-measure.org/resource/om-2/"/>
</rdf:Description>

<rdf:Description rdf:about="http://www.ontology-of-units-of-measure.org/resource/om-2/shake">
	<rdf:type rdf:resource="http://www.w3.org/2004/02/skos/core#Concept"/>
	<skos:inScheme rdf:resource="http://www.ontology-of-units-of-measure.org/resource/om-2/SingularUnit"/>
	<rdfs:comment xml:lang="en">The shake is a unit of time defined as 1.0e-8 second.</rdfs:comment>
	<rdfs:label xml:lang="en">shake</rdfs:label>
	<hasUnit xmlns="http://www.ontology-of-units-of-measure.org/resource/om-2/" rdf:resource="http://www.ontology-of-units-of-measure.org/resource/om-2/second-Time"/>
	<rdfs:isDefinedBy rdf:resource="http://www.ontology-of-units-of-measure.org/resource/om-2/"/>
</rdf:Description>

<rdf:Description rdf:about="http://www.ontology-of-units-of-measure.org/resource/om-2/week">
	<rdf:type rdf:resource="http://www.w3.org/2004/02/skos/core#Concept"/>
	<skos:inScheme rdf:resource="http://www.ontology-of-units-of-measure.org/resource/om-2/SingularUnit"/>
	<rdfs:comment xml:lang="en">The week is a unit of time defined as 6.04800e5 second.</rdfs:comment>
	<rdfs:label xml:lang="en">week</rdfs:label>
	<hasUnit xmlns="http://www.ontology-of-units-of-measure.org/resource/om-2/" rdf:resource="http://www.ontology-of-units-of-measure.org/resource/om-2/second-Time"/>
	<rdfs:isDefinedBy rdf:resource="http://www.ontology-of-units-of-measure.org/resource/om-2/"/>
</rdf:Description>

<rdf:Description rdf:about="http://www.ontology-of-units-of-measure.org/resource/om-2/year">
	<rdf:type rdf:resource="http://www.w3.org/2004/02/skos/core#Concept"/>
	<skos:inScheme rdf:resource="http://www.ontology-of-units-of-measure.org/resource/om-2/SingularUnit"/>
	<rdfs:comment xml:lang="en">The year is a unit of time defined as 3.1536e7 second.</rdfs:comment>
	<rdfs:label xml:lang="en">year</rdfs:label>
	<hasUnit xmlns="http://www.ontology-of-units-of-measure.org/resource/om-2/" rdf:resource="http://www.ontology-of-units-of-measure.org/resource/om-2/second-Time"/>
	<rdfs:isDefinedBy rdf:resource="http://www.ontology-of-units-of-measure.org/resource/om-2/"/>
</rdf:Description>

<rdf:Description rdf:about="http://www.ontology-of-units-of-measure.org/resource/om-2/year-Sidereal">
	<rdf:type rdf:resource="http://www.w3.org/2004/02/skos/core#Concept"/>
	<skos:inScheme rdf:resource="http://www.ontology-of-units-of-measure.org/resource/om-2/SingularUnit"/>
	<rdfs:comment xml:lang="en">The sidereal year is a unit of time defined as 3.155815e7 second.</rdfs:comment>
	<rdfs:label xml:lang="en">year (sidereal)</rdfs:label>
	<hasUnit xmlns="http://www.ontology-of-units-of-measure.org/resource/om-2/" rdf:resource="http://www.ontology-of-units-of-measure.org/resource/om-2/second-Time"/>
	<rdfs:isDefinedBy rdf:resource="http://www.ontology-of-units-of-measure.org/resource/om-2/"/>
</rdf:Description>

<rdf:Description rdf:about="http://www.ontology-of-units-of-measure.org/resource/om-2/year-Tropical">
	<rdf:type rdf:resource="http://www.w3.org/2004/02/skos/core#Concept"/>
	<skos:inScheme rdf:resource="http://www.ontology-of-units-of-measure.org/resource/om-2/SingularUnit"/>
	<rdfs:comment xml:lang="en">The tropical year is a unit of time defined as 3.155693e7 second.</rdfs:comment>
	<rdfs:label xml:lang="en">year (tropical)</rdfs:label>
	<hasUnit xmlns="http://www.ontology-of-units-of-measure.org/resource/om-2/" rdf:resource="http://www.ontology-of-units-of-measure.org/resource/om-2/second-Time"/>
	<rdfs:isDefinedBy rdf:resource="http://www.ontology-of-units-of-measure.org/resource/om-2/"/>
</rdf:Description>

<rdf:Description rdf:about="http://www.ontology-of-units-of-measure.org/resource/om-2/abmho">
	<rdf:type rdf:resource="http://www.w3.org/2004/02/skos/core#Concept"/>
	<skos:inScheme rdf:resource="http://www.ontology-of-units-of-measure.org/resource/om-2/SingularUnit"/>
	<rdfs:comment xml:lang="en">The abmho is a unit of electrical conductance defined as 1.0e9 siemens.</rdfs:comment>
	<rdfs:label xml:lang="en">abmho</rdfs:label>
	<hasUnit xmlns="http://www.ontology-of-units-of-measure.org/resource/om-2/" rdf:resource="http://www.ontology-of-units-of-measure.org/resource/om-2/siemens"/>
</rdf:Description>

<rdf:Description rdf:about="http://www.ontology-of-units-of-measure.org/resource/om-2/siemens">
	<rdf:type rdf:resource="http://www.w3.org/2004/02/skos/core#Concept"/>
</rdf:Description>

<rdf:Description rdf:about="http://www.ontology-of-units-of-measure.org/resource/om-2/abmho">
	<rdfs:isDefinedBy rdf:resource="http://www.ontology-of-units-of-measure.org/resource/om-2/"/>
</rdf:Description>

<rdf:Description rdf:about="http://www.ontology-of-units-of-measure.org/resource/om-2/siemens">
	<rdfs:isDefinedBy rdf:resource="http://www.ontology-of-units-of-measure.org/resource/om-2/"/>
</rdf:Description>

<rdf:Description rdf:about="http://www.ontology-of-units-of-measure.org/resource/om-2/mho">
	<rdf:type rdf:resource="http://www.w3.org/2004/02/skos/core#Concept"/>
	<skos:inScheme rdf:resource="http://www.ontology-of-units-of-measure.org/resource/om-2/SingularUnit"/>
	<rdfs:comment xml:lang="en">The mho is a unit of electrical conductance defined as 1 siemens.</rdfs:comment>
	<rdfs:label xml:lang="en">mho</rdfs:label>
	<hasUnit xmlns="http://www.ontology-of-units-of-measure.org/resource/om-2/" rdf:resource="http://www.ontology-of-units-of-measure.org/resource/om-2/siemens"/>
	<rdfs:isDefinedBy rdf:resource="http://www.ontology-of-units-of-measure.org/resource/om-2/"/>
</rdf:Description>

<rdf:Description rdf:about="http://www.ontology-of-units-of-measure.org/resource/om-2/statmho">
	<rdf:type rdf:resource="http://www.w3.org/2004/02/skos/core#Concept"/>
	<skos:inScheme rdf:resource="http://www.ontology-of-units-of-measure.org/resource/om-2/SingularUnit"/>
	<rdfs:comment xml:lang="en">The statmho is a unit of electrical conductance defined as 1.112650e-12 siemens.</rdfs:comment>
	<rdfs:label xml:lang="en">statmho</rdfs:label>
	<hasUnit xmlns="http://www.ontology-of-units-of-measure.org/resource/om-2/" rdf:resource="http://www.ontology-of-units-of-measure.org/resource/om-2/siemens"/>
	<rdfs:isDefinedBy rdf:resource="http://www.ontology-of-units-of-measure.org/resource/om-2/"/>
</rdf:Description>

<rdf:Description rdf:about="http://www.ontology-of-units-of-measure.org/resource/om-2/rem">
	<rdf:type rdf:resource="http://www.w3.org/2004/02/skos/core#Concept"/>
	<skos:inScheme rdf:resource="http://www.ontology-of-units-of-measure.org/resource/om-2/SingularUnit"/>
	<rdfs:comment xml:lang="en">The rem is a unit of dose equivalent defined as 1.0e-2 sievert.</rdfs:comment>
	<rdfs:label xml:lang="en">rem</rdfs:label>
	<hasUnit xmlns="http://www.ontology-of-units-of-measure.org/resource/om-2/" rdf:resource="http://www.ontology-of-units-of-measure.org/resource/om-2/sievert"/>
</rdf:Description>

<rdf:Description rdf:about="http://www.ontology-of-units-of-measure.org/resource/om-2/sievert">
	<rdf:type rdf:resource="http://www.w3.org/2004/02/skos/core#Concept"/>
</rdf:Description>

<rdf:Description rdf:about="http://www.ontology-of-units-of-measure.org/resource/om-2/rem">
	<rdfs:isDefinedBy rdf:resource="http://www.ontology-of-units-of-measure.org/resource/om-2/"/>
</rdf:Description>

<rdf:Description rdf:about="http://www.ontology-of-units-of-measure.org/resource/om-2/sievert">
	<rdfs:isDefinedBy rdf:resource="http://www.ontology-of-units-of-measure.org/resource/om-2/"/>
</rdf:Description>

<rdf:Description rdf:about="http://www.ontology-of-units-of-measure.org/resource/om-2/partsPerMillion">
	<rdf:type rdf:resource="http://www.w3.org/2004/02/skos/core#Concept"/>
	<skos:inScheme rdf:resource="http://www.ontology-of-units-of-measure.org/resource/om-2/SingularUnit"/>
	<rdfs:comment xml:lang="en">Parts per million is a unit of dimension one defined as 1/1 000 000.</rdfs:comment>
	<rdfs:label xml:lang="en">parts per million</rdfs:label>
	<hasUnit xmlns="http://www.ontology-of-units-of-measure.org/resource/om-2/" rdf:resource="http://www.ontology-of-units-of-measure.org/resource/om-2/one"/>
</rdf:Description>

<rdf:Description rdf:about="http://www.ontology-of-units-of-measure.org/resource/om-2/one">
	<rdf:type rdf:resource="http://www.w3.org/2004/02/skos/core#Concept"/>
</rdf:Description>

<rdf:Description rdf:about="http://www.ontology-of-units-of-measure.org/resource/om-2/partsPerMillion">
	<rdfs:isDefinedBy rdf:resource="http://www.ontology-of-units-of-measure.org/resource/om-2/"/>
</rdf:Description>

<rdf:Description rdf:about="http://www.ontology-of-units-of-measure.org/resource/om-2/one">
	<rdfs:isDefinedBy rdf:resource="http://www.ontology-of-units-of-measure.org/resource/om-2/"/>
</rdf:Description>

<rdf:Description rdf:about="http://www.ontology-of-units-of-measure.org/resource/om-2/atmosphere-Standard">
	<rdf:type rdf:resource="http://www.w3.org/2004/02/skos/core#Concept"/>
	<skos:inScheme rdf:resource="http://www.ontology-of-units-of-measure.org/resource/om-2/SingularUnit"/>
	<rdfs:comment xml:lang="en">The standard atmosphere is a unit of pressure defined as 1.01325e5 pascal.</rdfs:comment>
	<rdfs:label xml:lang="en">atmosphere (standard)</rdfs:label>
	<hasUnit xmlns="http://www.ontology-of-units-of-measure.org/resource/om-2/" rdf:resource="http://www.ontology-of-units-of-measure.org/resource/om-2/pascal"/>
</rdf:Description>

<rdf:Description rdf:about="http://www.ontology-of-units-of-measure.org/resource/om-2/pascal">
	<rdf:type rdf:resource="http://www.w3.org/2004/02/skos/core#Concept"/>
</rdf:Description>

<rdf:Description rdf:about="http://www.ontology-of-units-of-measure.org/resource/om-2/atmosphere-Standard">
	<rdfs:isDefinedBy rdf:resource="http://www.ontology-of-units-of-measure.org/resource/om-2/"/>
</rdf:Description>

<rdf:Description rdf:about="http://www.ontology-of-units-of-measure.org/resource/om-2/pascal">
	<rdfs:isDefinedBy rdf:resource="http://www.ontology-of-units-of-measure.org/resource/om-2/"/>
</rdf:Description>

<rdf:Description rdf:about="http://www.ontology-of-units-of-measure.org/resource/om-2/atmosphere-Technical">
	<rdf:type rdf:resource="http://www.w3.org/2004/02/skos/core#Concept"/>
	<skos:inScheme rdf:resource="http://www.ontology-of-units-of-measure.org/resource/om-2/SingularUnit"/>
	<rdfs:comment xml:lang="en">The technical atmosphere is a unit of pressure defined as 9.80665e4 pascal.</rdfs:comment>
	<rdfs:label xml:lang="en">atmosphere (technical)</rdfs:label>
	<hasUnit xmlns="http://www.ontology-of-units-of-measure.org/resource/om-2/" rdf:resource="http://www.ontology-of-units-of-measure.org/resource/om-2/pascal"/>
	<rdfs:isDefinedBy rdf:resource="http://www.ontology-of-units-of-measure.org/resource/om-2/"/>
</rdf:Description>

<rdf:Description rdf:about="http://www.ontology-of-units-of-measure.org/resource/om-2/bar">
	<rdf:type rdf:resource="http://www.w3.org/2004/02/skos/core#Concept"/>
	<skos:inScheme rdf:resource="http://www.ontology-of-units-of-measure.org/resource/om-2/SingularUnit"/>
	<rdfs:comment xml:lang="en">The bar is a unit of pressure defined as 100 000 pascal.</rdfs:comment>
	<rdfs:label xml:lang="en">bar</rdfs:label>
	<hasUnit xmlns="http://www.ontology-of-units-of-measure.org/resource/om-2/" rdf:resource="http://www.ontology-of-units-of-measure.org/resource/om-2/pascal"/>
	<rdfs:isDefinedBy rdf:resource="http://www.ontology-of-units-of-measure.org/resource/om-2/"/>
</rdf:Description>

<rdf:Description rdf:about="http://www.ontology-of-units-of-measure.org/resource/om-2/barye">
	<rdf:type rdf:resource="http://www.w3.org/2004/02/skos/core#Concept"/>
	<skos:inScheme rdf:resource="http://www.ontology-of-units-of-measure.org/resource/om-2/SingularUnit"/>
	<rdfs:comment xml:lang="en">The barye is a unit of pressure defined as 0.1 pascal.</rdfs:comment>
	<rdfs:label xml:lang="en">barye</rdfs:label>
	<hasUnit xmlns="http://www.ontology-of-units-of-measure.org/resource/om-2/" rdf:resource="http://www.ontology-of-units-of-measure.org/resource/om-2/pascal"/>
	<rdfs:isDefinedBy rdf:resource="http://www.ontology-of-units-of-measure.org/resource/om-2/"/>
</rdf:Description>

<rdf:Description rdf:about="http://www.ontology-of-units-of-measure.org/resource/om-2/dyne">
	<rdf:type rdf:resource="http://www.w3.org/2004/02/skos/core#Concept"/>
	<skos:inScheme rdf:resource="http://www.ontology-of-units-of-measure.org/resource/om-2/SingularUnit"/>
	<rdfs:comment xml:lang="en">The dyne is a unit of force defined as 1.0e-5 newton.</rdfs:comment>
	<rdfs:label xml:lang="en">dyne</rdfs:label>
	<hasUnit xmlns="http://www.ontology-of-units-of-measure.org/resource/om-2/" rdf:resource="http://www.ontology-of-units-of-measure.org/resource/om-2/newton"/>
</rdf:Description>

<rdf:Description rdf:about="http://www.ontology-of-units-of-measure.org/resource/om-2/newton">
	<rdf:type rdf:resource="http://www.w3.org/2004/02/skos/core#Concept"/>
</rdf:Description>

<rdf:Description rdf:about="http://www.ontology-of-units-of-measure.org/resource/om-2/dyne">
	<rdfs:isDefinedBy rdf:resource="http://www.ontology-of-units-of-measure.org/resource/om-2/"/>
</rdf:Description>

<rdf:Description rdf:about="http://www.ontology-of-units-of-measure.org/resource/om-2/newton">
	<rdfs:isDefinedBy rdf:resource="http://www.ontology-of-units-of-measure.org/resource/om-2/"/>
</rdf:Description>

<rdf:Description rdf:about="http://www.ontology-of-units-of-measure.org/resource/om-2/kip">
	<rdf:type rdf:resource="http://www.w3.org/2004/02/skos/core#Concept"/>
	<skos:inScheme rdf:resource="http://www.ontology-of-units-of-measure.org/resource/om-2/SingularUnit"/>
	<rdfs:comment xml:lang="en">The kip is a unit of force defined as 4.448222e3 newton.</rdfs:comment>
	<rdfs:label xml:lang="en">kip</rdfs:label>
	<hasUnit xmlns="http://www.ontology-of-units-of-measure.org/resource/om-2/" rdf:resource="http://www.ontology-of-units-of-measure.org/resource/om-2/newton"/>
	<rdfs:isDefinedBy rdf:resource="http://www.ontology-of-units-of-measure.org/resource/om-2/"/>
</rdf:Description>

<rdf:Description rdf:about="http://www.ontology-of-units-of-measure.org/resource/om-2/percent">
	<rdf:type rdf:resource="http://www.w3.org/2004/02/skos/core#Concept"/>
	<skos:inScheme rdf:resource="http://www.ontology-of-units-of-measure.org/resource/om-2/SingularUnit"/>
	<rdfs:comment xml:lang="en">The percent is a unit of dimension one defined as 1/100.</rdfs:comment>
	<rdfs:label xml:lang="en">percent</rdfs:label>
	<hasUnit xmlns="http://www.ontology-of-units-of-measure.org/resource/om-2/" rdf:resource="http://www.ontology-of-units-of-measure.org/resource/om-2/one"/>
	<rdfs:isDefinedBy rdf:resource="http://www.ontology-of-units-of-measure.org/resource/om-2/"/>
</rdf:Description>

<rdf:Description rdf:about="http://www.ontology-of-units-of-measure.org/resource/om-2/horsepower-Water">
	<rdf:type rdf:resource="http://www.w3.org/2004/02/skos/core#Concept"/>
	<skos:inScheme rdf:resource="http://www.ontology-of-units-of-measure.org/resource/om-2/SingularUnit"/>
	<rdfs:comment xml:lang="en">The water horsepower is a unit of power defined as 7.46043e2 watt.</rdfs:comment>
	<rdfs:label xml:lang="en">horsepower (water)</rdfs:label>
	<hasUnit xmlns="http://www.ontology-of-units-of-measure.org/resource/om-2/" rdf:resource="http://www.ontology-of-units-of-measure.org/resource/om-2/watt"/>
	<rdfs:isDefinedBy rdf:resource="http://www.ontology-of-units-of-measure.org/resource/om-2/"/>
</rdf:Description>

<rdf:Description rdf:about="http://www.ontology-of-units-of-measure.org/resource/om-2/gray">
	<skos:inScheme rdf:resource="http://www.ontology-of-units-of-measure.org/resource/om-2/SingularUnit"/>
	<rdfs:comment xml:lang="en">The gray is a unit of absorbed dose defined as joule divided by kilogram = square metre divided by second squared.</rdfs:comment>
	<rdfs:label xml:lang="en">gray</rdfs:label>
</rdf:Description>

<rdf:Description rdf:about="http://www.ontology-of-units-of-measure.org/resource/om-2/henry">
	<skos:inScheme rdf:resource="http://www.ontology-of-units-of-measure.org/resource/om-2/SingularUnit"/>
	<rdfs:comment xml:lang="en">The henry is a unit of inductance defined as square metre times kilogram divided by second squared times ampere squared = weber divided by ampere = volt second divided by ampere = (joule divided by coulomb) times second divided by (coulomb divided by second) = joule times second squared divided by coulomb squared = square metre times kilogram divided by coulomb squared.</rdfs:comment>
	<rdfs:label xml:lang="en">henry</rdfs:label>
</rdf:Description>

<rdf:Description rdf:about="http://www.ontology-of-units-of-measure.org/resource/om-2/hertz">
	<rdf:type rdf:resource="http://www.w3.org/2004/02/skos/core#Concept"/>
	<skos:inScheme rdf:resource="http://www.ontology-of-units-of-measure.org/resource/om-2/SingularUnit"/>
	<rdfs:comment xml:lang="en">The hertz is a unit of frequency defined as 1 divided by second.</rdfs:comment>
	<rdfs:label xml:lang="en">hertz</rdfs:label>
	<rdfs:isDefinedBy rdf:resource="http://www.ontology-of-units-of-measure.org/resource/om-2/"/>
</rdf:Description>

<rdf:Description rdf:about="http://www.ontology-of-units-of-measure.org/resource/om-2/knot-International">
	<rdf:type rdf:resource="http://www.w3.org/2004/02/skos/core#Concept"/>
	<skos:inScheme rdf:resource="http://www.ontology-of-units-of-measure.org/resource/om-2/SingularUnit"/>
	<rdfs:comment xml:lang="en">The international knot is a unit of speed defined as nautical mile per hour.</rdfs:comment>
	<rdfs:label xml:lang="en">knot (international)</rdfs:label>
	<rdfs:isDefinedBy rdf:resource="http://www.ontology-of-units-of-measure.org/resource/om-2/"/>
</rdf:Description>

<rdf:Description rdf:about="http://www.ontology-of-units-of-measure.org/resource/om-2/lambert">
	<rdf:type rdf:resource="http://www.w3.org/2004/02/skos/core#Concept"/>
	<skos:inScheme rdf:resource="http://www.ontology-of-units-of-measure.org/resource/om-2/SingularUnit"/>
	<rdfs:comment xml:lang="en">The lambert is a unit of luminance defined as 3.183099e3 candela per square metre.</rdfs:comment>
	<rdfs:label xml:lang="en">lambert</rdfs:label>
	<rdfs:isDefinedBy rdf:resource="http://www.ontology-of-units-of-measure.org/resource/om-2/"/>
</rdf:Description>

<rdf:Description rdf:about="http://www.ontology-of-units-of-measure.org/resource/om-2/liquidPint-US">
	<rdf:type rdf:resource="http://www.w3.org/2004/02/skos/core#Concept"/>
	<skos:inScheme rdf:resource="http://www.ontology-of-units-of-measure.org/resource/om-2/SingularUnit"/>
	<rdfs:comment xml:lang="en">The US liquid pint is a unit of volume defined as 4.731765e-4 cubic metre.</rdfs:comment>
	<rdfs:label xml:lang="en">liquid pint (US)</rdfs:label>
	<rdfs:isDefinedBy rdf:resource="http://www.ontology-of-units-of-measure.org/resource/om-2/"/>
</rdf:Description>

<rdf:Description rdf:about="http://www.ontology-of-units-of-measure.org/resource/om-2/liquidQuart-US">
	<rdf:type rdf:resource="http://www.w3.org/2004/02/skos/core#Concept"/>
	<skos:inScheme rdf:resource="http://www.ontology-of-units-of-measure.org/resource/om-2/SingularUnit"/>
	<rdfs:comment xml:lang="en">The US liquid quart is a unit of volume defined as 9.463529e-4 cubic metre.</rdfs:comment>
	<rdfs:label xml:lang="en">liquid quart (US)</rdfs:label>
	<rdfs:isDefinedBy rdf:resource="http://www.ontology-of-units-of-measure.org/resource/om-2/"/>
</rdf:Description>

<rdf:Description rdf:about="http://www.ontology-of-units-of-measure.org/resource/om-2/litre">
	<skos:inScheme rdf:resource="http://www.ontology-of-units-of-measure.org/resource/om-2/SingularUnit"/>
	<rdfs:comment xml:lang="en">The litre is a unit of volume defined as 1.0e-3 cubic metre.</rdfs:comment>
	<rdfs:label xml:lang="en">litre</rdfs:label>
</rdf:Description>

<rdf:Description rdf:about="http://www.ontology-of-units-of-measure.org/resource/om-2/lumen">
	<rdf:type rdf:resource="http://www.w3.org/2004/02/skos/core#Concept"/>
	<skos:inScheme rdf:resource="http://www.ontology-of-units-of-measure.org/resource/om-2/SingularUnit"/>
	<rdfs:comment xml:lang="en">The lumen is a unit of luminous flux defined as candela times steradian = lux times square metre.</rdfs:comment>
	<rdfs:label xml:lang="en">lumen</rdfs:label>
	<rdfs:isDefinedBy rdf:resource="http://www.ontology-of-units-of-measure.org/resource/om-2/"/>
</rdf:Description>

<rdf:Description rdf:about="http://www.ontology-of-units-of-measure.org/resource/om-2/lux">
	<skos:inScheme rdf:resource="http://www.ontology-of-units-of-measure.org/resource/om-2/SingularUnit"/>
	<rdfs:comment xml:lang="en">The lux is a unit of illuminance defined as lumen divided by square metre = candela times steradian divided by square metre.</rdfs:comment>
	<rdfs:label xml:lang="en">lux</rdfs:label>
</rdf:Description>

<rdf:Description rdf:about="http://www.ontology-of-units-of-measure.org/resource/om-2/metre">
	<skos:inScheme rdf:resource="http://www.ontology-of-units-of-measure.org/resource/om-2/SingularUnit"/>
	<rdfs:comment xml:lang="en">The metre is a unit of length defined as the length of the path travelled by light in vacuum during a time interval of 1/299 792 458 of a second.</rdfs:comment>
	<rdfs:label xml:lang="en">metre</rdfs:label>
</rdf:Description>

<rdf:Description rdf:about="http://www.ontology-of-units-of-measure.org/resource/om-2/molair">
	<rdf:type rdf:resource="http://www.w3.org/2004/02/skos/core#Concept"/>
	<skos:inScheme rdf:resource="http://www.ontology-of-units-of-measure.org/resource/om-2/SingularUnit"/>
	<rdfs:comment xml:lang="en">Molair is a unit of amount of substance concentration defined as 1 mole per litre.</rdfs:comment>
	<rdfs:label xml:lang="en">molair</rdfs:label>
	<rdfs:isDefinedBy rdf:resource="http://www.ontology-of-units-of-measure.org/resource/om-2/"/>
</rdf:Description>

<rdf:Description rdf:about="http://www.ontology-of-units-of-measure.org/resource/om-2/poise">
	<rdf:type rdf:resource="http://www.w3.org/2004/02/skos/core#Concept"/>
	<skos:inScheme rdf:resource="http://www.ontology-of-units-of-measure.org/resource/om-2/SingularUnit"/>
	<rdfs:comment xml:lang="en">The poise is a unit of dynamic viscosity defined as 1.0e-1 pascal second (time).</rdfs:comment>
	<rdfs:label xml:lang="en">poise</rdfs:label>
	<rdfs:isDefinedBy rdf:resource="http://www.ontology-of-units-of-measure.org/resource/om-2/"/>
</rdf:Description>

<rdf:Description rdf:about="http://www.ontology-of-units-of-measure.org/resource/om-2/poundApothecaries">
	<rdf:type rdf:resource="http://www.w3.org/2004/02/skos/core#Concept"/>
	<skos:inScheme rdf:resource="http://www.ontology-of-units-of-measure.org/resource/om-2/SingularUnit"/>
	<rdfs:comment xml:lang="en">The apothecaries' pound is a unit of mass defined as 3.732417e-1 kilogram.</rdfs:comment>
	<rdfs:label xml:lang="en">pound (apthecaries')</rdfs:label>
	<rdfs:isDefinedBy rdf:resource="http://www.ontology-of-units-of-measure.org/resource/om-2/"/>
</rdf:Description>

<rdf:Description rdf:about="http://www.ontology-of-units-of-measure.org/resource/om-2/poundAvoirdupois">
	<rdf:type rdf:resource="http://www.w3.org/2004/02/skos/core#Concept"/>
	<skos:inScheme rdf:resource="http://www.ontology-of-units-of-measure.org/resource/om-2/SingularUnit"/>
	<rdfs:comment xml:lang="en">The avoirdupois pound is a unit of mass defined as 4.535924e-1 kilogram.</rdfs:comment>
	<rdfs:label xml:lang="en">pound (avoirdupois)</rdfs:label>
	<rdfs:isDefinedBy rdf:resource="http://www.ontology-of-units-of-measure.org/resource/om-2/"/>
</rdf:Description>

<rdf:Description rdf:about="http://www.ontology-of-units-of-measure.org/resource/om-2/radian">
	<skos:inScheme rdf:resource="http://www.ontology-of-units-of-measure.org/resource/om-2/SingularUnit"/>
	<rdfs:comment xml:lang="en">The radian is a unit of angle defined as the angle subtended at the center of a circle by an arc that is equal in length to the radius of the circle.</rdfs:comment>
	<rdfs:label xml:lang="en">radian</rdfs:label>
</rdf:Description>

<rdf:Description rdf:about="http://www.ontology-of-units-of-measure.org/resource/om-2/rhe">
	<rdf:type rdf:resource="http://www.w3.org/2004/02/skos/core#Concept"/>
	<skos:inScheme rdf:resource="http://www.ontology-of-units-of-measure.org/resource/om-2/SingularUnit"/>
	<rdfs:comment xml:lang="en">The rhe is a unit of fluidity defined as 10 reciprocal pascal second (time).</rdfs:comment>
	<rdfs:label xml:lang="en">rhe</rdfs:label>
	<rdfs:isDefinedBy rdf:resource="http://www.ontology-of-units-of-measure.org/resource/om-2/"/>
</rdf:Description>

<rdf:Description rdf:about="http://www.ontology-of-units-of-measure.org/resource/om-2/röntgen">
	<rdf:type rdf:resource="http://www.w3.org/2004/02/skos/core#Concept"/>
	<skos:inScheme rdf:resource="http://www.ontology-of-units-of-measure.org/resource/om-2/SingularUnit"/>
	<rdfs:comment xml:lang="en">The röntgen is a unit of exposure to x and γ rays defined as 2.58e-4 coulomb per kilogram.</rdfs:comment>
	<rdfs:label xml:lang="en">röntgen</rdfs:label>
	<rdfs:isDefinedBy rdf:resource="http://www.ontology-of-units-of-measure.org/resource/om-2/"/>
</rdf:Description>

<rdf:Description rdf:about="http://www.ontology-of-units-of-measure.org/resource/om-2/second-Time">
	<skos:inScheme rdf:resource="http://www.ontology-of-units-of-measure.org/resource/om-2/SingularUnit"/>
	<rdfs:comment xml:lang="en">The second is a unit of time defined as the duration of 9 192 631 770 periods of the radiation corresponding to the transition between the two hyperfine levels of the ground state of the cesium 133 atom.</rdfs:comment>
	<rdfs:label xml:lang="en">second</rdfs:label>
</rdf:Description>

<rdf:Description rdf:about="http://www.ontology-of-units-of-measure.org/resource/om-2/steradian">
	<rdf:type rdf:resource="http://www.w3.org/2004/02/skos/core#Concept"/>
	<skos:inScheme rdf:resource="http://www.ontology-of-units-of-measure.org/resource/om-2/SingularUnit"/>
	<rdfs:comment xml:lang="en">The steradian is a unit of solid angle defined as the solid angle subtended at the center of a sphere by a portion of the surface of the sphere that has an area equal to the square of the radius of the sphere.</rdfs:comment>
	<rdfs:label xml:lang="en">steradian</rdfs:label>
	<rdfs:isDefinedBy rdf:resource="http://www.ontology-of-units-of-measure.org/resource/om-2/"/>
</rdf:Description>

<rdf:Description rdf:about="http://www.ontology-of-units-of-measure.org/resource/om-2/stere">
	<rdf:type rdf:resource="http://www.w3.org/2004/02/skos/core#Concept"/>
	<skos:inScheme rdf:resource="http://www.ontology-of-units-of-measure.org/resource/om-2/SingularUnit"/>
	<rdfs:comment xml:lang="en">The stere is a unit of volume defined as cubic metre.</rdfs:comment>
	<rdfs:label xml:lang="en">stere</rdfs:label>
	<rdfs:isDefinedBy rdf:resource="http://www.ontology-of-units-of-measure.org/resource/om-2/"/>
</rdf:Description>

<rdf:Description rdf:about="http://www.ontology-of-units-of-measure.org/resource/om-2/stilb">
	<rdf:type rdf:resource="http://www.w3.org/2004/02/skos/core#Concept"/>
	<skos:inScheme rdf:resource="http://www.ontology-of-units-of-measure.org/resource/om-2/SingularUnit"/>
	<rdfs:comment xml:lang="en">The stilb is a unit of luminance defined as 1.0e4 candela per square metre.</rdfs:comment>
	<rdfs:label xml:lang="en">stilb</rdfs:label>
	<rdfs:isDefinedBy rdf:resource="http://www.ontology-of-units-of-measure.org/resource/om-2/"/>
</rdf:Description>

<rdf:Description rdf:about="http://www.ontology-of-units-of-measure.org/resource/om-2/stokes">
	<rdf:type rdf:resource="http://www.w3.org/2004/02/skos/core#Concept"/>
	<skos:inScheme rdf:resource="http://www.ontology-of-units-of-measure.org/resource/om-2/SingularUnit"/>
	<rdfs:comment xml:lang="en">The stokes is a unit of kinematic viscosity defined as 1.0e-4 square metre per second (time).</rdfs:comment>
	<rdfs:label xml:lang="en">stokes</rdfs:label>
	<rdfs:isDefinedBy rdf:resource="http://www.ontology-of-units-of-measure.org/resource/om-2/"/>
</rdf:Description>

<rdf:Description rdf:about="http://www.ontology-of-units-of-measure.org/resource/om-2/tablespoon-US">
	<rdf:type rdf:resource="http://www.w3.org/2004/02/skos/core#Concept"/>
	<skos:inScheme rdf:resource="http://www.ontology-of-units-of-measure.org/resource/om-2/SingularUnit"/>
	<rdfs:comment xml:lang="en">The US tablespoon is a unit of volume defined as 1.478676e-5 cubic metre.</rdfs:comment>
	<rdfs:label xml:lang="en">tablespoon (US)</rdfs:label>
	<rdfs:isDefinedBy rdf:resource="http://www.ontology-of-units-of-measure.org/resource/om-2/"/>
</rdf:Description>

<rdf:Description rdf:about="http://www.ontology-of-units-of-measure.org/resource/om-2/abfarad">
	<rdf:type rdf:resource="http://www.w3.org/2004/02/skos/core#Concept"/>
	<skos:inScheme rdf:resource="http://www.ontology-of-units-of-measure.org/resource/om-2/SingularUnit"/>
	<rdfs:comment xml:lang="en">The abfarad is a unit of capacitance defined as 1.0e9 farad.</rdfs:comment>
	<rdfs:label xml:lang="en">abfarad</rdfs:label>
	<hasUnit xmlns="http://www.ontology-of-units-of-measure.org/resource/om-2/" rdf:resource="http://www.ontology-of-units-of-measure.org/resource/om-2/farad"/>
</rdf:Description>

<rdf:Description rdf:about="http://www.ontology-of-units-of-measure.org/resource/om-2/farad">
	<rdf:type rdf:resource="http://www.w3.org/2004/02/skos/core#Concept"/>
</rdf:Description>

<rdf:Description rdf:about="http://www.ontology-of-units-of-measure.org/resource/om-2/abfarad">
	<rdfs:isDefinedBy rdf:resource="http://www.ontology-of-units-of-measure.org/resource/om-2/"/>
</rdf:Description>

<rdf:Description rdf:about="http://www.ontology-of-units-of-measure.org/resource/om-2/farad">
	<rdfs:isDefinedBy rdf:resource="http://www.ontology-of-units-of-measure.org/resource/om-2/"/>
</rdf:Description>

<rdf:Description rdf:about="http://www.ontology-of-units-of-measure.org/resource/om-2/statfarad">
	<rdf:type rdf:resource="http://www.w3.org/2004/02/skos/core#Concept"/>
	<skos:inScheme rdf:resource="http://www.ontology-of-units-of-measure.org/resource/om-2/SingularUnit"/>
	<rdfs:comment xml:lang="en">The statfarad is a unit of capacitance defined as 1.112650e-12 farad.</rdfs:comment>
	<rdfs:label xml:lang="en">statfarad</rdfs:label>
	<hasUnit xmlns="http://www.ontology-of-units-of-measure.org/resource/om-2/" rdf:resource="http://www.ontology-of-units-of-measure.org/resource/om-2/farad"/>
	<rdfs:isDefinedBy rdf:resource="http://www.ontology-of-units-of-measure.org/resource/om-2/"/>
</rdf:Description>

<rdf:Description rdf:about="http://www.ontology-of-units-of-measure.org/resource/om-2/metreOfMercury">
	<rdf:type rdf:resource="http://www.w3.org/2004/02/skos/core#Concept"/>
	<skos:inScheme rdf:resource="http://www.ontology-of-units-of-measure.org/resource/om-2/SingularUnit"/>
	<rdfs:comment xml:lang="en">The metre of mercury is a unit of pressure defined as 133 322 pascal.</rdfs:comment>
	<rdfs:label xml:lang="en">metre of mercury</rdfs:label>
	<hasUnit xmlns="http://www.ontology-of-units-of-measure.org/resource/om-2/" rdf:resource="http://www.ontology-of-units-of-measure.org/resource/om-2/pascal"/>
	<rdfs:isDefinedBy rdf:resource="http://www.ontology-of-units-of-measure.org/resource/om-2/"/>
</rdf:Description>

<rdf:Description rdf:about="http://www.ontology-of-units-of-measure.org/resource/om-2/torr">
	<rdf:type rdf:resource="http://www.w3.org/2004/02/skos/core#Concept"/>
	<skos:inScheme rdf:resource="http://www.ontology-of-units-of-measure.org/resource/om-2/SingularUnit"/>
	<rdfs:comment xml:lang="en">The torr is a unit of pressure defined as 1.333224e2 pascal.</rdfs:comment>
	<rdfs:label xml:lang="en">torr</rdfs:label>
	<hasUnit xmlns="http://www.ontology-of-units-of-measure.org/resource/om-2/" rdf:resource="http://www.ontology-of-units-of-measure.org/resource/om-2/pascal"/>
	<rdfs:isDefinedBy rdf:resource="http://www.ontology-of-units-of-measure.org/resource/om-2/"/>
</rdf:Description>

<rdf:Description rdf:about="http://www.ontology-of-units-of-measure.org/resource/om-2/angstrom">
	<rdf:type rdf:resource="http://www.w3.org/2004/02/skos/core#Concept"/>
	<skos:inScheme rdf:resource="http://www.ontology-of-units-of-measure.org/resource/om-2/SingularUnit"/>
	<rdfs:comment xml:lang="en">The ångström is a unit of length defined as 1.0e-10 metre. The unit is often used for wavelengths of electromagnetic radiation or to express the sizes of atoms and molecules.</rdfs:comment>
	<rdfs:label xml:lang="en">ångström</rdfs:label>
	<hasUnit xmlns="http://www.ontology-of-units-of-measure.org/resource/om-2/" rdf:resource="http://www.ontology-of-units-of-measure.org/resource/om-2/metre"/>
	<rdfs:isDefinedBy rdf:resource="http://www.ontology-of-units-of-measure.org/resource/om-2/"/>
</rdf:Description>

<rdf:Description rdf:about="http://www.ontology-of-units-of-measure.org/resource/om-2/lightYear">
	<rdf:type rdf:resource="http://www.w3.org/2004/02/skos/core#Concept"/>
	<skos:inScheme rdf:resource="http://www.ontology-of-units-of-measure.org/resource/om-2/SingularUnit"/>
	<rdfs:comment xml:lang="en">The light year is a unit of length defined as 9.46073e15 metre.</rdfs:comment>
	<rdfs:label xml:lang="en">light year</rdfs:label>
	<hasUnit xmlns="http://www.ontology-of-units-of-measure.org/resource/om-2/" rdf:resource="http://www.ontology-of-units-of-measure.org/resource/om-2/metre"/>
	<rdfs:isDefinedBy rdf:resource="http://www.ontology-of-units-of-measure.org/resource/om-2/"/>
</rdf:Description>

<rdf:Description rdf:about="http://www.ontology-of-units-of-measure.org/resource/om-2/micron">
	<rdf:type rdf:resource="http://www.w3.org/2004/02/skos/core#Concept"/>
	<skos:inScheme rdf:resource="http://www.ontology-of-units-of-measure.org/resource/om-2/SingularUnit"/>
	<rdfs:comment xml:lang="en">The micron is a unit of length defined as 1.0e-6 metre.</rdfs:comment>
	<rdfs:label xml:lang="en">micron</rdfs:label>
	<hasUnit xmlns="http://www.ontology-of-units-of-measure.org/resource/om-2/" rdf:resource="http://www.ontology-of-units-of-measure.org/resource/om-2/metre"/>
	<rdfs:isDefinedBy rdf:resource="http://www.ontology-of-units-of-measure.org/resource/om-2/"/>
</rdf:Description>

<rdf:Description rdf:about="http://www.ontology-of-units-of-measure.org/resource/om-2/mil-Length">
	<rdf:type rdf:resource="http://www.w3.org/2004/02/skos/core#Concept"/>
	<skos:inScheme rdf:resource="http://www.ontology-of-units-of-measure.org/resource/om-2/SingularUnit"/>
	<rdfs:comment xml:lang="en">The mil (length) is a unit of length defined as 2.54e-5 metre.</rdfs:comment>
	<rdfs:label xml:lang="en">mil (length)</rdfs:label>
	<hasUnit xmlns="http://www.ontology-of-units-of-measure.org/resource/om-2/" rdf:resource="http://www.ontology-of-units-of-measure.org/resource/om-2/metre"/>
	<rdfs:isDefinedBy rdf:resource="http://www.ontology-of-units-of-measure.org/resource/om-2/"/>
</rdf:Description>

<rdf:Description rdf:about="http://www.ontology-of-units-of-measure.org/resource/om-2/mile-Statute">
	<rdf:type rdf:resource="http://www.w3.org/2004/02/skos/core#Concept"/>
	<skos:inScheme rdf:resource="http://www.ontology-of-units-of-measure.org/resource/om-2/SingularUnit"/>
	<rdfs:comment xml:lang="en">The statute mile is a unit of length defined as 1.609344e3 metre.</rdfs:comment>
	<rdfs:label xml:lang="en">mile (statute)</rdfs:label>
	<hasUnit xmlns="http://www.ontology-of-units-of-measure.org/resource/om-2/" rdf:resource="http://www.ontology-of-units-of-measure.org/resource/om-2/metre"/>
	<rdfs:isDefinedBy rdf:resource="http://www.ontology-of-units-of-measure.org/resource/om-2/"/>
</rdf:Description>

<rdf:Description rdf:about="http://www.ontology-of-units-of-measure.org/resource/om-2/mile-USSurvey">
	<rdf:type rdf:resource="http://www.w3.org/2004/02/skos/core#Concept"/>
	<skos:inScheme rdf:resource="http://www.ontology-of-units-of-measure.org/resource/om-2/SingularUnit"/>
	<rdfs:comment xml:lang="en">The US survey mile is a unit of length defined as 1.609347e3 metre.</rdfs:comment>
	<rdfs:label xml:lang="en">mile (US survey)</rdfs:label>
	<hasUnit xmlns="http://www.ontology-of-units-of-measure.org/resource/om-2/" rdf:resource="http://www.ontology-of-units-of-measure.org/resource/om-2/metre"/>
	<rdfs:isDefinedBy rdf:resource="http://www.ontology-of-units-of-measure.org/resource/om-2/"/>
</rdf:Description>

<rdf:Description rdf:about="http://www.ontology-of-units-of-measure.org/resource/om-2/point-Didot">
	<skos:inScheme rdf:resource="http://www.ontology-of-units-of-measure.org/resource/om-2/SingularUnit"/>
	<rdfs:comment xml:lang="en">The Didot point is a unit of length defined as 0.3759e-3 metre.</rdfs:comment>
	<rdfs:label xml:lang="en">point (Didot)</rdfs:label>
	<hasUnit xmlns="http://www.ontology-of-units-of-measure.org/resource/om-2/" rdf:resource="http://www.ontology-of-units-of-measure.org/resource/om-2/metre"/>
</rdf:Description>

<rdf:Description rdf:about="http://www.ontology-of-units-of-measure.org/resource/om-2/rod-US">
	<rdf:type rdf:resource="http://www.w3.org/2004/02/skos/core#Concept"/>
	<skos:inScheme rdf:resource="http://www.ontology-of-units-of-measure.org/resource/om-2/SingularUnit"/>
	<rdfs:comment xml:lang="en">The US rod is a unit of length defined as 5.029210 metre.</rdfs:comment>
	<rdfs:label xml:lang="en">rod (US)</rdfs:label>
	<hasUnit xmlns="http://www.ontology-of-units-of-measure.org/resource/om-2/" rdf:resource="http://www.ontology-of-units-of-measure.org/resource/om-2/metre"/>
	<rdfs:isDefinedBy rdf:resource="http://www.ontology-of-units-of-measure.org/resource/om-2/"/>
</rdf:Description>

<rdf:Description rdf:about="http://www.ontology-of-units-of-measure.org/resource/om-2/yard-International">
	<rdf:type rdf:resource="http://www.w3.org/2004/02/skos/core#Concept"/>
	<skos:inScheme rdf:resource="http://www.ontology-of-units-of-measure.org/resource/om-2/SingularUnit"/>
	<rdfs:comment xml:lang="en">The international yard is a unit of length defined as 9.144e-1 metre.</rdfs:comment>
	<rdfs:label xml:lang="en">yard (international)</rdfs:label>
	<hasUnit xmlns="http://www.ontology-of-units-of-measure.org/resource/om-2/" rdf:resource="http://www.ontology-of-units-of-measure.org/resource/om-2/metre"/>
	<rdfs:isDefinedBy rdf:resource="http://www.ontology-of-units-of-measure.org/resource/om-2/"/>
</rdf:Description>

<rdf:Description rdf:about="http://www.ontology-of-units-of-measure.org/resource/om-2/pound-Force">
	<rdf:type rdf:resource="http://www.w3.org/2004/02/skos/core#Concept"/>
	<skos:inScheme rdf:resource="http://www.ontology-of-units-of-measure.org/resource/om-2/SingularUnit"/>
	<rdfs:comment xml:lang="en">The pound-force is a unit of force defined as 4.448222 newton.</rdfs:comment>
	<rdfs:label xml:lang="en">pound-force</rdfs:label>
	<hasUnit xmlns="http://www.ontology-of-units-of-measure.org/resource/om-2/" rdf:resource="http://www.ontology-of-units-of-measure.org/resource/om-2/newton"/>
	<rdfs:isDefinedBy rdf:resource="http://www.ontology-of-units-of-measure.org/resource/om-2/"/>
</rdf:Description>

<rdf:Description rdf:about="http://www.ontology-of-units-of-measure.org/resource/om-2/poundal">
	<rdf:type rdf:resource="http://www.w3.org/2004/02/skos/core#Concept"/>
	<skos:inScheme rdf:resource="http://www.ontology-of-units-of-measure.org/resource/om-2/SingularUnit"/>
	<rdfs:comment xml:lang="en">The poundal is a unit of force defined as 1.382550e-1 newton.</rdfs:comment>
	<rdfs:label xml:lang="en">poundal</rdfs:label>
	<hasUnit xmlns="http://www.ontology-of-units-of-measure.org/resource/om-2/" rdf:resource="http://www.ontology-of-units-of-measure.org/resource/om-2/newton"/>
	<rdfs:isDefinedBy rdf:resource="http://www.ontology-of-units-of-measure.org/resource/om-2/"/>
</rdf:Description>

<rdf:Description rdf:about="http://www.ontology-of-units-of-measure.org/resource/om-2/ton-Force-Short">
	<rdf:type rdf:resource="http://www.w3.org/2004/02/skos/core#Concept"/>
	<skos:inScheme rdf:resource="http://www.ontology-of-units-of-measure.org/resource/om-2/SingularUnit"/>
	<rdfs:comment xml:lang="en">The short ton-force is a unit of force defined as 8.896443e3 newton.</rdfs:comment>
	<rdfs:label xml:lang="en">ton-force (short)</rdfs:label>
	<hasUnit xmlns="http://www.ontology-of-units-of-measure.org/resource/om-2/" rdf:resource="http://www.ontology-of-units-of-measure.org/resource/om-2/newton"/>
	<rdfs:isDefinedBy rdf:resource="http://www.ontology-of-units-of-measure.org/resource/om-2/"/>
</rdf:Description>

<rdf:Description rdf:about="http://www.ontology-of-units-of-measure.org/resource/om-2/abohm">
	<rdf:type rdf:resource="http://www.w3.org/2004/02/skos/core#Concept"/>
	<skos:inScheme rdf:resource="http://www.ontology-of-units-of-measure.org/resource/om-2/SingularUnit"/>
	<rdfs:comment xml:lang="en">The abohm is a unit of electrical resistance defined as 1.0e-9 ohm.</rdfs:comment>
	<rdfs:label xml:lang="en">abohm</rdfs:label>
	<hasUnit xmlns="http://www.ontology-of-units-of-measure.org/resource/om-2/" rdf:resource="http://www.ontology-of-units-of-measure.org/resource/om-2/ohm"/>
</rdf:Description>

<rdf:Description rdf:about="http://www.ontology-of-units-of-measure.org/resource/om-2/ohm">
	<rdf:type rdf:resource="http://www.w3.org/2004/02/skos/core#Concept"/>
</rdf:Description>

<rdf:Description rdf:about="http://www.ontology-of-units-of-measure.org/resource/om-2/abohm">
	<rdfs:isDefinedBy rdf:resource="http://www.ontology-of-units-of-measure.org/resource/om-2/"/>
</rdf:Description>

<rdf:Description rdf:about="http://www.ontology-of-units-of-measure.org/resource/om-2/ohm">
	<rdfs:isDefinedBy rdf:resource="http://www.ontology-of-units-of-measure.org/resource/om-2/"/>
</rdf:Description>

<rdf:Description rdf:about="http://www.ontology-of-units-of-measure.org/resource/om-2/statohm">
	<rdf:type rdf:resource="http://www.w3.org/2004/02/skos/core#Concept"/>
	<skos:inScheme rdf:resource="http://www.ontology-of-units-of-measure.org/resource/om-2/SingularUnit"/>
	<rdfs:comment xml:lang="en">The statohm is a unit of electrical resistance defined as 8.987552e11 ohm.</rdfs:comment>
	<rdfs:label xml:lang="en">statohm</rdfs:label>
	<hasUnit xmlns="http://www.ontology-of-units-of-measure.org/resource/om-2/" rdf:resource="http://www.ontology-of-units-of-measure.org/resource/om-2/ohm"/>
	<rdfs:isDefinedBy rdf:resource="http://www.ontology-of-units-of-measure.org/resource/om-2/"/>
</rdf:Description>

<rdf:Description rdf:about="http://www.ontology-of-units-of-measure.org/resource/om-2/magnitude">
	<rdf:type rdf:resource="http://www.w3.org/2004/02/skos/core#Concept"/>
	<skos:inScheme rdf:resource="http://www.ontology-of-units-of-measure.org/resource/om-2/SingularUnit"/>
	<rdfs:comment xml:lang="en">Eenheid waarmee de helderheid van sterren wordt aangegeven. Meestal wordt het symbool niet aangeduid (http://en.wikipedia.org/wiki/Magnitude_(astronomy)).</rdfs:comment>
	<rdfs:label xml:lang="en">magnitude</rdfs:label>
	<hasUnit xmlns="http://www.ontology-of-units-of-measure.org/resource/om-2/" rdf:resource="http://www.ontology-of-units-of-measure.org/resource/om-2/one"/>
	<rdfs:isDefinedBy rdf:resource="http://www.ontology-of-units-of-measure.org/resource/om-2/"/>
</rdf:Description>

<rdf:Description rdf:about="http://www.ontology-of-units-of-measure.org/resource/om-2/BritishThermalUnit-39F">
	<rdf:type rdf:resource="http://www.w3.org/2004/02/skos/core#Concept"/>
	<skos:inScheme rdf:resource="http://www.ontology-of-units-of-measure.org/resource/om-2/SingularUnit"/>
	<rdfs:comment xml:lang="en">The 39 °F British thermal unit is a unit of energy defined as 1.05967e3 joule.</rdfs:comment>
	<rdfs:label xml:lang="en">British thermal unit (39 °F)</rdfs:label>
	<hasUnit xmlns="http://www.ontology-of-units-of-measure.org/resource/om-2/" rdf:resource="http://www.ontology-of-units-of-measure.org/resource/om-2/joule"/>
	<rdfs:isDefinedBy rdf:resource="http://www.ontology-of-units-of-measure.org/resource/om-2/"/>
</rdf:Description>

<rdf:Description rdf:about="http://www.ontology-of-units-of-measure.org/resource/om-2/BritishThermalUnit-59F">
	<rdf:type rdf:resource="http://www.w3.org/2004/02/skos/core#Concept"/>
	<skos:inScheme rdf:resource="http://www.ontology-of-units-of-measure.org/resource/om-2/SingularUnit"/>
	<rdfs:comment xml:lang="en">The 59 °F British thermal unit is a unit of energy defined as 1.05480e3 joule.</rdfs:comment>
	<rdfs:label xml:lang="en">British thermal unit (59 °F)</rdfs:label>
	<hasUnit xmlns="http://www.ontology-of-units-of-measure.org/resource/om-2/" rdf:resource="http://www.ontology-of-units-of-measure.org/resource/om-2/joule"/>
	<rdfs:isDefinedBy rdf:resource="http://www.ontology-of-units-of-measure.org/resource/om-2/"/>
</rdf:Description>

<rdf:Description rdf:about="http://www.ontology-of-units-of-measure.org/resource/om-2/BritishThermalUnit-60F">
	<rdf:type rdf:resource="http://www.w3.org/2004/02/skos/core#Concept"/>
	<skos:inScheme rdf:resource="http://www.ontology-of-units-of-measure.org/resource/om-2/SingularUnit"/>
	<rdfs:comment xml:lang="en">The 60 °F British thermal unit is a unit of energy defined as 1.05468e3 joule.</rdfs:comment>
	<rdfs:label xml:lang="en">British thermal unit (60 °F)</rdfs:label>
	<hasUnit xmlns="http://www.ontology-of-units-of-measure.org/resource/om-2/" rdf:resource="http://www.ontology-of-units-of-measure.org/resource/om-2/joule"/>
	<rdfs:isDefinedBy rdf:resource="http://www.ontology-of-units-of-measure.org/resource/om-2/"/>
</rdf:Description>

<rdf:Description rdf:about="http://www.ontology-of-units-of-measure.org/resource/om-2/BritishThermalUnit-InternationalTable">
	<skos:inScheme rdf:resource="http://www.ontology-of-units-of-measure.org/resource/om-2/SingularUnit"/>
	<rdfs:comment xml:lang="en">The International Table British thermal unit is a unit of energy defined as 1.055056e3 joule.</rdfs:comment>
	<rdfs:label xml:lang="en">British thermal unit (International Table)</rdfs:label>
	<hasUnit xmlns="http://www.ontology-of-units-of-measure.org/resource/om-2/" rdf:resource="http://www.ontology-of-units-of-measure.org/resource/om-2/joule"/>
</rdf:Description>

<rdf:Description rdf:about="http://www.ontology-of-units-of-measure.org/resource/om-2/BritishThermalUnit-Mean">
	<rdf:type rdf:resource="http://www.w3.org/2004/02/skos/core#Concept"/>
	<skos:inScheme rdf:resource="http://www.ontology-of-units-of-measure.org/resource/om-2/SingularUnit"/>
	<rdfs:comment xml:lang="en">The mean British thermal unit is a unit of energy defined as 1.05587e3 joule.</rdfs:comment>
	<rdfs:label xml:lang="en">British thermal unit (mean)</rdfs:label>
	<hasUnit xmlns="http://www.ontology-of-units-of-measure.org/resource/om-2/" rdf:resource="http://www.ontology-of-units-of-measure.org/resource/om-2/joule"/>
	<rdfs:isDefinedBy rdf:resource="http://www.ontology-of-units-of-measure.org/resource/om-2/"/>
</rdf:Description>

<rdf:Description rdf:about="http://www.ontology-of-units-of-measure.org/resource/om-2/BritishThermalUnit-Thermochemical">
	<rdf:type rdf:resource="http://www.w3.org/2004/02/skos/core#Concept"/>
	<skos:inScheme rdf:resource="http://www.ontology-of-units-of-measure.org/resource/om-2/SingularUnit"/>
	<rdfs:comment xml:lang="en">The thermochemical British thermal unit is a unit of energy defined as 1.054350e3 joule.</rdfs:comment>
	<rdfs:label xml:lang="en">British thermal unit (thermochemical)</rdfs:label>
	<hasUnit xmlns="http://www.ontology-of-units-of-measure.org/resource/om-2/" rdf:resource="http://www.ontology-of-units-of-measure.org/resource/om-2/joule"/>
	<rdfs:isDefinedBy rdf:resource="http://www.ontology-of-units-of-measure.org/resource/om-2/"/>
</rdf:Description>

<rdf:Description rdf:about="http://www.ontology-of-units-of-measure.org/resource/om-2/circularMil">
	<rdf:type rdf:resource="http://www.w3.org/2004/02/skos/core#Concept"/>
	<skos:inScheme rdf:resource="http://www.ontology-of-units-of-measure.org/resource/om-2/SingularUnit"/>
	<rdfs:comment xml:lang="en">The cicular mil is a unit of area defined as 5.067075e-10 square metre.</rdfs:comment>
	<rdfs:label xml:lang="en">circular mil</rdfs:label>
	<rdfs:isDefinedBy rdf:resource="http://www.ontology-of-units-of-measure.org/resource/om-2/"/>
</rdf:Description>

<rdf:Description rdf:about="http://www.ontology-of-units-of-measure.org/resource/om-2/cord">
	<rdf:type rdf:resource="http://www.w3.org/2004/02/skos/core#Concept"/>
	<skos:inScheme rdf:resource="http://www.ontology-of-units-of-measure.org/resource/om-2/SingularUnit"/>
	<rdfs:comment xml:lang="en">The cord is a unit of volume defined as 3.624556 cubic metre.</rdfs:comment>
	<rdfs:label xml:lang="en">cord</rdfs:label>
	<rdfs:isDefinedBy rdf:resource="http://www.ontology-of-units-of-measure.org/resource/om-2/"/>
</rdf:Description>

<rdf:Description rdf:about="http://www.ontology-of-units-of-measure.org/resource/om-2/coulomb">
	<skos:inScheme rdf:resource="http://www.ontology-of-units-of-measure.org/resource/om-2/SingularUnit"/>
	<rdfs:comment xml:lang="en">The coulomb is a unit of electric charge defined as ampere times second = farad times volt.</rdfs:comment>
	<rdfs:label xml:lang="en">coulomb</rdfs:label>
</rdf:Description>

<rdf:Description rdf:about="http://www.ontology-of-units-of-measure.org/resource/om-2/cup-USCustomary">
	<rdf:type rdf:resource="http://www.w3.org/2004/02/skos/core#Concept"/>
	<skos:inScheme rdf:resource="http://www.ontology-of-units-of-measure.org/resource/om-2/SingularUnit"/>
	<rdfs:comment xml:lang="en">The US customary cup is a unit of volume defined as 2.365882e-4 cubic metre.</rdfs:comment>
	<rdfs:label xml:lang="en">cup (US customary)</rdfs:label>
	<rdfs:isDefinedBy rdf:resource="http://www.ontology-of-units-of-measure.org/resource/om-2/"/>
</rdf:Description>

<rdf:Description rdf:about="http://www.ontology-of-units-of-measure.org/resource/om-2/darcy">
	<rdf:type rdf:resource="http://www.w3.org/2004/02/skos/core#Concept"/>
	<skos:inScheme rdf:resource="http://www.ontology-of-units-of-measure.org/resource/om-2/SingularUnit"/>
	<rdfs:comment xml:lang="en">The darcy is a unit of area defined as 9.869233e-13 square metre.</rdfs:comment>
	<rdfs:label xml:lang="en">darcy</rdfs:label>
	<rdfs:isDefinedBy rdf:resource="http://www.ontology-of-units-of-measure.org/resource/om-2/"/>
</rdf:Description>

<rdf:Description rdf:about="http://www.ontology-of-units-of-measure.org/resource/om-2/debye">
	<rdf:type rdf:resource="http://www.w3.org/2004/02/skos/core#Concept"/>
	<skos:inScheme rdf:resource="http://www.ontology-of-units-of-measure.org/resource/om-2/SingularUnit"/>
	<rdfs:comment xml:lang="en">The debye is a unit of electric dipole moment defined as 3.33564e-30 coulomb metre.</rdfs:comment>
	<rdfs:label xml:lang="en">debye</rdfs:label>
	<rdfs:isDefinedBy rdf:resource="http://www.ontology-of-units-of-measure.org/resource/om-2/"/>
</rdf:Description>

<rdf:Description rdf:about="http://www.ontology-of-units-of-measure.org/resource/om-2/dryGallon-US">
	<rdf:type rdf:resource="http://www.w3.org/2004/02/skos/core#Concept"/>
	<skos:inScheme rdf:resource="http://www.ontology-of-units-of-measure.org/resource/om-2/SingularUnit"/>
	<rdfs:comment xml:lang="en">The US dry gallon is a unit of volume defined as 4.40488377086e-3 cubic metre.</rdfs:comment>
	<rdfs:label xml:lang="en">dry gallon (US)</rdfs:label>
	<rdfs:isDefinedBy rdf:resource="http://www.ontology-of-units-of-measure.org/resource/om-2/"/>
</rdf:Description>

<rdf:Description rdf:about="http://www.ontology-of-units-of-measure.org/resource/om-2/dryPint-US">
	<rdf:type rdf:resource="http://www.w3.org/2004/02/skos/core#Concept"/>
	<skos:inScheme rdf:resource="http://www.ontology-of-units-of-measure.org/resource/om-2/SingularUnit"/>
	<rdfs:comment xml:lang="en">The US dry pint is a unit of volume defined as 5.506105e-4 cubic metre.</rdfs:comment>
	<rdfs:label xml:lang="en">dry pint (US)</rdfs:label>
	<rdfs:isDefinedBy rdf:resource="http://www.ontology-of-units-of-measure.org/resource/om-2/"/>
</rdf:Description>

<rdf:Description rdf:about="http://www.ontology-of-units-of-measure.org/resource/om-2/dryQuart-US">
	<rdf:type rdf:resource="http://www.w3.org/2004/02/skos/core#Concept"/>
	<skos:inScheme rdf:resource="http://www.ontology-of-units-of-measure.org/resource/om-2/SingularUnit"/>
	<rdfs:comment xml:lang="en">The US dry quart is a unit of volume defined as 1.101221e-3 cubic metre.</rdfs:comment>
	<rdfs:label xml:lang="en">dry quart (US)</rdfs:label>
	<rdfs:isDefinedBy rdf:resource="http://www.ontology-of-units-of-measure.org/resource/om-2/"/>
</rdf:Description>

<rdf:Description rdf:about="http://www.ontology-of-units-of-measure.org/resource/om-2/farad">
	<skos:inScheme rdf:resource="http://www.ontology-of-units-of-measure.org/resource/om-2/SingularUnit"/>
	<rdfs:comment xml:lang="en">The farad is a unit of capacitance defined as ampere times second divided by volt = coulomb divided by volt = coulomb squared divided by joule = coulomb squared divided by newton times metre = second squared times coulomb squared divided by square metre times kilogram = second to the power 4 times ampere squared divided by square metre times kilogram.</rdfs:comment>
	<rdfs:label xml:lang="en">farad</rdfs:label>
</rdf:Description>

<rdf:Description rdf:about="http://www.ontology-of-units-of-measure.org/resource/om-2/fluidOunce-Imperial">
	<rdf:type rdf:resource="http://www.w3.org/2004/02/skos/core#Concept"/>
	<skos:inScheme rdf:resource="http://www.ontology-of-units-of-measure.org/resource/om-2/SingularUnit"/>
	<rdfs:comment xml:lang="en">The imperial fluid ounce is a unit of volume defined as 2.841306e-5 cubic metre.</rdfs:comment>
	<rdfs:label xml:lang="en">fluid ounce (imperial)</rdfs:label>
	<rdfs:isDefinedBy rdf:resource="http://www.ontology-of-units-of-measure.org/resource/om-2/"/>
</rdf:Description>

<rdf:Description rdf:about="http://www.ontology-of-units-of-measure.org/resource/om-2/fluidOunce-US">
	<rdf:type rdf:resource="http://www.w3.org/2004/02/skos/core#Concept"/>
	<skos:inScheme rdf:resource="http://www.ontology-of-units-of-measure.org/resource/om-2/SingularUnit"/>
	<rdfs:comment xml:lang="en">The US fluid ounce is a unit of volume defined as 2.957353e-5 cubic metre.</rdfs:comment>
	<rdfs:label xml:lang="en">fluid ounce (US)</rdfs:label>
	<rdfs:isDefinedBy rdf:resource="http://www.ontology-of-units-of-measure.org/resource/om-2/"/>
</rdf:Description>

<rdf:Description rdf:about="http://www.ontology-of-units-of-measure.org/resource/om-2/footlambert">
	<rdf:type rdf:resource="http://www.w3.org/2004/02/skos/core#Concept"/>
	<skos:inScheme rdf:resource="http://www.ontology-of-units-of-measure.org/resource/om-2/SingularUnit"/>
	<rdfs:comment xml:lang="en">The footlambert is a unit of luminance defined as 3.426259 candela per square metre.</rdfs:comment>
	<rdfs:label xml:lang="en">footlambert</rdfs:label>
	<rdfs:isDefinedBy rdf:resource="http://www.ontology-of-units-of-measure.org/resource/om-2/"/>
</rdf:Description>

<rdf:Description rdf:about="http://www.ontology-of-units-of-measure.org/resource/om-2/gal">
	<rdf:type rdf:resource="http://www.w3.org/2004/02/skos/core#Concept"/>
	<skos:inScheme rdf:resource="http://www.ontology-of-units-of-measure.org/resource/om-2/SingularUnit"/>
	<rdfs:comment xml:lang="en">The gal is a unit of acceleration defined as centimetre per second (time) squared.</rdfs:comment>
	<rdfs:label xml:lang="en">gal</rdfs:label>
	<rdfs:isDefinedBy rdf:resource="http://www.ontology-of-units-of-measure.org/resource/om-2/"/>
</rdf:Description>

<rdf:Description rdf:about="http://www.ontology-of-units-of-measure.org/resource/om-2/gallon-Imperial">
	<rdf:type rdf:resource="http://www.w3.org/2004/02/skos/core#Concept"/>
	<skos:inScheme rdf:resource="http://www.ontology-of-units-of-measure.org/resource/om-2/SingularUnit"/>
	<rdfs:comment xml:lang="en">The imperial gallon is a unit of volume defined as 4.54609e-3 cubic metre.</rdfs:comment>
	<rdfs:label xml:lang="en">gallon (imperial)</rdfs:label>
	<rdfs:isDefinedBy rdf:resource="http://www.ontology-of-units-of-measure.org/resource/om-2/"/>
</rdf:Description>

<rdf:Description rdf:about="http://www.ontology-of-units-of-measure.org/resource/om-2/gallon-US">
	<rdf:type rdf:resource="http://www.w3.org/2004/02/skos/core#Concept"/>
	<skos:inScheme rdf:resource="http://www.ontology-of-units-of-measure.org/resource/om-2/SingularUnit"/>
	<rdfs:comment xml:lang="en">The US gallon is a unit of volume defined as 3.785412e-3 cubic metre.</rdfs:comment>
	<rdfs:label xml:lang="en">gallon (US)</rdfs:label>
	<rdfs:isDefinedBy rdf:resource="http://www.ontology-of-units-of-measure.org/resource/om-2/"/>
</rdf:Description>

<rdf:Description rdf:about="http://www.ontology-of-units-of-measure.org/resource/om-2/gill-Imperial">
	<rdf:type rdf:resource="http://www.w3.org/2004/02/skos/core#Concept"/>
	<skos:inScheme rdf:resource="http://www.ontology-of-units-of-measure.org/resource/om-2/SingularUnit"/>
	<rdfs:comment xml:lang="en">The imperial gill is a unit of volume defined as 1.420653e-4 cubic metre.</rdfs:comment>
	<rdfs:label xml:lang="en">gill (imperial)</rdfs:label>
	<rdfs:isDefinedBy rdf:resource="http://www.ontology-of-units-of-measure.org/resource/om-2/"/>
</rdf:Description>

<rdf:Description rdf:about="http://www.ontology-of-units-of-measure.org/resource/om-2/gill-US">
	<rdf:type rdf:resource="http://www.w3.org/2004/02/skos/core#Concept"/>
	<skos:inScheme rdf:resource="http://www.ontology-of-units-of-measure.org/resource/om-2/SingularUnit"/>
	<rdfs:comment xml:lang="en">The US gill is a unit of volume defined as 1.182941e-4 cubic metre.</rdfs:comment>
	<rdfs:label xml:lang="en">gill (US)</rdfs:label>
	<rdfs:isDefinedBy rdf:resource="http://www.ontology-of-units-of-measure.org/resource/om-2/"/>
</rdf:Description>

<rdf:Description rdf:about="http://www.ontology-of-units-of-measure.org/resource/om-2/grain">
	<rdf:type rdf:resource="http://www.w3.org/2004/02/skos/core#Concept"/>
	<skos:inScheme rdf:resource="http://www.ontology-of-units-of-measure.org/resource/om-2/SingularUnit"/>
	<rdfs:comment xml:lang="en">The grain is a unit of mass defined as 6.479891e-5 kilogram.</rdfs:comment>
	<rdfs:label xml:lang="en">grain</rdfs:label>
	<rdfs:isDefinedBy rdf:resource="http://www.ontology-of-units-of-measure.org/resource/om-2/"/>
</rdf:Description>

<rdf:Description rdf:about="http://www.ontology-of-units-of-measure.org/resource/om-2/gram">
	<rdf:type rdf:resource="http://www.w3.org/2004/02/skos/core#Concept"/>
	<skos:inScheme rdf:resource="http://www.ontology-of-units-of-measure.org/resource/om-2/SingularUnit"/>
	<rdfs:comment xml:lang="en">The gram is a unit of mass defined as 1.0e-3 kilogram.</rdfs:comment>
	<rdfs:label xml:lang="en">gram</rdfs:label>
	<rdfs:isDefinedBy rdf:resource="http://www.ontology-of-units-of-measure.org/resource/om-2/"/>
</rdf:Description>

<rdf:Description rdf:about="http://www.ontology-of-units-of-measure.org/resource/om-2/hundredweight-British">
	<rdf:type rdf:resource="http://www.w3.org/2004/02/skos/core#Concept"/>
	<skos:inScheme rdf:resource="http://www.ontology-of-units-of-measure.org/resource/om-2/SingularUnit"/>
	<rdfs:comment xml:lang="en">The British hundredweight is a unit of mass defined as 5.080235e1 kilogram.</rdfs:comment>
	<rdfs:label xml:lang="en">hundredweight (British)</rdfs:label>
	<rdfs:isDefinedBy rdf:resource="http://www.ontology-of-units-of-measure.org/resource/om-2/"/>
</rdf:Description>

<rdf:Description rdf:about="http://www.ontology-of-units-of-measure.org/resource/om-2/hundredweight-US">
	<rdf:type rdf:resource="http://www.w3.org/2004/02/skos/core#Concept"/>
	<skos:inScheme rdf:resource="http://www.ontology-of-units-of-measure.org/resource/om-2/SingularUnit"/>
	<rdfs:comment xml:lang="en">The US hundredweight is a unit of mass defined as 4.535924e1 kilogram.</rdfs:comment>
	<rdfs:label xml:lang="en">hundredweight (US)</rdfs:label>
	<rdfs:isDefinedBy rdf:resource="http://www.ontology-of-units-of-measure.org/resource/om-2/"/>
</rdf:Description>

<rdf:Description rdf:about="http://www.ontology-of-units-of-measure.org/resource/om-2/joule">
	<skos:inScheme rdf:resource="http://www.ontology-of-units-of-measure.org/resource/om-2/SingularUnit"/>
	<rdfs:comment xml:lang="en">The joule is a unit of energy defined as kilogram times square metre divided by second squared.</rdfs:comment>
	<rdfs:label xml:lang="en">joule</rdfs:label>
</rdf:Description>

<rdf:Description rdf:about="http://www.ontology-of-units-of-measure.org/resource/om-2/katal">
	<rdf:type rdf:resource="http://www.w3.org/2004/02/skos/core#Concept"/>
	<skos:inScheme rdf:resource="http://www.ontology-of-units-of-measure.org/resource/om-2/SingularUnit"/>
	<rdfs:comment xml:lang="en">The katal is a unit of catalytic activity defined as mole divided by second.</rdfs:comment>
	<rdfs:label xml:lang="en">katal</rdfs:label>
	<rdfs:isDefinedBy rdf:resource="http://www.ontology-of-units-of-measure.org/resource/om-2/"/>
</rdf:Description>

<rdf:Description rdf:about="http://www.ontology-of-units-of-measure.org/resource/om-2/kayser">
	<rdf:type rdf:resource="http://www.w3.org/2004/02/skos/core#Concept"/>
	<skos:inScheme rdf:resource="http://www.ontology-of-units-of-measure.org/resource/om-2/SingularUnit"/>
	<rdfs:comment xml:lang="en">The kayser is a unit of wavenumber defined as 100 reciprocal metre.</rdfs:comment>
	<rdfs:label xml:lang="en">kayser</rdfs:label>
	<rdfs:isDefinedBy rdf:resource="http://www.ontology-of-units-of-measure.org/resource/om-2/"/>
</rdf:Description>

<rdf:Description rdf:about="http://www.ontology-of-units-of-measure.org/resource/om-2/SwissFranc">
	<rdf:type rdf:resource="http://www.w3.org/2004/02/skos/core#Concept"/>
	<skos:inScheme rdf:resource="http://www.ontology-of-units-of-measure.org/resource/om-2/SingularUnit"/>
	<rdfs:label xml:lang="en">Swiss franc</rdfs:label>
	<rdfs:isDefinedBy rdf:resource="http://www.ontology-of-units-of-measure.org/resource/om-2/"/>
</rdf:Description>

<rdf:Description rdf:about="http://www.ontology-of-units-of-measure.org/resource/om-2/TurkishLira">
	<rdf:type rdf:resource="http://www.w3.org/2004/02/skos/core#Concept"/>
	<skos:inScheme rdf:resource="http://www.ontology-of-units-of-measure.org/resource/om-2/SingularUnit"/>
	<rdfs:label xml:lang="en">Turkish lira</rdfs:label>
	<rdfs:isDefinedBy rdf:resource="http://www.ontology-of-units-of-measure.org/resource/om-2/"/>
</rdf:Description>

<rdf:Description rdf:about="http://www.ontology-of-units-of-measure.org/resource/om-2/UnitedStatesDollar">
	<rdf:type rdf:resource="http://www.w3.org/2004/02/skos/core#Concept"/>
	<skos:inScheme rdf:resource="http://www.ontology-of-units-of-measure.org/resource/om-2/SingularUnit"/>
	<rdfs:label xml:lang="en">United States dollar</rdfs:label>
	<rdfs:isDefinedBy rdf:resource="http://www.ontology-of-units-of-measure.org/resource/om-2/"/>
</rdf:Description>

<rdf:Description rdf:about="http://www.ontology-of-units-of-measure.org/resource/om-2/HongKongDollar">
	<rdf:type rdf:resource="http://www.w3.org/2004/02/skos/core#Concept"/>
	<skos:inScheme rdf:resource="http://www.ontology-of-units-of-measure.org/resource/om-2/SingularUnit"/>
	<rdfs:label xml:lang="en">Hong Kong dollar</rdfs:label>
	<rdfs:isDefinedBy rdf:resource="http://www.ontology-of-units-of-measure.org/resource/om-2/"/>
</rdf:Description>

<rdf:Description rdf:about="http://www.ontology-of-units-of-measure.org/resource/om-2/IndianRupee">
	<rdf:type rdf:resource="http://www.w3.org/2004/02/skos/core#Concept"/>
	<skos:inScheme rdf:resource="http://www.ontology-of-units-of-measure.org/resource/om-2/SingularUnit"/>
	<rdfs:label xml:lang="en">Indian rupee</rdfs:label>
	<rdfs:isDefinedBy rdf:resource="http://www.ontology-of-units-of-measure.org/resource/om-2/"/>
</rdf:Description>

<rdf:Description rdf:about="http://www.ontology-of-units-of-measure.org/resource/om-2/InternationalUnit">
	<rdf:type rdf:resource="http://www.w3.org/2004/02/skos/core#Concept"/>
	<skos:inScheme rdf:resource="http://www.ontology-of-units-of-measure.org/resource/om-2/SingularUnit"/>
	<rdfs:label xml:lang="en">International Unit</rdfs:label>
	<rdfs:isDefinedBy rdf:resource="http://www.ontology-of-units-of-measure.org/resource/om-2/"/>
</rdf:Description>

<rdf:Description rdf:about="http://www.ontology-of-units-of-measure.org/resource/om-2/jansky">
	<rdf:type rdf:resource="http://www.w3.org/2004/02/skos/core#Concept"/>
	<skos:inScheme rdf:resource="http://www.ontology-of-units-of-measure.org/resource/om-2/SingularUnit"/>
	<rdfs:label xml:lang="en">jansky</rdfs:label>
	<rdfs:isDefinedBy rdf:resource="http://www.ontology-of-units-of-measure.org/resource/om-2/"/>
</rdf:Description>

<rdf:Description rdf:about="http://www.ontology-of-units-of-measure.org/resource/om-2/JapaneseYen">
	<rdf:type rdf:resource="http://www.w3.org/2004/02/skos/core#Concept"/>
	<skos:inScheme rdf:resource="http://www.ontology-of-units-of-measure.org/resource/om-2/SingularUnit"/>
	<rdfs:label xml:lang="en">Japanese yen</rdfs:label>
	<rdfs:isDefinedBy rdf:resource="http://www.ontology-of-units-of-measure.org/resource/om-2/"/>
</rdf:Description>

<rdf:Description rdf:about="http://www.ontology-of-units-of-measure.org/resource/om-2/NewZealandDollar">
	<rdf:type rdf:resource="http://www.w3.org/2004/02/skos/core#Concept"/>
	<skos:inScheme rdf:resource="http://www.ontology-of-units-of-measure.org/resource/om-2/SingularUnit"/>
	<rdfs:label xml:lang="en">New Zealand dollar</rdfs:label>
	<rdfs:isDefinedBy rdf:resource="http://www.ontology-of-units-of-measure.org/resource/om-2/"/>
</rdf:Description>

<rdf:Description rdf:about="http://www.ontology-of-units-of-measure.org/resource/om-2/NorwegianKrone">
	<rdf:type rdf:resource="http://www.w3.org/2004/02/skos/core#Concept"/>
	<skos:inScheme rdf:resource="http://www.ontology-of-units-of-measure.org/resource/om-2/SingularUnit"/>
	<rdfs:label xml:lang="en">Norwegian krone</rdfs:label>
	<rdfs:isDefinedBy rdf:resource="http://www.ontology-of-units-of-measure.org/resource/om-2/"/>
</rdf:Description>

<rdf:Description rdf:about="http://www.ontology-of-units-of-measure.org/resource/om-2/SingaporeDollar">
	<rdf:type rdf:resource="http://www.w3.org/2004/02/skos/core#Concept"/>
	<skos:inScheme rdf:resource="http://www.ontology-of-units-of-measure.org/resource/om-2/SingularUnit"/>
	<rdfs:label xml:lang="en">Singapore dollar</rdfs:label>
	<rdfs:isDefinedBy rdf:resource="http://www.ontology-of-units-of-measure.org/resource/om-2/"/>
</rdf:Description>

<rdf:Description rdf:about="http://www.ontology-of-units-of-measure.org/resource/om-2/SouthAfricanRand">
	<rdf:type rdf:resource="http://www.w3.org/2004/02/skos/core#Concept"/>
	<skos:inScheme rdf:resource="http://www.ontology-of-units-of-measure.org/resource/om-2/SingularUnit"/>
	<rdfs:label xml:lang="en">South African rand</rdfs:label>
	<rdfs:isDefinedBy rdf:resource="http://www.ontology-of-units-of-measure.org/resource/om-2/"/>
</rdf:Description>

<rdf:Description rdf:about="http://www.ontology-of-units-of-measure.org/resource/om-2/deltaA450">
	<rdf:type rdf:resource="http://www.w3.org/2004/02/skos/core#Concept"/>
	<skos:inScheme rdf:resource="http://www.ontology-of-units-of-measure.org/resource/om-2/SingularUnit"/>
	<rdfs:label xml:lang="en">delta A450</rdfs:label>
	<rdfs:isDefinedBy rdf:resource="http://www.ontology-of-units-of-measure.org/resource/om-2/"/>
</rdf:Description>

<rdf:Description rdf:about="http://www.ontology-of-units-of-measure.org/resource/om-2/euro">
	<rdf:type rdf:resource="http://www.w3.org/2004/02/skos/core#Concept"/>
	<skos:inScheme rdf:resource="http://www.ontology-of-units-of-measure.org/resource/om-2/SingularUnit"/>
	<rdfs:label xml:lang="en">euro</rdfs:label>
	<rdfs:isDefinedBy rdf:resource="http://www.ontology-of-units-of-measure.org/resource/om-2/"/>
</rdf:Description>

<rdf:Description rdf:about="http://www.ontology-of-units-of-measure.org/resource/om-2/_0-100">
	<rdf:type rdf:resource="http://www.w3.org/2004/02/skos/core#Concept"/>
	<skos:inScheme rdf:resource="http://www.ontology-of-units-of-measure.org/resource/om-2/SingularUnit"/>
	<rdfs:label xml:lang="en">0-100</rdfs:label>
	<rdfs:isDefinedBy rdf:resource="http://www.ontology-of-units-of-measure.org/resource/om-2/"/>
</rdf:Description>

<rdf:Description rdf:about="http://www.ontology-of-units-of-measure.org/resource/om-2/_0-5">
	<rdf:type rdf:resource="http://www.w3.org/2004/02/skos/core#Concept"/>
	<skos:inScheme rdf:resource="http://www.ontology-of-units-of-measure.org/resource/om-2/SingularUnit"/>
	<rdfs:label xml:lang="en">0-5</rdfs:label>
	<rdfs:isDefinedBy rdf:resource="http://www.ontology-of-units-of-measure.org/resource/om-2/"/>
</rdf:Description>

<rdf:Description rdf:about="http://www.ontology-of-units-of-measure.org/resource/om-2/_1-0">
	<rdf:type rdf:resource="http://www.w3.org/2004/02/skos/core#Concept"/>
	<skos:inScheme rdf:resource="http://www.ontology-of-units-of-measure.org/resource/om-2/SingularUnit"/>
	<rdfs:label xml:lang="en">1/0</rdfs:label>
	<rdfs:isDefinedBy rdf:resource="http://www.ontology-of-units-of-measure.org/resource/om-2/"/>
</rdf:Description>

<rdf:Description rdf:about="http://www.ontology-of-units-of-measure.org/resource/om-2/_1-10">
	<rdf:type rdf:resource="http://www.w3.org/2004/02/skos/core#Concept"/>
	<skos:inScheme rdf:resource="http://www.ontology-of-units-of-measure.org/resource/om-2/SingularUnit"/>
	<rdfs:label xml:lang="en">1-10</rdfs:label>
	<rdfs:isDefinedBy rdf:resource="http://www.ontology-of-units-of-measure.org/resource/om-2/"/>
</rdf:Description>

<rdf:Description rdf:about="http://www.ontology-of-units-of-measure.org/resource/om-2/_1-5">
	<rdf:type rdf:resource="http://www.w3.org/2004/02/skos/core#Concept"/>
	<skos:inScheme rdf:resource="http://www.ontology-of-units-of-measure.org/resource/om-2/SingularUnit"/>
	<rdfs:label xml:lang="en">1-5</rdfs:label>
	<rdfs:isDefinedBy rdf:resource="http://www.ontology-of-units-of-measure.org/resource/om-2/"/>
</rdf:Description>

<rdf:Description rdf:about="http://www.ontology-of-units-of-measure.org/resource/om-2/AFS">
	<rdf:type rdf:resource="http://www.w3.org/2004/02/skos/core#Concept"/>
	<skos:inScheme rdf:resource="http://www.ontology-of-units-of-measure.org/resource/om-2/SingularUnit"/>
	<rdfs:label xml:lang="en">AFS</rdfs:label>
	<rdfs:isDefinedBy rdf:resource="http://www.ontology-of-units-of-measure.org/resource/om-2/"/>
</rdf:Description>

<rdf:Description rdf:about="http://www.ontology-of-units-of-measure.org/resource/om-2/AustralianDollar">
	<rdf:type rdf:resource="http://www.w3.org/2004/02/skos/core#Concept"/>
	<skos:inScheme rdf:resource="http://www.ontology-of-units-of-measure.org/resource/om-2/SingularUnit"/>
	<rdfs:label xml:lang="en">Australian dollar</rdfs:label>
	<rdfs:isDefinedBy rdf:resource="http://www.ontology-of-units-of-measure.org/resource/om-2/"/>
</rdf:Description>

<rdf:Description rdf:about="http://www.ontology-of-units-of-measure.org/resource/om-2/BrazilianReal">
	<rdf:type rdf:resource="http://www.w3.org/2004/02/skos/core#Concept"/>
	<skos:inScheme rdf:resource="http://www.ontology-of-units-of-measure.org/resource/om-2/SingularUnit"/>
	<rdfs:label xml:lang="en">Brazilian real</rdfs:label>
	<rdfs:isDefinedBy rdf:resource="http://www.ontology-of-units-of-measure.org/resource/om-2/"/>
</rdf:Description>

<rdf:Description rdf:about="http://www.ontology-of-units-of-measure.org/resource/om-2/CanadianDollar">
	<rdf:type rdf:resource="http://www.w3.org/2004/02/skos/core#Concept"/>
	<skos:inScheme rdf:resource="http://www.ontology-of-units-of-measure.org/resource/om-2/SingularUnit"/>
	<rdfs:label xml:lang="en">Canadian dollar</rdfs:label>
	<rdfs:isDefinedBy rdf:resource="http://www.ontology-of-units-of-measure.org/resource/om-2/"/>
</rdf:Description>

<rdf:Description rdf:about="http://www.ontology-of-units-of-measure.org/resource/om-2/ChineseYuan">
	<rdf:type rdf:resource="http://www.w3.org/2004/02/skos/core#Concept"/>
	<skos:inScheme rdf:resource="http://www.ontology-of-units-of-measure.org/resource/om-2/SingularUnit"/>
	<rdfs:label xml:lang="en">Chinese yuan</rdfs:label>
	<rdfs:isDefinedBy rdf:resource="http://www.ontology-of-units-of-measure.org/resource/om-2/"/>
</rdf:Description>

<rdf:Description rdf:about="http://www.ontology-of-units-of-measure.org/resource/om-2/colonyFormingUnit">
	<rdf:type rdf:resource="http://www.w3.org/2004/02/skos/core#Concept"/>
	<skos:inScheme rdf:resource="http://www.ontology-of-units-of-measure.org/resource/om-2/SingularUnit"/>
	<rdfs:label xml:lang="en">colony forming unit</rdfs:label>
	<rdfs:isDefinedBy rdf:resource="http://www.ontology-of-units-of-measure.org/resource/om-2/"/>
</rdf:Description>

<rdf:Description rdf:about="http://www.ontology-of-units-of-measure.org/resource/om-2/kelvin">
	<skos:inScheme rdf:resource="http://www.ontology-of-units-of-measure.org/resource/om-2/SingularUnit"/>
	<rdfs:comment xml:lang="en">The kelvin is a unit of temperature defined as 1/273.16 of the thermodynamic temperature of the triple point of water.</rdfs:comment>
	<rdfs:label xml:lang="en">kelvin</rdfs:label>
</rdf:Description>

<rdf:Description rdf:about="http://www.ontology-of-units-of-measure.org/resource/om-2/mole">
	<rdf:type rdf:resource="http://www.w3.org/2004/02/skos/core#Concept"/>
	<skos:inScheme rdf:resource="http://www.ontology-of-units-of-measure.org/resource/om-2/SingularUnit"/>
	<rdfs:comment xml:lang="en">The mole is a unit of amount of substance defined as the amount of substance of a system that contains as many elementary entities as there are atoms in 0.012 kilogram of carbon 12.</rdfs:comment>
	<rdfs:label xml:lang="en">mole</rdfs:label>
	<rdfs:isDefinedBy rdf:resource="http://www.ontology-of-units-of-measure.org/resource/om-2/"/>
</rdf:Description>

<rdf:Description rdf:about="http://www.ontology-of-units-of-measure.org/resource/om-2/month">
	<rdf:type rdf:resource="http://www.w3.org/2004/02/skos/core#Concept"/>
	<skos:inScheme rdf:resource="http://www.ontology-of-units-of-measure.org/resource/om-2/SingularUnit"/>
	<rdfs:comment xml:lang="en">The month is a unit of time.</rdfs:comment>
	<rdfs:label xml:lang="en">month</rdfs:label>
	<rdfs:isDefinedBy rdf:resource="http://www.ontology-of-units-of-measure.org/resource/om-2/"/>
</rdf:Description>

<rdf:Description rdf:about="http://www.ontology-of-units-of-measure.org/resource/om-2/newton">
	<skos:inScheme rdf:resource="http://www.ontology-of-units-of-measure.org/resource/om-2/SingularUnit"/>
	<rdfs:comment xml:lang="en">The newton is a unit of force defined as kilogram timesmetre divided by second squared.</rdfs:comment>
	<rdfs:label xml:lang="en">newton</rdfs:label>
</rdf:Description>

<rdf:Description rdf:about="http://www.ontology-of-units-of-measure.org/resource/om-2/oersted">
	<rdf:type rdf:resource="http://www.w3.org/2004/02/skos/core#Concept"/>
	<skos:inScheme rdf:resource="http://www.ontology-of-units-of-measure.org/resource/om-2/SingularUnit"/>
	<rdfs:comment xml:lang="en">The oersted is a unit of magnetic field defined as 7.957747e1 ampere per metre.</rdfs:comment>
	<rdfs:label xml:lang="en">oersted</rdfs:label>
	<rdfs:isDefinedBy rdf:resource="http://www.ontology-of-units-of-measure.org/resource/om-2/"/>
</rdf:Description>

<rdf:Description rdf:about="http://www.ontology-of-units-of-measure.org/resource/om-2/ohm">
	<skos:inScheme rdf:resource="http://www.ontology-of-units-of-measure.org/resource/om-2/SingularUnit"/>
	<rdfs:comment xml:lang="en">The ohm is a unit of electrical resistance defined as volt divided by ampere = square metre times kilogram divided by second to the power 3 times ampere squared.</rdfs:comment>
	<rdfs:label xml:lang="en">ohm</rdfs:label>
</rdf:Description>

<rdf:Description rdf:about="http://www.ontology-of-units-of-measure.org/resource/om-2/one">
	<skos:inScheme rdf:resource="http://www.ontology-of-units-of-measure.org/resource/om-2/SingularUnit"/>
	<rdfs:comment xml:lang="en">Unit one is a unit of dimension one.</rdfs:comment>
	<rdfs:label xml:lang="en">one</rdfs:label>
</rdf:Description>

<rdf:Description rdf:about="http://www.ontology-of-units-of-measure.org/resource/om-2/ounceApothecaries">
	<rdf:type rdf:resource="http://www.w3.org/2004/02/skos/core#Concept"/>
	<skos:inScheme rdf:resource="http://www.ontology-of-units-of-measure.org/resource/om-2/SingularUnit"/>
	<rdfs:comment xml:lang="en">The apothecaries' ounce is a unit of mass defined as 3.110348e-2 kilogram.</rdfs:comment>
	<rdfs:label xml:lang="en">ounce (apothecaries')</rdfs:label>
	<rdfs:isDefinedBy rdf:resource="http://www.ontology-of-units-of-measure.org/resource/om-2/"/>
</rdf:Description>

<rdf:Description rdf:about="http://www.ontology-of-units-of-measure.org/resource/om-2/ounceAvoirdupois">
	<rdf:type rdf:resource="http://www.w3.org/2004/02/skos/core#Concept"/>
	<skos:inScheme rdf:resource="http://www.ontology-of-units-of-measure.org/resource/om-2/SingularUnit"/>
	<rdfs:comment xml:lang="en">The avoirdupois ounce is a unit of mass defined as 2.834952e-2 kilogram.</rdfs:comment>
	<rdfs:label xml:lang="en">ounce (avoirdupois)</rdfs:label>
	<rdfs:isDefinedBy rdf:resource="http://www.ontology-of-units-of-measure.org/resource/om-2/"/>
</rdf:Description>

<rdf:Description rdf:about="http://www.ontology-of-units-of-measure.org/resource/om-2/pascal">
	<skos:inScheme rdf:resource="http://www.ontology-of-units-of-measure.org/resource/om-2/SingularUnit"/>
	<rdfs:comment xml:lang="en">The pascal is a unit of pressure and stress defined as newton divided by square metre = joule divided by cubic metre = kilogram divided by metre second squared.</rdfs:comment>
	<rdfs:label xml:lang="en">pascal</rdfs:label>
</rdf:Description>

<rdf:Description rdf:about="http://www.ontology-of-units-of-measure.org/resource/om-2/peck-US">
	<rdf:type rdf:resource="http://www.w3.org/2004/02/skos/core#Concept"/>
	<skos:inScheme rdf:resource="http://www.ontology-of-units-of-measure.org/resource/om-2/SingularUnit"/>
	<rdfs:comment xml:lang="en">The US peck is a unit of volume defined as 8.809768e-3 cubic metre.</rdfs:comment>
	<rdfs:label xml:lang="en">peck (US)</rdfs:label>
	<rdfs:isDefinedBy rdf:resource="http://www.ontology-of-units-of-measure.org/resource/om-2/"/>
</rdf:Description>

<rdf:Description rdf:about="http://www.ontology-of-units-of-measure.org/resource/om-2/pennyweight-Troy">
	<rdf:type rdf:resource="http://www.w3.org/2004/02/skos/core#Concept"/>
	<skos:inScheme rdf:resource="http://www.ontology-of-units-of-measure.org/resource/om-2/SingularUnit"/>
	<rdfs:comment xml:lang="en">The Troy pennyweight is a unit of mass defined as 1.555174e-3 kilogram.</rdfs:comment>
	<rdfs:label xml:lang="en">pennyweight (Troy)</rdfs:label>
	<rdfs:isDefinedBy rdf:resource="http://www.ontology-of-units-of-measure.org/resource/om-2/"/>
</rdf:Description>

<rdf:Description rdf:about="http://www.ontology-of-units-of-measure.org/resource/om-2/perm-0C">
	<rdf:type rdf:resource="http://www.w3.org/2004/02/skos/core#Concept"/>
	<skos:inScheme rdf:resource="http://www.ontology-of-units-of-measure.org/resource/om-2/SingularUnit"/>
	<rdfs:comment xml:lang="en">The 0 °C perm is a unit ofpermeance defined as 5.72135e-11 kilogram per pascal second (time) square metre.</rdfs:comment>
	<rdfs:label xml:lang="en">perm (0 °C)</rdfs:label>
	<rdfs:isDefinedBy rdf:resource="http://www.ontology-of-units-of-measure.org/resource/om-2/"/>
</rdf:Description>

<rdf:Description rdf:about="http://www.ontology-of-units-of-measure.org/resource/om-2/perm-23C">
	<rdf:type rdf:resource="http://www.w3.org/2004/02/skos/core#Concept"/>
	<skos:inScheme rdf:resource="http://www.ontology-of-units-of-measure.org/resource/om-2/SingularUnit"/>
	<rdfs:comment xml:lang="en">The 23 °C perm is a unit of permeance defined as 5.74525e-11 kilogram per pascal second (time) square metre.</rdfs:comment>
	<rdfs:label xml:lang="en">perm (23 °C)</rdfs:label>
	<rdfs:isDefinedBy rdf:resource="http://www.ontology-of-units-of-measure.org/resource/om-2/"/>
</rdf:Description>

<rdf:Description rdf:about="http://www.ontology-of-units-of-measure.org/resource/om-2/pint-Imperial">
	<rdf:type rdf:resource="http://www.w3.org/2004/02/skos/core#Concept"/>
	<skos:inScheme rdf:resource="http://www.ontology-of-units-of-measure.org/resource/om-2/SingularUnit"/>
	<rdfs:comment xml:lang="en">The pint is a unit of volume defined as 568.26125 millilitre.</rdfs:comment>
	<rdfs:label xml:lang="en">pint (imperial)</rdfs:label>
	<rdfs:isDefinedBy rdf:resource="http://www.ontology-of-units-of-measure.org/resource/om-2/"/>
</rdf:Description>

<rdf:Description rdf:about="http://www.ontology-of-units-of-measure.org/resource/om-2/siemens">
	<skos:inScheme rdf:resource="http://www.ontology-of-units-of-measure.org/resource/om-2/SingularUnit"/>
	<rdfs:comment xml:lang="en">The siemens is a unit of electrical conductance defined as 1 divided by ohm = ampere divided by volt = coulomb squared times second divided by kilogram times square metre = ampere squared times second to the power 3 divided by kilogram times square metre.</rdfs:comment>
	<rdfs:label xml:lang="en">siemens</rdfs:label>
</rdf:Description>

<rdf:Description rdf:about="http://www.ontology-of-units-of-measure.org/resource/om-2/sievert">
	<skos:inScheme rdf:resource="http://www.ontology-of-units-of-measure.org/resource/om-2/SingularUnit"/>
	<rdfs:comment xml:lang="en">The sievert is a unit of dose equivalent defined as joule divided by kilogram = square metre divided by second squared.</rdfs:comment>
	<rdfs:label xml:lang="en">sievert</rdfs:label>
</rdf:Description>

<rdf:Description rdf:about="http://www.ontology-of-units-of-measure.org/resource/om-2/slug">
	<rdf:type rdf:resource="http://www.w3.org/2004/02/skos/core#Concept"/>
	<skos:inScheme rdf:resource="http://www.ontology-of-units-of-measure.org/resource/om-2/SingularUnit"/>
	<rdfs:comment xml:lang="en">The slug is a unit of mass defined as 1.459390e1 kilogram.</rdfs:comment>
	<rdfs:label xml:lang="en">slug</rdfs:label>
	<rdfs:isDefinedBy rdf:resource="http://www.ontology-of-units-of-measure.org/resource/om-2/"/>
</rdf:Description>

<rdf:Description rdf:about="http://www.ontology-of-units-of-measure.org/resource/om-2/solarMass">
	<rdf:type rdf:resource="http://www.w3.org/2004/02/skos/core#Concept"/>
	<skos:inScheme rdf:resource="http://www.ontology-of-units-of-measure.org/resource/om-2/SingularUnit"/>
	<rdfs:comment xml:lang="en">Solar mass is a unit used in astronomy to denote stellar or galactic masses (http://en.wikipedia.org/wiki/SolarMass).</rdfs:comment>
	<rdfs:label xml:lang="en">solar mass</rdfs:label>
	<rdfs:isDefinedBy rdf:resource="http://www.ontology-of-units-of-measure.org/resource/om-2/"/>
</rdf:Description>

<rdf:Description rdf:about="http://www.ontology-of-units-of-measure.org/resource/om-2/MexicanPeso">
	<rdf:type rdf:resource="http://www.w3.org/2004/02/skos/core#Concept"/>
	<skos:inScheme rdf:resource="http://www.ontology-of-units-of-measure.org/resource/om-2/SingularUnit"/>
	<rdfs:label xml:lang="en">Mexican peso</rdfs:label>
	<rdfs:isDefinedBy rdf:resource="http://www.ontology-of-units-of-measure.org/resource/om-2/"/>
</rdf:Description>

<rdf:Description rdf:about="http://www.ontology-of-units-of-measure.org/resource/om-2/milligramRAE">
	<rdf:type rdf:resource="http://www.w3.org/2004/02/skos/core#Concept"/>
	<skos:inScheme rdf:resource="http://www.ontology-of-units-of-measure.org/resource/om-2/SingularUnit"/>
	<rdfs:label xml:lang="en">milligram RAE</rdfs:label>
	<rdfs:isDefinedBy rdf:resource="http://www.ontology-of-units-of-measure.org/resource/om-2/"/>
</rdf:Description>

<rdf:Description rdf:about="http://www.ontology-of-units-of-measure.org/resource/om-2/poundSterling">
	<rdf:type rdf:resource="http://www.w3.org/2004/02/skos/core#Concept"/>
	<skos:inScheme rdf:resource="http://www.ontology-of-units-of-measure.org/resource/om-2/SingularUnit"/>
	<rdfs:label xml:lang="en">pound sterling</rdfs:label>
	<rdfs:isDefinedBy rdf:resource="http://www.ontology-of-units-of-measure.org/resource/om-2/"/>
</rdf:Description>

<rdf:Description rdf:about="http://www.ontology-of-units-of-measure.org/resource/om-2/RussianRuble">
	<rdf:type rdf:resource="http://www.w3.org/2004/02/skos/core#Concept"/>
	<skos:inScheme rdf:resource="http://www.ontology-of-units-of-measure.org/resource/om-2/SingularUnit"/>
	<rdfs:label xml:lang="en">RussianRuble</rdfs:label>
	<rdfs:isDefinedBy rdf:resource="http://www.ontology-of-units-of-measure.org/resource/om-2/"/>
</rdf:Description>

<rdf:Description rdf:about="http://www.ontology-of-units-of-measure.org/resource/om-2/SouthKoreanWon">
	<rdf:type rdf:resource="http://www.w3.org/2004/02/skos/core#Concept"/>
	<skos:inScheme rdf:resource="http://www.ontology-of-units-of-measure.org/resource/om-2/SingularUnit"/>
	<rdfs:label xml:lang="en">South Korean won</rdfs:label>
	<rdfs:isDefinedBy rdf:resource="http://www.ontology-of-units-of-measure.org/resource/om-2/"/>
</rdf:Description>

<rdf:Description rdf:about="http://www.ontology-of-units-of-measure.org/resource/om-2/SwedishKrona">
	<rdf:type rdf:resource="http://www.w3.org/2004/02/skos/core#Concept"/>
	<skos:inScheme rdf:resource="http://www.ontology-of-units-of-measure.org/resource/om-2/SingularUnit"/>
	<rdfs:label xml:lang="en">Swedish krona</rdfs:label>
	<rdfs:isDefinedBy rdf:resource="http://www.ontology-of-units-of-measure.org/resource/om-2/"/>
</rdf:Description>

</rdf:RDF>