<?xml version="1.0" encoding="UTF-8"?>
<rdf:RDF
	xmlns:vann="http://purl.org/vocab/vann/"
	xmlns:voaf="http://purl.org/vocommons/voaf#"
	xmlns:rdfs="http://www.w3.org/2000/01/rdf-schema#"
	xmlns:owl="http://www.w3.org/2002/07/owl#"
	xmlns:skos="http://www.w3.org/2004/02/skos/core#"
	xmlns:rdf="http://www.w3.org/1999/02/22-rdf-syntax-ns#"
	xmlns:dcterms="http://purl.org/dc/terms/"
	xmlns:dc="http://purl.org/dc/elements/1.1/"
	xmlns:dcmit="http://purl.org/dc/dcmitype/"
	xmlns:sesame="http://www.openrdf.org/schema/sesame#"
	xmlns:xsd="http://www.w3.org/2001/XMLSchema#"
	xmlns:fn="http://www.w3.org/2005/xpath-functions#"
	xmlns:foaf="http://xmlns.com/foaf/0.1/"
	xmlns:hint="http://www.bigdata.com/queryHints#"
	xmlns:bd="http://www.bigdata.com/rdf#"
	xmlns:bds="http://www.bigdata.com/rdf/search#">

<rdf:Description rdf:about="http://www.ebusiness-unibw.org/ontologies/consumerelectronics/v1">
	<rdf:type rdf:resource="http://www.w3.org/2002/07/owl#Ontology"/>
</rdf:Description>

<rdf:Description rdf:about="http://www.ebusiness-unibw.org/ontologies/consumerelectronics/v1#DisplayType">
	<rdf:type rdf:resource="http://www.w3.org/2004/02/skos/core#ConceptScheme"/>
</rdf:Description>

<rdf:Description rdf:about="http://www.ebusiness-unibw.org/ontologies/consumerelectronics/v1#LCD">
	<rdf:type rdf:resource="http://www.w3.org/2004/02/skos/core#Concept"/>
	<skos:inScheme rdf:resource="http://www.ebusiness-unibw.org/ontologies/consumerelectronics/v1#DisplayType"/>
</rdf:Description>

<rdf:Description rdf:about="http://www.ebusiness-unibw.org/ontologies/consumerelectronics/v1#DisplayType">
	<rdfs:comment xml:lang="en">A display device is an output device for presentation of information for visual, tactile or auditive reception, acquired, stored, or transmitted in various forms.

(This description is partly based on or reuses content from the Wikipedia article "Display device" (http://en.wikipedia.org/wiki/Display_device) and is licensed under the GNU Free Documentation License (http://www.gnu.org/copyleft/fdl.html).)</rdfs:comment>
	<rdfs:label xml:lang="en">Display Type</rdfs:label>
</rdf:Description>

<rdf:Description rdf:about="http://www.ebusiness-unibw.org/ontologies/consumerelectronics/v1#LCD">
	<rdfs:comment xml:lang="en">A liquid crystal display (LCD) is an electronically-modulated optical device shaped into a thin, flat panel made up of any number of color or monochrome pixels filled with liquid crystals and arrayed in front of a light source (backlight) or reflector.

(This description is partly based on or reuses content from the Wikipedia article "Liquid crystal display" (http://en.wikipedia.org/wiki/Liquid_crystal_display) and is licensed under the GNU Free Documentation License (http://www.gnu.org/copyleft/fdl.html).)</rdfs:comment>
	<rdfs:label xml:lang="en">LCD</rdfs:label>
</rdf:Description>

<rdf:Description rdf:about="http://www.ebusiness-unibw.org/ontologies/consumerelectronics/v1#hasDisplayType">
	<rdfs:range rdf:resource="http://www.ebusiness-unibw.org/ontologies/consumerelectronics/v1#DisplayType"/>
	<rdfs:label xml:lang="en">display type</rdfs:label>
	<rdfs:comment xml:lang="en">Defines the type of the display like LCD or Plasma.</rdfs:comment>
	<rdf:type rdf:resource="http://www.w3.org/2002/07/owl#ObjectProperty"/>
</rdf:Description>

<rdf:Description rdf:about="http://www.ebusiness-unibw.org/ontologies/consumerelectronics/v1#DisplayType">
	<rdfs:isDefinedBy rdf:resource="http://www.ebusiness-unibw.org/ontologies/consumerelectronics/v1"/>
</rdf:Description>

<rdf:Description rdf:about="http://www.ebusiness-unibw.org/ontologies/consumerelectronics/v1#LCD">
	<rdfs:isDefinedBy rdf:resource="http://www.ebusiness-unibw.org/ontologies/consumerelectronics/v1"/>
</rdf:Description>

<rdf:Description rdf:about="http://www.ebusiness-unibw.org/ontologies/consumerelectronics/v1#Monochrome">
	<rdf:type rdf:resource="http://www.w3.org/2004/02/skos/core#Concept"/>
	<skos:inScheme rdf:resource="http://www.ebusiness-unibw.org/ontologies/consumerelectronics/v1#DisplayType"/>
	<rdfs:comment xml:lang="en">Ability to display just two colors (black/white).</rdfs:comment>
	<rdfs:label xml:lang="en">Monochrome</rdfs:label>
	<rdfs:isDefinedBy rdf:resource="http://www.ebusiness-unibw.org/ontologies/consumerelectronics/v1"/>
</rdf:Description>

<rdf:Description rdf:about="http://www.ebusiness-unibw.org/ontologies/consumerelectronics/v1#Multicolor">
	<rdf:type rdf:resource="http://www.w3.org/2004/02/skos/core#Concept"/>
	<skos:inScheme rdf:resource="http://www.ebusiness-unibw.org/ontologies/consumerelectronics/v1#DisplayType"/>
	<rdfs:comment xml:lang="en">Ability to display more than two different kinds of color.</rdfs:comment>
	<rdfs:label xml:lang="en">Multicolor</rdfs:label>
	<rdfs:isDefinedBy rdf:resource="http://www.ebusiness-unibw.org/ontologies/consumerelectronics/v1"/>
</rdf:Description>

<rdf:Description rdf:about="http://www.ebusiness-unibw.org/ontologies/consumerelectronics/v1#PDP">
	<rdf:type rdf:resource="http://www.w3.org/2004/02/skos/core#Concept"/>
	<skos:inScheme rdf:resource="http://www.ebusiness-unibw.org/ontologies/consumerelectronics/v1#DisplayType"/>
	<rdfs:comment xml:lang="en">A plasma display panel (PDP) is a type of flat panel display common to large TV displays (37in. [940mm]). Many tiny cells between two panels of glass hold an inert mixture of noble gases. The gas in the cells is electrically turned into a plasma which then excites phosphors to emit light.

(This description is partly based on or reuses content from the Wikipedia article "Digital newspaper technology - Plasma" (http://en.wikipedia.org/wiki/Digital_newspaper_technology#Plasma) and is licensed under the GNU Free Documentation License (http://www.gnu.org/copyleft/fdl.html).)</rdfs:comment>
	<rdfs:label xml:lang="en">PDP</rdfs:label>
	<rdfs:isDefinedBy rdf:resource="http://www.ebusiness-unibw.org/ontologies/consumerelectronics/v1"/>
</rdf:Description>

</rdf:RDF>