<?xml version="1.0" encoding="UTF-8"?>
<rdf:RDF
	xmlns:vann="http://purl.org/vocab/vann/"
	xmlns:voaf="http://purl.org/vocommons/voaf#"
	xmlns:rdfs="http://www.w3.org/2000/01/rdf-schema#"
	xmlns:owl="http://www.w3.org/2002/07/owl#"
	xmlns:skos="http://www.w3.org/2004/02/skos/core#"
	xmlns:rdf="http://www.w3.org/1999/02/22-rdf-syntax-ns#"
	xmlns:dcterms="http://purl.org/dc/terms/"
	xmlns:dc="http://purl.org/dc/elements/1.1/"
	xmlns:dcmit="http://purl.org/dc/dcmitype/"
	xmlns:sesame="http://www.openrdf.org/schema/sesame#"
	xmlns:xsd="http://www.w3.org/2001/XMLSchema#"
	xmlns:fn="http://www.w3.org/2005/xpath-functions#"
	xmlns:foaf="http://xmlns.com/foaf/0.1/"
	xmlns:hint="http://www.bigdata.com/queryHints#"
	xmlns:bd="http://www.bigdata.com/rdf#"
	xmlns:bds="http://www.bigdata.com/rdf/search#">

<rdf:Description rdf:about="http://data.doremus.org/ontology#">
	<rdf:type rdf:resource="http://www.w3.org/2002/07/owl#Ontology"/>
</rdf:Description>

<rdf:Description rdf:about="http://www.w3.org/2002/07/owl#SymmetricObjectProperty">
	<rdf:type rdf:resource="http://www.w3.org/2004/02/skos/core#ConceptScheme"/>
</rdf:Description>

<rdf:Description rdf:about="http://data.doremus.org/ontology#U83_has_relative_key">
	<rdf:type rdf:resource="http://www.w3.org/2004/02/skos/core#Concept"/>
	<skos:inScheme rdf:resource="http://www.w3.org/2002/07/owl#SymmetricObjectProperty"/>
	<rdfs:comment>see also http://en.wikipedia.org/wiki/Relative_key</rdfs:comment>
	<rdfs:label xml:lang="en">U83 has relative key</rdfs:label>
</rdf:Description>

<rdf:Description rdf:about="http://www.w3.org/2002/07/owl#SymmetricObjectProperty">
	<rdfs:isDefinedBy rdf:resource="http://data.doremus.org/ontology#"/>
</rdf:Description>

<rdf:Description rdf:about="http://data.doremus.org/ontology#U83_has_relative_key">
	<rdfs:isDefinedBy rdf:resource="http://data.doremus.org/ontology#"/>
	<rdfs:comment xml:lang="en">Examples: the key of 'C major' has 'A minor' as relative key</rdfs:comment>
	<rdfs:comment xml:lang="en">Scope Note: This class allows to connect two M4 Keys that are in a relative relationship, i.e. one is the relative major or minor of the other one.</rdfs:comment>
</rdf:Description>

<rdf:Description rdf:about="http://data.doremus.org/ontology#U84_has_parallel_key">
	<rdf:type rdf:resource="http://www.w3.org/2004/02/skos/core#Concept"/>
	<skos:inScheme rdf:resource="http://www.w3.org/2002/07/owl#SymmetricObjectProperty"/>
	<rdfs:comment>see also http://en.wikipedia.org/wiki/Parallel_key</rdfs:comment>
	<rdfs:label xml:lang="en">U84 has parallel key</rdfs:label>
	<rdfs:isDefinedBy rdf:resource="http://data.doremus.org/ontology#"/>
	<rdfs:comment xml:lang="en">Examples: the key of 'C major' has 'C minor' as parallel key</rdfs:comment>
	<rdfs:comment xml:lang="en">Scope Note: This class allows to connect two M4 Keys that are in a parallel relationship, i.e. one is the parallel major or minor of the other one.</rdfs:comment>
</rdf:Description>

<rdf:Description rdf:about="http://data.doremus.org/ontology#U85_has_closely_related_key">
	<rdf:type rdf:resource="http://www.w3.org/2004/02/skos/core#Concept"/>
	<skos:inScheme rdf:resource="http://www.w3.org/2002/07/owl#SymmetricObjectProperty"/>
	<rdfs:comment>see also http://en.wikipedia.org/wiki/Closely_related_key</rdfs:comment>
	<rdfs:label xml:lang="en">U85 has closely related key</rdfs:label>
	<rdfs:isDefinedBy rdf:resource="http://data.doremus.org/ontology#"/>
	<rdfs:comment xml:lang="en">Examples: the key of 'C major' has 'G major' and 'D minor' as closely related keys</rdfs:comment>
	<rdfs:comment xml:lang="en">Scope Note: This class allows to connect two M4 Keys that are mutually closely related from an harmonic point of view, e.g. they are commonly used destinations or transpositions in a modulation.</rdfs:comment>
</rdf:Description>

</rdf:RDF>