<?xml version="1.0" encoding="UTF-8"?>
<rdf:RDF
	xmlns:vann="http://purl.org/vocab/vann/"
	xmlns:voaf="http://purl.org/vocommons/voaf#"
	xmlns:rdfs="http://www.w3.org/2000/01/rdf-schema#"
	xmlns:owl="http://www.w3.org/2002/07/owl#"
	xmlns:skos="http://www.w3.org/2004/02/skos/core#"
	xmlns:rdf="http://www.w3.org/1999/02/22-rdf-syntax-ns#"
	xmlns:dcterms="http://purl.org/dc/terms/"
	xmlns:dc="http://purl.org/dc/elements/1.1/"
	xmlns:dcmit="http://purl.org/dc/dcmitype/"
	xmlns:sesame="http://www.openrdf.org/schema/sesame#"
	xmlns:xsd="http://www.w3.org/2001/XMLSchema#"
	xmlns:fn="http://www.w3.org/2005/xpath-functions#"
	xmlns:foaf="http://xmlns.com/foaf/0.1/"
	xmlns:hint="http://www.bigdata.com/queryHints#"
	xmlns:bd="http://www.bigdata.com/rdf#"
	xmlns:bds="http://www.bigdata.com/rdf/search#">

<rdf:Description rdf:about="http://www.ontology-of-units-of-measure.org/resource/om-2/">
	<rdf:type rdf:resource="http://www.w3.org/2002/07/owl#Ontology"/>
</rdf:Description>

<rdf:Description rdf:about="http://www.ontology-of-units-of-measure.org/resource/om-2/MolePerPrefixedLitre">
	<rdf:type rdf:resource="http://www.w3.org/2004/02/skos/core#ConceptScheme"/>
</rdf:Description>

<rdf:Description rdf:about="http://www.ontology-of-units-of-measure.org/resource/om-2/molePerAttolitre">
	<rdf:type rdf:resource="http://www.w3.org/2004/02/skos/core#Concept"/>
	<skos:inScheme rdf:resource="http://www.ontology-of-units-of-measure.org/resource/om-2/MolePerPrefixedLitre"/>
</rdf:Description>

<rdf:Description rdf:about="http://www.ontology-of-units-of-measure.org/resource/om-2/MolePerPrefixedLitre">
	<rdfs:label xml:lang="en">mole per prefixed litre</rdfs:label>
</rdf:Description>

<rdf:Description rdf:about="http://www.ontology-of-units-of-measure.org/resource/om-2/molePerAttolitre">
	<rdfs:comment xml:lang="en">Mole per attolitre is a unit of amount of substance concentration defined as mole divided by attolitre.</rdfs:comment>
	<rdfs:label xml:lang="en">mole per attolitre</rdfs:label>
</rdf:Description>

<rdf:Description rdf:about="http://www.ontology-of-units-of-measure.org/resource/om-2/MolePerPrefixedLitre">
	<rdfs:isDefinedBy rdf:resource="http://www.ontology-of-units-of-measure.org/resource/om-2/"/>
</rdf:Description>

<rdf:Description rdf:about="http://www.ontology-of-units-of-measure.org/resource/om-2/molePerAttolitre">
	<rdfs:isDefinedBy rdf:resource="http://www.ontology-of-units-of-measure.org/resource/om-2/"/>
</rdf:Description>

<rdf:Description rdf:about="http://www.ontology-of-units-of-measure.org/resource/om-2/molePerCentilitre">
	<rdf:type rdf:resource="http://www.w3.org/2004/02/skos/core#Concept"/>
	<skos:inScheme rdf:resource="http://www.ontology-of-units-of-measure.org/resource/om-2/MolePerPrefixedLitre"/>
	<rdfs:comment xml:lang="en">Mole per centilitre is a unit of amount of substance concentration defined as mole divided by centilitre.</rdfs:comment>
	<rdfs:label xml:lang="en">mole per centilitre</rdfs:label>
	<rdfs:isDefinedBy rdf:resource="http://www.ontology-of-units-of-measure.org/resource/om-2/"/>
</rdf:Description>

<rdf:Description rdf:about="http://www.ontology-of-units-of-measure.org/resource/om-2/molePerDecalitre">
	<rdf:type rdf:resource="http://www.w3.org/2004/02/skos/core#Concept"/>
	<skos:inScheme rdf:resource="http://www.ontology-of-units-of-measure.org/resource/om-2/MolePerPrefixedLitre"/>
	<rdfs:comment xml:lang="en">Mole per decalitre is a unit of amount of substance concentration defined as mole divided by decalitre.</rdfs:comment>
	<rdfs:label xml:lang="en">mole per decalitre</rdfs:label>
	<rdfs:isDefinedBy rdf:resource="http://www.ontology-of-units-of-measure.org/resource/om-2/"/>
</rdf:Description>

<rdf:Description rdf:about="http://www.ontology-of-units-of-measure.org/resource/om-2/molePerDecilitre">
	<rdf:type rdf:resource="http://www.w3.org/2004/02/skos/core#Concept"/>
	<skos:inScheme rdf:resource="http://www.ontology-of-units-of-measure.org/resource/om-2/MolePerPrefixedLitre"/>
	<rdfs:comment xml:lang="en">Mole per decilitre is a unit of amount of substance concentration defined as mole divided by decilitre.</rdfs:comment>
	<rdfs:label xml:lang="en">mole per decilitre</rdfs:label>
	<rdfs:isDefinedBy rdf:resource="http://www.ontology-of-units-of-measure.org/resource/om-2/"/>
</rdf:Description>

<rdf:Description rdf:about="http://www.ontology-of-units-of-measure.org/resource/om-2/molePerExalitre">
	<rdf:type rdf:resource="http://www.w3.org/2004/02/skos/core#Concept"/>
	<skos:inScheme rdf:resource="http://www.ontology-of-units-of-measure.org/resource/om-2/MolePerPrefixedLitre"/>
	<rdfs:comment xml:lang="en">Mole per exalitre is a unit of amount of substance concentration defined as mole divided by exalitre.</rdfs:comment>
	<rdfs:label xml:lang="en">mole per exalitre</rdfs:label>
	<rdfs:isDefinedBy rdf:resource="http://www.ontology-of-units-of-measure.org/resource/om-2/"/>
</rdf:Description>

<rdf:Description rdf:about="http://www.ontology-of-units-of-measure.org/resource/om-2/molePerFemtolitre">
	<rdf:type rdf:resource="http://www.w3.org/2004/02/skos/core#Concept"/>
	<skos:inScheme rdf:resource="http://www.ontology-of-units-of-measure.org/resource/om-2/MolePerPrefixedLitre"/>
	<rdfs:comment xml:lang="en">Mole per femtolitre is a unit of amount of substance concentration defined as mole divided by femtolitre.</rdfs:comment>
	<rdfs:label xml:lang="en">mole per femtolitre</rdfs:label>
	<rdfs:isDefinedBy rdf:resource="http://www.ontology-of-units-of-measure.org/resource/om-2/"/>
</rdf:Description>

<rdf:Description rdf:about="http://www.ontology-of-units-of-measure.org/resource/om-2/molePerGigalitre">
	<rdf:type rdf:resource="http://www.w3.org/2004/02/skos/core#Concept"/>
	<skos:inScheme rdf:resource="http://www.ontology-of-units-of-measure.org/resource/om-2/MolePerPrefixedLitre"/>
	<rdfs:comment xml:lang="en">Mole per gigalitre is a unit of amount of substance concentration defined as mole divided by gigalitre.</rdfs:comment>
	<rdfs:label xml:lang="en">mole per gigalitre</rdfs:label>
	<rdfs:isDefinedBy rdf:resource="http://www.ontology-of-units-of-measure.org/resource/om-2/"/>
</rdf:Description>

<rdf:Description rdf:about="http://www.ontology-of-units-of-measure.org/resource/om-2/molePerHectolitre">
	<rdf:type rdf:resource="http://www.w3.org/2004/02/skos/core#Concept"/>
	<skos:inScheme rdf:resource="http://www.ontology-of-units-of-measure.org/resource/om-2/MolePerPrefixedLitre"/>
	<rdfs:comment xml:lang="en">Mole per hectolitre is a unit of amount of substance concentration defined as mole divided by hectolitre.</rdfs:comment>
	<rdfs:label xml:lang="en">mole per hectolitre</rdfs:label>
	<rdfs:isDefinedBy rdf:resource="http://www.ontology-of-units-of-measure.org/resource/om-2/"/>
</rdf:Description>

<rdf:Description rdf:about="http://www.ontology-of-units-of-measure.org/resource/om-2/molePerKilolitre">
	<rdf:type rdf:resource="http://www.w3.org/2004/02/skos/core#Concept"/>
	<skos:inScheme rdf:resource="http://www.ontology-of-units-of-measure.org/resource/om-2/MolePerPrefixedLitre"/>
	<rdfs:comment xml:lang="en">Mole per kilolitre is a unit of amount of substance concentration defined as mole divided by kilolitre.</rdfs:comment>
	<rdfs:label xml:lang="en">mole per kilolitre</rdfs:label>
	<rdfs:isDefinedBy rdf:resource="http://www.ontology-of-units-of-measure.org/resource/om-2/"/>
</rdf:Description>

<rdf:Description rdf:about="http://www.ontology-of-units-of-measure.org/resource/om-2/molePerMegalitre">
	<rdf:type rdf:resource="http://www.w3.org/2004/02/skos/core#Concept"/>
	<skos:inScheme rdf:resource="http://www.ontology-of-units-of-measure.org/resource/om-2/MolePerPrefixedLitre"/>
	<rdfs:comment xml:lang="en">Mole per megalitre is a unit of amount of substance concentration defined as mole divided by megalitre.</rdfs:comment>
	<rdfs:label xml:lang="en">mole per megalitre</rdfs:label>
	<rdfs:isDefinedBy rdf:resource="http://www.ontology-of-units-of-measure.org/resource/om-2/"/>
</rdf:Description>

<rdf:Description rdf:about="http://www.ontology-of-units-of-measure.org/resource/om-2/molePerMicrolitre">
	<rdf:type rdf:resource="http://www.w3.org/2004/02/skos/core#Concept"/>
	<skos:inScheme rdf:resource="http://www.ontology-of-units-of-measure.org/resource/om-2/MolePerPrefixedLitre"/>
	<rdfs:comment xml:lang="en">Mole per microlitre is a unit of amount of substance concentration defined as mole divided by microlitre.</rdfs:comment>
	<rdfs:label xml:lang="en">mole per microlitre</rdfs:label>
	<rdfs:isDefinedBy rdf:resource="http://www.ontology-of-units-of-measure.org/resource/om-2/"/>
</rdf:Description>

<rdf:Description rdf:about="http://www.ontology-of-units-of-measure.org/resource/om-2/molePerMillilitre">
	<rdf:type rdf:resource="http://www.w3.org/2004/02/skos/core#Concept"/>
	<skos:inScheme rdf:resource="http://www.ontology-of-units-of-measure.org/resource/om-2/MolePerPrefixedLitre"/>
	<rdfs:comment xml:lang="en">Mole per millilitre is a unit of amount of substance concentration defined as mole divided by millilitre.</rdfs:comment>
	<rdfs:label xml:lang="en">mole per millilitre</rdfs:label>
	<rdfs:isDefinedBy rdf:resource="http://www.ontology-of-units-of-measure.org/resource/om-2/"/>
</rdf:Description>

<rdf:Description rdf:about="http://www.ontology-of-units-of-measure.org/resource/om-2/molePerNanolitre">
	<rdf:type rdf:resource="http://www.w3.org/2004/02/skos/core#Concept"/>
	<skos:inScheme rdf:resource="http://www.ontology-of-units-of-measure.org/resource/om-2/MolePerPrefixedLitre"/>
	<rdfs:comment xml:lang="en">Mole per nanolitre is a unit of amount of substance concentration defined as mole divided by nanolitre.</rdfs:comment>
	<rdfs:label xml:lang="en">mole per nanolitre</rdfs:label>
	<rdfs:isDefinedBy rdf:resource="http://www.ontology-of-units-of-measure.org/resource/om-2/"/>
</rdf:Description>

<rdf:Description rdf:about="http://www.ontology-of-units-of-measure.org/resource/om-2/molePerPetalitre">
	<rdf:type rdf:resource="http://www.w3.org/2004/02/skos/core#Concept"/>
	<skos:inScheme rdf:resource="http://www.ontology-of-units-of-measure.org/resource/om-2/MolePerPrefixedLitre"/>
	<rdfs:comment xml:lang="en">Mole per petalitre is a unit of amount of substance concentration defined as mole divided by petalitre.</rdfs:comment>
	<rdfs:label xml:lang="en">mole per petalitre</rdfs:label>
	<rdfs:isDefinedBy rdf:resource="http://www.ontology-of-units-of-measure.org/resource/om-2/"/>
</rdf:Description>

<rdf:Description rdf:about="http://www.ontology-of-units-of-measure.org/resource/om-2/molePerPicolitre">
	<rdf:type rdf:resource="http://www.w3.org/2004/02/skos/core#Concept"/>
	<skos:inScheme rdf:resource="http://www.ontology-of-units-of-measure.org/resource/om-2/MolePerPrefixedLitre"/>
	<rdfs:comment xml:lang="en">Mole per picolitre is a unit of amount of substance concentration defined as mole divided by picolitre.</rdfs:comment>
	<rdfs:label xml:lang="en">mole per picolitre</rdfs:label>
	<rdfs:isDefinedBy rdf:resource="http://www.ontology-of-units-of-measure.org/resource/om-2/"/>
</rdf:Description>

<rdf:Description rdf:about="http://www.ontology-of-units-of-measure.org/resource/om-2/molePerTeralitre">
	<rdf:type rdf:resource="http://www.w3.org/2004/02/skos/core#Concept"/>
	<skos:inScheme rdf:resource="http://www.ontology-of-units-of-measure.org/resource/om-2/MolePerPrefixedLitre"/>
	<rdfs:comment xml:lang="en">Mole per teralitre is a unit of amount of substance concentration defined as mole divided by teralitre.</rdfs:comment>
	<rdfs:label xml:lang="en">mole per teralitre</rdfs:label>
	<rdfs:isDefinedBy rdf:resource="http://www.ontology-of-units-of-measure.org/resource/om-2/"/>
</rdf:Description>

<rdf:Description rdf:about="http://www.ontology-of-units-of-measure.org/resource/om-2/molePerYoctolitre">
	<rdf:type rdf:resource="http://www.w3.org/2004/02/skos/core#Concept"/>
	<skos:inScheme rdf:resource="http://www.ontology-of-units-of-measure.org/resource/om-2/MolePerPrefixedLitre"/>
	<rdfs:comment xml:lang="en">Mole per yoctolitre is a unit of amount of substance concentration defined as mole divided by yoctolitre.</rdfs:comment>
	<rdfs:label xml:lang="en">mole per yoctolitre</rdfs:label>
	<rdfs:isDefinedBy rdf:resource="http://www.ontology-of-units-of-measure.org/resource/om-2/"/>
</rdf:Description>

<rdf:Description rdf:about="http://www.ontology-of-units-of-measure.org/resource/om-2/molePerYottalitre">
	<rdf:type rdf:resource="http://www.w3.org/2004/02/skos/core#Concept"/>
	<skos:inScheme rdf:resource="http://www.ontology-of-units-of-measure.org/resource/om-2/MolePerPrefixedLitre"/>
	<rdfs:comment xml:lang="en">Mole per yottalitre is a unit of amount of substance concentration defined as mole divided by yottalitre.</rdfs:comment>
	<rdfs:label xml:lang="en">mole per yottalitre</rdfs:label>
	<rdfs:isDefinedBy rdf:resource="http://www.ontology-of-units-of-measure.org/resource/om-2/"/>
</rdf:Description>

<rdf:Description rdf:about="http://www.ontology-of-units-of-measure.org/resource/om-2/molePerZeptolitre">
	<rdf:type rdf:resource="http://www.w3.org/2004/02/skos/core#Concept"/>
	<skos:inScheme rdf:resource="http://www.ontology-of-units-of-measure.org/resource/om-2/MolePerPrefixedLitre"/>
	<rdfs:comment xml:lang="en">Mole per zeptolitre is a unit of amount of substance concentration defined as mole divided by zeptolitre.</rdfs:comment>
	<rdfs:label xml:lang="en">mole per zeptolitre</rdfs:label>
	<rdfs:isDefinedBy rdf:resource="http://www.ontology-of-units-of-measure.org/resource/om-2/"/>
</rdf:Description>

<rdf:Description rdf:about="http://www.ontology-of-units-of-measure.org/resource/om-2/molePerZettalitre">
	<rdf:type rdf:resource="http://www.w3.org/2004/02/skos/core#Concept"/>
	<skos:inScheme rdf:resource="http://www.ontology-of-units-of-measure.org/resource/om-2/MolePerPrefixedLitre"/>
	<rdfs:comment xml:lang="en">Mole per zettalitre is a unit of amount of substance concentration defined as mole divided by zettalitre.</rdfs:comment>
	<rdfs:label xml:lang="en">mole per zettalitre</rdfs:label>
	<rdfs:isDefinedBy rdf:resource="http://www.ontology-of-units-of-measure.org/resource/om-2/"/>
</rdf:Description>

</rdf:RDF>