<?xml version="1.0" encoding="UTF-8"?>
<rdf:RDF
	xmlns:vann="http://purl.org/vocab/vann/"
	xmlns:voaf="http://purl.org/vocommons/voaf#"
	xmlns:rdfs="http://www.w3.org/2000/01/rdf-schema#"
	xmlns:owl="http://www.w3.org/2002/07/owl#"
	xmlns:skos="http://www.w3.org/2004/02/skos/core#"
	xmlns:rdf="http://www.w3.org/1999/02/22-rdf-syntax-ns#"
	xmlns:dcterms="http://purl.org/dc/terms/"
	xmlns:dc="http://purl.org/dc/elements/1.1/"
	xmlns:dcmit="http://purl.org/dc/dcmitype/"
	xmlns:sesame="http://www.openrdf.org/schema/sesame#"
	xmlns:xsd="http://www.w3.org/2001/XMLSchema#"
	xmlns:fn="http://www.w3.org/2005/xpath-functions#"
	xmlns:foaf="http://xmlns.com/foaf/0.1/"
	xmlns:hint="http://www.bigdata.com/queryHints#"
	xmlns:bd="http://www.bigdata.com/rdf#"
	xmlns:bds="http://www.bigdata.com/rdf/search#">

<rdf:Description rdf:about="https://w3id.org/cdc">
	<rdf:type rdf:resource="http://www.w3.org/2002/07/owl#Ontology"/>
</rdf:Description>

<rdf:Description rdf:about="https://w3id.org/cdc#DistributionRole">
	<rdf:type rdf:resource="http://www.w3.org/2004/02/skos/core#ConceptScheme"/>
</rdf:Description>

<rdf:Description rdf:about="https://w3id.org/cdc#complementLink">
	<rdf:type rdf:resource="http://www.w3.org/2004/02/skos/core#Concept"/>
	<skos:inScheme rdf:resource="https://w3id.org/cdc#DistributionRole"/>
</rdf:Description>

<rdf:Description rdf:about="https://w3id.org/cdc#DistributionRole">
	<rdfs:comment xml:lang="en">A distribution role defines the kind of qualified relation between two dataset distributions.</rdfs:comment>
	<rdfs:label xml:lang="en">distribution role</rdfs:label>
</rdf:Description>

<rdf:Description rdf:about="https://w3id.org/cdc#complementLink">
	<rdfs:comment xml:lang="en">A role of a qualified relation between a distribution of a dataset B that complements another dataset A, where the source distribution (subject of cdc:qualifiedDistributionRelation) complements the target dataset (object of dcterms:relation). The intermediate node between the distribution of dataset B and dataset A has a property cdc:hadDistributionRole pointing to cdc:complementLink. 

When the dataset B is the result of both additions and deletions on dataset A, dataset B should have a direct distribution with two subdistributions (cdc:hasSubDistribution): one containing triples to be deleted (cdc:DeletetionDistribution) from the source dataset and another containing triples that should be added (cdc:AdditionDistribution) to the source dataset. The qualified relation described above is established between the direct distribution of dataset B and dataset A .</rdfs:comment>
	<rdfs:label xml:lang="en">complement link</rdfs:label>
</rdf:Description>

<rdf:Description rdf:about="https://w3id.org/cdc#hadDistributionRole">
	<rdfs:range rdf:resource="https://w3id.org/cdc#DistributionRole"/>
	<rdfs:domain rdf:resource="https://w3id.org/cdc#DistributionRelation"/>
	<rdfs:label xml:lang="en">had distribution role</rdfs:label>
	<rdfs:comment xml:lang="en">A property to connect an instance of cdc:DistributionRelation to an instance of cdc:DistributionRole. The object of this property defines the type of the qualified distribution relation (cdc:qualifiedDistributionRelation) between a source distribution and another target DCAT entity.</rdfs:comment>
	<rdf:type rdf:resource="http://www.w3.org/2002/07/owl#ObjectProperty"/>
</rdf:Description>

<rdf:Description rdf:about="https://w3id.org/cdc#DistributionRole">
	<rdfs:isDefinedBy rdf:resource="https://w3id.org/cdc"/>
</rdf:Description>

<rdf:Description rdf:about="https://w3id.org/cdc#complementLink">
	<rdfs:isDefinedBy rdf:resource="https://w3id.org/cdc"/>
</rdf:Description>

<rdf:Description rdf:about="https://w3id.org/cdc#copiedDistributionLink">
	<rdf:type rdf:resource="http://www.w3.org/2004/02/skos/core#Concept"/>
	<skos:inScheme rdf:resource="https://w3id.org/cdc#DistributionRole"/>
	<rdfs:comment xml:lang="en">By connecting this node to a cdc:DistributionRelation instance, the source distribution (subject of cdc:qualifiedDistributionRelation) is marked as a copy of the target distribution (object of dcterms:relation).</rdfs:comment>
	<rdfs:label xml:lang="en">copied distribution of link</rdfs:label>
	<rdfs:isDefinedBy rdf:resource="https://w3id.org/cdc"/>
</rdf:Description>

<rdf:Description rdf:about="https://w3id.org/cdc#standaloneLink">
	<rdf:type rdf:resource="http://www.w3.org/2004/02/skos/core#Concept"/>
	<skos:inScheme rdf:resource="https://w3id.org/cdc#DistributionRole"/>
	<rdfs:comment xml:lang="en">A role of a qualified relation between a standalone distribution (cdc:StandaloneDistribution) and a complementing distribution (cdc:AdditionDistribution, cdc:DeletionDistribution or cdc:AdditionAndDeletionDistribution) of the same dataset.</rdfs:comment>
	<rdfs:label xml:lang="en">standalone link</rdfs:label>
	<rdfs:isDefinedBy rdf:resource="https://w3id.org/cdc"/>
</rdf:Description>

</rdf:RDF>