<?xml version="1.0" encoding="UTF-8"?>
<rdf:RDF
	xmlns:vann="http://purl.org/vocab/vann/"
	xmlns:voaf="http://purl.org/vocommons/voaf#"
	xmlns:rdfs="http://www.w3.org/2000/01/rdf-schema#"
	xmlns:owl="http://www.w3.org/2002/07/owl#"
	xmlns:skos="http://www.w3.org/2004/02/skos/core#"
	xmlns:rdf="http://www.w3.org/1999/02/22-rdf-syntax-ns#"
	xmlns:dcterms="http://purl.org/dc/terms/"
	xmlns:dc="http://purl.org/dc/elements/1.1/"
	xmlns:dcmit="http://purl.org/dc/dcmitype/"
	xmlns:sesame="http://www.openrdf.org/schema/sesame#"
	xmlns:xsd="http://www.w3.org/2001/XMLSchema#"
	xmlns:fn="http://www.w3.org/2005/xpath-functions#"
	xmlns:foaf="http://xmlns.com/foaf/0.1/"
	xmlns:hint="http://www.bigdata.com/queryHints#"
	xmlns:bd="http://www.bigdata.com/rdf#"
	xmlns:bds="http://www.bigdata.com/rdf/search#">

<rdf:Description rdf:about="http://www.ontology-of-units-of-measure.org/resource/om-2/">
	<rdf:type rdf:resource="http://www.w3.org/2002/07/owl#Ontology"/>
</rdf:Description>

<rdf:Description rdf:about="http://www.ontology-of-units-of-measure.org/resource/om-2/PrefixedMolePerLitre">
	<rdf:type rdf:resource="http://www.w3.org/2004/02/skos/core#ConceptScheme"/>
</rdf:Description>

<rdf:Description rdf:about="http://www.ontology-of-units-of-measure.org/resource/om-2/attomolePerLitre">
	<rdf:type rdf:resource="http://www.w3.org/2004/02/skos/core#Concept"/>
	<skos:inScheme rdf:resource="http://www.ontology-of-units-of-measure.org/resource/om-2/PrefixedMolePerLitre"/>
</rdf:Description>

<rdf:Description rdf:about="http://www.ontology-of-units-of-measure.org/resource/om-2/PrefixedMolePerLitre">
	<rdfs:label xml:lang="en">prefixed mole per litre</rdfs:label>
</rdf:Description>

<rdf:Description rdf:about="http://www.ontology-of-units-of-measure.org/resource/om-2/attomolePerLitre">
	<rdfs:comment xml:lang="en">Attomole per litre is a unit of amount of substance concentration defined as attomole divided by litre.</rdfs:comment>
	<rdfs:label xml:lang="en">attomole per litre</rdfs:label>
</rdf:Description>

<rdf:Description rdf:about="http://www.ontology-of-units-of-measure.org/resource/om-2/PrefixedMolePerLitre">
	<rdfs:isDefinedBy rdf:resource="http://www.ontology-of-units-of-measure.org/resource/om-2/"/>
</rdf:Description>

<rdf:Description rdf:about="http://www.ontology-of-units-of-measure.org/resource/om-2/attomolePerLitre">
	<rdfs:isDefinedBy rdf:resource="http://www.ontology-of-units-of-measure.org/resource/om-2/"/>
</rdf:Description>

<rdf:Description rdf:about="http://www.ontology-of-units-of-measure.org/resource/om-2/centimolePerLitre">
	<rdf:type rdf:resource="http://www.w3.org/2004/02/skos/core#Concept"/>
	<skos:inScheme rdf:resource="http://www.ontology-of-units-of-measure.org/resource/om-2/PrefixedMolePerLitre"/>
	<rdfs:comment xml:lang="en">Centimole per litre is a unit of amount of substance concentration defined as centimole divided by litre.</rdfs:comment>
	<rdfs:label xml:lang="en">centimole per litre</rdfs:label>
	<rdfs:isDefinedBy rdf:resource="http://www.ontology-of-units-of-measure.org/resource/om-2/"/>
</rdf:Description>

<rdf:Description rdf:about="http://www.ontology-of-units-of-measure.org/resource/om-2/decamolePerLitre">
	<rdf:type rdf:resource="http://www.w3.org/2004/02/skos/core#Concept"/>
	<skos:inScheme rdf:resource="http://www.ontology-of-units-of-measure.org/resource/om-2/PrefixedMolePerLitre"/>
	<rdfs:comment xml:lang="en">Decamole per litre is a unit of amount of substance concentration defined as decamole divided by litre.</rdfs:comment>
	<rdfs:label xml:lang="en">decamole per litre</rdfs:label>
	<rdfs:isDefinedBy rdf:resource="http://www.ontology-of-units-of-measure.org/resource/om-2/"/>
</rdf:Description>

<rdf:Description rdf:about="http://www.ontology-of-units-of-measure.org/resource/om-2/decimolePerLitre">
	<rdf:type rdf:resource="http://www.w3.org/2004/02/skos/core#Concept"/>
	<skos:inScheme rdf:resource="http://www.ontology-of-units-of-measure.org/resource/om-2/PrefixedMolePerLitre"/>
	<rdfs:comment xml:lang="en">Decimole per litre is a unit of amount of substance concentration defined as decimole divided by litre.</rdfs:comment>
	<rdfs:label xml:lang="en">decimole per litre</rdfs:label>
	<rdfs:isDefinedBy rdf:resource="http://www.ontology-of-units-of-measure.org/resource/om-2/"/>
</rdf:Description>

<rdf:Description rdf:about="http://www.ontology-of-units-of-measure.org/resource/om-2/examolePerLitre">
	<rdf:type rdf:resource="http://www.w3.org/2004/02/skos/core#Concept"/>
	<skos:inScheme rdf:resource="http://www.ontology-of-units-of-measure.org/resource/om-2/PrefixedMolePerLitre"/>
	<rdfs:comment xml:lang="en">Examole per litre is a unit of amount of substance concentration defined as examole divided by litre.</rdfs:comment>
	<rdfs:label xml:lang="en">examole per litre</rdfs:label>
	<rdfs:isDefinedBy rdf:resource="http://www.ontology-of-units-of-measure.org/resource/om-2/"/>
</rdf:Description>

<rdf:Description rdf:about="http://www.ontology-of-units-of-measure.org/resource/om-2/femtomolePerLitre">
	<rdf:type rdf:resource="http://www.w3.org/2004/02/skos/core#Concept"/>
	<skos:inScheme rdf:resource="http://www.ontology-of-units-of-measure.org/resource/om-2/PrefixedMolePerLitre"/>
	<rdfs:comment xml:lang="en">Femtomole per litre is a unit of amount of substance concentration defined as femtomole divided by litre.</rdfs:comment>
	<rdfs:label xml:lang="en">femtomole per litre</rdfs:label>
	<rdfs:isDefinedBy rdf:resource="http://www.ontology-of-units-of-measure.org/resource/om-2/"/>
</rdf:Description>

<rdf:Description rdf:about="http://www.ontology-of-units-of-measure.org/resource/om-2/gigamolePerLitre">
	<rdf:type rdf:resource="http://www.w3.org/2004/02/skos/core#Concept"/>
	<skos:inScheme rdf:resource="http://www.ontology-of-units-of-measure.org/resource/om-2/PrefixedMolePerLitre"/>
	<rdfs:comment xml:lang="en">Gigamole per litre is a unit of amount of substance concentration defined as gigamole divided by litre.</rdfs:comment>
	<rdfs:label xml:lang="en">gigamole per litre</rdfs:label>
	<rdfs:isDefinedBy rdf:resource="http://www.ontology-of-units-of-measure.org/resource/om-2/"/>
</rdf:Description>

<rdf:Description rdf:about="http://www.ontology-of-units-of-measure.org/resource/om-2/hectomolePerLitre">
	<rdf:type rdf:resource="http://www.w3.org/2004/02/skos/core#Concept"/>
	<skos:inScheme rdf:resource="http://www.ontology-of-units-of-measure.org/resource/om-2/PrefixedMolePerLitre"/>
	<rdfs:comment xml:lang="en">Hectomole per litre is a unit of amount of substance concentration defined as hectomole divided by litre.</rdfs:comment>
	<rdfs:label xml:lang="en">hectomole per litre</rdfs:label>
	<rdfs:isDefinedBy rdf:resource="http://www.ontology-of-units-of-measure.org/resource/om-2/"/>
</rdf:Description>

<rdf:Description rdf:about="http://www.ontology-of-units-of-measure.org/resource/om-2/kilomolePerLitre">
	<rdf:type rdf:resource="http://www.w3.org/2004/02/skos/core#Concept"/>
	<skos:inScheme rdf:resource="http://www.ontology-of-units-of-measure.org/resource/om-2/PrefixedMolePerLitre"/>
	<rdfs:comment xml:lang="en">Kilomole per litre is a unit of amount of substance concentration defined as kilomole divided by litre.</rdfs:comment>
	<rdfs:label xml:lang="en">kilomole per litre</rdfs:label>
	<rdfs:isDefinedBy rdf:resource="http://www.ontology-of-units-of-measure.org/resource/om-2/"/>
</rdf:Description>

<rdf:Description rdf:about="http://www.ontology-of-units-of-measure.org/resource/om-2/megamolePerLitre">
	<rdf:type rdf:resource="http://www.w3.org/2004/02/skos/core#Concept"/>
	<skos:inScheme rdf:resource="http://www.ontology-of-units-of-measure.org/resource/om-2/PrefixedMolePerLitre"/>
	<rdfs:comment xml:lang="en">Megamole per litre is a unit of amount of substance concentration defined as megamole divided by litre.</rdfs:comment>
	<rdfs:label xml:lang="en">megamole per litre</rdfs:label>
	<rdfs:isDefinedBy rdf:resource="http://www.ontology-of-units-of-measure.org/resource/om-2/"/>
</rdf:Description>

<rdf:Description rdf:about="http://www.ontology-of-units-of-measure.org/resource/om-2/micromolePerLitre">
	<rdf:type rdf:resource="http://www.w3.org/2004/02/skos/core#Concept"/>
	<skos:inScheme rdf:resource="http://www.ontology-of-units-of-measure.org/resource/om-2/PrefixedMolePerLitre"/>
	<rdfs:comment xml:lang="en">Micromole per litre is a unit of amount of substance concentration defined as micromole divided by litre.</rdfs:comment>
	<rdfs:label xml:lang="en">micromole per litre</rdfs:label>
	<rdfs:isDefinedBy rdf:resource="http://www.ontology-of-units-of-measure.org/resource/om-2/"/>
</rdf:Description>

<rdf:Description rdf:about="http://www.ontology-of-units-of-measure.org/resource/om-2/millimolePerLitre">
	<rdf:type rdf:resource="http://www.w3.org/2004/02/skos/core#Concept"/>
	<skos:inScheme rdf:resource="http://www.ontology-of-units-of-measure.org/resource/om-2/PrefixedMolePerLitre"/>
	<rdfs:comment xml:lang="en">Millimole per litre is a unit of amount of substance concentration defined as millimole divided by litre.</rdfs:comment>
	<rdfs:label xml:lang="en">millimole per litre</rdfs:label>
	<rdfs:isDefinedBy rdf:resource="http://www.ontology-of-units-of-measure.org/resource/om-2/"/>
</rdf:Description>

<rdf:Description rdf:about="http://www.ontology-of-units-of-measure.org/resource/om-2/nanomolePerLitre">
	<rdf:type rdf:resource="http://www.w3.org/2004/02/skos/core#Concept"/>
	<skos:inScheme rdf:resource="http://www.ontology-of-units-of-measure.org/resource/om-2/PrefixedMolePerLitre"/>
	<rdfs:comment xml:lang="en">Nanomole per litre is a unit of amount of substance concentration defined as nanomole divided by litre.</rdfs:comment>
	<rdfs:label xml:lang="en">nanomole per litre</rdfs:label>
	<rdfs:isDefinedBy rdf:resource="http://www.ontology-of-units-of-measure.org/resource/om-2/"/>
</rdf:Description>

<rdf:Description rdf:about="http://www.ontology-of-units-of-measure.org/resource/om-2/petamolePerLitre">
	<rdf:type rdf:resource="http://www.w3.org/2004/02/skos/core#Concept"/>
	<skos:inScheme rdf:resource="http://www.ontology-of-units-of-measure.org/resource/om-2/PrefixedMolePerLitre"/>
	<rdfs:comment xml:lang="en">Petamole per litre is a unit of amount of substance concentration defined as petamole divided by litre.</rdfs:comment>
	<rdfs:label xml:lang="en">petamole per litre</rdfs:label>
	<rdfs:isDefinedBy rdf:resource="http://www.ontology-of-units-of-measure.org/resource/om-2/"/>
</rdf:Description>

<rdf:Description rdf:about="http://www.ontology-of-units-of-measure.org/resource/om-2/picomolePerLitre">
	<rdf:type rdf:resource="http://www.w3.org/2004/02/skos/core#Concept"/>
	<skos:inScheme rdf:resource="http://www.ontology-of-units-of-measure.org/resource/om-2/PrefixedMolePerLitre"/>
	<rdfs:comment xml:lang="en">Picomole per litre is a unit of amount of substance concentration defined as picomole divided by litre.</rdfs:comment>
	<rdfs:label xml:lang="en">picomole per litre</rdfs:label>
	<rdfs:isDefinedBy rdf:resource="http://www.ontology-of-units-of-measure.org/resource/om-2/"/>
</rdf:Description>

<rdf:Description rdf:about="http://www.ontology-of-units-of-measure.org/resource/om-2/teramolePerLitre">
	<rdf:type rdf:resource="http://www.w3.org/2004/02/skos/core#Concept"/>
	<skos:inScheme rdf:resource="http://www.ontology-of-units-of-measure.org/resource/om-2/PrefixedMolePerLitre"/>
	<rdfs:comment xml:lang="en">Teramole per litre is a unit of amount of substance concentration defined as teramole divided by litre.</rdfs:comment>
	<rdfs:label xml:lang="en">teramole per litre</rdfs:label>
	<rdfs:isDefinedBy rdf:resource="http://www.ontology-of-units-of-measure.org/resource/om-2/"/>
</rdf:Description>

<rdf:Description rdf:about="http://www.ontology-of-units-of-measure.org/resource/om-2/yoctomolePerLitre">
	<rdf:type rdf:resource="http://www.w3.org/2004/02/skos/core#Concept"/>
	<skos:inScheme rdf:resource="http://www.ontology-of-units-of-measure.org/resource/om-2/PrefixedMolePerLitre"/>
	<rdfs:comment xml:lang="en">Yoctomole per litre is a unit of amount of substance concentration defined as yoctomole divided by litre.</rdfs:comment>
	<rdfs:label xml:lang="en">yoctomole per litre</rdfs:label>
	<rdfs:isDefinedBy rdf:resource="http://www.ontology-of-units-of-measure.org/resource/om-2/"/>
</rdf:Description>

<rdf:Description rdf:about="http://www.ontology-of-units-of-measure.org/resource/om-2/yottamolePerLitre">
	<rdf:type rdf:resource="http://www.w3.org/2004/02/skos/core#Concept"/>
	<skos:inScheme rdf:resource="http://www.ontology-of-units-of-measure.org/resource/om-2/PrefixedMolePerLitre"/>
	<rdfs:comment xml:lang="en">Yottamole per litre is a unit of amount of substance concentration defined as yottamole divided by litre.</rdfs:comment>
	<rdfs:label xml:lang="en">yottamole per litre</rdfs:label>
	<rdfs:isDefinedBy rdf:resource="http://www.ontology-of-units-of-measure.org/resource/om-2/"/>
</rdf:Description>

<rdf:Description rdf:about="http://www.ontology-of-units-of-measure.org/resource/om-2/zeptomolePerLitre">
	<rdf:type rdf:resource="http://www.w3.org/2004/02/skos/core#Concept"/>
	<skos:inScheme rdf:resource="http://www.ontology-of-units-of-measure.org/resource/om-2/PrefixedMolePerLitre"/>
	<rdfs:comment xml:lang="en">Zeptomole per litre is a unit of amount of substance concentration defined as zeptomole divided by litre.</rdfs:comment>
	<rdfs:label xml:lang="en">zeptomole per litre</rdfs:label>
	<rdfs:isDefinedBy rdf:resource="http://www.ontology-of-units-of-measure.org/resource/om-2/"/>
</rdf:Description>

<rdf:Description rdf:about="http://www.ontology-of-units-of-measure.org/resource/om-2/zettamolePerLitre">
	<rdf:type rdf:resource="http://www.w3.org/2004/02/skos/core#Concept"/>
	<skos:inScheme rdf:resource="http://www.ontology-of-units-of-measure.org/resource/om-2/PrefixedMolePerLitre"/>
	<rdfs:comment xml:lang="en">Zettamole per litre is a unit of amount of substance concentration defined as zettamole divided by litre.</rdfs:comment>
	<rdfs:label xml:lang="en">zettamole per litre</rdfs:label>
	<rdfs:isDefinedBy rdf:resource="http://www.ontology-of-units-of-measure.org/resource/om-2/"/>
</rdf:Description>

</rdf:RDF>