<?xml version="1.0" encoding="UTF-8"?>
<rdf:RDF
	xmlns:vann="http://purl.org/vocab/vann/"
	xmlns:voaf="http://purl.org/vocommons/voaf#"
	xmlns:rdfs="http://www.w3.org/2000/01/rdf-schema#"
	xmlns:owl="http://www.w3.org/2002/07/owl#"
	xmlns:skos="http://www.w3.org/2004/02/skos/core#"
	xmlns:rdf="http://www.w3.org/1999/02/22-rdf-syntax-ns#"
	xmlns:dcterms="http://purl.org/dc/terms/"
	xmlns:dc="http://purl.org/dc/elements/1.1/"
	xmlns:dcmit="http://purl.org/dc/dcmitype/"
	xmlns:sesame="http://www.openrdf.org/schema/sesame#"
	xmlns:xsd="http://www.w3.org/2001/XMLSchema#"
	xmlns:fn="http://www.w3.org/2005/xpath-functions#"
	xmlns:foaf="http://xmlns.com/foaf/0.1/"
	xmlns:hint="http://www.bigdata.com/queryHints#"
	xmlns:bd="http://www.bigdata.com/rdf#"
	xmlns:bds="http://www.bigdata.com/rdf/search#">

<rdf:Description rdf:about="http://purl.org/ontology/mo/">
	<rdf:type rdf:resource="http://www.w3.org/2002/07/owl#Ontology"/>
</rdf:Description>

<rdf:Description rdf:about="http://purl.org/ontology/mo/ReleaseType">
	<rdf:type rdf:resource="http://www.w3.org/2004/02/skos/core#ConceptScheme"/>
</rdf:Description>

<rdf:Description rdf:about="http://purl.org/ontology/mo/album">
	<rdf:type rdf:resource="http://www.w3.org/2004/02/skos/core#Concept"/>
	<skos:inScheme rdf:resource="http://purl.org/ontology/mo/ReleaseType"/>
</rdf:Description>

<rdf:Description rdf:about="http://purl.org/ontology/mo/ReleaseType">
	<rdfs:comment>
        Release type of a particular manifestation, such as "album" or "interview"...
    </rdfs:comment>
	<rdfs:label>Release type</rdfs:label>
</rdf:Description>

<rdf:Description rdf:about="http://purl.org/ontology/mo/album">
	<rdfs:comment>
        One or more track issued together.
            This is a type of MusicalManifestation defined by the musical industry.
    </rdfs:comment>
	<rdfs:label>album</rdfs:label>
</rdf:Description>

<rdf:Description rdf:about="http://purl.org/ontology/mo/release_type">
	<rdfs:range rdf:resource="http://purl.org/ontology/mo/ReleaseType"/>
	<rdfs:domain rdf:resource="http://purl.org/ontology/mo/MusicalManifestation"/>
	<rdfs:comment>
        Relates a musical manifestation to its release type (interview, spoken word, album, ...)
    </rdfs:comment>
	<rdf:type rdf:resource="http://www.w3.org/2002/07/owl#ObjectProperty"/>
</rdf:Description>

<rdf:Description rdf:about="http://purl.org/ontology/mo/ReleaseType">
	<rdfs:isDefinedBy rdf:resource="http://purl.org/ontology/mo/"/>
</rdf:Description>

<rdf:Description rdf:about="http://purl.org/ontology/mo/album">
	<rdfs:isDefinedBy rdf:resource="http://purl.org/ontology/mo/"/>
</rdf:Description>

<rdf:Description rdf:about="http://purl.org/ontology/mo/audiobook">
	<rdf:type rdf:resource="http://www.w3.org/2004/02/skos/core#Concept"/>
	<skos:inScheme rdf:resource="http://purl.org/ontology/mo/ReleaseType"/>
	<rdfs:comment>
        Book read by a narrator without music.
        This is a type of MusicalManifestation defined by the musical industry.
    </rdfs:comment>
	<rdfs:label>audio book</rdfs:label>
	<rdfs:isDefinedBy rdf:resource="http://purl.org/ontology/mo/"/>
</rdf:Description>

<rdf:Description rdf:about="http://purl.org/ontology/mo/compilation">
	<rdf:type rdf:resource="http://www.w3.org/2004/02/skos/core#Concept"/>
	<skos:inScheme rdf:resource="http://purl.org/ontology/mo/ReleaseType"/>
	<rdfs:comment>
        Collection of previously released manifestations of a musical expression by one or more artists.
        This is a type of MusicalManifestation defined by the musical industry.
    </rdfs:comment>
	<rdfs:label>compilation</rdfs:label>
	<rdfs:isDefinedBy rdf:resource="http://purl.org/ontology/mo/"/>
</rdf:Description>

<rdf:Description rdf:about="http://purl.org/ontology/mo/ep">
	<rdf:type rdf:resource="http://www.w3.org/2004/02/skos/core#Concept"/>
	<skos:inScheme rdf:resource="http://purl.org/ontology/mo/ReleaseType"/>
	<rdfs:comment>
            An EP
    </rdfs:comment>
	<rdfs:label>ep</rdfs:label>
	<rdfs:isDefinedBy rdf:resource="http://purl.org/ontology/mo/"/>
</rdf:Description>

<rdf:Description rdf:about="http://purl.org/ontology/mo/interview">
	<rdf:type rdf:resource="http://www.w3.org/2004/02/skos/core#Concept"/>
	<skos:inScheme rdf:resource="http://purl.org/ontology/mo/ReleaseType"/>
	<rdfs:comment>
        Recording of the questioning of a person.
        This is a type of MusicalManifestation defined by the musical industry.
    </rdfs:comment>
	<rdfs:label>interview</rdfs:label>
	<rdfs:isDefinedBy rdf:resource="http://purl.org/ontology/mo/"/>
</rdf:Description>

<rdf:Description rdf:about="http://purl.org/ontology/mo/live">
	<rdf:type rdf:resource="http://www.w3.org/2004/02/skos/core#Concept"/>
	<skos:inScheme rdf:resource="http://purl.org/ontology/mo/ReleaseType"/>
	<rdfs:comment>
        A musical manifestation that was recorded live.
        This is a type of MusicalManifestation defined by the musical industry.</rdfs:comment>
	<rdfs:label>live</rdfs:label>
	<rdfs:isDefinedBy rdf:resource="http://purl.org/ontology/mo/"/>
</rdf:Description>

<rdf:Description rdf:about="http://purl.org/ontology/mo/remix">
	<rdf:type rdf:resource="http://www.w3.org/2004/02/skos/core#Concept"/>
	<skos:inScheme rdf:resource="http://purl.org/ontology/mo/ReleaseType"/>
	<rdfs:comment>
        Musical manifestation that primarily contains remixed material. 
        This is a type of MusicalManifestation defined by the musical industry.
    </rdfs:comment>
	<rdfs:label>remix</rdfs:label>
	<rdfs:isDefinedBy rdf:resource="http://purl.org/ontology/mo/"/>
</rdf:Description>

<rdf:Description rdf:about="http://purl.org/ontology/mo/single">
	<rdf:type rdf:resource="http://www.w3.org/2004/02/skos/core#Concept"/>
	<skos:inScheme rdf:resource="http://purl.org/ontology/mo/ReleaseType"/>
	<rdfs:comment>A single or record single is a type of release, typically a recording of two tracks. In most cases, the single is a song that is released separately from an album, but it can still appear on an album.</rdfs:comment>
	<rdfs:label>single</rdfs:label>
	<rdfs:isDefinedBy rdf:resource="http://purl.org/ontology/mo/"/>
</rdf:Description>

<rdf:Description rdf:about="http://purl.org/ontology/mo/soundtrack">
	<rdf:type rdf:resource="http://www.w3.org/2004/02/skos/core#Concept"/>
	<skos:inScheme rdf:resource="http://purl.org/ontology/mo/ReleaseType"/>
	<rdfs:comment>
        Sound recording on a narrow strip of a motion picture film.
        This is a type of MusicalManifestation defined by the musical industry.
    </rdfs:comment>
	<rdfs:label>soundtrack</rdfs:label>
	<rdfs:isDefinedBy rdf:resource="http://purl.org/ontology/mo/"/>
</rdf:Description>

<rdf:Description rdf:about="http://purl.org/ontology/mo/spokenword">
	<rdf:type rdf:resource="http://www.w3.org/2004/02/skos/core#Concept"/>
	<skos:inScheme rdf:resource="http://purl.org/ontology/mo/ReleaseType"/>
	<rdfs:comment>
        Spoken word is a form of music or artistic performance in which lyrics, poetry, or stories are spoken rather than sung. 
        Spoken-word is often done with a musical background, but emphasis is kept on the speaker.
        This is a type of MusicalManifestation defined by the musical industry.
    </rdfs:comment>
	<rdfs:label>spoken word</rdfs:label>
	<rdfs:isDefinedBy rdf:resource="http://purl.org/ontology/mo/"/>
</rdf:Description>

</rdf:RDF>