<?xml version="1.0" encoding="UTF-8"?>
<rdf:RDF
	xmlns:vann="http://purl.org/vocab/vann/"
	xmlns:voaf="http://purl.org/vocommons/voaf#"
	xmlns:rdfs="http://www.w3.org/2000/01/rdf-schema#"
	xmlns:owl="http://www.w3.org/2002/07/owl#"
	xmlns:skos="http://www.w3.org/2004/02/skos/core#"
	xmlns:rdf="http://www.w3.org/1999/02/22-rdf-syntax-ns#"
	xmlns:dcterms="http://purl.org/dc/terms/"
	xmlns:dc="http://purl.org/dc/elements/1.1/"
	xmlns:dcmit="http://purl.org/dc/dcmitype/"
	xmlns:sesame="http://www.openrdf.org/schema/sesame#"
	xmlns:xsd="http://www.w3.org/2001/XMLSchema#"
	xmlns:fn="http://www.w3.org/2005/xpath-functions#"
	xmlns:foaf="http://xmlns.com/foaf/0.1/"
	xmlns:hint="http://www.bigdata.com/queryHints#"
	xmlns:bd="http://www.bigdata.com/rdf#"
	xmlns:bds="http://www.bigdata.com/rdf/search#">

<rdf:Description rdf:about="http://www.ontology-of-units-of-measure.org/resource/om-2/">
	<rdf:type rdf:resource="http://www.w3.org/2002/07/owl#Ontology"/>
</rdf:Description>

<rdf:Description rdf:about="http://www.ontology-of-units-of-measure.org/resource/om-2/PrefixedMetrePerSecond-TimeSquared">
	<rdf:type rdf:resource="http://www.w3.org/2004/02/skos/core#ConceptScheme"/>
</rdf:Description>

<rdf:Description rdf:about="http://www.ontology-of-units-of-measure.org/resource/om-2/attometrePerSecond-TimeSquared">
	<rdf:type rdf:resource="http://www.w3.org/2004/02/skos/core#Concept"/>
	<skos:inScheme rdf:resource="http://www.ontology-of-units-of-measure.org/resource/om-2/PrefixedMetrePerSecond-TimeSquared"/>
</rdf:Description>

<rdf:Description rdf:about="http://www.ontology-of-units-of-measure.org/resource/om-2/PrefixedMetrePerSecond-TimeSquared">
	<rdfs:label xml:lang="en">prefixed metre per second (time) squared</rdfs:label>
</rdf:Description>

<rdf:Description rdf:about="http://www.ontology-of-units-of-measure.org/resource/om-2/attometrePerSecond-TimeSquared">
	<rdfs:comment xml:lang="en">Attometre per second squared is a unit of acceleration defined as attometre divided by second squared.</rdfs:comment>
	<rdfs:label xml:lang="en">attometre per second squared</rdfs:label>
</rdf:Description>

<rdf:Description rdf:about="http://www.ontology-of-units-of-measure.org/resource/om-2/PrefixedMetrePerSecond-TimeSquared">
	<rdfs:isDefinedBy rdf:resource="http://www.ontology-of-units-of-measure.org/resource/om-2/"/>
</rdf:Description>

<rdf:Description rdf:about="http://www.ontology-of-units-of-measure.org/resource/om-2/attometrePerSecond-TimeSquared">
	<rdfs:isDefinedBy rdf:resource="http://www.ontology-of-units-of-measure.org/resource/om-2/"/>
</rdf:Description>

<rdf:Description rdf:about="http://www.ontology-of-units-of-measure.org/resource/om-2/centimetrePerSecond-TimeSquared">
	<rdf:type rdf:resource="http://www.w3.org/2004/02/skos/core#Concept"/>
	<skos:inScheme rdf:resource="http://www.ontology-of-units-of-measure.org/resource/om-2/PrefixedMetrePerSecond-TimeSquared"/>
	<rdfs:comment xml:lang="en">Centimetre per second squared is a unit of acceleration defined as centimetre divided by second squared.</rdfs:comment>
	<rdfs:label xml:lang="en">centimetre per second squared</rdfs:label>
	<rdfs:isDefinedBy rdf:resource="http://www.ontology-of-units-of-measure.org/resource/om-2/"/>
</rdf:Description>

<rdf:Description rdf:about="http://www.ontology-of-units-of-measure.org/resource/om-2/decametrePerSecond-TimeSquared">
	<rdf:type rdf:resource="http://www.w3.org/2004/02/skos/core#Concept"/>
	<skos:inScheme rdf:resource="http://www.ontology-of-units-of-measure.org/resource/om-2/PrefixedMetrePerSecond-TimeSquared"/>
	<rdfs:comment xml:lang="en">Decametre per second squared is a unit of acceleration defined as decametre divided by second squared.</rdfs:comment>
	<rdfs:label xml:lang="en">decametre per second squared</rdfs:label>
	<rdfs:isDefinedBy rdf:resource="http://www.ontology-of-units-of-measure.org/resource/om-2/"/>
</rdf:Description>

<rdf:Description rdf:about="http://www.ontology-of-units-of-measure.org/resource/om-2/decimetrePerSecond-TimeSquared">
	<rdf:type rdf:resource="http://www.w3.org/2004/02/skos/core#Concept"/>
	<skos:inScheme rdf:resource="http://www.ontology-of-units-of-measure.org/resource/om-2/PrefixedMetrePerSecond-TimeSquared"/>
	<rdfs:comment xml:lang="en">Decimetre per second squared is a unit of acceleration defined as decimetre divided by second squared.</rdfs:comment>
	<rdfs:label xml:lang="en">decimetre per second squared</rdfs:label>
	<rdfs:isDefinedBy rdf:resource="http://www.ontology-of-units-of-measure.org/resource/om-2/"/>
</rdf:Description>

<rdf:Description rdf:about="http://www.ontology-of-units-of-measure.org/resource/om-2/exametrePerSecond-TimeSquared">
	<rdf:type rdf:resource="http://www.w3.org/2004/02/skos/core#Concept"/>
	<skos:inScheme rdf:resource="http://www.ontology-of-units-of-measure.org/resource/om-2/PrefixedMetrePerSecond-TimeSquared"/>
	<rdfs:comment xml:lang="en">Exametre per second squared is a unit of acceleration defined as exametre divided by second squared.</rdfs:comment>
	<rdfs:label xml:lang="en">exametre per second squared</rdfs:label>
	<rdfs:isDefinedBy rdf:resource="http://www.ontology-of-units-of-measure.org/resource/om-2/"/>
</rdf:Description>

<rdf:Description rdf:about="http://www.ontology-of-units-of-measure.org/resource/om-2/femtometrePerSecond-TimeSquared">
	<rdf:type rdf:resource="http://www.w3.org/2004/02/skos/core#Concept"/>
	<skos:inScheme rdf:resource="http://www.ontology-of-units-of-measure.org/resource/om-2/PrefixedMetrePerSecond-TimeSquared"/>
	<rdfs:comment xml:lang="en">Femtometre per second squared is a unit of acceleration defined as femtometre divided by second squared.</rdfs:comment>
	<rdfs:label xml:lang="en">femtometre per second squared</rdfs:label>
	<rdfs:isDefinedBy rdf:resource="http://www.ontology-of-units-of-measure.org/resource/om-2/"/>
</rdf:Description>

<rdf:Description rdf:about="http://www.ontology-of-units-of-measure.org/resource/om-2/gigametrePerSecond-TimeSquared">
	<rdf:type rdf:resource="http://www.w3.org/2004/02/skos/core#Concept"/>
	<skos:inScheme rdf:resource="http://www.ontology-of-units-of-measure.org/resource/om-2/PrefixedMetrePerSecond-TimeSquared"/>
	<rdfs:comment xml:lang="en">Gigametre per second squared is a unit of acceleration defined as gigametre divided by second squared.</rdfs:comment>
	<rdfs:label xml:lang="en">gigametre per second squared</rdfs:label>
	<rdfs:isDefinedBy rdf:resource="http://www.ontology-of-units-of-measure.org/resource/om-2/"/>
</rdf:Description>

<rdf:Description rdf:about="http://www.ontology-of-units-of-measure.org/resource/om-2/hectometrePerSecond-TimeSquared">
	<rdf:type rdf:resource="http://www.w3.org/2004/02/skos/core#Concept"/>
	<skos:inScheme rdf:resource="http://www.ontology-of-units-of-measure.org/resource/om-2/PrefixedMetrePerSecond-TimeSquared"/>
	<rdfs:comment xml:lang="en">Hectometre per second squared is a unit of acceleration defined as hectometre divided by second squared.</rdfs:comment>
	<rdfs:label xml:lang="en">hectometre per second squared</rdfs:label>
	<rdfs:isDefinedBy rdf:resource="http://www.ontology-of-units-of-measure.org/resource/om-2/"/>
</rdf:Description>

<rdf:Description rdf:about="http://www.ontology-of-units-of-measure.org/resource/om-2/kilometrePerSecond-TimeSquared">
	<rdf:type rdf:resource="http://www.w3.org/2004/02/skos/core#Concept"/>
	<skos:inScheme rdf:resource="http://www.ontology-of-units-of-measure.org/resource/om-2/PrefixedMetrePerSecond-TimeSquared"/>
	<rdfs:comment xml:lang="en">Kilometre per second squared is a unit of acceleration defined as kilometre divided by second squared.</rdfs:comment>
	<rdfs:label xml:lang="en">kilometre per second squared</rdfs:label>
	<rdfs:isDefinedBy rdf:resource="http://www.ontology-of-units-of-measure.org/resource/om-2/"/>
</rdf:Description>

<rdf:Description rdf:about="http://www.ontology-of-units-of-measure.org/resource/om-2/megametrePerSecond-TimeSquared">
	<rdf:type rdf:resource="http://www.w3.org/2004/02/skos/core#Concept"/>
	<skos:inScheme rdf:resource="http://www.ontology-of-units-of-measure.org/resource/om-2/PrefixedMetrePerSecond-TimeSquared"/>
	<rdfs:comment xml:lang="en">Megametre per second squared is a unit of acceleration defined as megametre divided by second squared.</rdfs:comment>
	<rdfs:label xml:lang="en">megametre per second squared</rdfs:label>
	<rdfs:isDefinedBy rdf:resource="http://www.ontology-of-units-of-measure.org/resource/om-2/"/>
</rdf:Description>

<rdf:Description rdf:about="http://www.ontology-of-units-of-measure.org/resource/om-2/micrometrePerSecond-TimeSquared">
	<rdf:type rdf:resource="http://www.w3.org/2004/02/skos/core#Concept"/>
	<skos:inScheme rdf:resource="http://www.ontology-of-units-of-measure.org/resource/om-2/PrefixedMetrePerSecond-TimeSquared"/>
	<rdfs:comment xml:lang="en">Micrometre per second squared is a unit of acceleration defined as micrometre divided by second squared.</rdfs:comment>
	<rdfs:label xml:lang="en">micrometre per second squared</rdfs:label>
	<rdfs:isDefinedBy rdf:resource="http://www.ontology-of-units-of-measure.org/resource/om-2/"/>
</rdf:Description>

<rdf:Description rdf:about="http://www.ontology-of-units-of-measure.org/resource/om-2/millimetrePerSecond-TimeSquared">
	<rdf:type rdf:resource="http://www.w3.org/2004/02/skos/core#Concept"/>
	<skos:inScheme rdf:resource="http://www.ontology-of-units-of-measure.org/resource/om-2/PrefixedMetrePerSecond-TimeSquared"/>
	<rdfs:comment xml:lang="en">Millimetre per second squared is a unit of acceleration defined as millimetre divided by second squared.</rdfs:comment>
	<rdfs:label xml:lang="en">millimetre per second squared</rdfs:label>
	<rdfs:isDefinedBy rdf:resource="http://www.ontology-of-units-of-measure.org/resource/om-2/"/>
</rdf:Description>

<rdf:Description rdf:about="http://www.ontology-of-units-of-measure.org/resource/om-2/nanometrePerSecond-TimeSquared">
	<rdf:type rdf:resource="http://www.w3.org/2004/02/skos/core#Concept"/>
	<skos:inScheme rdf:resource="http://www.ontology-of-units-of-measure.org/resource/om-2/PrefixedMetrePerSecond-TimeSquared"/>
	<rdfs:comment xml:lang="en">Nanometre per second squared is a unit of acceleration defined as nanometre divided by second squared.</rdfs:comment>
	<rdfs:label xml:lang="en">nanometre per second squared</rdfs:label>
	<rdfs:isDefinedBy rdf:resource="http://www.ontology-of-units-of-measure.org/resource/om-2/"/>
</rdf:Description>

<rdf:Description rdf:about="http://www.ontology-of-units-of-measure.org/resource/om-2/petametrePerSecond-TimeSquared">
	<rdf:type rdf:resource="http://www.w3.org/2004/02/skos/core#Concept"/>
	<skos:inScheme rdf:resource="http://www.ontology-of-units-of-measure.org/resource/om-2/PrefixedMetrePerSecond-TimeSquared"/>
	<rdfs:comment xml:lang="en">Petametre per second squared is a unit of acceleration defined as petametre divided by second squared.</rdfs:comment>
	<rdfs:label xml:lang="en">petametre per second squared</rdfs:label>
	<rdfs:isDefinedBy rdf:resource="http://www.ontology-of-units-of-measure.org/resource/om-2/"/>
</rdf:Description>

<rdf:Description rdf:about="http://www.ontology-of-units-of-measure.org/resource/om-2/picometrePerSecond-TimeSquared">
	<rdf:type rdf:resource="http://www.w3.org/2004/02/skos/core#Concept"/>
	<skos:inScheme rdf:resource="http://www.ontology-of-units-of-measure.org/resource/om-2/PrefixedMetrePerSecond-TimeSquared"/>
	<rdfs:comment xml:lang="en">Picometre per second squared is a unit of acceleration defined as picometre divided by second squared.</rdfs:comment>
	<rdfs:label xml:lang="en">picometre per second squared</rdfs:label>
	<rdfs:isDefinedBy rdf:resource="http://www.ontology-of-units-of-measure.org/resource/om-2/"/>
</rdf:Description>

<rdf:Description rdf:about="http://www.ontology-of-units-of-measure.org/resource/om-2/terametrePerSecond-TimeSquared">
	<rdf:type rdf:resource="http://www.w3.org/2004/02/skos/core#Concept"/>
	<skos:inScheme rdf:resource="http://www.ontology-of-units-of-measure.org/resource/om-2/PrefixedMetrePerSecond-TimeSquared"/>
	<rdfs:comment xml:lang="en">Terametre per second squared is a unit of acceleration defined as terametre divided by second squared.</rdfs:comment>
	<rdfs:label xml:lang="en">terametre per second squared</rdfs:label>
	<rdfs:isDefinedBy rdf:resource="http://www.ontology-of-units-of-measure.org/resource/om-2/"/>
</rdf:Description>

<rdf:Description rdf:about="http://www.ontology-of-units-of-measure.org/resource/om-2/yoctometrePerSecond-TimeSquared">
	<rdf:type rdf:resource="http://www.w3.org/2004/02/skos/core#Concept"/>
	<skos:inScheme rdf:resource="http://www.ontology-of-units-of-measure.org/resource/om-2/PrefixedMetrePerSecond-TimeSquared"/>
	<rdfs:comment xml:lang="en">Yoctometre per second squared is a unit of acceleration defined as yoctometre divided by second squared.</rdfs:comment>
	<rdfs:label xml:lang="en">yoctometre per second squared</rdfs:label>
	<rdfs:isDefinedBy rdf:resource="http://www.ontology-of-units-of-measure.org/resource/om-2/"/>
</rdf:Description>

<rdf:Description rdf:about="http://www.ontology-of-units-of-measure.org/resource/om-2/yottametrePerSecond-TimeSquared">
	<rdf:type rdf:resource="http://www.w3.org/2004/02/skos/core#Concept"/>
	<skos:inScheme rdf:resource="http://www.ontology-of-units-of-measure.org/resource/om-2/PrefixedMetrePerSecond-TimeSquared"/>
	<rdfs:comment xml:lang="en">Yottametre per second squared is a unit of acceleration defined as yottametre divided by second squared.</rdfs:comment>
	<rdfs:label xml:lang="en">yottametre per second squared</rdfs:label>
	<rdfs:isDefinedBy rdf:resource="http://www.ontology-of-units-of-measure.org/resource/om-2/"/>
</rdf:Description>

<rdf:Description rdf:about="http://www.ontology-of-units-of-measure.org/resource/om-2/zeptometrePerSecond-TimeSquared">
	<rdf:type rdf:resource="http://www.w3.org/2004/02/skos/core#Concept"/>
	<skos:inScheme rdf:resource="http://www.ontology-of-units-of-measure.org/resource/om-2/PrefixedMetrePerSecond-TimeSquared"/>
	<rdfs:comment xml:lang="en">Zeptometre per second squared is a unit of acceleration defined as zeptometre divided by second squared.</rdfs:comment>
	<rdfs:label xml:lang="en">zeptometre per second squared</rdfs:label>
	<rdfs:isDefinedBy rdf:resource="http://www.ontology-of-units-of-measure.org/resource/om-2/"/>
</rdf:Description>

<rdf:Description rdf:about="http://www.ontology-of-units-of-measure.org/resource/om-2/zettametrePerSecond-TimeSquared">
	<rdf:type rdf:resource="http://www.w3.org/2004/02/skos/core#Concept"/>
	<skos:inScheme rdf:resource="http://www.ontology-of-units-of-measure.org/resource/om-2/PrefixedMetrePerSecond-TimeSquared"/>
	<rdfs:comment xml:lang="en">Zettametre per second squared is a unit of acceleration defined as zettametre divided by second squared.</rdfs:comment>
	<rdfs:label xml:lang="en">zettametre per second squared</rdfs:label>
	<rdfs:isDefinedBy rdf:resource="http://www.ontology-of-units-of-measure.org/resource/om-2/"/>
</rdf:Description>

</rdf:RDF>