<?xml version="1.0" encoding="UTF-8"?>
<rdf:RDF
	xmlns:vann="http://purl.org/vocab/vann/"
	xmlns:voaf="http://purl.org/vocommons/voaf#"
	xmlns:rdfs="http://www.w3.org/2000/01/rdf-schema#"
	xmlns:owl="http://www.w3.org/2002/07/owl#"
	xmlns:skos="http://www.w3.org/2004/02/skos/core#"
	xmlns:rdf="http://www.w3.org/1999/02/22-rdf-syntax-ns#"
	xmlns:dcterms="http://purl.org/dc/terms/"
	xmlns:dc="http://purl.org/dc/elements/1.1/"
	xmlns:dcmit="http://purl.org/dc/dcmitype/"
	xmlns:sesame="http://www.openrdf.org/schema/sesame#"
	xmlns:xsd="http://www.w3.org/2001/XMLSchema#"
	xmlns:fn="http://www.w3.org/2005/xpath-functions#"
	xmlns:foaf="http://xmlns.com/foaf/0.1/"
	xmlns:hint="http://www.bigdata.com/queryHints#"
	xmlns:bd="http://www.bigdata.com/rdf#"
	xmlns:bds="http://www.bigdata.com/rdf/search#">

<rdf:Description rdf:about="http://purl.oclc.org/NET/ssnx/cf/cf-property">
	<rdf:type rdf:resource="http://www.w3.org/2002/07/owl#Ontology"/>
</rdf:Description>

<rdf:Description rdf:about="http://purl.oclc.org/NET/ssnx/qu/dim#DiffusionCoefficient">
	<rdf:type rdf:resource="http://www.w3.org/2004/02/skos/core#ConceptScheme"/>
</rdf:Description>

<rdf:Description rdf:about="http://purl.oclc.org/NET/ssnx/qu/quantity#diffusionCoefficient">
	<rdf:type rdf:resource="http://www.w3.org/2004/02/skos/core#Concept"/>
	<skos:inScheme rdf:resource="http://purl.oclc.org/NET/ssnx/qu/dim#DiffusionCoefficient"/>
</rdf:Description>

<rdf:Description rdf:about="http://purl.oclc.org/NET/ssnx/qu/dim#DiffusionCoefficient">
	<rdfs:isDefinedBy rdf:resource="http://purl.oclc.org/NET/ssnx/cf/cf-property"/>
</rdf:Description>

<rdf:Description rdf:about="http://purl.oclc.org/NET/ssnx/qu/quantity#diffusionCoefficient">
	<rdfs:isDefinedBy rdf:resource="http://purl.oclc.org/NET/ssnx/cf/cf-property"/>
</rdf:Description>

<rdf:Description rdf:about="http://purl.oclc.org/NET/ssnx/cf/cf-property#atmosphere_heat_diffusivity">
	<rdf:type rdf:resource="http://www.w3.org/2004/02/skos/core#Concept"/>
	<skos:inScheme rdf:resource="http://purl.oclc.org/NET/ssnx/qu/dim#DiffusionCoefficient"/>
	<rdfs:label>atmosphere heat diffusivity</rdfs:label>
	<generalQuantityKind xmlns="http://purl.oclc.org/NET/ssnx/qu/qu#" rdf:resource="http://purl.oclc.org/NET/ssnx/qu/quantity#diffusionCoefficient"/>
	<rdfs:isDefinedBy rdf:resource="http://purl.oclc.org/NET/ssnx/cf/cf-property"/>
</rdf:Description>

<rdf:Description rdf:about="http://purl.oclc.org/NET/ssnx/cf/cf-property#atmosphere_horizontal_streamfunction">
	<rdf:type rdf:resource="http://www.w3.org/2004/02/skos/core#Concept"/>
	<skos:inScheme rdf:resource="http://purl.oclc.org/NET/ssnx/qu/dim#DiffusionCoefficient"/>
	<rdfs:comment>"Horizontal" indicates that the streamfunction applies to a horizontal velocity field on a particular vertical level.</rdfs:comment>
	<rdfs:label>atmosphere horizontal streamfunction</rdfs:label>
	<generalQuantityKind xmlns="http://purl.oclc.org/NET/ssnx/qu/qu#" rdf:resource="http://purl.oclc.org/NET/ssnx/qu/quantity#diffusionCoefficient"/>
	<rdfs:isDefinedBy rdf:resource="http://purl.oclc.org/NET/ssnx/cf/cf-property"/>
</rdf:Description>

<rdf:Description rdf:about="http://purl.oclc.org/NET/ssnx/cf/cf-property#atmosphere_horizontal_velocity_potential">
	<rdf:type rdf:resource="http://www.w3.org/2004/02/skos/core#Concept"/>
	<skos:inScheme rdf:resource="http://purl.oclc.org/NET/ssnx/qu/dim#DiffusionCoefficient"/>
	<rdfs:comment>A velocity is a vector quantity. "Horizontal" indicates that the velocity potential applies to a horizontal velocity field on a particular vertical level.</rdfs:comment>
	<rdfs:label>atmosphere horizontal velocity potential</rdfs:label>
	<generalQuantityKind xmlns="http://purl.oclc.org/NET/ssnx/qu/qu#" rdf:resource="http://purl.oclc.org/NET/ssnx/qu/quantity#diffusionCoefficient"/>
	<rdfs:isDefinedBy rdf:resource="http://purl.oclc.org/NET/ssnx/cf/cf-property"/>
</rdf:Description>

<rdf:Description rdf:about="http://purl.oclc.org/NET/ssnx/cf/cf-property#atmosphere_momentum_diffusivity">
	<rdf:type rdf:resource="http://www.w3.org/2004/02/skos/core#Concept"/>
	<skos:inScheme rdf:resource="http://purl.oclc.org/NET/ssnx/qu/dim#DiffusionCoefficient"/>
	<rdfs:label>atmosphere momentum diffusivity</rdfs:label>
	<generalQuantityKind xmlns="http://purl.oclc.org/NET/ssnx/qu/qu#" rdf:resource="http://purl.oclc.org/NET/ssnx/qu/quantity#diffusionCoefficient"/>
	<rdfs:isDefinedBy rdf:resource="http://purl.oclc.org/NET/ssnx/cf/cf-property"/>
</rdf:Description>

<rdf:Description rdf:about="http://purl.oclc.org/NET/ssnx/cf/cf-property#ocean_isopycnal_layer_thickness_diffusivity">
	<rdf:type rdf:resource="http://www.w3.org/2004/02/skos/core#Concept"/>
	<skos:inScheme rdf:resource="http://purl.oclc.org/NET/ssnx/qu/dim#DiffusionCoefficient"/>
	<rdfs:label>ocean isopycnal layer thickness diffusivity</rdfs:label>
	<generalQuantityKind xmlns="http://purl.oclc.org/NET/ssnx/qu/qu#" rdf:resource="http://purl.oclc.org/NET/ssnx/qu/quantity#diffusionCoefficient"/>
	<rdfs:isDefinedBy rdf:resource="http://purl.oclc.org/NET/ssnx/cf/cf-property"/>
</rdf:Description>

<rdf:Description rdf:about="http://purl.oclc.org/NET/ssnx/cf/cf-property#ocean_momentum_xy_laplacian_diffusivity">
	<rdf:type rdf:resource="http://www.w3.org/2004/02/skos/core#Concept"/>
	<skos:inScheme rdf:resource="http://purl.oclc.org/NET/ssnx/qu/dim#DiffusionCoefficient"/>
	<rdfs:comment> Diffusivity is also sometimes known as the coefficient of diffusion. Diffusion occurs as a result of a gradient in the spatial distribution of mass concentration, temperature or momentum.  The diffusivity may be very different in the vertical and horizontal directions. "xy diffusivity" means the lateral along_coordinate component of diffusivity due to motion which is not resolved on the grid scale of the model.  xy diffusivities are used in some ocean models to counteract the numerical instabilities inherent in certain implementations of rotated neutral diffusion. "laplacian diffusivity" means diffusivity for use with a Laplacian diffusion operator.</rdfs:comment>
	<rdfs:label>ocean momentum xy laplacian diffusivity</rdfs:label>
	<generalQuantityKind xmlns="http://purl.oclc.org/NET/ssnx/qu/qu#" rdf:resource="http://purl.oclc.org/NET/ssnx/qu/quantity#diffusionCoefficient"/>
	<rdfs:isDefinedBy rdf:resource="http://purl.oclc.org/NET/ssnx/cf/cf-property"/>
</rdf:Description>

<rdf:Description rdf:about="http://purl.oclc.org/NET/ssnx/cf/cf-property#ocean_tracer_bolus_laplacian_diffusivity">
	<rdf:type rdf:resource="http://www.w3.org/2004/02/skos/core#Concept"/>
	<skos:inScheme rdf:resource="http://purl.oclc.org/NET/ssnx/qu/dim#DiffusionCoefficient"/>
	<rdfs:comment> Diffusivity is also sometimes known as the coefficient of diffusion. Diffusion occurs as a result of a gradient in the spatial distribution of mass concentration, temperature or momentum.  The diffusivity may be very different in the vertical and horizontal directions. "Bolus diffusivity" means a lateral diffusivity. "laplacian diffusivity" means diffusivity for use with a Laplacian diffusion operator.</rdfs:comment>
	<rdfs:label>ocean tracer bolus laplacian diffusivity</rdfs:label>
	<generalQuantityKind xmlns="http://purl.oclc.org/NET/ssnx/qu/qu#" rdf:resource="http://purl.oclc.org/NET/ssnx/qu/quantity#diffusionCoefficient"/>
	<rdfs:isDefinedBy rdf:resource="http://purl.oclc.org/NET/ssnx/cf/cf-property"/>
</rdf:Description>

<rdf:Description rdf:about="http://purl.oclc.org/NET/ssnx/cf/cf-property#ocean_tracer_epineutral_laplacian_diffusivity">
	<rdf:type rdf:resource="http://www.w3.org/2004/02/skos/core#Concept"/>
	<skos:inScheme rdf:resource="http://purl.oclc.org/NET/ssnx/qu/dim#DiffusionCoefficient"/>
	<rdfs:comment> Diffusivity is also sometimes known as the coefficient of diffusion. Diffusion occurs as a result of a gradient in the spatial distribution of mass concentration, temperature or momentum.  The diffusivity may be very different in the vertical and horizontal directions. "epineutral diffusivity" means a lateral diffusivity along a either a neutral or isopycnal density surface due to motion which is not resolved on the grid scale of an ocean model. The type of density surface is dependent on the model formulation. "laplacian diffusivity" means diffusivity for use with a Laplacian diffusion operator.</rdfs:comment>
	<rdfs:label>ocean tracer epineutral laplacian diffusivity</rdfs:label>
	<generalQuantityKind xmlns="http://purl.oclc.org/NET/ssnx/qu/qu#" rdf:resource="http://purl.oclc.org/NET/ssnx/qu/quantity#diffusionCoefficient"/>
	<rdfs:isDefinedBy rdf:resource="http://purl.oclc.org/NET/ssnx/cf/cf-property"/>
</rdf:Description>

<rdf:Description rdf:about="http://purl.oclc.org/NET/ssnx/cf/cf-property#ocean_tracer_xy_laplacian_diffusivity">
	<rdf:type rdf:resource="http://www.w3.org/2004/02/skos/core#Concept"/>
	<skos:inScheme rdf:resource="http://purl.oclc.org/NET/ssnx/qu/dim#DiffusionCoefficient"/>
	<rdfs:comment> Diffusivity is also sometimes known as the coefficient of diffusion. Diffusion occurs as a result of a gradient in the spatial distribution of mass concentration, temperature or momentum.  The diffusivity may be very different in the vertical and horizontal directions. "xy diffusivity" means the lateral along_coordinate component of diffusivity due to motion which is not resolved on the grid scale of the model.  xy diffusivities are used in some ocean models to counteract the numerical instabilities inherent in certain implementations of rotated neutral diffusion. "laplacian diffusivity" means diffusivity for use with a Laplacian diffusion operator.</rdfs:comment>
	<rdfs:label>ocean tracer xy laplacian diffusivity</rdfs:label>
	<generalQuantityKind xmlns="http://purl.oclc.org/NET/ssnx/qu/qu#" rdf:resource="http://purl.oclc.org/NET/ssnx/qu/quantity#diffusionCoefficient"/>
	<rdfs:isDefinedBy rdf:resource="http://purl.oclc.org/NET/ssnx/cf/cf-property"/>
</rdf:Description>

<rdf:Description rdf:about="http://purl.oclc.org/NET/ssnx/cf/cf-property#ocean_vertical_diffusivity">
	<rdf:type rdf:resource="http://www.w3.org/2004/02/skos/core#Concept"/>
	<skos:inScheme rdf:resource="http://purl.oclc.org/NET/ssnx/qu/dim#DiffusionCoefficient"/>
	<rdfs:comment>"Vertical diffusivity" means the vertical component of diffusivity due to motion which is not resolved on the grid scale of the model.</rdfs:comment>
	<rdfs:label>ocean vertical diffusivity</rdfs:label>
	<generalQuantityKind xmlns="http://purl.oclc.org/NET/ssnx/qu/qu#" rdf:resource="http://purl.oclc.org/NET/ssnx/qu/quantity#diffusionCoefficient"/>
	<rdfs:isDefinedBy rdf:resource="http://purl.oclc.org/NET/ssnx/cf/cf-property"/>
</rdf:Description>

<rdf:Description rdf:about="http://purl.oclc.org/NET/ssnx/cf/cf-property#ocean_vertical_heat_diffusivity">
	<rdf:type rdf:resource="http://www.w3.org/2004/02/skos/core#Concept"/>
	<skos:inScheme rdf:resource="http://purl.oclc.org/NET/ssnx/qu/dim#DiffusionCoefficient"/>
	<rdfs:comment>"Vertical heat diffusivity" means the vertical component of the diffusivity of heat due to motion which is not resolved on the grid scale of the model.</rdfs:comment>
	<rdfs:label>ocean vertical heat diffusivity</rdfs:label>
	<generalQuantityKind xmlns="http://purl.oclc.org/NET/ssnx/qu/qu#" rdf:resource="http://purl.oclc.org/NET/ssnx/qu/quantity#diffusionCoefficient"/>
	<rdfs:isDefinedBy rdf:resource="http://purl.oclc.org/NET/ssnx/cf/cf-property"/>
</rdf:Description>

<rdf:Description rdf:about="http://purl.oclc.org/NET/ssnx/cf/cf-property#ocean_vertical_momentum_diffusivity">
	<rdf:type rdf:resource="http://www.w3.org/2004/02/skos/core#Concept"/>
	<skos:inScheme rdf:resource="http://purl.oclc.org/NET/ssnx/qu/dim#DiffusionCoefficient"/>
	<rdfs:comment>"Vertical momentum diffusivity" means the vertical component of the diffusivity of momentum due to motion which is not resolved on the grid scale of the model. </rdfs:comment>
	<rdfs:label>ocean vertical momentum diffusivity</rdfs:label>
	<generalQuantityKind xmlns="http://purl.oclc.org/NET/ssnx/qu/qu#" rdf:resource="http://purl.oclc.org/NET/ssnx/qu/quantity#diffusionCoefficient"/>
	<rdfs:isDefinedBy rdf:resource="http://purl.oclc.org/NET/ssnx/cf/cf-property"/>
</rdf:Description>

<rdf:Description rdf:about="http://purl.oclc.org/NET/ssnx/cf/cf-property#ocean_vertical_momentum_diffusivity_due_to_background">
	<rdf:type rdf:resource="http://www.w3.org/2004/02/skos/core#Concept"/>
	<skos:inScheme rdf:resource="http://purl.oclc.org/NET/ssnx/qu/dim#DiffusionCoefficient"/>
	<rdfs:comment> Diffusivity is also sometimes known as the coefficient of diffusion. Diffusion occurs as a result of a gradient in the spatial distribution of mass concentration, temperature or momentum.  The diffusivity may be very different in the vertical and horizontal directions. The construction vertical_X_diffusivity means the vertical component of thediffusivity of X due to motion which is not resolved on the grid scale of the model. "Due to background" means caused by a time invariant imposed field which may be eitherconstant over the globe or spatially varying, depending on the ocean model used. The specification of a physical process by the phrase due_to_process means that the quantity named is a  single term in a sum of terms which together compose the general quantity  named by omitting the phrase. </rdfs:comment>
	<rdfs:label>ocean vertical momentum diffusivity due to background</rdfs:label>
	<generalQuantityKind xmlns="http://purl.oclc.org/NET/ssnx/qu/qu#" rdf:resource="http://purl.oclc.org/NET/ssnx/qu/quantity#diffusionCoefficient"/>
	<rdfs:isDefinedBy rdf:resource="http://purl.oclc.org/NET/ssnx/cf/cf-property"/>
</rdf:Description>

<rdf:Description rdf:about="http://purl.oclc.org/NET/ssnx/cf/cf-property#ocean_vertical_momentum_diffusivity_due_to_convection">
	<rdf:type rdf:resource="http://www.w3.org/2004/02/skos/core#Concept"/>
	<skos:inScheme rdf:resource="http://purl.oclc.org/NET/ssnx/qu/dim#DiffusionCoefficient"/>
	<rdfs:comment>The specification of a physical process by the phrase due_to_process means that the quantity named is a single term in a sum of terms which together compose the general quantity named by omitting the phrase. "Vertical momentum diffusivity" means the vertical component of the diffusivity of momentum due to motion which is not resolved on the grid scale of the model. Convective mixing in the ocean is somtimes modelled as an enhanced diffusivity.</rdfs:comment>
	<rdfs:label>ocean vertical momentum diffusivity due to convection</rdfs:label>
	<generalQuantityKind xmlns="http://purl.oclc.org/NET/ssnx/qu/qu#" rdf:resource="http://purl.oclc.org/NET/ssnx/qu/quantity#diffusionCoefficient"/>
	<rdfs:isDefinedBy rdf:resource="http://purl.oclc.org/NET/ssnx/cf/cf-property"/>
</rdf:Description>

<rdf:Description rdf:about="http://purl.oclc.org/NET/ssnx/cf/cf-property#ocean_vertical_momentum_diffusivity_due_to_form_drag">
	<rdf:type rdf:resource="http://www.w3.org/2004/02/skos/core#Concept"/>
	<skos:inScheme rdf:resource="http://purl.oclc.org/NET/ssnx/qu/dim#DiffusionCoefficient"/>
	<rdfs:comment> Diffusivity is also sometimes known as the coefficient of diffusion. Diffusion occurs as a result of a gradient in the spatial distribution of mass concentration, temperature or momentum.  The diffusivity may be very different in the vertical and horizontal directions. The construction vertical_X_diffusivity means the vertical component of thediffusivity of X due to motion which is not resolved on the grid scale of the model. "Due to form drag" refers to a vertical diffusivity resulting from a model scheme representing  mesoscale eddy-induced form drag. The specification of a physical process by the phrase due_to_process means that the quantity named is a  single term in a sum of terms which together compose the general quantity  named by omitting the phrase. </rdfs:comment>
	<rdfs:label>ocean vertical momentum diffusivity due to form drag</rdfs:label>
	<generalQuantityKind xmlns="http://purl.oclc.org/NET/ssnx/qu/qu#" rdf:resource="http://purl.oclc.org/NET/ssnx/qu/quantity#diffusionCoefficient"/>
	<rdfs:isDefinedBy rdf:resource="http://purl.oclc.org/NET/ssnx/cf/cf-property"/>
</rdf:Description>

<rdf:Description rdf:about="http://purl.oclc.org/NET/ssnx/cf/cf-property#ocean_vertical_momentum_diffusivity_due_to_tides">
	<rdf:type rdf:resource="http://www.w3.org/2004/02/skos/core#Concept"/>
	<skos:inScheme rdf:resource="http://purl.oclc.org/NET/ssnx/qu/dim#DiffusionCoefficient"/>
	<rdfs:comment> Diffusivity is also sometimes known as the coefficient of diffusion. Diffusion occurs as a result of a gradient in the spatial distribution of mass concentration, temperature or momentum.  The diffusivity may be very different in the vertical and horizontal directions. The construction vertical_X_diffusivity means the vertical component of thediffusivity of X due to motion which is not resolved on the grid scale of the model. "Due to tides" means due to all astronomical gravity changes which manifest as tides.No distinction is made between different tidal components. The specification of a physicalprocess by the phrase due_to_process means that the quantity named is a  single term in a sum of terms which together compose the general quantity  named by omitting the phrase. </rdfs:comment>
	<rdfs:label>ocean vertical momentum diffusivity due to tides</rdfs:label>
	<generalQuantityKind xmlns="http://purl.oclc.org/NET/ssnx/qu/qu#" rdf:resource="http://purl.oclc.org/NET/ssnx/qu/quantity#diffusionCoefficient"/>
	<rdfs:isDefinedBy rdf:resource="http://purl.oclc.org/NET/ssnx/cf/cf-property"/>
</rdf:Description>

<rdf:Description rdf:about="http://purl.oclc.org/NET/ssnx/cf/cf-property#ocean_vertical_salt_diffusivity">
	<rdf:type rdf:resource="http://www.w3.org/2004/02/skos/core#Concept"/>
	<skos:inScheme rdf:resource="http://purl.oclc.org/NET/ssnx/qu/dim#DiffusionCoefficient"/>
	<rdfs:comment>"Vertical salt diffusivity" means the vertical component of the diffusivity of salt due to motion which is not resolved on the grid scale of the model.</rdfs:comment>
	<rdfs:label>ocean vertical salt diffusivity</rdfs:label>
	<generalQuantityKind xmlns="http://purl.oclc.org/NET/ssnx/qu/qu#" rdf:resource="http://purl.oclc.org/NET/ssnx/qu/quantity#diffusionCoefficient"/>
	<rdfs:isDefinedBy rdf:resource="http://purl.oclc.org/NET/ssnx/cf/cf-property"/>
</rdf:Description>

<rdf:Description rdf:about="http://purl.oclc.org/NET/ssnx/cf/cf-property#ocean_vertical_tracer_diffusivity">
	<rdf:type rdf:resource="http://www.w3.org/2004/02/skos/core#Concept"/>
	<skos:inScheme rdf:resource="http://purl.oclc.org/NET/ssnx/qu/dim#DiffusionCoefficient"/>
	<rdfs:comment>"Vertical tracer diffusivity" means the vertical component of the diffusivity of tracers, i.e. heat and salinity, due to motion which is not resolved on the grid scale of the model.</rdfs:comment>
	<rdfs:label>ocean vertical tracer diffusivity</rdfs:label>
	<generalQuantityKind xmlns="http://purl.oclc.org/NET/ssnx/qu/qu#" rdf:resource="http://purl.oclc.org/NET/ssnx/qu/quantity#diffusionCoefficient"/>
	<rdfs:isDefinedBy rdf:resource="http://purl.oclc.org/NET/ssnx/cf/cf-property"/>
</rdf:Description>

<rdf:Description rdf:about="http://purl.oclc.org/NET/ssnx/cf/cf-property#ocean_vertical_tracer_diffusivity_due_to_background">
	<rdf:type rdf:resource="http://www.w3.org/2004/02/skos/core#Concept"/>
	<skos:inScheme rdf:resource="http://purl.oclc.org/NET/ssnx/qu/dim#DiffusionCoefficient"/>
	<rdfs:comment> Diffusivity is also sometimes known as the coefficient of diffusion. Diffusion occurs as a result of a gradient in the spatial distribution of mass concentration, temperature or momentum.  The diffusivity may be very different in the vertical and horizontal directions. The construction vertical_X_diffusivity means the vertical component of thediffusivity of X due to motion which is not resolved on the grid scale of the model. "Due to background" means caused by a time invariant imposed field which may be eitherconstant over the globe or spatially varying, depending on the ocean model used. The specification of a physical process by the phrase due_to_process means that the quantity named is a  single term in a sum of terms which together compose the general quantity  named by omitting the phrase. </rdfs:comment>
	<rdfs:label>ocean vertical tracer diffusivity due to background</rdfs:label>
	<generalQuantityKind xmlns="http://purl.oclc.org/NET/ssnx/qu/qu#" rdf:resource="http://purl.oclc.org/NET/ssnx/qu/quantity#diffusionCoefficient"/>
	<rdfs:isDefinedBy rdf:resource="http://purl.oclc.org/NET/ssnx/cf/cf-property"/>
</rdf:Description>

<rdf:Description rdf:about="http://purl.oclc.org/NET/ssnx/cf/cf-property#ocean_vertical_tracer_diffusivity_due_to_convection">
	<rdf:type rdf:resource="http://www.w3.org/2004/02/skos/core#Concept"/>
	<skos:inScheme rdf:resource="http://purl.oclc.org/NET/ssnx/qu/dim#DiffusionCoefficient"/>
	<rdfs:comment>The specification of a physical process by the phrase due_to_process means that the quantity named is a single term in a sum of terms which together compose the general quantity named by omitting the phrase. "Vertical tracer diffusivity" means the vertical component of the diffusivity of tracers, i.e. heat and salinity, due to motion which is not resolved on the grid scale of the model.  Convective mixing in the ocean is sometimes modelled as an enhanced diffusivity.</rdfs:comment>
	<rdfs:label>ocean vertical tracer diffusivity due to convection</rdfs:label>
	<generalQuantityKind xmlns="http://purl.oclc.org/NET/ssnx/qu/qu#" rdf:resource="http://purl.oclc.org/NET/ssnx/qu/quantity#diffusionCoefficient"/>
	<rdfs:isDefinedBy rdf:resource="http://purl.oclc.org/NET/ssnx/cf/cf-property"/>
</rdf:Description>

<rdf:Description rdf:about="http://purl.oclc.org/NET/ssnx/cf/cf-property#ocean_vertical_tracer_diffusivity_due_to_tides">
	<rdf:type rdf:resource="http://www.w3.org/2004/02/skos/core#Concept"/>
	<skos:inScheme rdf:resource="http://purl.oclc.org/NET/ssnx/qu/dim#DiffusionCoefficient"/>
	<rdfs:comment> Diffusivity is also sometimes known as the coefficient of diffusion. Diffusion occurs as a result of a gradient in the spatial distribution of mass concentration, temperature or momentum.  The diffusivity may be very different in the vertical and horizontal directions. The construction vertical_X_diffusivity means the vertical component of thediffusivity of X due to motion which is not resolved on the grid scale of the model. "Due to tides" means due to all astronomical gravity changes which manifest as tides.No distinction is made between different tidal components. The specification of a physicalprocess by the phrase due_to_process means that the quantity named is a  single term in a sum of terms which together compose the general quantity  named by omitting the phrase. </rdfs:comment>
	<rdfs:label>ocean vertical tracer diffusivity due to tides</rdfs:label>
	<generalQuantityKind xmlns="http://purl.oclc.org/NET/ssnx/qu/qu#" rdf:resource="http://purl.oclc.org/NET/ssnx/qu/quantity#diffusionCoefficient"/>
	<rdfs:isDefinedBy rdf:resource="http://purl.oclc.org/NET/ssnx/cf/cf-property"/>
</rdf:Description>

<rdf:Description rdf:about="http://purl.oclc.org/NET/ssnx/cf/cf-property#ocean_vertical_tracer_diffusivity_due_to_wind_mixing">
	<rdf:type rdf:resource="http://www.w3.org/2004/02/skos/core#Concept"/>
	<skos:inScheme rdf:resource="http://purl.oclc.org/NET/ssnx/qu/dim#DiffusionCoefficient"/>
	<rdfs:comment>The specification of a physical process by the phrase due_to_process means that the quantity named is a single term in a sum of terms which together compose the general quantity named by omitting the phrase. "Vertical tracer diffusivity" means the vertical component of the diffusivity of tracers, i.e. heat and salinity, due to motion which is not resolved on the grid scale of the model.</rdfs:comment>
	<rdfs:label>ocean vertical tracer diffusivity due to wind mixing</rdfs:label>
	<generalQuantityKind xmlns="http://purl.oclc.org/NET/ssnx/qu/qu#" rdf:resource="http://purl.oclc.org/NET/ssnx/qu/quantity#diffusionCoefficient"/>
	<rdfs:isDefinedBy rdf:resource="http://purl.oclc.org/NET/ssnx/cf/cf-property"/>
</rdf:Description>

<rdf:Description rdf:about="http://purl.oclc.org/NET/ssnx/cf/cf-property#product_of_eastward_wind_and_geopotential_height">
	<rdf:type rdf:resource="http://www.w3.org/2004/02/skos/core#Concept"/>
	<skos:inScheme rdf:resource="http://purl.oclc.org/NET/ssnx/qu/dim#DiffusionCoefficient"/>
	<rdfs:comment>"product_of_X_and_Y" means X*Y. Geopotential is the sum of the specific gravitational potential energy relative to the geoid and the specific centripetal potential energy. Geopotential height is the geopotential divided by the standard acceleration due to gravity. It is numerically similar to the altitude (or geometric height) and not to the quantity with standard name height, which is relative to the surface. "Eastward" indicates a vector component which is positive when directed eastward (negative westward). Wind is defined as a two-dimensional (horizontal) air velocity vector, with no vertical component. (Vertical motion in the atmosphere has the standard name upward_air_velocity.)</rdfs:comment>
	<rdfs:label>product of eastward wind and geopotential height</rdfs:label>
	<generalQuantityKind xmlns="http://purl.oclc.org/NET/ssnx/qu/qu#" rdf:resource="http://purl.oclc.org/NET/ssnx/qu/quantity#diffusionCoefficient"/>
	<rdfs:isDefinedBy rdf:resource="http://purl.oclc.org/NET/ssnx/cf/cf-property"/>
</rdf:Description>

<rdf:Description rdf:about="http://purl.oclc.org/NET/ssnx/cf/cf-property#product_of_northward_wind_and_geopotential_height">
	<rdf:type rdf:resource="http://www.w3.org/2004/02/skos/core#Concept"/>
	<skos:inScheme rdf:resource="http://purl.oclc.org/NET/ssnx/qu/dim#DiffusionCoefficient"/>
	<rdfs:comment>"product_of_X_and_Y" means X*Y. Geopotential is the sum of the specific gravitational potential energy relative to the geoid and the specific centripetal potential energy. Geopotential height is the geopotential divided by the standard acceleration due to gravity. It is numerically similar to the altitude (or geometric height) and not to the quantity with standard name height, which is relative to the surface. "Northward" indicates a vector component which is positive when directed northward (negative southward). Wind is defined as a two-dimensional (horizontal) air velocity vector, with no vertical component. (Vertical motion in the atmosphere has the standard name upward_air_velocity.)</rdfs:comment>
	<rdfs:label>product of northward wind and geopotential height</rdfs:label>
	<generalQuantityKind xmlns="http://purl.oclc.org/NET/ssnx/qu/qu#" rdf:resource="http://purl.oclc.org/NET/ssnx/qu/quantity#diffusionCoefficient"/>
	<rdfs:isDefinedBy rdf:resource="http://purl.oclc.org/NET/ssnx/cf/cf-property"/>
</rdf:Description>

<rdf:Description rdf:about="http://purl.oclc.org/NET/ssnx/cf/cf-property#vertical_component_of_ocean_xy_tracer_diffusivity">
	<rdf:type rdf:resource="http://www.w3.org/2004/02/skos/core#Concept"/>
	<skos:inScheme rdf:resource="http://purl.oclc.org/NET/ssnx/qu/dim#DiffusionCoefficient"/>
	<rdfs:comment>The vertical_component_of_ocean_xy_tracer_diffusivity means the vertical component of the diffusivity of tracers in the ocean due to lateral mixing. This quantity could appear in formulations of lateral diffusivity in which "lateral" does not mean "iso-level", e.g. it would not be used for isopycnal diffusivity. "Tracer diffusivity" means the diffusivity of heat and salinity due to motion which is not resolved on the grid scale of the model.</rdfs:comment>
	<rdfs:label>vertical component of ocean xy tracer diffusivity</rdfs:label>
	<generalQuantityKind xmlns="http://purl.oclc.org/NET/ssnx/qu/qu#" rdf:resource="http://purl.oclc.org/NET/ssnx/qu/quantity#diffusionCoefficient"/>
	<rdfs:isDefinedBy rdf:resource="http://purl.oclc.org/NET/ssnx/cf/cf-property"/>
</rdf:Description>

</rdf:RDF>