<?xml version="1.0" encoding="UTF-8"?>
<rdf:RDF
	xmlns:vann="http://purl.org/vocab/vann/"
	xmlns:voaf="http://purl.org/vocommons/voaf#"
	xmlns:rdfs="http://www.w3.org/2000/01/rdf-schema#"
	xmlns:owl="http://www.w3.org/2002/07/owl#"
	xmlns:skos="http://www.w3.org/2004/02/skos/core#"
	xmlns:rdf="http://www.w3.org/1999/02/22-rdf-syntax-ns#"
	xmlns:dcterms="http://purl.org/dc/terms/"
	xmlns:dc="http://purl.org/dc/elements/1.1/"
	xmlns:dcmit="http://purl.org/dc/dcmitype/"
	xmlns:sesame="http://www.openrdf.org/schema/sesame#"
	xmlns:xsd="http://www.w3.org/2001/XMLSchema#"
	xmlns:fn="http://www.w3.org/2005/xpath-functions#"
	xmlns:foaf="http://xmlns.com/foaf/0.1/"
	xmlns:hint="http://www.bigdata.com/queryHints#"
	xmlns:bd="http://www.bigdata.com/rdf#"
	xmlns:bds="http://www.bigdata.com/rdf/search#">

<rdf:Description rdf:about="http://www.ebusiness-unibw.org/ontologies/consumerelectronics/v1">
	<rdf:type rdf:resource="http://www.w3.org/2002/07/owl#Ontology"/>
</rdf:Description>

<rdf:Description rdf:about="http://www.ebusiness-unibw.org/ontologies/consumerelectronics/v1#SignalFormat">
	<rdf:type rdf:resource="http://www.w3.org/2004/02/skos/core#ConceptScheme"/>
</rdf:Description>

<rdf:Description rdf:about="http://www.ebusiness-unibw.org/ontologies/consumerelectronics/v1#DVB">
	<rdf:type rdf:resource="http://www.w3.org/2004/02/skos/core#Concept"/>
	<skos:inScheme rdf:resource="http://www.ebusiness-unibw.org/ontologies/consumerelectronics/v1#SignalFormat"/>
</rdf:Description>

<rdf:Description rdf:about="http://www.ebusiness-unibw.org/ontologies/consumerelectronics/v1#SignalFormat">
	<rdfs:comment xml:lang="en">Type of the transmitted video format signal that is displayed by a monitor or TV panel.</rdfs:comment>
	<rdfs:label xml:lang="en">Signal format</rdfs:label>
</rdf:Description>

<rdf:Description rdf:about="http://www.ebusiness-unibw.org/ontologies/consumerelectronics/v1#DVB">
	<rdfs:comment xml:lang="en">Digital Video Broadcasting (DVB) is a suite of internationally accepted open standards for digital television. DVB systems distribute data using a variety of approaches, including by satellite (DVB-S, DVB-S2 and DVB-SH; also DVB-SMATV for distribution via SMATV); cable (DVB-C); terrestrial television (DVB-T, DVB-T2) and digital terrestrial television for handhelds (DVB-H,DVB-SH); and via microwave using DTT (DVB-MT), the MMDS (DVB-MC), and/or MVDS standards (DVB-MS).

(This description is partly based on or reuses content from the Wikipedia article "Digital Video Broadcasting" (http://en.wikipedia.org/wiki/Digital_Video_Broadcasting) and is licensed under the GNU Free Documentation License (http://www.gnu.org/copyleft/fdl.html).)</rdfs:comment>
	<rdfs:label xml:lang="en">DVB</rdfs:label>
</rdf:Description>

<rdf:Description rdf:about="http://www.ebusiness-unibw.org/ontologies/consumerelectronics/v1#SignalFormat">
	<rdfs:isDefinedBy rdf:resource="http://www.ebusiness-unibw.org/ontologies/consumerelectronics/v1"/>
</rdf:Description>

<rdf:Description rdf:about="http://www.ebusiness-unibw.org/ontologies/consumerelectronics/v1#DVB">
	<rdfs:isDefinedBy rdf:resource="http://www.ebusiness-unibw.org/ontologies/consumerelectronics/v1"/>
</rdf:Description>

<rdf:Description rdf:about="http://www.ebusiness-unibw.org/ontologies/consumerelectronics/v1#DVB_COFDM">
	<rdf:type rdf:resource="http://www.w3.org/2004/02/skos/core#Concept"/>
	<skos:inScheme rdf:resource="http://www.ebusiness-unibw.org/ontologies/consumerelectronics/v1#SignalFormat"/>
	<rdfs:comment xml:lang="en">Digital Video Broadcasting (DVB) is a suite of internationally accepted open standards for digital television. Coded OFDM (COFDM) and Discrete multi-tone modulation (DMT) is a frequency-division multiplexing (FDM) scheme utilized as a digital multi-carrier modulation method. A large number of closely-spaced orthogonal sub-carriers are used to carry data. The data is divided into several parallel data streams or channels, one for each sub-carrier. Each sub-carrier is modulated with a conventional modulation scheme (such as quadrature amplitude modulation or phase shift keying) at a low symbol rate, maintaining total data rates similar to conventional single-carrier modulation schemes in the same bandwidth.

(This description is partly based on or reuses content from the Wikipedia article "Digital Video Broadcasting" (http://en.wikipedia.org/wiki/Digital_Video_Broadcasting) and is licensed under the GNU Free Documentation License (http://www.gnu.org/copyleft/fdl.html).)</rdfs:comment>
	<rdfs:label xml:lang="en">DVB COFDM</rdfs:label>
	<rdfs:isDefinedBy rdf:resource="http://www.ebusiness-unibw.org/ontologies/consumerelectronics/v1"/>
</rdf:Description>

<rdf:Description rdf:about="http://www.ebusiness-unibw.org/ontologies/consumerelectronics/v1#Hyperband">
	<rdf:type rdf:resource="http://www.w3.org/2004/02/skos/core#Concept"/>
	<skos:inScheme rdf:resource="http://www.ebusiness-unibw.org/ontologies/consumerelectronics/v1#SignalFormat"/>
	<rdfs:comment xml:lang="en">Hyperband designates a range (band) of electromagnetic waves with frequencies between 300 MHz and 470 MHz. This is designated for kable TV especially to recieve digital TV normed for DVB-C.</rdfs:comment>
	<rdfs:label xml:lang="en">Hyperband</rdfs:label>
	<rdfs:isDefinedBy rdf:resource="http://www.ebusiness-unibw.org/ontologies/consumerelectronics/v1"/>
</rdf:Description>

<rdf:Description rdf:about="http://www.ebusiness-unibw.org/ontologies/consumerelectronics/v1#NICAM">
	<rdf:type rdf:resource="http://www.w3.org/2004/02/skos/core#Concept"/>
	<skos:inScheme rdf:resource="http://www.ebusiness-unibw.org/ontologies/consumerelectronics/v1#SignalFormat"/>
	<rdfs:comment xml:lang="en">NICAM stands for Near Instantaneous Companded Audio Multiplex. It is an early form of lossy compression for digital audio.

(This description is partly based on or reuses content from the Wikipedia article "NICAM" (http://en.wikipedia.org/wiki/NICAM) and is licensed under the GNU Free Documentation License (http://www.gnu.org/copyleft/fdl.html).)</rdfs:comment>
	<rdfs:label xml:lang="en">NICAM</rdfs:label>
	<rdfs:isDefinedBy rdf:resource="http://www.ebusiness-unibw.org/ontologies/consumerelectronics/v1"/>
</rdf:Description>

<rdf:Description rdf:about="http://www.ebusiness-unibw.org/ontologies/consumerelectronics/v1#NTSC">
	<rdf:type rdf:resource="http://www.w3.org/2004/02/skos/core#Concept"/>
	<skos:inScheme rdf:resource="http://www.ebusiness-unibw.org/ontologies/consumerelectronics/v1#SignalFormat"/>
	<rdfs:comment xml:lang="en">NTSC (National Television Standard Conversion) is the analog television system used in most of the Americas, Japan, South Korea, Taiwan, the Philippines, Burma, and some Pacific island nations and territories.

(This description is partly based on or reuses content from the Wikipedia article "NTSC" (http://en.wikipedia.org/wiki/NTSC) and is licensed under the GNU Free Documentation License (http://www.gnu.org/copyleft/fdl.html).)</rdfs:comment>
	<rdfs:label xml:lang="en">NTSC</rdfs:label>
	<rdfs:isDefinedBy rdf:resource="http://www.ebusiness-unibw.org/ontologies/consumerelectronics/v1"/>
</rdf:Description>

<rdf:Description rdf:about="http://www.ebusiness-unibw.org/ontologies/consumerelectronics/v1#PAL">
	<rdf:type rdf:resource="http://www.w3.org/2004/02/skos/core#Concept"/>
	<skos:inScheme rdf:resource="http://www.ebusiness-unibw.org/ontologies/consumerelectronics/v1#SignalFormat"/>
	<rdfs:comment xml:lang="en">PAL, short for Phase Alternating Line, is a colour-encoding system used in broadcast television systems in large parts of the world.

(This description is partly based on or reuses content from the Wikipedia article "PAL" (http://en.wikipedia.org/wiki/PAL) and is licensed under the GNU Free Documentation License (http://www.gnu.org/copyleft/fdl.html).)</rdfs:comment>
	<rdfs:label xml:lang="en">PAL</rdfs:label>
	<rdfs:isDefinedBy rdf:resource="http://www.ebusiness-unibw.org/ontologies/consumerelectronics/v1"/>
</rdf:Description>

<rdf:Description rdf:about="http://www.ebusiness-unibw.org/ontologies/consumerelectronics/v1#PAL-B_G">
	<rdf:type rdf:resource="http://www.w3.org/2004/02/skos/core#Concept"/>
	<skos:inScheme rdf:resource="http://www.ebusiness-unibw.org/ontologies/consumerelectronics/v1#SignalFormat"/>
	<rdfs:comment xml:lang="en">PAL, short for Phase Alternating Line, is a colour-encoding system used in broadcast television systems in large parts of the world. This is used in western europe.

(This description is partly based on or reuses content from the Wikipedia article "PAL" (http://en.wikipedia.org/wiki/PAL) and is licensed under the GNU Free Documentation License (http://www.gnu.org/copyleft/fdl.html).)</rdfs:comment>
	<rdfs:label xml:lang="en">PAL-B G</rdfs:label>
	<rdfs:isDefinedBy rdf:resource="http://www.ebusiness-unibw.org/ontologies/consumerelectronics/v1"/>
</rdf:Description>

<rdf:Description rdf:about="http://www.ebusiness-unibw.org/ontologies/consumerelectronics/v1#PAL-I">
	<rdf:type rdf:resource="http://www.w3.org/2004/02/skos/core#Concept"/>
	<skos:inScheme rdf:resource="http://www.ebusiness-unibw.org/ontologies/consumerelectronics/v1#SignalFormat"/>
	<rdfs:comment xml:lang="en">PAL, short for Phase Alternating Line, is a colour-encoding system used in broadcast television systems in large parts of the world. This is only used in Ireland, the UK, Hongkong and Macau.

(This description is partly based on or reuses content from the Wikipedia article "PAL" (http://en.wikipedia.org/wiki/PAL) and is licensed under the GNU Free Documentation License (http://www.gnu.org/copyleft/fdl.html).)</rdfs:comment>
	<rdfs:label xml:lang="en">PAL-I</rdfs:label>
	<rdfs:isDefinedBy rdf:resource="http://www.ebusiness-unibw.org/ontologies/consumerelectronics/v1"/>
</rdf:Description>

<rdf:Description rdf:about="http://www.ebusiness-unibw.org/ontologies/consumerelectronics/v1#PAL-L">
	<rdf:type rdf:resource="http://www.w3.org/2004/02/skos/core#Concept"/>
	<skos:inScheme rdf:resource="http://www.ebusiness-unibw.org/ontologies/consumerelectronics/v1#SignalFormat"/>
	<rdfs:comment xml:lang="en">PAL, short for Phase Alternating Line, is a colour-encoding system used in broadcast television systems in large parts of the world. PAL L is used on some hotel internal distribution systems, as well as other public display and plant television systems.

(This description is partly based on or reuses content from the Wikipedia article "PAL" (http://en.wikipedia.org/wiki/PAL) and is licensed under the GNU Free Documentation License (http://www.gnu.org/copyleft/fdl.html).)</rdfs:comment>
	<rdfs:label xml:lang="en">PAL-L</rdfs:label>
	<rdfs:isDefinedBy rdf:resource="http://www.ebusiness-unibw.org/ontologies/consumerelectronics/v1"/>
</rdf:Description>

<rdf:Description rdf:about="http://www.ebusiness-unibw.org/ontologies/consumerelectronics/v1#SECAM">
	<rdf:type rdf:resource="http://www.w3.org/2004/02/skos/core#Concept"/>
	<skos:inScheme rdf:resource="http://www.ebusiness-unibw.org/ontologies/consumerelectronics/v1#SignalFormat"/>
	<rdfs:comment xml:lang="en">SECAM, also written SÉCAM (Séquentiel couleur à mémoire, French for "Sequential Color with Memory"), is an analog color television system first used in France.

(This description is partly based on or reuses content from the Wikipedia article "SECAM" (http://en.wikipedia.org/wiki/SECAM) and is licensed under the GNU Free Documentation License (http://www.gnu.org/copyleft/fdl.html).)</rdfs:comment>
	<rdfs:label xml:lang="en">SECAM</rdfs:label>
	<rdfs:isDefinedBy rdf:resource="http://www.ebusiness-unibw.org/ontologies/consumerelectronics/v1"/>
</rdf:Description>

<rdf:Description rdf:about="http://www.ebusiness-unibw.org/ontologies/consumerelectronics/v1#SECAM-B_G">
	<rdf:type rdf:resource="http://www.w3.org/2004/02/skos/core#Concept"/>
	<skos:inScheme rdf:resource="http://www.ebusiness-unibw.org/ontologies/consumerelectronics/v1#SignalFormat"/>
	<rdfs:comment xml:lang="en">SECAM, also written SÉCAM (Séquentiel couleur à mémoire, French for "Sequential Color with Memory"), is an analog color television system first used in France. SECAM-B/G is used in the Middle East, former East Germany and Greece.

(This description is partly based on or reuses content from the Wikipedia article "SECAM" (http://en.wikipedia.org/wiki/SECAM) and is licensed under the GNU Free Documentation License (http://www.gnu.org/copyleft/fdl.html).)</rdfs:comment>
	<rdfs:label xml:lang="en">SECAM-B G</rdfs:label>
	<rdfs:isDefinedBy rdf:resource="http://www.ebusiness-unibw.org/ontologies/consumerelectronics/v1"/>
</rdf:Description>

<rdf:Description rdf:about="http://www.ebusiness-unibw.org/ontologies/consumerelectronics/v1#SECAM-D_K">
	<rdf:type rdf:resource="http://www.w3.org/2004/02/skos/core#Concept"/>
	<skos:inScheme rdf:resource="http://www.ebusiness-unibw.org/ontologies/consumerelectronics/v1#SignalFormat"/>
	<rdfs:comment xml:lang="en">SECAM, also written SÉCAM (Séquentiel couleur à mémoire, French for "Sequential Color with Memory"), is an analog color television system first used in France. SECAM D/K is used in the Commonwealth of Independent States and Eastern Europe (this is simply SECAM used with the D and K monochrome TV transmission standards).

(This description is partly based on or reuses content from the Wikipedia article "SECAM" (http://en.wikipedia.org/wiki/SECAM) and is licensed under the GNU Free Documentation License (http://www.gnu.org/copyleft/fdl.html).)</rdfs:comment>
	<rdfs:label xml:lang="en">SECAM-D K</rdfs:label>
	<rdfs:isDefinedBy rdf:resource="http://www.ebusiness-unibw.org/ontologies/consumerelectronics/v1"/>
</rdf:Description>

<rdf:Description rdf:about="http://www.ebusiness-unibw.org/ontologies/consumerelectronics/v1#SECAM-L">
	<rdf:type rdf:resource="http://www.w3.org/2004/02/skos/core#Concept"/>
	<skos:inScheme rdf:resource="http://www.ebusiness-unibw.org/ontologies/consumerelectronics/v1#SignalFormat"/>
	<rdfs:comment xml:lang="en">SECAM, also written SÉCAM (Séquentiel couleur à mémoire, French for "Sequential Color with Memory"), is an analog color television system first used in France. French SECAM (SECAM-L) is used only in France, Luxembourg (only RTL9 on CH 21 from Dudelange) and Tele Monte-Carlo Transmitters in the south of France.

(This description is partly based on or reuses content from the Wikipedia article "SECAM" (http://en.wikipedia.org/wiki/SECAM) and is licensed under the GNU Free Documentation License (http://www.gnu.org/copyleft/fdl.html).)</rdfs:comment>
	<rdfs:label xml:lang="en">SECAM-L</rdfs:label>
	<rdfs:isDefinedBy rdf:resource="http://www.ebusiness-unibw.org/ontologies/consumerelectronics/v1"/>
</rdf:Description>

<rdf:Description rdf:about="http://www.ebusiness-unibw.org/ontologies/consumerelectronics/v1#UHF">
	<rdf:type rdf:resource="http://www.w3.org/2004/02/skos/core#Concept"/>
	<skos:inScheme rdf:resource="http://www.ebusiness-unibw.org/ontologies/consumerelectronics/v1#SignalFormat"/>
	<rdfs:comment xml:lang="en">Ultra high frequency (UHF) designates a range (band) of electromagnetic waves with frequencies between 300 MHz and 3 GHz (3,000 MHz).

(This description is partly based on or reuses content from the Wikipedia article "UHF" (http://en.wikipedia.org/wiki/UHF) and is licensed under the GNU Free Documentation License (http://www.gnu.org/copyleft/fdl.html).)</rdfs:comment>
	<rdfs:label xml:lang="en">UHF</rdfs:label>
	<rdfs:isDefinedBy rdf:resource="http://www.ebusiness-unibw.org/ontologies/consumerelectronics/v1"/>
</rdf:Description>

<rdf:Description rdf:about="http://www.ebusiness-unibw.org/ontologies/consumerelectronics/v1#VHF">
	<rdf:type rdf:resource="http://www.w3.org/2004/02/skos/core#Concept"/>
	<skos:inScheme rdf:resource="http://www.ebusiness-unibw.org/ontologies/consumerelectronics/v1#SignalFormat"/>
	<rdfs:comment xml:lang="en">VHF (Very high frequency) is the radio frequency range from 30 MHz to 300 MHz.

(This description is partly based on or reuses content from the Wikipedia article "VHF" (http://en.wikipedia.org/wiki/VHF) and is licensed under the GNU Free Documentation License (http://www.gnu.org/copyleft/fdl.html).)</rdfs:comment>
	<rdfs:label xml:lang="en">VHF</rdfs:label>
	<rdfs:isDefinedBy rdf:resource="http://www.ebusiness-unibw.org/ontologies/consumerelectronics/v1"/>
</rdf:Description>

</rdf:RDF>