<?xml version="1.0" encoding="UTF-8"?>
<rdf:RDF
	xmlns:vann="http://purl.org/vocab/vann/"
	xmlns:voaf="http://purl.org/vocommons/voaf#"
	xmlns:rdfs="http://www.w3.org/2000/01/rdf-schema#"
	xmlns:owl="http://www.w3.org/2002/07/owl#"
	xmlns:skos="http://www.w3.org/2004/02/skos/core#"
	xmlns:rdf="http://www.w3.org/1999/02/22-rdf-syntax-ns#"
	xmlns:dcterms="http://purl.org/dc/terms/"
	xmlns:dc="http://purl.org/dc/elements/1.1/"
	xmlns:dcmit="http://purl.org/dc/dcmitype/"
	xmlns:sesame="http://www.openrdf.org/schema/sesame#"
	xmlns:xsd="http://www.w3.org/2001/XMLSchema#"
	xmlns:fn="http://www.w3.org/2005/xpath-functions#"
	xmlns:foaf="http://xmlns.com/foaf/0.1/"
	xmlns:hint="http://www.bigdata.com/queryHints#"
	xmlns:bd="http://www.bigdata.com/rdf#"
	xmlns:bds="http://www.bigdata.com/rdf/search#">

<rdf:Description rdf:about="http://purl.oclc.org/NET/ssnx/cf/cf-property">
	<rdf:type rdf:resource="http://www.w3.org/2002/07/owl#Ontology"/>
</rdf:Description>

<rdf:Description rdf:about="http://purl.oclc.org/NET/ssnx/qu/dim#Temperature">
	<rdf:type rdf:resource="http://www.w3.org/2004/02/skos/core#ConceptScheme"/>
</rdf:Description>

<rdf:Description rdf:about="http://purl.oclc.org/NET/ssnx/cf/cf-property#air_potential_temperature">
	<rdf:type rdf:resource="http://www.w3.org/2004/02/skos/core#Concept"/>
	<skos:inScheme rdf:resource="http://purl.oclc.org/NET/ssnx/qu/dim#Temperature"/>
	<rdfs:comment>Potential temperature is the temperature a parcel of air or sea water would have if moved adiabatically to sea level pressure.</rdfs:comment>
	<rdfs:label>air potential temperature</rdfs:label>
	<generalQuantityKind xmlns="http://purl.oclc.org/NET/ssnx/qu/qu#" rdf:resource="http://purl.oclc.org/NET/ssnx/qu/quantity#temperature"/>
</rdf:Description>

<rdf:Description rdf:about="http://purl.oclc.org/NET/ssnx/qu/quantity#temperature">
	<rdf:type rdf:resource="http://www.w3.org/2004/02/skos/core#Concept"/>
</rdf:Description>

<rdf:Description rdf:about="http://purl.oclc.org/NET/ssnx/qu/dim#Temperature">
	<rdfs:isDefinedBy rdf:resource="http://purl.oclc.org/NET/ssnx/cf/cf-property"/>
</rdf:Description>

<rdf:Description rdf:about="http://purl.oclc.org/NET/ssnx/cf/cf-property#air_potential_temperature">
	<rdfs:isDefinedBy rdf:resource="http://purl.oclc.org/NET/ssnx/cf/cf-property"/>
</rdf:Description>

<rdf:Description rdf:about="http://purl.oclc.org/NET/ssnx/qu/quantity#temperature">
	<rdfs:isDefinedBy rdf:resource="http://purl.oclc.org/NET/ssnx/cf/cf-property"/>
</rdf:Description>

<rdf:Description rdf:about="http://purl.oclc.org/NET/ssnx/cf/cf-property#air_temperature">
	<rdf:type rdf:resource="http://www.w3.org/2004/02/skos/core#Concept"/>
	<skos:inScheme rdf:resource="http://purl.oclc.org/NET/ssnx/qu/dim#Temperature"/>
	<rdfs:comment>Air temperature is the bulk temperature of the air, not the surface (skin) temperature.</rdfs:comment>
	<rdfs:label>air temperature</rdfs:label>
	<generalQuantityKind xmlns="http://purl.oclc.org/NET/ssnx/qu/qu#" rdf:resource="http://purl.oclc.org/NET/ssnx/qu/quantity#temperature"/>
	<rdfs:isDefinedBy rdf:resource="http://purl.oclc.org/NET/ssnx/cf/cf-property"/>
</rdf:Description>

<rdf:Description rdf:about="http://purl.oclc.org/NET/ssnx/cf/cf-property#air_temperature_anomaly">
	<rdf:type rdf:resource="http://www.w3.org/2004/02/skos/core#Concept"/>
	<skos:inScheme rdf:resource="http://purl.oclc.org/NET/ssnx/qu/dim#Temperature"/>
	<rdfs:comment>"anomaly" means difference from climatology. Air temperature is the bulk temperature of the air, not the surface (skin) temperature.</rdfs:comment>
	<rdfs:label>air temperature anomaly</rdfs:label>
	<generalQuantityKind xmlns="http://purl.oclc.org/NET/ssnx/qu/qu#" rdf:resource="http://purl.oclc.org/NET/ssnx/qu/quantity#temperature"/>
	<rdfs:isDefinedBy rdf:resource="http://purl.oclc.org/NET/ssnx/cf/cf-property"/>
</rdf:Description>

<rdf:Description rdf:about="http://purl.oclc.org/NET/ssnx/cf/cf-property#air_temperature_at_cloud_top">
	<rdf:type rdf:resource="http://www.w3.org/2004/02/skos/core#Concept"/>
	<skos:inScheme rdf:resource="http://purl.oclc.org/NET/ssnx/qu/dim#Temperature"/>
	<rdfs:comment>cloud_top refers to the top of the highest cloud. Air temperature is the bulk temperature of the air, not the surface (skin) temperature.</rdfs:comment>
	<rdfs:label>air temperature at cloud top</rdfs:label>
	<generalQuantityKind xmlns="http://purl.oclc.org/NET/ssnx/qu/qu#" rdf:resource="http://purl.oclc.org/NET/ssnx/qu/quantity#temperature"/>
	<rdfs:isDefinedBy rdf:resource="http://purl.oclc.org/NET/ssnx/cf/cf-property"/>
</rdf:Description>

<rdf:Description rdf:about="http://purl.oclc.org/NET/ssnx/cf/cf-property#air_temperature_threshold">
	<rdf:type rdf:resource="http://www.w3.org/2004/02/skos/core#Concept"/>
	<skos:inScheme rdf:resource="http://purl.oclc.org/NET/ssnx/qu/dim#Temperature"/>
	<rdfs:comment>Air temperature is the bulk temperature of the air, not the surface (skin) temperature. Air temperature excess and deficit are calculated relative to the air temperature threshold.</rdfs:comment>
	<rdfs:label>air temperature threshold</rdfs:label>
	<generalQuantityKind xmlns="http://purl.oclc.org/NET/ssnx/qu/qu#" rdf:resource="http://purl.oclc.org/NET/ssnx/qu/quantity#temperature"/>
	<rdfs:isDefinedBy rdf:resource="http://purl.oclc.org/NET/ssnx/cf/cf-property"/>
</rdf:Description>

<rdf:Description rdf:about="http://purl.oclc.org/NET/ssnx/cf/cf-property#brightness_temperature">
	<rdf:type rdf:resource="http://www.w3.org/2004/02/skos/core#Concept"/>
	<skos:inScheme rdf:resource="http://purl.oclc.org/NET/ssnx/qu/dim#Temperature"/>
	<rdfs:comment>The brightness temperature of a body is the temperature of a black body which radiates the same power per unit solid angle per unit area.</rdfs:comment>
	<rdfs:label>brightness temperature</rdfs:label>
	<generalQuantityKind xmlns="http://purl.oclc.org/NET/ssnx/qu/qu#" rdf:resource="http://purl.oclc.org/NET/ssnx/qu/quantity#temperature"/>
	<rdfs:isDefinedBy rdf:resource="http://purl.oclc.org/NET/ssnx/cf/cf-property"/>
</rdf:Description>

<rdf:Description rdf:about="http://purl.oclc.org/NET/ssnx/cf/cf-property#canopy_temperature">
	<rdf:type rdf:resource="http://www.w3.org/2004/02/skos/core#Concept"/>
	<skos:inScheme rdf:resource="http://purl.oclc.org/NET/ssnx/qu/dim#Temperature"/>
	<rdfs:comment>"Canopy" means the plant or vegetation canopy.  "Canopy_temperature" is the bulk temperature of the canopy, not the surface (skin) temperature.
</rdfs:comment>
	<rdfs:label>canopy temperature</rdfs:label>
	<generalQuantityKind xmlns="http://purl.oclc.org/NET/ssnx/qu/qu#" rdf:resource="http://purl.oclc.org/NET/ssnx/qu/quantity#temperature"/>
	<rdfs:isDefinedBy rdf:resource="http://purl.oclc.org/NET/ssnx/cf/cf-property"/>
</rdf:Description>

<rdf:Description rdf:about="http://purl.oclc.org/NET/ssnx/cf/cf-property#dew_point_depression">
	<rdf:type rdf:resource="http://www.w3.org/2004/02/skos/core#Concept"/>
	<skos:inScheme rdf:resource="http://purl.oclc.org/NET/ssnx/qu/dim#Temperature"/>
	<rdfs:comment>Dew point depression is also called dew point deficit. It is the amount by which the air temperature exceeds its dew point temperature. Dew point temperature is the temperature at which a parcel of air reaches saturation upon being cooled at constant pressure and specific humidity.</rdfs:comment>
	<rdfs:label>dew point depression</rdfs:label>
	<generalQuantityKind xmlns="http://purl.oclc.org/NET/ssnx/qu/qu#" rdf:resource="http://purl.oclc.org/NET/ssnx/qu/quantity#temperature"/>
	<rdfs:isDefinedBy rdf:resource="http://purl.oclc.org/NET/ssnx/cf/cf-property"/>
</rdf:Description>

<rdf:Description rdf:about="http://purl.oclc.org/NET/ssnx/cf/cf-property#dew_point_temperature">
	<rdf:type rdf:resource="http://www.w3.org/2004/02/skos/core#Concept"/>
	<skos:inScheme rdf:resource="http://purl.oclc.org/NET/ssnx/qu/dim#Temperature"/>
	<rdfs:comment>Dew point temperature is the temperature at which a parcel of air reaches saturation upon being cooled at constant pressure and specific humidity.</rdfs:comment>
	<rdfs:label>dew point temperature</rdfs:label>
	<generalQuantityKind xmlns="http://purl.oclc.org/NET/ssnx/qu/qu#" rdf:resource="http://purl.oclc.org/NET/ssnx/qu/quantity#temperature"/>
	<rdfs:isDefinedBy rdf:resource="http://purl.oclc.org/NET/ssnx/cf/cf-property"/>
</rdf:Description>

<rdf:Description rdf:about="http://purl.oclc.org/NET/ssnx/cf/cf-property#dynamic_tropopause_potential_temperature">
	<rdf:type rdf:resource="http://www.w3.org/2004/02/skos/core#Concept"/>
	<skos:inScheme rdf:resource="http://purl.oclc.org/NET/ssnx/qu/dim#Temperature"/>
	<rdfs:comment>The dynamical tropopause used in interpreting the dynamics of the upper troposphere and lower stratosphere.  There are various definitions of dynamical tropopause in the scientific literature.</rdfs:comment>
	<rdfs:label>dynamic tropopause potential temperature</rdfs:label>
	<generalQuantityKind xmlns="http://purl.oclc.org/NET/ssnx/qu/qu#" rdf:resource="http://purl.oclc.org/NET/ssnx/qu/quantity#temperature"/>
	<rdfs:isDefinedBy rdf:resource="http://purl.oclc.org/NET/ssnx/cf/cf-property"/>
</rdf:Description>

<rdf:Description rdf:about="http://purl.oclc.org/NET/ssnx/cf/cf-property#equivalent_potential_temperature">
	<rdf:type rdf:resource="http://www.w3.org/2004/02/skos/core#Concept"/>
	<skos:inScheme rdf:resource="http://purl.oclc.org/NET/ssnx/qu/dim#Temperature"/>
	<rdfs:comment>Potential temperature is the temperature a parcel of air or sea water would have if moved adiabatically to sea level pressure.</rdfs:comment>
	<rdfs:label>equivalent potential temperature</rdfs:label>
	<generalQuantityKind xmlns="http://purl.oclc.org/NET/ssnx/qu/qu#" rdf:resource="http://purl.oclc.org/NET/ssnx/qu/quantity#temperature"/>
	<rdfs:isDefinedBy rdf:resource="http://purl.oclc.org/NET/ssnx/cf/cf-property"/>
</rdf:Description>

<rdf:Description rdf:about="http://purl.oclc.org/NET/ssnx/cf/cf-property#equivalent_temperature">
	<rdf:type rdf:resource="http://www.w3.org/2004/02/skos/core#Concept"/>
	<skos:inScheme rdf:resource="http://purl.oclc.org/NET/ssnx/qu/dim#Temperature"/>
	<rdfs:label>equivalent temperature</rdfs:label>
	<generalQuantityKind xmlns="http://purl.oclc.org/NET/ssnx/qu/qu#" rdf:resource="http://purl.oclc.org/NET/ssnx/qu/quantity#temperature"/>
	<rdfs:isDefinedBy rdf:resource="http://purl.oclc.org/NET/ssnx/cf/cf-property"/>
</rdf:Description>

<rdf:Description rdf:about="http://purl.oclc.org/NET/ssnx/cf/cf-property#freezing_temperature_of_sea_water">
	<rdf:type rdf:resource="http://www.w3.org/2004/02/skos/core#Concept"/>
	<skos:inScheme rdf:resource="http://purl.oclc.org/NET/ssnx/qu/dim#Temperature"/>
	<rdfs:label>freezing temperature of sea water</rdfs:label>
	<generalQuantityKind xmlns="http://purl.oclc.org/NET/ssnx/qu/qu#" rdf:resource="http://purl.oclc.org/NET/ssnx/qu/quantity#temperature"/>
	<rdfs:isDefinedBy rdf:resource="http://purl.oclc.org/NET/ssnx/cf/cf-property"/>
</rdf:Description>

<rdf:Description rdf:about="http://purl.oclc.org/NET/ssnx/cf/cf-property#land_ice_temperature">
	<rdf:type rdf:resource="http://www.w3.org/2004/02/skos/core#Concept"/>
	<skos:inScheme rdf:resource="http://purl.oclc.org/NET/ssnx/qu/dim#Temperature"/>
	<rdfs:comment>"Land ice" means glaciers, ice-caps and ice-sheets resting on bedrock and also includes ice-shelves.</rdfs:comment>
	<rdfs:label>land ice temperature</rdfs:label>
	<generalQuantityKind xmlns="http://purl.oclc.org/NET/ssnx/qu/qu#" rdf:resource="http://purl.oclc.org/NET/ssnx/qu/quantity#temperature"/>
	<rdfs:isDefinedBy rdf:resource="http://purl.oclc.org/NET/ssnx/cf/cf-property"/>
</rdf:Description>

<rdf:Description rdf:about="http://purl.oclc.org/NET/ssnx/cf/cf-property#product_of_air_temperature_and_specific_humidity">
	<rdf:type rdf:resource="http://www.w3.org/2004/02/skos/core#Concept"/>
	<skos:inScheme rdf:resource="http://purl.oclc.org/NET/ssnx/qu/dim#Temperature"/>
	<rdfs:comment>"product_of_X_and_Y" means X*Y. "specific" means per unit mass. Air temperature is the bulk temperature of the air, not the surface (skin) temperature. Specific humidity is the mass fraction of water vapor in (moist) air.</rdfs:comment>
	<rdfs:label>product of air temperature and specific humidity</rdfs:label>
	<generalQuantityKind xmlns="http://purl.oclc.org/NET/ssnx/qu/qu#" rdf:resource="http://purl.oclc.org/NET/ssnx/qu/quantity#temperature"/>
	<rdfs:isDefinedBy rdf:resource="http://purl.oclc.org/NET/ssnx/cf/cf-property"/>
</rdf:Description>

<rdf:Description rdf:about="http://purl.oclc.org/NET/ssnx/cf/cf-property#pseudo_equivalent_potential_temperature">
	<rdf:type rdf:resource="http://www.w3.org/2004/02/skos/core#Concept"/>
	<skos:inScheme rdf:resource="http://purl.oclc.org/NET/ssnx/qu/dim#Temperature"/>
	<rdfs:comment>Potential temperature is the temperature a parcel of air or sea water would have if moved adiabatically to sea level pressure.</rdfs:comment>
	<rdfs:label>pseudo equivalent potential temperature</rdfs:label>
	<generalQuantityKind xmlns="http://purl.oclc.org/NET/ssnx/qu/qu#" rdf:resource="http://purl.oclc.org/NET/ssnx/qu/quantity#temperature"/>
	<rdfs:isDefinedBy rdf:resource="http://purl.oclc.org/NET/ssnx/cf/cf-property"/>
</rdf:Description>

<rdf:Description rdf:about="http://purl.oclc.org/NET/ssnx/cf/cf-property#pseudo_equivalent_temperature">
	<rdf:type rdf:resource="http://www.w3.org/2004/02/skos/core#Concept"/>
	<skos:inScheme rdf:resource="http://purl.oclc.org/NET/ssnx/qu/dim#Temperature"/>
	<rdfs:label>pseudo equivalent temperature</rdfs:label>
	<generalQuantityKind xmlns="http://purl.oclc.org/NET/ssnx/qu/qu#" rdf:resource="http://purl.oclc.org/NET/ssnx/qu/quantity#temperature"/>
	<rdfs:isDefinedBy rdf:resource="http://purl.oclc.org/NET/ssnx/cf/cf-property"/>
</rdf:Description>

<rdf:Description rdf:about="http://purl.oclc.org/NET/ssnx/cf/cf-property#sea_ice_temperature">
	<rdf:type rdf:resource="http://www.w3.org/2004/02/skos/core#Concept"/>
	<skos:inScheme rdf:resource="http://purl.oclc.org/NET/ssnx/qu/dim#Temperature"/>
	<rdfs:label>sea ice temperature</rdfs:label>
	<generalQuantityKind xmlns="http://purl.oclc.org/NET/ssnx/qu/qu#" rdf:resource="http://purl.oclc.org/NET/ssnx/qu/quantity#temperature"/>
	<rdfs:isDefinedBy rdf:resource="http://purl.oclc.org/NET/ssnx/cf/cf-property"/>
</rdf:Description>

<rdf:Description rdf:about="http://purl.oclc.org/NET/ssnx/cf/cf-property#sea_surface_foundation_temperature">
	<rdf:type rdf:resource="http://www.w3.org/2004/02/skos/core#Concept"/>
	<skos:inScheme rdf:resource="http://purl.oclc.org/NET/ssnx/qu/dim#Temperature"/>
	<rdfs:comment>The surface called "surface" means the lower boundary of the atmosphere. The sea surface foundation temperature is the water temperature that is not influenced by a thermally stratified layer of diurnal temperature variability (either by daytime warming or nocturnal cooling). The foundation temperature is named to indicate that it is the temperature from which the growth of the diurnal thermocline develops each day, noting that on some occasions with a deep mixed layer there is no clear foundation temperature in the surface layer. In general, sea surface foundation temperature will be similar to a night time minimum or pre-dawn value at depths of between approximately 1 and 5 meters. In the absence of any diurnal signal, the foundation temperature is considered equivalent to the quantity with standard name sea_surface_subskin_temperature. The sea surface foundation temperature defines a level in the upper water column that varies in depth, space, and time depending on the local balance between thermal stratification and turbulent energy and is expected to change slowly over the course of a day. If possible, a data variable with the standard name sea_surface_foundation_temperature should be used with a scalar vertical coordinate variable to specify the depth of the foundation level.
Sea surface foundation temperature is measured at the base of the diurnal thermocline or as close to the water surface as possible in the absence of thermal stratification. Only in situ contact thermometry is able to measure the sea surface foundation temperature. Analysis procedures must be used to estimate sea surface foundation temperature value from radiometric satellite measurements of the quantities with standard names sea_surface_skin_temperature and sea_surface_subskin_temperature.  Sea surface foundation temperature provides a connection with the historical concept of a "bulk" sea surface temperature considered representative of the oceanic mixed layer temperature that is typically represented by any sea temperature measurement within the upper ocean over a depth range of 1 to approximately 20 meters. The general term, "bulk" sea surface temperature, has the standard name sea_surface_temperature with no associated vertical coordinate axis. Sea surface foundation temperature provides a more precise, well-defined quantity than "bulk" sea surface temperature and, consequently, is more representative of the mixed layer temperature.  The temperature of sea water at a particular depth (other than the foundation level) should be reported using the standard name sea_water_temperature and, wherever possible, supplying a vertical coordinate axis or scalar coordinate variable.</rdfs:comment>
	<rdfs:label>sea surface foundation temperature</rdfs:label>
	<generalQuantityKind xmlns="http://purl.oclc.org/NET/ssnx/qu/qu#" rdf:resource="http://purl.oclc.org/NET/ssnx/qu/quantity#temperature"/>
	<rdfs:isDefinedBy rdf:resource="http://purl.oclc.org/NET/ssnx/cf/cf-property"/>
</rdf:Description>

<rdf:Description rdf:about="http://purl.oclc.org/NET/ssnx/cf/cf-property#sea_surface_skin_temperature">
	<rdf:type rdf:resource="http://www.w3.org/2004/02/skos/core#Concept"/>
	<skos:inScheme rdf:resource="http://purl.oclc.org/NET/ssnx/qu/dim#Temperature"/>
	<rdfs:comment>The surface called "surface" means the lower boundary of the atmosphere. The sea surface skin temperature is the temperature measured by an infrared radiometer typically operating at wavelengths in the range 3.7 - 12 micrometers. It represents the temperature within the conductive diffusion-dominated sub-layer at a depth of approximately 10 - 20 micrometers below the air-sea interface. Measurements of this quantity are subject to a large potential diurnal cycle including cool skin layer effects (especially at night under clear skies and low wind speed conditions) and warm layer effects in the daytime.</rdfs:comment>
	<rdfs:label>sea surface skin temperature</rdfs:label>
	<generalQuantityKind xmlns="http://purl.oclc.org/NET/ssnx/qu/qu#" rdf:resource="http://purl.oclc.org/NET/ssnx/qu/quantity#temperature"/>
	<rdfs:isDefinedBy rdf:resource="http://purl.oclc.org/NET/ssnx/cf/cf-property"/>
</rdf:Description>

<rdf:Description rdf:about="http://purl.oclc.org/NET/ssnx/cf/cf-property#sea_surface_subskin_temperature">
	<rdf:type rdf:resource="http://www.w3.org/2004/02/skos/core#Concept"/>
	<skos:inScheme rdf:resource="http://purl.oclc.org/NET/ssnx/qu/dim#Temperature"/>
	<rdfs:comment>The surface called "surface" means the lower boundary of the atmosphere. The sea surface subskin temperature is the temperature at the base of the conductive laminar sub-layer of the ocean surface, that is, at a depth of approximately 1 - 1.5 millimeters below the air-sea interface. For practical purposes, this quantity can be well approximated to the measurement of surface temperature by a microwave radiometer operating in the 6 - 11 gigahertz frequency range, but the relationship is neither direct nor invariant to changing physical conditions or to the specific geometry of the microwave measurements. Measurements of this quantity are subject to a large potential diurnal cycle due to thermal stratification of the upper ocean layer in low wind speed high solar irradiance conditions.</rdfs:comment>
	<rdfs:label>sea surface subskin temperature</rdfs:label>
	<generalQuantityKind xmlns="http://purl.oclc.org/NET/ssnx/qu/qu#" rdf:resource="http://purl.oclc.org/NET/ssnx/qu/quantity#temperature"/>
	<rdfs:isDefinedBy rdf:resource="http://purl.oclc.org/NET/ssnx/cf/cf-property"/>
</rdf:Description>

<rdf:Description rdf:about="http://purl.oclc.org/NET/ssnx/cf/cf-property#sea_surface_temperature">
	<rdf:type rdf:resource="http://www.w3.org/2004/02/skos/core#Concept"/>
	<skos:inScheme rdf:resource="http://purl.oclc.org/NET/ssnx/qu/dim#Temperature"/>
	<rdfs:comment>Sea surface temperature is usually abbreviated as "SST". It is the temperature of sea water near the surface (including the part under sea-ice, if any), and not the skin temperature, whose standard name is surface_temperature. For the temperature of sea water at a particular depth or layer, a data variable of sea_water_temperature with a vertical coordinate axis should be used.</rdfs:comment>
	<rdfs:label>sea surface temperature</rdfs:label>
	<generalQuantityKind xmlns="http://purl.oclc.org/NET/ssnx/qu/qu#" rdf:resource="http://purl.oclc.org/NET/ssnx/qu/quantity#temperature"/>
	<rdfs:isDefinedBy rdf:resource="http://purl.oclc.org/NET/ssnx/cf/cf-property"/>
</rdf:Description>

<rdf:Description rdf:about="http://purl.oclc.org/NET/ssnx/cf/cf-property#sea_water_potential_temperature">
	<rdf:type rdf:resource="http://www.w3.org/2004/02/skos/core#Concept"/>
	<skos:inScheme rdf:resource="http://purl.oclc.org/NET/ssnx/qu/dim#Temperature"/>
	<rdfs:comment>Potential temperature is the temperature a parcel of air or sea water would have if moved adiabatically to sea level pressure.</rdfs:comment>
	<rdfs:label>sea water potential temperature</rdfs:label>
	<generalQuantityKind xmlns="http://purl.oclc.org/NET/ssnx/qu/qu#" rdf:resource="http://purl.oclc.org/NET/ssnx/qu/quantity#temperature"/>
	<rdfs:isDefinedBy rdf:resource="http://purl.oclc.org/NET/ssnx/cf/cf-property"/>
</rdf:Description>

<rdf:Description rdf:about="http://purl.oclc.org/NET/ssnx/cf/cf-property#sea_water_temperature">
	<rdf:type rdf:resource="http://www.w3.org/2004/02/skos/core#Concept"/>
	<skos:inScheme rdf:resource="http://purl.oclc.org/NET/ssnx/qu/dim#Temperature"/>
	<rdfs:label>sea water temperature</rdfs:label>
	<generalQuantityKind xmlns="http://purl.oclc.org/NET/ssnx/qu/qu#" rdf:resource="http://purl.oclc.org/NET/ssnx/qu/quantity#temperature"/>
	<rdfs:isDefinedBy rdf:resource="http://purl.oclc.org/NET/ssnx/cf/cf-property"/>
</rdf:Description>

<rdf:Description rdf:about="http://purl.oclc.org/NET/ssnx/cf/cf-property#snow_temperature">
	<rdf:type rdf:resource="http://www.w3.org/2004/02/skos/core#Concept"/>
	<skos:inScheme rdf:resource="http://purl.oclc.org/NET/ssnx/qu/dim#Temperature"/>
	<rdfs:comment>Snow temperature is the bulk temperature of the snow, not the surface (skin) temperature.</rdfs:comment>
	<rdfs:label>snow temperature</rdfs:label>
	<generalQuantityKind xmlns="http://purl.oclc.org/NET/ssnx/qu/qu#" rdf:resource="http://purl.oclc.org/NET/ssnx/qu/quantity#temperature"/>
	<rdfs:isDefinedBy rdf:resource="http://purl.oclc.org/NET/ssnx/cf/cf-property"/>
</rdf:Description>

<rdf:Description rdf:about="http://purl.oclc.org/NET/ssnx/cf/cf-property#soil_temperature">
	<rdf:type rdf:resource="http://www.w3.org/2004/02/skos/core#Concept"/>
	<skos:inScheme rdf:resource="http://purl.oclc.org/NET/ssnx/qu/dim#Temperature"/>
	<rdfs:comment>Soil temperature is the bulk temperature of the soil, not the surface (skin) temperature.</rdfs:comment>
	<rdfs:label>soil temperature</rdfs:label>
	<generalQuantityKind xmlns="http://purl.oclc.org/NET/ssnx/qu/qu#" rdf:resource="http://purl.oclc.org/NET/ssnx/qu/quantity#temperature"/>
	<rdfs:isDefinedBy rdf:resource="http://purl.oclc.org/NET/ssnx/cf/cf-property"/>
</rdf:Description>

<rdf:Description rdf:about="http://purl.oclc.org/NET/ssnx/cf/cf-property#surface_brightness_temperature">
	<rdf:type rdf:resource="http://www.w3.org/2004/02/skos/core#Concept"/>
	<skos:inScheme rdf:resource="http://purl.oclc.org/NET/ssnx/qu/dim#Temperature"/>
	<rdfs:comment>The surface called "surface" means the lower boundary of the atmosphere.The brightness temperature of a body is the temperature of a black body which radiates the same power per unit solid angle per unit area.</rdfs:comment>
	<rdfs:label>surface brightness temperature</rdfs:label>
	<generalQuantityKind xmlns="http://purl.oclc.org/NET/ssnx/qu/qu#" rdf:resource="http://purl.oclc.org/NET/ssnx/qu/quantity#temperature"/>
	<rdfs:isDefinedBy rdf:resource="http://purl.oclc.org/NET/ssnx/cf/cf-property"/>
</rdf:Description>

<rdf:Description rdf:about="http://purl.oclc.org/NET/ssnx/cf/cf-property#surface_temperature">
	<rdf:type rdf:resource="http://www.w3.org/2004/02/skos/core#Concept"/>
	<skos:inScheme rdf:resource="http://purl.oclc.org/NET/ssnx/qu/dim#Temperature"/>
	<rdfs:comment>The surface called "surface" means the lower boundary of the atmosphere. The surface temperature is the temperature at the interface, not the bulk temperature of the medium above or below. Unless indicated in the cell_methods attribute, a quantity is assumed to apply to the whole area of each horizontal grid box. Previously, the qualifier where_type was used to specify that the quantity applies only to the part of the grid box of the named type.  Names containing the where_type qualifier are deprecated and newly created data should use the cell_methods attribute to indicate the horizontal area to which the quantity applies.</rdfs:comment>
	<rdfs:label>surface temperature</rdfs:label>
	<generalQuantityKind xmlns="http://purl.oclc.org/NET/ssnx/qu/qu#" rdf:resource="http://purl.oclc.org/NET/ssnx/qu/quantity#temperature"/>
	<rdfs:isDefinedBy rdf:resource="http://purl.oclc.org/NET/ssnx/cf/cf-property"/>
</rdf:Description>

<rdf:Description rdf:about="http://purl.oclc.org/NET/ssnx/cf/cf-property#surface_temperature_anomaly">
	<rdf:type rdf:resource="http://www.w3.org/2004/02/skos/core#Concept"/>
	<skos:inScheme rdf:resource="http://purl.oclc.org/NET/ssnx/qu/dim#Temperature"/>
	<rdfs:comment>The surface called "surface" means the lower boundary of the atmosphere. "anomaly" means difference from climatology. The surface temperature is the (skin) temperature at the interface, not the bulk temperature of the medium above or below.</rdfs:comment>
	<rdfs:label>surface temperature anomaly</rdfs:label>
	<generalQuantityKind xmlns="http://purl.oclc.org/NET/ssnx/qu/qu#" rdf:resource="http://purl.oclc.org/NET/ssnx/qu/quantity#temperature"/>
	<rdfs:isDefinedBy rdf:resource="http://purl.oclc.org/NET/ssnx/cf/cf-property"/>
</rdf:Description>

<rdf:Description rdf:about="http://purl.oclc.org/NET/ssnx/cf/cf-property#temperature_of_sensor_for_oxygen_in_sea_water">
	<rdf:type rdf:resource="http://www.w3.org/2004/02/skos/core#Concept"/>
	<skos:inScheme rdf:resource="http://purl.oclc.org/NET/ssnx/qu/dim#Temperature"/>
	<rdfs:comment>Temperature_of_sensor_for_oxygen_in_sea_water is the instrument temperature used in calculating the concentration of oxygen in sea water; it is not a measurement of the ambient water temperature.</rdfs:comment>
	<rdfs:label>temperature of sensor for oxygen in sea water</rdfs:label>
	<generalQuantityKind xmlns="http://purl.oclc.org/NET/ssnx/qu/qu#" rdf:resource="http://purl.oclc.org/NET/ssnx/qu/quantity#temperature"/>
	<rdfs:isDefinedBy rdf:resource="http://purl.oclc.org/NET/ssnx/cf/cf-property"/>
</rdf:Description>

<rdf:Description rdf:about="http://purl.oclc.org/NET/ssnx/cf/cf-property#toa_brightness_temperature">
	<rdf:type rdf:resource="http://www.w3.org/2004/02/skos/core#Concept"/>
	<skos:inScheme rdf:resource="http://purl.oclc.org/NET/ssnx/qu/dim#Temperature"/>
	<rdfs:comment> The brightness temperature of a body is the temperature of a black body which radiates the same power per unit solid angle per unit area.  "toa" means top of atmosphere. </rdfs:comment>
	<rdfs:label>toa brightness temperature</rdfs:label>
	<generalQuantityKind xmlns="http://purl.oclc.org/NET/ssnx/qu/qu#" rdf:resource="http://purl.oclc.org/NET/ssnx/qu/quantity#temperature"/>
	<rdfs:isDefinedBy rdf:resource="http://purl.oclc.org/NET/ssnx/cf/cf-property"/>
</rdf:Description>

<rdf:Description rdf:about="http://purl.oclc.org/NET/ssnx/cf/cf-property#toa_brightness_temperature_assuming_clear_sky">
	<rdf:type rdf:resource="http://www.w3.org/2004/02/skos/core#Concept"/>
	<skos:inScheme rdf:resource="http://purl.oclc.org/NET/ssnx/qu/dim#Temperature"/>
	<rdfs:comment> The brightness temperature of a body is the temperature of a black body which radiates the same power per unit solid angle per unit area.  A phrase assuming_condition  indicates that the named quantity is the value which would obtain if all  aspects of the system were unaltered except for the assumption of the  circumstances specified by the condition.  "toa" means top of atmosphere. </rdfs:comment>
	<rdfs:label>toa brightness temperature assuming clear sky</rdfs:label>
	<generalQuantityKind xmlns="http://purl.oclc.org/NET/ssnx/qu/qu#" rdf:resource="http://purl.oclc.org/NET/ssnx/qu/quantity#temperature"/>
	<rdfs:isDefinedBy rdf:resource="http://purl.oclc.org/NET/ssnx/cf/cf-property"/>
</rdf:Description>

<rdf:Description rdf:about="http://purl.oclc.org/NET/ssnx/cf/cf-property#tropopause_air_temperature">
	<rdf:type rdf:resource="http://www.w3.org/2004/02/skos/core#Concept"/>
	<skos:inScheme rdf:resource="http://purl.oclc.org/NET/ssnx/qu/dim#Temperature"/>
	<rdfs:comment>Air temperature is the bulk temperature of the air, not the surface (skin) temperature.</rdfs:comment>
	<rdfs:label>tropopause air temperature</rdfs:label>
	<generalQuantityKind xmlns="http://purl.oclc.org/NET/ssnx/qu/qu#" rdf:resource="http://purl.oclc.org/NET/ssnx/qu/quantity#temperature"/>
	<rdfs:isDefinedBy rdf:resource="http://purl.oclc.org/NET/ssnx/cf/cf-property"/>
</rdf:Description>

<rdf:Description rdf:about="http://purl.oclc.org/NET/ssnx/cf/cf-property#virtual_temperature">
	<rdf:type rdf:resource="http://www.w3.org/2004/02/skos/core#Concept"/>
	<skos:inScheme rdf:resource="http://purl.oclc.org/NET/ssnx/qu/dim#Temperature"/>
	<rdfs:comment>The virtual temperature of air is the temperature at which the dry air constituent of a parcel of moist air would have the same density as the moist air at the same pressure.</rdfs:comment>
	<rdfs:label>virtual temperature</rdfs:label>
	<generalQuantityKind xmlns="http://purl.oclc.org/NET/ssnx/qu/qu#" rdf:resource="http://purl.oclc.org/NET/ssnx/qu/quantity#temperature"/>
	<rdfs:isDefinedBy rdf:resource="http://purl.oclc.org/NET/ssnx/cf/cf-property"/>
</rdf:Description>

<rdf:Description rdf:about="http://purl.oclc.org/NET/ssnx/cf/cf-property#wet_bulb_temperature">
	<rdf:type rdf:resource="http://www.w3.org/2004/02/skos/core#Concept"/>
	<skos:inScheme rdf:resource="http://purl.oclc.org/NET/ssnx/qu/dim#Temperature"/>
	<rdfs:label>wet bulb temperature</rdfs:label>
	<generalQuantityKind xmlns="http://purl.oclc.org/NET/ssnx/qu/qu#" rdf:resource="http://purl.oclc.org/NET/ssnx/qu/quantity#temperature"/>
	<rdfs:isDefinedBy rdf:resource="http://purl.oclc.org/NET/ssnx/cf/cf-property"/>
</rdf:Description>

<rdf:Description rdf:about="http://purl.oclc.org/NET/ssnx/qu/quantity#temperature">
	<skos:inScheme rdf:resource="http://purl.oclc.org/NET/ssnx/qu/dim#Temperature"/>
</rdf:Description>

</rdf:RDF>