<?xml version="1.0" encoding="UTF-8"?>
<rdf:RDF
	xmlns:vann="http://purl.org/vocab/vann/"
	xmlns:voaf="http://purl.org/vocommons/voaf#"
	xmlns:rdfs="http://www.w3.org/2000/01/rdf-schema#"
	xmlns:owl="http://www.w3.org/2002/07/owl#"
	xmlns:skos="http://www.w3.org/2004/02/skos/core#"
	xmlns:rdf="http://www.w3.org/1999/02/22-rdf-syntax-ns#"
	xmlns:dcterms="http://purl.org/dc/terms/"
	xmlns:dc="http://purl.org/dc/elements/1.1/"
	xmlns:dcmit="http://purl.org/dc/dcmitype/"
	xmlns:sesame="http://www.openrdf.org/schema/sesame#"
	xmlns:xsd="http://www.w3.org/2001/XMLSchema#"
	xmlns:fn="http://www.w3.org/2005/xpath-functions#"
	xmlns:foaf="http://xmlns.com/foaf/0.1/"
	xmlns:hint="http://www.bigdata.com/queryHints#"
	xmlns:bd="http://www.bigdata.com/rdf#"
	xmlns:bds="http://www.bigdata.com/rdf/search#">

<rdf:Description rdf:about="http://rdf.geospecies.org/ont/geospecies">
	<rdf:type rdf:resource="http://www.w3.org/2002/07/owl#Ontology"/>
</rdf:Description>

<rdf:Description rdf:about="http://rdf.geospecies.org/ont/geospecies#Nativeness">
	<rdf:type rdf:resource="http://www.w3.org/2004/02/skos/core#ConceptScheme"/>
</rdf:Description>

<rdf:Description rdf:about="http://rdf.geospecies.org/ont/geospecies#nativeness_introduced">
	<rdf:type rdf:resource="http://www.w3.org/2004/02/skos/core#Concept"/>
	<skos:inScheme rdf:resource="http://rdf.geospecies.org/ont/geospecies#Nativeness"/>
</rdf:Description>

<rdf:Description rdf:about="http://rdf.geospecies.org/ont/geospecies#Nativeness">
	<rdfs:label>Nativeness</rdfs:label>
</rdf:Description>

<rdf:Description rdf:about="http://rdf.geospecies.org/ont/geospecies#nativeness_introduced">
	<rdfs:comment>The organism arrived in the region via an anthropogenic mechanism or mechanisms</rdfs:comment>
	<rdfs:label>Introduced</rdfs:label>
</rdf:Description>

<rdf:Description rdf:about="http://rdf.geospecies.org/ont/geospecies#Nativeness">
	<rdfs:isDefinedBy rdf:resource="http://rdf.geospecies.org/ont/geospecies"/>
</rdf:Description>

<rdf:Description rdf:about="http://rdf.geospecies.org/ont/geospecies#nativeness_introduced">
	<rdfs:isDefinedBy rdf:resource="http://rdf.geospecies.org/ont/geospecies"/>
</rdf:Description>

<rdf:Description rdf:about="http://rdf.geospecies.org/ont/geospecies#nativeness_invasive">
	<rdf:type rdf:resource="http://www.w3.org/2004/02/skos/core#Concept"/>
	<skos:inScheme rdf:resource="http://rdf.geospecies.org/ont/geospecies#Nativeness"/>
	<rdfs:comment>The organism is having a deleterious impact on another organism, multiple organisms or the ecosystem as a whole</rdfs:comment>
	<rdfs:label>Invasive</rdfs:label>
	<rdfs:isDefinedBy rdf:resource="http://rdf.geospecies.org/ont/geospecies"/>
</rdf:Description>

<rdf:Description rdf:about="http://rdf.geospecies.org/ont/geospecies#nativeness_managed">
	<rdf:type rdf:resource="http://www.w3.org/2004/02/skos/core#Concept"/>
	<skos:inScheme rdf:resource="http://rdf.geospecies.org/ont/geospecies#Nativeness"/>
	<rdfs:comment>The organism maintains its presence through intentional cultivation or husbandry</rdfs:comment>
	<rdfs:label>Managed</rdfs:label>
	<rdfs:isDefinedBy rdf:resource="http://rdf.geospecies.org/ont/geospecies"/>
</rdf:Description>

<rdf:Description rdf:about="http://rdf.geospecies.org/ont/geospecies#nativeness_native">
	<rdf:type rdf:resource="http://www.w3.org/2004/02/skos/core#Concept"/>
	<skos:inScheme rdf:resource="http://rdf.geospecies.org/ont/geospecies#Nativeness"/>
	<rdfs:comment>The organism either evolved in this region or arrived by non-anthropogenic means</rdfs:comment>
	<rdfs:label>Native</rdfs:label>
	<rdfs:isDefinedBy rdf:resource="http://rdf.geospecies.org/ont/geospecies"/>
</rdf:Description>

<rdf:Description rdf:about="http://rdf.geospecies.org/ont/geospecies#nativeness_naturalised">
	<rdf:type rdf:resource="http://www.w3.org/2004/02/skos/core#Concept"/>
	<skos:inScheme rdf:resource="http://rdf.geospecies.org/ont/geospecies#Nativeness"/>
	<rdfs:comment>The organism reproduces naturally and forms part of the local ecology</rdfs:comment>
	<rdfs:label>Naturalised</rdfs:label>
	<rdfs:isDefinedBy rdf:resource="http://rdf.geospecies.org/ont/geospecies"/>
</rdf:Description>

</rdf:RDF>