<?xml version="1.0" encoding="UTF-8"?>
<rdf:RDF
	xmlns:vann="http://purl.org/vocab/vann/"
	xmlns:voaf="http://purl.org/vocommons/voaf#"
	xmlns:rdfs="http://www.w3.org/2000/01/rdf-schema#"
	xmlns:owl="http://www.w3.org/2002/07/owl#"
	xmlns:skos="http://www.w3.org/2004/02/skos/core#"
	xmlns:rdf="http://www.w3.org/1999/02/22-rdf-syntax-ns#"
	xmlns:dcterms="http://purl.org/dc/terms/"
	xmlns:dc="http://purl.org/dc/elements/1.1/"
	xmlns:dcmit="http://purl.org/dc/dcmitype/"
	xmlns:sesame="http://www.openrdf.org/schema/sesame#"
	xmlns:xsd="http://www.w3.org/2001/XMLSchema#"
	xmlns:fn="http://www.w3.org/2005/xpath-functions#"
	xmlns:foaf="http://xmlns.com/foaf/0.1/"
	xmlns:hint="http://www.bigdata.com/queryHints#"
	xmlns:bd="http://www.bigdata.com/rdf#"
	xmlns:bds="http://www.bigdata.com/rdf/search#">

<rdf:Description rdf:about="https://w3id.org/cdc">
	<rdf:type rdf:resource="http://www.w3.org/2002/07/owl#Ontology"/>
</rdf:Description>

<rdf:Description rdf:about="https://w3id.org/cdc#DataManagementTag">
	<rdf:type rdf:resource="http://www.w3.org/2004/02/skos/core#ConceptScheme"/>
</rdf:Description>

<rdf:Description rdf:about="https://w3id.org/cdc#incoming">
	<rdf:type rdf:resource="http://www.w3.org/2004/02/skos/core#Concept"/>
	<skos:inScheme rdf:resource="https://w3id.org/cdc#DataManagementTag"/>
</rdf:Description>

<rdf:Description rdf:about="https://w3id.org/cdc#DataManagementTag">
	<rdfs:comment xml:lang="en">A tag that is linked to a DCAT catalog, dataset, distribution or data service instance node using the cdc:hasDataManagementTag property. CDC predefines three instances of this class, i.e. cdc:incoming, cdc:internal and cdc:outgoing. Each catalog, dataset, distribution or data service can only have one tag that is not supposed to change over the lifetime of the described resource unless it considers a dataset (that is not a catalog). When necessary, qualified relations between DCAT entities can also get a tag.</rdfs:comment>
	<rdfs:label xml:lang="en">data management tag</rdfs:label>
</rdf:Description>

<rdf:Description rdf:about="https://w3id.org/cdc#incoming">
	<rdfs:comment xml:lang="en">A predefined tag to mark an incoming catalog, dataset, distribution or data service. It can also be used to annotate qualified relations between DCAT entities.</rdfs:comment>
	<rdfs:label xml:lang="en">incoming</rdfs:label>
</rdf:Description>

<rdf:Description rdf:about="https://w3id.org/cdc#hasDataManagementTag">
	<rdfs:range rdf:resource="https://w3id.org/cdc#DataManagementTag"/>
	<rdfs:label xml:lang="en">has data management tag</rdfs:label>
	<rdfs:comment xml:lang="en">Connects a DCAT catalog, dataset, distribution, data service or qualified relation (cdc:DistributionRelation or dcat:Relation) to exactly one of the following predefined data management tags: cdc:internal, cdc:incoming or cdc:outgoing.</rdfs:comment>
	<rdf:type rdf:resource="http://www.w3.org/2002/07/owl#ObjectProperty"/>
</rdf:Description>

<rdf:Description rdf:about="https://w3id.org/cdc#DataManagementTag">
	<rdfs:isDefinedBy rdf:resource="https://w3id.org/cdc"/>
</rdf:Description>

<rdf:Description rdf:about="https://w3id.org/cdc#incoming">
	<rdfs:isDefinedBy rdf:resource="https://w3id.org/cdc"/>
</rdf:Description>

<rdf:Description rdf:about="https://w3id.org/cdc#internal">
	<rdf:type rdf:resource="http://www.w3.org/2004/02/skos/core#Concept"/>
	<skos:inScheme rdf:resource="https://w3id.org/cdc#DataManagementTag"/>
	<rdfs:comment xml:lang="en">A predefined tag to mark an internal (= not exchanged) catalog, dataset, distribution or data service. It can also be used to annotate qualified relations between DCAT entities.{</rdfs:comment>
	<rdfs:label xml:lang="en">internal</rdfs:label>
	<rdfs:isDefinedBy rdf:resource="https://w3id.org/cdc"/>
</rdf:Description>

<rdf:Description rdf:about="https://w3id.org/cdc#outgoing">
	<rdf:type rdf:resource="http://www.w3.org/2004/02/skos/core#Concept"/>
	<skos:inScheme rdf:resource="https://w3id.org/cdc#DataManagementTag"/>
	<rdfs:comment xml:lang="en">A predefined tag to mark an outgoing catalog, dataset, distribution or data service. It can also be used to annotate qualified relations between DCAT entities.{</rdfs:comment>
	<rdfs:label xml:lang="en">outgoing</rdfs:label>
	<rdfs:isDefinedBy rdf:resource="https://w3id.org/cdc"/>
</rdf:Description>

</rdf:RDF>