<?xml version="1.0" encoding="UTF-8"?>
<rdf:RDF
	xmlns:vann="http://purl.org/vocab/vann/"
	xmlns:voaf="http://purl.org/vocommons/voaf#"
	xmlns:rdfs="http://www.w3.org/2000/01/rdf-schema#"
	xmlns:owl="http://www.w3.org/2002/07/owl#"
	xmlns:skos="http://www.w3.org/2004/02/skos/core#"
	xmlns:rdf="http://www.w3.org/1999/02/22-rdf-syntax-ns#"
	xmlns:dcterms="http://purl.org/dc/terms/"
	xmlns:dc="http://purl.org/dc/elements/1.1/"
	xmlns:dcmit="http://purl.org/dc/dcmitype/"
	xmlns:sesame="http://www.openrdf.org/schema/sesame#"
	xmlns:xsd="http://www.w3.org/2001/XMLSchema#"
	xmlns:fn="http://www.w3.org/2005/xpath-functions#"
	xmlns:foaf="http://xmlns.com/foaf/0.1/"
	xmlns:hint="http://www.bigdata.com/queryHints#"
	xmlns:bd="http://www.bigdata.com/rdf#"
	xmlns:bds="http://www.bigdata.com/rdf/search#">

<rdf:Description rdf:about="http://w3id.org/vcb/fel#">
	<rdf:type rdf:resource="http://www.w3.org/2002/07/owl#Ontology"/>
</rdf:Description>

<rdf:Description rdf:about="http://w3id.org/vcb/fel#BaseFormClass">
	<rdf:type rdf:resource="http://www.w3.org/2004/02/skos/core#ConceptScheme"/>
</rdf:Description>

<rdf:Description rdf:about="http://w3id.org/vcb/fel#AliasProperForm">
	<rdf:type rdf:resource="http://www.w3.org/2004/02/skos/core#Concept"/>
	<skos:inScheme rdf:resource="http://w3id.org/vcb/fel#BaseFormClass"/>
</rdf:Description>

<rdf:Description rdf:about="http://w3id.org/vcb/fel#BaseFormClass">
	<rdfs:comment xml:lang="en">This meta-class gathers classes that divide annotations by the base-form of their mention, recognizing not only proper nouns as entities, but also other more flexible definitions, such as those that allow pronouns, numbers, temporal expressions, etc. Current instances of this meta-class include: ProperForm, NumericTemporalForm, CommonForm, and ProForm.</rdfs:comment>
	<rdfs:label xml:lang="en">Base Form Class</rdfs:label>
</rdf:Description>

<rdf:Description rdf:about="http://w3id.org/vcb/fel#AliasProperForm">
	<rdfs:comment xml:lang="en">This class is concerned with all the proper-noun mentions with a different morpheme than the primary label of the knowledge base entity to which if refers (though it may be a known alias). For instance, the mention 'King of Pop' targeting wiki:Michael_Jackson is considered an AliasProperForm.</rdfs:comment>
	<rdfs:label xml:lang="en">Alias Proper Form</rdfs:label>
	<rdfs:subClassOf rdf:resource="http://w3id.org/vcb/fel#ProperForm"/>
</rdf:Description>

<rdf:Description rdf:about="http://w3id.org/vcb/fel#ProperForm">
	<rdf:type rdf:resource="http://www.w3.org/2004/02/skos/core#Concept"/>
</rdf:Description>

<rdf:Description rdf:about="http://w3id.org/vcb/fel#BaseFormClass">
	<rdfs:isDefinedBy rdf:resource="http://w3id.org/vcb/fel#"/>
</rdf:Description>

<rdf:Description rdf:about="http://w3id.org/vcb/fel#AliasProperForm">
	<rdfs:isDefinedBy rdf:resource="http://w3id.org/vcb/fel#"/>
</rdf:Description>

<rdf:Description rdf:about="http://w3id.org/vcb/fel#ProperForm">
	<rdfs:isDefinedBy rdf:resource="http://w3id.org/vcb/fel#"/>
</rdf:Description>

<rdf:Description rdf:about="http://w3id.org/vcb/fel#ExtendedProperForm">
	<rdf:type rdf:resource="http://www.w3.org/2004/02/skos/core#Concept"/>
	<skos:inScheme rdf:resource="http://w3id.org/vcb/fel#BaseFormClass"/>
	<rdfs:comment xml:lang="en">This class gathers all proper-name mentions longer than the label of the knowledgebase entity but containing the label. For example, the mention 'Michael Joseph Jackson' targeting wiki:Michael_Jackson is considered an ExtendedProperForm.</rdfs:comment>
	<rdfs:label xml:lang="en">Extended Proper Form</rdfs:label>
	<rdfs:subClassOf rdf:resource="http://w3id.org/vcb/fel#ProperForm"/>
	<rdfs:isDefinedBy rdf:resource="http://w3id.org/vcb/fel#"/>
</rdf:Description>

<rdf:Description rdf:about="http://w3id.org/vcb/fel#FullProperForm">
	<rdf:type rdf:resource="http://www.w3.org/2004/02/skos/core#Concept"/>
	<skos:inScheme rdf:resource="http://w3id.org/vcb/fel#BaseFormClass"/>
	<rdfs:comment xml:lang="en">This class gathers all proper-form mentions that (almost) exactly match with the label of the knowledgebase entity. For example, the mention 'Michael Jackson' targeting wiki:Michael_Jackson is considered Full. This class also includes mentions that are syntactically close to the knowlegebase entity (specifically, the lemmas should be the same and in the same order), for instance 'German' pointing to wiki:Germany is also considered a FullProperForm.</rdfs:comment>
	<rdfs:label xml:lang="en">Full Proper Form</rdfs:label>
	<rdfs:subClassOf rdf:resource="http://w3id.org/vcb/fel#ProperForm"/>
	<rdfs:isDefinedBy rdf:resource="http://w3id.org/vcb/fel#"/>
</rdf:Description>

<rdf:Description rdf:about="http://w3id.org/vcb/fel#ShortProperForm">
	<rdf:type rdf:resource="http://www.w3.org/2004/02/skos/core#Concept"/>
	<skos:inScheme rdf:resource="http://w3id.org/vcb/fel#BaseFormClass"/>
	<rdfs:comment xml:lang="en">This class is concerned with all the proper-name mentions that are shorter than the label of the knowledgebase entity while still being based on the label. For instance, the mentions 'Jackson' or 'M. Jackson' targeting wiki:Michael_Jackson are considered ShortProperForm.</rdfs:comment>
	<rdfs:label xml:lang="en">Short Proper Form</rdfs:label>
	<rdfs:subClassOf rdf:resource="http://w3id.org/vcb/fel#ProperForm"/>
	<rdfs:isDefinedBy rdf:resource="http://w3id.org/vcb/fel#"/>
</rdf:Description>

<rdf:Description rdf:about="http://w3id.org/vcb/fel#CommonForm">
	<rdf:type rdf:resource="http://www.w3.org/2004/02/skos/core#Concept"/>
	<skos:inScheme rdf:resource="http://w3id.org/vcb/fel#BaseFormClass"/>
	<rdfs:comment xml:lang="en">This class gathers all the mentions with a corresponding entity in the knowledgebase, but that does not correspond to a Proper Form, Pro-Form or Numeric/Temporal Form. For instance, the mention 'bfelt' referring to wiki:Bfelt_(clothing) is considered CommonForm.</rdfs:comment>
	<rdfs:label xml:lang="en">Common Form</rdfs:label>
	<rdfs:isDefinedBy rdf:resource="http://w3id.org/vcb/fel#"/>
</rdf:Description>

<rdf:Description rdf:about="http://w3id.org/vcb/fel#NumericTemporalForm">
	<rdf:type rdf:resource="http://www.w3.org/2004/02/skos/core#Concept"/>
	<skos:inScheme rdf:resource="http://w3id.org/vcb/fel#BaseFormClass"/>
	<rdfs:comment xml:lang="en">This class gathers all mentions based on numeric and temporal expressions, such as: '1', 'one', '12/23/2019', etc. (as were included in MUC-6).</rdfs:comment>
	<rdfs:label xml:lang="en">Numeric and Temporal Form</rdfs:label>
	<rdfs:isDefinedBy rdf:resource="http://w3id.org/vcb/fel#"/>
</rdf:Description>

<rdf:Description rdf:about="http://w3id.org/vcb/fel#ProForm">
	<rdf:type rdf:resource="http://www.w3.org/2004/02/skos/core#Concept"/>
	<skos:inScheme rdf:resource="http://w3id.org/vcb/fel#BaseFormClass"/>
	<rdfs:comment xml:lang="en">This class gathers all mentions based on pronouns, pro-adjective, etc. For example, the mentions 'he', 'theirs', etc., are considered ProForm (assuming they link to a knowledgebase entity).</rdfs:comment>
	<rdfs:label xml:lang="en">Pro-Form</rdfs:label>
	<rdfs:isDefinedBy rdf:resource="http://w3id.org/vcb/fel#"/>
</rdf:Description>

<rdf:Description rdf:about="http://w3id.org/vcb/fel#ProperForm">
	<skos:inScheme rdf:resource="http://w3id.org/vcb/fel#BaseFormClass"/>
	<rdfs:comment xml:lang="en">This class gathers all mentions based on names (proper nouns), e.g., 'Michael Jackson', 'USA', 'King of the Pop', 'B. Obama', etc. Such mentions do not have to be nouns if they are based on proper nouns, as in the case of 'French, 'Orwellian', etc. Such mentions may use abbreviated or extended forms of names; we add a new level in the class hierarchy to separate them: Full, Extended, Short or Alias.</rdfs:comment>
	<rdfs:label xml:lang="en">Proper Form</rdfs:label>
</rdf:Description>

</rdf:RDF>