<?xml version="1.0" encoding="UTF-8"?>
<rdf:RDF
	xmlns:vann="http://purl.org/vocab/vann/"
	xmlns:voaf="http://purl.org/vocommons/voaf#"
	xmlns:rdfs="http://www.w3.org/2000/01/rdf-schema#"
	xmlns:owl="http://www.w3.org/2002/07/owl#"
	xmlns:skos="http://www.w3.org/2004/02/skos/core#"
	xmlns:rdf="http://www.w3.org/1999/02/22-rdf-syntax-ns#"
	xmlns:dcterms="http://purl.org/dc/terms/"
	xmlns:dc="http://purl.org/dc/elements/1.1/"
	xmlns:dcmit="http://purl.org/dc/dcmitype/"
	xmlns:sesame="http://www.openrdf.org/schema/sesame#"
	xmlns:xsd="http://www.w3.org/2001/XMLSchema#"
	xmlns:fn="http://www.w3.org/2005/xpath-functions#"
	xmlns:foaf="http://xmlns.com/foaf/0.1/"
	xmlns:hint="http://www.bigdata.com/queryHints#"
	xmlns:bd="http://www.bigdata.com/rdf#"
	xmlns:bds="http://www.bigdata.com/rdf/search#">

<rdf:Description rdf:about="http://www.ebusiness-unibw.org/ontologies/consumerelectronics/v1">
	<rdf:type rdf:resource="http://www.w3.org/2002/07/owl#Ontology"/>
</rdf:Description>

<rdf:Description rdf:about="http://www.ebusiness-unibw.org/ontologies/consumerelectronics/v1#AudioInterfaceType">
	<rdf:type rdf:resource="http://www.w3.org/2004/02/skos/core#ConceptScheme"/>
</rdf:Description>

<rdf:Description rdf:about="http://www.ebusiness-unibw.org/ontologies/consumerelectronics/v1#Audio2.5mm">
	<rdf:type rdf:resource="http://www.w3.org/2004/02/skos/core#Concept"/>
	<skos:inScheme rdf:resource="http://www.ebusiness-unibw.org/ontologies/consumerelectronics/v1#AudioInterfaceType"/>
</rdf:Description>

<rdf:Description rdf:about="http://www.ebusiness-unibw.org/ontologies/consumerelectronics/v1#AudioInterfaceType">
	<rdfs:comment xml:lang="en">Interface generally refers to an abstraction that an entity provides of itself to the outside (refers to audio output).

(This description is partly based on or reuses content from the Wikipedia article "Interface (computer science)" (http://en.wikipedia.org/wiki/Interface_(computer_science)) and is licensed under the GNU Free Documentation License (http://www.gnu.org/copyleft/fdl.html).)</rdfs:comment>
	<rdfs:label xml:lang="en">Audio Interface Type</rdfs:label>
</rdf:Description>

<rdf:Description rdf:about="http://www.ebusiness-unibw.org/ontologies/consumerelectronics/v1#Audio2.5mm">
	<rdfs:comment xml:lang="en">Audio interface type of a specific diameter.</rdfs:comment>
	<rdfs:label xml:lang="en">Audio 2.5mm</rdfs:label>
</rdf:Description>

<rdf:Description rdf:about="http://www.ebusiness-unibw.org/ontologies/consumerelectronics/v1#hasAudioInterfaceType">
	<rdfs:range rdf:resource="http://www.ebusiness-unibw.org/ontologies/consumerelectronics/v1#AudioInterfaceType"/>
	<rdfs:label xml:lang="en">audio interface type</rdfs:label>
	<rdfs:comment xml:lang="en">Defines the type of interfaces used to transfer audio signals.</rdfs:comment>
	<rdf:type rdf:resource="http://www.w3.org/2002/07/owl#ObjectProperty"/>
</rdf:Description>

<rdf:Description rdf:about="http://www.ebusiness-unibw.org/ontologies/consumerelectronics/v1#AudioInterfaceType">
	<rdfs:isDefinedBy rdf:resource="http://www.ebusiness-unibw.org/ontologies/consumerelectronics/v1"/>
</rdf:Description>

<rdf:Description rdf:about="http://www.ebusiness-unibw.org/ontologies/consumerelectronics/v1#Audio2.5mm">
	<rdfs:isDefinedBy rdf:resource="http://www.ebusiness-unibw.org/ontologies/consumerelectronics/v1"/>
</rdf:Description>

<rdf:Description rdf:about="http://www.ebusiness-unibw.org/ontologies/consumerelectronics/v1#Audio3.5mm">
	<rdf:type rdf:resource="http://www.w3.org/2004/02/skos/core#Concept"/>
	<skos:inScheme rdf:resource="http://www.ebusiness-unibw.org/ontologies/consumerelectronics/v1#AudioInterfaceType"/>
	<rdfs:comment xml:lang="en">Audio interface type of a specific diameter.</rdfs:comment>
	<rdfs:label xml:lang="en">Audio 3.5mm</rdfs:label>
	<rdfs:isDefinedBy rdf:resource="http://www.ebusiness-unibw.org/ontologies/consumerelectronics/v1"/>
</rdf:Description>

<rdf:Description rdf:about="http://www.ebusiness-unibw.org/ontologies/consumerelectronics/v1#BluetoothAudio">
	<rdf:type rdf:resource="http://www.w3.org/2004/02/skos/core#Concept"/>
	<skos:inScheme rdf:resource="http://www.ebusiness-unibw.org/ontologies/consumerelectronics/v1#AudioInterfaceType"/>
	<rdfs:comment xml:lang="en">Bluetooth is a wireless protocol utilizing short-range communications technology facilitating data transmission over short distances from fixed and mobile devices, creating wireless personal area networks (refers to audio).</rdfs:comment>
	<rdfs:label xml:lang="en">Bluetooth audio</rdfs:label>
	<rdfs:isDefinedBy rdf:resource="http://www.ebusiness-unibw.org/ontologies/consumerelectronics/v1"/>
</rdf:Description>

</rdf:RDF>