<?xml version="1.0" encoding="UTF-8"?>
<rdf:RDF
	xmlns:vann="http://purl.org/vocab/vann/"
	xmlns:voaf="http://purl.org/vocommons/voaf#"
	xmlns:rdfs="http://www.w3.org/2000/01/rdf-schema#"
	xmlns:owl="http://www.w3.org/2002/07/owl#"
	xmlns:skos="http://www.w3.org/2004/02/skos/core#"
	xmlns:rdf="http://www.w3.org/1999/02/22-rdf-syntax-ns#"
	xmlns:dcterms="http://purl.org/dc/terms/"
	xmlns:dc="http://purl.org/dc/elements/1.1/"
	xmlns:dcmit="http://purl.org/dc/dcmitype/"
	xmlns:sesame="http://www.openrdf.org/schema/sesame#"
	xmlns:xsd="http://www.w3.org/2001/XMLSchema#"
	xmlns:fn="http://www.w3.org/2005/xpath-functions#"
	xmlns:foaf="http://xmlns.com/foaf/0.1/"
	xmlns:hint="http://www.bigdata.com/queryHints#"
	xmlns:bd="http://www.bigdata.com/rdf#"
	xmlns:bds="http://www.bigdata.com/rdf/search#">

<rdf:Description rdf:about="http://purl.oclc.org/NET/ssnx/cf/cf-property">
	<rdf:type rdf:resource="http://www.w3.org/2002/07/owl#Ontology"/>
</rdf:Description>

<rdf:Description rdf:about="http://purl.oclc.org/NET/ssnx/qu/dim#Distance">
	<rdf:type rdf:resource="http://www.w3.org/2004/02/skos/core#ConceptScheme"/>
</rdf:Description>

<rdf:Description rdf:about="http://purl.oclc.org/NET/ssnx/cf/cf-property#convective_cloud_base_altitude">
	<rdf:type rdf:resource="http://www.w3.org/2004/02/skos/core#Concept"/>
	<skos:inScheme rdf:resource="http://purl.oclc.org/NET/ssnx/qu/dim#Distance"/>
	<rdfs:comment>cloud_base refers to the base of the lowest cloud. Altitude is the (geometric) height above the geoid, which is the reference geopotential surface. The geoid is similar to mean sea level. Convective cloud is that produced by the convection schemes in an atmosphere model.</rdfs:comment>
	<rdfs:label>convective cloud base altitude</rdfs:label>
	<generalQuantityKind xmlns="http://purl.oclc.org/NET/ssnx/qu/qu#" rdf:resource="http://purl.oclc.org/NET/ssnx/qu/quantity#distance"/>
</rdf:Description>

<rdf:Description rdf:about="http://purl.oclc.org/NET/ssnx/qu/quantity#distance">
	<rdf:type rdf:resource="http://www.w3.org/2004/02/skos/core#Concept"/>
</rdf:Description>

<rdf:Description rdf:about="http://purl.oclc.org/NET/ssnx/qu/dim#Distance">
	<rdfs:isDefinedBy rdf:resource="http://purl.oclc.org/NET/ssnx/cf/cf-property"/>
</rdf:Description>

<rdf:Description rdf:about="http://purl.oclc.org/NET/ssnx/cf/cf-property#convective_cloud_base_altitude">
	<rdfs:isDefinedBy rdf:resource="http://purl.oclc.org/NET/ssnx/cf/cf-property"/>
</rdf:Description>

<rdf:Description rdf:about="http://purl.oclc.org/NET/ssnx/qu/quantity#distance">
	<rdfs:isDefinedBy rdf:resource="http://purl.oclc.org/NET/ssnx/cf/cf-property"/>
</rdf:Description>

<rdf:Description rdf:about="http://purl.oclc.org/NET/ssnx/cf/cf-property#convective_cloud_top_altitude">
	<rdf:type rdf:resource="http://www.w3.org/2004/02/skos/core#Concept"/>
	<skos:inScheme rdf:resource="http://purl.oclc.org/NET/ssnx/qu/dim#Distance"/>
	<rdfs:comment>cloud_top refers to the top of the highest cloud. Altitude is the (geometric) height above the geoid, which is the reference geopotential surface. The geoid is similar to mean sea level. Convective cloud is that produced by the convection schemes in an atmosphere model.</rdfs:comment>
	<rdfs:label>convective cloud top altitude</rdfs:label>
	<generalQuantityKind xmlns="http://purl.oclc.org/NET/ssnx/qu/qu#" rdf:resource="http://purl.oclc.org/NET/ssnx/qu/quantity#distance"/>
	<rdfs:isDefinedBy rdf:resource="http://purl.oclc.org/NET/ssnx/cf/cf-property"/>
</rdf:Description>

<rdf:Description rdf:about="http://purl.oclc.org/NET/ssnx/cf/cf-property#depth">
	<rdf:type rdf:resource="http://www.w3.org/2004/02/skos/core#Concept"/>
	<skos:inScheme rdf:resource="http://purl.oclc.org/NET/ssnx/qu/dim#Distance"/>
	<rdfs:comment>Depth is the vertical distance below the surface.</rdfs:comment>
	<rdfs:label>depth</rdfs:label>
	<generalQuantityKind xmlns="http://purl.oclc.org/NET/ssnx/qu/qu#" rdf:resource="http://purl.oclc.org/NET/ssnx/qu/quantity#distance"/>
	<rdfs:isDefinedBy rdf:resource="http://purl.oclc.org/NET/ssnx/cf/cf-property"/>
</rdf:Description>

<rdf:Description rdf:about="http://purl.oclc.org/NET/ssnx/cf/cf-property#depth_at_maximum_upward_derivative_of_sea_water_potential_temperature">
	<rdf:type rdf:resource="http://www.w3.org/2004/02/skos/core#Concept"/>
	<skos:inScheme rdf:resource="http://purl.oclc.org/NET/ssnx/qu/dim#Distance"/>
	<rdfs:comment>This quantity, often used to indicate the "thermocline depth", is the depth of the maximum vertical gradient of sea water potential temperature.  Depth is the vertical distance below the surface. Potential temperature is the temperature a parcel of air or sea water would have if moved adiabatically to sea level pressure.</rdfs:comment>
	<rdfs:label>depth at maximum upward derivative of sea water potential temperature</rdfs:label>
	<generalQuantityKind xmlns="http://purl.oclc.org/NET/ssnx/qu/qu#" rdf:resource="http://purl.oclc.org/NET/ssnx/qu/quantity#distance"/>
	<rdfs:isDefinedBy rdf:resource="http://purl.oclc.org/NET/ssnx/cf/cf-property"/>
</rdf:Description>

<rdf:Description rdf:about="http://purl.oclc.org/NET/ssnx/cf/cf-property#depth_at_shallowest_local_minimum_in_vertical_profile_of_mole_concentration_of_dissolved_molecular_oxygen_in_sea_water">
	<rdf:type rdf:resource="http://www.w3.org/2004/02/skos/core#Concept"/>
	<skos:inScheme rdf:resource="http://purl.oclc.org/NET/ssnx/qu/dim#Distance"/>
	<rdfs:comment> Depth is the vertical distance below the surface.   'Mole concentration' means number of moles per unit volume, also called "molarity", and is used in the construction mole_concentration_of_X_in_Y, where X is a material constituent of Y.  A chemical or biological species denoted by X may be described by a single term such as 'nitrogen' or a phrase such as 'nox_expressed_as_nitrogen'. The concentration of any chemical species, whether particulate or dissolved, may vary with depth in the ocean.  A depth profile may go through one or more local minima in concentration. The  depth_at_shallowest_local_minimum_in_vertical_profile_of_mole_concentration_of_dissolved_molecular_oxygen_in_sea_water is the depth of the local minimum in the oxygen concentration that occurs closest to the sea surface.</rdfs:comment>
	<rdfs:label>depth at shallowest local minimum in vertical profile of mole concentration of dissolved molecular oxygen in sea water</rdfs:label>
	<generalQuantityKind xmlns="http://purl.oclc.org/NET/ssnx/qu/qu#" rdf:resource="http://purl.oclc.org/NET/ssnx/qu/quantity#distance"/>
	<rdfs:isDefinedBy rdf:resource="http://purl.oclc.org/NET/ssnx/cf/cf-property"/>
</rdf:Description>

<rdf:Description rdf:about="http://purl.oclc.org/NET/ssnx/cf/cf-property#depth_of_isosurface_of_sea_water_potential_temperature">
	<rdf:type rdf:resource="http://www.w3.org/2004/02/skos/core#Concept"/>
	<skos:inScheme rdf:resource="http://purl.oclc.org/NET/ssnx/qu/dim#Distance"/>
	<rdfs:comment>This quantity, sometimes called the "isotherm depth", is the depth (if it exists) at which the sea water potential temperature equals some specified value. This value should be specified in a scalar coordinate variable. Depth is the vertical distance below the surface. Potential temperature is the temperature a parcel of air or sea water would have if moved adiabatically to sea level pressure.</rdfs:comment>
	<rdfs:label>depth of isosurface of sea water potential temperature</rdfs:label>
	<generalQuantityKind xmlns="http://purl.oclc.org/NET/ssnx/qu/qu#" rdf:resource="http://purl.oclc.org/NET/ssnx/qu/quantity#distance"/>
	<rdfs:isDefinedBy rdf:resource="http://purl.oclc.org/NET/ssnx/cf/cf-property"/>
</rdf:Description>

<rdf:Description rdf:about="http://purl.oclc.org/NET/ssnx/cf/cf-property#eastward_sea_ice_displacement">
	<rdf:type rdf:resource="http://www.w3.org/2004/02/skos/core#Concept"/>
	<skos:inScheme rdf:resource="http://purl.oclc.org/NET/ssnx/qu/dim#Distance"/>
	<rdfs:comment>"Eastward" indicates a vector component which is positive when directed eastward (negative westward).  "Displacement" means the change in geospatial position of an object that has moved over time. If possible, the time interval over which the motion took place should be specified using a bounds variable for the time coordinate variable.  A displacement can be represented as a vector. Such a vector should however not be interpreted as describing a rectilinear, constant speed motion but merely as an indication that the start point of the vector is found at the tip of the vector after the time interval associated with the displacement variable.  A displacement does not prescribe a trajectory. Sea ice displacement can be defined as a two-dimensional vector, with no vertical component. An eastward displacement is the distance calculated from the change in a moving object's longitude between the start and end of the time interval associated with the displacement variable.</rdfs:comment>
	<rdfs:label>eastward sea ice displacement</rdfs:label>
	<generalQuantityKind xmlns="http://purl.oclc.org/NET/ssnx/qu/qu#" rdf:resource="http://purl.oclc.org/NET/ssnx/qu/quantity#distance"/>
	<rdfs:isDefinedBy rdf:resource="http://purl.oclc.org/NET/ssnx/cf/cf-property"/>
</rdf:Description>

<rdf:Description rdf:about="http://purl.oclc.org/NET/ssnx/cf/cf-property#equilibrium_line_altitude">
	<rdf:type rdf:resource="http://www.w3.org/2004/02/skos/core#Concept"/>
	<skos:inScheme rdf:resource="http://purl.oclc.org/NET/ssnx/qu/dim#Distance"/>
	<rdfs:comment>Altitude is the (geometric) height above the geoid, which is the reference geopotential surface. The geoid is similar to mean sea level. The equilibrium line is the locus of points on a land ice surface at which ice accumulation balances ice ablation over the year.</rdfs:comment>
	<rdfs:label>equilibrium line altitude</rdfs:label>
	<generalQuantityKind xmlns="http://purl.oclc.org/NET/ssnx/qu/qu#" rdf:resource="http://purl.oclc.org/NET/ssnx/qu/quantity#distance"/>
	<rdfs:isDefinedBy rdf:resource="http://purl.oclc.org/NET/ssnx/cf/cf-property"/>
</rdf:Description>

<rdf:Description rdf:about="http://purl.oclc.org/NET/ssnx/cf/cf-property#freezing_level_altitude">
	<rdf:type rdf:resource="http://www.w3.org/2004/02/skos/core#Concept"/>
	<skos:inScheme rdf:resource="http://purl.oclc.org/NET/ssnx/qu/dim#Distance"/>
	<rdfs:comment>Altitude is the (geometric) height above the geoid, which is the reference geopotential surface. The geoid is similar to mean sea level.</rdfs:comment>
	<rdfs:label>freezing level altitude</rdfs:label>
	<generalQuantityKind xmlns="http://purl.oclc.org/NET/ssnx/qu/qu#" rdf:resource="http://purl.oclc.org/NET/ssnx/qu/quantity#distance"/>
	<rdfs:isDefinedBy rdf:resource="http://purl.oclc.org/NET/ssnx/cf/cf-property"/>
</rdf:Description>

<rdf:Description rdf:about="http://purl.oclc.org/NET/ssnx/cf/cf-property#global_average_sea_level_change">
	<rdf:type rdf:resource="http://www.w3.org/2004/02/skos/core#Concept"/>
	<skos:inScheme rdf:resource="http://purl.oclc.org/NET/ssnx/qu/dim#Distance"/>
	<rdfs:comment>Global average sea level change is due to change in volume of the water in the ocean, caused by mass and/or density change, or to change in the volume of the ocean basins, caused by tectonics etc. It is sometimes called "eustatic", which is a term that also has other definitions. It differs from the change in the global average sea surface height relative to the centre of the Earth by the global average vertical movement of the ocean floor. Zero sea level change is an arbitrary level.</rdfs:comment>
	<rdfs:label>global average sea level change</rdfs:label>
	<generalQuantityKind xmlns="http://purl.oclc.org/NET/ssnx/qu/qu#" rdf:resource="http://purl.oclc.org/NET/ssnx/qu/quantity#distance"/>
	<rdfs:isDefinedBy rdf:resource="http://purl.oclc.org/NET/ssnx/cf/cf-property"/>
</rdf:Description>

<rdf:Description rdf:about="http://purl.oclc.org/NET/ssnx/cf/cf-property#global_average_steric_sea_level_change">
	<rdf:type rdf:resource="http://www.w3.org/2004/02/skos/core#Concept"/>
	<skos:inScheme rdf:resource="http://purl.oclc.org/NET/ssnx/qu/dim#Distance"/>
	<rdfs:comment> Global average steric sea level change is caused by changes in sea water density due to changes in temperature (thermosteric) and salinity (halosteric). Zero sea level change is an arbitrary level. </rdfs:comment>
	<rdfs:label>global average steric sea level change</rdfs:label>
	<generalQuantityKind xmlns="http://purl.oclc.org/NET/ssnx/qu/qu#" rdf:resource="http://purl.oclc.org/NET/ssnx/qu/quantity#distance"/>
	<rdfs:isDefinedBy rdf:resource="http://purl.oclc.org/NET/ssnx/cf/cf-property"/>
</rdf:Description>

<rdf:Description rdf:about="http://purl.oclc.org/NET/ssnx/cf/cf-property#global_average_thermosteric_sea_level_change">
	<rdf:type rdf:resource="http://www.w3.org/2004/02/skos/core#Concept"/>
	<skos:inScheme rdf:resource="http://purl.oclc.org/NET/ssnx/qu/dim#Distance"/>
	<rdfs:comment>Global average thermosteric sea level change is the part caused by change in density due to change in temperature i.e. thermal expansion. Zero sea level change is an arbitrary level.</rdfs:comment>
	<rdfs:label>global average thermosteric sea level change</rdfs:label>
	<generalQuantityKind xmlns="http://purl.oclc.org/NET/ssnx/qu/qu#" rdf:resource="http://purl.oclc.org/NET/ssnx/qu/quantity#distance"/>
	<rdfs:isDefinedBy rdf:resource="http://purl.oclc.org/NET/ssnx/cf/cf-property"/>
</rdf:Description>

<rdf:Description rdf:about="http://purl.oclc.org/NET/ssnx/cf/cf-property#magnitude_of_derivative_of_position_wrt_model_level_number">
	<rdf:type rdf:resource="http://www.w3.org/2004/02/skos/core#Concept"/>
	<skos:inScheme rdf:resource="http://purl.oclc.org/NET/ssnx/qu/dim#Distance"/>
	<rdfs:comment>The quantity with standard name magnitude_of_derivative_of_position_wrt_model_level_number (known in differential geometry as a "scale factor") is | (dr/dk)ij|, where r(i,j,k) is the vector 3D position of the point with coordinate indices (i,j,k). It is a measure of the gridblock spacing in the z-direction.</rdfs:comment>
	<rdfs:label>magnitude of derivative of position wrt model level number</rdfs:label>
	<generalQuantityKind xmlns="http://purl.oclc.org/NET/ssnx/qu/qu#" rdf:resource="http://purl.oclc.org/NET/ssnx/qu/quantity#distance"/>
	<rdfs:isDefinedBy rdf:resource="http://purl.oclc.org/NET/ssnx/cf/cf-property"/>
</rdf:Description>

<rdf:Description rdf:about="http://purl.oclc.org/NET/ssnx/cf/cf-property#magnitude_of_derivative_of_position_wrt_x_coordinate_index">
	<rdf:type rdf:resource="http://www.w3.org/2004/02/skos/core#Concept"/>
	<skos:inScheme rdf:resource="http://purl.oclc.org/NET/ssnx/qu/dim#Distance"/>
	<rdfs:comment>The quantity with standard name magnitude_of_derivative_of_position_wrt_x_coordinate_index (known in differential geometry as a "scale factor") is | (dr/di)jk|, where r(i,j,k) is the vector 3D position of the point with coordinate indices (i,j,k). It is a measure of the gridblock spacing in the x-direction.</rdfs:comment>
	<rdfs:label>magnitude of derivative of position wrt x coordinate index</rdfs:label>
	<generalQuantityKind xmlns="http://purl.oclc.org/NET/ssnx/qu/qu#" rdf:resource="http://purl.oclc.org/NET/ssnx/qu/quantity#distance"/>
	<rdfs:isDefinedBy rdf:resource="http://purl.oclc.org/NET/ssnx/cf/cf-property"/>
</rdf:Description>

<rdf:Description rdf:about="http://purl.oclc.org/NET/ssnx/cf/cf-property#magnitude_of_derivative_of_position_wrt_y_coordinate_index">
	<rdf:type rdf:resource="http://www.w3.org/2004/02/skos/core#Concept"/>
	<skos:inScheme rdf:resource="http://purl.oclc.org/NET/ssnx/qu/dim#Distance"/>
	<rdfs:comment>The quantity with standard name magnitude_of_derivative_of_position_wrt_y_coordinate_index (known in differential geometry as a "scale factor") is | (dr/dj)ik|, where r(i,j,k) is the vector 3D position of the point with coordinate indices (i,j,k). It is a measure of the gridblock spacing in the y-direction.</rdfs:comment>
	<rdfs:label>magnitude of derivative of position wrt y coordinate index</rdfs:label>
	<generalQuantityKind xmlns="http://purl.oclc.org/NET/ssnx/qu/qu#" rdf:resource="http://purl.oclc.org/NET/ssnx/qu/quantity#distance"/>
	<rdfs:isDefinedBy rdf:resource="http://purl.oclc.org/NET/ssnx/cf/cf-property"/>
</rdf:Description>

<rdf:Description rdf:about="http://purl.oclc.org/NET/ssnx/cf/cf-property#minimum_depth_of_aragonite_undersaturation_in_sea_water">
	<rdf:type rdf:resource="http://www.w3.org/2004/02/skos/core#Concept"/>
	<skos:inScheme rdf:resource="http://purl.oclc.org/NET/ssnx/qu/dim#Distance"/>
	<rdfs:comment> Depth is the vertical distance below the surface.   'Undersaturation' means that a solution is unsaturated with respect to a solute. Aragonite is a mineral that is a polymorph of calcium carbonate. The chemical formula of aragonite is CaCO3. Standard names also exist for calcite, another polymorph of calcium carbonate. The "minimum depth of undersaturation", sometimes called the "saturation horizon", is the shallowest depth at which a body of water is an undersaturated solution of a named solute.</rdfs:comment>
	<rdfs:label>minimum depth of aragonite undersaturation in sea water</rdfs:label>
	<generalQuantityKind xmlns="http://purl.oclc.org/NET/ssnx/qu/qu#" rdf:resource="http://purl.oclc.org/NET/ssnx/qu/quantity#distance"/>
	<rdfs:isDefinedBy rdf:resource="http://purl.oclc.org/NET/ssnx/cf/cf-property"/>
</rdf:Description>

<rdf:Description rdf:about="http://purl.oclc.org/NET/ssnx/cf/cf-property#minimum_depth_of_calcite_undersaturation_in_sea_water">
	<rdf:type rdf:resource="http://www.w3.org/2004/02/skos/core#Concept"/>
	<skos:inScheme rdf:resource="http://purl.oclc.org/NET/ssnx/qu/dim#Distance"/>
	<rdfs:comment> Depth is the vertical distance below the surface.   'Undersaturation' means that a solution is unsaturated with respect to a solute. Calcite is a mineral that is a  polymorph of calcium carbonate. The chemical formula of calcite is CaCO3. Standard names also exist for aragonite, another polymorph of calcium carbonate. The "minimum depth of undersaturation", sometimes called the "saturation horizon", is the shallowest depth at which a body of water is an undersaturated solution of a named solute.</rdfs:comment>
	<rdfs:label>minimum depth of calcite undersaturation in sea water</rdfs:label>
	<generalQuantityKind xmlns="http://purl.oclc.org/NET/ssnx/qu/qu#" rdf:resource="http://purl.oclc.org/NET/ssnx/qu/quantity#distance"/>
	<rdfs:isDefinedBy rdf:resource="http://purl.oclc.org/NET/ssnx/cf/cf-property"/>
</rdf:Description>

<rdf:Description rdf:about="http://purl.oclc.org/NET/ssnx/cf/cf-property#northward_sea_ice_displacement">
	<rdf:type rdf:resource="http://www.w3.org/2004/02/skos/core#Concept"/>
	<skos:inScheme rdf:resource="http://purl.oclc.org/NET/ssnx/qu/dim#Distance"/>
	<rdfs:comment>"Northward" indicates a vector component which is positive when directed northward (negative southward).  "Displacement" means the change in geospatial position of an object that has moved over time. If possible, the time interval over which the motion took place should be specified using a bounds variable for the time coordinate variable.  A displacement can be represented as a vector. Such a vector should however not be interpreted as describing a rectilinear, constant speed motion but merely as an indication that the start point of the vector is found at the tip of the vector after the time interval associated with the displacement variable.  A displacement does not prescribe a trajectory. Sea ice displacement can be defined as a two-dimensional vector, with no vertical component. A northward displacement is the distance calculated from the change in a moving object's latitude between the start and end of the time interval associated with the displacement variable.</rdfs:comment>
	<rdfs:label>northward sea ice displacement</rdfs:label>
	<generalQuantityKind xmlns="http://purl.oclc.org/NET/ssnx/qu/qu#" rdf:resource="http://purl.oclc.org/NET/ssnx/qu/quantity#distance"/>
	<rdfs:isDefinedBy rdf:resource="http://purl.oclc.org/NET/ssnx/cf/cf-property"/>
</rdf:Description>

<rdf:Description rdf:about="http://purl.oclc.org/NET/ssnx/cf/cf-property#projection_x_coordinate">
	<rdf:type rdf:resource="http://www.w3.org/2004/02/skos/core#Concept"/>
	<skos:inScheme rdf:resource="http://purl.oclc.org/NET/ssnx/qu/dim#Distance"/>
	<rdfs:comment>"x" indicates a vector component along the grid x-axis, when this is not true longitude, positive with increasing x. Projection coordinates are distances in the x- and y-directions on a plane onto which the surface of the Earth has been projected according to a map projection. The relationship between the projection coordinates and latitude and longitude is described by the grid_mapping.</rdfs:comment>
	<rdfs:label>projection x coordinate</rdfs:label>
	<generalQuantityKind xmlns="http://purl.oclc.org/NET/ssnx/qu/qu#" rdf:resource="http://purl.oclc.org/NET/ssnx/qu/quantity#distance"/>
	<rdfs:isDefinedBy rdf:resource="http://purl.oclc.org/NET/ssnx/cf/cf-property"/>
</rdf:Description>

<rdf:Description rdf:about="http://purl.oclc.org/NET/ssnx/cf/cf-property#projection_y_coordinate">
	<rdf:type rdf:resource="http://www.w3.org/2004/02/skos/core#Concept"/>
	<skos:inScheme rdf:resource="http://purl.oclc.org/NET/ssnx/qu/dim#Distance"/>
	<rdfs:comment>"y" indicates a vector component along the grid y-axis, when this is not true latitude, positive with increasing y. Projection coordinates are distances in the x- and y-directions on a plane onto which the surface of the Earth has been projected according to a map projection. The relationship between the projection coordinates and latitude and longitude is described by the grid_mapping.</rdfs:comment>
	<rdfs:label>projection y coordinate</rdfs:label>
	<generalQuantityKind xmlns="http://purl.oclc.org/NET/ssnx/qu/qu#" rdf:resource="http://purl.oclc.org/NET/ssnx/qu/quantity#distance"/>
	<rdfs:isDefinedBy rdf:resource="http://purl.oclc.org/NET/ssnx/cf/cf-property"/>
</rdf:Description>

<rdf:Description rdf:about="http://purl.oclc.org/NET/ssnx/cf/cf-property#root_depth">
	<rdf:type rdf:resource="http://www.w3.org/2004/02/skos/core#Concept"/>
	<skos:inScheme rdf:resource="http://purl.oclc.org/NET/ssnx/qu/dim#Distance"/>
	<rdfs:comment>Depth is the vertical distance below the surface. The root depth is maximum depth of soil reached by plant roots, from which they can extract moisture.</rdfs:comment>
	<rdfs:label>root depth</rdfs:label>
	<generalQuantityKind xmlns="http://purl.oclc.org/NET/ssnx/qu/qu#" rdf:resource="http://purl.oclc.org/NET/ssnx/qu/quantity#distance"/>
	<rdfs:isDefinedBy rdf:resource="http://purl.oclc.org/NET/ssnx/cf/cf-property"/>
</rdf:Description>

<rdf:Description rdf:about="http://purl.oclc.org/NET/ssnx/cf/cf-property#sea_floor_depth_below_geoid">
	<rdf:type rdf:resource="http://www.w3.org/2004/02/skos/core#Concept"/>
	<skos:inScheme rdf:resource="http://purl.oclc.org/NET/ssnx/qu/dim#Distance"/>
	<rdfs:comment>The geoid is a surface of constant geopotential with which mean sea level would coincide if the ocean were at rest. (The volume enclosed between the geoid and the sea floor equals the mean volume of water in the ocean.) In an ocean GCM the geoid is the surface of zero depth, or the rigid lid if the model uses that approximation.</rdfs:comment>
	<rdfs:label>sea floor depth below geoid</rdfs:label>
	<generalQuantityKind xmlns="http://purl.oclc.org/NET/ssnx/qu/qu#" rdf:resource="http://purl.oclc.org/NET/ssnx/qu/quantity#distance"/>
	<rdfs:isDefinedBy rdf:resource="http://purl.oclc.org/NET/ssnx/cf/cf-property"/>
</rdf:Description>

<rdf:Description rdf:about="http://purl.oclc.org/NET/ssnx/cf/cf-property#sea_floor_depth_below_sea_level">
	<rdf:type rdf:resource="http://www.w3.org/2004/02/skos/core#Concept"/>
	<skos:inScheme rdf:resource="http://purl.oclc.org/NET/ssnx/qu/dim#Distance"/>
	<rdfs:comment>sea_level means mean sea level, which is close to the geoid in sea areas.</rdfs:comment>
	<rdfs:label>sea floor depth below sea level</rdfs:label>
	<generalQuantityKind xmlns="http://purl.oclc.org/NET/ssnx/qu/qu#" rdf:resource="http://purl.oclc.org/NET/ssnx/qu/quantity#distance"/>
	<rdfs:isDefinedBy rdf:resource="http://purl.oclc.org/NET/ssnx/cf/cf-property"/>
</rdf:Description>

<rdf:Description rdf:about="http://purl.oclc.org/NET/ssnx/cf/cf-property#sea_floor_depth_below_sea_surface">
	<rdf:type rdf:resource="http://www.w3.org/2004/02/skos/core#Concept"/>
	<skos:inScheme rdf:resource="http://purl.oclc.org/NET/ssnx/qu/dim#Distance"/>
	<rdfs:comment>The sea_floor_depth_below_sea_surface is the vertical distance between the sea surface and the seabed as measured at a given point in space including the variance caused by tides and possibly waves.</rdfs:comment>
	<rdfs:label>sea floor depth below sea surface</rdfs:label>
	<generalQuantityKind xmlns="http://purl.oclc.org/NET/ssnx/qu/qu#" rdf:resource="http://purl.oclc.org/NET/ssnx/qu/quantity#distance"/>
	<rdfs:isDefinedBy rdf:resource="http://purl.oclc.org/NET/ssnx/cf/cf-property"/>
</rdf:Description>

<rdf:Description rdf:about="http://purl.oclc.org/NET/ssnx/cf/cf-property#sea_ice_displacement">
	<rdf:type rdf:resource="http://www.w3.org/2004/02/skos/core#Concept"/>
	<skos:inScheme rdf:resource="http://purl.oclc.org/NET/ssnx/qu/dim#Distance"/>
	<rdfs:comment>"Displacement" means the change in geospatial position of an object that has moved over time. If possible, the time interval over which the motion took place should be specified using a bounds variable for the time coordinate variable.  A displacement can be represented as a vector. Such a vector should however not be interpreted as describing a rectilinear, constant speed motion but merely as an indication that the start point of the vector is found at the tip of the vector after the time interval associated with the displacement variable.  A displacement does not prescribe a trajectory. Sea ice displacement can be defined as a two-dimensional vector, with no vertical component. In that case, "displacement" is also the distance across the earth's surface calculated from the change in a moving object's geospatial position between the start and end of the time interval associated with the displacement variable.</rdfs:comment>
	<rdfs:label>sea ice displacement</rdfs:label>
	<generalQuantityKind xmlns="http://purl.oclc.org/NET/ssnx/qu/qu#" rdf:resource="http://purl.oclc.org/NET/ssnx/qu/quantity#distance"/>
	<rdfs:isDefinedBy rdf:resource="http://purl.oclc.org/NET/ssnx/cf/cf-property"/>
</rdf:Description>

<rdf:Description rdf:about="http://purl.oclc.org/NET/ssnx/cf/cf-property#sea_ice_draft">
	<rdf:type rdf:resource="http://www.w3.org/2004/02/skos/core#Concept"/>
	<skos:inScheme rdf:resource="http://purl.oclc.org/NET/ssnx/qu/dim#Distance"/>
	<rdfs:comment>Sea ice draft is the depth of the sea-ice lower surface below the water surface.</rdfs:comment>
	<rdfs:label>sea ice draft</rdfs:label>
	<generalQuantityKind xmlns="http://purl.oclc.org/NET/ssnx/qu/qu#" rdf:resource="http://purl.oclc.org/NET/ssnx/qu/quantity#distance"/>
	<rdfs:isDefinedBy rdf:resource="http://purl.oclc.org/NET/ssnx/cf/cf-property"/>
</rdf:Description>

<rdf:Description rdf:about="http://purl.oclc.org/NET/ssnx/cf/cf-property#sea_ice_freeboard">
	<rdf:type rdf:resource="http://www.w3.org/2004/02/skos/core#Concept"/>
	<skos:inScheme rdf:resource="http://purl.oclc.org/NET/ssnx/qu/dim#Distance"/>
	<rdfs:comment>Sea ice freeboard is the height of the sea-ice upper surface above the water surface.</rdfs:comment>
	<rdfs:label>sea ice freeboard</rdfs:label>
	<generalQuantityKind xmlns="http://purl.oclc.org/NET/ssnx/qu/qu#" rdf:resource="http://purl.oclc.org/NET/ssnx/qu/quantity#distance"/>
	<rdfs:isDefinedBy rdf:resource="http://purl.oclc.org/NET/ssnx/cf/cf-property"/>
</rdf:Description>

<rdf:Description rdf:about="http://purl.oclc.org/NET/ssnx/cf/cf-property#sea_ice_x_displacement">
	<rdf:type rdf:resource="http://www.w3.org/2004/02/skos/core#Concept"/>
	<skos:inScheme rdf:resource="http://purl.oclc.org/NET/ssnx/qu/dim#Distance"/>
	<rdfs:comment>"x" indicates a vector component along the grid x-axis, when this is not true longitude, positive with increasing x.  "Displacement" means the change in geospatial position of an object that has moved over time. If possible, the time interval over which the motion took place should be specified using a bounds variable for the time coordinate variable.  A displacement can be represented as a vector. Such a vector should however not be interpreted as describing a rectilinear, constant speed motion but merely as an indication that the start point of the vector is found at the tip of the vector after the time interval associated with the displacement variable.  A displacement does not prescribe a trajectory. Sea ice displacement can be defined as a two-dimensional vector, with no vertical component. An x displacement is calculated from the difference in the moving object's grid x coordinate between the start and end of the time interval associated with the displacement variable.</rdfs:comment>
	<rdfs:label>sea ice x displacement</rdfs:label>
	<generalQuantityKind xmlns="http://purl.oclc.org/NET/ssnx/qu/qu#" rdf:resource="http://purl.oclc.org/NET/ssnx/qu/quantity#distance"/>
	<rdfs:isDefinedBy rdf:resource="http://purl.oclc.org/NET/ssnx/cf/cf-property"/>
</rdf:Description>

<rdf:Description rdf:about="http://purl.oclc.org/NET/ssnx/cf/cf-property#sea_ice_y_displacement">
	<rdf:type rdf:resource="http://www.w3.org/2004/02/skos/core#Concept"/>
	<skos:inScheme rdf:resource="http://purl.oclc.org/NET/ssnx/qu/dim#Distance"/>
	<rdfs:comment>"y" indicates a vector component along the grid y-axis, when this is not true latitude, positive with increasing y.  "Displacement" means the change in geospatial position of an object that has moved over time. If possible, the time interval over which the motion took place should be specified using a bounds variable for the time coordinate variable.  A displacement can be represented as a vector. Such a vector should however not be interpreted as describing a rectilinear, constant speed motion but merely as an indication that the start point of the vector is found at the tip of the vector after the time interval associated with the displacement variable.  A displacement does not prescribe a trajectory. Sea ice displacement can be defined as a two-dimensional vector, with no vertical component. A y displacement is calculated from the difference in the moving object's grid y coordinate between the start and end of the time interval associated with the displacement variable.</rdfs:comment>
	<rdfs:label>sea ice y displacement</rdfs:label>
	<generalQuantityKind xmlns="http://purl.oclc.org/NET/ssnx/qu/qu#" rdf:resource="http://purl.oclc.org/NET/ssnx/qu/quantity#distance"/>
	<rdfs:isDefinedBy rdf:resource="http://purl.oclc.org/NET/ssnx/cf/cf-property"/>
</rdf:Description>

<rdf:Description rdf:about="http://purl.oclc.org/NET/ssnx/cf/cf-property#secchi_depth_of_sea_water">
	<rdf:type rdf:resource="http://www.w3.org/2004/02/skos/core#Concept"/>
	<skos:inScheme rdf:resource="http://purl.oclc.org/NET/ssnx/qu/dim#Distance"/>
	<rdfs:comment> Depth is the vertical distance below the surface.  A Secchi disk is a patterned disk that is used to measure water transparency in oceans and lakes. The disk is lowered into the water and the depth at which the pattern is no longer visible is the called the secchi depth.</rdfs:comment>
	<rdfs:label>secchi depth of sea water</rdfs:label>
	<generalQuantityKind xmlns="http://purl.oclc.org/NET/ssnx/qu/qu#" rdf:resource="http://purl.oclc.org/NET/ssnx/qu/quantity#distance"/>
	<rdfs:isDefinedBy rdf:resource="http://purl.oclc.org/NET/ssnx/cf/cf-property"/>
</rdf:Description>

<rdf:Description rdf:about="http://purl.oclc.org/NET/ssnx/cf/cf-property#surface_altitude">
	<rdf:type rdf:resource="http://www.w3.org/2004/02/skos/core#Concept"/>
	<skos:inScheme rdf:resource="http://purl.oclc.org/NET/ssnx/qu/dim#Distance"/>
	<rdfs:comment>The surface called "surface" means the lower boundary of the atmosphere. Altitude is the (geometric) height above the geoid, which is the reference geopotential surface. The geoid is similar to mean sea level.</rdfs:comment>
	<rdfs:label>surface altitude</rdfs:label>
	<generalQuantityKind xmlns="http://purl.oclc.org/NET/ssnx/qu/qu#" rdf:resource="http://purl.oclc.org/NET/ssnx/qu/quantity#distance"/>
	<rdfs:isDefinedBy rdf:resource="http://purl.oclc.org/NET/ssnx/cf/cf-property"/>
</rdf:Description>

<rdf:Description rdf:about="http://purl.oclc.org/NET/ssnx/cf/cf-property#tropopause_altitude">
	<rdf:type rdf:resource="http://www.w3.org/2004/02/skos/core#Concept"/>
	<skos:inScheme rdf:resource="http://purl.oclc.org/NET/ssnx/qu/dim#Distance"/>
	<rdfs:comment>Altitude is the (geometric) height above the geoid, which is the reference geopotential surface. The geoid is similar to mean sea level.</rdfs:comment>
	<rdfs:label>tropopause altitude</rdfs:label>
	<generalQuantityKind xmlns="http://purl.oclc.org/NET/ssnx/qu/qu#" rdf:resource="http://purl.oclc.org/NET/ssnx/qu/quantity#distance"/>
	<rdfs:isDefinedBy rdf:resource="http://purl.oclc.org/NET/ssnx/cf/cf-property"/>
</rdf:Description>

<rdf:Description rdf:about="http://purl.oclc.org/NET/ssnx/cf/cf-property#visibility_in_air">
	<rdf:type rdf:resource="http://www.w3.org/2004/02/skos/core#Concept"/>
	<skos:inScheme rdf:resource="http://purl.oclc.org/NET/ssnx/qu/dim#Distance"/>
	<rdfs:comment>The visibility is the distance at which something can be seen.</rdfs:comment>
	<rdfs:label>visibility in air</rdfs:label>
	<generalQuantityKind xmlns="http://purl.oclc.org/NET/ssnx/qu/qu#" rdf:resource="http://purl.oclc.org/NET/ssnx/qu/quantity#distance"/>
	<rdfs:isDefinedBy rdf:resource="http://purl.oclc.org/NET/ssnx/cf/cf-property"/>
</rdf:Description>

<rdf:Description rdf:about="http://purl.oclc.org/NET/ssnx/cf/cf-property#atmosphere_hybrid_height_coordinate">
	<rdf:type rdf:resource="http://www.w3.org/2004/02/skos/core#Concept"/>
	<skos:inScheme rdf:resource="http://purl.oclc.org/NET/ssnx/qu/dim#Distance"/>
	<rdfs:comment>See Appendix D of the CF convention for information about dimensionless vertical coordinates.</rdfs:comment>
	<rdfs:label>atmosphere hybrid height coordinate</rdfs:label>
	<generalQuantityKind xmlns="http://purl.oclc.org/NET/ssnx/qu/qu#" rdf:resource="http://purl.oclc.org/NET/ssnx/qu/quantity#height"/>
</rdf:Description>

<rdf:Description rdf:about="http://purl.oclc.org/NET/ssnx/qu/quantity#height">
	<rdf:type rdf:resource="http://www.w3.org/2004/02/skos/core#Concept"/>
</rdf:Description>

<rdf:Description rdf:about="http://purl.oclc.org/NET/ssnx/cf/cf-property#atmosphere_hybrid_height_coordinate">
	<rdfs:isDefinedBy rdf:resource="http://purl.oclc.org/NET/ssnx/cf/cf-property"/>
</rdf:Description>

<rdf:Description rdf:about="http://purl.oclc.org/NET/ssnx/qu/quantity#height">
	<rdfs:isDefinedBy rdf:resource="http://purl.oclc.org/NET/ssnx/cf/cf-property"/>
</rdf:Description>

<rdf:Description rdf:about="http://purl.oclc.org/NET/ssnx/cf/cf-property#canopy_height">
	<rdf:type rdf:resource="http://www.w3.org/2004/02/skos/core#Concept"/>
	<skos:inScheme rdf:resource="http://purl.oclc.org/NET/ssnx/qu/dim#Distance"/>
	<rdfs:comment>Height is the vertical distance above the surface. "Canopy" means the plant or vegetation canopy.</rdfs:comment>
	<rdfs:label>canopy height</rdfs:label>
	<generalQuantityKind xmlns="http://purl.oclc.org/NET/ssnx/qu/qu#" rdf:resource="http://purl.oclc.org/NET/ssnx/qu/quantity#height"/>
	<rdfs:isDefinedBy rdf:resource="http://purl.oclc.org/NET/ssnx/cf/cf-property"/>
</rdf:Description>

<rdf:Description rdf:about="http://purl.oclc.org/NET/ssnx/cf/cf-property#convective_cloud_base_height">
	<rdf:type rdf:resource="http://www.w3.org/2004/02/skos/core#Concept"/>
	<skos:inScheme rdf:resource="http://purl.oclc.org/NET/ssnx/qu/dim#Distance"/>
	<rdfs:comment>cloud_base refers to the base of the lowest cloud. Height is the vertical distance above the surface. Convective cloud is that produced by the convection schemes in an atmosphere model.</rdfs:comment>
	<rdfs:label>convective cloud base height</rdfs:label>
	<generalQuantityKind xmlns="http://purl.oclc.org/NET/ssnx/qu/qu#" rdf:resource="http://purl.oclc.org/NET/ssnx/qu/quantity#height"/>
	<rdfs:isDefinedBy rdf:resource="http://purl.oclc.org/NET/ssnx/cf/cf-property"/>
</rdf:Description>

<rdf:Description rdf:about="http://purl.oclc.org/NET/ssnx/cf/cf-property#convective_cloud_top_height">
	<rdf:type rdf:resource="http://www.w3.org/2004/02/skos/core#Concept"/>
	<skos:inScheme rdf:resource="http://purl.oclc.org/NET/ssnx/qu/dim#Distance"/>
	<rdfs:comment>cloud_top refers to the top of the highest cloud. Height is the vertical distance above the surface. Convective cloud is that produced by the convection schemes in an atmosphere model.</rdfs:comment>
	<rdfs:label>convective cloud top height</rdfs:label>
	<generalQuantityKind xmlns="http://purl.oclc.org/NET/ssnx/qu/qu#" rdf:resource="http://purl.oclc.org/NET/ssnx/qu/quantity#height"/>
	<rdfs:isDefinedBy rdf:resource="http://purl.oclc.org/NET/ssnx/cf/cf-property"/>
</rdf:Description>

<rdf:Description rdf:about="http://purl.oclc.org/NET/ssnx/cf/cf-property#geoid_height_above_reference_ellipsoid">
	<rdf:type rdf:resource="http://www.w3.org/2004/02/skos/core#Concept"/>
	<skos:inScheme rdf:resource="http://purl.oclc.org/NET/ssnx/qu/dim#Distance"/>
	<rdfs:comment>The geoid is a surface of constant geopotential with which mean sea level would coincide if the ocean were at rest. (The volume enclosed between the geoid and the sea floor equals the mean volume of water in the ocean.) In an ocean GCM the geoid is the surface of zero depth, or the rigid lid if the model uses that approximation.  A reference ellipsoid is a regular mathematical figure that approximates the irregular shape of the geoid. A number of reference ellipsoids are defined for use in the field of geodesy.</rdfs:comment>
	<rdfs:label>geoid height above reference ellipsoid</rdfs:label>
	<generalQuantityKind xmlns="http://purl.oclc.org/NET/ssnx/qu/qu#" rdf:resource="http://purl.oclc.org/NET/ssnx/qu/quantity#height"/>
	<rdfs:isDefinedBy rdf:resource="http://purl.oclc.org/NET/ssnx/cf/cf-property"/>
</rdf:Description>

<rdf:Description rdf:about="http://purl.oclc.org/NET/ssnx/cf/cf-property#geopotential_height">
	<rdf:type rdf:resource="http://www.w3.org/2004/02/skos/core#Concept"/>
	<skos:inScheme rdf:resource="http://purl.oclc.org/NET/ssnx/qu/dim#Distance"/>
	<rdfs:comment>Geopotential is the sum of the specific gravitational potential energy relative to the geoid and the specific centripetal potential energy. Geopotential height is the geopotential divided by the standard acceleration due to gravity. It is numerically similar to the altitude (or geometric height) and not to the quantity with standard name height, which is relative to the surface.</rdfs:comment>
	<rdfs:label>geopotential height</rdfs:label>
	<generalQuantityKind xmlns="http://purl.oclc.org/NET/ssnx/qu/qu#" rdf:resource="http://purl.oclc.org/NET/ssnx/qu/quantity#height"/>
	<rdfs:isDefinedBy rdf:resource="http://purl.oclc.org/NET/ssnx/cf/cf-property"/>
</rdf:Description>

<rdf:Description rdf:about="http://purl.oclc.org/NET/ssnx/cf/cf-property#geopotential_height_anomaly">
	<rdf:type rdf:resource="http://www.w3.org/2004/02/skos/core#Concept"/>
	<skos:inScheme rdf:resource="http://purl.oclc.org/NET/ssnx/qu/dim#Distance"/>
	<rdfs:comment>"anomaly" means difference from climatology. Geopotential is the sum of the specific gravitational potential energy relative to the geoid and the specific centripetal potential energy. Geopotential height is the geopotential divided by the standard acceleration due to gravity. It is numerically similar to the altitude (or geometric height) and not to the quantity with standard name height, which is relative to the surface.</rdfs:comment>
	<rdfs:label>geopotential height anomaly</rdfs:label>
	<generalQuantityKind xmlns="http://purl.oclc.org/NET/ssnx/qu/qu#" rdf:resource="http://purl.oclc.org/NET/ssnx/qu/quantity#height"/>
	<rdfs:isDefinedBy rdf:resource="http://purl.oclc.org/NET/ssnx/cf/cf-property"/>
</rdf:Description>

<rdf:Description rdf:about="http://purl.oclc.org/NET/ssnx/cf/cf-property#height">
	<rdf:type rdf:resource="http://www.w3.org/2004/02/skos/core#Concept"/>
	<skos:inScheme rdf:resource="http://purl.oclc.org/NET/ssnx/qu/dim#Distance"/>
	<rdfs:comment>Height is the vertical distance above the surface.</rdfs:comment>
	<rdfs:label>height</rdfs:label>
	<generalQuantityKind xmlns="http://purl.oclc.org/NET/ssnx/qu/qu#" rdf:resource="http://purl.oclc.org/NET/ssnx/qu/quantity#height"/>
	<rdfs:isDefinedBy rdf:resource="http://purl.oclc.org/NET/ssnx/cf/cf-property"/>
</rdf:Description>

<rdf:Description rdf:about="http://purl.oclc.org/NET/ssnx/cf/cf-property#height_above_reference_ellipsoid">
	<rdf:type rdf:resource="http://www.w3.org/2004/02/skos/core#Concept"/>
	<skos:inScheme rdf:resource="http://purl.oclc.org/NET/ssnx/qu/dim#Distance"/>
	<rdfs:comment>Height is the vertical distance above a surface. A reference ellipsoid is a mathematical figure that approximates the geoid. The geoid is a surface of constant geopotential with which mean sea level would coincide if the ocean were at rest. The ellipsoid is an approximation because the geoid is an irregular shape. A number of reference ellipsoids are defined for use in the field of geodesy.</rdfs:comment>
	<rdfs:label>height above reference ellipsoid</rdfs:label>
	<generalQuantityKind xmlns="http://purl.oclc.org/NET/ssnx/qu/qu#" rdf:resource="http://purl.oclc.org/NET/ssnx/qu/quantity#height"/>
	<rdfs:isDefinedBy rdf:resource="http://purl.oclc.org/NET/ssnx/cf/cf-property"/>
</rdf:Description>

<rdf:Description rdf:about="http://purl.oclc.org/NET/ssnx/cf/cf-property#height_at_cloud_top">
	<rdf:type rdf:resource="http://www.w3.org/2004/02/skos/core#Concept"/>
	<skos:inScheme rdf:resource="http://purl.oclc.org/NET/ssnx/qu/dim#Distance"/>
	<rdfs:comment>cloud_top refers to the top of the highest cloud. Height is the vertical distance above the surface.</rdfs:comment>
	<rdfs:label>height at cloud top</rdfs:label>
	<generalQuantityKind xmlns="http://purl.oclc.org/NET/ssnx/qu/qu#" rdf:resource="http://purl.oclc.org/NET/ssnx/qu/quantity#height"/>
	<rdfs:isDefinedBy rdf:resource="http://purl.oclc.org/NET/ssnx/cf/cf-property"/>
</rdf:Description>

<rdf:Description rdf:about="http://purl.oclc.org/NET/ssnx/cf/cf-property#ocean_rigid_lid_pressure_expressed_as_sea_surface_height_above_geoid">
	<rdf:type rdf:resource="http://www.w3.org/2004/02/skos/core#Concept"/>
	<skos:inScheme rdf:resource="http://purl.oclc.org/NET/ssnx/qu/dim#Distance"/>
	<rdfs:comment>"Ocean rigid lid pressure" means the pressure at the surface of an ocean model assuming that it is bounded above by a rigid lid.</rdfs:comment>
	<rdfs:label>ocean rigid lid pressure expressed as sea surface height above geoid</rdfs:label>
	<generalQuantityKind xmlns="http://purl.oclc.org/NET/ssnx/qu/qu#" rdf:resource="http://purl.oclc.org/NET/ssnx/qu/quantity#height"/>
	<rdfs:isDefinedBy rdf:resource="http://purl.oclc.org/NET/ssnx/cf/cf-property"/>
</rdf:Description>

<rdf:Description rdf:about="http://purl.oclc.org/NET/ssnx/cf/cf-property#sea_surface_height_above_geoid">
	<rdf:type rdf:resource="http://www.w3.org/2004/02/skos/core#Concept"/>
	<skos:inScheme rdf:resource="http://purl.oclc.org/NET/ssnx/qu/dim#Distance"/>
	<rdfs:comment>The geoid is a surface of constant geopotential with which mean sea level would coincide if the ocean were at rest. (The volume enclosed between the geoid and the sea floor equals the mean volume of water in the ocean.) In an ocean GCM the geoid is the surface of zero depth, or the rigid lid if the model uses that approximation. "Sea surface height" is a time-varying quantity. By definition of the geoid, the global average of the time-mean sea surface height (i.e. mean sea level) above the geoid must be zero. The standard name for the height of the sea surface above mean sea level is sea_surface_height_above_sea_level. The standard name for the height of the sea surface above the reference ellipsoid is sea_surface_height_above_reference_ellipsoid.</rdfs:comment>
	<rdfs:label>sea surface height above geoid</rdfs:label>
	<generalQuantityKind xmlns="http://purl.oclc.org/NET/ssnx/qu/qu#" rdf:resource="http://purl.oclc.org/NET/ssnx/qu/quantity#height"/>
	<rdfs:isDefinedBy rdf:resource="http://purl.oclc.org/NET/ssnx/cf/cf-property"/>
</rdf:Description>

<rdf:Description rdf:about="http://purl.oclc.org/NET/ssnx/cf/cf-property#sea_surface_height_above_reference_ellipsoid">
	<rdf:type rdf:resource="http://www.w3.org/2004/02/skos/core#Concept"/>
	<skos:inScheme rdf:resource="http://purl.oclc.org/NET/ssnx/qu/dim#Distance"/>
	<rdfs:comment>"Sea surface height" is a time-varying quantity.  A reference ellipsoid is a mathematical figure that approximates the geoid.  The geoid is a surface of constant geopotential with which mean sea level would coincide if the ocean were at rest.  The ellipsoid is an approximation because the geoid is an irregular shape. A number of reference ellipsoids are defined for use in the field of geodesy.  The standard name for the height of the sea surface above the geoid is sea_surface_height_above_geoid.  The standard name for the height of the sea surface above mean sea level is sea_surface_height_above_sea_level.</rdfs:comment>
	<rdfs:label>sea surface height above reference ellipsoid</rdfs:label>
	<generalQuantityKind xmlns="http://purl.oclc.org/NET/ssnx/qu/qu#" rdf:resource="http://purl.oclc.org/NET/ssnx/qu/quantity#height"/>
	<rdfs:isDefinedBy rdf:resource="http://purl.oclc.org/NET/ssnx/cf/cf-property"/>
</rdf:Description>

<rdf:Description rdf:about="http://purl.oclc.org/NET/ssnx/cf/cf-property#radiation_wavelength">
	<rdf:type rdf:resource="http://www.w3.org/2004/02/skos/core#Concept"/>
	<skos:inScheme rdf:resource="http://purl.oclc.org/NET/ssnx/qu/dim#Distance"/>
	<rdfs:comment>The radiation wavelength can refer to any electromagnetic wave, such as light, heat radiation and radio waves.</rdfs:comment>
	<rdfs:label>radiation wavelength</rdfs:label>
	<generalQuantityKind xmlns="http://purl.oclc.org/NET/ssnx/qu/qu#" rdf:resource="http://purl.oclc.org/NET/ssnx/qu/quantity#length"/>
</rdf:Description>

<rdf:Description rdf:about="http://purl.oclc.org/NET/ssnx/qu/quantity#length">
	<rdf:type rdf:resource="http://www.w3.org/2004/02/skos/core#Concept"/>
</rdf:Description>

<rdf:Description rdf:about="http://purl.oclc.org/NET/ssnx/cf/cf-property#radiation_wavelength">
	<rdfs:isDefinedBy rdf:resource="http://purl.oclc.org/NET/ssnx/cf/cf-property"/>
</rdf:Description>

<rdf:Description rdf:about="http://purl.oclc.org/NET/ssnx/qu/quantity#length">
	<rdfs:isDefinedBy rdf:resource="http://purl.oclc.org/NET/ssnx/cf/cf-property"/>
</rdf:Description>

<rdf:Description rdf:about="http://purl.oclc.org/NET/ssnx/cf/cf-property#surface_roughness_length">
	<rdf:type rdf:resource="http://www.w3.org/2004/02/skos/core#Concept"/>
	<skos:inScheme rdf:resource="http://purl.oclc.org/NET/ssnx/qu/dim#Distance"/>
	<rdfs:comment>The surface called "surface" means the lower boundary of the atmosphere.</rdfs:comment>
	<rdfs:label>surface roughness length</rdfs:label>
	<generalQuantityKind xmlns="http://purl.oclc.org/NET/ssnx/qu/qu#" rdf:resource="http://purl.oclc.org/NET/ssnx/qu/quantity#length"/>
	<rdfs:isDefinedBy rdf:resource="http://purl.oclc.org/NET/ssnx/cf/cf-property"/>
</rdf:Description>

<rdf:Description rdf:about="http://purl.oclc.org/NET/ssnx/cf/cf-property#surface_roughness_length_for_heat_in_air">
	<rdf:type rdf:resource="http://www.w3.org/2004/02/skos/core#Concept"/>
	<skos:inScheme rdf:resource="http://purl.oclc.org/NET/ssnx/qu/dim#Distance"/>
	<rdfs:comment>The surface called "surface" means the lower boundary of the atmosphere.</rdfs:comment>
	<rdfs:label>surface roughness length for heat in air</rdfs:label>
	<generalQuantityKind xmlns="http://purl.oclc.org/NET/ssnx/qu/qu#" rdf:resource="http://purl.oclc.org/NET/ssnx/qu/quantity#length"/>
	<rdfs:isDefinedBy rdf:resource="http://purl.oclc.org/NET/ssnx/cf/cf-property"/>
</rdf:Description>

<rdf:Description rdf:about="http://purl.oclc.org/NET/ssnx/cf/cf-property#surface_roughness_length_for_momentum_in_air">
	<rdf:type rdf:resource="http://www.w3.org/2004/02/skos/core#Concept"/>
	<skos:inScheme rdf:resource="http://purl.oclc.org/NET/ssnx/qu/dim#Distance"/>
	<rdfs:comment>The surface called "surface" means the lower boundary of the atmosphere.</rdfs:comment>
	<rdfs:label>surface roughness length for momentum in air</rdfs:label>
	<generalQuantityKind xmlns="http://purl.oclc.org/NET/ssnx/qu/qu#" rdf:resource="http://purl.oclc.org/NET/ssnx/qu/quantity#length"/>
	<rdfs:isDefinedBy rdf:resource="http://purl.oclc.org/NET/ssnx/cf/cf-property"/>
</rdf:Description>

<rdf:Description rdf:about="http://purl.oclc.org/NET/ssnx/cf/cf-property#effective_radius_of_convective_cloud_ice_particle">
	<rdf:type rdf:resource="http://www.w3.org/2004/02/skos/core#Concept"/>
	<skos:inScheme rdf:resource="http://purl.oclc.org/NET/ssnx/qu/dim#Distance"/>
	<rdfs:comment> The effective radius of a size distribution of particles, such as aerosols, cloud droplets or ice crystals, is the area weighted mean radius of particle size. It is calculated as the ratio of the third to the second moment of the particle size distribution. Convective cloud is that produced by the convection schemes in an atmosphere model. </rdfs:comment>
	<rdfs:label>effective radius of convective cloud ice particle</rdfs:label>
	<generalQuantityKind xmlns="http://purl.oclc.org/NET/ssnx/qu/qu#" rdf:resource="http://purl.oclc.org/NET/ssnx/qu/quantity#radius"/>
</rdf:Description>

<rdf:Description rdf:about="http://purl.oclc.org/NET/ssnx/qu/quantity#radius">
	<rdf:type rdf:resource="http://www.w3.org/2004/02/skos/core#Concept"/>
</rdf:Description>

<rdf:Description rdf:about="http://purl.oclc.org/NET/ssnx/cf/cf-property#effective_radius_of_convective_cloud_ice_particle">
	<rdfs:isDefinedBy rdf:resource="http://purl.oclc.org/NET/ssnx/cf/cf-property"/>
</rdf:Description>

<rdf:Description rdf:about="http://purl.oclc.org/NET/ssnx/qu/quantity#radius">
	<rdfs:isDefinedBy rdf:resource="http://purl.oclc.org/NET/ssnx/cf/cf-property"/>
</rdf:Description>

<rdf:Description rdf:about="http://purl.oclc.org/NET/ssnx/cf/cf-property#effective_radius_of_convective_cloud_liquid_water_particle">
	<rdf:type rdf:resource="http://www.w3.org/2004/02/skos/core#Concept"/>
	<skos:inScheme rdf:resource="http://purl.oclc.org/NET/ssnx/qu/dim#Distance"/>
	<rdfs:comment> The effective radius of a size distribution of particles, such as aerosols, cloud droplets or ice crystals, is the area weighted mean radius of particle size. It is calculated as the ratio of the third to the second moment of the particle size distribution. Convective cloud is that produced by the convection schemes in an atmosphere model. </rdfs:comment>
	<rdfs:label>effective radius of convective cloud liquid water particle</rdfs:label>
	<generalQuantityKind xmlns="http://purl.oclc.org/NET/ssnx/qu/qu#" rdf:resource="http://purl.oclc.org/NET/ssnx/qu/quantity#radius"/>
	<rdfs:isDefinedBy rdf:resource="http://purl.oclc.org/NET/ssnx/cf/cf-property"/>
</rdf:Description>

<rdf:Description rdf:about="http://purl.oclc.org/NET/ssnx/cf/cf-property#effective_radius_of_convective_cloud_rain_particle">
	<rdf:type rdf:resource="http://www.w3.org/2004/02/skos/core#Concept"/>
	<skos:inScheme rdf:resource="http://purl.oclc.org/NET/ssnx/qu/dim#Distance"/>
	<rdfs:comment> The effective radius of a size distribution of particles, such as aerosols, cloud droplets or ice crystals, is the area weighted mean radius of particle size. It is calculated as the ratio of the third to the second moment of the particle size distribution. Convective cloud is that produced by the convection schemes in an atmosphere model. </rdfs:comment>
	<rdfs:label>effective radius of convective cloud rain particle</rdfs:label>
	<generalQuantityKind xmlns="http://purl.oclc.org/NET/ssnx/qu/qu#" rdf:resource="http://purl.oclc.org/NET/ssnx/qu/quantity#radius"/>
	<rdfs:isDefinedBy rdf:resource="http://purl.oclc.org/NET/ssnx/cf/cf-property"/>
</rdf:Description>

<rdf:Description rdf:about="http://purl.oclc.org/NET/ssnx/cf/cf-property#effective_radius_of_convective_cloud_snow_particle">
	<rdf:type rdf:resource="http://www.w3.org/2004/02/skos/core#Concept"/>
	<skos:inScheme rdf:resource="http://purl.oclc.org/NET/ssnx/qu/dim#Distance"/>
	<rdfs:comment> The effective radius of a size distribution of particles, such as aerosols, cloud droplets or ice crystals, is the area weighted mean radius of particle size. It is calculated as the ratio of the third to the second moment of the particle size distribution. Convective cloud is that produced by the convection schemes in an atmosphere model. </rdfs:comment>
	<rdfs:label>effective radius of convective cloud snow particle</rdfs:label>
	<generalQuantityKind xmlns="http://purl.oclc.org/NET/ssnx/qu/qu#" rdf:resource="http://purl.oclc.org/NET/ssnx/qu/quantity#radius"/>
	<rdfs:isDefinedBy rdf:resource="http://purl.oclc.org/NET/ssnx/cf/cf-property"/>
</rdf:Description>

<rdf:Description rdf:about="http://purl.oclc.org/NET/ssnx/cf/cf-property#effective_radius_of_stratiform_cloud_graupel_particle">
	<rdf:type rdf:resource="http://www.w3.org/2004/02/skos/core#Concept"/>
	<skos:inScheme rdf:resource="http://purl.oclc.org/NET/ssnx/qu/dim#Distance"/>
	<rdfs:comment> The effective radius of a size distribution of particles, such as aerosols, cloud droplets or ice crystals, is the area weighted mean radius of particle size. It is calculated as the ratio of the third to the second moment of the particle size distribution. In an atmosphere model, stratiform cloud is that produced by large-scale convergence (not the convection schemes).  </rdfs:comment>
	<rdfs:label>effective radius of stratiform cloud graupel particle</rdfs:label>
	<generalQuantityKind xmlns="http://purl.oclc.org/NET/ssnx/qu/qu#" rdf:resource="http://purl.oclc.org/NET/ssnx/qu/quantity#radius"/>
	<rdfs:isDefinedBy rdf:resource="http://purl.oclc.org/NET/ssnx/cf/cf-property"/>
</rdf:Description>

<rdf:Description rdf:about="http://purl.oclc.org/NET/ssnx/cf/cf-property#effective_radius_of_stratiform_cloud_ice_particle">
	<rdf:type rdf:resource="http://www.w3.org/2004/02/skos/core#Concept"/>
	<skos:inScheme rdf:resource="http://purl.oclc.org/NET/ssnx/qu/dim#Distance"/>
	<rdfs:comment> The effective radius of a size distribution of particles, such as aerosols, cloud droplets or ice crystals, is the area weighted mean radius of particle size. It is calculated as the ratio of the third to the second moment of the particle size distribution. In an atmosphere model, stratiform cloud is that produced by large-scale convergence (not the convection schemes). </rdfs:comment>
	<rdfs:label>effective radius of stratiform cloud ice particle</rdfs:label>
	<generalQuantityKind xmlns="http://purl.oclc.org/NET/ssnx/qu/qu#" rdf:resource="http://purl.oclc.org/NET/ssnx/qu/quantity#radius"/>
	<rdfs:isDefinedBy rdf:resource="http://purl.oclc.org/NET/ssnx/cf/cf-property"/>
</rdf:Description>

<rdf:Description rdf:about="http://purl.oclc.org/NET/ssnx/cf/cf-property#effective_radius_of_stratiform_cloud_liquid_water_particle">
	<rdf:type rdf:resource="http://www.w3.org/2004/02/skos/core#Concept"/>
	<skos:inScheme rdf:resource="http://purl.oclc.org/NET/ssnx/qu/dim#Distance"/>
	<rdfs:comment> The effective radius of a size distribution of particles, such as aerosols, cloud droplets or ice crystals, is the area weighted mean radius of particle size. It is calculated as the ratio of the third to the second moment of the particle size distribution. In an atmosphere model, stratiform cloud is that produced by large-scale convergence (not the convection schemes). </rdfs:comment>
	<rdfs:label>effective radius of stratiform cloud liquid water particle</rdfs:label>
	<generalQuantityKind xmlns="http://purl.oclc.org/NET/ssnx/qu/qu#" rdf:resource="http://purl.oclc.org/NET/ssnx/qu/quantity#radius"/>
	<rdfs:isDefinedBy rdf:resource="http://purl.oclc.org/NET/ssnx/cf/cf-property"/>
</rdf:Description>

<rdf:Description rdf:about="http://purl.oclc.org/NET/ssnx/cf/cf-property#effective_radius_of_stratiform_cloud_rain_particle">
	<rdf:type rdf:resource="http://www.w3.org/2004/02/skos/core#Concept"/>
	<skos:inScheme rdf:resource="http://purl.oclc.org/NET/ssnx/qu/dim#Distance"/>
	<rdfs:comment> The effective radius of a size distribution of particles, such as aerosols, cloud droplets or ice crystals, is the area weighted mean radius of particle size. It is calculated as the ratio of the third to the second moment of the particle size distribution. In an atmosphere model, stratiform cloud is that produced by large-scale convergence (not the convection schemes). </rdfs:comment>
	<rdfs:label>effective radius of stratiform cloud rain particle</rdfs:label>
	<generalQuantityKind xmlns="http://purl.oclc.org/NET/ssnx/qu/qu#" rdf:resource="http://purl.oclc.org/NET/ssnx/qu/quantity#radius"/>
	<rdfs:isDefinedBy rdf:resource="http://purl.oclc.org/NET/ssnx/cf/cf-property"/>
</rdf:Description>

<rdf:Description rdf:about="http://purl.oclc.org/NET/ssnx/cf/cf-property#effective_radius_of_stratiform_cloud_snow_particle">
	<rdf:type rdf:resource="http://www.w3.org/2004/02/skos/core#Concept"/>
	<skos:inScheme rdf:resource="http://purl.oclc.org/NET/ssnx/qu/dim#Distance"/>
	<rdfs:comment> The effective radius of a size distribution of particles, such as aerosols, cloud droplets or ice crystals, is the area weighted mean radius of particle size. It is calculated as the ratio of the third to the second moment of the particle size distribution. In an atmosphere model, stratiform cloud is that produced by large-scale convergence (not the convection schemes). </rdfs:comment>
	<rdfs:label>effective radius of stratiform cloud snow particle</rdfs:label>
	<generalQuantityKind xmlns="http://purl.oclc.org/NET/ssnx/qu/qu#" rdf:resource="http://purl.oclc.org/NET/ssnx/qu/quantity#radius"/>
	<rdfs:isDefinedBy rdf:resource="http://purl.oclc.org/NET/ssnx/cf/cf-property"/>
</rdf:Description>

<rdf:Description rdf:about="http://purl.oclc.org/NET/ssnx/cf/cf-property#atmosphere_boundary_layer_thickness">
	<rdf:type rdf:resource="http://www.w3.org/2004/02/skos/core#Concept"/>
	<skos:inScheme rdf:resource="http://purl.oclc.org/NET/ssnx/qu/dim#Distance"/>
	<rdfs:comment>The atmosphere boundary layer thickness is the "depth" or "height" of the (atmosphere) planetary boundary layer.</rdfs:comment>
	<rdfs:label>atmosphere boundary layer thickness</rdfs:label>
	<generalQuantityKind xmlns="http://purl.oclc.org/NET/ssnx/qu/qu#" rdf:resource="http://purl.oclc.org/NET/ssnx/qu/quantity#thickness"/>
</rdf:Description>

<rdf:Description rdf:about="http://purl.oclc.org/NET/ssnx/qu/quantity#thickness">
	<rdf:type rdf:resource="http://www.w3.org/2004/02/skos/core#Concept"/>
</rdf:Description>

<rdf:Description rdf:about="http://purl.oclc.org/NET/ssnx/cf/cf-property#atmosphere_boundary_layer_thickness">
	<rdfs:isDefinedBy rdf:resource="http://purl.oclc.org/NET/ssnx/cf/cf-property"/>
</rdf:Description>

<rdf:Description rdf:about="http://purl.oclc.org/NET/ssnx/qu/quantity#thickness">
	<rdfs:isDefinedBy rdf:resource="http://purl.oclc.org/NET/ssnx/cf/cf-property"/>
</rdf:Description>

<rdf:Description rdf:about="http://purl.oclc.org/NET/ssnx/cf/cf-property#cell_thickness">
	<rdf:type rdf:resource="http://www.w3.org/2004/02/skos/core#Concept"/>
	<skos:inScheme rdf:resource="http://purl.oclc.org/NET/ssnx/qu/dim#Distance"/>
	<rdfs:comment> "Thickness" means the vertical extent of a layer. "Cell" refers to a model grid-cell.</rdfs:comment>
	<rdfs:label>cell thickness</rdfs:label>
	<generalQuantityKind xmlns="http://purl.oclc.org/NET/ssnx/qu/qu#" rdf:resource="http://purl.oclc.org/NET/ssnx/qu/quantity#thickness"/>
	<rdfs:isDefinedBy rdf:resource="http://purl.oclc.org/NET/ssnx/cf/cf-property"/>
</rdf:Description>

<rdf:Description rdf:about="http://purl.oclc.org/NET/ssnx/cf/cf-property#equivalent_thickness_at_stp_of_atmosphere_ozone_content">
	<rdf:type rdf:resource="http://www.w3.org/2004/02/skos/core#Concept"/>
	<skos:inScheme rdf:resource="http://purl.oclc.org/NET/ssnx/qu/dim#Distance"/>
	<rdfs:comment>"stp" means standard temperature (0 degC) and pressure (101325 Pa). "Content" indicates a quantity per unit area. The "atmosphere content" of a quantity refers to the vertical integral from the surface to the top of the atmosphere. For the content between specified levels in the atmosphere, standard names including content_of_atmosphere_layer are used. The equivalent thickness at STP of a particular constituent of the atmosphere is the thickness of the layer that the gas would occupy if it was separated from the other constituents and gathered together at STP.</rdfs:comment>
	<rdfs:label>equivalent thickness at stp of atmosphere ozone content</rdfs:label>
	<generalQuantityKind xmlns="http://purl.oclc.org/NET/ssnx/qu/qu#" rdf:resource="http://purl.oclc.org/NET/ssnx/qu/quantity#thickness"/>
	<rdfs:isDefinedBy rdf:resource="http://purl.oclc.org/NET/ssnx/cf/cf-property"/>
</rdf:Description>

<rdf:Description rdf:about="http://purl.oclc.org/NET/ssnx/cf/cf-property#floating_ice_thickness">
	<rdf:type rdf:resource="http://www.w3.org/2004/02/skos/core#Concept"/>
	<skos:inScheme rdf:resource="http://purl.oclc.org/NET/ssnx/qu/dim#Distance"/>
	<rdfs:comment>"Floating ice" means any ice that is floating on water, e.g. on a sea or lake surface.  "Thickness" means the vertical extent of the ice.</rdfs:comment>
	<rdfs:label>floating ice thickness</rdfs:label>
	<generalQuantityKind xmlns="http://purl.oclc.org/NET/ssnx/qu/qu#" rdf:resource="http://purl.oclc.org/NET/ssnx/qu/quantity#thickness"/>
	<rdfs:isDefinedBy rdf:resource="http://purl.oclc.org/NET/ssnx/cf/cf-property"/>
</rdf:Description>

<rdf:Description rdf:about="http://purl.oclc.org/NET/ssnx/cf/cf-property#land_ice_thickness">
	<rdf:type rdf:resource="http://www.w3.org/2004/02/skos/core#Concept"/>
	<skos:inScheme rdf:resource="http://purl.oclc.org/NET/ssnx/qu/dim#Distance"/>
	<rdfs:comment>"Land ice" means glaciers, ice-caps and ice-sheets resting on bedrock and also includes ice-shelves. "Thickness" means the vertical extent of a layer.</rdfs:comment>
	<rdfs:label>land ice thickness</rdfs:label>
	<generalQuantityKind xmlns="http://purl.oclc.org/NET/ssnx/qu/qu#" rdf:resource="http://purl.oclc.org/NET/ssnx/qu/quantity#thickness"/>
	<rdfs:isDefinedBy rdf:resource="http://purl.oclc.org/NET/ssnx/cf/cf-property"/>
</rdf:Description>

<rdf:Description rdf:about="http://purl.oclc.org/NET/ssnx/cf/cf-property#lwe_thickness_of_atmosphere_water_vapor_content">
	<rdf:type rdf:resource="http://www.w3.org/2004/02/skos/core#Concept"/>
	<skos:inScheme rdf:resource="http://purl.oclc.org/NET/ssnx/qu/dim#Distance"/>
	<rdfs:comment>"lwe" means liquid water equivalent. The construction lwe_thickness_of_X_amount or _content means the vertical extent of a layer of liquid water having the same mass per unit area. "Content" indicates a quantity per unit area. The "atmosphere content" of a quantity refers to the vertical integral from the surface to the top of the atmosphere. For the content between specified levels in the atmosphere, standard names including content_of_atmosphere_layer are used. Atmosphere water vapor content is sometimes referred to as "precipitable water", although this term does not imply the water could all be precipitated.</rdfs:comment>
	<rdfs:label>lwe thickness of atmosphere water vapor content</rdfs:label>
	<generalQuantityKind xmlns="http://purl.oclc.org/NET/ssnx/qu/qu#" rdf:resource="http://purl.oclc.org/NET/ssnx/qu/quantity#thickness"/>
	<rdfs:isDefinedBy rdf:resource="http://purl.oclc.org/NET/ssnx/cf/cf-property"/>
</rdf:Description>

<rdf:Description rdf:about="http://purl.oclc.org/NET/ssnx/cf/cf-property#lwe_thickness_of_canopy_water_amount">
	<rdf:type rdf:resource="http://www.w3.org/2004/02/skos/core#Concept"/>
	<skos:inScheme rdf:resource="http://purl.oclc.org/NET/ssnx/qu/dim#Distance"/>
	<rdfs:comment>"lwe" means liquid water equivalent. "Amount" means mass per unit area. The construction lwe_thickness_of_X_amount or _content means the vertical extent of a layer of liquid water having the same mass per unit area. "Water" means water in all phases, including frozen i.e. ice and snow. "Canopy" means the plant or vegetation canopy. The canopy water is the water on the canopy.</rdfs:comment>
	<rdfs:label>lwe thickness of canopy water amount</rdfs:label>
	<generalQuantityKind xmlns="http://purl.oclc.org/NET/ssnx/qu/qu#" rdf:resource="http://purl.oclc.org/NET/ssnx/qu/quantity#thickness"/>
	<rdfs:isDefinedBy rdf:resource="http://purl.oclc.org/NET/ssnx/cf/cf-property"/>
</rdf:Description>

<rdf:Description rdf:about="http://purl.oclc.org/NET/ssnx/cf/cf-property#lwe_thickness_of_convective_precipitation_amount">
	<rdf:type rdf:resource="http://www.w3.org/2004/02/skos/core#Concept"/>
	<skos:inScheme rdf:resource="http://purl.oclc.org/NET/ssnx/qu/dim#Distance"/>
	<rdfs:comment>"lwe" means liquid water equivalent. "Amount" means mass per unit area. The construction lwe_thickness_of_X_amount or _content means the vertical extent of a layer of liquid water having the same mass per unit area.</rdfs:comment>
	<rdfs:label>lwe thickness of convective precipitation amount</rdfs:label>
	<generalQuantityKind xmlns="http://purl.oclc.org/NET/ssnx/qu/qu#" rdf:resource="http://purl.oclc.org/NET/ssnx/qu/quantity#thickness"/>
	<rdfs:isDefinedBy rdf:resource="http://purl.oclc.org/NET/ssnx/cf/cf-property"/>
</rdf:Description>

<rdf:Description rdf:about="http://purl.oclc.org/NET/ssnx/cf/cf-property#lwe_thickness_of_convective_snowfall_amount">
	<rdf:type rdf:resource="http://www.w3.org/2004/02/skos/core#Concept"/>
	<skos:inScheme rdf:resource="http://purl.oclc.org/NET/ssnx/qu/dim#Distance"/>
	<rdfs:comment>"lwe" means liquid water equivalent. "Amount" means mass per unit area. The construction lwe_thickness_of_X_amount or _content means the vertical extent of a layer of liquid water having the same mass per unit area.</rdfs:comment>
	<rdfs:label>lwe thickness of convective snowfall amount</rdfs:label>
	<generalQuantityKind xmlns="http://purl.oclc.org/NET/ssnx/qu/qu#" rdf:resource="http://purl.oclc.org/NET/ssnx/qu/quantity#thickness"/>
	<rdfs:isDefinedBy rdf:resource="http://purl.oclc.org/NET/ssnx/cf/cf-property"/>
</rdf:Description>

<rdf:Description rdf:about="http://purl.oclc.org/NET/ssnx/cf/cf-property#lwe_thickness_of_frozen_water_content_of_soil_layer">
	<rdf:type rdf:resource="http://www.w3.org/2004/02/skos/core#Concept"/>
	<skos:inScheme rdf:resource="http://purl.oclc.org/NET/ssnx/qu/dim#Distance"/>
	<rdfs:comment>"frozen_water" means ice. "lwe" means liquid water equivalent. The construction lwe_thickness_of_X_amount or _content means the vertical extent of a layer of liquid water having the same mass per unit area. "Content" indicates a quantity per unit area. "Layer" means any layer with upper and lower boundaries that have constant values in some vertical coordinate. There must be a vertical coordinate variable indicating the extent of the layer(s). If the layers are model layers, the vertical coordinate can be model_level_number, but it is recommended to specify a physical coordinate (in a scalar or auxiliary coordinate variable) as well. Quantities defined for a soil layer must have a vertical coordinate variable with boundaries indicating the extent of the layer(s).</rdfs:comment>
	<rdfs:label>lwe thickness of frozen water content of soil layer</rdfs:label>
	<generalQuantityKind xmlns="http://purl.oclc.org/NET/ssnx/qu/qu#" rdf:resource="http://purl.oclc.org/NET/ssnx/qu/quantity#thickness"/>
	<rdfs:isDefinedBy rdf:resource="http://purl.oclc.org/NET/ssnx/cf/cf-property"/>
</rdf:Description>

<rdf:Description rdf:about="http://purl.oclc.org/NET/ssnx/cf/cf-property#lwe_thickness_of_large_scale_precipitation_amount">
	<rdf:type rdf:resource="http://www.w3.org/2004/02/skos/core#Concept"/>
	<skos:inScheme rdf:resource="http://purl.oclc.org/NET/ssnx/qu/dim#Distance"/>
	<rdfs:comment>"lwe" means liquid water equivalent. "Amount" means mass per unit area. The construction lwe_thickness_of_X_amount or _content means the vertical extent of a layer of liquid water having the same mass per unit area.</rdfs:comment>
	<rdfs:label>lwe thickness of large scale precipitation amount</rdfs:label>
	<generalQuantityKind xmlns="http://purl.oclc.org/NET/ssnx/qu/qu#" rdf:resource="http://purl.oclc.org/NET/ssnx/qu/quantity#thickness"/>
	<rdfs:isDefinedBy rdf:resource="http://purl.oclc.org/NET/ssnx/cf/cf-property"/>
</rdf:Description>

<rdf:Description rdf:about="http://purl.oclc.org/NET/ssnx/cf/cf-property#lwe_thickness_of_large_scale_snowfall_amount">
	<rdf:type rdf:resource="http://www.w3.org/2004/02/skos/core#Concept"/>
	<skos:inScheme rdf:resource="http://purl.oclc.org/NET/ssnx/qu/dim#Distance"/>
	<rdfs:comment>"lwe" means liquid water equivalent. "Amount" means mass per unit area. The construction lwe_thickness_of_X_amount or _content means the vertical extent of a layer of liquid water having the same mass per unit area.</rdfs:comment>
	<rdfs:label>lwe thickness of large scale snowfall amount</rdfs:label>
	<generalQuantityKind xmlns="http://purl.oclc.org/NET/ssnx/qu/qu#" rdf:resource="http://purl.oclc.org/NET/ssnx/qu/quantity#thickness"/>
	<rdfs:isDefinedBy rdf:resource="http://purl.oclc.org/NET/ssnx/cf/cf-property"/>
</rdf:Description>

<rdf:Description rdf:about="http://purl.oclc.org/NET/ssnx/cf/cf-property#lwe_thickness_of_moisture_content_of_soil_layer">
	<rdf:type rdf:resource="http://www.w3.org/2004/02/skos/core#Concept"/>
	<skos:inScheme rdf:resource="http://purl.oclc.org/NET/ssnx/qu/dim#Distance"/>
	<rdfs:comment>"lwe" means liquid water equivalent. "moisture" means water in all phases contained in soil. The construction lwe_thickness_of_X_amount or _content means the vertical extent of a layer of liquid water having the same mass per unit area. "Content" indicates a quantity per unit area. "Layer" means any layer with upper and lower boundaries that have constant values in some vertical coordinate. There must be a vertical coordinate variable indicating the extent of the layer(s). If the layers are model layers, the vertical coordinate can be model_level_number, but it is recommended to specify a physical coordinate (in a scalar or auxiliary coordinate variable) as well. Quantities defined for a soil layer must have a vertical coordinate variable with boundaries indicating the extent of the layer(s).</rdfs:comment>
	<rdfs:label>lwe thickness of moisture content of soil layer</rdfs:label>
	<generalQuantityKind xmlns="http://purl.oclc.org/NET/ssnx/qu/qu#" rdf:resource="http://purl.oclc.org/NET/ssnx/qu/quantity#thickness"/>
	<rdfs:isDefinedBy rdf:resource="http://purl.oclc.org/NET/ssnx/cf/cf-property"/>
</rdf:Description>

<rdf:Description rdf:about="http://purl.oclc.org/NET/ssnx/cf/cf-property#lwe_thickness_of_precipitation_amount">
	<rdf:type rdf:resource="http://www.w3.org/2004/02/skos/core#Concept"/>
	<skos:inScheme rdf:resource="http://purl.oclc.org/NET/ssnx/qu/dim#Distance"/>
	<rdfs:comment>"lwe" means liquid water equivalent. "Amount" means mass per unit area. The construction lwe_thickness_of_X_amount or _content means the vertical extent of a layer of liquid water having the same mass per unit area.</rdfs:comment>
	<rdfs:label>lwe thickness of precipitation amount</rdfs:label>
	<generalQuantityKind xmlns="http://purl.oclc.org/NET/ssnx/qu/qu#" rdf:resource="http://purl.oclc.org/NET/ssnx/qu/quantity#thickness"/>
	<rdfs:isDefinedBy rdf:resource="http://purl.oclc.org/NET/ssnx/cf/cf-property"/>
</rdf:Description>

<rdf:Description rdf:about="http://purl.oclc.org/NET/ssnx/cf/cf-property#lwe_thickness_of_snowfall_amount">
	<rdf:type rdf:resource="http://www.w3.org/2004/02/skos/core#Concept"/>
	<skos:inScheme rdf:resource="http://purl.oclc.org/NET/ssnx/qu/dim#Distance"/>
	<rdfs:comment>"lwe" means liquid water equivalent. "Amount" means mass per unit area. The construction lwe_thickness_of_X_amount or _content means the vertical extent of a layer of liquid water having the same mass per unit area.</rdfs:comment>
	<rdfs:label>lwe thickness of snowfall amount</rdfs:label>
	<generalQuantityKind xmlns="http://purl.oclc.org/NET/ssnx/qu/qu#" rdf:resource="http://purl.oclc.org/NET/ssnx/qu/quantity#thickness"/>
	<rdfs:isDefinedBy rdf:resource="http://purl.oclc.org/NET/ssnx/cf/cf-property"/>
</rdf:Description>

<rdf:Description rdf:about="http://purl.oclc.org/NET/ssnx/cf/cf-property#lwe_thickness_of_soil_moisture_content">
	<rdf:type rdf:resource="http://www.w3.org/2004/02/skos/core#Concept"/>
	<skos:inScheme rdf:resource="http://purl.oclc.org/NET/ssnx/qu/dim#Distance"/>
	<rdfs:comment>"lwe" means liquid water equivalent. "moisture" means water in all phases contained in soil. The construction lwe_thickness_of_X_amount or _content means the vertical extent of a layer of liquid water having the same mass per unit area. "Content" indicates a quantity per unit area. The "soil content" of a quantity refers to the vertical integral from the surface down to the bottom of the soil model. For the content between specified levels in the soil, standard names including content_of_soil_layer are used.</rdfs:comment>
	<rdfs:label>lwe thickness of soil moisture content</rdfs:label>
	<generalQuantityKind xmlns="http://purl.oclc.org/NET/ssnx/qu/qu#" rdf:resource="http://purl.oclc.org/NET/ssnx/qu/quantity#thickness"/>
	<rdfs:isDefinedBy rdf:resource="http://purl.oclc.org/NET/ssnx/cf/cf-property"/>
</rdf:Description>

<rdf:Description rdf:about="http://purl.oclc.org/NET/ssnx/cf/cf-property#lwe_thickness_of_surface_snow_amount">
	<rdf:type rdf:resource="http://www.w3.org/2004/02/skos/core#Concept"/>
	<skos:inScheme rdf:resource="http://purl.oclc.org/NET/ssnx/qu/dim#Distance"/>
	<rdfs:comment>The surface called "surface" means the lower boundary of the atmosphere. "lwe" means liquid water equivalent. "Amount" means mass per unit area. The construction lwe_thickness_of_X_amount or _content means the vertical extent of a layer of liquid water having the same mass per unit area. Surface amount refers to the amount on the ground, excluding that on the plant or vegetation canopy.</rdfs:comment>
	<rdfs:label>lwe thickness of surface snow amount</rdfs:label>
	<generalQuantityKind xmlns="http://purl.oclc.org/NET/ssnx/qu/qu#" rdf:resource="http://purl.oclc.org/NET/ssnx/qu/quantity#thickness"/>
	<rdfs:isDefinedBy rdf:resource="http://purl.oclc.org/NET/ssnx/cf/cf-property"/>
</rdf:Description>

<rdf:Description rdf:about="http://purl.oclc.org/NET/ssnx/cf/cf-property#lwe_thickness_of_water_evaporation_amount">
	<rdf:type rdf:resource="http://www.w3.org/2004/02/skos/core#Concept"/>
	<skos:inScheme rdf:resource="http://purl.oclc.org/NET/ssnx/qu/dim#Distance"/>
	<rdfs:comment>"lwe" means liquid water equivalent. "Amount" means mass per unit area. The construction lwe_thickness_of_X_amount or _content means the vertical extent of a layer of liquid water having the same mass per unit area. "Water" means water in all phases. Evaporation is the conversion of liquid or solid into vapor. (The conversion of solid alone into vapor is called "sublimation".)</rdfs:comment>
	<rdfs:label>lwe thickness of water evaporation amount</rdfs:label>
	<generalQuantityKind xmlns="http://purl.oclc.org/NET/ssnx/qu/qu#" rdf:resource="http://purl.oclc.org/NET/ssnx/qu/quantity#thickness"/>
	<rdfs:isDefinedBy rdf:resource="http://purl.oclc.org/NET/ssnx/cf/cf-property"/>
</rdf:Description>

<rdf:Description rdf:about="http://purl.oclc.org/NET/ssnx/cf/cf-property#ocean_mixed_layer_thickness">
	<rdf:type rdf:resource="http://www.w3.org/2004/02/skos/core#Concept"/>
	<skos:inScheme rdf:resource="http://purl.oclc.org/NET/ssnx/qu/dim#Distance"/>
	<rdfs:comment>The ocean mixed layer is the upper part of the ocean, regarded as being well-mixed. Various criteria are used to define the mixed layer; this can be specified by using a standard name of ocean_mixed_layer_defined_byX.</rdfs:comment>
	<rdfs:label>ocean mixed layer thickness</rdfs:label>
	<generalQuantityKind xmlns="http://purl.oclc.org/NET/ssnx/qu/qu#" rdf:resource="http://purl.oclc.org/NET/ssnx/qu/quantity#thickness"/>
	<rdfs:isDefinedBy rdf:resource="http://purl.oclc.org/NET/ssnx/cf/cf-property"/>
</rdf:Description>

<rdf:Description rdf:about="http://purl.oclc.org/NET/ssnx/cf/cf-property#ocean_mixed_layer_thickness_defined_by_mixing_scheme">
	<rdf:type rdf:resource="http://www.w3.org/2004/02/skos/core#Concept"/>
	<skos:inScheme rdf:resource="http://purl.oclc.org/NET/ssnx/qu/dim#Distance"/>
	<rdfs:comment>The ocean mixed layer is the upper part of the ocean, regarded as being well-mixed. The base of the mixed layer defined by the mixing scheme is a diagnostic of ocean models.</rdfs:comment>
	<rdfs:label>ocean mixed layer thickness defined by mixing scheme</rdfs:label>
	<generalQuantityKind xmlns="http://purl.oclc.org/NET/ssnx/qu/qu#" rdf:resource="http://purl.oclc.org/NET/ssnx/qu/quantity#thickness"/>
	<rdfs:isDefinedBy rdf:resource="http://purl.oclc.org/NET/ssnx/cf/cf-property"/>
</rdf:Description>

<rdf:Description rdf:about="http://purl.oclc.org/NET/ssnx/cf/cf-property#ocean_mixed_layer_thickness_defined_by_sigma_t">
	<rdf:type rdf:resource="http://www.w3.org/2004/02/skos/core#Concept"/>
	<skos:inScheme rdf:resource="http://purl.oclc.org/NET/ssnx/qu/dim#Distance"/>
	<rdfs:comment>The ocean mixed layer is the upper part of the ocean, regarded as being well-mixed. The base of the mixed layer defined by temperature, sigma or sigma_theta is the level at which the quantity indicated differs from its surface value by a certain amount.</rdfs:comment>
	<rdfs:label>ocean mixed layer thickness defined by sigma t</rdfs:label>
	<generalQuantityKind xmlns="http://purl.oclc.org/NET/ssnx/qu/qu#" rdf:resource="http://purl.oclc.org/NET/ssnx/qu/quantity#thickness"/>
	<rdfs:isDefinedBy rdf:resource="http://purl.oclc.org/NET/ssnx/cf/cf-property"/>
</rdf:Description>

<rdf:Description rdf:about="http://purl.oclc.org/NET/ssnx/cf/cf-property#ocean_mixed_layer_thickness_defined_by_sigma_theta">
	<rdf:type rdf:resource="http://www.w3.org/2004/02/skos/core#Concept"/>
	<skos:inScheme rdf:resource="http://purl.oclc.org/NET/ssnx/qu/dim#Distance"/>
	<rdfs:comment>The ocean mixed layer is the upper part of the ocean, regarded as being well-mixed. The base of the mixed layer defined by temperature, sigma or sigma_theta is the level at which the quantity indicated differs from its surface value by a certain amount.</rdfs:comment>
	<rdfs:label>ocean mixed layer thickness defined by sigma theta</rdfs:label>
	<generalQuantityKind xmlns="http://purl.oclc.org/NET/ssnx/qu/qu#" rdf:resource="http://purl.oclc.org/NET/ssnx/qu/quantity#thickness"/>
	<rdfs:isDefinedBy rdf:resource="http://purl.oclc.org/NET/ssnx/cf/cf-property"/>
</rdf:Description>

<rdf:Description rdf:about="http://purl.oclc.org/NET/ssnx/cf/cf-property#ocean_mixed_layer_thickness_defined_by_temperature">
	<rdf:type rdf:resource="http://www.w3.org/2004/02/skos/core#Concept"/>
	<skos:inScheme rdf:resource="http://purl.oclc.org/NET/ssnx/qu/dim#Distance"/>
	<rdfs:comment>The ocean mixed layer is the upper part of the ocean, regarded as being well-mixed. The base of the mixed layer defined by temperature, sigma or sigma_theta is the level at which the quantity indicated differs from its surface value by a certain amount.</rdfs:comment>
	<rdfs:label>ocean mixed layer thickness defined by temperature</rdfs:label>
	<generalQuantityKind xmlns="http://purl.oclc.org/NET/ssnx/qu/qu#" rdf:resource="http://purl.oclc.org/NET/ssnx/qu/quantity#thickness"/>
	<rdfs:isDefinedBy rdf:resource="http://purl.oclc.org/NET/ssnx/cf/cf-property"/>
</rdf:Description>

<rdf:Description rdf:about="http://purl.oclc.org/NET/ssnx/cf/cf-property#ocean_mixed_layer_thickness_defined_by_vertical_tracer_diffusivity">
	<rdf:type rdf:resource="http://www.w3.org/2004/02/skos/core#Concept"/>
	<skos:inScheme rdf:resource="http://purl.oclc.org/NET/ssnx/qu/dim#Distance"/>
	<rdfs:comment>The ocean mixed layer is the upper part of the ocean, regarded as being well-mixed. The base of the mixed layer defined by temperature, sigma, sigma_theta, or vertical diffusivity is the level at which the quantity indicated differs from its surface value by a certain amount. The amount by which the quantity differs can be specified by a scalar coordinate variable.</rdfs:comment>
	<rdfs:label>ocean mixed layer thickness defined by vertical tracer diffusivity</rdfs:label>
	<generalQuantityKind xmlns="http://purl.oclc.org/NET/ssnx/qu/qu#" rdf:resource="http://purl.oclc.org/NET/ssnx/qu/quantity#thickness"/>
	<rdfs:isDefinedBy rdf:resource="http://purl.oclc.org/NET/ssnx/cf/cf-property"/>
</rdf:Description>

<rdf:Description rdf:about="http://purl.oclc.org/NET/ssnx/cf/cf-property#surface_snow_thickness">
	<rdf:type rdf:resource="http://www.w3.org/2004/02/skos/core#Concept"/>
	<skos:inScheme rdf:resource="http://purl.oclc.org/NET/ssnx/qu/dim#Distance"/>
	<rdfs:comment>The surface called "surface" means the lower boundary of the atmosphere. Unless indicated in the cell_methods attribute, a quantity is assumed to apply to the whole area of each horizontal grid box. Previously, the qualifier where_type was used to specify that the quantity applies only to the part of the grid box of the named type.  Names containing the where_type qualifier are deprecated and newly created data should use the cell_methods attribute to indicate the horizontal area to which the quantity applies.</rdfs:comment>
	<rdfs:label>surface snow thickness</rdfs:label>
	<generalQuantityKind xmlns="http://purl.oclc.org/NET/ssnx/qu/qu#" rdf:resource="http://purl.oclc.org/NET/ssnx/qu/quantity#thickness"/>
	<rdfs:isDefinedBy rdf:resource="http://purl.oclc.org/NET/ssnx/cf/cf-property"/>
</rdf:Description>

<rdf:Description rdf:about="http://purl.oclc.org/NET/ssnx/cf/cf-property#thickness_of_convective_rainfall_amount">
	<rdf:type rdf:resource="http://www.w3.org/2004/02/skos/core#Concept"/>
	<skos:inScheme rdf:resource="http://purl.oclc.org/NET/ssnx/qu/dim#Distance"/>
	<rdfs:comment>"Amount" means mass per unit area. The construction thickness_of_[X_]rainfall_amount means the accumulated "depth" of rainfall i.e. the thickness of a layer of liquid water having the same mass per unit area as the rainfall amount.</rdfs:comment>
	<rdfs:label>thickness of convective rainfall amount</rdfs:label>
	<generalQuantityKind xmlns="http://purl.oclc.org/NET/ssnx/qu/qu#" rdf:resource="http://purl.oclc.org/NET/ssnx/qu/quantity#thickness"/>
	<rdfs:isDefinedBy rdf:resource="http://purl.oclc.org/NET/ssnx/cf/cf-property"/>
</rdf:Description>

<rdf:Description rdf:about="http://purl.oclc.org/NET/ssnx/cf/cf-property#thickness_of_convective_snowfall_amount">
	<rdf:type rdf:resource="http://www.w3.org/2004/02/skos/core#Concept"/>
	<skos:inScheme rdf:resource="http://purl.oclc.org/NET/ssnx/qu/dim#Distance"/>
	<rdfs:comment>"Amount" means mass per unit area. The construction thickness_of_[X_]snowfall_amount means the accumulated "depth" of snow which fell i.e. the thickness of the layer of snow at its own density. There are corresponding standard names for liquid water equivalent (lwe) thickness.</rdfs:comment>
	<rdfs:label>thickness of convective snowfall amount</rdfs:label>
	<generalQuantityKind xmlns="http://purl.oclc.org/NET/ssnx/qu/qu#" rdf:resource="http://purl.oclc.org/NET/ssnx/qu/quantity#thickness"/>
	<rdfs:isDefinedBy rdf:resource="http://purl.oclc.org/NET/ssnx/cf/cf-property"/>
</rdf:Description>

<rdf:Description rdf:about="http://purl.oclc.org/NET/ssnx/cf/cf-property#thickness_of_large_scale_rainfall_amount">
	<rdf:type rdf:resource="http://www.w3.org/2004/02/skos/core#Concept"/>
	<skos:inScheme rdf:resource="http://purl.oclc.org/NET/ssnx/qu/dim#Distance"/>
	<rdfs:comment>"Amount" means mass per unit area. The construction thickness_of_[X_]rainfall_amount means the accumulated "depth" of rainfall i.e. the thickness of a layer of liquid water having the same mass per unit area as the rainfall amount.</rdfs:comment>
	<rdfs:label>thickness of large scale rainfall amount</rdfs:label>
	<generalQuantityKind xmlns="http://purl.oclc.org/NET/ssnx/qu/qu#" rdf:resource="http://purl.oclc.org/NET/ssnx/qu/quantity#thickness"/>
	<rdfs:isDefinedBy rdf:resource="http://purl.oclc.org/NET/ssnx/cf/cf-property"/>
</rdf:Description>

<rdf:Description rdf:about="http://purl.oclc.org/NET/ssnx/cf/cf-property#thickness_of_large_scale_snowfall_amount">
	<rdf:type rdf:resource="http://www.w3.org/2004/02/skos/core#Concept"/>
	<skos:inScheme rdf:resource="http://purl.oclc.org/NET/ssnx/qu/dim#Distance"/>
	<rdfs:comment>"Amount" means mass per unit area. The construction thickness_of_[X_]snowfall_amount means the accumulated "depth" of snow which fell i.e. the thickness of the layer of snow at its own density. There are corresponding standard names for liquid water equivalent (lwe) thickness.</rdfs:comment>
	<rdfs:label>thickness of large scale snowfall amount</rdfs:label>
	<generalQuantityKind xmlns="http://purl.oclc.org/NET/ssnx/qu/qu#" rdf:resource="http://purl.oclc.org/NET/ssnx/qu/quantity#thickness"/>
	<rdfs:isDefinedBy rdf:resource="http://purl.oclc.org/NET/ssnx/cf/cf-property"/>
</rdf:Description>

<rdf:Description rdf:about="http://purl.oclc.org/NET/ssnx/cf/cf-property#thickness_of_rainfall_amount">
	<rdf:type rdf:resource="http://www.w3.org/2004/02/skos/core#Concept"/>
	<skos:inScheme rdf:resource="http://purl.oclc.org/NET/ssnx/qu/dim#Distance"/>
	<rdfs:comment>"Amount" means mass per unit area. The construction thickness_of_[X_]rainfall_amount means the accumulated "depth" of rainfall i.e. the thickness of a layer of liquid water having the same mass per unit area as the rainfall amount.</rdfs:comment>
	<rdfs:label>thickness of rainfall amount</rdfs:label>
	<generalQuantityKind xmlns="http://purl.oclc.org/NET/ssnx/qu/qu#" rdf:resource="http://purl.oclc.org/NET/ssnx/qu/quantity#thickness"/>
	<rdfs:isDefinedBy rdf:resource="http://purl.oclc.org/NET/ssnx/cf/cf-property"/>
</rdf:Description>

<rdf:Description rdf:about="http://purl.oclc.org/NET/ssnx/cf/cf-property#thickness_of_snowfall_amount">
	<rdf:type rdf:resource="http://www.w3.org/2004/02/skos/core#Concept"/>
	<skos:inScheme rdf:resource="http://purl.oclc.org/NET/ssnx/qu/dim#Distance"/>
	<rdfs:comment>"Amount" means mass per unit area. The construction thickness_of_[X_]snowfall_amount means the accumulated "depth" of snow which fell i.e. the thickness of the layer of snow at its own density. There are corresponding standard names for liquid water equivalent (lwe) thickness.</rdfs:comment>
	<rdfs:label>thickness of snowfall amount</rdfs:label>
	<generalQuantityKind xmlns="http://purl.oclc.org/NET/ssnx/qu/qu#" rdf:resource="http://purl.oclc.org/NET/ssnx/qu/quantity#thickness"/>
	<rdfs:isDefinedBy rdf:resource="http://purl.oclc.org/NET/ssnx/cf/cf-property"/>
</rdf:Description>

<rdf:Description rdf:about="http://purl.oclc.org/NET/ssnx/qu/quantity#distance">
	<skos:inScheme rdf:resource="http://purl.oclc.org/NET/ssnx/qu/dim#Distance"/>
</rdf:Description>

<rdf:Description rdf:about="http://purl.oclc.org/NET/ssnx/qu/quantity#height">
	<skos:inScheme rdf:resource="http://purl.oclc.org/NET/ssnx/qu/dim#Distance"/>
</rdf:Description>

<rdf:Description rdf:about="http://purl.oclc.org/NET/ssnx/qu/quantity#length">
	<skos:inScheme rdf:resource="http://purl.oclc.org/NET/ssnx/qu/dim#Distance"/>
</rdf:Description>

<rdf:Description rdf:about="http://purl.oclc.org/NET/ssnx/qu/quantity#radius">
	<skos:inScheme rdf:resource="http://purl.oclc.org/NET/ssnx/qu/dim#Distance"/>
</rdf:Description>

<rdf:Description rdf:about="http://purl.oclc.org/NET/ssnx/qu/quantity#thickness">
	<skos:inScheme rdf:resource="http://purl.oclc.org/NET/ssnx/qu/dim#Distance"/>
</rdf:Description>

<rdf:Description rdf:about="http://purl.oclc.org/NET/ssnx/cf/cf-property#snow_grain_size">
	<rdf:type rdf:resource="http://www.w3.org/2004/02/skos/core#Concept"/>
	<skos:inScheme rdf:resource="http://purl.oclc.org/NET/ssnx/qu/dim#Distance"/>
	<rdfs:label>snow grain size</rdfs:label>
	<generalQuantityKind xmlns="http://purl.oclc.org/NET/ssnx/qu/qu#" rdf:resource="http://purl.oclc.org/NET/ssnx/qu/quantity#distance"/>
	<rdfs:isDefinedBy rdf:resource="http://purl.oclc.org/NET/ssnx/cf/cf-property"/>
</rdf:Description>

<rdf:Description rdf:about="http://purl.oclc.org/NET/ssnx/cf/cf-property#height_above_sea_floor">
	<rdf:type rdf:resource="http://www.w3.org/2004/02/skos/core#Concept"/>
	<skos:inScheme rdf:resource="http://purl.oclc.org/NET/ssnx/qu/dim#Distance"/>
	<rdfs:label>height above sea floor</rdfs:label>
	<generalQuantityKind xmlns="http://purl.oclc.org/NET/ssnx/qu/qu#" rdf:resource="http://purl.oclc.org/NET/ssnx/qu/quantity#height"/>
	<rdfs:isDefinedBy rdf:resource="http://purl.oclc.org/NET/ssnx/cf/cf-property"/>
</rdf:Description>

<rdf:Description rdf:about="http://purl.oclc.org/NET/ssnx/cf/cf-property#sea_surface_height_above_sea_level">
	<rdf:type rdf:resource="http://www.w3.org/2004/02/skos/core#Concept"/>
	<skos:inScheme rdf:resource="http://purl.oclc.org/NET/ssnx/qu/dim#Distance"/>
	<rdfs:comment>sea_level means mean sea level, which is close to the geoid in sea areas. "Sea surface height" is a time-varying quantity. The standard name for the height of the sea surface above the geoid is sea_surface_height_above_geoid. The standard name for the height of the sea surface above the reference ellipsoid is sea_surface_height_above_reference_ellipsoid.</rdfs:comment>
	<rdfs:label>sea surface height above sea level</rdfs:label>
	<generalQuantityKind xmlns="http://purl.oclc.org/NET/ssnx/qu/qu#" rdf:resource="http://purl.oclc.org/NET/ssnx/qu/quantity#height"/>
	<rdfs:isDefinedBy rdf:resource="http://purl.oclc.org/NET/ssnx/cf/cf-property"/>
</rdf:Description>

<rdf:Description rdf:about="http://purl.oclc.org/NET/ssnx/cf/cf-property#sea_surface_height_amplitude_due_to_earth_tide">
	<rdf:type rdf:resource="http://www.w3.org/2004/02/skos/core#Concept"/>
	<skos:inScheme rdf:resource="http://purl.oclc.org/NET/ssnx/qu/dim#Distance"/>
	<rdfs:comment>The specification of a physical process by the phrase due_to_process means that the quantity named is a single term in a sum of terms which together compose the general quantity named by omitting the phrase. Tides are a significant contributor to the observed sea surface height; earth tide means the solid earth tide.</rdfs:comment>
	<rdfs:label>sea surface height amplitude due to earth tide</rdfs:label>
	<generalQuantityKind xmlns="http://purl.oclc.org/NET/ssnx/qu/qu#" rdf:resource="http://purl.oclc.org/NET/ssnx/qu/quantity#height"/>
	<rdfs:isDefinedBy rdf:resource="http://purl.oclc.org/NET/ssnx/cf/cf-property"/>
</rdf:Description>

<rdf:Description rdf:about="http://purl.oclc.org/NET/ssnx/cf/cf-property#sea_surface_height_amplitude_due_to_equilibrium_ocean_tide">
	<rdf:type rdf:resource="http://www.w3.org/2004/02/skos/core#Concept"/>
	<skos:inScheme rdf:resource="http://purl.oclc.org/NET/ssnx/qu/dim#Distance"/>
	<rdfs:comment>The specification of a physical process by the phrase due_to_process means that the quantity named is a single term in a sum of terms which together compose the general quantity named by omitting the phrase. Tides are a significant contributor to the observed sea surface height; equilibrium ocean tide refers to the long period ocean tide.</rdfs:comment>
	<rdfs:label>sea surface height amplitude due to equilibrium ocean tide</rdfs:label>
	<generalQuantityKind xmlns="http://purl.oclc.org/NET/ssnx/qu/qu#" rdf:resource="http://purl.oclc.org/NET/ssnx/qu/quantity#height"/>
	<rdfs:isDefinedBy rdf:resource="http://purl.oclc.org/NET/ssnx/cf/cf-property"/>
</rdf:Description>

<rdf:Description rdf:about="http://purl.oclc.org/NET/ssnx/cf/cf-property#sea_surface_height_amplitude_due_to_geocentric_ocean_tide">
	<rdf:type rdf:resource="http://www.w3.org/2004/02/skos/core#Concept"/>
	<skos:inScheme rdf:resource="http://purl.oclc.org/NET/ssnx/qu/dim#Distance"/>
	<rdfs:comment>The specification of a physical process by the phrase due_to_process means that the quantity named is a single term in a sum of terms which together compose the general quantity named by omitting the phrase. Tides are a significant contributor to the observed sea surface height; geocentric ocean tide means the sum total of ocean tide and load tide.</rdfs:comment>
	<rdfs:label>sea surface height amplitude due to geocentric ocean tide</rdfs:label>
	<generalQuantityKind xmlns="http://purl.oclc.org/NET/ssnx/qu/qu#" rdf:resource="http://purl.oclc.org/NET/ssnx/qu/quantity#height"/>
	<rdfs:isDefinedBy rdf:resource="http://purl.oclc.org/NET/ssnx/cf/cf-property"/>
</rdf:Description>

<rdf:Description rdf:about="http://purl.oclc.org/NET/ssnx/cf/cf-property#sea_surface_height_amplitude_due_to_non_equilibrium_ocean_tide">
	<rdf:type rdf:resource="http://www.w3.org/2004/02/skos/core#Concept"/>
	<skos:inScheme rdf:resource="http://purl.oclc.org/NET/ssnx/qu/dim#Distance"/>
	<rdfs:comment>The specification of a physical process by the phrase due_to_process means that the quantity named is a single term in a sum of terms which together compose the general quantity named by omitting the phrase. Tides are a significant contributor to the observed sea surface height; non equilibrium ocean tide refers to the long period ocean tide.</rdfs:comment>
	<rdfs:label>sea surface height amplitude due to non equilibrium ocean tide</rdfs:label>
	<generalQuantityKind xmlns="http://purl.oclc.org/NET/ssnx/qu/qu#" rdf:resource="http://purl.oclc.org/NET/ssnx/qu/quantity#height"/>
	<rdfs:isDefinedBy rdf:resource="http://purl.oclc.org/NET/ssnx/cf/cf-property"/>
</rdf:Description>

<rdf:Description rdf:about="http://purl.oclc.org/NET/ssnx/cf/cf-property#sea_surface_height_amplitude_due_to_pole_tide">
	<rdf:type rdf:resource="http://www.w3.org/2004/02/skos/core#Concept"/>
	<skos:inScheme rdf:resource="http://purl.oclc.org/NET/ssnx/qu/dim#Distance"/>
	<rdfs:comment>The specification of a physical process by the phrase due_to_process means that the quantity named is a single term in a sum of terms which together compose the general quantity named by omitting the phrase. Tides are a significant contributor to the observed sea surface height; the pole tide occurs due to variations in the earth's rotation.</rdfs:comment>
	<rdfs:label>sea surface height amplitude due to pole tide</rdfs:label>
	<generalQuantityKind xmlns="http://purl.oclc.org/NET/ssnx/qu/qu#" rdf:resource="http://purl.oclc.org/NET/ssnx/qu/quantity#height"/>
	<rdfs:isDefinedBy rdf:resource="http://purl.oclc.org/NET/ssnx/cf/cf-property"/>
</rdf:Description>

<rdf:Description rdf:about="http://purl.oclc.org/NET/ssnx/cf/cf-property#sea_surface_height_bias_due_to_sea_surface_roughness">
	<rdf:type rdf:resource="http://www.w3.org/2004/02/skos/core#Concept"/>
	<skos:inScheme rdf:resource="http://purl.oclc.org/NET/ssnx/qu/dim#Distance"/>
	<rdfs:comment>The specification of a physical process by the phrase due_to_process means that the quantity named is a single term in a sum of terms which together compose the general quantity named by omitting the phrase.  Altimeter pulses tend to be more strongly refelected by the troughs of sea surface waves than by the crests leading to a bias in the measured sea surface height. This quantity is commonly known as "sea state bias".</rdfs:comment>
	<rdfs:label>sea surface height bias due to sea surface roughness</rdfs:label>
	<generalQuantityKind xmlns="http://purl.oclc.org/NET/ssnx/qu/qu#" rdf:resource="http://purl.oclc.org/NET/ssnx/qu/quantity#height"/>
	<rdfs:isDefinedBy rdf:resource="http://purl.oclc.org/NET/ssnx/cf/cf-property"/>
</rdf:Description>

<rdf:Description rdf:about="http://purl.oclc.org/NET/ssnx/cf/cf-property#sea_surface_height_correction_due_to_air_pressure_and_wind_at_high_frequency">
	<rdf:type rdf:resource="http://www.w3.org/2004/02/skos/core#Concept"/>
	<skos:inScheme rdf:resource="http://purl.oclc.org/NET/ssnx/qu/dim#Distance"/>
	<rdfs:comment>The specification of a physical process by the phrase due_to_process means that the quantity named is a single term in a sum of terms which together compose the general quantity named by omitting the phrase. "Air pressure and wind at high frequency" means variations in air pressure with periods shorter  than 20 days. These give rise to corresponding variations in sea surface topography. The quantity sea_surface_height_correction_due_to_air_pressure_and_wind_at_high_frequency  should be applied by adding it to the quantity with standard name altimeter_range.  Additional altimeter range corrections are given by the quantities with standard names altimeter_range_correction_due_to_wet_troposphere, altimeter_range_correction_due_to_dry_troposphere, altimeter_range_correction_due_to_ionosphere and sea_surface_height_correction_due_to_air_pressure_at_low_frequency.</rdfs:comment>
	<rdfs:label>sea surface height correction due to air pressure and wind at high frequency</rdfs:label>
	<generalQuantityKind xmlns="http://purl.oclc.org/NET/ssnx/qu/qu#" rdf:resource="http://purl.oclc.org/NET/ssnx/qu/quantity#height"/>
	<rdfs:isDefinedBy rdf:resource="http://purl.oclc.org/NET/ssnx/cf/cf-property"/>
</rdf:Description>

<rdf:Description rdf:about="http://purl.oclc.org/NET/ssnx/cf/cf-property#sea_surface_height_correction_due_to_air_pressure_at_low_frequency">
	<rdf:type rdf:resource="http://www.w3.org/2004/02/skos/core#Concept"/>
	<skos:inScheme rdf:resource="http://purl.oclc.org/NET/ssnx/qu/dim#Distance"/>
	<rdfs:comment>The specification of a physical process by the phrase due_to_process means that the quantity named is a single term in a sum of terms which together compose the general quantity named by omitting the phrase. "Air pressure at low frequency" means variations in air pressure with periods longer than 20 days. These give rise to corresponding variations in sea surface topography. The quantity sea_surface_height_correction_due_to_air_pressure_at_low_frequency is commonly called the "inverted barometer effect" and the correction should be applied by adding it to the quantity with standard name altimeter_range.  Additional altimeter range corrections are given by the quantities with standard names altimeter_range_correction_due_to_wet_troposphere, altimeter_range_correction_due_to_dry_troposphere, altimeter_range_correction_due_to_ionosphere and sea_surface_height_correction_due_to_air_pressure_and_wind_at_high_frequency.</rdfs:comment>
	<rdfs:label>sea surface height correction due to air pressure at low frequency</rdfs:label>
	<generalQuantityKind xmlns="http://purl.oclc.org/NET/ssnx/qu/qu#" rdf:resource="http://purl.oclc.org/NET/ssnx/qu/quantity#height"/>
	<rdfs:isDefinedBy rdf:resource="http://purl.oclc.org/NET/ssnx/cf/cf-property"/>
</rdf:Description>

<rdf:Description rdf:about="http://purl.oclc.org/NET/ssnx/cf/cf-property#sea_surface_swell_wave_significant_height">
	<rdf:type rdf:resource="http://www.w3.org/2004/02/skos/core#Concept"/>
	<skos:inScheme rdf:resource="http://purl.oclc.org/NET/ssnx/qu/dim#Distance"/>
	<rdfs:comment>Height is the vertical distance above the surface. Swell waves are waves on the ocean surface.</rdfs:comment>
	<rdfs:label>sea surface swell wave significant height</rdfs:label>
	<generalQuantityKind xmlns="http://purl.oclc.org/NET/ssnx/qu/qu#" rdf:resource="http://purl.oclc.org/NET/ssnx/qu/quantity#height"/>
	<rdfs:isDefinedBy rdf:resource="http://purl.oclc.org/NET/ssnx/cf/cf-property"/>
</rdf:Description>

<rdf:Description rdf:about="http://purl.oclc.org/NET/ssnx/cf/cf-property#sea_surface_wave_significant_height">
	<rdf:type rdf:resource="http://www.w3.org/2004/02/skos/core#Concept"/>
	<skos:inScheme rdf:resource="http://purl.oclc.org/NET/ssnx/qu/dim#Distance"/>
	<rdfs:comment>Height is the vertical distance above the surface.</rdfs:comment>
	<rdfs:label>sea surface wave significant height</rdfs:label>
	<generalQuantityKind xmlns="http://purl.oclc.org/NET/ssnx/qu/qu#" rdf:resource="http://purl.oclc.org/NET/ssnx/qu/quantity#height"/>
	<rdfs:isDefinedBy rdf:resource="http://purl.oclc.org/NET/ssnx/cf/cf-property"/>
</rdf:Description>

<rdf:Description rdf:about="http://purl.oclc.org/NET/ssnx/cf/cf-property#sea_surface_wind_wave_significant_height">
	<rdf:type rdf:resource="http://www.w3.org/2004/02/skos/core#Concept"/>
	<skos:inScheme rdf:resource="http://purl.oclc.org/NET/ssnx/qu/dim#Distance"/>
	<rdfs:comment>Height is the vertical distance above the surface. Wind waves are waves on the ocean surface. Wind is defined as a two-dimensional (horizontal) air velocity vector, with no vertical component. (Vertical motion in the atmosphere has the standard name upward_air_velocity.)</rdfs:comment>
	<rdfs:label>sea surface wind wave significant height</rdfs:label>
	<generalQuantityKind xmlns="http://purl.oclc.org/NET/ssnx/qu/qu#" rdf:resource="http://purl.oclc.org/NET/ssnx/qu/quantity#height"/>
	<rdfs:isDefinedBy rdf:resource="http://purl.oclc.org/NET/ssnx/cf/cf-property"/>
</rdf:Description>

<rdf:Description rdf:about="http://purl.oclc.org/NET/ssnx/cf/cf-property#sea_ice_thickness">
	<rdf:type rdf:resource="http://www.w3.org/2004/02/skos/core#Concept"/>
	<skos:inScheme rdf:resource="http://purl.oclc.org/NET/ssnx/qu/dim#Distance"/>
	<rdfs:label>sea ice thickness</rdfs:label>
	<generalQuantityKind xmlns="http://purl.oclc.org/NET/ssnx/qu/qu#" rdf:resource="http://purl.oclc.org/NET/ssnx/qu/quantity#thickness"/>
	<rdfs:isDefinedBy rdf:resource="http://purl.oclc.org/NET/ssnx/cf/cf-property"/>
</rdf:Description>

<rdf:Description rdf:about="http://purl.oclc.org/NET/ssnx/cf/cf-property#altimeter_range">
	<rdf:type rdf:resource="http://www.w3.org/2004/02/skos/core#Concept"/>
	<skos:inScheme rdf:resource="http://purl.oclc.org/NET/ssnx/qu/dim#Distance"/>
	<rdfs:comment>An altimeter operates by sending out a short pulse of radiation and measuring the time required for the pulse to return from the sea surface; this measurement is used to calculate the distance between the instrument and the sea surface.  That measurement is called the "altimeter range" and does not include any range corrections.</rdfs:comment>
	<rdfs:label>altimeter range</rdfs:label>
	<generalQuantityKind xmlns="http://purl.oclc.org/NET/ssnx/qu/qu#" rdf:resource="http://purl.oclc.org/NET/ssnx/qu/quantity#distance"/>
	<rdfs:isDefinedBy rdf:resource="http://purl.oclc.org/NET/ssnx/cf/cf-property"/>
</rdf:Description>

<rdf:Description rdf:about="http://purl.oclc.org/NET/ssnx/cf/cf-property#altimeter_range_correction_due_to_dry_troposphere">
	<rdf:type rdf:resource="http://www.w3.org/2004/02/skos/core#Concept"/>
	<skos:inScheme rdf:resource="http://purl.oclc.org/NET/ssnx/qu/dim#Distance"/>
	<rdfs:comment>The specification of a physical process by the phrase due_to_process means that the quantity named is a single term in a sum of terms which together compose the general quantity named by omitting the phrase.   To apply the altimeter range correction it must be added to the quantity with standard name altimeter_range.  "Correction_due_to_dry_troposphere" means a correction for dry gases in the troposphere, i.e. excluding the effect of liquid water.  Additional altimeter range corrections are given by the quantities with standard names altimeter_range_correction_due_to_wet_troposphere, altimeter_range_correction_due_to_ionosphere, sea_surface_height_correction_due_to_air_pressure_at_low_frequency and sea_surface_height_correction_due_to_air_pressure_and_wind_at_high_frequency.</rdfs:comment>
	<rdfs:label>altimeter range correction due to dry troposphere</rdfs:label>
	<generalQuantityKind xmlns="http://purl.oclc.org/NET/ssnx/qu/qu#" rdf:resource="http://purl.oclc.org/NET/ssnx/qu/quantity#distance"/>
	<rdfs:isDefinedBy rdf:resource="http://purl.oclc.org/NET/ssnx/cf/cf-property"/>
</rdf:Description>

<rdf:Description rdf:about="http://purl.oclc.org/NET/ssnx/cf/cf-property#altimeter_range_correction_due_to_ionosphere">
	<rdf:type rdf:resource="http://www.w3.org/2004/02/skos/core#Concept"/>
	<skos:inScheme rdf:resource="http://purl.oclc.org/NET/ssnx/qu/dim#Distance"/>
	<rdfs:comment>The specification of a physical process by the phrase due_to_process means that the quantity named is a single term in a sum of terms which together compose the general quantity named by omitting the phrase.   To apply the altimeter range correction it must be added to the quantity with standard name altimeter_range.  "Correction_due_to_ionosphere" means a correction for the atmosphere's electron content in the ionosphere. Additional altimeter range corrections are given by the quantities with standard names altimeter_range_correction_due_to_wet_troposphere, altimeter_range_correction_due_to_dry_troposphere, sea_surface_height_correction_due_to_air_pressure_at_low_frequency and sea_surface_height_correction_due_to_air_pressure_and_wind_at_high_frequency.</rdfs:comment>
	<rdfs:label>altimeter range correction due to ionosphere</rdfs:label>
	<generalQuantityKind xmlns="http://purl.oclc.org/NET/ssnx/qu/qu#" rdf:resource="http://purl.oclc.org/NET/ssnx/qu/quantity#distance"/>
	<rdfs:isDefinedBy rdf:resource="http://purl.oclc.org/NET/ssnx/cf/cf-property"/>
</rdf:Description>

<rdf:Description rdf:about="http://purl.oclc.org/NET/ssnx/cf/cf-property#altimeter_range_correction_due_to_wet_troposphere">
	<rdf:type rdf:resource="http://www.w3.org/2004/02/skos/core#Concept"/>
	<skos:inScheme rdf:resource="http://purl.oclc.org/NET/ssnx/qu/dim#Distance"/>
	<rdfs:comment>The specification of a physical process by the phrase due_to_process means that the quantity named is a single term in a sum of terms which together compose the general quantity named by omitting the phrase.   To apply the altimeter range correction it must be added to the quantity with standard name altimeter_range.  "Correction_due_to_wet_troposphere" means a correction for the effect of liquid water in the troposphere.  Additional altimeter range corrections are given by the quantities with standard names altimeter_range_correction_due_to_dry_troposphere, altimeter_range_correction_due_to_ionosphere, sea_surface_height_correction_due_to_air_pressure_at_low_frequency and sea_surface_height_correction_due_to_air_pressure_and_wind_at_high_frequency.</rdfs:comment>
	<rdfs:label>altimeter range correction due to wet troposphere</rdfs:label>
	<generalQuantityKind xmlns="http://purl.oclc.org/NET/ssnx/qu/qu#" rdf:resource="http://purl.oclc.org/NET/ssnx/qu/quantity#distance"/>
	<rdfs:isDefinedBy rdf:resource="http://purl.oclc.org/NET/ssnx/cf/cf-property"/>
</rdf:Description>

<rdf:Description rdf:about="http://purl.oclc.org/NET/ssnx/cf/cf-property#altitude">
	<rdf:type rdf:resource="http://www.w3.org/2004/02/skos/core#Concept"/>
	<skos:inScheme rdf:resource="http://purl.oclc.org/NET/ssnx/qu/dim#Distance"/>
	<rdfs:comment>Altitude is the (geometric) height above the geoid, which is the reference geopotential surface. The geoid is similar to mean sea level.</rdfs:comment>
	<rdfs:label>altitude</rdfs:label>
	<generalQuantityKind xmlns="http://purl.oclc.org/NET/ssnx/qu/qu#" rdf:resource="http://purl.oclc.org/NET/ssnx/qu/quantity#distance"/>
	<rdfs:isDefinedBy rdf:resource="http://purl.oclc.org/NET/ssnx/cf/cf-property"/>
</rdf:Description>

<rdf:Description rdf:about="http://purl.oclc.org/NET/ssnx/cf/cf-property#altitude_at_top_of_dry_convection">
	<rdf:type rdf:resource="http://www.w3.org/2004/02/skos/core#Concept"/>
	<skos:inScheme rdf:resource="http://purl.oclc.org/NET/ssnx/qu/dim#Distance"/>
	<rdfs:comment>Altitude is the (geometric) height above the geoid, which is the reference geopotential surface. The geoid is similar to mean sea level.</rdfs:comment>
	<rdfs:label>altitude at top of dry convection</rdfs:label>
	<generalQuantityKind xmlns="http://purl.oclc.org/NET/ssnx/qu/qu#" rdf:resource="http://purl.oclc.org/NET/ssnx/qu/quantity#distance"/>
	<rdfs:isDefinedBy rdf:resource="http://purl.oclc.org/NET/ssnx/cf/cf-property"/>
</rdf:Description>

<rdf:Description rdf:about="http://purl.oclc.org/NET/ssnx/cf/cf-property#bedrock_altitude">
	<rdf:type rdf:resource="http://www.w3.org/2004/02/skos/core#Concept"/>
	<skos:inScheme rdf:resource="http://purl.oclc.org/NET/ssnx/qu/dim#Distance"/>
	<rdfs:comment>Altitude is the (geometric) height above the geoid, which is the reference geopotential surface. The geoid is similar to mean sea level. "Bedrock" is the solid Earth surface beneath land ice or ocean water.</rdfs:comment>
	<rdfs:label>bedrock altitude</rdfs:label>
	<generalQuantityKind xmlns="http://purl.oclc.org/NET/ssnx/qu/qu#" rdf:resource="http://purl.oclc.org/NET/ssnx/qu/quantity#distance"/>
	<rdfs:isDefinedBy rdf:resource="http://purl.oclc.org/NET/ssnx/cf/cf-property"/>
</rdf:Description>

<rdf:Description rdf:about="http://purl.oclc.org/NET/ssnx/cf/cf-property#bedrock_altitude_change_due_to_isostatic_adjustment">
	<rdf:type rdf:resource="http://www.w3.org/2004/02/skos/core#Concept"/>
	<skos:inScheme rdf:resource="http://purl.oclc.org/NET/ssnx/qu/dim#Distance"/>
	<rdfs:comment>The specification of a physical process by the phrase due_to_process means that the quantity named is a single term in a sum of terms which together compose the general quantity named by omitting the phrase. Altitude is the (geometric) height above the geoid, which is the reference geopotential surface. The geoid is similar to mean sea level. "Bedrock" is the solid Earth surface beneath land ice or ocean water. The zero of bedrock altitude change is arbitrary. Isostatic adjustment is the vertical movement of the lithosphere due to changing surface ice and water loads.</rdfs:comment>
	<rdfs:label>bedrock altitude change due to isostatic adjustment</rdfs:label>
	<generalQuantityKind xmlns="http://purl.oclc.org/NET/ssnx/qu/qu#" rdf:resource="http://purl.oclc.org/NET/ssnx/qu/quantity#distance"/>
	<rdfs:isDefinedBy rdf:resource="http://purl.oclc.org/NET/ssnx/cf/cf-property"/>
</rdf:Description>

<rdf:Description rdf:about="http://purl.oclc.org/NET/ssnx/cf/cf-property#cloud_base_altitude">
	<rdf:type rdf:resource="http://www.w3.org/2004/02/skos/core#Concept"/>
	<skos:inScheme rdf:resource="http://purl.oclc.org/NET/ssnx/qu/dim#Distance"/>
	<rdfs:comment>cloud_base refers to the base of the lowest cloud. Altitude is the (geometric) height above the geoid, which is the reference geopotential surface. The geoid is similar to mean sea level.</rdfs:comment>
	<rdfs:label>cloud base altitude</rdfs:label>
	<generalQuantityKind xmlns="http://purl.oclc.org/NET/ssnx/qu/qu#" rdf:resource="http://purl.oclc.org/NET/ssnx/qu/quantity#distance"/>
	<rdfs:isDefinedBy rdf:resource="http://purl.oclc.org/NET/ssnx/cf/cf-property"/>
</rdf:Description>

<rdf:Description rdf:about="http://purl.oclc.org/NET/ssnx/cf/cf-property#cloud_top_altitude">
	<rdf:type rdf:resource="http://www.w3.org/2004/02/skos/core#Concept"/>
	<skos:inScheme rdf:resource="http://purl.oclc.org/NET/ssnx/qu/dim#Distance"/>
	<rdfs:comment>cloud_top refers to the top of the highest cloud. Altitude is the (geometric) height above the geoid, which is the reference geopotential surface. The geoid is similar to mean sea level.</rdfs:comment>
	<rdfs:label>cloud top altitude</rdfs:label>
	<generalQuantityKind xmlns="http://purl.oclc.org/NET/ssnx/qu/qu#" rdf:resource="http://purl.oclc.org/NET/ssnx/qu/quantity#distance"/>
	<rdfs:isDefinedBy rdf:resource="http://purl.oclc.org/NET/ssnx/cf/cf-property"/>
</rdf:Description>

</rdf:RDF>