<?xml version="1.0" encoding="UTF-8"?>
<rdf:RDF
	xmlns:vann="http://purl.org/vocab/vann/"
	xmlns:voaf="http://purl.org/vocommons/voaf#"
	xmlns:rdfs="http://www.w3.org/2000/01/rdf-schema#"
	xmlns:owl="http://www.w3.org/2002/07/owl#"
	xmlns:skos="http://www.w3.org/2004/02/skos/core#"
	xmlns:rdf="http://www.w3.org/1999/02/22-rdf-syntax-ns#"
	xmlns:dcterms="http://purl.org/dc/terms/"
	xmlns:dc="http://purl.org/dc/elements/1.1/"
	xmlns:dcmit="http://purl.org/dc/dcmitype/"
	xmlns:sesame="http://www.openrdf.org/schema/sesame#"
	xmlns:xsd="http://www.w3.org/2001/XMLSchema#"
	xmlns:fn="http://www.w3.org/2005/xpath-functions#"
	xmlns:foaf="http://xmlns.com/foaf/0.1/"
	xmlns:hint="http://www.bigdata.com/queryHints#"
	xmlns:bd="http://www.bigdata.com/rdf#"
	xmlns:bds="http://www.bigdata.com/rdf/search#">

<rdf:Description rdf:about="http://www.ebusiness-unibw.org/ontologies/consumerelectronics/v1">
	<rdf:type rdf:resource="http://www.w3.org/2002/07/owl#Ontology"/>
</rdf:Description>

<rdf:Description rdf:about="http://www.ebusiness-unibw.org/ontologies/consumerelectronics/v1#ComputerDisplayResolution">
	<rdf:type rdf:resource="http://www.w3.org/2004/02/skos/core#ConceptScheme"/>
</rdf:Description>

<rdf:Description rdf:about="http://www.ebusiness-unibw.org/ontologies/consumerelectronics/v1#ComputerDisplayResolution_1024x768_60_70_75_85Hz">
	<rdf:type rdf:resource="http://www.w3.org/2004/02/skos/core#Concept"/>
	<skos:inScheme rdf:resource="http://www.ebusiness-unibw.org/ontologies/consumerelectronics/v1#ComputerDisplayResolution"/>
</rdf:Description>

<rdf:Description rdf:about="http://www.ebusiness-unibw.org/ontologies/consumerelectronics/v1#ComputerDisplayResolution">
	<rdfs:comment xml:lang="en">The display resolution of a computer display typically refers to the number of distinct pixels in each dimension that can be displayed.

(This description is partly based on or reuses content from the Wikipedia article "Display resolution" (http://en.wikipedia.org/wiki/Display_resolution) and is licensed under the GNU Free Documentation License (http://www.gnu.org/copyleft/fdl.html).)</rdfs:comment>
	<rdfs:label xml:lang="en">Computer display resolution</rdfs:label>
</rdf:Description>

<rdf:Description rdf:about="http://www.ebusiness-unibw.org/ontologies/consumerelectronics/v1#ComputerDisplayResolution_1024x768_60_70_75_85Hz">
	<rdfs:comment xml:lang="en">Display resolution specified as the width and height in pixels, color depth measured in bits, and refresh rate expressed in hertz; here Extended Graphics Array.

(This description is partly based on or reuses content from the Wikipedia article "Display resolution" (http://en.wikipedia.org/wiki/Display_resolution) and is licensed under the GNU Free Documentation License (http://www.gnu.org/copyleft/fdl.html).)</rdfs:comment>
	<rdfs:label xml:lang="en">Computer display resolution 1024x768 60 70 75 85Hz</rdfs:label>
</rdf:Description>

<rdf:Description rdf:about="http://www.ebusiness-unibw.org/ontologies/consumerelectronics/v1#ComputerDisplayResolution">
	<rdfs:isDefinedBy rdf:resource="http://www.ebusiness-unibw.org/ontologies/consumerelectronics/v1"/>
</rdf:Description>

<rdf:Description rdf:about="http://www.ebusiness-unibw.org/ontologies/consumerelectronics/v1#ComputerDisplayResolution_1024x768_60_70_75_85Hz">
	<rdfs:isDefinedBy rdf:resource="http://www.ebusiness-unibw.org/ontologies/consumerelectronics/v1"/>
</rdf:Description>

<rdf:Description rdf:about="http://www.ebusiness-unibw.org/ontologies/consumerelectronics/v1#ComputerDisplayResolution_640x480_60_72_75_85Hz">
	<rdf:type rdf:resource="http://www.w3.org/2004/02/skos/core#Concept"/>
	<skos:inScheme rdf:resource="http://www.ebusiness-unibw.org/ontologies/consumerelectronics/v1#ComputerDisplayResolution"/>
	<rdfs:comment xml:lang="en">Display resolution specified as the width and height in pixels, color depth measured in bits, and refresh rate expressed in hertz; here Video Graphics Array.

(This description is partly based on or reuses content from the Wikipedia article "Display resolution" (http://en.wikipedia.org/wiki/Display_resolution) and is licensed under the GNU Free Documentation License (http://www.gnu.org/copyleft/fdl.html).)</rdfs:comment>
	<rdfs:label xml:lang="en">Computer display resolution 640x480 60 72 75 85Hz</rdfs:label>
	<rdfs:isDefinedBy rdf:resource="http://www.ebusiness-unibw.org/ontologies/consumerelectronics/v1"/>
</rdf:Description>

<rdf:Description rdf:about="http://www.ebusiness-unibw.org/ontologies/consumerelectronics/v1#ComputerDisplayResolution_800x600_60_72_75_85Hz">
	<rdf:type rdf:resource="http://www.w3.org/2004/02/skos/core#Concept"/>
	<skos:inScheme rdf:resource="http://www.ebusiness-unibw.org/ontologies/consumerelectronics/v1#ComputerDisplayResolution"/>
	<rdfs:comment xml:lang="en">Display resolution specified as the width and height in pixels, color depth measured in bits, and refresh rate expressed in hertz; here Super Video Graphics Array.

(This description is partly based on or reuses content from the Wikipedia article "Display resolution" (http://en.wikipedia.org/wiki/Display_resolution) and is licensed under the GNU Free Documentation License (http://www.gnu.org/copyleft/fdl.html).)</rdfs:comment>
	<rdfs:label xml:lang="en">Computer display resolution 800x600 60 72 75 85Hz</rdfs:label>
	<rdfs:isDefinedBy rdf:resource="http://www.ebusiness-unibw.org/ontologies/consumerelectronics/v1"/>
</rdf:Description>

</rdf:RDF>