<?xml version="1.0" encoding="UTF-8"?>
<rdf:RDF
	xmlns:vann="http://purl.org/vocab/vann/"
	xmlns:voaf="http://purl.org/vocommons/voaf#"
	xmlns:rdfs="http://www.w3.org/2000/01/rdf-schema#"
	xmlns:owl="http://www.w3.org/2002/07/owl#"
	xmlns:skos="http://www.w3.org/2004/02/skos/core#"
	xmlns:rdf="http://www.w3.org/1999/02/22-rdf-syntax-ns#"
	xmlns:dcterms="http://purl.org/dc/terms/"
	xmlns:dc="http://purl.org/dc/elements/1.1/"
	xmlns:dcmit="http://purl.org/dc/dcmitype/"
	xmlns:sesame="http://www.openrdf.org/schema/sesame#"
	xmlns:xsd="http://www.w3.org/2001/XMLSchema#"
	xmlns:fn="http://www.w3.org/2005/xpath-functions#"
	xmlns:foaf="http://xmlns.com/foaf/0.1/"
	xmlns:hint="http://www.bigdata.com/queryHints#"
	xmlns:bd="http://www.bigdata.com/rdf#"
	xmlns:bds="http://www.bigdata.com/rdf/search#">

<rdf:Description rdf:about="http://sparql.sstu.ru:3030/speciality/">
	<rdf:type rdf:resource="http://www.w3.org/2002/07/owl#Ontology"/>
</rdf:Description>

<rdf:Description rdf:about="http://sparql.sstu.ru:3030/speciality/TheList">
	<rdf:type rdf:resource="http://www.w3.org/2004/02/skos/core#ConceptScheme"/>
</rdf:Description>

<rdf:Description rdf:about="http://sparql.sstu.ru:3030/speciality/lists/1">
	<rdf:type rdf:resource="http://www.w3.org/2004/02/skos/core#Concept"/>
	<skos:inScheme rdf:resource="http://sparql.sstu.ru:3030/speciality/TheList"/>
</rdf:Description>

<rdf:Description rdf:about="http://sparql.sstu.ru:3030/speciality/TheList">
	<rdfs:comment>Перечень – именованная совокупность специальностей и УГСН, содержащие эти специальности. Перечень имеет название, дату введения и каким утвержден документом.</rdfs:comment>
</rdf:Description>

<rdf:Description rdf:about="http://sparql.sstu.ru:3030/speciality/lists/1">
	<rdfs:label>ОКСО</rdfs:label>
</rdf:Description>

<rdf:Description rdf:about="http://sparql.sstu.ru:3030/speciality/isPartOfList">
	<rdfs:range rdf:resource="http://sparql.sstu.ru:3030/speciality/TheList"/>
	<rdfs:domain rdf:resource="http://sparql.sstu.ru:3030/speciality/UGSN"/>
	<rdfs:comment>свойство, показывающее, что определенная УГСН входит в определенный перечень</rdfs:comment>
	<rdf:type rdf:resource="http://www.w3.org/2002/07/owl#ObjectProperty"/>
</rdf:Description>

<rdf:Description rdf:about="http://sparql.sstu.ru:3030/speciality/TheList">
	<rdfs:isDefinedBy rdf:resource="http://sparql.sstu.ru:3030/speciality/"/>
</rdf:Description>

<rdf:Description rdf:about="http://sparql.sstu.ru:3030/speciality/lists/1">
	<rdfs:isDefinedBy rdf:resource="http://sparql.sstu.ru:3030/speciality/"/>
</rdf:Description>

<rdf:Description rdf:about="http://sparql.sstu.ru:3030/speciality/TheList">
	<rdfs:comment xml:lang="en">List - named set of specialties (Speciality) and UGSN (UGSN), containing these specialty. The list has the name, the date of administration, and how the document was approved.</rdfs:comment>
</rdf:Description>

<rdf:Description rdf:about="http://sparql.sstu.ru:3030/speciality/lists/2">
	<rdf:type rdf:resource="http://www.w3.org/2004/02/skos/core#Concept"/>
	<skos:inScheme rdf:resource="http://sparql.sstu.ru:3030/speciality/TheList"/>
	<rdfs:label>Перечни 1136, 337</rdfs:label>
	<rdfs:isDefinedBy rdf:resource="http://sparql.sstu.ru:3030/speciality/"/>
</rdf:Description>

<rdf:Description rdf:about="http://sparql.sstu.ru:3030/speciality/lists/3">
	<rdf:type rdf:resource="http://www.w3.org/2004/02/skos/core#Concept"/>
	<skos:inScheme rdf:resource="http://sparql.sstu.ru:3030/speciality/TheList"/>
	<rdfs:label>Перечень 1061</rdfs:label>
	<rdfs:isDefinedBy rdf:resource="http://sparql.sstu.ru:3030/speciality/"/>
</rdf:Description>

<rdf:Description rdf:about="http://sparql.sstu.ru:3030/speciality/isPartOfList">
	<rdfs:comment xml:lang="en">Property indicating that a certain UGSN (UGSN) included in a certain list (TheList)</rdfs:comment>
</rdf:Description>

</rdf:RDF>