<?xml version="1.0" encoding="UTF-8"?>
<rdf:RDF
	xmlns:vann="http://purl.org/vocab/vann/"
	xmlns:voaf="http://purl.org/vocommons/voaf#"
	xmlns:rdfs="http://www.w3.org/2000/01/rdf-schema#"
	xmlns:owl="http://www.w3.org/2002/07/owl#"
	xmlns:skos="http://www.w3.org/2004/02/skos/core#"
	xmlns:rdf="http://www.w3.org/1999/02/22-rdf-syntax-ns#"
	xmlns:dcterms="http://purl.org/dc/terms/"
	xmlns:dc="http://purl.org/dc/elements/1.1/"
	xmlns:dcmit="http://purl.org/dc/dcmitype/"
	xmlns:sesame="http://www.openrdf.org/schema/sesame#"
	xmlns:xsd="http://www.w3.org/2001/XMLSchema#"
	xmlns:fn="http://www.w3.org/2005/xpath-functions#"
	xmlns:foaf="http://xmlns.com/foaf/0.1/"
	xmlns:hint="http://www.bigdata.com/queryHints#"
	xmlns:bd="http://www.bigdata.com/rdf#"
	xmlns:bds="http://www.bigdata.com/rdf/search#">

<rdf:Description rdf:about="http://www.ebusiness-unibw.org/ontologies/consumerelectronics/v1">
	<rdf:type rdf:resource="http://www.w3.org/2002/07/owl#Ontology"/>
</rdf:Description>

<rdf:Description rdf:about="http://www.ebusiness-unibw.org/ontologies/consumerelectronics/v1#DataFormatVideo">
	<rdf:type rdf:resource="http://www.w3.org/2004/02/skos/core#ConceptScheme"/>
</rdf:Description>

<rdf:Description rdf:about="http://www.ebusiness-unibw.org/ontologies/consumerelectronics/v1#AVCH">
	<rdf:type rdf:resource="http://www.w3.org/2004/02/skos/core#Concept"/>
	<skos:inScheme rdf:resource="http://www.ebusiness-unibw.org/ontologies/consumerelectronics/v1#DataFormatVideo"/>
</rdf:Description>

<rdf:Description rdf:about="http://www.ebusiness-unibw.org/ontologies/consumerelectronics/v1#DataFormatVideo">
	<rdfs:comment xml:lang="en">A data format is a particular way to encode information for storage in a computer file (refers to video data).

(This description is partly based on or reuses content from the Wikipedia article "File Format" (http://en.wikipedia.org/wiki/File_format) and is licensed under the GNU Free Documentation License (http://www.gnu.org/copyleft/fdl.html).)</rdfs:comment>
	<rdfs:label xml:lang="en">Data Format Video</rdfs:label>
</rdf:Description>

<rdf:Description rdf:about="http://www.ebusiness-unibw.org/ontologies/consumerelectronics/v1#AVCH">
	<rdfs:comment xml:lang="en">A high-definition and standard-definition recording format for use in digital tapeless camcorders. The format is comparable to other handheld video camera recording formats, particularly HDV and TOD.

(This description is partly based on or reuses content from the Wikipedia article "HDV" (http://en.wikipedia.org/wiki/HDV) and is licensed under the GNU Free Documentation License (http://www.gnu.org/copyleft/fdl.html).)</rdfs:comment>
	<rdfs:label xml:lang="en">AVCH</rdfs:label>
</rdf:Description>

<rdf:Description rdf:about="http://www.ebusiness-unibw.org/ontologies/consumerelectronics/v1#DataFormatVideo">
	<rdfs:isDefinedBy rdf:resource="http://www.ebusiness-unibw.org/ontologies/consumerelectronics/v1"/>
</rdf:Description>

<rdf:Description rdf:about="http://www.ebusiness-unibw.org/ontologies/consumerelectronics/v1#AVCH">
	<rdfs:isDefinedBy rdf:resource="http://www.ebusiness-unibw.org/ontologies/consumerelectronics/v1"/>
</rdf:Description>

<rdf:Description rdf:about="http://www.ebusiness-unibw.org/ontologies/consumerelectronics/v1#AVI">
	<rdf:type rdf:resource="http://www.w3.org/2004/02/skos/core#Concept"/>
	<skos:inScheme rdf:resource="http://www.ebusiness-unibw.org/ontologies/consumerelectronics/v1#DataFormatVideo"/>
	<rdfs:comment xml:lang="en">A multimedia container format introduced by Microsoft.</rdfs:comment>
	<rdfs:label xml:lang="en">AVI</rdfs:label>
	<rdfs:isDefinedBy rdf:resource="http://www.ebusiness-unibw.org/ontologies/consumerelectronics/v1"/>
	<rdfs:label rdf:datatype="http://www.w3.org/2001/XMLSchema#string">AVI</rdfs:label>
</rdf:Description>

<rdf:Description rdf:about="http://www.ebusiness-unibw.org/ontologies/consumerelectronics/v1#DV">
	<rdf:type rdf:resource="http://www.w3.org/2004/02/skos/core#Concept"/>
	<skos:inScheme rdf:resource="http://www.ebusiness-unibw.org/ontologies/consumerelectronics/v1#DataFormatVideo"/>
	<rdfs:comment xml:lang="en">Digital Video (DV) is a digital video format created by Sony, JVC, Panasonic and other video camera producers, and launched in 1995. The DV specification (originally known as the Blue Book, current official name IEC 61834) defines both the codec and the tape format.

(This description is partly based on or reuses content from the Wikipedia article "DV" (http://en.wikipedia.org/wiki/DV) and is licensed under the GNU Free Documentation License (http://www.gnu.org/copyleft/fdl.html).)</rdfs:comment>
	<rdfs:label xml:lang="en">DV</rdfs:label>
	<rdfs:isDefinedBy rdf:resource="http://www.ebusiness-unibw.org/ontologies/consumerelectronics/v1"/>
</rdf:Description>

<rdf:Description rdf:about="http://www.ebusiness-unibw.org/ontologies/consumerelectronics/v1#H.264">
	<rdf:type rdf:resource="http://www.w3.org/2004/02/skos/core#Concept"/>
	<skos:inScheme rdf:resource="http://www.ebusiness-unibw.org/ontologies/consumerelectronics/v1#DataFormatVideo"/>
	<rdfs:comment xml:lang="en">H.264 is a standard for video compression, and is equivalent to MPEG-4 Part 10, or MPEG-4 AVC (for Advanced Video Coding). As of 2008, it is the latest block-oriented motion-compensation-based codec standard developed by the ITU-T Video Coding Experts Group (VCEG) together with the ISO/IEC Moving Picture Experts Group (MPEG), and it was the product of a partnership effort known as the Joint Video Team (JVT).

(This description is partly based on or reuses content from the Wikipedia article "H.264" (http://en.wikipedia.org/wiki/H.264) and is licensed under the GNU Free Documentation License (http://www.gnu.org/copyleft/fdl.html).)</rdfs:comment>
	<rdfs:label xml:lang="en">H.264</rdfs:label>
	<rdfs:isDefinedBy rdf:resource="http://www.ebusiness-unibw.org/ontologies/consumerelectronics/v1"/>
</rdf:Description>

<rdf:Description rdf:about="http://www.ebusiness-unibw.org/ontologies/consumerelectronics/v1#MOV">
	<rdf:type rdf:resource="http://www.w3.org/2004/02/skos/core#Concept"/>
	<skos:inScheme rdf:resource="http://www.ebusiness-unibw.org/ontologies/consumerelectronics/v1#DataFormatVideo"/>
	<rdfs:comment xml:lang="en">The QuickTime (.mov) file format functions as a multimedia container file that contains one or more tracks, each of which stores a particular type of data: audio, video, effects, or text (e.g. for subtitles).

(This description is partly based on or reuses content from the Wikipedia article "QuickTime" (http://en.wikipedia.org/wiki/QuickTime) and is licensed under the GNU Free Documentation License (http://www.gnu.org/copyleft/fdl.html).)</rdfs:comment>
	<rdfs:label xml:lang="en">MOV</rdfs:label>
	<rdfs:isDefinedBy rdf:resource="http://www.ebusiness-unibw.org/ontologies/consumerelectronics/v1"/>
</rdf:Description>

<rdf:Description rdf:about="http://www.ebusiness-unibw.org/ontologies/consumerelectronics/v1#MP4_Video">
	<rdf:type rdf:resource="http://www.w3.org/2004/02/skos/core#Concept"/>
	<skos:inScheme rdf:resource="http://www.ebusiness-unibw.org/ontologies/consumerelectronics/v1#DataFormatVideo"/>
	<rdfs:comment xml:lang="en">A collection of methods defining compression of video digital data.</rdfs:comment>
	<rdfs:label xml:lang="en">MP4 Video</rdfs:label>
	<rdfs:isDefinedBy rdf:resource="http://www.ebusiness-unibw.org/ontologies/consumerelectronics/v1"/>
</rdf:Description>

<rdf:Description rdf:about="http://www.ebusiness-unibw.org/ontologies/consumerelectronics/v1#MPEG">
	<rdf:type rdf:resource="http://www.w3.org/2004/02/skos/core#Concept"/>
	<skos:inScheme rdf:resource="http://www.ebusiness-unibw.org/ontologies/consumerelectronics/v1#DataFormatVideo"/>
	<rdfs:comment xml:lang="en">Includes all kinds of MPEG formats.</rdfs:comment>
	<rdfs:label xml:lang="en">MPEG</rdfs:label>
	<rdfs:isDefinedBy rdf:resource="http://www.ebusiness-unibw.org/ontologies/consumerelectronics/v1"/>
</rdf:Description>

<rdf:Description rdf:about="http://www.ebusiness-unibw.org/ontologies/consumerelectronics/v1#WMV">
	<rdf:type rdf:resource="http://www.w3.org/2004/02/skos/core#Concept"/>
	<skos:inScheme rdf:resource="http://www.ebusiness-unibw.org/ontologies/consumerelectronics/v1#DataFormatVideo"/>
	<rdfs:comment xml:lang="en">A compressed video file format for several proprietary codecs developed by Microsoft.</rdfs:comment>
	<rdfs:label xml:lang="en">WMV</rdfs:label>
	<rdfs:isDefinedBy rdf:resource="http://www.ebusiness-unibw.org/ontologies/consumerelectronics/v1"/>
</rdf:Description>

</rdf:RDF>