<?xml version="1.0" encoding="UTF-8"?>
<rdf:RDF
	xmlns:vann="http://purl.org/vocab/vann/"
	xmlns:voaf="http://purl.org/vocommons/voaf#"
	xmlns:rdfs="http://www.w3.org/2000/01/rdf-schema#"
	xmlns:owl="http://www.w3.org/2002/07/owl#"
	xmlns:skos="http://www.w3.org/2004/02/skos/core#"
	xmlns:rdf="http://www.w3.org/1999/02/22-rdf-syntax-ns#"
	xmlns:dcterms="http://purl.org/dc/terms/"
	xmlns:dc="http://purl.org/dc/elements/1.1/"
	xmlns:dcmit="http://purl.org/dc/dcmitype/"
	xmlns:sesame="http://www.openrdf.org/schema/sesame#"
	xmlns:xsd="http://www.w3.org/2001/XMLSchema#"
	xmlns:fn="http://www.w3.org/2005/xpath-functions#"
	xmlns:foaf="http://xmlns.com/foaf/0.1/"
	xmlns:hint="http://www.bigdata.com/queryHints#"
	xmlns:bd="http://www.bigdata.com/rdf#"
	xmlns:bds="http://www.bigdata.com/rdf/search#">

<rdf:Description rdf:about="http://www.aktors.org/ontology/portal">
	<rdf:type rdf:resource="http://www.w3.org/2002/07/owl#Ontology"/>
</rdf:Description>

<rdf:Description rdf:about="http://www.aktors.org/ontology/portal#Organization-Size">
	<rdf:type rdf:resource="http://www.w3.org/2004/02/skos/core#ConceptScheme"/>
</rdf:Description>

<rdf:Description rdf:about="http://www.aktors.org/ontology/portal#large-size">
	<rdf:type rdf:resource="http://www.w3.org/2004/02/skos/core#Concept"/>
	<skos:inScheme rdf:resource="http://www.aktors.org/ontology/portal#Organization-Size"/>
</rdf:Description>

<rdf:Description rdf:about="http://www.aktors.org/ontology/portal#Organization-Size">
	<rdfs:comment>We use EU guidelines to distinguish between different organization sizes</rdfs:comment>
	<rdfs:label>Organization Size</rdfs:label>
</rdf:Description>

<rdf:Description rdf:about="http://www.aktors.org/ontology/portal#large-size">
	<rdfs:comment>An organization with more than 250 employees</rdfs:comment>
	<rdfs:label>large</rdfs:label>
</rdf:Description>

<rdf:Description rdf:about="http://www.aktors.org/ontology/portal#has-size">
	<rdfs:range rdf:resource="http://www.aktors.org/ontology/portal#Organization-Size"/>
	<rdf:type rdf:resource="http://www.w3.org/2002/07/owl#ObjectProperty"/>
</rdf:Description>

<rdf:Description rdf:about="http://www.aktors.org/ontology/portal#Organization-Size">
	<rdfs:isDefinedBy rdf:resource="http://www.aktors.org/ontology/portal"/>
</rdf:Description>

<rdf:Description rdf:about="http://www.aktors.org/ontology/portal#large-size">
	<rdfs:isDefinedBy rdf:resource="http://www.aktors.org/ontology/portal"/>
</rdf:Description>

<rdf:Description rdf:about="http://www.aktors.org/ontology/portal#medium-size">
	<rdf:type rdf:resource="http://www.w3.org/2004/02/skos/core#Concept"/>
	<skos:inScheme rdf:resource="http://www.aktors.org/ontology/portal#Organization-Size"/>
	<rdfs:comment>An organization with no more than 250 employees.  It also has to be independent, i.e., less than 25% owned by one enterprise (or jointly by several enterprises) falling outside the definition of medium-sized enterprise. Finally, either the turnover total must be less than 40M Euros or the balance sheet total must be less than 27M Euros.</rdfs:comment>
	<rdfs:label>medium</rdfs:label>
	<rdfs:isDefinedBy rdf:resource="http://www.aktors.org/ontology/portal"/>
</rdf:Description>

<rdf:Description rdf:about="http://www.aktors.org/ontology/portal#micro-size">
	<rdf:type rdf:resource="http://www.w3.org/2004/02/skos/core#Concept"/>
	<skos:inScheme rdf:resource="http://www.aktors.org/ontology/portal#Organization-Size"/>
	<rdfs:comment>An organization with no more than 10 employees.  It also has to be independent, i.e., less than 25% owned by one enterprise (or jointly by several enterprises) falling outside the definition of micro-sized enterprise.</rdfs:comment>
	<rdfs:label>micro</rdfs:label>
	<rdfs:isDefinedBy rdf:resource="http://www.aktors.org/ontology/portal"/>
</rdf:Description>

<rdf:Description rdf:about="http://www.aktors.org/ontology/portal#small-size">
	<rdf:type rdf:resource="http://www.w3.org/2004/02/skos/core#Concept"/>
	<skos:inScheme rdf:resource="http://www.aktors.org/ontology/portal#Organization-Size"/>
	<rdfs:comment>An organization with no more than 50 employees.  It also has to be independent, i.e., less than 25% owned by one enterprise (or jointly by several enterprises) falling outside the definition of small-sized enterprise. Finally, either the turnover total must be less than 7M Euros or the balance sheet total must be less than 5M Euros.</rdfs:comment>
	<rdfs:label>small</rdfs:label>
	<rdfs:isDefinedBy rdf:resource="http://www.aktors.org/ontology/portal"/>
</rdf:Description>

<rdf:Description rdf:about="http://www.aktors.org/ontology/portal#very-large-size">
	<rdf:type rdf:resource="http://www.w3.org/2004/02/skos/core#Concept"/>
	<skos:inScheme rdf:resource="http://www.aktors.org/ontology/portal#Organization-Size"/>
	<rdfs:comment>An organization with over 10000 employees</rdfs:comment>
	<rdfs:label>very large</rdfs:label>
	<rdfs:isDefinedBy rdf:resource="http://www.aktors.org/ontology/portal"/>
</rdf:Description>

</rdf:RDF>