<?xml version="1.0" encoding="UTF-8"?>
<rdf:RDF
	xmlns:vann="http://purl.org/vocab/vann/"
	xmlns:voaf="http://purl.org/vocommons/voaf#"
	xmlns:rdfs="http://www.w3.org/2000/01/rdf-schema#"
	xmlns:owl="http://www.w3.org/2002/07/owl#"
	xmlns:skos="http://www.w3.org/2004/02/skos/core#"
	xmlns:rdf="http://www.w3.org/1999/02/22-rdf-syntax-ns#"
	xmlns:dcterms="http://purl.org/dc/terms/"
	xmlns:dc="http://purl.org/dc/elements/1.1/"
	xmlns:dcmit="http://purl.org/dc/dcmitype/"
	xmlns:sesame="http://www.openrdf.org/schema/sesame#"
	xmlns:xsd="http://www.w3.org/2001/XMLSchema#"
	xmlns:fn="http://www.w3.org/2005/xpath-functions#"
	xmlns:foaf="http://xmlns.com/foaf/0.1/"
	xmlns:hint="http://www.bigdata.com/queryHints#"
	xmlns:bd="http://www.bigdata.com/rdf#"
	xmlns:bds="http://www.bigdata.com/rdf/search#">

<rdf:Description rdf:about="https://w3id.org/arco/ontology/context-description">
	<rdf:type rdf:resource="http://www.w3.org/2002/07/owl#Ontology"/>
</rdf:Description>

<rdf:Description rdf:about="https://w3id.org/arco/ontology/context-description/AlternativeDatingType">
	<rdf:type rdf:resource="http://www.w3.org/2004/02/skos/core#ConceptScheme"/>
</rdf:Description>

<rdf:Description rdf:about="https://w3id.org/arco/ontology/context-description/DifferentDating">
	<rdf:type rdf:resource="http://www.w3.org/2004/02/skos/core#Concept"/>
	<skos:inScheme rdf:resource="https://w3id.org/arco/ontology/context-description/AlternativeDatingType"/>
</rdf:Description>

<rdf:Description rdf:about="https://w3id.org/arco/ontology/context-description/AlternativeDatingType">
	<rdfs:comment xml:lang="en">This class represents the type of alternative dating of a cultural property (different dating, obsolete dating, other method dating)</rdfs:comment>
	<rdfs:label xml:lang="en">Alternative dating type</rdfs:label>
</rdf:Description>

<rdf:Description rdf:about="https://w3id.org/arco/ontology/context-description/DifferentDating">
	<rdfs:comment xml:lang="en">This individual represents a different type of dating than the one present in cultural entity's chronological information.</rdfs:comment>
	<rdfs:label xml:lang="en">Different dating</rdfs:label>
</rdf:Description>

<rdf:Description rdf:about="https://w3id.org/arco/ontology/context-description/hasAlternativeDatingType">
	<rdfs:range rdf:resource="https://w3id.org/arco/ontology/context-description/AlternativeDatingType"/>
	<rdfs:domain rdf:resource="https://w3id.org/arco/ontology/context-description/AlternativeDating"/>
	<rdfs:label xml:lang="en">has alternative dating type</rdfs:label>
	<rdfs:comment xml:lang="en">This property relates an alternative dating to its type.</rdfs:comment>
	<rdf:type rdf:resource="http://www.w3.org/2002/07/owl#ObjectProperty"/>
</rdf:Description>

<rdf:Description rdf:about="https://w3id.org/arco/ontology/context-description/AlternativeDatingType">
	<rdfs:isDefinedBy rdf:resource="https://w3id.org/arco/ontology/context-description"/>
</rdf:Description>

<rdf:Description rdf:about="https://w3id.org/arco/ontology/context-description/DifferentDating">
	<rdfs:isDefinedBy rdf:resource="https://w3id.org/arco/ontology/context-description"/>
</rdf:Description>

<rdf:Description rdf:about="https://w3id.org/arco/ontology/context-description/ObsoleteDating">
	<rdf:type rdf:resource="http://www.w3.org/2004/02/skos/core#Concept"/>
	<skos:inScheme rdf:resource="https://w3id.org/arco/ontology/context-description/AlternativeDatingType"/>
	<rdfs:comment xml:lang="en">This individual represents an obsolete dating.</rdfs:comment>
	<rdfs:label xml:lang="en">Obsolete dating</rdfs:label>
	<rdfs:isDefinedBy rdf:resource="https://w3id.org/arco/ontology/context-description"/>
</rdf:Description>

<rdf:Description rdf:about="https://w3id.org/arco/ontology/context-description/OtherMethodOfDating">
	<rdf:type rdf:resource="http://www.w3.org/2004/02/skos/core#Concept"/>
	<skos:inScheme rdf:resource="https://w3id.org/arco/ontology/context-description/AlternativeDatingType"/>
	<rdfs:comment xml:lang="en">This individual represents a different type of dating method than the one present in cultural entity's chronological information.</rdfs:comment>
	<rdfs:label xml:lang="en">Other method of dating</rdfs:label>
	<rdfs:isDefinedBy rdf:resource="https://w3id.org/arco/ontology/context-description"/>
</rdf:Description>

</rdf:RDF>