<?xml version="1.0" encoding="UTF-8"?>
<rdf:RDF
	xmlns:vann="http://purl.org/vocab/vann/"
	xmlns:voaf="http://purl.org/vocommons/voaf#"
	xmlns:rdfs="http://www.w3.org/2000/01/rdf-schema#"
	xmlns:owl="http://www.w3.org/2002/07/owl#"
	xmlns:skos="http://www.w3.org/2004/02/skos/core#"
	xmlns:rdf="http://www.w3.org/1999/02/22-rdf-syntax-ns#"
	xmlns:dcterms="http://purl.org/dc/terms/"
	xmlns:dc="http://purl.org/dc/elements/1.1/"
	xmlns:dcmit="http://purl.org/dc/dcmitype/"
	xmlns:sesame="http://www.openrdf.org/schema/sesame#"
	xmlns:xsd="http://www.w3.org/2001/XMLSchema#"
	xmlns:fn="http://www.w3.org/2005/xpath-functions#"
	xmlns:foaf="http://xmlns.com/foaf/0.1/"
	xmlns:hint="http://www.bigdata.com/queryHints#"
	xmlns:bd="http://www.bigdata.com/rdf#"
	xmlns:bds="http://www.bigdata.com/rdf/search#">

<rdf:Description rdf:about="http://rdf.geospecies.org/ont/geospecies">
	<rdf:type rdf:resource="http://www.w3.org/2002/07/owl#Ontology"/>
</rdf:Description>

<rdf:Description rdf:about="http://rdf.geospecies.org/ont/geospecies#Omernik_Level_III_Ecoregion_Classification">
	<rdf:type rdf:resource="http://www.w3.org/2004/02/skos/core#ConceptScheme"/>
</rdf:Description>

<rdf:Description rdf:about="http://rdf.geospecies.org/ont/geospecies#Omernik_3_50_Northern_Lakes_and_Forests">
	<rdf:type rdf:resource="http://www.w3.org/2004/02/skos/core#Concept"/>
	<skos:inScheme rdf:resource="http://rdf.geospecies.org/ont/geospecies#Omernik_Level_III_Ecoregion_Classification"/>
</rdf:Description>

<rdf:Description rdf:about="http://rdf.geospecies.org/ont/geospecies#Omernik_Level_III_Ecoregion_Classification">
	<rdfs:comment>The ecoregions shown here have been derived from Omernik (1987) and from refinements of Omernik's framework that have been made for other projects. These ongoing or recently completed projects, conducted in collaboration with the U.S. EPA regional offices, state resource management agencies, and with other federal agencies, involve refining ecoregions, defining subregions, and locating sets of reference sites. Designed to serve as a spatial framework for environmental resource management, ecoregions denote areas within which ecosystems (and the type, quality, and quantity of environmental resources) are generally similar. The most immediate needs are to develop regional biological criteria and water quality standards and to set management goals for nonpoint source pollution. 

The approach used to compile this map is based on the premise that ecological regions can be identified through the analysis of the patterns and the composition of biotic and abiotic phenomena that affect or reflect differences in ecosystem quality and integrity (Wiken 1986; Omernik 1987, 1995). These phenomena include geology, physiography, vegetation, climate, soils, land use, wildlife, and hydrology. The relative importance of each characteristic varies from one ecological region to another regardless of the hierarchical level. Because of possible confusion with other meanings of terms for different levels of ecological regions, a Roman numeral classification scheme has been adopted for this effort. Level I is the coarsest level, dividing North America into 15 ecological regions, whereas at Level II the continent is subdivided into 52 classes (CEC 1997). Level III is the hierarchical level shown on this map. For portions of the United States the ecoregions have been further subdivided to Level IV. The applications of the ecoregions are explained in Gallant et al. (1989) and in reports and publications from the state and regional projects. 

For additional information, contact James M. Omernik, U.S. EPA National Health and Environmental Effects Laboratory (NHEERL), 200 SW 35th Street, Corvallis, OR 97333 (phone: 541-754-4458 and email: omernik.james@epa.gov).</rdfs:comment>
	<rdfs:label>Omernik_Level_Three_Classification</rdfs:label>
</rdf:Description>

<rdf:Description rdf:about="http://rdf.geospecies.org/ont/geospecies#Omernik_3_50_Northern_Lakes_and_Forests">
	<rdfs:comment>The Northern Lakes and Forests (50) is an ecoregion of relatively nutrient poor glacial soils, coniferous and northern hardwoods forests, undulating till plains, morainal hills, broad lacustrine basins, and areas of extensive sandy outwash plains. Soils are formed primarily from sandy and loamy glacial drift material and generally lack the arability of those in adjacent ecoregions to the south. Ecoregion 50 also has lower annual temperatures and a frost-free period that is
considerably shorter than other ecoregions in Wisconsin. These conditions generally hinder agriculture; therefore, woodland and forest are the predominant land use/land cover. The numerous lakes that dot the landscape are clearer, at a lower trophic state (mostly oligotrophic to mesotrophic with few eutrophic lakes), and less productive than those in ecoregions to the south. Streams of ecoregion 50 are mostly perennial, originating in lakes and wetlands; however, stream density is relatively low compared to ecoregions to the south. The Northern Lakes and Forests region is the only ecoregion in Wisconsin where acid sensitive lakes are found. Portions of the southern boundary of ecoregion 50 roughly correspond to the southernmost extent of lakes with alkalinity values less than 400 meq/l (Omernik and Griffith 1986).</rdfs:comment>
	<rdfs:label>Omernik_4_Northern Lakes and Forests</rdfs:label>
</rdf:Description>

<rdf:Description rdf:about="http://rdf.geospecies.org/ont/geospecies#hasOmernik_3_Ecozone">
	<rdfs:range rdf:resource="http://rdf.geospecies.org/ont/geospecies#Omernik_Level_III_Ecoregion_Classification"/>
	<rdfs:domain rdf:resource="http://rdf.geospecies.org/ont/geospecies#Location"/>
	<rdfs:label>hasOmernik_3_Ecozone</rdfs:label>
	<rdf:type rdf:resource="http://www.w3.org/2002/07/owl#ObjectProperty"/>
</rdf:Description>

<rdf:Description rdf:about="http://rdf.geospecies.org/ont/geospecies#Omernik_Level_III_Ecoregion_Classification">
	<rdfs:isDefinedBy rdf:resource="http://rdf.geospecies.org/ont/geospecies"/>
</rdf:Description>

<rdf:Description rdf:about="http://rdf.geospecies.org/ont/geospecies#Omernik_3_50_Northern_Lakes_and_Forests">
	<rdfs:isDefinedBy rdf:resource="http://rdf.geospecies.org/ont/geospecies"/>
</rdf:Description>

<rdf:Description rdf:about="http://rdf.geospecies.org/ont/geospecies#Omernik_3_51_North_Central_Hardwood_Forests">
	<rdf:type rdf:resource="http://www.w3.org/2004/02/skos/core#Concept"/>
	<skos:inScheme rdf:resource="http://rdf.geospecies.org/ont/geospecies#Omernik_Level_III_Ecoregion_Classification"/>
	<rdfs:comment>The North Central Hardwoods Forests (51) ecoregion is transitional between the predominantly forested Northern Lakes and Forests (50) and the agricultural ecoregions to the south. Nearly level to rolling till plains, lacustrine basins, outwash plains, and rolling to hilly moraines comprise the physiography of this region. The land use/land cover in this ecoregion consists of a mosaic of forests, wetlands and lakes, cropland agriculture, pasture, and dairy operations. The growing season is generally longer and warmer than that of ecoregion 50 to the north, and the soils are more arable and fertile, contributing to the greater agricultural component of the land use. Lake densities are generally lower here than in the Northern Lakes and Forests, and lake trophic states tend to be higher, with higher percentages in eutrophic and hypereutrophic classes. Stream density is highly variable, with some areas having virtually no streams--in wetland and kettle terrain--to others with high densities of perennial streams.</rdfs:comment>
	<rdfs:label>Omernik_3_North_Central_Hardwood_Forests</rdfs:label>
	<rdfs:isDefinedBy rdf:resource="http://rdf.geospecies.org/ont/geospecies"/>
</rdf:Description>

<rdf:Description rdf:about="http://rdf.geospecies.org/ont/geospecies#Omernik_3_52_Driftless_Area">
	<rdf:type rdf:resource="http://www.w3.org/2004/02/skos/core#Concept"/>
	<skos:inScheme rdf:resource="http://rdf.geospecies.org/ont/geospecies#Omernik_Level_III_Ecoregion_Classification"/>
	<rdfs:comment>The hilly uplands of the Driftless Area (52) ecoregion easily distinguish it from surrounding ecoregions. Much of the area consists of a deeply dissected loess-capped plateau. Also called the Paleozoic Plateau because there is evidence of glacial drift in this region, the glacial deposits have done little to affect the landscape compared to the subduing influences in adjacent ecoregions. Livestock and dairy farming are major land uses and have had a major impact on stream quality. In contrast to the adjacent glaciated ecoregions, the Driftless Area has few lakes, most of which are reservoirs with generally high trophic states, and a stream density and flow that is generally greater than regions to the east.</rdfs:comment>
	<rdfs:label>Omernik_3_Driftless_Area</rdfs:label>
	<rdfs:isDefinedBy rdf:resource="http://rdf.geospecies.org/ont/geospecies"/>
</rdf:Description>

<rdf:Description rdf:about="http://rdf.geospecies.org/ont/geospecies#Omernik_3_53_Southeastern_Wisconsin_Till_Plains">
	<rdf:type rdf:resource="http://www.w3.org/2004/02/skos/core#Concept"/>
	<skos:inScheme rdf:resource="http://rdf.geospecies.org/ont/geospecies#Omernik_Level_III_Ecoregion_Classification"/>
	<rdfs:comment>The Southeastern Wisconsin Till Plains (53) ecoregion supports a mosaic of vegetation types and represents a transition between the hardwood forests and oak savannas of the ecoregions to the west and the tall-grass prairies of the Central Corn Belt Plains (54) to the south. Similar to the Corn Belt Plains (54) ecoregion, land use in the Southeastern Wisconsin Till Plains (53) is mostly cropland, but the crops historically have been largely forage and feed grains to support dairy operations, rather than corn and soybeans for cash crops. The ecoregion has a higher plant hardiness value than ecoregions to the north and west, a different mosaic of soils than western ecoregions, and flatter topography. There are fewer lakes here than in ecoregions to the north, but considerably more than in the western Driftless Area (52) and the southern Central Corn Belt Plains (47). The region also has a relatively high diversity of aquatic species.</rdfs:comment>
	<rdfs:label>Omernik_3_Southeastern_Wisconsin_Till_Plains</rdfs:label>
	<rdfs:isDefinedBy rdf:resource="http://rdf.geospecies.org/ont/geospecies"/>
</rdf:Description>

<rdf:Description rdf:about="http://rdf.geospecies.org/ont/geospecies#Omernik_3_47_Western_Corn_Belt_Plains">
	<rdf:type rdf:resource="http://www.w3.org/2004/02/skos/core#Concept"/>
	<skos:inScheme rdf:resource="http://rdf.geospecies.org/ont/geospecies#Omernik_Level_III_Ecoregion_Classification"/>
	<rdfs:label>Omernik_3_Western Corn Belt Plains</rdfs:label>
	<rdfs:isDefinedBy rdf:resource="http://rdf.geospecies.org/ont/geospecies"/>
</rdf:Description>

</rdf:RDF>