<rdf:RDF
    xmlns:dct="http://purl.org/dc/terms/"
    xmlns:rdf="http://www.w3.org/1999/02/22-rdf-syntax-ns#"
    xmlns:dc="http://purl.org/dc/elements/1.1/"
    xmlns:owl="http://www.w3.org/2002/07/owl#"
    xmlns:dcmit="http://purl.org/dc/dcmitype/"
    xmlns:skos="http://www.w3.org/2004/02/skos/core#"
    xmlns:voaf="http://purl.org/vocommons/voaf#"
    xmlns:rdfs="http://www.w3.org/2000/01/rdf-schema#"
    xmlns:vann="http://purl.org/vocab/vann/">
  <skos:Concept rdf:about="http://www.ebusiness-unibw.org/ontologies/consumerelectronics/v1#Cardstock">
    <rdfs:label xml:lang="en">cardstock</rdfs:label>
    <rdfs:label xml:lang="de">Fotokarton</rdfs:label>
    <rdfs:comment xml:lang="en">A paper stock that is thicker and more durable than normal writing or printing paper, but thinner and more flexible than other forms of paperboard.

(This description is partly based on or reuses content from the Wikipedia article "Cardstock" (http://en.wikipedia.org/wiki/Card_stock) and is licensed under the GNU Free Documentation License (http://www.gnu.org/copyleft/fdl.html).)</rdfs:comment>
    <skos:inScheme>
      <skos:ConceptScheme rdf:about="http://www.ebusiness-unibw.org/ontologies/consumerelectronics/v1#MediaType"/>
    </skos:inScheme>
  </skos:Concept>
  <skos:Concept rdf:about="http://www.ebusiness-unibw.org/ontologies/consumerelectronics/v1#Postcard">
    <rdfs:label xml:lang="en">Postcard</rdfs:label>
    <rdfs:label xml:lang="de">Postkarte</rdfs:label>
    <rdfs:comment xml:lang="en">Rectangular piece of thick paper or thin cardboard intended for writing and mailing without an envelope.</rdfs:comment>
    <skos:inScheme rdf:resource="http://www.ebusiness-unibw.org/ontologies/consumerelectronics/v1#MediaType"/>
  </skos:Concept>
  <skos:Concept rdf:about="http://www.ebusiness-unibw.org/ontologies/consumerelectronics/v1#Photopaper">
    <rdfs:label xml:lang="en">Photo paper</rdfs:label>
    <rdfs:label xml:lang="de">Fotopapier</rdfs:label>
    <rdfs:comment xml:lang="en">Kind of paper that is specifically designed to print high quality digital photos.</rdfs:comment>
    <skos:inScheme rdf:resource="http://www.ebusiness-unibw.org/ontologies/consumerelectronics/v1#MediaType"/>
  </skos:Concept>
  <skos:Concept rdf:about="http://www.ebusiness-unibw.org/ontologies/consumerelectronics/v1#LaserPrintingPaper">
    <rdfs:label xml:lang="en">Laser printing paper</rdfs:label>
    <rdfs:label xml:lang="de">Laserdruckpapier</rdfs:label>
    <rdfs:comment xml:lang="en">Special sort of paper used in laser printers.</rdfs:comment>
    <skos:inScheme rdf:resource="http://www.ebusiness-unibw.org/ontologies/consumerelectronics/v1#MediaType"/>
  </skos:Concept>
  <skos:Concept rdf:about="http://www.ebusiness-unibw.org/ontologies/consumerelectronics/v1#Label">
    <rdfs:label xml:lang="de">Etikett</rdfs:label>
    <rdfs:label xml:lang="en">Label</rdfs:label>
    <rdfs:comment xml:lang="en">Media type that can be printed on one side and has a glued area on the other side.</rdfs:comment>
    <skos:inScheme rdf:resource="http://www.ebusiness-unibw.org/ontologies/consumerelectronics/v1#MediaType"/>
  </skos:Concept>
  <skos:Concept rdf:about="http://www.ebusiness-unibw.org/ontologies/consumerelectronics/v1#PlainPaper">
    <rdfs:label xml:lang="en">Plain paper</rdfs:label>
    <rdfs:label xml:lang="de">Normalpapier</rdfs:label>
    <rdfs:comment xml:lang="en">Thin material mainly used for writing upon, printing upon or packaging.</rdfs:comment>
    <skos:inScheme rdf:resource="http://www.ebusiness-unibw.org/ontologies/consumerelectronics/v1#MediaType"/>
  </skos:Concept>
  <skos:Concept rdf:about="http://www.ebusiness-unibw.org/ontologies/consumerelectronics/v1#Envelope">
    <rdfs:label xml:lang="de">Briefkuvert</rdfs:label>
    <rdfs:label xml:lang="en">Envelope</rdfs:label>
    <rdfs:comment xml:lang="en">Is a packaging product, usually made of flat material such as paper or cardboard.</rdfs:comment>
    <skos:inScheme rdf:resource="http://www.ebusiness-unibw.org/ontologies/consumerelectronics/v1#MediaType"/>
  </skos:Concept>
  <skos:Concept rdf:about="http://www.ebusiness-unibw.org/ontologies/consumerelectronics/v1#Transparency">
    <rdfs:label xml:lang="en">Transparency</rdfs:label>
    <rdfs:label xml:lang="de">Folie</rdfs:label>
    <rdfs:comment xml:lang="en">A thin sheet of transparent flexible material, typically cellulose acetate, onto which you can print.</rdfs:comment>
    <skos:inScheme rdf:resource="http://www.ebusiness-unibw.org/ontologies/consumerelectronics/v1#MediaType"/>
  </skos:Concept>
</rdf:RDF>
