<rdf:RDF
    xmlns:dct="http://purl.org/dc/terms/"
    xmlns:rdf="http://www.w3.org/1999/02/22-rdf-syntax-ns#"
    xmlns:dc="http://purl.org/dc/elements/1.1/"
    xmlns:owl="http://www.w3.org/2002/07/owl#"
    xmlns:dcmit="http://purl.org/dc/dcmitype/"
    xmlns:skos="http://www.w3.org/2004/02/skos/core#"
    xmlns:voaf="http://purl.org/vocommons/voaf#"
    xmlns:rdfs="http://www.w3.org/2000/01/rdf-schema#"
    xmlns:vann="http://purl.org/vocab/vann/">
  <skos:Concept rdf:about="http://data.doremus.org/ontology#U84_has_parallel_key">
    <rdfs:comment xml:lang="fr">Scope Note: Cette classe permet de connecter deux M4 Tonalité qui sont en une relation parallèle, c'est-à-dire l'une est la parallèle majeur ou mineur de l'autre.</rdfs:comment>
    <rdfs:comment xml:lang="fr">Exemples: la clé de 'Do majeur' a 'Do mineur' pour tonalité parallèle</rdfs:comment>
    <rdfs:comment>see also http://en.wikipedia.org/wiki/Parallel_key</rdfs:comment>
    <rdfs:comment xml:lang="en">Examples: the key of 'C major' has 'C minor' as parallel key</rdfs:comment>
    <rdfs:label xml:lang="en">U84 has parallel key</rdfs:label>
    <rdfs:label xml:lang="fr">U84 a pour tonalité parallèle</rdfs:label>
    <rdfs:comment xml:lang="en">Scope Note: This class allows to connect two M4 Keys that are in a parallel relationship, i.e. one is the parallel major or minor of the other one.</rdfs:comment>
    <skos:inScheme>
      <skos:ConceptScheme rdf:about="http://www.w3.org/2002/07/owl#SymmetricObjectProperty"/>
    </skos:inScheme>
  </skos:Concept>
  <skos:Concept rdf:about="http://data.doremus.org/ontology#U83_has_relative_key">
    <rdfs:comment xml:lang="fr">Exemples: la clé de 'Do majeur' a 'La mineur' pour tonalité relative</rdfs:comment>
    <rdfs:comment>see also http://en.wikipedia.org/wiki/Relative_key</rdfs:comment>
    <rdfs:comment xml:lang="en">Scope Note: This class allows to connect two M4 Keys that are in a relative relationship, i.e. one is the relative major or minor of the other one.</rdfs:comment>
    <rdfs:comment xml:lang="fr">Scope Note: Cette classe permet de connecter deux M4 Tonalité qui sont en relation par rapport à l'armure, c'est-à-dire l'une est la relatif majeur ou mineur de l'autre.</rdfs:comment>
    <rdfs:label xml:lang="en">U83 has relative key</rdfs:label>
    <rdfs:label xml:lang="fr">U83 a pour tonalité relative</rdfs:label>
    <rdfs:comment xml:lang="en">Examples: the key of 'C major' has 'A minor' as relative key</rdfs:comment>
    <skos:inScheme rdf:resource="http://www.w3.org/2002/07/owl#SymmetricObjectProperty"/>
  </skos:Concept>
  <skos:Concept rdf:about="http://data.doremus.org/ontology#U85_has_closely_related_key">
    <rdfs:comment xml:lang="en">Scope Note: This class allows to connect two M4 Keys that are mutually closely related from an harmonic point of view, e.g. they are commonly used destinations or transpositions in a modulation.</rdfs:comment>
    <rdfs:comment xml:lang="fr">Scope Note: Cette classe permet de connecter deux M4 Tonalité qui sont étroitement liées d'un point de vue harmonique, par ex. ceux sont des destinations ou des transpositions fréquemment utilisées dans une modulation</rdfs:comment>
    <rdfs:comment xml:lang="en">Examples: the key of 'C major' has 'G major' and 'D minor' as closely related keys</rdfs:comment>
    <rdfs:comment>see also http://en.wikipedia.org/wiki/Closely_related_key</rdfs:comment>
    <rdfs:label xml:lang="en">U85 has closely related key</rdfs:label>
    <rdfs:label xml:lang="fr">U85 a pour tonalité étroitement lié</rdfs:label>
    <rdfs:comment xml:lang="fr">Exemples: la clé de 'Do majeur' a 'Sol majeur' et 'Re majeur' pour tonalités étroitement liées</rdfs:comment>
    <skos:inScheme rdf:resource="http://www.w3.org/2002/07/owl#SymmetricObjectProperty"/>
  </skos:Concept>
</rdf:RDF>
