<rdf:RDF
    xmlns:dct="http://purl.org/dc/terms/"
    xmlns:rdf="http://www.w3.org/1999/02/22-rdf-syntax-ns#"
    xmlns:dc="http://purl.org/dc/elements/1.1/"
    xmlns:owl="http://www.w3.org/2002/07/owl#"
    xmlns:dcmit="http://purl.org/dc/dcmitype/"
    xmlns:skos="http://www.w3.org/2004/02/skos/core#"
    xmlns:voaf="http://purl.org/vocommons/voaf#"
    xmlns:rdfs="http://www.w3.org/2000/01/rdf-schema#"
    xmlns:vann="http://purl.org/vocab/vann/">
  <skos:Concept rdf:about="http://www.ebusiness-unibw.org/ontologies/consumerelectronics/v1#FocusManual">
    <rdfs:label xml:lang="en">Focus manual</rdfs:label>
    <rdfs:label xml:lang="de">Manueller Fokus</rdfs:label>
    <rdfs:comment xml:lang="en">A manual focus allows the operator to adjust the focus of the lens by hand.

(This description is partly based on or reuses content from the Wikipedia article "Manual focus" (http://en.wikipedia.org/wiki/Manual_focus) and is licensed under the GNU Free Documentation License (http://www.gnu.org/copyleft/fdl.html).)</rdfs:comment>
    <skos:inScheme>
      <skos:ConceptScheme rdf:about="http://www.ebusiness-unibw.org/ontologies/consumerelectronics/v1#Focus"/>
    </skos:inScheme>
  </skos:Concept>
  <skos:Concept rdf:about="http://www.ebusiness-unibw.org/ontologies/consumerelectronics/v1#FocusFixed">
    <rdfs:label xml:lang="en">Focus fixed</rdfs:label>
    <rdfs:label xml:lang="de">Starrer Fokus</rdfs:label>
    <rdfs:comment xml:lang="en">A photographic lens for which the focus is not adjustable is called a fixed-focus lens.

(This description is partly based on or reuses content from the Wikipedia article "Fixed focus" (http://en.wikipedia.org/wiki/Fixed_focus) and is licensed under the GNU Free Documentation License (http://www.gnu.org/copyleft/fdl.html).)</rdfs:comment>
    <skos:inScheme rdf:resource="http://www.ebusiness-unibw.org/ontologies/consumerelectronics/v1#Focus"/>
  </skos:Concept>
  <skos:Concept rdf:about="http://www.ebusiness-unibw.org/ontologies/consumerelectronics/v1#FocusAuto">
    <rdfs:label xml:lang="en">Focus auto</rdfs:label>
    <rdfs:label xml:lang="de">Autofokus</rdfs:label>
    <rdfs:comment xml:lang="en">Autofocus (or AF) is a feature of some optical systems that allows them to obtain (and in some systems to also continuously maintain) correct focus on a subject, instead of requiring the operator to adjust focus manually.

(This description is partly based on or reuses content from the Wikipedia article "Autofocus" (http://en.wikipedia.org/wiki/Autofocus) and is licensed under the GNU Free Documentation License (http://www.gnu.org/copyleft/fdl.html).)</rdfs:comment>
    <skos:inScheme rdf:resource="http://www.ebusiness-unibw.org/ontologies/consumerelectronics/v1#Focus"/>
  </skos:Concept>
</rdf:RDF>
