<rdf:RDF
    xmlns:dct="http://purl.org/dc/terms/"
    xmlns:rdf="http://www.w3.org/1999/02/22-rdf-syntax-ns#"
    xmlns:dc="http://purl.org/dc/elements/1.1/"
    xmlns:owl="http://www.w3.org/2002/07/owl#"
    xmlns:dcmit="http://purl.org/dc/dcmitype/"
    xmlns:skos="http://www.w3.org/2004/02/skos/core#"
    xmlns:voaf="http://purl.org/vocommons/voaf#"
    xmlns:rdfs="http://www.w3.org/2000/01/rdf-schema#"
    xmlns:vann="http://purl.org/vocab/vann/">
  <owl:Ontology rdf:about="http://www.ebusiness-unibw.org/ontologies/consumerelectronics/v1"/>
  <owl:ObjectProperty rdf:about="http://www.ebusiness-unibw.org/ontologies/consumerelectronics/v1#hasViewFinder">
    <rdfs:isDefinedBy rdf:resource="http://www.ebusiness-unibw.org/ontologies/consumerelectronics/v1"/>
    <rdfs:comment xml:lang="en">A viewfinder is what the photographer looks through to compose, and in many cases to focus, the picture.

(This description is partly based on or reuses content from the Wikipedia article "Viewfinder" (http://en.wikipedia.org/wiki/Viewfinder) and is licensed under the GNU Free Documentation License (http://www.gnu.org/copyleft/fdl.html).)</rdfs:comment>
    <rdfs:label xml:lang="en">viewfinder</rdfs:label>
    <rdfs:range>
      <skos:ConceptScheme rdf:about="http://www.ebusiness-unibw.org/ontologies/consumerelectronics/v1#ViewFinder">
        <rdfs:isDefinedBy rdf:resource="http://www.ebusiness-unibw.org/ontologies/consumerelectronics/v1"/>
      </skos:ConceptScheme>
    </rdfs:range>
  </owl:ObjectProperty>
  <skos:Concept rdf:about="http://www.ebusiness-unibw.org/ontologies/consumerelectronics/v1#ViewFinderOptical">
    <rdfs:isDefinedBy rdf:resource="http://www.ebusiness-unibw.org/ontologies/consumerelectronics/v1"/>
    <rdfs:label xml:lang="en">Viewfinder optical</rdfs:label>
    <rdfs:comment xml:lang="en">An optical viewfinder is simply a reversed telescope mounted to see what the camera will see.

(This description is partly based on or reuses content from the Wikipedia article "Viewfinder" (http://en.wikipedia.org/wiki/Viewfinder) and is licensed under the GNU Free Documentation License (http://www.gnu.org/copyleft/fdl.html).)</rdfs:comment>
    <skos:inScheme rdf:resource="http://www.ebusiness-unibw.org/ontologies/consumerelectronics/v1#ViewFinder"/>
  </skos:Concept>
  <skos:Concept rdf:about="http://www.ebusiness-unibw.org/ontologies/consumerelectronics/v1#ViewFinderElectronic">
    <rdfs:isDefinedBy rdf:resource="http://www.ebusiness-unibw.org/ontologies/consumerelectronics/v1"/>
    <rdfs:label xml:lang="en">Viewfinder electronic</rdfs:label>
    <rdfs:comment xml:lang="en">An electronic viewfinder or EVF is a viewfinder where the image captured by the lens is projected electronically onto a miniature display. The image on this display is used to assist in aiming the camera at the scene to be photographed.

(This description is partly based on or reuses content from the Wikipedia article "Electronic viewfinder" (http://en.wikipedia.org/wiki/Electronic_viewfinder) and is licensed under the GNU Free Documentation License (http://www.gnu.org/copyleft/fdl.html).)</rdfs:comment>
    <skos:inScheme rdf:resource="http://www.ebusiness-unibw.org/ontologies/consumerelectronics/v1#ViewFinder"/>
  </skos:Concept>
</rdf:RDF>
