<rdf:RDF
    xmlns:dct="http://purl.org/dc/terms/"
    xmlns:rdf="http://www.w3.org/1999/02/22-rdf-syntax-ns#"
    xmlns:dc="http://purl.org/dc/elements/1.1/"
    xmlns:owl="http://www.w3.org/2002/07/owl#"
    xmlns:dcmit="http://purl.org/dc/dcmitype/"
    xmlns:skos="http://www.w3.org/2004/02/skos/core#"
    xmlns:voaf="http://purl.org/vocommons/voaf#"
    xmlns:rdfs="http://www.w3.org/2000/01/rdf-schema#"
    xmlns:vann="http://purl.org/vocab/vann/">
  <owl:Ontology rdf:about="http://www.ebusiness-unibw.org/ontologies/consumerelectronics/v1"/>
  <skos:Concept rdf:about="http://www.ebusiness-unibw.org/ontologies/consumerelectronics/v1#Digital">
    <rdfs:isDefinedBy rdf:resource="http://www.ebusiness-unibw.org/ontologies/consumerelectronics/v1"/>
    <rdfs:label xml:lang="en">Digital</rdfs:label>
    <rdfs:comment xml:lang="en">A digital system uses discrete (discontinuous) values, usually but not always symbolized numerically (hence called "digital") to represent information for input, processing, transmission, storage.

(This description is partly based on or reuses content from the Wikipedia article "Digital" (http://en.wikipedia.org/wiki/Digital) and is licensed under the GNU Free Documentation License (http://www.gnu.org/copyleft/fdl.html).)</rdfs:comment>
    <skos:inScheme>
      <skos:ConceptScheme rdf:about="http://www.ebusiness-unibw.org/ontologies/consumerelectronics/v1#TunerType">
        <rdfs:isDefinedBy rdf:resource="http://www.ebusiness-unibw.org/ontologies/consumerelectronics/v1"/>
        <rdfs:label xml:lang="en">Type of TV tuner that is used to convert RF television transmissions into audio and video signals.

(This description is partly based on or reuses content from the Wikipedia article "Tuner (electronics)" (http://en.wikipedia.org/wiki/Tuner_(electronics)) and is licensed under the GNU Free Documentation License (http://www.gnu.org/copyleft/fdl.html).)</rdfs:label>
        <rdfs:comment xml:lang="en">Type of TV tuner that is used to convert RF television transmissions into audio and video signals.

(This description is partly based on or reuses content from the Wikipedia article "Tuner (electronics)" (http://en.wikipedia.org/wiki/Tuner_(electronics)) and is licensed under the GNU Free Documentation License (http://www.gnu.org/copyleft/fdl.html).)</rdfs:comment>
      </skos:ConceptScheme>
    </skos:inScheme>
  </skos:Concept>
  <skos:Concept rdf:about="http://www.ebusiness-unibw.org/ontologies/consumerelectronics/v1#Analog">
    <rdfs:isDefinedBy rdf:resource="http://www.ebusiness-unibw.org/ontologies/consumerelectronics/v1"/>
    <rdfs:label xml:lang="en">Analog</rdfs:label>
    <rdfs:comment xml:lang="en">An analog or analogue signal is any continuous signal for which the time varying feature (variable) of the signal is a representation of some other time varying quantity, i.e analogous to another time varying signal.

(This description is partly based on or reuses content from the Wikipedia article "Analog signal" (http://en.wikipedia.org/wiki/Analog_signal) and is licensed under the GNU Free Documentation License (http://www.gnu.org/copyleft/fdl.html).)</rdfs:comment>
    <skos:inScheme rdf:resource="http://www.ebusiness-unibw.org/ontologies/consumerelectronics/v1#TunerType"/>
  </skos:Concept>
</rdf:RDF>
