<rdf:RDF
    xmlns:dct="http://purl.org/dc/terms/"
    xmlns:rdf="http://www.w3.org/1999/02/22-rdf-syntax-ns#"
    xmlns:dc="http://purl.org/dc/elements/1.1/"
    xmlns:owl="http://www.w3.org/2002/07/owl#"
    xmlns:dcmit="http://purl.org/dc/dcmitype/"
    xmlns:skos="http://www.w3.org/2004/02/skos/core#"
    xmlns:voaf="http://purl.org/vocommons/voaf#"
    xmlns:rdfs="http://www.w3.org/2000/01/rdf-schema#"
    xmlns:vann="http://purl.org/vocab/vann/">
  <owl:Ontology rdf:about="http://ontology.it/itsmo/v1"/>
  <owl:ObjectProperty rdf:about="http://ontology.it/itsmo/v1#hasStatus">
    <rdfs:isDefinedBy rdf:resource="http://ontology.it/itsmo/v1"/>
    <rdfs:comment xml:lang="en">the referenced resource is a stage in the life cycle of the described resource.</rdfs:comment>
    <rdfs:label rdf:datatype="http://www.w3.org/2001/XMLSchema#string"
    >hasStatus</rdfs:label>
    <rdfs:range>
      <skos:ConceptScheme rdf:about="http://ontology.it/itsmo/v1#LifeCycleStage">
        <rdfs:isDefinedBy rdf:resource="http://ontology.it/itsmo/v1"/>
        <rdfs:label xml:lang="en">A stage in the life of a configuration item. The lifecycle defines the 
    categories for status and the status transitions that are permitted. For 
    example:

    &lt;ul&gt;
      &lt;li&gt;
        The lifecycle of an application includes requirements, design, build, 
        deploy, operate, optimize.
      &lt;/li&gt;
      &lt;li&gt;
        The expanded incident lifecycle includes detection, diagnosis, repair, 
        recovery and restoration
      &lt;/li&gt;
      &lt;li&gt;
        The lifecycle of a server may include: ordered, received, in test, 
        live, disposed etc
      &lt;/li&gt;
    &lt;/ul&gt;</rdfs:label>
        <rdfs:comment xml:lang="en">A stage in the life of a configuration item. The lifecycle defines the 
    categories for status and the status transitions that are permitted. For 
    example:

    &lt;ul&gt;
      &lt;li&gt;
        The lifecycle of an application includes requirements, design, build, 
        deploy, operate, optimize.
      &lt;/li&gt;
      &lt;li&gt;
        The expanded incident lifecycle includes detection, diagnosis, repair, 
        recovery and restoration
      &lt;/li&gt;
      &lt;li&gt;
        The lifecycle of a server may include: ordered, received, in test, 
        live, disposed etc
      &lt;/li&gt;
    &lt;/ul&gt;</rdfs:comment>
      </skos:ConceptScheme>
    </rdfs:range>
  </owl:ObjectProperty>
  <skos:Concept rdf:about="http://ontology.it/itsmo/v1#Retire">
    <rdfs:isDefinedBy rdf:resource="http://ontology.it/itsmo/v1"/>
    <rdfs:label rdf:datatype="http://www.w3.org/2001/XMLSchema#string"
    >Retire</rdfs:label>
    <rdfs:comment xml:lang="en">Permanent removal of a configuration item, from the live environment. Being retired is a stage in the lifecycle of many configuration items.</rdfs:comment>
    <skos:inScheme rdf:resource="http://ontology.it/itsmo/v1#LifeCycleStage"/>
  </skos:Concept>
</rdf:RDF>
