<rdf:RDF
    xmlns:dct="http://purl.org/dc/terms/"
    xmlns:rdf="http://www.w3.org/1999/02/22-rdf-syntax-ns#"
    xmlns:dc="http://purl.org/dc/elements/1.1/"
    xmlns:owl="http://www.w3.org/2002/07/owl#"
    xmlns:dcmit="http://purl.org/dc/dcmitype/"
    xmlns:skos="http://www.w3.org/2004/02/skos/core#"
    xmlns:voaf="http://purl.org/vocommons/voaf#"
    xmlns:rdfs="http://www.w3.org/2000/01/rdf-schema#"
    xmlns:vann="http://purl.org/vocab/vann/">
  <owl:Ontology rdf:about="http://online-presence.net/opo/ns#"/>
  <skos:Concept rdf:about="http://online-presence.net/opo/ns#ConstrainedFindability">
    <rdfs:isDefinedBy rdf:resource="http://online-presence.net/opo/ns#"/>
    <rdfs:label xml:lang="en">ConstrainedFindability</rdfs:label>
    <rdfs:comment xml:lang="en">The Agent's contact details cannot be found by anyone on
			the Web, but the findability is controled by some
			rules/policies.</rdfs:comment>
    <skos:inScheme>
      <skos:ConceptScheme rdf:about="http://online-presence.net/opo/ns#Findability">
        <rdfs:isDefinedBy rdf:resource="http://online-presence.net/opo/ns#"/>
        <rdfs:label xml:lang="en">The OnlinePresenceComponent used to represent the
			possibility to find contact details of an Agent in a public
			listing</rdfs:label>
        <rdfs:comment xml:lang="en">The OnlinePresenceComponent used to represent the
			possibility to find contact details of an Agent in a public
			listing</rdfs:comment>
      </skos:ConceptScheme>
    </skos:inScheme>
  </skos:Concept>
  <skos:Concept rdf:about="http://online-presence.net/opo/ns#PubliclyFindable">
    <rdfs:isDefinedBy rdf:resource="http://online-presence.net/opo/ns#"/>
    <rdfs:label xml:lang="en">PubliclyFindable</rdfs:label>
    <rdfs:comment xml:lang="en">The Agent's contact details canbe found by anyone on the
			Web</rdfs:comment>
    <skos:inScheme rdf:resource="http://online-presence.net/opo/ns#Findability"/>
  </skos:Concept>
</rdf:RDF>
