<rdf:RDF
    xmlns:dct="http://purl.org/dc/terms/"
    xmlns:rdf="http://www.w3.org/1999/02/22-rdf-syntax-ns#"
    xmlns:dc="http://purl.org/dc/elements/1.1/"
    xmlns:owl="http://www.w3.org/2002/07/owl#"
    xmlns:dcmit="http://purl.org/dc/dcmitype/"
    xmlns:skos="http://www.w3.org/2004/02/skos/core#"
    xmlns:voaf="http://purl.org/vocommons/voaf#"
    xmlns:rdfs="http://www.w3.org/2000/01/rdf-schema#"
    xmlns:vann="http://purl.org/vocab/vann/">
  <owl:Ontology rdf:about="http://www.aktors.org/ontology/portal"/>
  <owl:ObjectProperty rdf:about="http://www.aktors.org/ontology/portal#has-size">
    <rdfs:isDefinedBy rdf:resource="http://www.aktors.org/ontology/portal"/>
    <rdfs:range>
      <skos:ConceptScheme rdf:about="http://www.aktors.org/ontology/portal#Organization-Size">
        <rdfs:isDefinedBy rdf:resource="http://www.aktors.org/ontology/portal"/>
      </skos:ConceptScheme>
    </rdfs:range>
  </owl:ObjectProperty>
  <skos:Concept rdf:about="http://www.aktors.org/ontology/portal#small-size">
    <rdfs:isDefinedBy rdf:resource="http://www.aktors.org/ontology/portal"/>
    <rdfs:label>small</rdfs:label>
    <rdfs:comment>An organization with no more than 50 employees.  It also has to be independent, i.e., less than 25% owned by one enterprise (or jointly by several enterprises) falling outside the definition of small-sized enterprise. Finally, either the turnover total must be less than 7M Euros or the balance sheet total must be less than 5M Euros.</rdfs:comment>
    <skos:inScheme rdf:resource="http://www.aktors.org/ontology/portal#Organization-Size"/>
  </skos:Concept>
  <skos:Concept rdf:about="http://www.aktors.org/ontology/portal#very-large-size">
    <rdfs:isDefinedBy rdf:resource="http://www.aktors.org/ontology/portal"/>
    <rdfs:label>very large</rdfs:label>
    <rdfs:comment>An organization with over 10000 employees</rdfs:comment>
    <skos:inScheme rdf:resource="http://www.aktors.org/ontology/portal#Organization-Size"/>
  </skos:Concept>
  <skos:Concept rdf:about="http://www.aktors.org/ontology/portal#medium-size">
    <rdfs:isDefinedBy rdf:resource="http://www.aktors.org/ontology/portal"/>
    <rdfs:label>medium</rdfs:label>
    <rdfs:comment>An organization with no more than 250 employees.  It also has to be independent, i.e., less than 25% owned by one enterprise (or jointly by several enterprises) falling outside the definition of medium-sized enterprise. Finally, either the turnover total must be less than 40M Euros or the balance sheet total must be less than 27M Euros.</rdfs:comment>
    <skos:inScheme rdf:resource="http://www.aktors.org/ontology/portal#Organization-Size"/>
  </skos:Concept>
  <skos:Concept rdf:about="http://www.aktors.org/ontology/portal#large-size">
    <rdfs:isDefinedBy rdf:resource="http://www.aktors.org/ontology/portal"/>
    <rdfs:label>large</rdfs:label>
    <rdfs:comment>An organization with more than 250 employees</rdfs:comment>
    <skos:inScheme rdf:resource="http://www.aktors.org/ontology/portal#Organization-Size"/>
  </skos:Concept>
  <skos:Concept rdf:about="http://www.aktors.org/ontology/portal#micro-size">
    <rdfs:isDefinedBy rdf:resource="http://www.aktors.org/ontology/portal"/>
    <rdfs:label>micro</rdfs:label>
    <rdfs:comment>An organization with no more than 10 employees.  It also has to be independent, i.e., less than 25% owned by one enterprise (or jointly by several enterprises) falling outside the definition of micro-sized enterprise.</rdfs:comment>
    <skos:inScheme rdf:resource="http://www.aktors.org/ontology/portal#Organization-Size"/>
  </skos:Concept>
</rdf:RDF>
