<rdf:RDF
    xmlns:dct="http://purl.org/dc/terms/"
    xmlns:rdf="http://www.w3.org/1999/02/22-rdf-syntax-ns#"
    xmlns:dc="http://purl.org/dc/elements/1.1/"
    xmlns:owl="http://www.w3.org/2002/07/owl#"
    xmlns:dcmit="http://purl.org/dc/dcmitype/"
    xmlns:skos="http://www.w3.org/2004/02/skos/core#"
    xmlns:voaf="http://purl.org/vocommons/voaf#"
    xmlns:rdfs="http://www.w3.org/2000/01/rdf-schema#"
    xmlns:vann="http://purl.org/vocab/vann/">
  <owl:Ontology rdf:about="http://www.ebusiness-unibw.org/ontologies/consumerelectronics/v1"/>
  <owl:ObjectProperty rdf:about="http://www.ebusiness-unibw.org/ontologies/consumerelectronics/v1#hasSensorType">
    <rdfs:isDefinedBy rdf:resource="http://www.ebusiness-unibw.org/ontologies/consumerelectronics/v1"/>
    <rdfs:comment xml:lang="en">Defines type of device that measures a physical quantity and converts it into a signal which can be read by an observer or by an instrument.</rdfs:comment>
    <rdfs:label xml:lang="en">sensor type</rdfs:label>
    <rdfs:range>
      <skos:ConceptScheme rdf:about="http://www.ebusiness-unibw.org/ontologies/consumerelectronics/v1#SensorType">
        <rdfs:isDefinedBy rdf:resource="http://www.ebusiness-unibw.org/ontologies/consumerelectronics/v1"/>
        <rdfs:label xml:lang="en">Type of device that measures a physical quantity and converts it into a signal which can be read by an observer or by an instrument.

(This description is partly based on or reuses content from the Wikipedia article "Sensor" (http://en.wikipedia.org/wiki/Sensor) and is licensed under the GNU Free Documentation License (http://www.gnu.org/copyleft/fdl.html).)</rdfs:label>
        <rdfs:comment xml:lang="en">Type of device that measures a physical quantity and converts it into a signal which can be read by an observer or by an instrument.

(This description is partly based on or reuses content from the Wikipedia article "Sensor" (http://en.wikipedia.org/wiki/Sensor) and is licensed under the GNU Free Documentation License (http://www.gnu.org/copyleft/fdl.html).)</rdfs:comment>
      </skos:ConceptScheme>
    </rdfs:range>
  </owl:ObjectProperty>
  <skos:Concept rdf:about="http://www.ebusiness-unibw.org/ontologies/consumerelectronics/v1#SensorType_3CCD">
    <rdfs:isDefinedBy rdf:resource="http://www.ebusiness-unibw.org/ontologies/consumerelectronics/v1"/>
    <rdfs:label xml:lang="en">Three-CCD</rdfs:label>
    <rdfs:comment xml:lang="en">3CCD is a term used to describe an imaging system employed by some still cameras, video cameras, telecine and camcorders.

(This description is partly based on or reuses content from the Wikipedia article "Three-CCD" (http://en.wikipedia.org/wiki/Three-CCD) and is licensed under the GNU Free Documentation License (http://www.gnu.org/copyleft/fdl.html).)</rdfs:comment>
    <skos:inScheme rdf:resource="http://www.ebusiness-unibw.org/ontologies/consumerelectronics/v1#SensorType"/>
  </skos:Concept>
  <skos:Concept rdf:about="http://www.ebusiness-unibw.org/ontologies/consumerelectronics/v1#CMOS">
    <rdfs:isDefinedBy rdf:resource="http://www.ebusiness-unibw.org/ontologies/consumerelectronics/v1"/>
    <rdfs:label xml:lang="en">CMOS</rdfs:label>
    <rdfs:comment xml:lang="en">Complementary metal-oxide-semiconductor (CMOS) (pronounced "see-moss", IPA: /ˈsiːmɒs/), is a major class of integrated circuits. CMOS technology is used in microprocessors, microcontrollers, static RAM, and other digital logic circuits. CMOS technology is also used for a wide variety of analog circuits such as image sensors, data converters, and highly integrated transceivers for many types of communication. Frank Wanlass successfully patented CMOS in 1967 (US Patent 3,356,858).

(This description is partly based on or reuses content from the Wikipedia article "CMOS" (http://en.wikipedia.org/wiki/CMOS) and is licensed under the GNU Free Documentation License (http://www.gnu.org/copyleft/fdl.html).)</rdfs:comment>
    <skos:inScheme rdf:resource="http://www.ebusiness-unibw.org/ontologies/consumerelectronics/v1#SensorType"/>
  </skos:Concept>
</rdf:RDF>
