<rdf:RDF
    xmlns:dct="http://purl.org/dc/terms/"
    xmlns:rdf="http://www.w3.org/1999/02/22-rdf-syntax-ns#"
    xmlns:dc="http://purl.org/dc/elements/1.1/"
    xmlns:owl="http://www.w3.org/2002/07/owl#"
    xmlns:dcmit="http://purl.org/dc/dcmitype/"
    xmlns:skos="http://www.w3.org/2004/02/skos/core#"
    xmlns:voaf="http://purl.org/vocommons/voaf#"
    xmlns:rdfs="http://www.w3.org/2000/01/rdf-schema#"
    xmlns:vann="http://purl.org/vocab/vann/">
  <owl:Ontology rdf:about="http://www.ebusiness-unibw.org/ontologies/consumerelectronics/v1"/>
  <skos:Concept rdf:about="http://www.ebusiness-unibw.org/ontologies/consumerelectronics/v1#GameMode">
    <rdfs:isDefinedBy rdf:resource="http://www.ebusiness-unibw.org/ontologies/consumerelectronics/v1"/>
    <rdfs:label xml:lang="en">Game mode</rdfs:label>
    <rdfs:comment xml:lang="en">A special mode providing more performance of the television to optimize pictures when games are played on a LCD or plasma panel.</rdfs:comment>
    <skos:inScheme>
      <skos:ConceptScheme rdf:about="http://www.ebusiness-unibw.org/ontologies/consumerelectronics/v1#GeneralFeatures">
        <rdfs:isDefinedBy rdf:resource="http://www.ebusiness-unibw.org/ontologies/consumerelectronics/v1"/>
      </skos:ConceptScheme>
    </skos:inScheme>
  </skos:Concept>
  <skos:Concept rdf:about="http://www.ebusiness-unibw.org/ontologies/consumerelectronics/v1#AutoChannelSearch">
    <rdfs:isDefinedBy rdf:resource="http://www.ebusiness-unibw.org/ontologies/consumerelectronics/v1"/>
    <rdfs:label xml:lang="en">Auto channel search</rdfs:label>
    <rdfs:comment xml:lang="en">Gives an indication of preprogrammed channels for the user of a television so that he does not need to programm it himself.</rdfs:comment>
    <skos:inScheme rdf:resource="http://www.ebusiness-unibw.org/ontologies/consumerelectronics/v1#GeneralFeatures"/>
  </skos:Concept>
  <skos:Concept rdf:about="http://www.ebusiness-unibw.org/ontologies/consumerelectronics/v1#OnScreenDisplay">
    <rdfs:isDefinedBy rdf:resource="http://www.ebusiness-unibw.org/ontologies/consumerelectronics/v1"/>
    <rdfs:label xml:lang="en">on screen display</rdfs:label>
    <rdfs:comment xml:lang="en">An on-screen display (abbreviated OSD) is an image superimposed on a screen picture, commonly used by modern televisions, VCRs, and DVD players to display information such as volume, channel, and time.

(This description is partly based on or reuses content from the Wikipedia article "On-screen display" (http://en.wikipedia.org/wiki/On-screen_display) and is licensed under the GNU Free Documentation License (http://www.gnu.org/copyleft/fdl.html).)</rdfs:comment>
    <skos:inScheme rdf:resource="http://www.ebusiness-unibw.org/ontologies/consumerelectronics/v1#GeneralFeatures"/>
  </skos:Concept>
  <skos:Concept rdf:about="http://www.ebusiness-unibw.org/ontologies/consumerelectronics/v1#PowerLED">
    <rdfs:isDefinedBy rdf:resource="http://www.ebusiness-unibw.org/ontologies/consumerelectronics/v1"/>
    <rdfs:label xml:lang="en">Power LED</rdfs:label>
    <rdfs:comment xml:lang="en">It is a semiconductor diode that emits light when an electric current is applied in the forward direction of the device used to show the power status of an electrical device.

(This description is partly based on or reuses content from the Wikipedia article "LED" (http://en.wikipedia.org/wiki/Led) and is licensed under the GNU Free Documentation License (http://www.gnu.org/copyleft/fdl.html).)</rdfs:comment>
    <skos:inScheme rdf:resource="http://www.ebusiness-unibw.org/ontologies/consumerelectronics/v1#GeneralFeatures"/>
  </skos:Concept>
  <skos:Concept rdf:about="http://www.ebusiness-unibw.org/ontologies/consumerelectronics/v1#IntegratedClock">
    <rdfs:isDefinedBy rdf:resource="http://www.ebusiness-unibw.org/ontologies/consumerelectronics/v1"/>
    <rdfs:label xml:lang="en">Integrated clock</rdfs:label>
    <rdfs:comment xml:lang="en">Clock integrated in a device.</rdfs:comment>
    <skos:inScheme rdf:resource="http://www.ebusiness-unibw.org/ontologies/consumerelectronics/v1#GeneralFeatures"/>
  </skos:Concept>
  <skos:Concept rdf:about="http://www.ebusiness-unibw.org/ontologies/consumerelectronics/v1#SleepTimer">
    <rdfs:isDefinedBy rdf:resource="http://www.ebusiness-unibw.org/ontologies/consumerelectronics/v1"/>
    <rdfs:label xml:lang="en">Sleep timer</rdfs:label>
    <rdfs:comment xml:lang="en">A sleep timer is a function on many modern televisions that shut off the power after a preset amount of time. The setting is usually made either from the remote control or the television menus. They are intended to allow viewers to watch as they fall asleep.

(This description is partly based on or reuses content from the Wikipedia article "Sleep timer" (http://en.wikipedia.org/wiki/Sleep_timer) and is licensed under the GNU Free Documentation License (http://www.gnu.org/copyleft/fdl.html).)</rdfs:comment>
    <skos:inScheme rdf:resource="http://www.ebusiness-unibw.org/ontologies/consumerelectronics/v1#GeneralFeatures"/>
  </skos:Concept>
  <skos:Concept rdf:about="http://www.ebusiness-unibw.org/ontologies/consumerelectronics/v1#StandbyLED">
    <rdfs:isDefinedBy rdf:resource="http://www.ebusiness-unibw.org/ontologies/consumerelectronics/v1"/>
    <rdfs:label xml:lang="en">Standby LED</rdfs:label>
    <rdfs:comment xml:lang="en">It is a semiconductor diode that emits light when an electric current is applied in the forward direction of the device used to show the standby status of an electrical device.

(This description is partly based on or reuses content from the Wikipedia article "LED" (http://en.wikipedia.org/wiki/Led) and is licensed under the GNU Free Documentation License (http://www.gnu.org/copyleft/fdl.html).)</rdfs:comment>
    <skos:inScheme rdf:resource="http://www.ebusiness-unibw.org/ontologies/consumerelectronics/v1#GeneralFeatures"/>
  </skos:Concept>
  <skos:Concept rdf:about="http://www.ebusiness-unibw.org/ontologies/consumerelectronics/v1#ChildSafetyLock">
    <rdfs:isDefinedBy rdf:resource="http://www.ebusiness-unibw.org/ontologies/consumerelectronics/v1"/>
    <rdfs:label xml:lang="en">Child safety lock</rdfs:label>
    <rdfs:comment xml:lang="en">A child safety lock is a special-purpose lock that is designed to help prevent children from getting at any dangerous contents.

(This description is partly based on or reuses content from the Wikipedia article "Child safety lock" (http://en.wikipedia.org/wiki/Child_safety_lock) and is licensed under the GNU Free Documentation License (http://www.gnu.org/copyleft/fdl.html).)</rdfs:comment>
    <skos:inScheme rdf:resource="http://www.ebusiness-unibw.org/ontologies/consumerelectronics/v1#GeneralFeatures"/>
  </skos:Concept>
  <skos:Concept rdf:about="http://www.ebusiness-unibw.org/ontologies/consumerelectronics/v1#OnOffTimer">
    <rdfs:isDefinedBy rdf:resource="http://www.ebusiness-unibw.org/ontologies/consumerelectronics/v1"/>
    <rdfs:label xml:lang="en">On off timer</rdfs:label>
    <rdfs:comment xml:lang="en">Describes the possibility to maintain a designated  time when the television or electrical device should be switched off or on automatically.</rdfs:comment>
    <skos:inScheme rdf:resource="http://www.ebusiness-unibw.org/ontologies/consumerelectronics/v1#GeneralFeatures"/>
  </skos:Concept>
  <skos:Concept rdf:about="http://www.ebusiness-unibw.org/ontologies/consumerelectronics/v1#Anti-ReflectionCoatedScreen">
    <rdfs:isDefinedBy rdf:resource="http://www.ebusiness-unibw.org/ontologies/consumerelectronics/v1"/>
    <rdfs:label xml:lang="en">Anti-reflection coated screen</rdfs:label>
    <rdfs:comment xml:lang="en">The screen has a short persistence phosphor with an anti-reflection and anti-static coating.</rdfs:comment>
    <skos:inScheme rdf:resource="http://www.ebusiness-unibw.org/ontologies/consumerelectronics/v1#GeneralFeatures"/>
  </skos:Concept>
  <skos:Concept rdf:about="http://www.ebusiness-unibw.org/ontologies/consumerelectronics/v1#EPG">
    <rdfs:isDefinedBy rdf:resource="http://www.ebusiness-unibw.org/ontologies/consumerelectronics/v1"/>
    <rdfs:label xml:lang="en">EPG</rdfs:label>
    <rdfs:comment xml:lang="en">An electronic program(me) guide (EPG) or interactive program(me) guide (IPG) or electronic service guide (ESG) is an digital guide to scheduled broadcast television or radio programs, typically displayed on-screen with functions allowing a viewer to navigate, select, and discover content by time, title, channel, genre, etc. by use of their remote control, a keyboard, or other input devices such as a phone keypad.

(This description is partly based on or reuses content from the Wikipedia article "Electronic program guide" (http://en.wikipedia.org/wiki/Electronic_program_guide) and is licensed under the GNU Free Documentation License (http://www.gnu.org/copyleft/fdl.html).)</rdfs:comment>
    <skos:inScheme rdf:resource="http://www.ebusiness-unibw.org/ontologies/consumerelectronics/v1#GeneralFeatures"/>
  </skos:Concept>
  <skos:Concept rdf:about="http://www.ebusiness-unibw.org/ontologies/consumerelectronics/v1#TeletextFunction">
    <rdfs:isDefinedBy rdf:resource="http://www.ebusiness-unibw.org/ontologies/consumerelectronics/v1"/>
    <rdfs:label xml:lang="en">Teletext function</rdfs:label>
    <rdfs:comment xml:lang="en">Teletext (or "broadcast Teletext") is a television information retrieval service developed in the United Kingdom in the early 1970s. It offers a range of text-based information, typically including national, international and sporting news, weather and TV schedules.

(This description is partly based on or reuses content from the Wikipedia article "Teletext" (http://en.wikipedia.org/wiki/Teletext) and is licensed under the GNU Free Documentation License (http://www.gnu.org/copyleft/fdl.html).)</rdfs:comment>
    <skos:inScheme rdf:resource="http://www.ebusiness-unibw.org/ontologies/consumerelectronics/v1#GeneralFeatures"/>
  </skos:Concept>
  <skos:Concept rdf:about="http://www.ebusiness-unibw.org/ontologies/consumerelectronics/v1#FirmwareUpgradable">
    <rdfs:isDefinedBy rdf:resource="http://www.ebusiness-unibw.org/ontologies/consumerelectronics/v1"/>
    <rdfs:label xml:lang="en">Firmware upgradable</rdfs:label>
    <rdfs:comment xml:lang="en">The term upgrade refers to the replacement of a product with a newer version of that same product, here it is the replacement of the firmware with a newer version of it.</rdfs:comment>
    <skos:inScheme rdf:resource="http://www.ebusiness-unibw.org/ontologies/consumerelectronics/v1#GeneralFeatures"/>
  </skos:Concept>
  <skos:Concept rdf:about="http://www.ebusiness-unibw.org/ontologies/consumerelectronics/v1#PlugAndPlay">
    <rdfs:isDefinedBy rdf:resource="http://www.ebusiness-unibw.org/ontologies/consumerelectronics/v1"/>
    <rdfs:label xml:lang="en">Plug and Play</rdfs:label>
    <rdfs:comment xml:lang="en">Describes any hardware specification that alleviates the need for user configuration of device resources.

(This description is partly based on or reuses content from the Wikipedia article "Legacy Plug and Play" (http://en.wikipedia.org/wiki/Legacy_Plug_and_Play) and is licensed under the GNU Free Documentation License (http://www.gnu.org/copyleft/fdl.html).)</rdfs:comment>
    <skos:inScheme rdf:resource="http://www.ebusiness-unibw.org/ontologies/consumerelectronics/v1#GeneralFeatures"/>
  </skos:Concept>
  <skos:Concept rdf:about="http://www.ebusiness-unibw.org/ontologies/consumerelectronics/v1#Timer">
    <rdfs:isDefinedBy rdf:resource="http://www.ebusiness-unibw.org/ontologies/consumerelectronics/v1"/>
    <rdfs:label xml:lang="en">Timer</rdfs:label>
    <rdfs:comment xml:lang="en">A timer is a specialized type of clock counting backwards to a predefined end.

(This description is partly based on or reuses content from the Wikipedia article "Timer" (http://en.wikipedia.org/wiki/Timer) and is licensed under the GNU Free Documentation License (http://www.gnu.org/copyleft/fdl.html).)</rdfs:comment>
    <skos:inScheme rdf:resource="http://www.ebusiness-unibw.org/ontologies/consumerelectronics/v1#GeneralFeatures"/>
  </skos:Concept>
  <skos:Concept rdf:about="http://www.ebusiness-unibw.org/ontologies/consumerelectronics/v1#CommonInterface">
    <rdfs:isDefinedBy rdf:resource="http://www.ebusiness-unibw.org/ontologies/consumerelectronics/v1"/>
    <rdfs:label xml:lang="en">Common interface</rdfs:label>
    <rdfs:comment xml:lang="en">The Common Interface is an extensible digital interconnect found in the digital TV market.

(This description is partly based on or reuses content from the Wikipedia article "Common Interface" (http://en.wikipedia.org/wiki/Common_Interface) and is licensed under the GNU Free Documentation License (http://www.gnu.org/copyleft/fdl.html).)</rdfs:comment>
    <skos:inScheme rdf:resource="http://www.ebusiness-unibw.org/ontologies/consumerelectronics/v1#GeneralFeatures"/>
  </skos:Concept>
  <skos:Concept rdf:about="http://www.ebusiness-unibw.org/ontologies/consumerelectronics/v1#DVB-T">
    <rdfs:isDefinedBy rdf:resource="http://www.ebusiness-unibw.org/ontologies/consumerelectronics/v1"/>
    <rdfs:label xml:lang="en">DVB-T</rdfs:label>
    <rdfs:comment xml:lang="en">DVB-T is an abbreviation for Digital Video Broadcasting - Terrestrial; it is the DVB European-based consortium standard for the broadcast transmission of digital terrestrial television. This system transmits compressed digital audio, video and other data in an MPEG transport stream, using COFDM modulation.

(This description is partly based on or reuses content from the Wikipedia article "DVB-T" (http://en.wikipedia.org/wiki/DVB-T) and is licensed under the GNU Free Documentation License (http://www.gnu.org/copyleft/fdl.html).)</rdfs:comment>
    <skos:inScheme rdf:resource="http://www.ebusiness-unibw.org/ontologies/consumerelectronics/v1#GeneralFeatures"/>
  </skos:Concept>
</rdf:RDF>
