<rdf:RDF
    xmlns:dct="http://purl.org/dc/terms/"
    xmlns:rdf="http://www.w3.org/1999/02/22-rdf-syntax-ns#"
    xmlns:dc="http://purl.org/dc/elements/1.1/"
    xmlns:owl="http://www.w3.org/2002/07/owl#"
    xmlns:dcmit="http://purl.org/dc/dcmitype/"
    xmlns:skos="http://www.w3.org/2004/02/skos/core#"
    xmlns:voaf="http://purl.org/vocommons/voaf#"
    xmlns:rdfs="http://www.w3.org/2000/01/rdf-schema#"
    xmlns:vann="http://purl.org/vocab/vann/">
  <owl:Ontology rdf:about="http://www.ebusiness-unibw.org/ontologies/consumerelectronics/v1"/>
  <skos:Concept rdf:about="http://www.ebusiness-unibw.org/ontologies/consumerelectronics/v1#PictureInPicture">
    <rdfs:isDefinedBy rdf:resource="http://www.ebusiness-unibw.org/ontologies/consumerelectronics/v1"/>
    <rdfs:label xml:lang="en">Picture in Picture</rdfs:label>
    <rdfs:comment xml:lang="en">Picture in Picture (PiP) is a feature of some television receivers and similar devices. One program (channel) is displayed on the full TV screen at the same time as one or more other programs are displayed in inset windows. Sound is usually from the main program only.

(This description is partly based on or reuses content from the Wikipedia article "Picture in picture" (http://en.wikipedia.org/wiki/Picture-in-picture) and is licensed under the GNU Free Documentation License (http://www.gnu.org/copyleft/fdl.html).)</rdfs:comment>
    <skos:inScheme>
      <skos:ConceptScheme rdf:about="http://www.ebusiness-unibw.org/ontologies/consumerelectronics/v1#VideoFeatures">
        <rdfs:isDefinedBy rdf:resource="http://www.ebusiness-unibw.org/ontologies/consumerelectronics/v1"/>
        <rdfs:label xml:lang="en">Additional video equipment and abilities.</rdfs:label>
        <rdfs:comment xml:lang="en">Additional video equipment and abilities.</rdfs:comment>
      </skos:ConceptScheme>
    </skos:inScheme>
  </skos:Concept>
  <skos:Concept rdf:about="http://www.ebusiness-unibw.org/ontologies/consumerelectronics/v1#AmbilightSpectraActiveFrame">
    <rdfs:isDefinedBy rdf:resource="http://www.ebusiness-unibw.org/ontologies/consumerelectronics/v1"/>
    <rdfs:label xml:lang="en">Ambilight Spectra Active Frame</rdfs:label>
    <rdfs:comment xml:lang="en">Active Frame is a single soft halo of light powered by 126 LEDs.</rdfs:comment>
    <skos:inScheme rdf:resource="http://www.ebusiness-unibw.org/ontologies/consumerelectronics/v1#VideoFeatures"/>
  </skos:Concept>
  <skos:Concept rdf:about="http://www.ebusiness-unibw.org/ontologies/consumerelectronics/v1#CombFilter">
    <rdfs:isDefinedBy rdf:resource="http://www.ebusiness-unibw.org/ontologies/consumerelectronics/v1"/>
    <rdfs:label xml:lang="en">Comb filter</rdfs:label>
    <rdfs:comment xml:lang="en">In signal processing, a comb filter adds a delayed version of a signal to itself, causing constructive and destructive interference. The frequency response of a comb filter consists of a series of regularly-spaced spikes, giving the appearance of a comb.

(This description is partly based on or reuses content from the Wikipedia article "Comb filter" (http://en.wikipedia.org/wiki/Comb_filter) and is licensed under the GNU Free Documentation License (http://www.gnu.org/copyleft/fdl.html).)</rdfs:comment>
    <skos:inScheme rdf:resource="http://www.ebusiness-unibw.org/ontologies/consumerelectronics/v1#VideoFeatures"/>
  </skos:Concept>
  <skos:Concept rdf:about="http://www.ebusiness-unibw.org/ontologies/consumerelectronics/v1#DigitalImageScalingTechnology">
    <rdfs:isDefinedBy rdf:resource="http://www.ebusiness-unibw.org/ontologies/consumerelectronics/v1"/>
    <rdfs:label xml:lang="en">Digital Image Scaling Technology</rdfs:label>
    <rdfs:comment xml:lang="en">Seamlessly up-scales any video source to display at full high definition 1080p.</rdfs:comment>
    <skos:inScheme rdf:resource="http://www.ebusiness-unibw.org/ontologies/consumerelectronics/v1#VideoFeatures"/>
  </skos:Concept>
  <skos:Concept rdf:about="http://www.ebusiness-unibw.org/ontologies/consumerelectronics/v1#ContrastPlus">
    <rdfs:isDefinedBy rdf:resource="http://www.ebusiness-unibw.org/ontologies/consumerelectronics/v1"/>
    <rdfs:label xml:lang="en">Contrast Plus</rdfs:label>
    <rdfs:comment xml:lang="en">Ensures that, according to the scene, the screen always displays the best possible contrast. This results in a depth of focus, which lends an extraordinary power to the television image, making it appear almost touchable.</rdfs:comment>
    <skos:inScheme rdf:resource="http://www.ebusiness-unibw.org/ontologies/consumerelectronics/v1#VideoFeatures"/>
  </skos:Concept>
  <skos:Concept rdf:about="http://www.ebusiness-unibw.org/ontologies/consumerelectronics/v1#AmbilightSpectra3">
    <rdfs:isDefinedBy rdf:resource="http://www.ebusiness-unibw.org/ontologies/consumerelectronics/v1"/>
    <rdfs:label xml:lang="en">Ambilight Spectra 3</rdfs:label>
    <rdfs:comment xml:lang="en">Enlarges the screen further by projecting a glow of light from the back of the screen onto the surrounding wall. Ambilight adjusts automatically the colour and brightness of the light surrounding the TV to match with the picture.</rdfs:comment>
    <skos:inScheme rdf:resource="http://www.ebusiness-unibw.org/ontologies/consumerelectronics/v1#VideoFeatures"/>
  </skos:Concept>
  <skos:Concept rdf:about="http://www.ebusiness-unibw.org/ontologies/consumerelectronics/v1#PixelPlus3HD">
    <rdfs:isDefinedBy rdf:resource="http://www.ebusiness-unibw.org/ontologies/consumerelectronics/v1"/>
    <rdfs:label xml:lang="en">Pixel Plus 3 HD</rdfs:label>
    <rdfs:comment xml:lang="en">Pixel Plus 3 HD offers the unique combination of ultimate sharpness, natural detail, vivid colours and smooth natural motion on all qualities of HD, standard TV signals and multimedia content for high definition displays. Each pixel of the incoming picture is enhanced to better match the surrounding pixels, resulting in a more natural picture. Artefacts and noise in all sources from multimedia to standard TV and also in highly compressed HD are detected and reduced.</rdfs:comment>
    <skos:inScheme rdf:resource="http://www.ebusiness-unibw.org/ontologies/consumerelectronics/v1#VideoFeatures"/>
  </skos:Concept>
  <skos:Concept rdf:about="http://www.ebusiness-unibw.org/ontologies/consumerelectronics/v1#PixelPlusHD">
    <rdfs:isDefinedBy rdf:resource="http://www.ebusiness-unibw.org/ontologies/consumerelectronics/v1"/>
    <rdfs:label xml:lang="en">Pixel Plus HD</rdfs:label>
    <rdfs:comment xml:lang="en">Pixel Plus HD is a picture processing technology that enables viewers to watch content that is vivid, natural and real.</rdfs:comment>
    <skos:inScheme rdf:resource="http://www.ebusiness-unibw.org/ontologies/consumerelectronics/v1#VideoFeatures"/>
  </skos:Concept>
  <skos:Concept rdf:about="http://www.ebusiness-unibw.org/ontologies/consumerelectronics/v1#ProgressiveScan">
    <rdfs:isDefinedBy rdf:resource="http://www.ebusiness-unibw.org/ontologies/consumerelectronics/v1"/>
    <rdfs:label xml:lang="en">Progressive Scan</rdfs:label>
    <rdfs:comment xml:lang="en">Progressive or noninterlaced scanning is a method for displaying, storing or transmitting moving images in which all the lines of each frame are drawn in sequence.

(This description is partly based on or reuses content from the Wikipedia article "Progressive scan" (http://en.wikipedia.org/wiki/Progressive_scan) and is licensed under the GNU Free Documentation License (http://www.gnu.org/copyleft/fdl.html).)</rdfs:comment>
    <skos:inScheme rdf:resource="http://www.ebusiness-unibw.org/ontologies/consumerelectronics/v1#VideoFeatures"/>
  </skos:Concept>
  <skos:Concept rdf:about="http://www.ebusiness-unibw.org/ontologies/consumerelectronics/v1#PerfectPixelHD">
    <rdfs:isDefinedBy rdf:resource="http://www.ebusiness-unibw.org/ontologies/consumerelectronics/v1"/>
    <rdfs:label xml:lang="en">Perfect Pixel HD</rdfs:label>
    <rdfs:comment xml:lang="en">Perfect Pixel HD Engine offers the unique combination of ultimate sharpness, natural detail, vivid colours and smooth natural motion on all qualities of HD, standard TV signals and multimedia content, for high definition displays. Each pixel of the incoming picture is enhanced to better match the surrounding pixels, resulting in a more natural picture.</rdfs:comment>
    <skos:inScheme rdf:resource="http://www.ebusiness-unibw.org/ontologies/consumerelectronics/v1#VideoFeatures"/>
  </skos:Concept>
  <skos:Concept rdf:about="http://www.ebusiness-unibw.org/ontologies/consumerelectronics/v1#FullHD">
    <rdfs:isDefinedBy rdf:resource="http://www.ebusiness-unibw.org/ontologies/consumerelectronics/v1"/>
    <rdfs:label xml:lang="en">Full HD</rdfs:label>
    <rdfs:comment xml:lang="en">Usually assumes a widescreen aspect ratio of 16:9, implying a horizontal resolution of 1920 pixels. This creates a frame resolution of 1920Ã—1080, or 2,073,600 pixels in total.

(This description is partly based on or reuses content from the Wikipedia article "1080p" (http://en.wikipedia.org/wiki/1080p) and is licensed under the GNU Free Documentation License (http://www.gnu.org/copyleft/fdl.html).)</rdfs:comment>
    <skos:inScheme rdf:resource="http://www.ebusiness-unibw.org/ontologies/consumerelectronics/v1#VideoFeatures"/>
  </skos:Concept>
  <skos:Concept rdf:about="http://www.ebusiness-unibw.org/ontologies/consumerelectronics/v1#AmbilightSpectra2">
    <rdfs:isDefinedBy rdf:resource="http://www.ebusiness-unibw.org/ontologies/consumerelectronics/v1"/>
    <rdfs:label xml:lang="en">Ambilight Spectra 2</rdfs:label>
    <rdfs:comment xml:lang="en">Ambilight Spectra 2 generates reactive ambient lighting on both sides of a Flat TV.</rdfs:comment>
    <skos:inScheme rdf:resource="http://www.ebusiness-unibw.org/ontologies/consumerelectronics/v1#VideoFeatures"/>
  </skos:Concept>
  <skos:Concept rdf:about="http://www.ebusiness-unibw.org/ontologies/consumerelectronics/v1#DigitalCrystalClear">
    <rdfs:isDefinedBy rdf:resource="http://www.ebusiness-unibw.org/ontologies/consumerelectronics/v1"/>
    <rdfs:label xml:lang="en">Digital Crystal Clear</rdfs:label>
    <rdfs:comment xml:lang="en">Digital Crystal Clear is a package of picture innovations that digitally adjusts and optimises picture quality to optimal contrast, colour and sharpness levels.</rdfs:comment>
    <skos:inScheme rdf:resource="http://www.ebusiness-unibw.org/ontologies/consumerelectronics/v1#VideoFeatures"/>
  </skos:Concept>
  <skos:Concept rdf:about="http://www.ebusiness-unibw.org/ontologies/consumerelectronics/v1#Acuity">
    <rdfs:isDefinedBy rdf:resource="http://www.ebusiness-unibw.org/ontologies/consumerelectronics/v1"/>
    <rdfs:label xml:lang="en">Acuity</rdfs:label>
    <rdfs:comment xml:lang="en">Is acuteness or clearness of vision, especially form vision, which is dependent on the sharpness of the retinal focus within the eye and the sensitivity of the interpretative faculty of the brain.

(This description is partly based on or reuses content from the Wikipedia article "Visual acuity" (http://en.wikipedia.org/wiki/Visual_acuity) and is licensed under the GNU Free Documentation License (http://www.gnu.org/copyleft/fdl.html).)</rdfs:comment>
    <skos:inScheme rdf:resource="http://www.ebusiness-unibw.org/ontologies/consumerelectronics/v1#VideoFeatures"/>
  </skos:Concept>
  <skos:Concept rdf:about="http://www.ebusiness-unibw.org/ontologies/consumerelectronics/v1#PixelPlus2">
    <rdfs:isDefinedBy rdf:resource="http://www.ebusiness-unibw.org/ontologies/consumerelectronics/v1"/>
    <rdfs:label xml:lang="en">Pixelplus 2</rdfs:label>
    <rdfs:comment xml:lang="en">Pixelplus 2 is a technology which allows motion reinterpolation on 480p and 576p material.</rdfs:comment>
    <skos:inScheme rdf:resource="http://www.ebusiness-unibw.org/ontologies/consumerelectronics/v1#VideoFeatures"/>
  </skos:Concept>
  <skos:Concept rdf:about="http://www.ebusiness-unibw.org/ontologies/consumerelectronics/v1#ScreenFormatAdjustments">
    <rdfs:isDefinedBy rdf:resource="http://www.ebusiness-unibw.org/ontologies/consumerelectronics/v1"/>
    <rdfs:label xml:lang="en">Screen format adjustments</rdfs:label>
    <rdfs:comment xml:lang="en">Includes the possibility to switch between different screen formats.</rdfs:comment>
    <skos:inScheme rdf:resource="http://www.ebusiness-unibw.org/ontologies/consumerelectronics/v1#VideoFeatures"/>
  </skos:Concept>
  <skos:Concept rdf:about="http://www.ebusiness-unibw.org/ontologies/consumerelectronics/v1#Ambilight1">
    <rdfs:label rdf:datatype="http://www.w3.org/2001/XMLSchema#string"
    >Ambilight 1</rdfs:label>
    <rdfs:isDefinedBy rdf:resource="http://www.ebusiness-unibw.org/ontologies/consumerelectronics/v1"/>
    <rdfs:label xml:lang="en">Ambilight 1</rdfs:label>
    <rdfs:comment xml:lang="en">Ambilight, which is short for Ambient Lighting Technology, is a feature invented by Philips Electronics, generating light effects around the TV that correspond to the video content.

(This description is partly based on or reuses content from the Wikipedia article "Ambilight" (http://en.wikipedia.org/wiki/Ambilight) and is licensed under the GNU Free Documentation License (http://www.gnu.org/copyleft/fdl.html).)</rdfs:comment>
    <skos:inScheme rdf:resource="http://www.ebusiness-unibw.org/ontologies/consumerelectronics/v1#VideoFeatures"/>
  </skos:Concept>
</rdf:RDF>
