<rdf:RDF
    xmlns:dct="http://purl.org/dc/terms/"
    xmlns:rdf="http://www.w3.org/1999/02/22-rdf-syntax-ns#"
    xmlns:dc="http://purl.org/dc/elements/1.1/"
    xmlns:owl="http://www.w3.org/2002/07/owl#"
    xmlns:dcmit="http://purl.org/dc/dcmitype/"
    xmlns:skos="http://www.w3.org/2004/02/skos/core#"
    xmlns:voaf="http://purl.org/vocommons/voaf#"
    xmlns:rdfs="http://www.w3.org/2000/01/rdf-schema#"
    xmlns:vann="http://purl.org/vocab/vann/">
  <skos:Concept rdf:about="http://www.ebusiness-unibw.org/ontologies/consumerelectronics/v1#Format5.1ch">
    <rdfs:label xml:lang="en">Format 5.1ch</rdfs:label>
    <rdfs:comment xml:lang="en">Encompasses a range of techniques for enriching (expanding and deepening) the sound reproduction quality, of an audio source, with additional audio channels reproduced via additional, discrete speakers.</rdfs:comment>
    <skos:inScheme>
      <skos:ConceptScheme rdf:about="http://www.ebusiness-unibw.org/ontologies/consumerelectronics/v1#DataFormatAudio"/>
    </skos:inScheme>
  </skos:Concept>
  <skos:Concept rdf:about="http://www.ebusiness-unibw.org/ontologies/consumerelectronics/v1#AIFF">
    <rdfs:label xml:lang="en">AIFF</rdfs:label>
    <rdfs:comment xml:lang="en">Audio Interchange File Format (AIFF) is an audio file format standard used for storing sound data for personal computers and other electronic audio devices.

(This description is partly based on or reuses content from the Wikipedia article "Audio Interchange File Format" (http://en.wikipedia.org/wiki/Audio_Interchange_File_Format) and is licensed under the GNU Free Documentation License (http://www.gnu.org/copyleft/fdl.html).)</rdfs:comment>
    <skos:inScheme rdf:resource="http://www.ebusiness-unibw.org/ontologies/consumerelectronics/v1#DataFormatAudio"/>
  </skos:Concept>
  <skos:Concept rdf:about="http://www.ebusiness-unibw.org/ontologies/consumerelectronics/v1#WMA">
    <rdfs:label xml:lang="en">WMA</rdfs:label>
    <rdfs:comment xml:lang="en">An audio data compression technology developed by Microsoft.</rdfs:comment>
    <skos:inScheme rdf:resource="http://www.ebusiness-unibw.org/ontologies/consumerelectronics/v1#DataFormatAudio"/>
  </skos:Concept>
  <skos:Concept rdf:about="http://www.ebusiness-unibw.org/ontologies/consumerelectronics/v1#WAV">
    <rdfs:label xml:lang="en">WAV</rdfs:label>
    <rdfs:comment xml:lang="en">WAV (or WAVE), short for Waveform audio format, is a Microsoft and IBM audio file format standard for storing an audio bitstream on PCs.

(This description is partly based on or reuses content from the Wikipedia article "WAV" (http://en.wikipedia.org/wiki/WAV) and is licensed under the GNU Free Documentation License (http://www.gnu.org/copyleft/fdl.html).)</rdfs:comment>
    <skos:inScheme rdf:resource="http://www.ebusiness-unibw.org/ontologies/consumerelectronics/v1#DataFormatAudio"/>
  </skos:Concept>
  <skos:Concept rdf:about="http://www.ebusiness-unibw.org/ontologies/consumerelectronics/v1#MP4_Audio">
    <rdfs:label xml:lang="en">MP4 Audio</rdfs:label>
    <rdfs:comment xml:lang="en">A collection of methods defining compression of audio digital data.</rdfs:comment>
    <skos:inScheme rdf:resource="http://www.ebusiness-unibw.org/ontologies/consumerelectronics/v1#DataFormatAudio"/>
  </skos:Concept>
  <skos:Concept rdf:about="http://www.ebusiness-unibw.org/ontologies/consumerelectronics/v1#ALE">
    <rdfs:label xml:lang="en">ALE</rdfs:label>
    <rdfs:comment xml:lang="en">Apple Lossless (also known as Apple Lossless Encoder, ALE, or Apple Lossless Audio Codec, ALAC) is an audio codec developed by Apple Inc. for lossless data compression of digital music.

(This description is partly based on or reuses content from the Wikipedia article "Apple Lossless" (http://en.wikipedia.org/wiki/Apple_Lossless) and is licensed under the GNU Free Documentation License (http://www.gnu.org/copyleft/fdl.html).)</rdfs:comment>
    <skos:inScheme rdf:resource="http://www.ebusiness-unibw.org/ontologies/consumerelectronics/v1#DataFormatAudio"/>
  </skos:Concept>
  <skos:Concept rdf:about="http://www.ebusiness-unibw.org/ontologies/consumerelectronics/v1#AAC-LC">
    <rdfs:label xml:lang="en">AAC-LC</rdfs:label>
    <rdfs:comment xml:lang="en">Advanced Audio Coding (AAC) is a standardized, lossy compression and encoding scheme for digital audio.

(This description is partly based on or reuses content from the Wikipedia article "Advanced Audio Coding" (http://en.wikipedia.org/wiki/Advanced_Audio_Coding) and is licensed under the GNU Free Documentation License (http://www.gnu.org/copyleft/fdl.html).)</rdfs:comment>
    <skos:inScheme rdf:resource="http://www.ebusiness-unibw.org/ontologies/consumerelectronics/v1#DataFormatAudio"/>
  </skos:Concept>
  <skos:Concept rdf:about="http://www.ebusiness-unibw.org/ontologies/consumerelectronics/v1#DolbyDigital">
    <rdfs:label xml:lang="en">DolbyDigital</rdfs:label>
    <rdfs:comment xml:lang="en">The marketing name for a series of lossy audio compression technologies developed by Dolby Laboratories.

(This description is partly based on or reuses content from the Wikipedia article "Dolby Digital" (http://en.wikipedia.org/wiki/Dolby_Digital) and is licensed under the GNU Free Documentation License (http://www.gnu.org/copyleft/fdl.html).)</rdfs:comment>
    <skos:inScheme rdf:resource="http://www.ebusiness-unibw.org/ontologies/consumerelectronics/v1#DataFormatAudio"/>
  </skos:Concept>
  <skos:Concept rdf:about="http://www.ebusiness-unibw.org/ontologies/consumerelectronics/v1#MP3">
    <rdfs:label xml:lang="en">MP3</rdfs:label>
    <rdfs:comment xml:lang="en">A digital audio encoding format using a form of lossy data compression.</rdfs:comment>
    <skos:inScheme rdf:resource="http://www.ebusiness-unibw.org/ontologies/consumerelectronics/v1#DataFormatAudio"/>
  </skos:Concept>
  <skos:Concept rdf:about="http://www.ebusiness-unibw.org/ontologies/consumerelectronics/v1#FLAC">
    <rdfs:label xml:lang="en">FLAC</rdfs:label>
    <rdfs:comment xml:lang="en">Free Lossless Audio Codec (FLAC) is a file format for lossless audio data compression.

(This description is partly based on or reuses content from the Wikipedia article "Free Lossless Audio Codec" (http://en.wikipedia.org/wiki/Free_Lossless_Audio_Codec) and is licensed under the GNU Free Documentation License (http://www.gnu.org/copyleft/fdl.html).)</rdfs:comment>
    <skos:inScheme rdf:resource="http://www.ebusiness-unibw.org/ontologies/consumerelectronics/v1#DataFormatAudio"/>
  </skos:Concept>
  <skos:Concept rdf:about="http://www.ebusiness-unibw.org/ontologies/consumerelectronics/v1#OGG">
    <rdfs:label xml:lang="en">OGG</rdfs:label>
    <rdfs:comment xml:lang="en">Ogg is a free, open standard container format maintained by the Xiph.Org Foundation.</rdfs:comment>
    <skos:inScheme rdf:resource="http://www.ebusiness-unibw.org/ontologies/consumerelectronics/v1#DataFormatAudio"/>
  </skos:Concept>
  <skos:Concept rdf:about="http://www.ebusiness-unibw.org/ontologies/consumerelectronics/v1#ASF">
    <rdfs:label xml:lang="en">ASF</rdfs:label>
    <rdfs:comment xml:lang="en">Advanced Systems Format (formerly Advanced Streaming Format, Active Streaming Format) is Microsoft's proprietary digital audio/digital video container format, especially meant for streaming media. ASF is part of the Windows Media framework.

(This description is partly based on or reuses content from the Wikipedia article "Advanced Systems Format" (http://en.wikipedia.org/wiki/Advanced_Systems_Format) and is licensed under the GNU Free Documentation License (http://www.gnu.org/copyleft/fdl.html).)</rdfs:comment>
    <skos:inScheme rdf:resource="http://www.ebusiness-unibw.org/ontologies/consumerelectronics/v1#DataFormatAudio"/>
  </skos:Concept>
</rdf:RDF>
