<rdf:RDF
    xmlns:dct="http://purl.org/dc/terms/"
    xmlns:rdf="http://www.w3.org/1999/02/22-rdf-syntax-ns#"
    xmlns:dc="http://purl.org/dc/elements/1.1/"
    xmlns:owl="http://www.w3.org/2002/07/owl#"
    xmlns:dcmit="http://purl.org/dc/dcmitype/"
    xmlns:skos="http://www.w3.org/2004/02/skos/core#"
    xmlns:voaf="http://purl.org/vocommons/voaf#"
    xmlns:rdfs="http://www.w3.org/2000/01/rdf-schema#"
    xmlns:vann="http://purl.org/vocab/vann/">
  <owl:ObjectProperty rdf:about="http://www.ebusiness-unibw.org/ontologies/consumerelectronics/v1#hasConnectivity">
    <rdfs:comment xml:lang="en">Defines the possibilities to connect different kinds of electronical devices.</rdfs:comment>
    <rdfs:label xml:lang="en">connectivity</rdfs:label>
    <rdfs:range>
      <skos:ConceptScheme rdf:about="http://www.ebusiness-unibw.org/ontologies/consumerelectronics/v1#Connectivity"/>
    </rdfs:range>
  </owl:ObjectProperty>
  <skos:Concept rdf:about="http://www.ebusiness-unibw.org/ontologies/consumerelectronics/v1#RS-232">
    <rdfs:label xml:lang="en">RS-232</rdfs:label>
    <rdfs:comment xml:lang="en">In telecommunications, RS-232 (Recommended Standard 232) is a standard for serial binary data signals connecting between a DTE (Data Terminal Equipment) and a DCE (Data Circuit-terminating Equipment). It is commonly used in computer serial ports.

(This description is partly based on or reuses content from the Wikipedia article "RS-232" (http://en.wikipedia.org/wiki/RS-232) and is licensed under the GNU Free Documentation License (http://www.gnu.org/copyleft/fdl.html).)</rdfs:comment>
    <skos:inScheme rdf:resource="http://www.ebusiness-unibw.org/ontologies/consumerelectronics/v1#Connectivity"/>
  </skos:Concept>
  <skos:Concept rdf:about="http://www.ebusiness-unibw.org/ontologies/consumerelectronics/v1#PCIn">
    <rdfs:label xml:lang="en">PC in</rdfs:label>
    <rdfs:comment xml:lang="en">Port to connect a PC with the electronical device.</rdfs:comment>
    <skos:inScheme rdf:resource="http://www.ebusiness-unibw.org/ontologies/consumerelectronics/v1#Connectivity"/>
  </skos:Concept>
  <skos:Concept rdf:about="http://www.ebusiness-unibw.org/ontologies/consumerelectronics/v1#RGB">
    <rdfs:label xml:lang="en">RGB</rdfs:label>
    <rdfs:comment xml:lang="en">The RGB color model is an additive color model in which red, green, and blue light are added together in various ways to reproduce a broad array of colors. The name of the model comes from the initials of the three additive primary colors, red, green, and blue. Typical RGB input devices are color TV and video cameras, image scanners, and digital cameras. Typical RGB output devices are TV sets of various technologies (CRT, LCD, plasma, etc.), computer and mobile phone displays, video projectors, multicolor LED displays, and large screens as JumboTron, etc. Color printers, on the other hand, are usually not RGB devices, but subtractive color devices (typically CMYK color model).

(This description is partly based on or reuses content from the Wikipedia article "RGB" (http://en.wikipedia.org/wiki/RGB) and is licensed under the GNU Free Documentation License (http://www.gnu.org/copyleft/fdl.html).)</rdfs:comment>
    <skos:inScheme rdf:resource="http://www.ebusiness-unibw.org/ontologies/consumerelectronics/v1#Connectivity"/>
  </skos:Concept>
  <skos:Concept rdf:about="http://www.ebusiness-unibw.org/ontologies/consumerelectronics/v1#RF">
    <rdfs:label xml:lang="en">RF</rdfs:label>
    <rdfs:comment xml:lang="en">An RF connector is an electrical connector designed to work at radio frequencies in the multi-megahertz range. RF connectors are typically used with coaxial cables and are designed to maintain the shielding that the coaxial design offers. Better models also minimize the change in transmission line impedance at the connection. Mechanically they provide a fastening mechanism (thread, bayonet, braces, push pull) and springs for a low ohmic electric contact while sparing the gold surface thus allowing above 1000 reconnects and reducing the insertion force. Research activity in the area of radio-frequency (RF) circuit design has surged in the last decade in direct response to the enormous market demand for inexpensive, high data rate wireless transceivers.

(This description is partly based on or reuses content from the Wikipedia article "RF connector" (http://en.wikipedia.org/wiki/RF_connector) and is licensed under the GNU Free Documentation License (http://www.gnu.org/copyleft/fdl.html).)</rdfs:comment>
    <skos:inScheme rdf:resource="http://www.ebusiness-unibw.org/ontologies/consumerelectronics/v1#Connectivity"/>
  </skos:Concept>
  <skos:Concept rdf:about="http://www.ebusiness-unibw.org/ontologies/consumerelectronics/v1#HeadphoneLineOut_2.5mm">
    <rdfs:label xml:lang="en">Headphone line out 2.5mm</rdfs:label>
    <rdfs:comment xml:lang="en">Port to connect headphones with an electronical device. Here the port has the diameter of 2,5 millimetres.</rdfs:comment>
    <skos:inScheme rdf:resource="http://www.ebusiness-unibw.org/ontologies/consumerelectronics/v1#Connectivity"/>
  </skos:Concept>
  <skos:Concept rdf:about="http://www.ebusiness-unibw.org/ontologies/consumerelectronics/v1#DigitalAudioOpticalOut">
    <rdfs:label xml:lang="en">Digital audio optical out</rdfs:label>
    <rdfs:comment xml:lang="en">Digital audio uses digital signals for sound reproduction. This includes analog-to-digital conversion, digital-to-analog conversion, storage, and transmission. TOSLINK or Optical Cable is a standardized optical fiber connection system.

(This description is partly based on or reuses content from the Wikipedia article "Digital audio" (http://en.wikipedia.org/wiki/Digital_audio) and is licensed under the GNU Free Documentation License (http://www.gnu.org/copyleft/fdl.html).)</rdfs:comment>
    <skos:inScheme rdf:resource="http://www.ebusiness-unibw.org/ontologies/consumerelectronics/v1#Connectivity"/>
  </skos:Concept>
  <skos:Concept rdf:about="http://www.ebusiness-unibw.org/ontologies/consumerelectronics/v1#PCMCIA">
    <rdfs:label xml:lang="en">PCMCIA</rdfs:label>
    <rdfs:comment xml:lang="en">The Personal Computer Memory Card International Association is an international standards body that defines and promotes the PC Card (formerly known as "PCMCIA card") and ExpressCard standards. Although the organization's name refers to memory cards, their standards are not limited to memory devices. These cards can be used for wireless connectivity, modem and other functions in laptop/notebook PCs that may be lacking them natively.

(This description is partly based on or reuses content from the Wikipedia article "PCMCIA" (http://en.wikipedia.org/wiki/PCMCIA) and is licensed under the GNU Free Documentation License (http://www.gnu.org/copyleft/fdl.html).)</rdfs:comment>
    <skos:inScheme rdf:resource="http://www.ebusiness-unibw.org/ontologies/consumerelectronics/v1#Connectivity"/>
  </skos:Concept>
  <skos:Concept rdf:about="http://www.ebusiness-unibw.org/ontologies/consumerelectronics/v1#DLNA_Ethernet">
    <rdfs:label xml:lang="en">DLNA Ethernet</rdfs:label>
    <rdfs:comment xml:lang="en">The Digital Living Network Alliance is an international, cross-industry collaboration of consumer electronics, computing industry and mobile device companies. Members of DLNA develop a concept of wired and wireless interoperable networks where digital content such as photos, music, and videos can be shared through consumer electronics (CE), personal computers (PCs), and mobile devices in and beyond the home.

(This description is partly based on or reuses content from the Wikipedia article "Digital Living Network Alliance" (http://en.wikipedia.org/wiki/Digital_Living_Network_Alliance) and is licensed under the GNU Free Documentation License (http://www.gnu.org/copyleft/fdl.html).)</rdfs:comment>
    <skos:inScheme rdf:resource="http://www.ebusiness-unibw.org/ontologies/consumerelectronics/v1#Connectivity"/>
  </skos:Concept>
  <skos:Concept rdf:about="http://www.ebusiness-unibw.org/ontologies/consumerelectronics/v1#CompositeVideoIn">
    <rdfs:label xml:lang="en">Composite video in</rdfs:label>
    <rdfs:comment xml:lang="en">Composite video is the format of an analog television (picture only) signal before it is combined with a sound signal and modulated onto an RF carrier. It is usually in a standard format such as NTSC, PAL, or SECAM. It is a composite of three source signals called Y, U and V (together referred to as YUV) with sync pulses. Here the input is meant.

(This description is partly based on or reuses content from the Wikipedia article "Composite video" (http://en.wikipedia.org/wiki/Composite_video) and is licensed under the GNU Free Documentation License (http://www.gnu.org/copyleft/fdl.html).)</rdfs:comment>
    <skos:inScheme rdf:resource="http://www.ebusiness-unibw.org/ontologies/consumerelectronics/v1#Connectivity"/>
  </skos:Concept>
  <skos:Concept rdf:about="http://www.ebusiness-unibw.org/ontologies/consumerelectronics/v1#DVI">
    <rdfs:label xml:lang="en">DVI</rdfs:label>
    <rdfs:comment xml:lang="en">The Digital Visual Interface (DVI) is a video interface standard designed to maximize the visual quality of digital display devices such as flat panel LCD computer displays and digital projectors. It is designed for carrying uncompressed digital video data to a display. It is partially compatible with the High-Definition Multimedia Interface (HDMI) standard in digital mode (DVI-D), and VGA in analog mode (DVI-A).

(This description is partly based on or reuses content from the Wikipedia article "Digital Visual Interface" (http://en.wikipedia.org/wiki/Digital_Visual_Interface) and is licensed under the GNU Free Documentation License (http://www.gnu.org/copyleft/fdl.html).)</rdfs:comment>
    <skos:inScheme rdf:resource="http://www.ebusiness-unibw.org/ontologies/consumerelectronics/v1#Connectivity"/>
  </skos:Concept>
  <skos:Concept rdf:about="http://www.ebusiness-unibw.org/ontologies/consumerelectronics/v1#ComponentVideoIn">
    <rdfs:label xml:lang="en">Component video in</rdfs:label>
    <rdfs:comment xml:lang="en">Component video is a video signal that has been split into two or more components. In popular use, it refers to a type of analog video information that is transmitted or stored as three separate signals. Component video can be contrasted with composite video (NTSC, PAL or SECAM) in which all the video information is combined into a single line-level signal. Like composite, component video cables do not carry audio and are often paired with audio cables. Here the input is meant.

(This description is partly based on or reuses content from the Wikipedia article "Component video" (http://en.wikipedia.org/wiki/Component_video) and is licensed under the GNU Free Documentation License (http://www.gnu.org/copyleft/fdl.html).)</rdfs:comment>
    <skos:inScheme rdf:resource="http://www.ebusiness-unibw.org/ontologies/consumerelectronics/v1#Connectivity"/>
  </skos:Concept>
  <skos:Concept rdf:about="http://www.ebusiness-unibw.org/ontologies/consumerelectronics/v1#YPbPr">
    <rdfs:label xml:lang="en">YPbPr</rdfs:label>
    <rdfs:comment xml:lang="en">YPbPR is the analog video signal carried by component video cable in consumer electronics. The green cable carries Y, the blue cable carries PB and the red cable carries PR.

(This description is partly based on or reuses content from the Wikipedia article "YPbPr" (http://en.wikipedia.org/wiki/YPbPr) and is licensed under the GNU Free Documentation License (http://www.gnu.org/copyleft/fdl.html).)</rdfs:comment>
    <skos:inScheme rdf:resource="http://www.ebusiness-unibw.org/ontologies/consumerelectronics/v1#Connectivity"/>
  </skos:Concept>
  <skos:Concept rdf:about="http://www.ebusiness-unibw.org/ontologies/consumerelectronics/v1#CVBS_in">
    <rdfs:label xml:lang="en">CVBS in</rdfs:label>
    <rdfs:comment xml:lang="en">Composite video is often designated by the CVBS acronym, meaning any of "Color, Video, Blank and Sync", "Composite Video Baseband Signal", "Composite Video Burst Signal", or "Composite Video with Burst and Sync". Here the input is meant.</rdfs:comment>
    <skos:inScheme rdf:resource="http://www.ebusiness-unibw.org/ontologies/consumerelectronics/v1#Connectivity"/>
  </skos:Concept>
  <skos:Concept rdf:about="http://www.ebusiness-unibw.org/ontologies/consumerelectronics/v1#TRSConnector">
    <rdfs:label xml:lang="en">TRS connector</rdfs:label>
    <rdfs:comment xml:lang="en">A TRS connector (tip, ring, sleeve) also called an audio jack, phone plug, jack plug, stereo plug, mini-jack, or mini-stereo, is a common audio connector. It is cylindrical in shape, typically with three contacts, although sometimes with two (a TS connector) or four (a TRRS connector).

(This description is partly based on or reuses content from the Wikipedia article "TRS connector" (http://en.wikipedia.org/wiki/TRS_connector) and is licensed under the GNU Free Documentation License (http://www.gnu.org/copyleft/fdl.html).)</rdfs:comment>
    <skos:inScheme rdf:resource="http://www.ebusiness-unibw.org/ontologies/consumerelectronics/v1#Connectivity"/>
  </skos:Concept>
  <skos:Concept rdf:about="http://www.ebusiness-unibw.org/ontologies/consumerelectronics/v1#SubwooferOut">
    <rdfs:label xml:lang="en">Subwoofer out</rdfs:label>
    <rdfs:comment xml:lang="en">A connection port for a subwoover. Subwoofer is a woofer, or a complete loudspeaker dedicated to the reproduction of bass audio frequencies, from perhaps 150 Hz down as far as 20 Hz, or in rare cases lower.

(This description is partly based on or reuses content from the Wikipedia article "Subwoofer" (http://en.wikipedia.org/wiki/Subwoofer) and is licensed under the GNU Free Documentation License (http://www.gnu.org/copyleft/fdl.html).)</rdfs:comment>
    <skos:inScheme rdf:resource="http://www.ebusiness-unibw.org/ontologies/consumerelectronics/v1#Connectivity"/>
  </skos:Concept>
  <skos:Concept rdf:about="http://www.ebusiness-unibw.org/ontologies/consumerelectronics/v1#AV">
    <rdfs:label xml:lang="en">AV</rdfs:label>
    <rdfs:comment xml:lang="en">Audio connectors and video connectors are electrical connectors for carrying an audio signal or video signal, either in an analog or digital format. Analog A/V connectors often use shielded cable to inhibit RF interference and noise.

(This description is partly based on or reuses content from the Wikipedia article "Audio and video connector" (http://en.wikipedia.org/wiki/Audio_and_video_connector) and is licensed under the GNU Free Documentation License (http://www.gnu.org/copyleft/fdl.html).)</rdfs:comment>
    <skos:inScheme rdf:resource="http://www.ebusiness-unibw.org/ontologies/consumerelectronics/v1#Connectivity"/>
  </skos:Concept>
  <skos:Concept rdf:about="http://www.ebusiness-unibw.org/ontologies/consumerelectronics/v1#SCART">
    <rdfs:label xml:lang="en">SCART</rdfs:label>
    <rdfs:comment xml:lang="en">SCART (from Syndicat des Constructeurs d'Appareils Radiorécepteurs et Téléviseurs, Radio and Television Receiver Manufacturer's Association) is a French-originated standard and associated 21-pin connector for connecting audio-visual (AV) equipment together.

(This description is partly based on or reuses content from the Wikipedia article "SCART" (http://en.wikipedia.org/wiki/SCART) and is licensed under the GNU Free Documentation License (http://www.gnu.org/copyleft/fdl.html).)</rdfs:comment>
    <skos:inScheme rdf:resource="http://www.ebusiness-unibw.org/ontologies/consumerelectronics/v1#Connectivity"/>
  </skos:Concept>
  <skos:Concept rdf:about="http://www.ebusiness-unibw.org/ontologies/consumerelectronics/v1#DigitalAudioCoaxialOut">
    <rdfs:label xml:lang="en">Digital audio coaxial out</rdfs:label>
    <rdfs:comment xml:lang="en">Digital audio uses digital signals for sound reproduction. This includes analog-to-digital conversion, digital-to-analog conversion, storage and transmission. From the signal point of view, a connector can be viewed as a short, rigid cable. The connector usually has the same impedance as the related cable and probably has a similar cutoff frequency although its dielectric may be different. Some connectors are gold or rhodium plated, while some connectors use nickel or tin plating. Silver is also used due to its excellent conductivity. Although silver tends to oxidize rather quickly, the silver oxide that is produced is still conductive. This may pose a cosmetic issue but it does not degrade the performance of the connector. Here the output is meant.

(This description is partly based on or reuses content from the Wikipedia article "Digital audio" (http://en.wikipedia.org/wiki/Digital_audio) and is licensed under the GNU Free Documentation License (http://www.gnu.org/copyleft/fdl.html).)</rdfs:comment>
    <skos:inScheme rdf:resource="http://www.ebusiness-unibw.org/ontologies/consumerelectronics/v1#Connectivity"/>
  </skos:Concept>
  <skos:Concept rdf:about="http://www.ebusiness-unibw.org/ontologies/consumerelectronics/v1#HeadphoneLineOut_3.5mm">
    <rdfs:label xml:lang="en">Headphone line out 3,5 mm</rdfs:label>
    <rdfs:comment xml:lang="en">Port to connect headphones with an electronical device. Here the port has the diameter of 3,5 millimetres.</rdfs:comment>
    <skos:inScheme rdf:resource="http://www.ebusiness-unibw.org/ontologies/consumerelectronics/v1#Connectivity"/>
  </skos:Concept>
  <skos:Concept rdf:about="http://www.ebusiness-unibw.org/ontologies/consumerelectronics/v1#HDMI">
    <rdfs:label xml:lang="en">HDMI</rdfs:label>
    <rdfs:comment xml:lang="en">HDMI (High-Definition Multimedia Interface) is a compact audio/video interface for transmitting uncompressed digital data. It represents a digital alternative to consumer analog standards such as Radio Frequency (RF) coaxial cable, composite video, S-Video, SCART, component video, D-Terminal, and VGA. HDMI connects digital audio/video sources such as set-top boxes, Blu-ray Disc players, personal computers (PCs), video game consoles, and AV receivers to compatible digital audio devices, computer monitors, and digital televisions.

(This description is partly based on or reuses content from the Wikipedia article "HDMI" (http://en.wikipedia.org/wiki/HDMI) and is licensed under the GNU Free Documentation License (http://www.gnu.org/copyleft/fdl.html).)</rdfs:comment>
    <skos:inScheme rdf:resource="http://www.ebusiness-unibw.org/ontologies/consumerelectronics/v1#Connectivity"/>
  </skos:Concept>
  <skos:Concept rdf:about="http://www.ebusiness-unibw.org/ontologies/consumerelectronics/v1#CVBS_out">
    <rdfs:label xml:lang="en">CVBS out</rdfs:label>
    <rdfs:comment xml:lang="en">Composite video is often designated by the CVBS acronym, meaning any of "Color, Video, Blank and Sync", "Composite Video Baseband Signal", "Composite Video Burst Signal", or "Composite Video with Burst and Sync". Here the output is meant.</rdfs:comment>
    <skos:inScheme rdf:resource="http://www.ebusiness-unibw.org/ontologies/consumerelectronics/v1#Connectivity"/>
  </skos:Concept>
  <skos:Concept rdf:about="http://www.ebusiness-unibw.org/ontologies/consumerelectronics/v1#ComponentVideoOut">
    <rdfs:label xml:lang="en">Component video out</rdfs:label>
    <rdfs:comment xml:lang="en">Component video is a video signal that has been split into two or more components. In popular use, it refers to a type of analog video information that is transmitted or stored as three separate signals. Component video can be contrasted with composite video (NTSC, PAL or SECAM) in which all the video information is combined into a single line-level signal. Like composite, component video cables do not carry audio and are often paired with audio cables. Here the output is meant.

(This description is partly based on or reuses content from the Wikipedia article "Component video" (http://en.wikipedia.org/wiki/Component_video) and is licensed under the GNU Free Documentation License (http://www.gnu.org/copyleft/fdl.html).)</rdfs:comment>
    <skos:inScheme rdf:resource="http://www.ebusiness-unibw.org/ontologies/consumerelectronics/v1#Connectivity"/>
  </skos:Concept>
  <skos:Concept rdf:about="http://www.ebusiness-unibw.org/ontologies/consumerelectronics/v1#PCAudioIn">
    <rdfs:label xml:lang="en">PC Audio out</rdfs:label>
    <rdfs:comment xml:lang="en">Port to connect the audio cables for a PC with the electronical device.</rdfs:comment>
    <skos:inScheme rdf:resource="http://www.ebusiness-unibw.org/ontologies/consumerelectronics/v1#Connectivity"/>
  </skos:Concept>
</rdf:RDF>
