<rdf:RDF
    xmlns:dct="http://purl.org/dc/terms/"
    xmlns:rdf="http://www.w3.org/1999/02/22-rdf-syntax-ns#"
    xmlns:dc="http://purl.org/dc/elements/1.1/"
    xmlns:owl="http://www.w3.org/2002/07/owl#"
    xmlns:dcmit="http://purl.org/dc/dcmitype/"
    xmlns:skos="http://www.w3.org/2004/02/skos/core#"
    xmlns:voaf="http://purl.org/vocommons/voaf#"
    xmlns:rdfs="http://www.w3.org/2000/01/rdf-schema#"
    xmlns:vann="http://purl.org/vocab/vann/">
  <rdf:Description rdf:about="http://purl.org/ipo/core#hasPreCondition">
    <rdfs:comment xml:lang="en">Indicates a precondition for the Action be executed.

A precondition may represent a prerequisite for execution of the Action, without which it is not guaranteed correct execution.</rdfs:comment>
    <rdfs:label xml:lang="en">hasPreCondition</rdfs:label>
    <rdfs:domain rdf:resource="http://purl.org/ipo/core#Action"/>
    <rdfs:range>
      <skos:ConceptScheme rdf:about="http://purl.org/ipo/core#BooleanExpression"/>
    </rdfs:range>
  </rdf:Description>
  <skos:Concept rdf:about="http://purl.org/ipo/core#false">
    <skos:inScheme rdf:resource="http://purl.org/ipo/core#BooleanExpression"/>
  </skos:Concept>
  <skos:Concept rdf:about="http://purl.org/ipo/core#true">
    <skos:inScheme rdf:resource="http://purl.org/ipo/core#BooleanExpression"/>
  </skos:Concept>
  <rdf:Description rdf:about="http://purl.org/ipo/core#hasGuardCondition">
    <rdfs:comment xml:lang="en">Indicates a BooleanExpression for that a Transition occurs.
For example, a Transition can have as guardCondition that the Step of origin be executed 10 times. So while this Step does is not executes 10 times, will not be started the Step of destination. This example illustrates a repeating structure within the workflow.</rdfs:comment>
    <rdfs:label xml:lang="en">hasGuardCondition</rdfs:label>
    <rdfs:domain rdf:resource="http://purl.org/ipo/core#Transition"/>
    <rdfs:range rdf:resource="http://purl.org/ipo/core#BooleanExpression"/>
  </rdf:Description>
  <rdf:Description rdf:about="http://purl.org/ipo/core#hasPostCondition">
    <rdfs:comment xml:lang="en">Indicates a postcondition (effect) will be reached after executing the Action.</rdfs:comment>
    <rdfs:label xml:lang="en">hasPostCondition</rdfs:label>
    <rdfs:domain rdf:resource="http://purl.org/ipo/core#Action"/>
    <rdfs:range rdf:resource="http://purl.org/ipo/core#BooleanExpression"/>
  </rdf:Description>
</rdf:RDF>
