<rdf:RDF
    xmlns:dct="http://purl.org/dc/terms/"
    xmlns:rdf="http://www.w3.org/1999/02/22-rdf-syntax-ns#"
    xmlns:dc="http://purl.org/dc/elements/1.1/"
    xmlns:owl="http://www.w3.org/2002/07/owl#"
    xmlns:dcmit="http://purl.org/dc/dcmitype/"
    xmlns:skos="http://www.w3.org/2004/02/skos/core#"
    xmlns:voaf="http://purl.org/vocommons/voaf#"
    xmlns:rdfs="http://www.w3.org/2000/01/rdf-schema#"
    xmlns:vann="http://purl.org/vocab/vann/">
  <skos:Concept rdf:about="http://www.ebusiness-unibw.org/ontologies/consumerelectronics/v1#RoHS">
    <rdfs:label xml:lang="en">RoHS</rdfs:label>
    <rdfs:comment xml:lang="en">The Directive on the restriction of the use of certain hazardous substances in electrical and electronic equipment 2002/95/EC.

(This description is partly based on or reuses content from the Wikipedia article "ROHS" (http://en.wikipedia.org/wiki/ROHS) and is licensed under the GNU Free Documentation License (http://www.gnu.org/copyleft/fdl.html).)</rdfs:comment>
    <skos:inScheme>
      <skos:ConceptScheme rdf:about="http://www.ebusiness-unibw.org/ontologies/consumerelectronics/v1#Certificate"/>
    </skos:inScheme>
  </skos:Concept>
  <rdf:Description rdf:about="http://www.ebusiness-unibw.org/ontologies/consumerelectronics/v1#hasCertificate">
    <rdfs:comment xml:lang="en">Defines the type of certificate of a product used to attest quality standards.</rdfs:comment>
    <rdfs:label xml:lang="en">certificate</rdfs:label>
    <rdfs:range rdf:resource="http://www.ebusiness-unibw.org/ontologies/consumerelectronics/v1#Certificate"/>
  </rdf:Description>
  <skos:Concept rdf:about="http://www.ebusiness-unibw.org/ontologies/consumerelectronics/v1#CE_Mark">
    <rdfs:label xml:lang="en">CE Mark</rdfs:label>
    <rdfs:comment xml:lang="en">The CE marking (also known as CE mark) is a mandatory conformity mark on many products placed on the single market in the European Economic Area (EEA).

(This description is partly based on or reuses content from the Wikipedia article "CE mark" (http://en.wikipedia.org/wiki/CE_mark) and is licensed under the GNU Free Documentation License (http://www.gnu.org/copyleft/fdl.html).)</rdfs:comment>
    <skos:inScheme rdf:resource="http://www.ebusiness-unibw.org/ontologies/consumerelectronics/v1#Certificate"/>
  </skos:Concept>
</rdf:RDF>
