<rdf:RDF
    xmlns:dct="http://purl.org/dc/terms/"
    xmlns:rdf="http://www.w3.org/1999/02/22-rdf-syntax-ns#"
    xmlns:dc="http://purl.org/dc/elements/1.1/"
    xmlns:owl="http://www.w3.org/2002/07/owl#"
    xmlns:dcmit="http://purl.org/dc/dcmitype/"
    xmlns:skos="http://www.w3.org/2004/02/skos/core#"
    xmlns:voaf="http://purl.org/vocommons/voaf#"
    xmlns:rdfs="http://www.w3.org/2000/01/rdf-schema#"
    xmlns:vann="http://purl.org/vocab/vann/">
  <skos:Concept rdf:about="http://lod.taxonconcept.org/ontology/txn.owl#Sex_undetermined">
    <rdfs:label>Sex Undetermined</rdfs:label>
    <skos:inScheme>
      <skos:ConceptScheme rdf:about="http://lod.taxonconcept.org/ontology/txn.owl#Sex"/>
    </skos:inScheme>
  </skos:Concept>
  <skos:Concept rdf:about="http://lod.taxonconcept.org/ontology/txn.owl#Sex_male">
    <rdfs:label xml:lang="en">male</rdfs:label>
    <rdfs:comment xml:lang="en">Male (♂) refers to the sex of an organism, or part of an organism, which produces small mobile gametes, called spermatozoa.</rdfs:comment>
    <skos:inScheme rdf:resource="http://lod.taxonconcept.org/ontology/txn.owl#Sex"/>
  </skos:Concept>
  <skos:Concept rdf:about="http://lod.taxonconcept.org/ontology/txn.owl#Sex_unknowable">
    <rdfs:label>Sex Unknowable</rdfs:label>
    <skos:inScheme rdf:resource="http://lod.taxonconcept.org/ontology/txn.owl#Sex"/>
  </skos:Concept>
  <skos:Concept rdf:about="http://lod.taxonconcept.org/ontology/txn.owl#Sex_hermaphrodite">
    <rdfs:label xml:lang="en">hermaphrodite</rdfs:label>
    <rdfs:comment xml:lang="en">one organism having both male and female sexual characteristics and organs; at birth an unambiguous assignment of male or female cannot be made</rdfs:comment>
    <skos:inScheme rdf:resource="http://lod.taxonconcept.org/ontology/txn.owl#Sex"/>
  </skos:Concept>
  <skos:Concept rdf:about="http://lod.taxonconcept.org/ontology/txn.owl#Sex_female">
    <rdfs:label xml:lang="en">female</rdfs:label>
    <rdfs:comment xml:lang="en">Female (♀) is the sex of an organism, or a part of an organism, which produces mobile ova (egg cells).</rdfs:comment>
    <skos:inScheme rdf:resource="http://lod.taxonconcept.org/ontology/txn.owl#Sex"/>
  </skos:Concept>
</rdf:RDF>
