<rdf:RDF
    xmlns:dct="http://purl.org/dc/terms/"
    xmlns:rdf="http://www.w3.org/1999/02/22-rdf-syntax-ns#"
    xmlns:dc="http://purl.org/dc/elements/1.1/"
    xmlns:owl="http://www.w3.org/2002/07/owl#"
    xmlns:dcmit="http://purl.org/dc/dcmitype/"
    xmlns:skos="http://www.w3.org/2004/02/skos/core#"
    xmlns:voaf="http://purl.org/vocommons/voaf#"
    xmlns:rdfs="http://www.w3.org/2000/01/rdf-schema#"
    xmlns:vann="http://purl.org/vocab/vann/">
  <rdf:Description rdf:about="http://www.ebusiness-unibw.org/ontologies/consumerelectronics/v1#hasZoom">
    <rdfs:comment xml:lang="en">Zoom is a method of decreasing (narrowing) the apparent angle of view of a photographic or video image.

(This description is partly based on or reuses content from the Wikipedia article "Digital zoom" (http://en.wikipedia.org/wiki/Digital_zoom) and is licensed under the GNU Free Documentation License (http://www.gnu.org/copyleft/fdl.html).)</rdfs:comment>
    <rdfs:label xml:lang="en">zoom</rdfs:label>
    <rdfs:range>
      <skos:ConceptScheme rdf:about="http://www.ebusiness-unibw.org/ontologies/consumerelectronics/v1#Zoom"/>
    </rdfs:range>
  </rdf:Description>
  <skos:Concept rdf:about="http://www.ebusiness-unibw.org/ontologies/consumerelectronics/v1#ZoomOptical">
    <rdfs:label xml:lang="en">Zoom optical</rdfs:label>
    <rdfs:comment xml:lang="en">An optical zoom is a mechanical assembly of lens elements with the ability to vary its focal length (and thus angle of view), as opposed to a fixed focal length (FFL) lens (see prime lens).

(This description is partly based on or reuses content from the Wikipedia article "Zoom lens" (http://en.wikipedia.org/wiki/Zoom_lens) and is licensed under the GNU Free Documentation License (http://www.gnu.org/copyleft/fdl.html).)</rdfs:comment>
    <skos:inScheme rdf:resource="http://www.ebusiness-unibw.org/ontologies/consumerelectronics/v1#Zoom"/>
  </skos:Concept>
  <skos:Concept rdf:about="http://www.ebusiness-unibw.org/ontologies/consumerelectronics/v1#ZoomDigital">
    <rdfs:label xml:lang="en">Zoom digital</rdfs:label>
    <rdfs:comment xml:lang="en">Zoom is a method of decreasing (narrowing) the apparent angle of view of a photographic or video image.

(This description is partly based on or reuses content from the Wikipedia article "Digital zoom" (http://en.wikipedia.org/wiki/Digital_zoom) and is licensed under the GNU Free Documentation License (http://www.gnu.org/copyleft/fdl.html).)</rdfs:comment>
    <skos:inScheme rdf:resource="http://www.ebusiness-unibw.org/ontologies/consumerelectronics/v1#Zoom"/>
  </skos:Concept>
</rdf:RDF>
