<rdf:RDF
    xmlns:dct="http://purl.org/dc/terms/"
    xmlns:rdf="http://www.w3.org/1999/02/22-rdf-syntax-ns#"
    xmlns:dc="http://purl.org/dc/elements/1.1/"
    xmlns:owl="http://www.w3.org/2002/07/owl#"
    xmlns:dcmit="http://purl.org/dc/dcmitype/"
    xmlns:skos="http://www.w3.org/2004/02/skos/core#"
    xmlns:voaf="http://purl.org/vocommons/voaf#"
    xmlns:rdfs="http://www.w3.org/2000/01/rdf-schema#"
    xmlns:vann="http://purl.org/vocab/vann/">
  <owl:ObjectProperty rdf:about="http://www.ebusiness-unibw.org/ontologies/consumerelectronics/v1#hasProcessorType">
    <rdfs:comment xml:lang="en">The type of central processing unit (CPU) as an electronic circuit that can execute printing tasks or programs.</rdfs:comment>
    <rdfs:label xml:lang="en">processor type</rdfs:label>
    <rdfs:range>
      <skos:ConceptScheme rdf:about="http://www.ebusiness-unibw.org/ontologies/consumerelectronics/v1#ProcessorType"/>
    </rdfs:range>
  </owl:ObjectProperty>
  <skos:Concept rdf:about="http://www.ebusiness-unibw.org/ontologies/consumerelectronics/v1#G4_Class_Processor">
    <rdfs:label xml:lang="en">G4 Class Processor</rdfs:label>
    <rdfs:comment xml:lang="en">A designation used by Apple Computer to describe a fourth generation of 32-bit PowerPC microprocessors.

(This description is partly based on or reuses content from the Wikipedia article "PowerPC_G4" (http://en.wikipedia.org/wiki/PowerPC_G4) and is licensed under the GNU Free Documentation License (http://www.gnu.org/copyleft/fdl.html).)</rdfs:comment>
    <skos:inScheme rdf:resource="http://www.ebusiness-unibw.org/ontologies/consumerelectronics/v1#ProcessorType"/>
  </skos:Concept>
  <skos:Concept rdf:about="http://www.ebusiness-unibw.org/ontologies/consumerelectronics/v1#PowerPC_32_bit">
    <rdfs:label xml:lang="en">PowerPC 32 bit</rdfs:label>
    <rdfs:comment xml:lang="en">A RISC instruction set architecture created by the 1991 Apple-IBM-Motorola alliance, known as AIM. Originally intended for personal computers, PowerPC CPUs have since become popular embedded and high-performance processors.</rdfs:comment>
    <skos:inScheme rdf:resource="http://www.ebusiness-unibw.org/ontologies/consumerelectronics/v1#ProcessorType"/>
  </skos:Concept>
  <skos:Concept rdf:about="http://www.ebusiness-unibw.org/ontologies/consumerelectronics/v1#RISC">
    <rdfs:label xml:lang="en">RISC</rdfs:label>
    <rdfs:comment xml:lang="en">Reduced instruction set computing, represents a CPU design strategy emphasizing the insight that simplified instructions that "do less" may still provide for higher performance if this simplicity can be utilized to make instructions execute very quickly.</rdfs:comment>
    <skos:inScheme rdf:resource="http://www.ebusiness-unibw.org/ontologies/consumerelectronics/v1#ProcessorType"/>
  </skos:Concept>
</rdf:RDF>
