<rdf:RDF
    xmlns:dct="http://purl.org/dc/terms/"
    xmlns:rdf="http://www.w3.org/1999/02/22-rdf-syntax-ns#"
    xmlns:dc="http://purl.org/dc/elements/1.1/"
    xmlns:owl="http://www.w3.org/2002/07/owl#"
    xmlns:dcmit="http://purl.org/dc/dcmitype/"
    xmlns:skos="http://www.w3.org/2004/02/skos/core#"
    xmlns:voaf="http://purl.org/vocommons/voaf#"
    xmlns:rdfs="http://www.w3.org/2000/01/rdf-schema#"
    xmlns:vann="http://purl.org/vocab/vann/">
  <owl:ObjectProperty rdf:about="http://purl.org/ontology/mo/release_type">
    <rdfs:comment>
        Relates a musical manifestation to its release type (interview, spoken word, album, ...)
    </rdfs:comment>
    <rdfs:domain rdf:resource="http://purl.org/ontology/mo/MusicalManifestation"/>
    <rdfs:range>
      <skos:ConceptScheme rdf:about="http://purl.org/ontology/mo/ReleaseType"/>
    </rdfs:range>
  </owl:ObjectProperty>
  <skos:Concept rdf:about="http://purl.org/ontology/mo/audiobook">
    <rdfs:label>audio book</rdfs:label>
    <rdfs:comment>
        Book read by a narrator without music.
        This is a type of MusicalManifestation defined by the musical industry.
    </rdfs:comment>
    <skos:inScheme rdf:resource="http://purl.org/ontology/mo/ReleaseType"/>
  </skos:Concept>
  <skos:Concept rdf:about="http://purl.org/ontology/mo/live">
    <rdfs:label>live</rdfs:label>
    <rdfs:comment>
        A musical manifestation that was recorded live.
        This is a type of MusicalManifestation defined by the musical industry.</rdfs:comment>
    <skos:inScheme rdf:resource="http://purl.org/ontology/mo/ReleaseType"/>
  </skos:Concept>
  <skos:Concept rdf:about="http://purl.org/ontology/mo/interview">
    <rdfs:label>interview</rdfs:label>
    <rdfs:comment>
        Recording of the questioning of a person.
        This is a type of MusicalManifestation defined by the musical industry.
    </rdfs:comment>
    <skos:inScheme rdf:resource="http://purl.org/ontology/mo/ReleaseType"/>
  </skos:Concept>
  <skos:Concept rdf:about="http://purl.org/ontology/mo/spokenword">
    <rdfs:label>spoken word</rdfs:label>
    <rdfs:comment>
        Spoken word is a form of music or artistic performance in which lyrics, poetry, or stories are spoken rather than sung. 
        Spoken-word is often done with a musical background, but emphasis is kept on the speaker.
        This is a type of MusicalManifestation defined by the musical industry.
    </rdfs:comment>
    <skos:inScheme rdf:resource="http://purl.org/ontology/mo/ReleaseType"/>
  </skos:Concept>
  <skos:Concept rdf:about="http://purl.org/ontology/mo/album">
    <rdfs:label>album</rdfs:label>
    <rdfs:comment>
        One or more track issued together.
            This is a type of MusicalManifestation defined by the musical industry.
    </rdfs:comment>
    <skos:inScheme rdf:resource="http://purl.org/ontology/mo/ReleaseType"/>
  </skos:Concept>
  <skos:Concept rdf:about="http://purl.org/ontology/mo/soundtrack">
    <rdfs:label>soundtrack</rdfs:label>
    <rdfs:comment>
        Sound recording on a narrow strip of a motion picture film.
        This is a type of MusicalManifestation defined by the musical industry.
    </rdfs:comment>
    <skos:inScheme rdf:resource="http://purl.org/ontology/mo/ReleaseType"/>
  </skos:Concept>
  <skos:Concept rdf:about="http://purl.org/ontology/mo/ep">
    <rdfs:label>ep</rdfs:label>
    <rdfs:comment>
            An EP
    </rdfs:comment>
    <skos:inScheme rdf:resource="http://purl.org/ontology/mo/ReleaseType"/>
  </skos:Concept>
  <skos:Concept rdf:about="http://purl.org/ontology/mo/single">
    <rdfs:label>single</rdfs:label>
    <rdfs:comment>A single or record single is a type of release, typically a recording of two tracks. In most cases, the single is a song that is released separately from an album, but it can still appear on an album.</rdfs:comment>
    <skos:inScheme rdf:resource="http://purl.org/ontology/mo/ReleaseType"/>
  </skos:Concept>
  <skos:Concept rdf:about="http://purl.org/ontology/mo/compilation">
    <rdfs:label>compilation</rdfs:label>
    <rdfs:comment>
        Collection of previously released manifestations of a musical expression by one or more artists.
        This is a type of MusicalManifestation defined by the musical industry.
    </rdfs:comment>
    <skos:inScheme rdf:resource="http://purl.org/ontology/mo/ReleaseType"/>
  </skos:Concept>
  <skos:Concept rdf:about="http://purl.org/ontology/mo/remix">
    <rdfs:label>remix</rdfs:label>
    <rdfs:comment>
        Musical manifestation that primarily contains remixed material. 
        This is a type of MusicalManifestation defined by the musical industry.
    </rdfs:comment>
    <skos:inScheme rdf:resource="http://purl.org/ontology/mo/ReleaseType"/>
  </skos:Concept>
</rdf:RDF>
