<rdf:RDF
    xmlns:dct="http://purl.org/dc/terms/"
    xmlns:rdf="http://www.w3.org/1999/02/22-rdf-syntax-ns#"
    xmlns:dc="http://purl.org/dc/elements/1.1/"
    xmlns:owl="http://www.w3.org/2002/07/owl#"
    xmlns:dcmit="http://purl.org/dc/dcmitype/"
    xmlns:skos="http://www.w3.org/2004/02/skos/core#"
    xmlns:voaf="http://purl.org/vocommons/voaf#"
    xmlns:rdfs="http://www.w3.org/2000/01/rdf-schema#"
    xmlns:vann="http://purl.org/vocab/vann/">
  <owl:ObjectProperty rdf:about="http://purl.org/ontology/mo/release_status">
    <rdfs:comment>
                Relates a musical manifestation to its release status (bootleg, ...)
        </rdfs:comment>
    <rdfs:domain rdf:resource="http://purl.org/ontology/mo/MusicalManifestation"/>
    <rdfs:range>
      <skos:ConceptScheme rdf:about="http://purl.org/ontology/mo/ReleaseStatus"/>
    </rdfs:range>
  </owl:ObjectProperty>
  <skos:Concept rdf:about="http://purl.org/ontology/mo/official">
    <rdfs:label>official</rdfs:label>
    <rdfs:comment>Any musical work or the expression of a musical work officially sanctioned by the artist and/or their corporate body.</rdfs:comment>
    <skos:inScheme rdf:resource="http://purl.org/ontology/mo/ReleaseStatus"/>
  </skos:Concept>
  <skos:Concept rdf:about="http://purl.org/ontology/mo/bootleg">
    <rdfs:label>bootleg</rdfs:label>
    <rdfs:comment>An unofficial/underground musical work or the expression of a musical work that was not sanctioned by the artist and/or the corporate body. </rdfs:comment>
    <skos:inScheme rdf:resource="http://purl.org/ontology/mo/ReleaseStatus"/>
  </skos:Concept>
  <skos:Concept rdf:about="http://purl.org/ontology/mo/promotion">
    <rdfs:label>promotion</rdfs:label>
    <rdfs:comment>A giveaway musical work or the expression of a musical work intended to promote an upcoming official musical work or the expression of a musical work.</rdfs:comment>
    <skos:inScheme rdf:resource="http://purl.org/ontology/mo/ReleaseStatus"/>
  </skos:Concept>
</rdf:RDF>
